
<http://sw.cyc.com/2006/07/27/cyc/091401hj_htmMt> <http://www.w3.org/2000/01/rdf-schema#comment> """Source microtheory holding some of the information content of the
web site http://www.fbi.gov/pressrel/pressrel01/091401hj.htm.""" ;
	<http://sw.cyc.com/2006/07/27/cyc/genlMt> <http://sw.cyc.com/2006/07/27/cyc/AnalystDatabaseMt> , <http://sw.cyc.com/2006/07/27/cyc/SAICCounterTDBCollectorMt> , <http://sw.cyc.com/2006/07/27/cyc/SAICTerrorismEventsDataMt> , <http://sw.cyc.com/2006/07/27/cyc/SAICBioTerrorismEventsDataMt> , <http://sw.cyc.com/2006/07/27/cyc/PatternsOfGlobalTerrorism1998Mt> , <http://sw.cyc.com/2006/07/27/cyc/PatternsOfGlobalTerrorism1997Mt> , <http://sw.cyc.com/2006/07/27/cyc/LDSCGeneralCollectorMt> , <http://sw.cyc.com/2006/07/27/cyc/SAICTerroristGroupsDataMt> , <http://sw.cyc.com/2006/07/27/cyc/TerrorismTacticsMt> , <http://sw.cyc.com/2006/07/27/cyc/LDSCExperimentalTermsMt> , <http://sw.cyc.com/2006/07/27/cyc/MIPTDatabase19681997-TermsMt> , <http://sw.cyc.com/2006/07/27/cyc/MIPTDatabase19982002-TermsMt> , <http://sw.cyc.com/2006/07/27/cyc/SAICAlQaidaDataMt> , <http://sw.cyc.com/2006/07/27/cyc/BaseKB> , <http://sw.cyc.com/2006/07/27/cyc/LDSCDemonstrationSpindleHeadMt> , <http://sw.cyc.com/2006/07/27/cyc/MIPT-TerroristEventsMt> ;
	a <http://sw.cyc.com/2006/07/27/cyc/SourceMicrotheory> , <http://sw.cyc.com/2006/07/27/cyc/PropositionalInformationThing> , <http://sw.cyc.com/2006/07/27/cyc/DataMicrotheory> ;
	<http://sw.cyc.com/2006/07/27/cyc/prettyString-Canonical> "FBI List of Hijackers -Web Source" .

<http://sw.cyc.com/2006/07/27/cyc/genlMt> <http://www.w3.org/2000/01/rdf-schema#comment> "A reflexive and transitive #$BinaryPredicate that relates a #$Microtheory to a #$Microtheory.  <code>(#$genlMt SPEC-MT GENL-MT)</code> means that <code>SPEC-MT</code> is a specialization or extension of <code>GENL-MT</code>.  (Note that it need not be a <i>proper</i> specialization or extension.)  In particular, this entails that everything that is true in <code>GENL-MT</code> is also true in <code>SPEC-MT</code>.  This relation is sometimes expressed informally by saying that <code>SPEC-MT</code> \"sees\" <code>GENL-MT</code>." ;
	a <http://www.w3.org/2002/07/owl#TransitiveProperty> , <http://sw.cyc.com/2006/07/27/cyc/MicrotheoryRelatingPredicate> , <http://sw.cyc.com/2006/07/27/cyc/AntiSymmetricBinaryPredicate> , <http://sw.cyc.com/2006/07/27/cyc/ReflexiveBinaryPredicate> , <http://sw.cyc.com/2006/07/27/cyc/DefaultMonotonicPredicate> , <http://sw.cyc.com/2006/07/27/cyc/RuleMacroPredicate> , <http://sw.cyc.com/2006/07/27/cyc/MicrotheoryPredicate> , <http://sw.cyc.com/2006/07/27/cyc/Predicate> , <http://sw.cyc.com/2006/07/27/cyc/Mt-Topic> , <http://sw.cyc.com/2006/07/27/cyc/BaseKBPredicate> , <http://sw.cyc.com/2006/07/27/cyc/MtExpansion-Topic> , <http://sw.cyc.com/2006/07/27/cyc/VocabularyForStatingRelationshipsBetweenMicrotheories-MtExpansion-Topic> , <http://sw.cyc.com/2006/07/27/cyc/HLPredicate> ;
	<http://sw.cyc.com/2006/07/27/cyc/prettyString-Canonical> "Genl Mt" ;
	<http://sw.cyc.com/2006/07/27/cyc/quotedIsa> <http://sw.cyc.com/2006/07/27/cyc/OpenCycDefinitionalPredicate> ;
	<http://www.w3.org/2000/01/rdf-schema#domain> <http://sw.cyc.com/2006/07/27/cyc/Microtheory> ;
	<http://sw.cyc.com/2006/07/27/cyc/arity> "2"^^<http://www.w3.org/2001/XMLSchema#long> ;
	<http://www.w3.org/2000/01/rdf-schema#range> <http://sw.cyc.com/2006/07/27/cyc/Microtheory> ;
	<http://www.w3.org/2000/01/rdf-schema#subPropertyOf> <http://sw.cyc.com/2006/07/27/cyc/generalizations> , <http://sw.cyc.com/2006/07/27/cyc/genlMt-WOFT> ;
	<http://sw.cyc.com/2006/07/27/cyc/arg1Format> <http://sw.cyc.com/2006/07/27/cyc/SetTheFormat> ;
	<http://sw.cyc.com/2006/07/27/cyc/arg2Format> <http://sw.cyc.com/2006/07/27/cyc/SetTheFormat> ;
	<http://sw.cyc.com/2006/07/27/cyc/oldConstantName> "baseMt" ;
	<http://sw.cyc.com/2006/07/27/cyc/typedGenlPreds> <http://sw.cyc.com/2006/07/27/cyc/generalizations> ;
	<http://sw.cyc.com/2006/07/27/cyc/predicateConventionMt> <http://sw.cyc.com/2006/07/27/cyc/UniversalVocabularyMt> ;
	<http://sw.cyc.com/2006/07/27/cyc/fanOutArg> "1"^^<http://www.w3.org/2001/XMLSchema#long> .

<http://sw.cyc.com/2006/07/27/cyc/AnalystDatabaseMt> <http://www.w3.org/2000/01/rdf-schema#comment> "This microtheory contains currently true assertions about users of the CAE and their workflow." ;
	<http://sw.cyc.com/2006/07/27/cyc/genlMt> <http://sw.cyc.com/2006/07/27/cyc/SAICCounterTDBCollectorMt> , <http://sw.cyc.com/2006/07/27/cyc/SAICTerrorismEventsDataMt> , <http://sw.cyc.com/2006/07/27/cyc/SAICBioTerrorismEventsDataMt> , <http://sw.cyc.com/2006/07/27/cyc/PatternsOfGlobalTerrorism1998Mt> , <http://sw.cyc.com/2006/07/27/cyc/PatternsOfGlobalTerrorism1997Mt> , <http://sw.cyc.com/2006/07/27/cyc/LDSCGeneralCollectorMt> , <http://sw.cyc.com/2006/07/27/cyc/SAICTerroristGroupsDataMt> , <http://sw.cyc.com/2006/07/27/cyc/TerrorismTacticsMt> , <http://sw.cyc.com/2006/07/27/cyc/LDSCExperimentalTermsMt> , <http://sw.cyc.com/2006/07/27/cyc/MIPTDatabase19681997-TermsMt> , <http://sw.cyc.com/2006/07/27/cyc/MIPTDatabase19982002-TermsMt> , <http://sw.cyc.com/2006/07/27/cyc/SAICAlQaidaDataMt> , <http://sw.cyc.com/2006/07/27/cyc/BaseKB> , <http://sw.cyc.com/2006/07/27/cyc/LDSCDemonstrationSpindleHeadMt> , <http://sw.cyc.com/2006/07/27/cyc/MIPT-TerroristEventsMt> , <http://sw.cyc.com/2006/07/27/cyc/ABSSimulatorActivityMt> , <http://sw.cyc.com/2006/07/27/cyc/AllPeopleAreHumanMt> , <http://sw.cyc.com/2006/07/27/cyc/WeaponsOfMassDestructionTacticsMt> , <http://sw.cyc.com/2006/07/27/cyc/TerrorismInTheMiddleEastFactsheetMt> , <http://sw.cyc.com/2006/07/27/cyc/IranGovernmentOrganizationDataMt> , <http://sw.cyc.com/2006/07/27/cyc/CIAWorldFactbook1996Mt> , <http://sw.cyc.com/2006/07/27/cyc/CIAWorldFactbook1994Mt> , <http://sw.cyc.com/2006/07/27/cyc/KEInteractionResourceTestMt> , <http://sw.cyc.com/2006/07/27/cyc/PathModelDeonticReasoningMt> , <http://sw.cyc.com/2006/07/27/cyc/IAMissionObligationVocabMt> , <http://sw.cyc.com/2006/07/27/cyc/CIAWorldFactbook1997Mt> , <http://sw.cyc.com/2006/07/27/cyc/RecentEventsMt> .

<http://sw.cyc.com/2006/07/27/cyc/105MMRifledBoreCannon> <http://sw.cyc.com/2006/07/27/cyc/prettyString> "105 mm rifled bore gun" , "105 mm rifled bore guns" , "105 millimeter rifled bore gun" , "105 millimeter rifled bore guns" , "105 millimeter rifled gun" , "105 millimeter rifled guns" , "105 mm rifled bore cannons" ;
	<http://www.w3.org/2000/01/rdf-schema#subClassOf> <http://sw.cyc.com/2006/07/27/cyc/TankCannon> , <http://sw.cyc.com/2006/07/27/cyc/RifledBoreWeapon> .

<http://sw.cyc.com/2006/07/27/cyc/TankCannon> <http://www.w3.org/2000/01/rdf-schema#comment> """The #$TankCannon has a large-caliber (usually over 75mm) and fires
rounds at a high velocity and with a low trajectory.  The #$TankCannon is the
main weapon on tanks.""" ;
	a <http://sw.cyc.com/2006/07/27/cyc/ExistingObjectType> , <http://sw.cyc.com/2006/07/27/cyc/KEClarifyingCollectionType> , <http://sw.cyc.com/2006/07/27/cyc/MilitaryWeaponType> ;
	<http://sw.cyc.com/2006/07/27/cyc/prettyString-Canonical> "tank cannon" ;
	<http://sw.cyc.com/2006/07/27/cyc/prettyString> "tank gun" , "tank guns" , "tank cannons" ;
	<http://www.w3.org/2000/01/rdf-schema#subClassOf> <http://sw.cyc.com/2006/07/27/cyc/Cannon> , <http://sw.cyc.com/2006/07/27/cyc/ProjectileLauncher-Direct> .

<http://sw.cyc.com/2006/07/27/cyc/RifledBoreWeapon> <http://www.w3.org/2000/01/rdf-schema#comment> "The collection of #$ProjectileLaunchers that have #$Bores with spiralled scoring.  Rifling the #$Bore increases the accuracy of the #$ProjectileWeapon." ;
	a <http://sw.cyc.com/2006/07/27/cyc/SpatiallyDisjointObjectType> , <http://sw.cyc.com/2006/07/27/cyc/KEClarifyingCollectionType> , <http://sw.cyc.com/2006/07/27/cyc/GunTypeByBarrelType> ;
	<http://sw.cyc.com/2006/07/27/cyc/prettyString-Canonical> "rifled bore weapon" ;
	<http://www.w3.org/2000/01/rdf-schema#subClassOf> <http://sw.cyc.com/2006/07/27/cyc/ProjectileLauncher> ;
	<http://www.w3.org/2002/07/owl#disjointWith> <http://sw.cyc.com/2006/07/27/cyc/SmoothBoreWeapon> .

<http://sw.cyc.com/2006/07/27/cyc/WeaponType> <http://www.w3.org/2000/01/rdf-schema#comment> "A #$SecondOrderCollection.  #$WeaponType is the collection of all specializations of #$Weapon." ;
	a <http://sw.cyc.com/2006/07/27/cyc/FacetingCollectionType> , <http://sw.cyc.com/2006/07/27/cyc/SecondOrderCollection> ;
	<http://sw.cyc.com/2006/07/27/cyc/prettyString-Canonical> "type of weapon" ;
	<http://sw.cyc.com/2006/07/27/cyc/prettyString> "types of weapon" ;
	<http://www.w3.org/2000/01/rdf-schema#subClassOf> <http://sw.cyc.com/2006/07/27/cyc/ArtifactTypeByGenericCategory> , <http://sw.cyc.com/2006/07/27/cyc/TemporalStuffType> , <http://sw.cyc.com/2006/07/27/cyc/KEClarifyingCollectionType> ;
	<http://sw.cyc.com/2006/07/27/cyc/typeGenls> <http://sw.cyc.com/2006/07/27/cyc/Weapon> .

<http://sw.cyc.com/2006/07/27/cyc/ExistingObjectType> <http://www.w3.org/2000/01/rdf-schema#comment> """A collection of collections.  Each instance of #$ExistingObjectType is a specialization of #$PartiallyTangible (q.v.).  Moreover, each instance of #$ExistingObjectType is a collection that is temporally stuff-like (see #$TemporalStuffType) but physically-spatially object-like (see #$ObjectType) -- i.e.  object-like with respect to some physical-spatial part-whole predicate (e.g. some specialization of #$properPhysicalDecompositions).
<p>
Consider the collection #$BookCopy. #$BookCopy is a specialization of #$PartiallyTangible. Further, #$BookCopy is temporally stuff-like: any one of the #$timeSlices of a given copy <code>COPY</code> of (say) \"Moby Dick\" is still a copy of \"Moby Dick\". (Most collections of tangible objects are temporally stuff-like in this way.)   But #$BookCopy is spatially <i>object-like</i>: if we take a scalpel and slice <code>COPY</code> into ten pieces, each piece is not a copy of \"Moby Dick\".  So #$BookCopy is an instance of #$ExistingObjectType.
<p>
See also #$StuffType and #$ExistingStuffType.""" ;
	a <http://sw.cyc.com/2006/07/27/cyc/AtemporalNecessarilyEssentialCollectionType> , <http://sw.cyc.com/2006/07/27/cyc/FacetingCollectionType> , <http://sw.cyc.com/2006/07/27/cyc/SecondOrderCollection> , <http://sw.cyc.com/2006/07/27/cyc/Top-Topic> , <http://sw.cyc.com/2006/07/27/cyc/CollectionClosedUnderSpecialization> ;
	<http://sw.cyc.com/2006/07/27/cyc/prettyString-Canonical> "type of object" ;
	<http://sw.cyc.com/2006/07/27/cyc/prettyString> "types of object" , "kind of existing objects" , "kinds of existing objects" , "kind of existing object" , "kinds of existing object" , "type of temporally enduring object" , "types of temporally enduring object" , "type of existing object" , "types of existing object" , "existing object type" , "existing object types" ;
	<http://www.w3.org/2000/01/rdf-schema#subClassOf> <http://sw.cyc.com/2006/07/27/cyc/ObjectType> , <http://sw.cyc.com/2006/07/27/cyc/FirstOrderCollection> , <http://sw.cyc.com/2006/07/27/cyc/TemporalStuffType> ;
	<http://www.w3.org/2002/07/owl#disjointWith> <http://sw.cyc.com/2006/07/27/cyc/PhysiologicalConditionType> , <http://sw.cyc.com/2006/07/27/cyc/DurativeEventType> , <http://sw.cyc.com/2006/07/27/cyc/WavePropagationType> , <http://sw.cyc.com/2006/07/27/cyc/AttackByComputerOperationActionType> , <http://sw.cyc.com/2006/07/27/cyc/ControllableAutonomousActionType> ;
	<http://sw.cyc.com/2006/07/27/cyc/typeGenls> <http://sw.cyc.com/2006/07/27/cyc/PartiallyTangible> .

<http://sw.cyc.com/2006/07/27/cyc/106235-09-TheSoftwarePatch> a <http://sw.cyc.com/2006/07/27/cyc/Individual> , <http://sw.cyc.com/2006/07/27/cyc/ArchitectureIndependentComputerPatchProgram> , <http://sw.cyc.com/2006/07/27/cyc/ComputerPatchProgram> .

<http://sw.cyc.com/2006/07/27/cyc/AnalystDatabaseMt> <http://sw.cyc.com/2006/07/27/cyc/genlMt> <http://sw.cyc.com/2006/07/27/cyc/WorldWideWebURLMt> .

<http://sw.cyc.com/2006/07/27/cyc/SAICTerrorismEventsDataMt> <http://sw.cyc.com/2006/07/27/cyc/genlMt> <http://sw.cyc.com/2006/07/27/cyc/SAICAlQaidaDataMt> .

<http://sw.cyc.com/2006/07/27/cyc/SAICBioTerrorismEventsDataMt> <http://sw.cyc.com/2006/07/27/cyc/genlMt> <http://sw.cyc.com/2006/07/27/cyc/CIAWorldFactbook1997Mt> .

<http://sw.cyc.com/2006/07/27/cyc/PatternsOfGlobalTerrorism1998Mt> <http://sw.cyc.com/2006/07/27/cyc/genlMt> <http://sw.cyc.com/2006/07/27/cyc/RealTimeMt> .

<http://sw.cyc.com/2006/07/27/cyc/PatternsOfGlobalTerrorism1997Mt> <http://sw.cyc.com/2006/07/27/cyc/genlMt> <http://sw.cyc.com/2006/07/27/cyc/PatternDetectorMt> .

<http://sw.cyc.com/2006/07/27/cyc/LDSCGeneralCollectorMt> <http://sw.cyc.com/2006/07/27/cyc/genlMt> <http://sw.cyc.com/2006/07/27/cyc/NDUForum-BioterrorismMt> .

<http://sw.cyc.com/2006/07/27/cyc/SAICTerroristGroupsDataMt> <http://sw.cyc.com/2006/07/27/cyc/genlMt> <http://sw.cyc.com/2006/07/27/cyc/CurrentWorldDataCollectorMt-NonHomocentric> .

<http://sw.cyc.com/2006/07/27/cyc/SAICAlQaidaDataMt> <http://sw.cyc.com/2006/07/27/cyc/genlMt> <http://sw.cyc.com/2006/07/27/cyc/LDSCDemonstrationSpindleHeadMt> .

<http://sw.cyc.com/2006/07/27/cyc/LDSCDemonstrationSpindleHeadMt> a <http://sw.cyc.com/2006/07/27/cyc/Microtheory> .

<http://sw.cyc.com/2006/07/27/cyc/DataMicrotheory> a <http://sw.cyc.com/2006/07/27/cyc/MicrotheoryType> .

<http://sw.cyc.com/2006/07/27/cyc/10000Maniacs-MusicGroup> <http://sw.cyc.com/2006/07/27/cyc/prettyString> "10,000 Maniacs" .

<http://sw.cyc.com/2006/07/27/cyc/StrategyGameProgram> a <http://sw.cyc.com/2006/07/27/cyc/AtemporalNecessarilyEssentialCollectionType> .

<http://sw.cyc.com/2006/07/27/cyc/105MMRifledBoreCannon> <http://sw.cyc.com/2006/07/27/cyc/prettyString> "105 mm rifled guns" .

<http://sw.cyc.com/2006/07/27/cyc/106235-09-TheSoftwarePatch> <http://sw.cyc.com/2006/07/27/cyc/prettyString-Canonical> "Sun patch 106235-09" .

<http://sw.cyc.com/2006/07/27/cyc/ArcadeGameProgram> <http://www.w3.org/2000/01/rdf-schema#subClassOf> <http://sw.cyc.com/2006/07/27/cyc/ComputerGameProgram> .

<http://sw.cyc.com/2006/07/27/cyc/BlueUnit> a <http://sw.cyc.com/2006/07/27/cyc/ExistingObjectType> .

<http://sw.cyc.com/2006/07/27/cyc/123tkShop-TheProgram> a <http://sw.cyc.com/2006/07/27/cyc/UnversionedProgram> .

<http://sw.cyc.com/2006/07/27/cyc/DramaticMovie> <http://www.w3.org/2000/01/rdf-schema#comment> "#$DramaticMovie is a collection of instances of #$Movie-CW each of which relates a story involving human conflict." .

<http://sw.cyc.com/2006/07/27/cyc/PartiallyTangible> <http://sw.cyc.com/2006/07/27/cyc/facets-Generic> <http://sw.cyc.com/2006/07/27/cyc/EfficaciousSubstanceTypeByComposition> .

<http://sw.cyc.com/2006/07/27/cyc/12InchTelevisionSet> <http://sw.cyc.com/2006/07/27/cyc/prettyString> "12 inch television sets" .

<http://sw.cyc.com/2006/07/27/cyc/14East-TheCompany> a <http://sw.cyc.com/2006/07/27/cyc/Individual> .

<http://sw.cyc.com/2006/07/27/cyc/Business> <http://sw.cyc.com/2006/07/27/cyc/prettyString> "business organization" .

<http://sw.cyc.com/2006/07/27/cyc/1990sPopMusicPerformer> a <http://sw.cyc.com/2006/07/27/cyc/MusicalPerformanceAgentTypeByGenre> .

<http://sw.cyc.com/2006/07/27/cyc/CommandUnit-MilitarySpecialty> a <http://sw.cyc.com/2006/07/27/cyc/GenericMilitaryOrganizations-Organization-Topic> .

<http://sw.cyc.com/2006/07/27/cyc/1On1BasketballGame-TheGame> a <http://sw.cyc.com/2006/07/27/cyc/OnlineGameProgram> .

<http://sw.cyc.com/2006/07/27/cyc/1stGradeSuccessStarter-TheGame> a <http://sw.cyc.com/2006/07/27/cyc/ComputerGameProgram> .

<http://sw.cyc.com/2006/07/27/cyc/1stManeuverRegiment-RRS> <http://sw.cyc.com/2006/07/27/cyc/quotedIsa> <http://sw.cyc.com/2006/07/27/cyc/FACToryIrrelevantTerm> .

<http://sw.cyc.com/2006/07/27/cyc/Novel-CW> <http://www.w3.org/2000/01/rdf-schema#comment> "The collection of all #$ConceptualWorks that are novels." .

<http://sw.cyc.com/2006/07/27/cyc/208MotorizedRifleDivision-RRS> a <http://sw.cyc.com/2006/07/27/cyc/Individual> .

<http://sw.cyc.com/2006/07/27/cyc/21cSagemanDataGroup2> <http://sw.cyc.com/2006/07/27/cyc/prettyString-Canonical> "21c sageman data group 2" .

<http://sw.cyc.com/2006/07/27/cyc/21cTestGroup2-2> <http://www.w3.org/2000/01/rdf-schema#comment> "21c group2 2  ." .

<http://sw.cyc.com/2006/07/27/cyc/21cTestGroup6> a <http://sw.cyc.com/2006/07/27/cyc/21cSagemanDataGroup> .

<http://sw.cyc.com/2006/07/27/cyc/25InchTelevisionSet> <http://www.w3.org/2000/01/rdf-schema#subClassOf> <http://sw.cyc.com/2006/07/27/cyc/ManufacturedGoods> .

<http://sw.cyc.com/2006/07/27/cyc/25thInfantryDivision-Light-Washington> a <http://sw.cyc.com/2006/07/27/cyc/Individual> .

<http://sw.cyc.com/2006/07/27/cyc/2ByteIntegerDatatype> <http://sw.cyc.com/2006/07/27/cyc/prettyString> "two-byte integer" .

<http://sw.cyc.com/2006/07/27/cyc/DestroyingAnEnemyForce> <http://sw.cyc.com/2006/07/27/cyc/prettyString> "has destroyed an enemy force" .

<http://sw.cyc.com/2006/07/27/cyc/2ndMID> <http://sw.cyc.com/2006/07/27/cyc/prettyString> "the Blue 2nd MID" .

<http://sw.cyc.com/2006/07/27/cyc/IntermediateAdjustableRateLoanTypeByInitialAdjustmentPeriod> a <http://sw.cyc.com/2006/07/27/cyc/SecondOrderCollection> .

<http://sw.cyc.com/2006/07/27/cyc/35InchTelevisionSet> <http://sw.cyc.com/2006/07/27/cyc/prettyString> "35 inch television sets" .

<http://sw.cyc.com/2006/07/27/cyc/38thParallel-North> <http://sw.cyc.com/2006/07/27/cyc/prettyString-Canonical> "38th Parallel North" .

<http://sw.cyc.com/2006/07/27/cyc/3DComputerWallpaperFile> a <http://sw.cyc.com/2006/07/27/cyc/ObjectType> .

<http://sw.cyc.com/2006/07/27/cyc/3DFlowerboxScreenSaver-TheProgram> a <http://sw.cyc.com/2006/07/27/cyc/Individual> .

<http://sw.cyc.com/2006/07/27/cyc/3DFlyingObjectsScreenSaver-TheProgram> <http://sw.cyc.com/2006/07/27/cyc/prettyString-Canonical> "OpenGL 3D Flying Objects Screen Saver" .

<http://sw.cyc.com/2006/07/27/cyc/3DMazeScreenSaver-TheProgram> a <http://sw.cyc.com/2006/07/27/cyc/ScreenSaver> .

<http://sw.cyc.com/2006/07/27/cyc/3-DUltraPinball2CreepNight-TheGame> a <http://sw.cyc.com/2006/07/27/cyc/UnversionedProgram> .

<http://sw.cyc.com/2006/07/27/cyc/40thParallel-North> a <http://sw.cyc.com/2006/07/27/cyc/LatitudeLine> .

<http://sw.cyc.com/2006/07/27/cyc/4ByteTwosComplementInteger> a <http://sw.cyc.com/2006/07/27/cyc/4ByteIntegerDatatype> .

<http://sw.cyc.com/2006/07/27/cyc/4-TheDigit> <http://sw.cyc.com/2006/07/27/cyc/prettyString> "the numerals 4" .

<http://sw.cyc.com/2006/07/27/cyc/602ProLANSUITE2000a-TheProgram> a <http://sw.cyc.com/2006/07/27/cyc/Individual> .

<http://sw.cyc.com/2006/07/27/cyc/76MMRifledBoreCannon> <http://sw.cyc.com/2006/07/27/cyc/prettyString> "76 millimeter rifled cannon" .

<http://sw.cyc.com/2006/07/27/cyc/83rdMeridian-West> a <http://sw.cyc.com/2006/07/27/cyc/LongitudeLine> .

<http://sw.cyc.com/2006/07/27/cyc/8ByteRealDatatype> a <http://sw.cyc.com/2006/07/27/cyc/SKSIDataTypeDescriptions-Topic> .

<http://sw.cyc.com/2006/07/27/cyc/A1Stats-TheProgram> a <http://sw.cyc.com/2006/07/27/cyc/Individual> .

<http://sw.cyc.com/2006/07/27/cyc/A-5C-Fighter> a <http://sw.cyc.com/2006/07/27/cyc/TransportationDeviceType> .

<http://sw.cyc.com/2006/07/27/cyc/AAAIConference-2005> <http://sw.cyc.com/2006/07/27/cyc/prettyString> "The 21st National Conference on Artificial Intelligence" .

<http://sw.cyc.com/2006/07/27/cyc/AAAIPress> <http://sw.cyc.com/2006/07/27/cyc/prettyString-Canonical> "AAAI Press" .

<http://sw.cyc.com/2006/07/27/cyc/Organization> <http://www.w3.org/2002/07/owl#disjointWith> <http://sw.cyc.com/2006/07/27/cyc/ComputerMarketCategory> .

<http://sw.cyc.com/2006/07/27/cyc/ServiceEvent> a <http://sw.cyc.com/2006/07/27/cyc/TemporalStuffType> .

<http://sw.cyc.com/2006/07/27/cyc/GeographicalThing> a <http://sw.cyc.com/2006/07/27/cyc/SpatiallyDisjointObjectType> .

<http://sw.cyc.com/2006/07/27/cyc/AAMilne> a <http://sw.cyc.com/2006/07/27/cyc/Writer> .

<http://sw.cyc.com/2006/07/27/cyc/Person> a <http://sw.cyc.com/2006/07/27/cyc/CandidateKBCompletenessNode> .

<http://sw.cyc.com/2006/07/27/cyc/Aana-DistrictWesternSamoa> a <http://sw.cyc.com/2006/07/27/cyc/Individual> .

<http://sw.cyc.com/2006/07/27/cyc/Actor> <http://sw.cyc.com/2006/07/27/cyc/prettyString> "player" .

<http://sw.cyc.com/2006/07/27/cyc/AaronVsRuth-TheGame> <http://sw.cyc.com/2006/07/27/cyc/prettyString-Canonical> "Aaron Vs. Ruth" .

<http://sw.cyc.com/2006/07/27/cyc/DrugProduct> a <http://sw.cyc.com/2006/07/27/cyc/TemporallyExistingThingTypeFrequentlyForSale> .

<http://sw.cyc.com/2006/07/27/cyc/AbaCloth> <http://www.w3.org/2000/01/rdf-schema#comment> "The collection of #$Cloth woven from goat and camel hair, made in the #$ArabianPeninsula, #$Syria, or nearby places." .

<http://sw.cyc.com/2006/07/27/cyc/Aba-Garment> <http://sw.cyc.com/2006/07/27/cyc/prettyString> "abas" .

<http://sw.cyc.com/2006/07/27/cyc/123tkShop-TheProgram> a <http://sw.cyc.com/2006/07/27/cyc/LocalProgram> , <http://sw.cyc.com/2006/07/27/cyc/UserProgram> ;
	<http://sw.cyc.com/2006/07/27/cyc/prettyString-Canonical> "123tkShop" .

<http://sw.cyc.com/2006/07/27/cyc/LocalProgram> <http://www.w3.org/2000/01/rdf-schema#comment> "A specialization of #$ApplicationProgram. Each instance of #$LocalProgram is a program that cannot be accessed remotely (i.e. across a #$ComputerNetwork). #$LocalProgram is dijoint with #$ServerProgram, and the two form a partition of #$ComputerProgram-CW." ;
	a <http://www.w3.org/2002/07/owl#Class> , <http://sw.cyc.com/2006/07/27/cyc/ObjectType> , <http://sw.cyc.com/2006/07/27/cyc/AtemporalNecessarilyEssentialCollectionType> ;
	<http://sw.cyc.com/2006/07/27/cyc/prettyString-Canonical> "local program" ;
	<http://sw.cyc.com/2006/07/27/cyc/prettyString> "local programme" , "local programs" , "local programz" ;
	<http://www.w3.org/2000/01/rdf-schema#subClassOf> <http://sw.cyc.com/2006/07/27/cyc/ApplicationProgram> .

<http://sw.cyc.com/2006/07/27/cyc/UserProgram> <http://www.w3.org/2000/01/rdf-schema#comment> "#$UserProgram is a specialization of #$ComputerProgram-CW.  It is the collection of programs whose running processes computer users typically interact with.  Computer users are usually able to configure these programs to suit their individual needs.  For example, #$NetscapeNavigator is a #$UserProgram because users interact with it when they browse web pages, and they can configure it to implement various security features, to store passwords, to cache a history, etc. Note that #$UserProgram and #$ServiceProgram partition #$ComputerProgram-CW." ;
	a <http://www.w3.org/2002/07/owl#Class> , <http://sw.cyc.com/2006/07/27/cyc/ObjectType> , <http://sw.cyc.com/2006/07/27/cyc/AtemporalNecessarilyEssentialCollectionType> ;
	<http://sw.cyc.com/2006/07/27/cyc/prettyString-Canonical> "user program" ;
	<http://sw.cyc.com/2006/07/27/cyc/prettyString> "user programme" , "user programs" , "user programz" ;
	<http://www.w3.org/2000/01/rdf-schema#subClassOf> <http://sw.cyc.com/2006/07/27/cyc/ApplicationProgram> ;
	<http://www.w3.org/2002/07/owl#disjointWith> <http://sw.cyc.com/2006/07/27/cyc/ServiceProgram> .

<http://sw.cyc.com/2006/07/27/cyc/123tkShopUpgrade-TheSoftwarePatch> a <http://sw.cyc.com/2006/07/27/cyc/ArchitectureIndependentComputerPatchProgram> ;
	<http://sw.cyc.com/2006/07/27/cyc/prettyString-Canonical> "123tk Shop Upgrade The Software Patch" .

<http://sw.cyc.com/2006/07/27/cyc/124CbtEngrBn> a <http://sw.cyc.com/2006/07/27/cyc/Individual> , <http://sw.cyc.com/2006/07/27/cyc/BlueUnit> , <http://sw.cyc.com/2006/07/27/cyc/Battalion-MilitaryEchelon> , <http://sw.cyc.com/2006/07/27/cyc/EngineeringUnit-MilitarySpecialty> ;
	<http://sw.cyc.com/2006/07/27/cyc/prettyString-Canonical> "124 Cbt Engr Bn" ;
	<http://sw.cyc.com/2006/07/27/cyc/quotedIsa> <http://sw.cyc.com/2006/07/27/cyc/FACToryIrrelevantTerm> .

<http://sw.cyc.com/2006/07/27/cyc/Battalion-MilitaryEchelon> <http://www.w3.org/2000/01/rdf-schema#comment> """A #$MilitaryUnitTypeByEchelon and a subcollection of #$ModernMilitaryOrganization. #$Battalion-MilitaryEchelon is and an instance of both #$USArmyEchelon and #$USMarineCorpsEchelon.  
<p>
In the US Army, a battalion consists of between 300 and 1,000 soldiers, and is typically made up of four to six companies (see #$Company-MilitaryEchelon).  Two to five battalions typically make up an army #$Brigade-MilitaryEchelon.
<p>
In the US Marine Corps, a battalion consists of roughly 1,200 marines, and is typically made up of five companies.  Five battalions typically make up a marine #$Regiment-MilitaryEchelon.""" ;
	a <http://sw.cyc.com/2006/07/27/cyc/GenericMilitaryOrganizations-Organization-Topic> , <http://sw.cyc.com/2006/07/27/cyc/MilitaryOrganizationConcept> , <http://sw.cyc.com/2006/07/27/cyc/IranianArmyEchelon> , <http://sw.cyc.com/2006/07/27/cyc/USArmyEchelon> , <http://sw.cyc.com/2006/07/27/cyc/BPVEchelon> , <http://sw.cyc.com/2006/07/27/cyc/USMarineCorpsEchelon> ;
	<http://sw.cyc.com/2006/07/27/cyc/prettyString-Canonical> "battalion" ;
	<http://sw.cyc.com/2006/07/27/cyc/prettyString> "battalions" ;
	<http://www.w3.org/2000/01/rdf-schema#subClassOf> <http://sw.cyc.com/2006/07/27/cyc/ModernMilitaryOrganization> , <http://sw.cyc.com/2006/07/27/cyc/CPOF-MilitaryUnit> .

<http://sw.cyc.com/2006/07/27/cyc/EngineeringUnit-MilitarySpecialty> <http://www.w3.org/2000/01/rdf-schema#comment> "The collection of all military units specialized to provide engineering support to other military units." ;
	a <http://sw.cyc.com/2006/07/27/cyc/KEClarifyingCollectionType> , <http://sw.cyc.com/2006/07/27/cyc/MilitaryUnitSpecialtyType> , <http://sw.cyc.com/2006/07/27/cyc/GenericMilitaryOrganizations-Organization-Topic> , <http://sw.cyc.com/2006/07/27/cyc/MilitaryOrganizationConcept> , <http://sw.cyc.com/2006/07/27/cyc/BPVItemType> , <http://sw.cyc.com/2006/07/27/cyc/BPVAgentType> , <http://sw.cyc.com/2006/07/27/cyc/BPVMilitaryUnitType> , <http://sw.cyc.com/2006/07/27/cyc/CPOF-MilitaryUnitType> , <http://sw.cyc.com/2006/07/27/cyc/CPOF-UnitSpecialtyClassificationType> ;
	<http://sw.cyc.com/2006/07/27/cyc/prettyString-Canonical> "engineering unit" ;
	<http://sw.cyc.com/2006/07/27/cyc/prettyString> "engineering units" ;
	<http://www.w3.org/2000/01/rdf-schema#subClassOf> <http://sw.cyc.com/2006/07/27/cyc/Platoon-MilitaryEchelon> , <http://sw.cyc.com/2006/07/27/cyc/ModernMilitaryUnit-Deployable> , <http://sw.cyc.com/2006/07/27/cyc/BPVMilitaryUnit> , <http://sw.cyc.com/2006/07/27/cyc/BPVAgent> , <http://sw.cyc.com/2006/07/27/cyc/BPVItem> , <http://sw.cyc.com/2006/07/27/cyc/CPOF-MilitaryUnit> , <http://sw.cyc.com/2006/07/27/cyc/MaterialSupportUnit-MilitarySpecialty> .

<http://sw.cyc.com/2006/07/27/cyc/125CbtEngrBn> a <http://sw.cyc.com/2006/07/27/cyc/Individual> , <http://sw.cyc.com/2006/07/27/cyc/BlueUnit> , <http://sw.cyc.com/2006/07/27/cyc/Battalion-MilitaryEchelon> , <http://sw.cyc.com/2006/07/27/cyc/EngineeringUnit-MilitarySpecialty> ;
	<http://sw.cyc.com/2006/07/27/cyc/prettyString-Canonical> "125 Cbt Engr Bn" ;
	<http://sw.cyc.com/2006/07/27/cyc/quotedIsa> <http://sw.cyc.com/2006/07/27/cyc/FACToryIrrelevantTerm> .

<http://sw.cyc.com/2006/07/27/cyc/125MMSmoothBoreCannon> <http://www.w3.org/2000/01/rdf-schema#comment> """A kind of #$Cannon
 common on Chinese Tanks.""" ;
	a <http://sw.cyc.com/2006/07/27/cyc/WeaponType> , <http://sw.cyc.com/2006/07/27/cyc/ExistingObjectType> ;
	<http://sw.cyc.com/2006/07/27/cyc/prettyString-Canonical> "125 mm smooth bore cannon" ;
	<http://sw.cyc.com/2006/07/27/cyc/prettyString> "125 millimeter smooth bore gun" , "125 millimeter smooth bore guns" , "125 mm smooth bore gun" , "125 mm smooth bore guns" , "125 millimeter smooth bore cannon" , "125 millimeter smooth bore cannons" , "125 mm smooth bore cannons" ;
	<http://www.w3.org/2000/01/rdf-schema#subClassOf> <http://sw.cyc.com/2006/07/27/cyc/TankCannon> , <http://sw.cyc.com/2006/07/27/cyc/SmoothBoreWeapon> .

<http://sw.cyc.com/2006/07/27/cyc/SmoothBoreWeapon> <http://www.w3.org/2000/01/rdf-schema#comment> "The collection of #$ProjectileLaunchers that have #$Bores with smooth surfaces." ;
	a <http://sw.cyc.com/2006/07/27/cyc/KEClarifyingCollectionType> , <http://sw.cyc.com/2006/07/27/cyc/GunTypeByBarrelType> ;
	<http://sw.cyc.com/2006/07/27/cyc/prettyString-Canonical> "smooth bore weapon" ;
	<http://sw.cyc.com/2006/07/27/cyc/prettyString> "smooth bore weapons" ;
	<http://www.w3.org/2000/01/rdf-schema#subClassOf> <http://sw.cyc.com/2006/07/27/cyc/Gun> .

<http://sw.cyc.com/2006/07/27/cyc/12AngryMen-TheMovie> a <http://sw.cyc.com/2006/07/27/cyc/Individual> , <http://sw.cyc.com/2006/07/27/cyc/DramaticMovie> ;
	<http://sw.cyc.com/2006/07/27/cyc/prettyString-Canonical> "Twelve Angry Men" ;
	<http://sw.cyc.com/2006/07/27/cyc/prettyString> "12 Angry Men" .

<http://sw.cyc.com/2006/07/27/cyc/12InchTelevisionSet> <http://www.w3.org/2000/01/rdf-schema#subClassOf> <http://sw.cyc.com/2006/07/27/cyc/ManufacturedGoods> , <http://sw.cyc.com/2006/07/27/cyc/TelevisionSet> .

<http://sw.cyc.com/2006/07/27/cyc/ManufacturedGoods> <http://www.w3.org/2000/01/rdf-schema#comment> "The collection of all #$Artifacts that are made or processed in large-scale industrial operations for distribution (normally sale) to agents outside the manufacturing organization.  This includes manufactured stuff, e.g. Finlandia vodka; refined ore, e.g. iron; otherwise procesed natural material, e.g. cut diamonds, as well as manufactured objects.  This collection excludes handicrafts; privately made stuff, e.g. moonshine; and other artifacts produced by one or a few people on a small scale." ;
	a <http://sw.cyc.com/2006/07/27/cyc/TemporalStuffType> ;
	<http://sw.cyc.com/2006/07/27/cyc/prettyString-Canonical> "product" ;
	<http://sw.cyc.com/2006/07/27/cyc/prettyString> "products" , "manufactured goods" ;
	<http://www.w3.org/2000/01/rdf-schema#subClassOf> <http://sw.cyc.com/2006/07/27/cyc/Artifact-HumanCreated> .

<http://sw.cyc.com/2006/07/27/cyc/TelevisionSet> <http://www.w3.org/2000/01/rdf-schema#comment> "A television set" ;
	a <http://sw.cyc.com/2006/07/27/cyc/SpatiallyDisjointObjectType> , <http://sw.cyc.com/2006/07/27/cyc/ManufacturedGoodsType> , <http://sw.cyc.com/2006/07/27/cyc/DeviceTypeByFunction> ;
	<http://sw.cyc.com/2006/07/27/cyc/prettyString-Canonical> "television set" ;
	<http://sw.cyc.com/2006/07/27/cyc/prettyString> "televisions" , "TV" , "TVs" , "television" , "TV set" , "TV sets" , "television receiver" , "television receivers" , "idiot box" , "idiot boxes" , "boob tube" , "boob tubes" , "television sets" ;
	<http://www.w3.org/2000/01/rdf-schema#subClassOf> <http://sw.cyc.com/2006/07/27/cyc/ManufacturedGoods> , <http://sw.cyc.com/2006/07/27/cyc/NotVeryRoundObject> , <http://sw.cyc.com/2006/07/27/cyc/ElectronicHouseholdAppliance> , <http://sw.cyc.com/2006/07/27/cyc/FrontAndBackSidedObject> , <http://sw.cyc.com/2006/07/27/cyc/CommunicationDevice> ;
	<http://sw.cyc.com/2006/07/27/cyc/facets-Strict> <http://sw.cyc.com/2006/07/27/cyc/TelevisionSetTypeBySize> , <http://sw.cyc.com/2006/07/27/cyc/TelevisionSetTypeByColor> , <http://sw.cyc.com/2006/07/27/cyc/TelevisionSetTypeByProjectionStyle> .

<http://sw.cyc.com/2006/07/27/cyc/SpatiallyDisjointObjectType> <http://www.w3.org/2000/01/rdf-schema#comment> """A collection of collections and a specialization of #$ObjectType (q.v.). Each instance of #$SpatiallyDisjointObjectType is a collection C of spatial things (see #$SpatialThing), where each of the spatial things in C is spatially disjoint with the other spatial things in C.
<p>
For example, the collection #$Dog is an instance of #$SpatiallyDisjointObjectType, since dogs do not spatially overlap.  Even pregnant dogs do not spatially overlap the pups they bear; rather, pregnant dogs contain their unborn pups.  Other instances of #$SpatiallyDisjointObjectType include #$LatitudeLine, #$CompactDisc-Audio, and #$PlanetaryBody.  An important specialization of #$SpatiallyDisjointObjectType is #$SpatiallyDisjointRegionType (a collection of specializations of #$GeographicalRegion, such as #$City and #$TrueContinent).""" ;
	a <http://sw.cyc.com/2006/07/27/cyc/FacetingCollectionType> , <http://sw.cyc.com/2006/07/27/cyc/SecondOrderCollection> ;
	<http://sw.cyc.com/2006/07/27/cyc/prettyString-Canonical> "spatially disjoint object type" ;
	<http://www.w3.org/2000/01/rdf-schema#subClassOf> <http://sw.cyc.com/2006/07/27/cyc/ObjectType> ;
	<http://www.w3.org/2002/07/owl#disjointWith> <http://sw.cyc.com/2006/07/27/cyc/ExistingStuffType> ;
	<http://sw.cyc.com/2006/07/27/cyc/typeGenls> <http://sw.cyc.com/2006/07/27/cyc/SpatialThing> .

<http://sw.cyc.com/2006/07/27/cyc/TelevisionSetTypeBySize> <http://www.w3.org/2000/01/rdf-schema#comment> "A collection of collections. Each instance is a spec of #$TelevisionSet whose instances are all of the same size." ;
	a <http://sw.cyc.com/2006/07/27/cyc/FacetingCollectionType> , <http://sw.cyc.com/2006/07/27/cyc/SecondOrderCollection> , <http://sw.cyc.com/2006/07/27/cyc/DisjointCollectionType> ;
	<http://sw.cyc.com/2006/07/27/cyc/prettyString-Canonical> "type of television classified by size" ;
	<http://sw.cyc.com/2006/07/27/cyc/prettyString> "types of television classified by size" ;
	<http://www.w3.org/2000/01/rdf-schema#subClassOf> <http://sw.cyc.com/2006/07/27/cyc/ArtifactTypeByGenericCategory> , <http://sw.cyc.com/2006/07/27/cyc/ManufacturedGoodsType> , <http://sw.cyc.com/2006/07/27/cyc/FacetInstanceCollection> , <http://sw.cyc.com/2006/07/27/cyc/ConventionalClassificationType> ;
	<http://sw.cyc.com/2006/07/27/cyc/sharedNotes> <http://sw.cyc.com/2006/07/27/cyc/SharedNoteOnGenlsRelationsBetweenFacetingCollectionTypes> ;
	<http://sw.cyc.com/2006/07/27/cyc/typeGenls> <http://sw.cyc.com/2006/07/27/cyc/TelevisionSet> .

<http://sw.cyc.com/2006/07/27/cyc/133SignalsBatt-RRS> a <http://sw.cyc.com/2006/07/27/cyc/Individual> , <http://sw.cyc.com/2006/07/27/cyc/BlueUnit> , <http://sw.cyc.com/2006/07/27/cyc/Battalion-MilitaryEchelon> , <http://sw.cyc.com/2006/07/27/cyc/SignalsUnit-MilitarySpecialty> ;
	<http://sw.cyc.com/2006/07/27/cyc/prettyString-Canonical> "133 Sig Bn" ;
	<http://sw.cyc.com/2006/07/27/cyc/quotedIsa> <http://sw.cyc.com/2006/07/27/cyc/FACToryIrrelevantTerm> .

<http://sw.cyc.com/2006/07/27/cyc/SignalsUnit-MilitarySpecialty> <http://www.w3.org/2000/01/rdf-schema#comment> "The collection of all military units whose mission profile involves           interception, direction-finding, or analysis of EM signals of any           kind." ;
	a <http://sw.cyc.com/2006/07/27/cyc/KEClarifyingCollectionType> , <http://sw.cyc.com/2006/07/27/cyc/MilitaryUnitSpecialtyType> , <http://sw.cyc.com/2006/07/27/cyc/GenericMilitaryOrganizations-Organization-Topic> , <http://sw.cyc.com/2006/07/27/cyc/MilitaryOrganizationConcept> ;
	<http://sw.cyc.com/2006/07/27/cyc/prettyString-Canonical> "signals unit" ;
	<http://sw.cyc.com/2006/07/27/cyc/prettyString> "signals units" ;
	<http://www.w3.org/2000/01/rdf-schema#subClassOf> <http://sw.cyc.com/2006/07/27/cyc/ModernMilitaryUnit-Deployable> .

<http://sw.cyc.com/2006/07/27/cyc/13InchTelevisionSet> a <http://sw.cyc.com/2006/07/27/cyc/ExistingObjectType> , <http://sw.cyc.com/2006/07/27/cyc/SpatiallyDisjointObjectType> , <http://sw.cyc.com/2006/07/27/cyc/TelevisionSetTypeBySize> ;
	<http://sw.cyc.com/2006/07/27/cyc/prettyString-Canonical> "13 inch television set" ;
	<http://sw.cyc.com/2006/07/27/cyc/prettyString> "13 inch television sets" ;
	<http://www.w3.org/2000/01/rdf-schema#subClassOf> <http://sw.cyc.com/2006/07/27/cyc/ManufacturedGoods> , <http://sw.cyc.com/2006/07/27/cyc/TelevisionSet> .

<http://sw.cyc.com/2006/07/27/cyc/1489683-TheSoftwarePatch> a <http://sw.cyc.com/2006/07/27/cyc/Individual> , <http://sw.cyc.com/2006/07/27/cyc/ArchitectureIndependentComputerPatchProgram> , <http://sw.cyc.com/2006/07/27/cyc/ComputerPatchProgram> ;
	<http://sw.cyc.com/2006/07/27/cyc/prettyString-Canonical> "Oracle software patch 1489683" .

<http://sw.cyc.com/2006/07/27/cyc/1990sPopMusicPerformer> <http://sw.cyc.com/2006/07/27/cyc/prettyString-Canonical> "1990s pop music performer" ;
	<http://www.w3.org/2000/01/rdf-schema#subClassOf> <http://sw.cyc.com/2006/07/27/cyc/MusicPerformanceAgent> .

<http://sw.cyc.com/2006/07/27/cyc/1993SmugglingOfCWTechnologyToSyriaFromRussia> a <http://sw.cyc.com/2006/07/27/cyc/Individual> ;
	<http://sw.cyc.com/2006/07/27/cyc/prettyString-Canonical> "1993 Smuggling Of CW Technology To Syria From Russia" .

<http://sw.cyc.com/2006/07/27/cyc/1996LebaneseParliamentaryElections> a <http://sw.cyc.com/2006/07/27/cyc/Individual> ;
	<http://sw.cyc.com/2006/07/27/cyc/prettyString-Canonical> "1996 Lebanese Parliamentary election" ;
	<http://sw.cyc.com/2006/07/27/cyc/prettyString> "1996 Lebanese Parliamentary elections" .

<http://sw.cyc.com/2006/07/27/cyc/19InchTelevisionSet> a <http://sw.cyc.com/2006/07/27/cyc/ExistingObjectType> , <http://sw.cyc.com/2006/07/27/cyc/SpatiallyDisjointObjectType> , <http://sw.cyc.com/2006/07/27/cyc/TelevisionSetTypeBySize> ;
	<http://sw.cyc.com/2006/07/27/cyc/prettyString-Canonical> "19 inch television set" ;
	<http://sw.cyc.com/2006/07/27/cyc/prettyString> "19 inch television sets" ;
	<http://www.w3.org/2000/01/rdf-schema#subClassOf> <http://sw.cyc.com/2006/07/27/cyc/ManufacturedGoods> , <http://sw.cyc.com/2006/07/27/cyc/TelevisionSet> .

<http://sw.cyc.com/2006/07/27/cyc/1ByteIntegerDatatype> a <http://sw.cyc.com/2006/07/27/cyc/FixedSizeComputerDatatypeType> , <http://sw.cyc.com/2006/07/27/cyc/SKSIDataTypeDescriptions-Topic> ;
	<http://sw.cyc.com/2006/07/27/cyc/prettyString-Canonical> "1-byte integer" ;
	<http://sw.cyc.com/2006/07/27/cyc/prettyString> "one-byte integer" , "one-byte integers" , "1-byte integers" ;
	<http://www.w3.org/2000/01/rdf-schema#subClassOf> <http://sw.cyc.com/2006/07/27/cyc/IntegerComputerNumber> , <http://sw.cyc.com/2006/07/27/cyc/ProgramObject> .

<http://sw.cyc.com/2006/07/27/cyc/IntegerComputerNumber> <http://www.w3.org/2000/01/rdf-schema#comment> "The collection of all computer data types that are capable (only) of representing some subset of the integers or values related to representing integer values such as NAN." ;
	a <http://sw.cyc.com/2006/07/27/cyc/FixedSizeComputerDatatypeType> , <http://sw.cyc.com/2006/07/27/cyc/SKSIDataTypeDescriptions-Topic> ;
	<http://sw.cyc.com/2006/07/27/cyc/prettyString-Canonical> "computer integer" ;
	<http://sw.cyc.com/2006/07/27/cyc/prettyString> "computer integers" ;
	<http://www.w3.org/2000/01/rdf-schema#subClassOf> <http://sw.cyc.com/2006/07/27/cyc/ProgramObject> .

<http://sw.cyc.com/2006/07/27/cyc/ProgramObject> <http://www.w3.org/2000/01/rdf-schema#comment> "A specialization of #$ComputerAIS. #$ProgramObject is the collection of all data structures that are explicitly referenced in computer programs. All data types are considered to be specializations of this collection." ;
	a <http://sw.cyc.com/2006/07/27/cyc/SKSIDataTypeDescriptions-Topic> , <http://sw.cyc.com/2006/07/27/cyc/CandidateKBCompletenessNode> , <http://sw.cyc.com/2006/07/27/cyc/ComputerDatatypeType> ;
	<http://sw.cyc.com/2006/07/27/cyc/prettyString-Canonical> "programming datastructure" ;
	<http://sw.cyc.com/2006/07/27/cyc/prettyString> "programming datastructures" ;
	<http://www.w3.org/2000/01/rdf-schema#subClassOf> <http://sw.cyc.com/2006/07/27/cyc/ComputerAIS> .

<http://sw.cyc.com/2006/07/27/cyc/FixedSizeComputerDatatypeType> <http://www.w3.org/2000/01/rdf-schema#comment> "The collection of all computer data types such that all program variables or database fields which are typed by a particular instance of this collection all have the same amount of memory allocated to store their values, whether or not the value could be stored in less space.  For example, the base 10 integer, 250, could be stored in a field or variable that is typed TINYINT, or #$1ByteIntegerDatatype.  In this case, one byte of storage is allocated to hold the value.  It can also be stored as a #$4ByteIntegerDatatype, and then 4 bytes of storage will be allocated, even though it could fit in a smaller space. " ;
	a <http://sw.cyc.com/2006/07/27/cyc/FacetingCollectionType> , <http://sw.cyc.com/2006/07/27/cyc/SecondOrderCollection> ;
	<http://sw.cyc.com/2006/07/27/cyc/prettyString-Canonical> "fixed-size data type" ;
	<http://sw.cyc.com/2006/07/27/cyc/prettyString> "fixed-size data types" ;
	<http://www.w3.org/2000/01/rdf-schema#subClassOf> <http://sw.cyc.com/2006/07/27/cyc/ComputerDatatypeType> .

<http://sw.cyc.com/2006/07/27/cyc/SKSIDataTypeDescriptions-Topic> <http://www.w3.org/2000/01/rdf-schema#comment> "#$SKSIDataTypeDescriptions-Topic is the #$Topic containing the #$CycL terms used to describe data types for SKSI." ;
	a <http://sw.cyc.com/2006/07/27/cyc/KBDependentCollection> , <http://sw.cyc.com/2006/07/27/cyc/CycVocabularyTopic> ;
	<http://sw.cyc.com/2006/07/27/cyc/prettyString-Canonical> "SKSI data type descriptions topic" ;
	<http://www.w3.org/2000/01/rdf-schema#subClassOf> <http://sw.cyc.com/2006/07/27/cyc/SKSI-Topic> .

<http://sw.cyc.com/2006/07/27/cyc/1MMRRegimentHQ-RRS> a <http://sw.cyc.com/2006/07/27/cyc/Individual> , <http://sw.cyc.com/2006/07/27/cyc/Platoon-MilitaryEchelon> , <http://sw.cyc.com/2006/07/27/cyc/CommandUnit-MilitarySpecialty> , <http://sw.cyc.com/2006/07/27/cyc/RedUnit> ;
	<http://sw.cyc.com/2006/07/27/cyc/prettyString-Canonical> "HQ/1 MRR" ;
	<http://sw.cyc.com/2006/07/27/cyc/quotedIsa> <http://sw.cyc.com/2006/07/27/cyc/FACToryIrrelevantTerm> .

<http://sw.cyc.com/2006/07/27/cyc/CommandUnit-MilitarySpecialty> <http://www.w3.org/2000/01/rdf-schema#comment> "A #$MilitaryUnitSpecialtyType and thus a specialization of #$ModernMilitaryOrganization.  This is the collection of all military units that play a command role.  An important specialization of this collection is #$HeadquartersUnit-MilitarySpecialty." ;
	a <http://sw.cyc.com/2006/07/27/cyc/MilitaryUnitSpecialtyType> .

<http://sw.cyc.com/2006/07/27/cyc/Regiment-MilitaryEchelon> <http://www.w3.org/2000/01/rdf-schema#comment> """A #$MilitaryUnitTypeByEchelon and a subcollection of #$ModernMilitaryOrganization.  #$Regiment-MilitaryEchelon is and an instance of #$USMarineCorpsEchelon and #$USArmyEchelon.  
<p>
In the US Marine Corps, a regiment consists of roughly 6,000 marines, and is typically made up of five battalions (see #$Battalion-MilitaryEchelon)
<p>
In the US Army, certain brigade-sized units (see #$Brigade-MilitaryEchelon) are sometimes called \"regiments\".""" ;
	a <http://sw.cyc.com/2006/07/27/cyc/GenericMilitaryOrganizations-Organization-Topic> , <http://sw.cyc.com/2006/07/27/cyc/MilitaryOrganizationConcept> , <http://sw.cyc.com/2006/07/27/cyc/IranianArmyEchelon> , <http://sw.cyc.com/2006/07/27/cyc/USArmyEchelon> , <http://sw.cyc.com/2006/07/27/cyc/USMarineCorpsEchelon> ;
	<http://sw.cyc.com/2006/07/27/cyc/prettyString-Canonical> "regiment" ;
	<http://sw.cyc.com/2006/07/27/cyc/prettyString> "regiments" ;
	<http://www.w3.org/2000/01/rdf-schema#subClassOf> <http://sw.cyc.com/2006/07/27/cyc/ModernMilitaryOrganization> .

<http://sw.cyc.com/2006/07/27/cyc/1stStateBancorpInc> a <http://sw.cyc.com/2006/07/27/cyc/Individual> , <http://sw.cyc.com/2006/07/27/cyc/PubliclyHeldCorporation> ;
	<http://sw.cyc.com/2006/07/27/cyc/prettyString-Canonical> "1st State Bancorp Inc" .

<http://sw.cyc.com/2006/07/27/cyc/1stUpMailServer-TheProgram> <http://www.w3.org/2000/01/rdf-schema#comment> """#$1stUpMailServer-TheProgram is an email server which supports most common
internet protocols and email software offered by Upland Solutions.""" ;
	a <http://sw.cyc.com/2006/07/27/cyc/Individual> , <http://sw.cyc.com/2006/07/27/cyc/UnversionedProgram> , <http://sw.cyc.com/2006/07/27/cyc/SMTPServerProgram> , <http://sw.cyc.com/2006/07/27/cyc/ServerProgram> ;
	<http://sw.cyc.com/2006/07/27/cyc/prettyString-Canonical> "1st Up Mail Server" .

<http://sw.cyc.com/2006/07/27/cyc/SMTPServerProgram> <http://www.w3.org/2000/01/rdf-schema#comment> """#$SMTPServerProgram is the collection of #$ServerPrograms that implement the Simple Mail Transfer Protocol (SMTP), the #$Internet's standard host-to-host mail transport protocol that traditionally
operates over TCP, port 25. A UNIX user can type 'telnet hostname 25'
and connect with an #$SMTPServerProgram on hostname, if one is present.""" ;
	a <http://sw.cyc.com/2006/07/27/cyc/KEClarifyingCollectionType> , <http://sw.cyc.com/2006/07/27/cyc/ComputerProgramTypeByFunction> ;
	<http://sw.cyc.com/2006/07/27/cyc/prettyString-Canonical> "SMTP server program" ;
	<http://sw.cyc.com/2006/07/27/cyc/prettyString> "SMTP server programme" , "SMTP server programs" , "SMTP server programz" ;
	<http://www.w3.org/2000/01/rdf-schema#subClassOf> <http://sw.cyc.com/2006/07/27/cyc/EMailServerProgram> , <http://sw.cyc.com/2006/07/27/cyc/InternetMailAccessServerProgram> .

<http://sw.cyc.com/2006/07/27/cyc/ServerProgram> <http://www.w3.org/2000/01/rdf-schema#comment> "A specialization of #$NetworkingProgram. Each instance of this collection is a #$ComputerProgram-CW used to process requests that come in across a #$ComputerNetwork. It is thus to be contrasted with #$LocalProgram. More technically, the defining characteristic of a #$ServerProgram is that it listens on a port." ;
	a <http://sw.cyc.com/2006/07/27/cyc/ObjectType> , <http://sw.cyc.com/2006/07/27/cyc/AtemporalNecessarilyEssentialCollectionType> , <http://sw.cyc.com/2006/07/27/cyc/KEClarifyingCollectionType> , <http://sw.cyc.com/2006/07/27/cyc/MachineProtocolParticipantType> ;
	<http://sw.cyc.com/2006/07/27/cyc/prettyString-Canonical> "server program" ;
	<http://sw.cyc.com/2006/07/27/cyc/prettyString> "servers" , "Server" , "server programme" , "server programs" , "server programz" ;
	<http://www.w3.org/2000/01/rdf-schema#subClassOf> <http://sw.cyc.com/2006/07/27/cyc/NetworkingProgram> ;
	<http://sw.cyc.com/2006/07/27/cyc/quotedIsa> <http://sw.cyc.com/2006/07/27/cyc/ExtractedByNounLearnerFromMotleyFoolUKCorpus> ;
	<http://www.w3.org/2002/07/owl#disjointWith> <http://sw.cyc.com/2006/07/27/cyc/LocalProgram> .

<http://sw.cyc.com/2006/07/27/cyc/1-TheDigit> <http://www.w3.org/2000/01/rdf-schema#comment> "The numeral 1 of the Arabic Number system.  This is '1' as a #$Character-Abstract rather than the physical #$WrittenCharacter or the abstract mathematical #$Number-General (see #$One)." ;
	a <http://sw.cyc.com/2006/07/27/cyc/ArabicNumeral> ;
	<http://sw.cyc.com/2006/07/27/cyc/prettyString-Canonical> "the numeral 1" ;
	<http://sw.cyc.com/2006/07/27/cyc/prettyString> "the numerals 1" .

<http://sw.cyc.com/2006/07/27/cyc/1YearAdjustableRateLoan> <http://www.w3.org/2000/01/rdf-schema#comment> "An instance of #$AdjustableRateLoanTypeByAdjustmentPeriod.  Instances of this collection are loans whose adjustment period (c.f., #$adjustmentPeriod) is 1 year -- i.e., every year, the interest rate (c.f., #$interestRate) of the loan is subject to change." ;
	a <http://sw.cyc.com/2006/07/27/cyc/AdjustableRateLoanTypeByAdjustmentPeriod> ;
	<http://sw.cyc.com/2006/07/27/cyc/prettyString-Canonical> "one year adjustable rate loan" ;
	<http://sw.cyc.com/2006/07/27/cyc/prettyString> "12 month adjustable rate loan" , "12 month adjustable rate loans" , "twelve month adjustable rate loan" , "twelve month adjustable rate loans" , "1 year adjustable rate loan" , "1 year adjustable rate loans" , "one year adjustable rate loans" ;
	<http://www.w3.org/2000/01/rdf-schema#subClassOf> <http://sw.cyc.com/2006/07/27/cyc/AdjustableRateLoan-ConsistentAdjustmentPeriod> .

<http://sw.cyc.com/2006/07/27/cyc/AdjustableRateLoan-ConsistentAdjustmentPeriod> <http://www.w3.org/2000/01/rdf-schema#comment> "The collection of instances of #$AdjustableRateLoan that have a consistent adjustment period (c.f., #$adjustmentPeriod), e.g., the interest rate adjusts every 6 months." ;
	a <http://sw.cyc.com/2006/07/27/cyc/ObjectType> , <http://sw.cyc.com/2006/07/27/cyc/TemporalStuffType> ;
	<http://sw.cyc.com/2006/07/27/cyc/prettyString-Canonical> "adjustible rate loan with a consistent adjustment period" ;
	<http://sw.cyc.com/2006/07/27/cyc/prettyString> "adjustible rate loans with a consistent adjustment period" ;
	<http://www.w3.org/2000/01/rdf-schema#subClassOf> <http://sw.cyc.com/2006/07/27/cyc/AdjustableRateLoan> ;
	<http://sw.cyc.com/2006/07/27/cyc/facets-Generic> <http://sw.cyc.com/2006/07/27/cyc/AdjustableRateLoanTypeByAdjustmentPeriod> ;
	<http://sw.cyc.com/2006/07/27/cyc/requiredArg1Pred> <http://sw.cyc.com/2006/07/27/cyc/adjustmentPeriod> ;
	<http://sw.cyc.com/2006/07/27/cyc/facets-Partition> <http://sw.cyc.com/2006/07/27/cyc/AdjustableRateLoanTypeByAdjustmentPeriod> .

<http://sw.cyc.com/2006/07/27/cyc/AdjustableRateLoanTypeByAdjustmentPeriod> a <http://sw.cyc.com/2006/07/27/cyc/FacetingCollectionType> , <http://sw.cyc.com/2006/07/27/cyc/SecondOrderCollection> , <http://sw.cyc.com/2006/07/27/cyc/DisjointCollectionType> ;
	<http://sw.cyc.com/2006/07/27/cyc/prettyString-Canonical> "adjustable rate loan type by adjustment period" ;
	<http://www.w3.org/2000/01/rdf-schema#subClassOf> <http://sw.cyc.com/2006/07/27/cyc/TemporalStuffType> , <http://sw.cyc.com/2006/07/27/cyc/FacetInstanceCollection> ;
	<http://sw.cyc.com/2006/07/27/cyc/sharedNotes> <http://sw.cyc.com/2006/07/27/cyc/SharedNoteOnGenlsRelationsBetweenFacetingCollectionTypes> ;
	<http://sw.cyc.com/2006/07/27/cyc/typeGenls> <http://sw.cyc.com/2006/07/27/cyc/AdjustableRateLoan-ConsistentAdjustmentPeriod> .

<http://sw.cyc.com/2006/07/27/cyc/2000ShortageOfWorldSupplyOfOpium> a <http://sw.cyc.com/2006/07/27/cyc/Individual> , <http://sw.cyc.com/2006/07/27/cyc/Shortage> ;
	<http://sw.cyc.com/2006/07/27/cyc/prettyString-Canonical> "the marked reduction in the world supply of opium, from 2000 to 2002" .

<http://sw.cyc.com/2006/07/27/cyc/Shortage> <http://www.w3.org/2000/01/rdf-schema#comment> "A collection of events.  In each instance of #$Shortage, some            #$ProductType is #$inShortSupply.  For unexpected #$Shortages            use the more specialized collection #$SupplyShock." ;
	a <http://sw.cyc.com/2006/07/27/cyc/TemporalObjectType> ;
	<http://sw.cyc.com/2006/07/27/cyc/prettyString-Canonical> "shortage" ;
	<http://sw.cyc.com/2006/07/27/cyc/prettyString> "shortages" ;
	<http://www.w3.org/2000/01/rdf-schema#subClassOf> <http://sw.cyc.com/2006/07/27/cyc/Event> ;
	<http://sw.cyc.com/2006/07/27/cyc/requiredArg1Pred> <http://sw.cyc.com/2006/07/27/cyc/inShortSupply> .

<http://sw.cyc.com/2006/07/27/cyc/2001-ASpaceOdyssey-TheBook> a <http://sw.cyc.com/2006/07/27/cyc/Individual> , <http://sw.cyc.com/2006/07/27/cyc/Novel-CW> ;
	<http://sw.cyc.com/2006/07/27/cyc/prettyString-Canonical> "2001 A Space Odyssey" ;
	<http://sw.cyc.com/2006/07/27/cyc/prettyString> "2001" , "2001: A Space Odyssey" .

<http://sw.cyc.com/2006/07/27/cyc/208MotorizedRifleDivision-RRS> a <http://sw.cyc.com/2006/07/27/cyc/RedUnit> , <http://sw.cyc.com/2006/07/27/cyc/MotorizedRifleDivision> ;
	<http://sw.cyc.com/2006/07/27/cyc/prettyString-Canonical> "208th MRD" ;
	<http://sw.cyc.com/2006/07/27/cyc/quotedIsa> <http://sw.cyc.com/2006/07/27/cyc/FACToryIrrelevantTerm> .

<http://sw.cyc.com/2006/07/27/cyc/MotorizedRifleDivision> a <http://sw.cyc.com/2006/07/27/cyc/ExistingObjectType> , <http://sw.cyc.com/2006/07/27/cyc/GenericMilitaryOrganizations-Organization-Topic> , <http://sw.cyc.com/2006/07/27/cyc/MilitaryOrganizationConcept> ;
	<http://sw.cyc.com/2006/07/27/cyc/prettyString-Canonical> "motorized rifle division" ;
	<http://sw.cyc.com/2006/07/27/cyc/prettyString> "motorized rifle divisions" ;
	<http://www.w3.org/2000/01/rdf-schema#subClassOf> <http://sw.cyc.com/2006/07/27/cyc/Division-MilitaryEchelon> , <http://sw.cyc.com/2006/07/27/cyc/RifleUnit-MilitarySpecialty> .

<http://sw.cyc.com/2006/07/27/cyc/208thArtyRegt-RRS> a <http://sw.cyc.com/2006/07/27/cyc/Individual> , <http://sw.cyc.com/2006/07/27/cyc/RedUnit> , <http://sw.cyc.com/2006/07/27/cyc/Regiment-MilitaryEchelon> , <http://sw.cyc.com/2006/07/27/cyc/FieldArtilleryUnit-MilitarySpecialty> ;
	<http://sw.cyc.com/2006/07/27/cyc/prettyString-Canonical> "208thArty Regt" ;
	<http://sw.cyc.com/2006/07/27/cyc/quotedIsa> <http://sw.cyc.com/2006/07/27/cyc/FACToryIrrelevantTerm> .

<http://sw.cyc.com/2006/07/27/cyc/FieldArtilleryUnit-MilitarySpecialty> <http://www.w3.org/2000/01/rdf-schema#comment> "The collection of all military units trained and equipped for handling heavy           guns used for indirect fire against land-based targets." ;
	a <http://sw.cyc.com/2006/07/27/cyc/KEClarifyingCollectionType> , <http://sw.cyc.com/2006/07/27/cyc/MilitaryUnitSpecialtyType> , <http://sw.cyc.com/2006/07/27/cyc/GenericMilitaryOrganizations-Organization-Topic> , <http://sw.cyc.com/2006/07/27/cyc/MilitaryOrganizationConcept> , <http://sw.cyc.com/2006/07/27/cyc/CPOF-MilitaryUnitType> ;
	<http://sw.cyc.com/2006/07/27/cyc/prettyString-Canonical> "field artillery unit" ;
	<http://sw.cyc.com/2006/07/27/cyc/prettyString> "field artillery units" ;
	<http://www.w3.org/2000/01/rdf-schema#subClassOf> <http://sw.cyc.com/2006/07/27/cyc/ModernMilitaryUnit-Deployable> , <http://sw.cyc.com/2006/07/27/cyc/ArtilleryUnit-MilitarySpecialty> , <http://sw.cyc.com/2006/07/27/cyc/CPOF-MilitaryUnit> .

<http://sw.cyc.com/2006/07/27/cyc/208thTankRegiment-RRS> a <http://sw.cyc.com/2006/07/27/cyc/Individual> , <http://sw.cyc.com/2006/07/27/cyc/RedUnit> , <http://sw.cyc.com/2006/07/27/cyc/Regiment-MilitaryEchelon> , <http://sw.cyc.com/2006/07/27/cyc/ArmoredUnit-MilitarySpecialty> ;
	<http://sw.cyc.com/2006/07/27/cyc/prettyString-Canonical> "208th TR" ;
	<http://sw.cyc.com/2006/07/27/cyc/quotedIsa> <http://sw.cyc.com/2006/07/27/cyc/FACToryIrrelevantTerm> .

<http://sw.cyc.com/2006/07/27/cyc/ArmoredUnit-MilitarySpecialty> <http://www.w3.org/2000/01/rdf-schema#comment> "The collection of all military units that employ motorized vehicles engineered to resist           penetration by explosives and projectile weapons. In modern armed           forces, it usually entails the presence of tanks and heavy artillery." ;
	a <http://sw.cyc.com/2006/07/27/cyc/KEClarifyingCollectionType> , <http://sw.cyc.com/2006/07/27/cyc/MilitaryUnitSpecialtyType> , <http://sw.cyc.com/2006/07/27/cyc/GenericMilitaryOrganizations-Organization-Topic> , <http://sw.cyc.com/2006/07/27/cyc/MilitaryOrganizationConcept> , <http://sw.cyc.com/2006/07/27/cyc/CPOF-UnitSpecialtyClassificationType> ;
	<http://sw.cyc.com/2006/07/27/cyc/prettyString-Canonical> "armored unit" ;
	<http://sw.cyc.com/2006/07/27/cyc/prettyString> "tank unit" , "tank units" , "armored units" ;
	<http://www.w3.org/2000/01/rdf-schema#subClassOf> <http://sw.cyc.com/2006/07/27/cyc/ManeuverUnit-MilitarySpecialty> , <http://sw.cyc.com/2006/07/27/cyc/ModernMilitaryUnit-Deployable> , <http://sw.cyc.com/2006/07/27/cyc/HeavyForce> .

<http://sw.cyc.com/2006/07/27/cyc/208TRRegimentHQ-RRS> a <http://sw.cyc.com/2006/07/27/cyc/Individual> , <http://sw.cyc.com/2006/07/27/cyc/Platoon-MilitaryEchelon> , <http://sw.cyc.com/2006/07/27/cyc/CommandUnit-MilitarySpecialty> , <http://sw.cyc.com/2006/07/27/cyc/RedUnit> ;
	<http://sw.cyc.com/2006/07/27/cyc/prettyString-Canonical> "HQ/208 TR" ;
	<http://sw.cyc.com/2006/07/27/cyc/quotedIsa> <http://sw.cyc.com/2006/07/27/cyc/FACToryIrrelevantTerm> .

<http://sw.cyc.com/2006/07/27/cyc/20BroadStreet> <http://www.w3.org/2000/01/rdf-schema#comment> "20 Broad Street is the headquarters of the #$NewYorkStockExchange.  It is the building in which the organization hosts its main trading floor." ;
	a <http://sw.cyc.com/2006/07/27/cyc/OfficeBuilding> , <http://sw.cyc.com/2006/07/27/cyc/CommercialFacility> ;
	<http://sw.cyc.com/2006/07/27/cyc/prettyString-Canonical> "20 Broad Street" ;
	<http://sw.cyc.com/2006/07/27/cyc/quotedIsa> <http://sw.cyc.com/2006/07/27/cyc/FACToryIrrelevantTerm> .

<http://sw.cyc.com/2006/07/27/cyc/CommercialFacility> <http://www.w3.org/2000/01/rdf-schema#comment> "The collection of all #$ConstructionArtifacts that are dedicated to serving as the #$physicalQuarters of some #$CommercialOrganization." ;
	a <http://sw.cyc.com/2006/07/27/cyc/ExistingObjectType> , <http://sw.cyc.com/2006/07/27/cyc/SpatiallyDisjointObjectType> ;
	<http://sw.cyc.com/2006/07/27/cyc/prettyString-Canonical> "commercial facility" ;
	<http://sw.cyc.com/2006/07/27/cyc/prettyString> "the physical quarters of commercial organizations" , "commercial facilities" ;
	<http://www.w3.org/2000/01/rdf-schema#subClassOf> <http://sw.cyc.com/2006/07/27/cyc/ConstructionArtifact> , <http://sw.cyc.com/2006/07/27/cyc/Workplace> , <http://sw.cyc.com/2006/07/27/cyc/Facility-Generic> .

<http://sw.cyc.com/2006/07/27/cyc/20InchTelevisionSet> a <http://sw.cyc.com/2006/07/27/cyc/ExistingObjectType> , <http://sw.cyc.com/2006/07/27/cyc/SpatiallyDisjointObjectType> , <http://sw.cyc.com/2006/07/27/cyc/TelevisionSetTypeBySize> ;
	<http://sw.cyc.com/2006/07/27/cyc/prettyString-Canonical> "20 inch television set" ;
	<http://sw.cyc.com/2006/07/27/cyc/prettyString> "20 inch television sets" ;
	<http://www.w3.org/2000/01/rdf-schema#subClassOf> <http://sw.cyc.com/2006/07/27/cyc/ManufacturedGoods> , <http://sw.cyc.com/2006/07/27/cyc/TelevisionSet> .

<http://sw.cyc.com/2006/07/27/cyc/20thCenturyIndustries> a <http://sw.cyc.com/2006/07/27/cyc/Individual> , <http://sw.cyc.com/2006/07/27/cyc/PubliclyHeldCorporation> ;
	<http://sw.cyc.com/2006/07/27/cyc/prettyString-Canonical> "20th Century Industries" .

<http://sw.cyc.com/2006/07/27/cyc/20thCenturyTriviaChallenge-TheGame> a <http://sw.cyc.com/2006/07/27/cyc/Individual> , <http://sw.cyc.com/2006/07/27/cyc/UnversionedProgram> , <http://sw.cyc.com/2006/07/27/cyc/ComputerGameProgram> ;
	<http://sw.cyc.com/2006/07/27/cyc/prettyString-Canonical> "the game 20th Century Trivia Challenge" .

<http://sw.cyc.com/2006/07/27/cyc/20thMRD> a <http://sw.cyc.com/2006/07/27/cyc/RedUnit> , <http://sw.cyc.com/2006/07/27/cyc/MotorizedRifleDivision> ;
	<http://sw.cyc.com/2006/07/27/cyc/prettyString-Canonical> "the 20th Motorized Rifle Division" ;
	<http://sw.cyc.com/2006/07/27/cyc/prettyString> "the Red 20th Motorized Infantry Division" , "the 20th Red Motorized Rifle Division" .

<http://sw.cyc.com/2006/07/27/cyc/21cSagemanDataGroup2> <http://www.w3.org/2000/01/rdf-schema#comment> "The second collection of groups from 21c." ;
	a <http://www.w3.org/2002/07/owl#Class> , <http://sw.cyc.com/2006/07/27/cyc/NonAbducibleCollection> ;
	<http://www.w3.org/2000/01/rdf-schema#subClassOf> <http://sw.cyc.com/2006/07/27/cyc/Group> .

<http://sw.cyc.com/2006/07/27/cyc/Group> <http://www.w3.org/2000/01/rdf-schema#comment> "A collection of temporal objects.  Each instance of #$Group is a composite object made up of one or more individual objects or events.  A group is related to each of its members by the predicate #$groupMembers (q.v.).  Note that instances of #$Group are <i>not</i> collections.  A group has temporal extent and might have spatial location, while a collection is timeless and nonspatial.  It is of course possible to define a collection parallel to any given group, so that the instances of the collection are exactly the group-members of that group; e.g. each toe on my left foot (and nothing else) is both an instance of the collection of my left toes and a member of the group of toes on my left foot.  But that group (of my left toes) is a spatiotemporal thing while the correlated collection (of my left toes) is not.  Similarly, if a certain flock of pigeons is considered as having a location, a spatial extent, and a time of existence, then the flock is being considered a <i>group</i> and not a collection.  Finally, unlike a collection, a group cannot be empty, but must have <i>at least one</i> group-member.  As a default, a group whose group-members all are instances of #$SomethingExisting is itself an instance of #$SomethingExisting, and a group whose group-members all are #$Events is itself an #$Event.  Instances of #$Group include #$QueensGuard, #$ThreeWiseMen, #$SantasReindeer, and #$InternationalCommunity." ;
	a <http://sw.cyc.com/2006/07/27/cyc/FirstOrderCollection> , <http://sw.cyc.com/2006/07/27/cyc/KEClarifyingCollectionType> , <http://sw.cyc.com/2006/07/27/cyc/Group-Topic> ;
	<http://sw.cyc.com/2006/07/27/cyc/prettyString-Canonical> "group of things" ;
	<http://sw.cyc.com/2006/07/27/cyc/prettyString> "GROUP" , "cluster" , "assemblage" , "assemblages" , "groups" , "grouping" , "groupings" , "clusters" , "litany" , "groups of things" ;
	<http://www.w3.org/2000/01/rdf-schema#subClassOf> <http://sw.cyc.com/2006/07/27/cyc/TemporalThing> .

<http://sw.cyc.com/2006/07/27/cyc/NonAbducibleCollection> <http://www.w3.org/2000/01/rdf-schema#comment> """The collection #$NonAbducibleCollection is a sub-collection of 
#$SetOrCollection.  Abductive inferences sometimes involve hypothesizing 
the existence of entities as part of the explanation of some assertion or 
set of assertions. Cyc will not hypothesize the existence of instances of 
the collections that are instances of #$NonAbducibleCollection.  Roughly, 
abductive inferences consume conceptual / theoretical knowledge rather 
than produce it.  So, #$SecondOrderCollection is an instance of 
#$NonAbducibleCollection because Cyc should be employing existing 
theoretical knowledge about instances of #$SecondOrderCollection rather 
than hypothesizing new instances.""" ;
	a <http://sw.cyc.com/2006/07/27/cyc/VariedOrderCollection> ;
	<http://sw.cyc.com/2006/07/27/cyc/prettyString-Canonical> "non abducible collection" ;
	<http://www.w3.org/2000/01/rdf-schema#subClassOf> <http://sw.cyc.com/2006/07/27/cyc/SetOrCollection> ;
	<http://sw.cyc.com/2006/07/27/cyc/quotedIsa> <http://sw.cyc.com/2006/07/27/cyc/AbductionConstraintConstant> .

<http://sw.cyc.com/2006/07/27/cyc/21cSagemanDataGroup> a <http://www.w3.org/2002/07/owl#Class> , <http://sw.cyc.com/2006/07/27/cyc/NonAbducibleCollection> ;
	<http://sw.cyc.com/2006/07/27/cyc/prettyString-Canonical> "21c sageman data group" ;
	<http://www.w3.org/2000/01/rdf-schema#subClassOf> <http://sw.cyc.com/2006/07/27/cyc/Group> .

<http://sw.cyc.com/2006/07/27/cyc/21cSNATrustNetwork> <http://www.w3.org/2000/01/rdf-schema#comment> "The collection of groups each of which is a candidate for being a \"trust network\"." ;
	a <http://www.w3.org/2002/07/owl#Class> ;
	<http://sw.cyc.com/2006/07/27/cyc/prettyString-Canonical> "21c SNA trust network" ;
	<http://www.w3.org/2000/01/rdf-schema#subClassOf> <http://sw.cyc.com/2006/07/27/cyc/Group> .

<http://sw.cyc.com/2006/07/27/cyc/21cTestGroup10> <http://www.w3.org/2000/01/rdf-schema#comment> "21c group  10    ." ;
	a <http://sw.cyc.com/2006/07/27/cyc/Group> , <http://sw.cyc.com/2006/07/27/cyc/21cSagemanDataGroup> ;
	<http://sw.cyc.com/2006/07/27/cyc/prettyString-Canonical> "21c Test Group 10" .

<http://sw.cyc.com/2006/07/27/cyc/21cTestGroup11> <http://www.w3.org/2000/01/rdf-schema#comment> "21c group 11     ." ;
	a <http://sw.cyc.com/2006/07/27/cyc/Group> , <http://sw.cyc.com/2006/07/27/cyc/21cSagemanDataGroup> ;
	<http://sw.cyc.com/2006/07/27/cyc/prettyString-Canonical> "21c Test Group 11" .

<http://sw.cyc.com/2006/07/27/cyc/21cTestGroup12> <http://www.w3.org/2000/01/rdf-schema#comment> "21c group 12    ." ;
	a <http://sw.cyc.com/2006/07/27/cyc/Group> , <http://sw.cyc.com/2006/07/27/cyc/21cSagemanDataGroup> ;
	<http://sw.cyc.com/2006/07/27/cyc/prettyString-Canonical> "21c Test Group 12" .

<http://sw.cyc.com/2006/07/27/cyc/21cTestGroup1> <http://www.w3.org/2000/01/rdf-schema#comment> "21c group 1." ;
	a <http://sw.cyc.com/2006/07/27/cyc/Group> , <http://sw.cyc.com/2006/07/27/cyc/21cSagemanDataGroup> ;
	<http://sw.cyc.com/2006/07/27/cyc/prettyString-Canonical> "21c Test Group 1" .

<http://sw.cyc.com/2006/07/27/cyc/21cTestGroup2-0> <http://www.w3.org/2000/01/rdf-schema#comment> "21c group2 0   ." ;
	a <http://sw.cyc.com/2006/07/27/cyc/21cSagemanDataGroup2> , <http://sw.cyc.com/2006/07/27/cyc/Group> ;
	<http://sw.cyc.com/2006/07/27/cyc/prettyString-Canonical> "21c Test Group 2 0" .

<http://sw.cyc.com/2006/07/27/cyc/21cTestGroup2-10> <http://www.w3.org/2000/01/rdf-schema#comment> "21c group2 10  ." ;
	a <http://sw.cyc.com/2006/07/27/cyc/21cSagemanDataGroup2> , <http://sw.cyc.com/2006/07/27/cyc/Group> ;
	<http://sw.cyc.com/2006/07/27/cyc/prettyString-Canonical> "21c Test Group 2 10" .

<http://sw.cyc.com/2006/07/27/cyc/21cTestGroup2-11> <http://www.w3.org/2000/01/rdf-schema#comment> "21c group2 11   ." ;
	a <http://sw.cyc.com/2006/07/27/cyc/21cSagemanDataGroup2> , <http://sw.cyc.com/2006/07/27/cyc/Group> ;
	<http://sw.cyc.com/2006/07/27/cyc/prettyString-Canonical> "21c Test Group 2 11" .

<http://sw.cyc.com/2006/07/27/cyc/21cTestGroup2-12> <http://www.w3.org/2000/01/rdf-schema#comment> "21c group2 12  ." ;
	a <http://sw.cyc.com/2006/07/27/cyc/21cSagemanDataGroup2> , <http://sw.cyc.com/2006/07/27/cyc/Group> ;
	<http://sw.cyc.com/2006/07/27/cyc/prettyString-Canonical> "21c Test Group 2 12" .

<http://sw.cyc.com/2006/07/27/cyc/21cTestGroup2-13> <http://www.w3.org/2000/01/rdf-schema#comment> "21c group2 13  ." ;
	a <http://sw.cyc.com/2006/07/27/cyc/21cSagemanDataGroup2> , <http://sw.cyc.com/2006/07/27/cyc/Group> ;
	<http://sw.cyc.com/2006/07/27/cyc/prettyString-Canonical> "21c Test Group 2 13" .

<http://sw.cyc.com/2006/07/27/cyc/21cTestGroup2-1> <http://www.w3.org/2000/01/rdf-schema#comment> "21c group2 1  ." ;
	a <http://sw.cyc.com/2006/07/27/cyc/21cSagemanDataGroup2> , <http://sw.cyc.com/2006/07/27/cyc/Group> ;
	<http://sw.cyc.com/2006/07/27/cyc/prettyString-Canonical> "21c Test Group 2 1" .

<http://sw.cyc.com/2006/07/27/cyc/21cTestGroup2-2> a <http://sw.cyc.com/2006/07/27/cyc/21cSagemanDataGroup2> , <http://sw.cyc.com/2006/07/27/cyc/Group> ;
	<http://sw.cyc.com/2006/07/27/cyc/prettyString-Canonical> "21c Test Group 2 2" .

<http://sw.cyc.com/2006/07/27/cyc/21cTestGroup2-3> <http://www.w3.org/2000/01/rdf-schema#comment> "21c group2 3  ." ;
	a <http://sw.cyc.com/2006/07/27/cyc/21cSagemanDataGroup2> , <http://sw.cyc.com/2006/07/27/cyc/Group> ;
	<http://sw.cyc.com/2006/07/27/cyc/prettyString-Canonical> "21c Test Group 2 3" .

<http://sw.cyc.com/2006/07/27/cyc/21cTestGroup2-4> <http://www.w3.org/2000/01/rdf-schema#comment> "21c group2 4  ." ;
	a <http://sw.cyc.com/2006/07/27/cyc/21cSagemanDataGroup2> , <http://sw.cyc.com/2006/07/27/cyc/Group> ;
	<http://sw.cyc.com/2006/07/27/cyc/prettyString-Canonical> "21c Test Group 2 4" .

<http://sw.cyc.com/2006/07/27/cyc/21cTestGroup2-5> <http://www.w3.org/2000/01/rdf-schema#comment> "21c group2 5   ." ;
	a <http://sw.cyc.com/2006/07/27/cyc/21cSagemanDataGroup2> , <http://sw.cyc.com/2006/07/27/cyc/Group> ;
	<http://sw.cyc.com/2006/07/27/cyc/prettyString-Canonical> "21c Test Group 2 5" .

<http://sw.cyc.com/2006/07/27/cyc/21cTestGroup2-6> <http://www.w3.org/2000/01/rdf-schema#comment> "21c group2 6   ." ;
	a <http://sw.cyc.com/2006/07/27/cyc/21cSagemanDataGroup2> , <http://sw.cyc.com/2006/07/27/cyc/Group> ;
	<http://sw.cyc.com/2006/07/27/cyc/prettyString-Canonical> "21c Test Group 2 6" .

<http://sw.cyc.com/2006/07/27/cyc/21cTestGroup2-7> <http://www.w3.org/2000/01/rdf-schema#comment> "21c group2 7  ." ;
	a <http://sw.cyc.com/2006/07/27/cyc/21cSagemanDataGroup2> , <http://sw.cyc.com/2006/07/27/cyc/Group> ;
	<http://sw.cyc.com/2006/07/27/cyc/prettyString-Canonical> "21c Test Group 2 7" .

<http://sw.cyc.com/2006/07/27/cyc/21cTestGroup2-8> <http://www.w3.org/2000/01/rdf-schema#comment> "21c group2 8  ." ;
	a <http://sw.cyc.com/2006/07/27/cyc/21cSagemanDataGroup2> , <http://sw.cyc.com/2006/07/27/cyc/Group> ;
	<http://sw.cyc.com/2006/07/27/cyc/prettyString-Canonical> "21c Test Group 2 8" .

<http://sw.cyc.com/2006/07/27/cyc/21cTestGroup2-9> <http://www.w3.org/2000/01/rdf-schema#comment> "21c group2 9  ." ;
	a <http://sw.cyc.com/2006/07/27/cyc/21cSagemanDataGroup2> , <http://sw.cyc.com/2006/07/27/cyc/Group> ;
	<http://sw.cyc.com/2006/07/27/cyc/prettyString-Canonical> "21c Test Group 2 9" .

<http://sw.cyc.com/2006/07/27/cyc/21cTestGroup2> <http://www.w3.org/2000/01/rdf-schema#comment> "21c group 2     ." ;
	a <http://sw.cyc.com/2006/07/27/cyc/Group> , <http://sw.cyc.com/2006/07/27/cyc/21cSagemanDataGroup> ;
	<http://sw.cyc.com/2006/07/27/cyc/prettyString-Canonical> "21c Test Group 2" .

<http://sw.cyc.com/2006/07/27/cyc/21cTestGroup3> <http://www.w3.org/2000/01/rdf-schema#comment> "21c group 3     ." ;
	a <http://sw.cyc.com/2006/07/27/cyc/Group> , <http://sw.cyc.com/2006/07/27/cyc/21cSagemanDataGroup> ;
	<http://sw.cyc.com/2006/07/27/cyc/prettyString-Canonical> "21c Test Group 3" .

<http://sw.cyc.com/2006/07/27/cyc/21cTestGroup4> <http://www.w3.org/2000/01/rdf-schema#comment> "21c group 4     ." ;
	a <http://sw.cyc.com/2006/07/27/cyc/Group> , <http://sw.cyc.com/2006/07/27/cyc/21cSagemanDataGroup> ;
	<http://sw.cyc.com/2006/07/27/cyc/prettyString-Canonical> "21c Test Group 4" .

<http://sw.cyc.com/2006/07/27/cyc/21cTestGroup5> <http://www.w3.org/2000/01/rdf-schema#comment> "21c group 5    ." ;
	a <http://sw.cyc.com/2006/07/27/cyc/Group> , <http://sw.cyc.com/2006/07/27/cyc/21cSagemanDataGroup> ;
	<http://sw.cyc.com/2006/07/27/cyc/prettyString-Canonical> "21c Test Group 5" .

<http://sw.cyc.com/2006/07/27/cyc/21cTestGroup6> <http://www.w3.org/2000/01/rdf-schema#comment> "21c group 6     ." ;
	a <http://sw.cyc.com/2006/07/27/cyc/Group> ;
	<http://sw.cyc.com/2006/07/27/cyc/prettyString-Canonical> "21c Test Group 6" .

<http://sw.cyc.com/2006/07/27/cyc/21cTestGroup7> <http://www.w3.org/2000/01/rdf-schema#comment> "21c group 7    ." ;
	a <http://sw.cyc.com/2006/07/27/cyc/Group> , <http://sw.cyc.com/2006/07/27/cyc/21cSagemanDataGroup> ;
	<http://sw.cyc.com/2006/07/27/cyc/prettyString-Canonical> "21c Test Group 7" .

<http://sw.cyc.com/2006/07/27/cyc/21cTestGroup8> <http://www.w3.org/2000/01/rdf-schema#comment> "21c group 8     ." ;
	a <http://sw.cyc.com/2006/07/27/cyc/Group> , <http://sw.cyc.com/2006/07/27/cyc/21cSagemanDataGroup> ;
	<http://sw.cyc.com/2006/07/27/cyc/prettyString-Canonical> "21c Test Group 8" .

<http://sw.cyc.com/2006/07/27/cyc/21cTestGroup9> <http://www.w3.org/2000/01/rdf-schema#comment> "21c group 9      ." ;
	a <http://sw.cyc.com/2006/07/27/cyc/Group> , <http://sw.cyc.com/2006/07/27/cyc/21cSagemanDataGroup> ;
	<http://sw.cyc.com/2006/07/27/cyc/prettyString-Canonical> "21c Test Group 9" .

<http://sw.cyc.com/2006/07/27/cyc/21JumpStreet-TheTVShow> a <http://sw.cyc.com/2006/07/27/cyc/Individual> , <http://sw.cyc.com/2006/07/27/cyc/TVSeriesProduct> ;
	<http://sw.cyc.com/2006/07/27/cyc/prettyString-Canonical> "21 Jump Street" .

<http://sw.cyc.com/2006/07/27/cyc/TVSeriesProduct> <http://www.w3.org/2000/01/rdf-schema#comment> "The collection of all TV series considered as #$ConceptualWorks.  Each instance of #$TVSeriesProduct has a (large) number of instances of #$TVShow-SingleCW as #$subWorks." ;
	a <http://sw.cyc.com/2006/07/27/cyc/ObjectType> , <http://sw.cyc.com/2006/07/27/cyc/AtemporalNecessarilyEssentialCollectionType> , <http://sw.cyc.com/2006/07/27/cyc/KEClarifyingCollectionType> ;
	<http://sw.cyc.com/2006/07/27/cyc/prettyString-Canonical> "television series" ;
	<http://sw.cyc.com/2006/07/27/cyc/prettyString> "TV series" , "T.V. series" ;
	<http://www.w3.org/2000/01/rdf-schema#subClassOf> <http://sw.cyc.com/2006/07/27/cyc/TVShow-CW> , <http://sw.cyc.com/2006/07/27/cyc/BroadcastSeriesProduct> .

<http://sw.cyc.com/2006/07/27/cyc/21stCenturyHoldingCompany> a <http://sw.cyc.com/2006/07/27/cyc/Individual> , <http://sw.cyc.com/2006/07/27/cyc/PubliclyHeldCorporation> ;
	<http://sw.cyc.com/2006/07/27/cyc/prettyString-Canonical> "21st Century Holding Company" .

<http://sw.cyc.com/2006/07/27/cyc/23rdArmoredDivision> a <http://sw.cyc.com/2006/07/27/cyc/BlueUnit> , <http://sw.cyc.com/2006/07/27/cyc/ArmoredDivision> ;
	<http://sw.cyc.com/2006/07/27/cyc/prettyString-Canonical> "the 23rd Armored Division" ;
	<http://sw.cyc.com/2006/07/27/cyc/prettyString> "the Blue 23rd Armd Div" , "the 23rd Blue Armd Div" , "the 23rd Armd Div" , "the 23rd Blue Armored Division" , "the Blue 23rd Armored Division" .

<http://sw.cyc.com/2006/07/27/cyc/ArmoredDivision> <http://www.w3.org/2000/01/rdf-schema#comment> """The collection of all echelons at the division level that
include armorded units within their ranks.""" ;
	a <http://sw.cyc.com/2006/07/27/cyc/ExistingObjectType> , <http://sw.cyc.com/2006/07/27/cyc/GenericMilitaryOrganizations-Organization-Topic> , <http://sw.cyc.com/2006/07/27/cyc/MilitaryOrganizationConcept> ;
	<http://sw.cyc.com/2006/07/27/cyc/prettyString-Canonical> "armored division" ;
	<http://sw.cyc.com/2006/07/27/cyc/prettyString> "tank division" , "tank divisions" , "armored divisions" ;
	<http://www.w3.org/2000/01/rdf-schema#subClassOf> <http://sw.cyc.com/2006/07/27/cyc/ArmoredUnit-MilitarySpecialty> , <http://sw.cyc.com/2006/07/27/cyc/Division-MilitaryEchelon> .

<http://sw.cyc.com/2006/07/27/cyc/247MediaInc> a <http://sw.cyc.com/2006/07/27/cyc/Individual> , <http://sw.cyc.com/2006/07/27/cyc/PubliclyHeldCorporation> ;
	<http://sw.cyc.com/2006/07/27/cyc/prettyString-Canonical> "247 Media Inc" .

<http://sw.cyc.com/2006/07/27/cyc/24-tolueneDiisocyanate> a <http://sw.cyc.com/2006/07/27/cyc/ChemicalCompoundTypeByChemicalSpecies> , <http://sw.cyc.com/2006/07/27/cyc/TemporallyExistingThingTypeFrequentlyForSale> ;
	<http://sw.cyc.com/2006/07/27/cyc/prettyString-Canonical> "2,4-tolueneDiisocyanate" ;
	<http://www.w3.org/2000/01/rdf-schema#subClassOf> <http://sw.cyc.com/2006/07/27/cyc/PartiallyTangible> .

<http://sw.cyc.com/2006/07/27/cyc/25InchTelevisionSet> a <http://sw.cyc.com/2006/07/27/cyc/ExistingObjectType> , <http://sw.cyc.com/2006/07/27/cyc/SpatiallyDisjointObjectType> , <http://sw.cyc.com/2006/07/27/cyc/TelevisionSetTypeBySize> ;
	<http://sw.cyc.com/2006/07/27/cyc/prettyString-Canonical> "25 inch television set" ;
	<http://sw.cyc.com/2006/07/27/cyc/prettyString> "25 inch television sets" .

<http://sw.cyc.com/2006/07/27/cyc/25thInfantryDivision-Light-Washington> a <http://sw.cyc.com/2006/07/27/cyc/Brigade-MilitaryEchelon> , <http://sw.cyc.com/2006/07/27/cyc/LightMechanizedUnit-MilitarySpecialty> , <http://sw.cyc.com/2006/07/27/cyc/ModernMilitaryUnit-Deployable> , <http://sw.cyc.com/2006/07/27/cyc/UnitedStatesMilitaryOrganization> ;
	<http://sw.cyc.com/2006/07/27/cyc/prettyString-Canonical> "25th Infantry Division (Light), Washington" .

<http://sw.cyc.com/2006/07/27/cyc/27InchTelevisionSet> a <http://sw.cyc.com/2006/07/27/cyc/ExistingObjectType> , <http://sw.cyc.com/2006/07/27/cyc/SpatiallyDisjointObjectType> , <http://sw.cyc.com/2006/07/27/cyc/TelevisionSetTypeBySize> ;
	<http://sw.cyc.com/2006/07/27/cyc/prettyString-Canonical> "27 inch television set" ;
	<http://sw.cyc.com/2006/07/27/cyc/prettyString> "27 inch television sets" ;
	<http://www.w3.org/2000/01/rdf-schema#subClassOf> <http://sw.cyc.com/2006/07/27/cyc/ManufacturedGoods> , <http://sw.cyc.com/2006/07/27/cyc/TelevisionSet> .

<http://sw.cyc.com/2006/07/27/cyc/28DaysLater-TheMovie> a <http://sw.cyc.com/2006/07/27/cyc/Individual> , <http://sw.cyc.com/2006/07/27/cyc/Movie-CW> , <http://sw.cyc.com/2006/07/27/cyc/PropositionalConceptualWork-ThrillerGenre> , <http://sw.cyc.com/2006/07/27/cyc/PropositionalConceptualWork-ScienceFictionGenre> , <http://sw.cyc.com/2006/07/27/cyc/PropositionalConceptualWork-HorrorGenre> ;
	<http://sw.cyc.com/2006/07/27/cyc/prettyString-Canonical> "28 Days Later..." .

<http://sw.cyc.com/2006/07/27/cyc/PropositionalConceptualWork-ThrillerGenre> <http://www.w3.org/2000/01/rdf-schema#comment> """The collection of instances of #$PropositionalConceptualWork that are of the 
thriller genre. #$AlfredHitchcock's #$Psycho-TheMovie is an example of a 
movie in this genre.      """ ;
	a <http://sw.cyc.com/2006/07/27/cyc/PCWTypeByGenre> ;
	<http://sw.cyc.com/2006/07/27/cyc/prettyString-Canonical> "thriller" ;
	<http://sw.cyc.com/2006/07/27/cyc/prettyString> "thrillers" ;
	<http://www.w3.org/2000/01/rdf-schema#subClassOf> <http://sw.cyc.com/2006/07/27/cyc/PropositionalConceptualWork> .

<http://sw.cyc.com/2006/07/27/cyc/PropositionalConceptualWork-ScienceFictionGenre> <http://www.w3.org/2000/01/rdf-schema#comment> """The collection of instances of #$PropositionalConceptualWork that are of the
science fiction genre.  #$RobertHeinlein and #$IsaacAsimov are famous writers of this genre.
<p>""" ;
	a <http://sw.cyc.com/2006/07/27/cyc/PCWTypeByGenre> ;
	<http://sw.cyc.com/2006/07/27/cyc/prettyString-Canonical> "science fiction" ;
	<http://sw.cyc.com/2006/07/27/cyc/prettyString> "sci-fi storey" , "sci-fi story" , "sci-fi stories" ;
	<http://www.w3.org/2000/01/rdf-schema#subClassOf> <http://sw.cyc.com/2006/07/27/cyc/PropositionalConceptualWork> .

<http://sw.cyc.com/2006/07/27/cyc/PropositionalConceptualWork-HorrorGenre> <http://www.w3.org/2000/01/rdf-schema#comment> "The collection of instances of #$PropositionalConceptualWork that are of the  horror genre.  #$JohnCarpenter-MovieDirector's #$Halloween-TheMovie is an example of a movie  in this genre.       " ;
	a <http://sw.cyc.com/2006/07/27/cyc/PCWTypeByGenre> ;
	<http://sw.cyc.com/2006/07/27/cyc/prettyString-Canonical> "horror work" ;
	<http://sw.cyc.com/2006/07/27/cyc/prettyString> "horror works" ;
	<http://www.w3.org/2000/01/rdf-schema#subClassOf> <http://sw.cyc.com/2006/07/27/cyc/PropositionalConceptualWork> .

<http://sw.cyc.com/2006/07/27/cyc/29InchTelevisionSet> a <http://sw.cyc.com/2006/07/27/cyc/ExistingObjectType> , <http://sw.cyc.com/2006/07/27/cyc/SpatiallyDisjointObjectType> , <http://sw.cyc.com/2006/07/27/cyc/TelevisionSetTypeBySize> ;
	<http://sw.cyc.com/2006/07/27/cyc/prettyString-Canonical> "29 inch television set" ;
	<http://sw.cyc.com/2006/07/27/cyc/prettyString> "29 inch television sets" ;
	<http://www.w3.org/2000/01/rdf-schema#subClassOf> <http://sw.cyc.com/2006/07/27/cyc/ManufacturedGoods> , <http://sw.cyc.com/2006/07/27/cyc/TelevisionSet> .

<http://sw.cyc.com/2006/07/27/cyc/29thGuardsTankDivision> a <http://sw.cyc.com/2006/07/27/cyc/RedUnit> , <http://sw.cyc.com/2006/07/27/cyc/ArmoredDivision> ;
	<http://sw.cyc.com/2006/07/27/cyc/prettyString-Canonical> "the 29th Guards Tank Division" ;
	<http://sw.cyc.com/2006/07/27/cyc/prettyString> "the Red 29th Guards Tank Division" , "the 29th Red Guards Tank Division" .

<http://sw.cyc.com/2006/07/27/cyc/2AMBackgammon-TheGame> a <http://sw.cyc.com/2006/07/27/cyc/Individual> , <http://sw.cyc.com/2006/07/27/cyc/OnlineGameProgram> , <http://sw.cyc.com/2006/07/27/cyc/PuzzleGameProgram> ;
	<http://sw.cyc.com/2006/07/27/cyc/prettyString-Canonical> "2AM Backgammon" .

<http://sw.cyc.com/2006/07/27/cyc/PuzzleGameProgram> <http://www.w3.org/2000/01/rdf-schema#comment> "The collection of all  #$ComputerGamePrograms that are simulated versions of puzzles." ;
	a <http://sw.cyc.com/2006/07/27/cyc/KEClarifyingCollectionType> , <http://sw.cyc.com/2006/07/27/cyc/ComputerProgramTypeByFunction> ;
	<http://sw.cyc.com/2006/07/27/cyc/prettyString-Canonical> "puzzle computer game" ;
	<http://sw.cyc.com/2006/07/27/cyc/prettyString> "puzzle" , "puzzles" , "puzzle computer games" ;
	<http://www.w3.org/2000/01/rdf-schema#subClassOf> <http://sw.cyc.com/2006/07/27/cyc/ComputerGameProgram> .

<http://sw.cyc.com/2006/07/27/cyc/2AMChess-TheGame> a <http://sw.cyc.com/2006/07/27/cyc/Individual> , <http://sw.cyc.com/2006/07/27/cyc/OnlineGameProgram> , <http://sw.cyc.com/2006/07/27/cyc/PuzzleGameProgram> ;
	<http://sw.cyc.com/2006/07/27/cyc/prettyString-Canonical> "2AM Chess" .

<http://sw.cyc.com/2006/07/27/cyc/2AMInc> a <http://sw.cyc.com/2006/07/27/cyc/Individual> , <http://sw.cyc.com/2006/07/27/cyc/SoftwareVendor> ;
	<http://sw.cyc.com/2006/07/27/cyc/prettyString-Canonical> "2AM Inc." .

<http://sw.cyc.com/2006/07/27/cyc/2AMPoker-TheGame> a <http://sw.cyc.com/2006/07/27/cyc/Individual> , <http://sw.cyc.com/2006/07/27/cyc/PuzzleGameProgram> ;
	<http://sw.cyc.com/2006/07/27/cyc/prettyString-Canonical> "2AM Poker" .

<http://sw.cyc.com/2006/07/27/cyc/2Amys-FoodServiceEstablishment> <http://sw.cyc.com/2006/07/27/cyc/prettyString-Canonical> "2 Amys" .

<http://sw.cyc.com/2006/07/27/cyc/2ByteIntegerDatatype> <http://www.w3.org/2000/01/rdf-schema#comment> "The collection of all computer data types that employ exactly 2 bytes to represent some subset of the integers or values related to represnting integer values such as NAN. Note that this does not specify, for example, whether the data type represents positive integers only, or is in two's complement representation." ;
	a <http://sw.cyc.com/2006/07/27/cyc/FixedSizeComputerDatatypeType> , <http://sw.cyc.com/2006/07/27/cyc/SKSIDataTypeDescriptions-Topic> ;
	<http://sw.cyc.com/2006/07/27/cyc/prettyString-Canonical> "2-byte integer" ;
	<http://sw.cyc.com/2006/07/27/cyc/prettyString> "two-byte integers" , "2-byte integers" ;
	<http://www.w3.org/2000/01/rdf-schema#subClassOf> <http://sw.cyc.com/2006/07/27/cyc/IntegerComputerNumber> , <http://sw.cyc.com/2006/07/27/cyc/ProgramObject> .

<http://sw.cyc.com/2006/07/27/cyc/2ByteTwosComplementInteger> a <http://sw.cyc.com/2006/07/27/cyc/2ByteIntegerDatatype> , <http://sw.cyc.com/2006/07/27/cyc/TwosComplementIntegerDatatype> ;
	<http://sw.cyc.com/2006/07/27/cyc/prettyString-Canonical> "2 Byte Twos Complement Integer" .

<http://sw.cyc.com/2006/07/27/cyc/TwosComplementIntegerDatatype> <http://www.w3.org/2000/01/rdf-schema#comment> "The collection of all computer data types which represent integers using a two's complement representation. Hence, able to represent both positive and negative integers." ;
	a <http://sw.cyc.com/2006/07/27/cyc/FixedSizeComputerDatatypeType> ;
	<http://sw.cyc.com/2006/07/27/cyc/prettyString-Canonical> "twos-complement integer" ;
	<http://sw.cyc.com/2006/07/27/cyc/prettyString> "2s complement integer" , "2s complement integers" , "twos-complement integers" ;
	<http://www.w3.org/2000/01/rdf-schema#subClassOf> <http://sw.cyc.com/2006/07/27/cyc/IntegerComputerNumber> , <http://sw.cyc.com/2006/07/27/cyc/ProgramObject> .

<http://sw.cyc.com/2006/07/27/cyc/2MMRRegimentHQ-RRS> a <http://sw.cyc.com/2006/07/27/cyc/Individual> , <http://sw.cyc.com/2006/07/27/cyc/Platoon-MilitaryEchelon> , <http://sw.cyc.com/2006/07/27/cyc/CommandUnit-MilitarySpecialty> , <http://sw.cyc.com/2006/07/27/cyc/RedUnit> ;
	<http://sw.cyc.com/2006/07/27/cyc/prettyString-Canonical> "HQ/2 MRR" ;
	<http://sw.cyc.com/2006/07/27/cyc/quotedIsa> <http://sw.cyc.com/2006/07/27/cyc/FACToryIrrelevantTerm> .

<http://sw.cyc.com/2006/07/27/cyc/2ndManeuverBrigade-RRS> a <http://sw.cyc.com/2006/07/27/cyc/Individual> , <http://sw.cyc.com/2006/07/27/cyc/BlueUnit> , <http://sw.cyc.com/2006/07/27/cyc/PartiallyTangible> , <http://sw.cyc.com/2006/07/27/cyc/Brigade-MilitaryEchelon> , <http://sw.cyc.com/2006/07/27/cyc/ManeuverUnit-MilitarySpecialty> , <http://sw.cyc.com/2006/07/27/cyc/SpatialThing-Localized> ;
	<http://sw.cyc.com/2006/07/27/cyc/prettyString-Canonical> "Blue 2nd Bde 54th Mech Inf Div" ;
	<http://sw.cyc.com/2006/07/27/cyc/prettyString> "Blue 2nd Bde" ;
	<http://sw.cyc.com/2006/07/27/cyc/quotedIsa> <http://sw.cyc.com/2006/07/27/cyc/FACToryIrrelevantTerm> .

<http://sw.cyc.com/2006/07/27/cyc/SpatialThing-Localized> <http://www.w3.org/2000/01/rdf-schema#comment> """A specialization of both #$SpatialThing and #$TemporalThing.  This is the collection of all spatial things, tangible or intangible, that can meaningfully be said to have location or position in the empirical universe.   
<p>
Examples of spatially-localized things include all #$PartiallyTangible things, such as trees and ships, as well as certain #$Intangible spatial things, like the #$EarthsEquator.  Also included are those events that can be pinned-down to specific places (see #$Event-Localized), and thus all #$PhysicalEvents.  Excluded from this collection are any #$SpatialThings that are <i>not</i> localized, such as -- arguably -- purely abstract geometrical figures (e.g. a Platonic sphere). 
<p>
Note that a fictional or imaginary object (such as Frodo, Captain Queeg, or #$HAL9000-TheComputer) is typically localized with respect to the universe of the fictional/imagnary context in which it is found, and so is an instance of #$SpatialThing-Localized with respect to that context.""" ;
	a <http://sw.cyc.com/2006/07/27/cyc/QAClarifyingCollectionType> , <http://sw.cyc.com/2006/07/27/cyc/StuffType> , <http://sw.cyc.com/2006/07/27/cyc/TestOWLExportConcept> ;
	<http://sw.cyc.com/2006/07/27/cyc/prettyString-Canonical> "localized spatial thing" ;
	<http://sw.cyc.com/2006/07/27/cyc/prettyString> "thing with a location" , "things with a location" , "locatable thing" , "locatable things" , "localized spatial things" ;
	<http://www.w3.org/2000/01/rdf-schema#subClassOf> <http://sw.cyc.com/2006/07/27/cyc/SpatialThing> , <http://sw.cyc.com/2006/07/27/cyc/TemporallyExistingThing> , <http://sw.cyc.com/2006/07/27/cyc/Boundary-Underspecified> ;
	<http://sw.cyc.com/2006/07/27/cyc/facets-Generic> <http://sw.cyc.com/2006/07/27/cyc/SpatialThingTypeByGenericLocation> ;
	<http://sw.cyc.com/2006/07/27/cyc/requiredArg2Pred> <http://sw.cyc.com/2006/07/27/cyc/spatiallyRelated> .

<http://sw.cyc.com/2006/07/27/cyc/2ndManeuverRegiment-RRS> a <http://sw.cyc.com/2006/07/27/cyc/Individual> , <http://sw.cyc.com/2006/07/27/cyc/RedUnit> , <http://sw.cyc.com/2006/07/27/cyc/ManeuverUnit-MilitarySpecialty> , <http://sw.cyc.com/2006/07/27/cyc/Regiment-MilitaryEchelon> ;
	<http://sw.cyc.com/2006/07/27/cyc/prettyString-Canonical> "2nd MRR" ;
	<http://sw.cyc.com/2006/07/27/cyc/quotedIsa> <http://sw.cyc.com/2006/07/27/cyc/FACToryIrrelevantTerm> .

<http://sw.cyc.com/2006/07/27/cyc/2ndMIDDestroyAtChester> a <http://www.w3.org/2002/07/owl#Class> , <http://sw.cyc.com/2006/07/27/cyc/Mission-AssignedActionType> ;
	<http://sw.cyc.com/2006/07/27/cyc/prettyString-Canonical> "destroying enemy forces at Objective CHESTER" ;
	<http://sw.cyc.com/2006/07/27/cyc/prettyString> "destroy enemy forces at Objective CHESTER" , "destroyed enemy forces at Objective CHESTER" , "destroys enemy forces at Objective CHESTER" , "have destroyed enemy forces at Objective CHESTER" , "has destroyed enemy forces at Objective CHESTER" , "will destroy enemy forces at Objective CHESTER" , "had destroyed enemy forces at Objective CHESTER" , "will have destroyed enemy forces at Objective CHESTER" ;
	<http://www.w3.org/2000/01/rdf-schema#subClassOf> <http://sw.cyc.com/2006/07/27/cyc/DestroyingAnEnemyForce> , <http://sw.cyc.com/2006/07/27/cyc/OccupyingAnObjective> .

<http://sw.cyc.com/2006/07/27/cyc/DestroyingAnEnemyForce> <http://www.w3.org/2000/01/rdf-schema#comment> "To destroy an enemy force is to physically render it combat-ineffective until it is reconstituted. The amount of damage needed to render a unit combat-ineffective depends on the unit's type, discipline, and morale. It normally requires greater than percent personnel or equipment casualties. Destroying armored or dug-in targets with area fire weapons requires a large amount of ammunition and  considerable time, so forces do not normally attempt it unless they have terminally guided munitions." ;
	a <http://sw.cyc.com/2006/07/27/cyc/TemporalObjectType> , <http://sw.cyc.com/2006/07/27/cyc/MilitaryTaskedActionType> ;
	<http://sw.cyc.com/2006/07/27/cyc/prettyString-Canonical> "destroying an enemy force" ;
	<http://sw.cyc.com/2006/07/27/cyc/prettyString> "destroy an enemy force" , "destroyed an enemy force" , "destroys an enemy force" , "have destroyed an enemy force" .

<http://sw.cyc.com/2006/07/27/cyc/MechanizedInfantryDivision> <http://www.w3.org/2000/01/rdf-schema#comment> """The collection of all
#$MechanizedInfantryUnit-MilitarySpecialty at the echelon level of
division.""" ;
	a <http://sw.cyc.com/2006/07/27/cyc/ExistingObjectType> , <http://sw.cyc.com/2006/07/27/cyc/GenericMilitaryOrganizations-Organization-Topic> , <http://sw.cyc.com/2006/07/27/cyc/MilitaryOrganizationConcept> ;
	<http://sw.cyc.com/2006/07/27/cyc/prettyString-Canonical> "mechanized infantry division" ;
	<http://sw.cyc.com/2006/07/27/cyc/prettyString> "mechanized infantry divisions" ;
	<http://www.w3.org/2000/01/rdf-schema#subClassOf> <http://sw.cyc.com/2006/07/27/cyc/Division-MilitaryEchelon> , <http://sw.cyc.com/2006/07/27/cyc/MechanizedInfantryUnit-MilitarySpecialty> .

<http://sw.cyc.com/2006/07/27/cyc/2s12-Mortar> a <http://sw.cyc.com/2006/07/27/cyc/WeaponType> , <http://sw.cyc.com/2006/07/27/cyc/ExistingObjectType> ;
	<http://sw.cyc.com/2006/07/27/cyc/prettyString-Canonical> "M1943" ;
	<http://sw.cyc.com/2006/07/27/cyc/prettyString> "M43" , "M43s" , "2s12" , "2s12s" , "2s12 120mm towed mortar" , "2s12 120mm towed mortars" , "M1943s" ;
	<http://www.w3.org/2000/01/rdf-schema#subClassOf> <http://sw.cyc.com/2006/07/27/cyc/Mortar-120mm-Standard> , <http://sw.cyc.com/2006/07/27/cyc/Platform-Military> .

<http://sw.cyc.com/2006/07/27/cyc/Mortar-120mm-Standard> <http://www.w3.org/2000/01/rdf-schema#comment> "A mortar which fires 120mm shells." ;
	a <http://sw.cyc.com/2006/07/27/cyc/WeaponType> , <http://sw.cyc.com/2006/07/27/cyc/ExistingObjectType> ;
	<http://sw.cyc.com/2006/07/27/cyc/prettyString-Canonical> "120mm mortar" ;
	<http://sw.cyc.com/2006/07/27/cyc/prettyString> "standard 120mm mortar" , "standard 120mm mortars" , "120mm mortars" ;
	<http://www.w3.org/2000/01/rdf-schema#subClassOf> <http://sw.cyc.com/2006/07/27/cyc/MortarLauncher-Heavy> .

<http://sw.cyc.com/2006/07/27/cyc/Platform-Military> <http://www.w3.org/2000/01/rdf-schema#comment> "#$Platform-Military is a specialization of #$MilitaryHardware and #$TransportationDevice.  Each instance of #$Platform-Military is a transportation device which can carry military equipment such as #$Weapons, personnel and communications equipment. When a #$Platform-Military is armed with a #$Weapon, such as a #$Tank-Vehicle, it will result in a type of #$WeaponSystem." ;
	a <http://sw.cyc.com/2006/07/27/cyc/ExistingObjectType> , <http://sw.cyc.com/2006/07/27/cyc/SpatiallyDisjointObjectType> ;
	<http://sw.cyc.com/2006/07/27/cyc/prettyString-Canonical> "military platform" ;
	<http://sw.cyc.com/2006/07/27/cyc/prettyString> "platform" , "platforms" , "military platforms" ;
	<http://www.w3.org/2000/01/rdf-schema#subClassOf> <http://sw.cyc.com/2006/07/27/cyc/TransportationDevice> , <http://sw.cyc.com/2006/07/27/cyc/MilitaryHardware> , <http://sw.cyc.com/2006/07/27/cyc/DurableGood> ;
	<http://sw.cyc.com/2006/07/27/cyc/quotedIsa> <http://sw.cyc.com/2006/07/27/cyc/TerrorismOntologyConstant> .

<http://sw.cyc.com/2006/07/27/cyc/2-TheDigit> <http://www.w3.org/2000/01/rdf-schema#comment> "The numeral 2 of the Arabic Number system.  This is '2' as a #$Character-Abstract rather than the physical #$WrittenCharacter or the abstract mathematical #$Number-General." ;
	a <http://sw.cyc.com/2006/07/27/cyc/ArabicNumeral> ;
	<http://sw.cyc.com/2006/07/27/cyc/prettyString-Canonical> "the numeral 2" ;
	<http://sw.cyc.com/2006/07/27/cyc/prettyString> "the numerals 2" .

<http://sw.cyc.com/2006/07/27/cyc/3086VBC352-3-TheSoftwarePatch> a <http://sw.cyc.com/2006/07/27/cyc/Individual> , <http://sw.cyc.com/2006/07/27/cyc/ArchitectureIndependentComputerPatchProgram> , <http://sw.cyc.com/2006/07/27/cyc/ComputerPatchProgram> ;
	<http://sw.cyc.com/2006/07/27/cyc/prettyString-Canonical> "Trend Micro Patch 3086VBC352-3" .

<http://sw.cyc.com/2006/07/27/cyc/3-1AdjustableRateLoan> <http://www.w3.org/2000/01/rdf-schema#comment> "The collection of instances of #$AdjustableRateLoan that have a three year initialAdjustmentPeriod and readjust annually thereafter." ;
	a <http://sw.cyc.com/2006/07/27/cyc/IntermediateAdjustableRateLoanTypeByInitialAdjustmentPeriod> ;
	<http://sw.cyc.com/2006/07/27/cyc/prettyString-Canonical> "3/1 loan" ;
	<http://sw.cyc.com/2006/07/27/cyc/prettyString> "3/1 adjustible rate loan" , "3/1 adjustible rate loans" , "3/1 loans" ;
	<http://www.w3.org/2000/01/rdf-schema#subClassOf> <http://sw.cyc.com/2006/07/27/cyc/IntermediateAdjustableRateLoan> .

<http://sw.cyc.com/2006/07/27/cyc/IntermediateAdjustableRateLoan> <http://www.w3.org/2000/01/rdf-schema#comment> "The collection of instances of #$AdjustableRateLoan whose interest rate (c.f., #$interestRate) adjusts annually after a relatively longer initial adjustment period (c.f., #$initialAdjustmentPeriod), typically 3 or 5 years." ;
	a <http://sw.cyc.com/2006/07/27/cyc/ObjectType> , <http://sw.cyc.com/2006/07/27/cyc/TemporalStuffType> ;
	<http://sw.cyc.com/2006/07/27/cyc/prettyString-Canonical> "intermediate adjustible rate loan" ;
	<http://sw.cyc.com/2006/07/27/cyc/prettyString> "intermediate adjustible rate loans" ;
	<http://www.w3.org/2000/01/rdf-schema#subClassOf> <http://sw.cyc.com/2006/07/27/cyc/AdjustableRateLoan> ;
	<http://www.w3.org/2002/07/owl#disjointWith> <http://sw.cyc.com/2006/07/27/cyc/AdjustableRateLoan-ConsistentAdjustmentPeriod> ;
	<http://sw.cyc.com/2006/07/27/cyc/facets-Generic> <http://sw.cyc.com/2006/07/27/cyc/IntermediateAdjustableRateLoanTypeByInitialAdjustmentPeriod> .

<http://sw.cyc.com/2006/07/27/cyc/IntermediateAdjustableRateLoanTypeByInitialAdjustmentPeriod> a <http://sw.cyc.com/2006/07/27/cyc/FacetingCollectionType> .

<http://sw.cyc.com/2006/07/27/cyc/35InchTelevisionSet> <http://www.w3.org/2000/01/rdf-schema#subClassOf> <http://sw.cyc.com/2006/07/27/cyc/ManufacturedGoods> , <http://sw.cyc.com/2006/07/27/cyc/TelevisionSet> .

<http://sw.cyc.com/2006/07/27/cyc/35thParallel-North> a <http://sw.cyc.com/2006/07/27/cyc/Individual> , <http://sw.cyc.com/2006/07/27/cyc/LatitudeLine> ;
	<http://sw.cyc.com/2006/07/27/cyc/prettyString-Canonical> "North 35th Parallel " .

<http://sw.cyc.com/2006/07/27/cyc/LatitudeLine> <http://www.w3.org/2000/01/rdf-schema#comment> "The collection of lines around the earth which are parallel to the #$EarthsEquator." ;
	a <http://sw.cyc.com/2006/07/27/cyc/SpatiallyDisjointObjectType> , <http://sw.cyc.com/2006/07/27/cyc/TemporalStuffType> , <http://sw.cyc.com/2006/07/27/cyc/CartographicFeatureType> ;
	<http://sw.cyc.com/2006/07/27/cyc/prettyString-Canonical> "line of latitude" ;
	<http://sw.cyc.com/2006/07/27/cyc/prettyString> "latitude" , "latitudes" , "Parallel" , "parallels" , "parallel of latitude" , "parallels of latitude" , "lines of latitude" ;
	<http://www.w3.org/2000/01/rdf-schema#subClassOf> <http://sw.cyc.com/2006/07/27/cyc/ClosedLinearObject> , <http://sw.cyc.com/2006/07/27/cyc/GeographicalPlace-1D> .

<http://sw.cyc.com/2006/07/27/cyc/36thParallel-North> <http://www.w3.org/2000/01/rdf-schema#comment> "The 36th parallel in the northern hemisphere of #$PlanetEarth." ;
	a <http://sw.cyc.com/2006/07/27/cyc/Individual> , <http://sw.cyc.com/2006/07/27/cyc/LatitudeLine> ;
	<http://sw.cyc.com/2006/07/27/cyc/prettyString-Canonical> "36th Parallel North" .

<http://sw.cyc.com/2006/07/27/cyc/37-SearchEngine> a <http://sw.cyc.com/2006/07/27/cyc/Individual> , <http://sw.cyc.com/2006/07/27/cyc/UnversionedProgram> , <http://sw.cyc.com/2006/07/27/cyc/SearchEngine> ;
	<http://sw.cyc.com/2006/07/27/cyc/prettyString-Canonical> "37.com" ;
	<http://sw.cyc.com/2006/07/27/cyc/prettyString> "37" .

<http://sw.cyc.com/2006/07/27/cyc/SearchEngine> <http://www.w3.org/2000/01/rdf-schema#comment> "A collection of computer programs. Each #$SearchEngine takes as input a query string (which may be natural language, a specified syntax, or just a series of words) and returns a list of 'hits' - pointers to documents the search engine believes are relevant to the query. The domain for a search engine may be the World Wide Web, Usenet newsgroups, an individual #$ComputerDisk, or any other online collection of documents." ;
	a <http://sw.cyc.com/2006/07/27/cyc/KEClarifyingCollectionType> , <http://sw.cyc.com/2006/07/27/cyc/ComputerProgramTypeByFunction> ;
	<http://sw.cyc.com/2006/07/27/cyc/prettyString-Canonical> "search engine" ;
	<http://sw.cyc.com/2006/07/27/cyc/prettyString> "directories" , "directory" , "web searcher" , "web searchers" , "webferret" , "webferrets" , "websearch engine" , "websearch engines" , "warez search engine" , "warez search engines" , "web-search engine" , "web-search engines" , "websearching engine" , "websearching engines" , "web searching engine" , "web searching engines" , "searching engine" , "searching engines" , "web-searching engine" , "web-searching engines" , "web search engine" , "web search engines" , "search robot" , "search robots" , "search engines" , "Web directory" , "Web directories" ;
	<http://www.w3.org/2000/01/rdf-schema#subClassOf> <http://sw.cyc.com/2006/07/27/cyc/InternetProgram> , <http://sw.cyc.com/2006/07/27/cyc/SearchStringProgram> .

<http://sw.cyc.com/2006/07/27/cyc/37thParallel-North> <http://www.w3.org/2000/01/rdf-schema#comment> "The 37th parallel in the northern hemisphere of #$PlanetEarth." ;
	a <http://sw.cyc.com/2006/07/27/cyc/Individual> , <http://sw.cyc.com/2006/07/27/cyc/LatitudeLine> ;
	<http://sw.cyc.com/2006/07/27/cyc/prettyString-Canonical> "37th Parallel North" .

<http://sw.cyc.com/2006/07/27/cyc/38Special-MusicGroup> a <http://sw.cyc.com/2006/07/27/cyc/Individual> ;
	<http://sw.cyc.com/2006/07/27/cyc/prettyString-Canonical> "38 Special" .

<http://sw.cyc.com/2006/07/27/cyc/38thParallel-North> <http://www.w3.org/2000/01/rdf-schema#comment> "The 38th parallel in the northern hemisphere of #$PlanetEarth." ;
	a <http://sw.cyc.com/2006/07/27/cyc/Individual> , <http://sw.cyc.com/2006/07/27/cyc/LatitudeLine> .

<http://sw.cyc.com/2006/07/27/cyc/3DComputerWallpaperFile> <http://sw.cyc.com/2006/07/27/cyc/prettyString-Canonical> "Three-dimensional wallpaper" ;
	<http://sw.cyc.com/2006/07/27/cyc/prettyString> "3D wallpaper" ;
	<http://www.w3.org/2000/01/rdf-schema#subClassOf> <http://sw.cyc.com/2006/07/27/cyc/ComputerWallpaperFile> .

<http://sw.cyc.com/2006/07/27/cyc/ComputerWallpaperFile> <http://www.w3.org/2000/01/rdf-schema#comment> "A collection of #$ComputerImageFiles. Each instance of #$ComputerWallpaperFile represents an image that is intended to be displayed as the background of the GUI of an #$OperatingSystem like #$MSWindows, or the background of a web page." ;
	a <http://sw.cyc.com/2006/07/27/cyc/ObjectType> ;
	<http://sw.cyc.com/2006/07/27/cyc/prettyString-Canonical> "wallpaper" ;
	<http://sw.cyc.com/2006/07/27/cyc/prettyString> "background" , "backgrounds" , "wallpapers" , "wallpaper theme" , "wallpaper themes" , "background theme" , "background themes" , "wall-paper theme" , "wall-paper themes" , "wall paper theme" , "wall paper themes" , "desktop background" , "desktop backgrounds" , "background image" , "background images" , "wallp file" , "wallp files" , "wallpaper file" , "wallpaper files" , "computer wallpaper" , "computer wallpapers" , "wall paper" , "wall papers" ;
	<http://www.w3.org/2000/01/rdf-schema#subClassOf> <http://sw.cyc.com/2006/07/27/cyc/ComputerImageFile> , <http://sw.cyc.com/2006/07/27/cyc/ComputerDesktopTheme> .

<http://sw.cyc.com/2006/07/27/cyc/ObjectType> <http://www.w3.org/2000/01/rdf-schema#comment> """The collection of all collections that are \"object-like\" in at least one respect. A collection <code>COL</code> is object-like just in case there is some sense of 'part' according to which any (or nearly any) given proper part of an instance of <code>COL</code> is <i>not</i> itself an instance of <code>COL</code>; when this happens <code>COL</code> is said to be object-like with respect to that sense of 'part'.
<p>
More precisely, for a collection <code>COL</code> to be an instance of #$ObjectType it is sufficient that there be some specialization <code>PARTPRED</code> of #$properParts such that, for any <code>OBJ1</code> and <code>OBJ2</code>, if <code>(#$isa OBJ1 COL)</code> and <code>(PARTPRED OBJ1 OBJ2)</code> both hold, then <code>(#$isa OBJ2 COL)</code> does <i>not</i> hold.  (Also sufficient for <code>COL</code>'s being an object-type is that there be some specialization <code>INVPARTPRED</code> of the <i>inverse</i> of #$properParts (see #$genlInverse) such that <code>(INVPARTPRED OBJ2 OBJ1)</code>, with everything else remaining the same as above.)  Note that neither of the above sufficient conditions for <code>COL</code>'s being an object-type is strictly necessary: some exceptions are allowed.  Thus as long as either one of the above conditionals holds in <i>nearly</i> all cases, <code>COL</code> should be considered an instance of #$ObjectType.
<p>
Here are two examples.  Consider #$Automobile.  Take an instance of that, say my car.  Now consider one of the proper #$physicalParts of my car, say the steering wheel.  The steering wheel is <i>not</i> an instance of #$Automobile.  And the same would be true for any proper physical part of any car.  So #$Automobile is an #$ObjectType.  Consider #$CalendarYear. No proper #$timeSlices of a year is itself a year.  So #$CalendarYear is an #$ObjectType.  
<p>
See #$StuffType for the contrasting (though not disjoint) notion of being stuff-like.""" ;
	a <http://sw.cyc.com/2006/07/27/cyc/AtemporalNecessarilyEssentialCollectionType> , <http://sw.cyc.com/2006/07/27/cyc/FacetingCollectionType> , <http://sw.cyc.com/2006/07/27/cyc/SecondOrderCollection> , <http://sw.cyc.com/2006/07/27/cyc/Top-Topic> ;
	<http://sw.cyc.com/2006/07/27/cyc/prettyString-Canonical> "type of object" ;
	<http://sw.cyc.com/2006/07/27/cyc/prettyString> "types of object" , "kind of object" , "kinds of object" , "object type" , "object types" ;
	<http://www.w3.org/2000/01/rdf-schema#subClassOf> <http://sw.cyc.com/2006/07/27/cyc/FirstOrderCollection> ;
	<http://sw.cyc.com/2006/07/27/cyc/typeGenls> <http://sw.cyc.com/2006/07/27/cyc/Individual> ;
	<http://sw.cyc.com/2006/07/27/cyc/facets-Generic> <http://sw.cyc.com/2006/07/27/cyc/ObjectTypeTypeByStatusAfterEvent> .

<http://sw.cyc.com/2006/07/27/cyc/3ddesktop-TheProgram> a <http://sw.cyc.com/2006/07/27/cyc/UnversionedProgram> , <http://sw.cyc.com/2006/07/27/cyc/DesktopSwitcherProgram> ;
	<http://sw.cyc.com/2006/07/27/cyc/prettyString-Canonical> "3ddesktop" .

<http://sw.cyc.com/2006/07/27/cyc/DesktopSwitcherProgram> a <http://sw.cyc.com/2006/07/27/cyc/ComputerProgramTypeByFunction> ;
	<http://sw.cyc.com/2006/07/27/cyc/prettyString-Canonical> "desktop switcher program" ;
	<http://sw.cyc.com/2006/07/27/cyc/prettyString> "desktop switcher programme" , "desktop switcher programs" , "desktop switcher programz" ;
	<http://www.w3.org/2000/01/rdf-schema#subClassOf> <http://sw.cyc.com/2006/07/27/cyc/UtilityProgram> .

<http://sw.cyc.com/2006/07/27/cyc/3ddiag-TheProgram> a <http://sw.cyc.com/2006/07/27/cyc/UnversionedProgram> , <http://sw.cyc.com/2006/07/27/cyc/ConfiguringProgram> ;
	<http://sw.cyc.com/2006/07/27/cyc/prettyString-Canonical> "3ddiag" .

<http://sw.cyc.com/2006/07/27/cyc/ConfiguringProgram> <http://www.w3.org/2000/01/rdf-schema#comment> "The collection of programs that are used to configure other programs, computers or computer networks." ;
	a <http://sw.cyc.com/2006/07/27/cyc/KEClarifyingCollectionType> , <http://sw.cyc.com/2006/07/27/cyc/ComputerProgramTypeByFunction> ;
	<http://sw.cyc.com/2006/07/27/cyc/prettyString-Canonical> "configuring program" ;
	<http://sw.cyc.com/2006/07/27/cyc/prettyString> "configuring programme" , "configuring programs" , "configuring programz" ;
	<http://www.w3.org/2000/01/rdf-schema#subClassOf> <http://sw.cyc.com/2006/07/27/cyc/AdministrationProgram> .

<http://sw.cyc.com/2006/07/27/cyc/3DFlowerboxScreenSaver-TheProgram> <http://www.w3.org/2000/01/rdf-schema#comment> "An instance of #$ScreenSaver." .

<http://sw.cyc.com/2006/07/27/cyc/3DMazeScreenSaver-TheProgram> <http://sw.cyc.com/2006/07/27/cyc/prettyString-Canonical> "OpenGL 3D Maze Screen Saver" .

<http://sw.cyc.com/2006/07/27/cyc/3DOCompany> a <http://sw.cyc.com/2006/07/27/cyc/Individual> , <http://sw.cyc.com/2006/07/27/cyc/PubliclyHeldCorporation> , <http://sw.cyc.com/2006/07/27/cyc/CommercialOrganization> ;
	<http://sw.cyc.com/2006/07/27/cyc/prettyString-Canonical> "3DO Company" ;
	<http://sw.cyc.com/2006/07/27/cyc/prettyString> "3DO" .

<http://sw.cyc.com/2006/07/27/cyc/CommercialOrganization> <http://www.w3.org/2000/01/rdf-schema#comment> "A specialization of #$Organization.  Each instance of #$CommercialOrganization is an organization whose primary goal is to generate a profit for its owners, usually through the buying and selling of goods or services.  A given instance of #$CommercialOrganization may also be an instance of #$Business, or it may merely be a sub-organization of some instance of #$Business." ;
	a <http://sw.cyc.com/2006/07/27/cyc/ExistingObjectType> , <http://sw.cyc.com/2006/07/27/cyc/AtemporalNecessarilyEssentialCollectionType> , <http://sw.cyc.com/2006/07/27/cyc/QAClarifyingCollectionType> , <http://sw.cyc.com/2006/07/27/cyc/OrganizationsByBusinessProfitNature-Organization-Topic> , <http://sw.cyc.com/2006/07/27/cyc/OrganizationTypeByProfitMotive> ;
	<http://sw.cyc.com/2006/07/27/cyc/prettyString-Canonical> "commercial organization" ;
	<http://sw.cyc.com/2006/07/27/cyc/prettyString> "commercial organisation" , "commercial organisations" , "commercial organizations" ;
	<http://www.w3.org/2000/01/rdf-schema#subClassOf> <http://sw.cyc.com/2006/07/27/cyc/Organization> , <http://sw.cyc.com/2006/07/27/cyc/LegalAgent> , <http://sw.cyc.com/2006/07/27/cyc/Agent-NonGeographical> , <http://sw.cyc.com/2006/07/27/cyc/BusinessRelatedThing> ;
	<http://sw.cyc.com/2006/07/27/cyc/quotedIsa> <http://sw.cyc.com/2006/07/27/cyc/TerrorismOntologyConstant> ;
	<http://www.w3.org/2002/07/owl#disjointWith> <http://sw.cyc.com/2006/07/27/cyc/NonProfitOrganization> , <http://sw.cyc.com/2006/07/27/cyc/GovernmentalOrganization> ;
	<http://sw.cyc.com/2006/07/27/cyc/siblingDisjointExceptions> <http://sw.cyc.com/2006/07/27/cyc/PrivatelyHeldCorporation> ;
	<http://sw.cyc.com/2006/07/27/cyc/facets-Partition> <http://sw.cyc.com/2006/07/27/cyc/OrganizationTypeByOwnership> .

<http://sw.cyc.com/2006/07/27/cyc/3DPinball-TheProgram> a <http://sw.cyc.com/2006/07/27/cyc/Individual> , <http://sw.cyc.com/2006/07/27/cyc/UnversionedProgram> , <http://sw.cyc.com/2006/07/27/cyc/ComputerGameProgram> , <http://sw.cyc.com/2006/07/27/cyc/LocalProgram> , <http://sw.cyc.com/2006/07/27/cyc/UserProgram> ;
	<http://sw.cyc.com/2006/07/27/cyc/prettyString-Canonical> "3D Pinball" ;
	<http://sw.cyc.com/2006/07/27/cyc/prettyString> "pinball.exe" .

<http://sw.cyc.com/2006/07/27/cyc/3DPipesScreenSaver-TheProgram> <http://www.w3.org/2000/01/rdf-schema#comment> "An instance of #$ScreenSaver." ;
	a <http://sw.cyc.com/2006/07/27/cyc/Individual> , <http://sw.cyc.com/2006/07/27/cyc/UnversionedProgram> , <http://sw.cyc.com/2006/07/27/cyc/FileReadingProgram-Visual> , <http://sw.cyc.com/2006/07/27/cyc/ScreenSaver> ;
	<http://sw.cyc.com/2006/07/27/cyc/prettyString-Canonical> "OpenGL 3D Pipes Screen Saver" .

<http://sw.cyc.com/2006/07/27/cyc/3DRailroadMaster-TheGame> a <http://sw.cyc.com/2006/07/27/cyc/Individual> , <http://sw.cyc.com/2006/07/27/cyc/ComputerGameProgram> , <http://sw.cyc.com/2006/07/27/cyc/SimulationGameProgram> ;
	<http://sw.cyc.com/2006/07/27/cyc/prettyString-Canonical> "3D Railroad Master" .

<http://sw.cyc.com/2006/07/27/cyc/SimulationGameProgram> <http://www.w3.org/2000/01/rdf-schema#comment> "The collection of all #$ComputerGameProgram that simulate a complex system of a certain type, such as a city, ecosystem, large building, art colony, or vehicle. Instances are game titles such as \"SimCity 2000\" or \"Microsoft Flight Simulator\"." ;
	a <http://www.w3.org/2002/07/owl#Class> , <http://sw.cyc.com/2006/07/27/cyc/AtemporalNecessarilyEssentialCollectionType> , <http://sw.cyc.com/2006/07/27/cyc/KEClarifyingCollectionType> , <http://sw.cyc.com/2006/07/27/cyc/ComputerProgramTypeByFunction> ;
	<http://sw.cyc.com/2006/07/27/cyc/prettyString-Canonical> "simulation game" ;
	<http://sw.cyc.com/2006/07/27/cyc/prettyString> "simulations" , "simulation" , "simulation games" , "simulator" , "simulators" ;
	<http://www.w3.org/2000/01/rdf-schema#subClassOf> <http://sw.cyc.com/2006/07/27/cyc/ComputerGameProgram> , <http://sw.cyc.com/2006/07/27/cyc/FileReadingProgram-Visual> ;
	<http://sw.cyc.com/2006/07/27/cyc/siblingDisjointExceptions> <http://sw.cyc.com/2006/07/27/cyc/ArcadeGameProgram> , <http://sw.cyc.com/2006/07/27/cyc/ActionGameProgram> , <http://sw.cyc.com/2006/07/27/cyc/RoleplayingGameProgram> .

<http://sw.cyc.com/2006/07/27/cyc/3DRealms> a <http://sw.cyc.com/2006/07/27/cyc/Individual> , <http://sw.cyc.com/2006/07/27/cyc/SoftwareVendor> ;
	<http://sw.cyc.com/2006/07/27/cyc/prettyString-Canonical> "3D Realms" .

<http://sw.cyc.com/2006/07/27/cyc/3dSystemsCorporation> a <http://sw.cyc.com/2006/07/27/cyc/Individual> , <http://sw.cyc.com/2006/07/27/cyc/PubliclyHeldCorporation> ;
	<http://sw.cyc.com/2006/07/27/cyc/prettyString-Canonical> "3d Systems Corporation" .

<http://sw.cyc.com/2006/07/27/cyc/3DTextScreenSaver-TheProgram> <http://www.w3.org/2000/01/rdf-schema#comment> "An instance of #$ScreenSaver." ;
	a <http://sw.cyc.com/2006/07/27/cyc/Individual> , <http://sw.cyc.com/2006/07/27/cyc/UnversionedProgram> , <http://sw.cyc.com/2006/07/27/cyc/FileReadingProgram-Visual> , <http://sw.cyc.com/2006/07/27/cyc/ScreenSaver> ;
	<http://sw.cyc.com/2006/07/27/cyc/prettyString-Canonical> "OpenGL 3D Text Screen Saver" .

<http://sw.cyc.com/2006/07/27/cyc/3DUltraMiniGolfDeluxe-TheGame> a <http://sw.cyc.com/2006/07/27/cyc/Individual> , <http://sw.cyc.com/2006/07/27/cyc/ComputerGameProgram> , <http://sw.cyc.com/2006/07/27/cyc/ArcadeGameProgram> ;
	<http://sw.cyc.com/2006/07/27/cyc/prettyString-Canonical> "3D Ultra Mini Golf Deluxe" .

<http://sw.cyc.com/2006/07/27/cyc/3DUltraMiniGolf-TheGame> a <http://sw.cyc.com/2006/07/27/cyc/Individual> , <http://sw.cyc.com/2006/07/27/cyc/UnversionedProgram> , <http://sw.cyc.com/2006/07/27/cyc/ComputerGameProgram> , <http://sw.cyc.com/2006/07/27/cyc/ActionGameProgram> ;
	<http://sw.cyc.com/2006/07/27/cyc/prettyString-Canonical> "3D Ultra Mini Golf" .

<http://sw.cyc.com/2006/07/27/cyc/3DUltraNascarPinball-TheGame> a <http://sw.cyc.com/2006/07/27/cyc/Individual> , <http://sw.cyc.com/2006/07/27/cyc/ComputerGameProgram> , <http://sw.cyc.com/2006/07/27/cyc/ArcadeGameProgram> ;
	<http://sw.cyc.com/2006/07/27/cyc/prettyString-Canonical> "3D Ultra Nascar Pinball" .

<http://sw.cyc.com/2006/07/27/cyc/3-DUltraPinball2CreepNight-TheGame> a <http://sw.cyc.com/2006/07/27/cyc/Individual> , <http://sw.cyc.com/2006/07/27/cyc/ComputerGameProgram> , <http://sw.cyc.com/2006/07/27/cyc/ActionGameProgram> ;
	<http://sw.cyc.com/2006/07/27/cyc/prettyString-Canonical> "3-D Ultra Pinball 2: Creep Night" ;
	<http://sw.cyc.com/2006/07/27/cyc/prettyString> "3-D Ultra Pinball 2 Creep Night" .

<http://sw.cyc.com/2006/07/27/cyc/3DUltraPinballCollection-TheGame> a <http://sw.cyc.com/2006/07/27/cyc/Individual> , <http://sw.cyc.com/2006/07/27/cyc/ComputerGameProgram> , <http://sw.cyc.com/2006/07/27/cyc/ArcadeGameProgram> ;
	<http://sw.cyc.com/2006/07/27/cyc/prettyString-Canonical> "the game 3D Ultra Pinball Collection" .

<http://sw.cyc.com/2006/07/27/cyc/3-DUltraPinballTheLostContinent-TheGame> a <http://sw.cyc.com/2006/07/27/cyc/Individual> , <http://sw.cyc.com/2006/07/27/cyc/UnversionedProgram> , <http://sw.cyc.com/2006/07/27/cyc/ComputerGameProgram> , <http://sw.cyc.com/2006/07/27/cyc/ActionGameProgram> ;
	<http://sw.cyc.com/2006/07/27/cyc/prettyString-Canonical> "3-D Ultra Pinball : The Lost Continent" ;
	<http://sw.cyc.com/2006/07/27/cyc/prettyString> "3-D Ultra Pinball the Lost Continent" .

<http://sw.cyc.com/2006/07/27/cyc/3dwm-TheProgram> a <http://sw.cyc.com/2006/07/27/cyc/UnversionedProgram> , <http://sw.cyc.com/2006/07/27/cyc/DesktopEnvironmentProgram> ;
	<http://sw.cyc.com/2006/07/27/cyc/prettyString-Canonical> "3dwm" .

<http://sw.cyc.com/2006/07/27/cyc/DesktopEnvironmentProgram> a <http://sw.cyc.com/2006/07/27/cyc/ComputerProgramTypeByFunction> ;
	<http://sw.cyc.com/2006/07/27/cyc/prettyString-Canonical> "desktop environment program" ;
	<http://sw.cyc.com/2006/07/27/cyc/prettyString> "desktop environment programme" , "desktop environment programs" , "desktop environment programz" ;
	<http://www.w3.org/2000/01/rdf-schema#subClassOf> <http://sw.cyc.com/2006/07/27/cyc/LocalProgram> , <http://sw.cyc.com/2006/07/27/cyc/GraphicalUserInterfaceProgram> , <http://sw.cyc.com/2006/07/27/cyc/CommandInterpreter> .

<http://sw.cyc.com/2006/07/27/cyc/3Man-TheProgram> <http://www.w3.org/2000/01/rdf-schema#comment> "#$3Man-TheProgram in an instance of  #$ExecutableExploit that takes advantage of a vulnerability in the #$Man-TheProgram shipped with some #$Linux vendors, including versions of #$Linux-RedHat.  It allows a local user to hack into and alter a manpage and execute code on it with the privileges of the user running #$Man-TheProgram." ;
	a <http://sw.cyc.com/2006/07/27/cyc/Individual> , <http://sw.cyc.com/2006/07/27/cyc/ExecutableExploit> ;
	<http://sw.cyc.com/2006/07/27/cyc/prettyString-Canonical> "the program 3 Man" .

<http://sw.cyc.com/2006/07/27/cyc/ExecutableExploit> <http://www.w3.org/2000/01/rdf-schema#comment> """#$MaliciousComputerPrograms that are
distinct, executable programs.""" ;
	a <http://sw.cyc.com/2006/07/27/cyc/ObjectType> ;
	<http://sw.cyc.com/2006/07/27/cyc/prettyString-Canonical> "executable exploit code" ;
	<http://sw.cyc.com/2006/07/27/cyc/prettyString> "executable exploit" , "executable exploits" ;
	<http://www.w3.org/2000/01/rdf-schema#subClassOf> <http://sw.cyc.com/2006/07/27/cyc/LocalProgram> , <http://sw.cyc.com/2006/07/27/cyc/UserProgram> , <http://sw.cyc.com/2006/07/27/cyc/MaliciousComputerProgram> .

<http://sw.cyc.com/2006/07/27/cyc/3MMRRegimentHQ-RRS> a <http://sw.cyc.com/2006/07/27/cyc/Individual> , <http://sw.cyc.com/2006/07/27/cyc/Platoon-MilitaryEchelon> , <http://sw.cyc.com/2006/07/27/cyc/CommandUnit-MilitarySpecialty> , <http://sw.cyc.com/2006/07/27/cyc/RedUnit> ;
	<http://sw.cyc.com/2006/07/27/cyc/prettyString-Canonical> "HQ/3 MRR" ;
	<http://sw.cyc.com/2006/07/27/cyc/quotedIsa> <http://sw.cyc.com/2006/07/27/cyc/FACToryIrrelevantTerm> .

<http://sw.cyc.com/2006/07/27/cyc/3rdManeuverBrigade-RRS> a <http://sw.cyc.com/2006/07/27/cyc/Individual> , <http://sw.cyc.com/2006/07/27/cyc/BlueUnit> , <http://sw.cyc.com/2006/07/27/cyc/Brigade-MilitaryEchelon> , <http://sw.cyc.com/2006/07/27/cyc/ManeuverUnit-MilitarySpecialty> ;
	<http://sw.cyc.com/2006/07/27/cyc/prettyString-Canonical> "3rd Bde" ;
	<http://sw.cyc.com/2006/07/27/cyc/quotedIsa> <http://sw.cyc.com/2006/07/27/cyc/FACToryIrrelevantTerm> .

<http://sw.cyc.com/2006/07/27/cyc/3rdManeuverRegiment-RRS> a <http://sw.cyc.com/2006/07/27/cyc/Individual> , <http://sw.cyc.com/2006/07/27/cyc/RedUnit> , <http://sw.cyc.com/2006/07/27/cyc/ManeuverUnit-MilitarySpecialty> , <http://sw.cyc.com/2006/07/27/cyc/Regiment-MilitaryEchelon> ;
	<http://sw.cyc.com/2006/07/27/cyc/prettyString-Canonical> "3rd MRR" ;
	<http://sw.cyc.com/2006/07/27/cyc/quotedIsa> <http://sw.cyc.com/2006/07/27/cyc/FACToryIrrelevantTerm> .

<http://sw.cyc.com/2006/07/27/cyc/3-TheDigit> <http://www.w3.org/2000/01/rdf-schema#comment> "The numeral 3 of the Arabic Number system.  This is '3' as a #$Character-Abstract rather than the physical #$WrittenCharacter or the abstract mathematical #$Number-General." ;
	a <http://sw.cyc.com/2006/07/27/cyc/ArabicNumeral> ;
	<http://sw.cyc.com/2006/07/27/cyc/prettyString-Canonical> "the numeral 3" ;
	<http://sw.cyc.com/2006/07/27/cyc/prettyString> "the numerals 3" .

<http://sw.cyc.com/2006/07/27/cyc/400thCycKBBuild> <http://www.w3.org/2000/01/rdf-schema#comment> "The 400th Cyc KB build.  This event occured on January 25th, 2001 at Cycorp in Austin, Texas." ;
	a <http://sw.cyc.com/2006/07/27/cyc/Individual> , <http://sw.cyc.com/2006/07/27/cyc/SocialGathering> ;
	<http://sw.cyc.com/2006/07/27/cyc/prettyString-Canonical> "400th Cyc KB Build" .

<http://sw.cyc.com/2006/07/27/cyc/SocialGathering> <http://www.w3.org/2000/01/rdf-schema#comment> "A specialization of #$SocialOccurrence.  Each instance of #$SocialGathering is an intentional social gathering of people who have the same or similar purposes in attending, and in which there is communication between the participants.  Specializations include #$BabyShower, #$Carnival, and #$Rally.  Note that a group of people waiting to board an elevator is not typically a #$SocialGathering, even though they share a common purpose, since they are not expected to talk to each other." ;
	a <http://sw.cyc.com/2006/07/27/cyc/TemporalObjectType> , <http://sw.cyc.com/2006/07/27/cyc/SomeSampleKindsOfSocialActions-Social-Topic> ;
	<http://sw.cyc.com/2006/07/27/cyc/prettyString-Canonical> "social occasion" ;
	<http://sw.cyc.com/2006/07/27/cyc/prettyString> "gathering" , "gatherings" , "social" , "get-together" , "get-togethers" , "more social" , "most social" , "Local event" , "Local events" , "social occasions" ;
	<http://www.w3.org/2000/01/rdf-schema#subClassOf> <http://sw.cyc.com/2006/07/27/cyc/SocialOccurrence> , <http://sw.cyc.com/2006/07/27/cyc/CulturalActivity> ;
	<http://www.w3.org/2002/07/owl#disjointWith> <http://sw.cyc.com/2006/07/27/cyc/IntrinsicStateChangeEvent> , <http://sw.cyc.com/2006/07/27/cyc/SingleDoerAction> , <http://sw.cyc.com/2006/07/27/cyc/ConflictEvent> , <http://sw.cyc.com/2006/07/27/cyc/MentalSituation-SingleSubject> ;
	<http://sw.cyc.com/2006/07/27/cyc/requiredActorSlots> <http://sw.cyc.com/2006/07/27/cyc/attendees> .

<http://sw.cyc.com/2006/07/27/cyc/40thParallel-North> <http://www.w3.org/2000/01/rdf-schema#comment> "The 40th parallel in the northern hemisphere of #$PlanetEarth." ;
	a <http://sw.cyc.com/2006/07/27/cyc/Individual> ;
	<http://sw.cyc.com/2006/07/27/cyc/prettyString-Canonical> "40th Parallel North" .

<http://sw.cyc.com/2006/07/27/cyc/413HopeSt-TheTVShow> a <http://sw.cyc.com/2006/07/27/cyc/Individual> , <http://sw.cyc.com/2006/07/27/cyc/TVSeriesProduct> ;
	<http://sw.cyc.com/2006/07/27/cyc/prettyString-Canonical> "413 Hope St" .

<http://sw.cyc.com/2006/07/27/cyc/48Hours-TheMovie> a <http://sw.cyc.com/2006/07/27/cyc/Individual> , <http://sw.cyc.com/2006/07/27/cyc/ActionMovie> , <http://sw.cyc.com/2006/07/27/cyc/ComedyMovie> ;
	<http://sw.cyc.com/2006/07/27/cyc/prettyString-Canonical> "48 Hours" .

<http://sw.cyc.com/2006/07/27/cyc/ActionMovie> <http://www.w3.org/2000/01/rdf-schema#comment> "#$ActionMovie is a collection of instances of #$Movie-CW each of which relates a story characterized by fast-moving action such as car chases and kick-boxing." ;
	a <http://sw.cyc.com/2006/07/27/cyc/QAClarifyingCollectionType> , <http://sw.cyc.com/2006/07/27/cyc/MovieTypeByGenre> ;
	<http://sw.cyc.com/2006/07/27/cyc/prettyString-Canonical> "action movie" ;
	<http://sw.cyc.com/2006/07/27/cyc/prettyString> "action flick" , "action flicks" , "action film" , "action films" , "action movies" ;
	<http://www.w3.org/2000/01/rdf-schema#subClassOf> <http://sw.cyc.com/2006/07/27/cyc/Movie-CW> , <http://sw.cyc.com/2006/07/27/cyc/PropositionalConceptualWork-ActionGenre> .

<http://sw.cyc.com/2006/07/27/cyc/ComedyMovie> <http://www.w3.org/2000/01/rdf-schema#comment> "#$ComedyMovie is a collection of instances of #$Movie-CW each of which relates a humorous story." ;
	a <http://sw.cyc.com/2006/07/27/cyc/MovieTypeByGenre> ;
	<http://sw.cyc.com/2006/07/27/cyc/prettyString-Canonical> "comedy movie" ;
	<http://sw.cyc.com/2006/07/27/cyc/prettyString> "comedy" , "comedies" , "comedy flick" , "comedy flicks" , "comedy film" , "comedy films" , "comedy movies" ;
	<http://www.w3.org/2000/01/rdf-schema#subClassOf> <http://sw.cyc.com/2006/07/27/cyc/Movie-CW> , <http://sw.cyc.com/2006/07/27/cyc/PropositionalConceptualWork-ComedyGenre> .

<http://sw.cyc.com/2006/07/27/cyc/4ByteIntegerDatatype> <http://www.w3.org/2000/01/rdf-schema#comment> "The collection of all computer data types that employ exactly 4 bytes to represent some subset of the integers or values related to represnting integer values such as NAN. Note that this does not specify, for example, whether the data type represents positive integers only, or is in two's complement representation." ;
	a <http://sw.cyc.com/2006/07/27/cyc/FixedSizeComputerDatatypeType> , <http://sw.cyc.com/2006/07/27/cyc/SKSIDataTypeDescriptions-Topic> ;
	<http://sw.cyc.com/2006/07/27/cyc/prettyString-Canonical> "4-byte integer" ;
	<http://sw.cyc.com/2006/07/27/cyc/prettyString> "four-byte integer" , "four-byte integers" , "4-byte integers" ;
	<http://www.w3.org/2000/01/rdf-schema#subClassOf> <http://sw.cyc.com/2006/07/27/cyc/IntegerComputerNumber> , <http://sw.cyc.com/2006/07/27/cyc/ProgramObject> .

<http://sw.cyc.com/2006/07/27/cyc/4ByteRealDatatype> <http://www.w3.org/2000/01/rdf-schema#comment> "The collection of all computer data types that employ exactly 4 bytes to represent some subset of the real numbers." ;
	a <http://sw.cyc.com/2006/07/27/cyc/FixedSizeComputerDatatypeType> , <http://sw.cyc.com/2006/07/27/cyc/SKSIDataTypeDescriptions-Topic> ;
	<http://sw.cyc.com/2006/07/27/cyc/prettyString-Canonical> "4 byte real datatype" ;
	<http://www.w3.org/2000/01/rdf-schema#subClassOf> <http://sw.cyc.com/2006/07/27/cyc/RealNumberDatatype> .

<http://sw.cyc.com/2006/07/27/cyc/RealNumberDatatype> <http://www.w3.org/2000/01/rdf-schema#comment> "The collection of all computer data types that are capable (only) of representing some subset of the real numbers." ;
	a <http://sw.cyc.com/2006/07/27/cyc/SKSIDataTypeDescriptions-Topic> , <http://sw.cyc.com/2006/07/27/cyc/ComputerDatatypeType> ;
	<http://sw.cyc.com/2006/07/27/cyc/prettyString-Canonical> "real number datatype" ;
	<http://www.w3.org/2000/01/rdf-schema#subClassOf> <http://sw.cyc.com/2006/07/27/cyc/ProgramObject> , <http://sw.cyc.com/2006/07/27/cyc/NumberObject> .

<http://sw.cyc.com/2006/07/27/cyc/4ByteTwosComplementInteger> a <http://sw.cyc.com/2006/07/27/cyc/TwosComplementIntegerDatatype> .

<http://sw.cyc.com/2006/07/27/cyc/50WaysToLeaveYourLover-TheSong> a <http://sw.cyc.com/2006/07/27/cyc/Individual> , <http://sw.cyc.com/2006/07/27/cyc/HitSong-CW> ;
	<http://sw.cyc.com/2006/07/27/cyc/prettyString-Canonical> "50 Ways to Leave Your Lover" .

<http://sw.cyc.com/2006/07/27/cyc/HitSong-CW> <http://www.w3.org/2000/01/rdf-schema#comment> "The collection of all hit songs." ;
	a <http://sw.cyc.com/2006/07/27/cyc/TemporalObjectType> ;
	<http://sw.cyc.com/2006/07/27/cyc/prettyString-Canonical> "hit song" ;
	<http://sw.cyc.com/2006/07/27/cyc/prettyString> "hit songs" ;
	<http://www.w3.org/2000/01/rdf-schema#subClassOf> <http://sw.cyc.com/2006/07/27/cyc/Song-CW> , <http://sw.cyc.com/2006/07/27/cyc/HitConceptualWork> .

<http://sw.cyc.com/2006/07/27/cyc/5-1AdjustableRateLoan> <http://www.w3.org/2000/01/rdf-schema#comment> "The collection of instances of #$AdjustableRateLoan that have a five year initialAdjustmentPeriod and readjust annually thereafter." ;
	a <http://sw.cyc.com/2006/07/27/cyc/IntermediateAdjustableRateLoanTypeByInitialAdjustmentPeriod> ;
	<http://sw.cyc.com/2006/07/27/cyc/prettyString-Canonical> "5/1 adjustible rate loan" ;
	<http://sw.cyc.com/2006/07/27/cyc/prettyString> "5/1 loan" , "5/1 loans" , "5/1 adjustible rate loans" ;
	<http://www.w3.org/2000/01/rdf-schema#subClassOf> <http://sw.cyc.com/2006/07/27/cyc/IntermediateAdjustableRateLoan> .

<http://sw.cyc.com/2006/07/27/cyc/54thAviationBrigade> a <http://sw.cyc.com/2006/07/27/cyc/Individual> , <http://sw.cyc.com/2006/07/27/cyc/BlueUnit> , <http://sw.cyc.com/2006/07/27/cyc/Brigade-MilitaryEchelon> , <http://sw.cyc.com/2006/07/27/cyc/AviationUnit-MilitarySpecialty> ;
	<http://sw.cyc.com/2006/07/27/cyc/prettyString-Canonical> "54th Cbt Avn Bde" ;
	<http://sw.cyc.com/2006/07/27/cyc/quotedIsa> <http://sw.cyc.com/2006/07/27/cyc/FACToryIrrelevantTerm> .

<http://sw.cyc.com/2006/07/27/cyc/AviationUnit-MilitarySpecialty> <http://www.w3.org/2000/01/rdf-schema#comment> "The collection of instances of #$ModernMilitaryUnit-Deployable that rely on the use of #$MilitaryAircraft for closing with and engaging the enemy. Instances of #$AviationUnit-MilitarySpecialty include attack, reconnaissance and transport units." ;
	a <http://sw.cyc.com/2006/07/27/cyc/KEClarifyingCollectionType> , <http://sw.cyc.com/2006/07/27/cyc/MilitaryUnitSpecialtyType> , <http://sw.cyc.com/2006/07/27/cyc/GenericMilitaryOrganizations-Organization-Topic> , <http://sw.cyc.com/2006/07/27/cyc/MilitaryOrganizationConcept> , <http://sw.cyc.com/2006/07/27/cyc/CPOF-UnitSpecialtyClassificationType> ;
	<http://sw.cyc.com/2006/07/27/cyc/prettyString-Canonical> "aviation unit" ;
	<http://sw.cyc.com/2006/07/27/cyc/prettyString> "air unit" , "air units" , "aviation units" ;
	<http://www.w3.org/2000/01/rdf-schema#subClassOf> <http://sw.cyc.com/2006/07/27/cyc/ModernMilitaryUnit-Deployable> .

<http://sw.cyc.com/2006/07/27/cyc/54thChemCo-RRS> a <http://sw.cyc.com/2006/07/27/cyc/Individual> , <http://sw.cyc.com/2006/07/27/cyc/BlueUnit> , <http://sw.cyc.com/2006/07/27/cyc/Company-MilitaryEchelon> , <http://sw.cyc.com/2006/07/27/cyc/ChemicalWeaponsUnit-MilitarySpecialty> ;
	<http://sw.cyc.com/2006/07/27/cyc/prettyString-Canonical> "54th Cml Co" ;
	<http://sw.cyc.com/2006/07/27/cyc/quotedIsa> <http://sw.cyc.com/2006/07/27/cyc/FACToryIrrelevantTerm> .

<http://sw.cyc.com/2006/07/27/cyc/Company-MilitaryEchelon> <http://www.w3.org/2000/01/rdf-schema#comment> """A #$MilitaryUnitTypeByEchelon and a subcollection of #$ModernMilitaryOrganization. #$Company-MilitaryEchelon is and an instance of both #$USArmyEchelon and #$USMarineCorpsEchelon.  
<p>
In the US Army, a company consists of between 60 and 190 soldiers, and is typically made up of three to five platoons (see #$Platoon-MilitaryEchelon).  Two to five companies typically make up an army #$Battalion-MilitaryEchelon.
<p>
In the US Marine Corps, a company consists of roughly 240 marines, and is typically made up of four platoons.  Five companies typically make up a marine #$Battalion-MilitaryEchelon.""" ;
	a <http://sw.cyc.com/2006/07/27/cyc/GenericMilitaryOrganizations-Organization-Topic> , <http://sw.cyc.com/2006/07/27/cyc/MilitaryOrganizationConcept> , <http://sw.cyc.com/2006/07/27/cyc/IranianArmyEchelon> , <http://sw.cyc.com/2006/07/27/cyc/USArmyEchelon> , <http://sw.cyc.com/2006/07/27/cyc/BPVEchelon> , <http://sw.cyc.com/2006/07/27/cyc/USMarineCorpsEchelon> ;
	<http://sw.cyc.com/2006/07/27/cyc/prettyString-Canonical> "military company" ;
	<http://sw.cyc.com/2006/07/27/cyc/prettyString> "company" , "companies" , "military companies" ;
	<http://www.w3.org/2000/01/rdf-schema#subClassOf> <http://sw.cyc.com/2006/07/27/cyc/ModernMilitaryOrganization> , <http://sw.cyc.com/2006/07/27/cyc/CPOF-MilitaryUnit> .

<http://sw.cyc.com/2006/07/27/cyc/ChemicalWeaponsUnit-MilitarySpecialty> <http://www.w3.org/2000/01/rdf-schema#comment> "The collection of all military unit that has been organized, equipped,           and trained for operations involving the handling, employment,           and/or containment of chemical weapons." ;
	a <http://sw.cyc.com/2006/07/27/cyc/KEClarifyingCollectionType> , <http://sw.cyc.com/2006/07/27/cyc/MilitaryUnitSpecialtyType> , <http://sw.cyc.com/2006/07/27/cyc/GenericMilitaryOrganizations-Organization-Topic> , <http://sw.cyc.com/2006/07/27/cyc/MilitaryOrganizationConcept> ;
	<http://sw.cyc.com/2006/07/27/cyc/prettyString-Canonical> "chemical weapons unit" ;
	<http://sw.cyc.com/2006/07/27/cyc/prettyString> "chemical weapons units" ;
	<http://www.w3.org/2000/01/rdf-schema#subClassOf> <http://sw.cyc.com/2006/07/27/cyc/WeaponsUnit-MilitarySpecialty> .

<http://sw.cyc.com/2006/07/27/cyc/54thDivisionArtillery-RRS> a <http://sw.cyc.com/2006/07/27/cyc/Individual> , <http://sw.cyc.com/2006/07/27/cyc/BlueUnit> , <http://sw.cyc.com/2006/07/27/cyc/Brigade-MilitaryEchelon> , <http://sw.cyc.com/2006/07/27/cyc/FieldArtilleryUnit-MilitarySpecialty> ;
	<http://sw.cyc.com/2006/07/27/cyc/prettyString-Canonical> "54th DIVARTY" ;
	<http://sw.cyc.com/2006/07/27/cyc/quotedIsa> <http://sw.cyc.com/2006/07/27/cyc/FACToryIrrelevantTerm> .

<http://sw.cyc.com/2006/07/27/cyc/54-TheMovie> <http://www.w3.org/2000/01/rdf-schema#comment> "The movie starring Mike Meyers and Salma Hayek." ;
	a <http://sw.cyc.com/2006/07/27/cyc/Individual> , <http://sw.cyc.com/2006/07/27/cyc/Movie-CW> ;
	<http://sw.cyc.com/2006/07/27/cyc/prettyString-Canonical> "54" ;
	<http://sw.cyc.com/2006/07/27/cyc/prettyString> "Studio 54" .

<http://sw.cyc.com/2006/07/27/cyc/54thEngineerBde-RRS> a <http://sw.cyc.com/2006/07/27/cyc/Individual> , <http://sw.cyc.com/2006/07/27/cyc/BlueUnit> , <http://sw.cyc.com/2006/07/27/cyc/EngineeringUnit-MilitarySpecialty> , <http://sw.cyc.com/2006/07/27/cyc/Brigade-MilitaryEchelon> ;
	<http://sw.cyc.com/2006/07/27/cyc/prettyString-Canonical> "54th Engr Bde" ;
	<http://sw.cyc.com/2006/07/27/cyc/quotedIsa> <http://sw.cyc.com/2006/07/27/cyc/FACToryIrrelevantTerm> .

<http://sw.cyc.com/2006/07/27/cyc/54thMechInfDivision-RRS> a <http://sw.cyc.com/2006/07/27/cyc/Individual> , <http://sw.cyc.com/2006/07/27/cyc/BlueUnit> , <http://sw.cyc.com/2006/07/27/cyc/MechanizedInfantryDivision> ;
	<http://sw.cyc.com/2006/07/27/cyc/prettyString-Canonical> "54th Mech Inf Div" ;
	<http://sw.cyc.com/2006/07/27/cyc/quotedIsa> <http://sw.cyc.com/2006/07/27/cyc/FACToryIrrelevantTerm> .

<http://sw.cyc.com/2006/07/27/cyc/5-TheDigit> <http://www.w3.org/2000/01/rdf-schema#comment> "The numeral 5 of the Arabic Number system.  This is '5' as a #$Character-Abstract rather than the physical #$WrittenCharacter or the abstract mathematical #$Number-General." ;
	a <http://sw.cyc.com/2006/07/27/cyc/ArabicNumeral> ;
	<http://sw.cyc.com/2006/07/27/cyc/prettyString-Canonical> "the numeral 5" ;
	<http://sw.cyc.com/2006/07/27/cyc/prettyString> "the numerals 5" .

<http://sw.cyc.com/2006/07/27/cyc/602ProLANSUITE2000a-TheProgram> <http://www.w3.org/2000/01/rdf-schema#comment> """602Pro LAN SUITE is an application which provides connection sharing,
email and fax services for networks. Remote administration
capabilities exist through an integrated HTTP-server.""" ;
	a <http://sw.cyc.com/2006/07/27/cyc/UnversionedProgram> , <http://sw.cyc.com/2006/07/27/cyc/ServerProgram> ;
	<http://sw.cyc.com/2006/07/27/cyc/prettyString-Canonical> "Software602 602Pro LAN SUITE 2000a" .

<http://sw.cyc.com/2006/07/27/cyc/60FtDolls-MusicGroup> a <http://sw.cyc.com/2006/07/27/cyc/Individual> ;
	<http://sw.cyc.com/2006/07/27/cyc/prettyString-Canonical> "60 ft. dolls" ;
	<http://sw.cyc.com/2006/07/27/cyc/prettyString> "60 Ft Dolls" .

<http://sw.cyc.com/2006/07/27/cyc/64Mutant_Fix_article-TheSoftwarePatch> a <http://sw.cyc.com/2006/07/27/cyc/Individual> , <http://sw.cyc.com/2006/07/27/cyc/ArchitectureIndependentComputerPatchProgram> , <http://sw.cyc.com/2006/07/27/cyc/ComputerPatchProgram> ;
	<http://sw.cyc.com/2006/07/27/cyc/prettyString-Canonical> "Post-Nuke 6.4 mutant fix" .

<http://sw.cyc.com/2006/07/27/cyc/6MonthAdjustableRateLoan> <http://www.w3.org/2000/01/rdf-schema#comment> "An instance of #$AdjustableRateLoanTypeByAdjustmentPeriod.  Instances of this collection are loans whose adjustment period (c.f., #$adjustmentPeriod) is 6 months -- i.e., every 6 months, the interest rate (c.f., #$interestRate) of the loan is subject to change." ;
	a <http://sw.cyc.com/2006/07/27/cyc/AdjustableRateLoanTypeByAdjustmentPeriod> ;
	<http://sw.cyc.com/2006/07/27/cyc/prettyString-Canonical> "6 month adjustable rate loan" ;
	<http://sw.cyc.com/2006/07/27/cyc/prettyString> "semi annual adjustable rate loan" , "semi annual adjustable rate loans" , "semi-annual adjustable rate loan" , "semi-annual adjustable rate loans" , "semiannual adjustable rate loan" , "semiannual adjustable rate loans" , "six month adjustable rate loan" , "six month adjustable rate loans" , "6 month adjustable rate loans" ;
	<http://www.w3.org/2000/01/rdf-schema#subClassOf> <http://sw.cyc.com/2006/07/27/cyc/AdjustableRateLoan-ConsistentAdjustmentPeriod> .

<http://sw.cyc.com/2006/07/27/cyc/6-TheDigit> <http://www.w3.org/2000/01/rdf-schema#comment> "The numeral 6 of the Arabic Number system.  This is '6' as a #$Character-Abstract rather than the physical #$WrittenCharacter or the abstract mathematical #$Number-General." ;
	a <http://sw.cyc.com/2006/07/27/cyc/ArabicNumeral> ;
	<http://sw.cyc.com/2006/07/27/cyc/prettyString-Canonical> "the numeral 6" ;
	<http://sw.cyc.com/2006/07/27/cyc/prettyString> "the numerals 6" .

<http://sw.cyc.com/2006/07/27/cyc/701PennsylvaniaAvenueRestaurantAndBar-FoodServiceEstablishment> <http://sw.cyc.com/2006/07/27/cyc/prettyString-Canonical> "701 Pennsylvania Avenue Restaurant & Bar" .

<http://sw.cyc.com/2006/07/27/cyc/747JumboJet-TheGame> a <http://sw.cyc.com/2006/07/27/cyc/Individual> , <http://sw.cyc.com/2006/07/27/cyc/ComputerGameProgram> , <http://sw.cyc.com/2006/07/27/cyc/SimulationGameProgram> ;
	<http://sw.cyc.com/2006/07/27/cyc/prettyString-Canonical> "747 Jumbo Jet" .

<http://sw.cyc.com/2006/07/27/cyc/76MMRifledBoreCannon> <http://www.w3.org/2000/01/rdf-schema#comment> """A kind of #$Cannon
 common on #$Tank-Vehicles.""" ;
	a <http://sw.cyc.com/2006/07/27/cyc/WeaponType> , <http://sw.cyc.com/2006/07/27/cyc/ExistingObjectType> , <http://sw.cyc.com/2006/07/27/cyc/SpatiallyDisjointObjectType> ;
	<http://sw.cyc.com/2006/07/27/cyc/prettyString-Canonical> "76 mm rifled bore cannon" ;
	<http://sw.cyc.com/2006/07/27/cyc/prettyString> "76 millimeter rifled bore gun" , "76 millimeter rifled bore guns" , "76 millimeter rifled bore cannon" , "76 millimeter rifled bore cannons" , "76 mm rifled cannon" , "76 mm rifled cannons" , "76 mm rifled gun" , "76 mm rifled guns" , "76 millimeter rifled gun" , "76 millimeter rifled guns" , "76 mm rifled bore gun" , "76 mm rifled bore guns" , "76 millimeter rifled cannons" , "76 mm rifled bore cannons" ;
	<http://www.w3.org/2000/01/rdf-schema#subClassOf> <http://sw.cyc.com/2006/07/27/cyc/RifledBoreWeapon> .

<http://sw.cyc.com/2006/07/27/cyc/7-ElevenInc> a <http://sw.cyc.com/2006/07/27/cyc/Individual> , <http://sw.cyc.com/2006/07/27/cyc/PubliclyHeldCorporation> ;
	<http://sw.cyc.com/2006/07/27/cyc/prettyString-Canonical> "7 Eleven" ;
	<http://sw.cyc.com/2006/07/27/cyc/prettyString> "7 Eleven, Inc." .

<http://sw.cyc.com/2006/07/27/cyc/7-MusicGroup> a <http://sw.cyc.com/2006/07/27/cyc/Individual> ;
	<http://sw.cyc.com/2006/07/27/cyc/prettyString-Canonical> "7" .

<http://sw.cyc.com/2006/07/27/cyc/7Seconds-MusicGroup> a <http://sw.cyc.com/2006/07/27/cyc/Individual> , <http://sw.cyc.com/2006/07/27/cyc/RockMusicPerformer> , <http://sw.cyc.com/2006/07/27/cyc/Band-MusicGroup> , <http://sw.cyc.com/2006/07/27/cyc/PunkMusicPerformer> ;
	<http://sw.cyc.com/2006/07/27/cyc/prettyString-Canonical> "7 Seconds" ;
	<http://sw.cyc.com/2006/07/27/cyc/prettyString> "Seven Seconds" .

<http://sw.cyc.com/2006/07/27/cyc/RockMusicPerformer> <http://www.w3.org/2000/01/rdf-schema#comment> "The collection of individuals or groups that perform rock music." ;
	a <http://sw.cyc.com/2006/07/27/cyc/MusicalPerformanceAgentTypeByGenre> ;
	<http://sw.cyc.com/2006/07/27/cyc/prettyString-Canonical> "performer of rock music" ;
	<http://sw.cyc.com/2006/07/27/cyc/prettyString> "performers of rock music" ;
	<http://www.w3.org/2000/01/rdf-schema#subClassOf> <http://sw.cyc.com/2006/07/27/cyc/MusicPerformanceAgent> .

<http://sw.cyc.com/2006/07/27/cyc/Band-MusicGroup> <http://www.w3.org/2000/01/rdf-schema#comment> "A collection of music performance organizations.  An element of #$Band-MusicGroup is a (small or large) group of musicians who play non-Classical music together on either a regular or intermittent schedule.  For example, the #$RollingStones or the University of Texas marching band -- but not the Chicago Symphony Orchestra." ;
	a <http://sw.cyc.com/2006/07/27/cyc/ExistingObjectType> , <http://www.w3.org/2002/07/owl#Class> , <http://sw.cyc.com/2006/07/27/cyc/AtemporalNecessarilyEssentialCollectionType> , <http://sw.cyc.com/2006/07/27/cyc/KEClarifyingCollectionType> , <http://sw.cyc.com/2006/07/27/cyc/OrganizationsByFunction-Organization-Topic> ;
	<http://sw.cyc.com/2006/07/27/cyc/prettyString-Canonical> "band" ;
	<http://sw.cyc.com/2006/07/27/cyc/prettyString> "bands" ;
	<http://www.w3.org/2000/01/rdf-schema#subClassOf> <http://sw.cyc.com/2006/07/27/cyc/OrganizationOfPeopleOnly> , <http://sw.cyc.com/2006/07/27/cyc/MusicPerformanceOrganization> ;
	<http://sw.cyc.com/2006/07/27/cyc/covering> <http://sw.cyc.com/2006/07/27/cyc/MusicalPerformanceAgentTypeByGenre> .

<http://sw.cyc.com/2006/07/27/cyc/PunkMusicPerformer> <http://www.w3.org/2000/01/rdf-schema#comment> "The collection of individuals or groups that perform punk rock." ;
	a <http://sw.cyc.com/2006/07/27/cyc/MusicalPerformanceAgentTypeByGenre> ;
	<http://sw.cyc.com/2006/07/27/cyc/prettyString-Canonical> "punk music performer" ;
	<http://www.w3.org/2000/01/rdf-schema#subClassOf> <http://sw.cyc.com/2006/07/27/cyc/RockMusicPerformer> .

<http://sw.cyc.com/2006/07/27/cyc/7-TheDigit> <http://www.w3.org/2000/01/rdf-schema#comment> "The numeral 7 of the Arabic Number system.  This is '7' as a #$Character-Abstract rather than the physical #$WrittenCharacter or the abstract mathematical #$Number-General." ;
	a <http://sw.cyc.com/2006/07/27/cyc/ArabicNumeral> ;
	<http://sw.cyc.com/2006/07/27/cyc/prettyString-Canonical> "the numeral 7" ;
	<http://sw.cyc.com/2006/07/27/cyc/prettyString> "the numerals 7" .

<http://sw.cyc.com/2006/07/27/cyc/7thHeaven-TheTVShow> a <http://sw.cyc.com/2006/07/27/cyc/Individual> , <http://sw.cyc.com/2006/07/27/cyc/TVSeriesProduct> ;
	<http://sw.cyc.com/2006/07/27/cyc/prettyString-Canonical> "7th Heaven" .

<http://sw.cyc.com/2006/07/27/cyc/7thLevelInc> a <http://sw.cyc.com/2006/07/27/cyc/Individual> , <http://sw.cyc.com/2006/07/27/cyc/PubliclyHeldCorporation> ;
	<http://sw.cyc.com/2006/07/27/cyc/prettyString-Canonical> "7th Level, Inc." ;
	<http://sw.cyc.com/2006/07/27/cyc/prettyString> "7th Level" .

<http://sw.cyc.com/2006/07/27/cyc/7YearBitch-MusicGroup> a <http://sw.cyc.com/2006/07/27/cyc/Individual> ;
	<http://sw.cyc.com/2006/07/27/cyc/prettyString-Canonical> "7 Year Bitch" .

<http://sw.cyc.com/2006/07/27/cyc/800-JRCigarInc> a <http://sw.cyc.com/2006/07/27/cyc/Individual> , <http://sw.cyc.com/2006/07/27/cyc/PubliclyHeldCorporation> ;
	<http://sw.cyc.com/2006/07/27/cyc/prettyString-Canonical> "800 JR Cigar, Inc." ;
	<http://sw.cyc.com/2006/07/27/cyc/prettyString> "800 JR Cigar" .

<http://sw.cyc.com/2006/07/27/cyc/802-11WirelessLANProtocol> a <http://sw.cyc.com/2006/07/27/cyc/InternetStandard> , <http://sw.cyc.com/2006/07/27/cyc/PhysicalLayerProtocol> , <http://sw.cyc.com/2006/07/27/cyc/MediumAccessControlSublayerProtocol> ;
	<http://sw.cyc.com/2006/07/27/cyc/prettyString-Canonical> "IEEE 802.11 Wireless LAN Protocol" ;
	<http://sw.cyc.com/2006/07/27/cyc/prettyString> "Wireless LAN" , "IEEE 802.11" .

<http://sw.cyc.com/2006/07/27/cyc/InternetStandard> <http://www.w3.org/2000/01/rdf-schema#comment> "An internet standard is a kind of product specification, applicable to #$NetworkingPrograms, concerning how the product behaves in the #$Internet environment." ;
	a <http://sw.cyc.com/2006/07/27/cyc/ObjectType> ;
	<http://sw.cyc.com/2006/07/27/cyc/prettyString-Canonical> "Internet standard" ;
	<http://sw.cyc.com/2006/07/27/cyc/prettyString> "Internet standards" ;
	<http://www.w3.org/2000/01/rdf-schema#subClassOf> <http://sw.cyc.com/2006/07/27/cyc/ProductStandard> .

<http://sw.cyc.com/2006/07/27/cyc/PhysicalLayerProtocol> <http://www.w3.org/2000/01/rdf-schema#comment> "The collection of all network protocols that implement a physical layer. An instance of #$PhysicalLayerProtocol is the  connector between nodes in a network,  or the medium through which data physically travels." ;
	a <http://sw.cyc.com/2006/07/27/cyc/ObjectType> ;
	<http://sw.cyc.com/2006/07/27/cyc/prettyString-Canonical> "physical layer protocol" ;
	<http://sw.cyc.com/2006/07/27/cyc/prettyString> "physical layer protocols" ;
	<http://www.w3.org/2000/01/rdf-schema#subClassOf> <http://sw.cyc.com/2006/07/27/cyc/ProtocolStackLayer> .

<http://sw.cyc.com/2006/07/27/cyc/MediumAccessControlSublayerProtocol> <http://www.w3.org/2000/01/rdf-schema#comment> """An instance of #$MediumAccessControlSublayerProtocol is a sublayer of an
instance of #$DataLinkLayerProtocol. A #$MediumAccessControlSublayerProtocol is used in 
broadcast networks to prevent collisions. Collisions occur when two or 
more machines attempt to send data at the same time.""" ;
	a <http://sw.cyc.com/2006/07/27/cyc/ObjectType> ;
	<http://sw.cyc.com/2006/07/27/cyc/prettyString-Canonical> "MAC" ;
	<http://www.w3.org/2000/01/rdf-schema#subClassOf> <http://sw.cyc.com/2006/07/27/cyc/ProtocolStackLayer> .

<http://sw.cyc.com/2006/07/27/cyc/81stMeridian-West> <http://www.w3.org/2000/01/rdf-schema#comment> "The 81st meridian west of the #$PrimeMeridian of #$PlanetEarth." ;
	a <http://sw.cyc.com/2006/07/27/cyc/Individual> , <http://sw.cyc.com/2006/07/27/cyc/LongitudeLine> ;
	<http://sw.cyc.com/2006/07/27/cyc/prettyString-Canonical> "81st Meridian West" .

<http://sw.cyc.com/2006/07/27/cyc/LongitudeLine> <http://www.w3.org/2000/01/rdf-schema#comment> "A line between the North Pole (see #$AxialNorthPoleOfEarth) and the South Pole (see #$AxialSouthPoleOfEarth), intersecting the #$EarthsEquator at 90 degrees." ;
	a <http://sw.cyc.com/2006/07/27/cyc/SpatiallyDisjointObjectType> , <http://sw.cyc.com/2006/07/27/cyc/TemporalStuffType> , <http://sw.cyc.com/2006/07/27/cyc/CartographicFeatureType> ;
	<http://sw.cyc.com/2006/07/27/cyc/prettyString-Canonical> "line of longitude" ;
	<http://sw.cyc.com/2006/07/27/cyc/prettyString> "longitude" , "meridian" , "meridians" , "lines of longitude" ;
	<http://www.w3.org/2000/01/rdf-schema#subClassOf> <http://sw.cyc.com/2006/07/27/cyc/GeographicalPlace-1D> , <http://sw.cyc.com/2006/07/27/cyc/Semiellipse> .

<http://sw.cyc.com/2006/07/27/cyc/82ndMeridian-West> <http://www.w3.org/2000/01/rdf-schema#comment> "The meridian." , "The 82nd meridian west of the #$PrimeMeridian of #$PlanetEarth." ;
	a <http://sw.cyc.com/2006/07/27/cyc/Individual> , <http://sw.cyc.com/2006/07/27/cyc/LongitudeLine> ;
	<http://sw.cyc.com/2006/07/27/cyc/prettyString-Canonical> "82nd Meridian West" .

<http://sw.cyc.com/2006/07/27/cyc/83rdMeridian-West> <http://www.w3.org/2000/01/rdf-schema#comment> "The 83rd meridian west of the #$PrimeMeridian of #$PlanetEarth." ;
	a <http://sw.cyc.com/2006/07/27/cyc/Individual> ;
	<http://sw.cyc.com/2006/07/27/cyc/prettyString-Canonical> "83rd Meridian West" .

<http://sw.cyc.com/2006/07/27/cyc/84thMeridian-West> <http://www.w3.org/2000/01/rdf-schema#comment> "The 84th meridian west of the #$PrimeMeridian of #$PlanetEarth." ;
	a <http://sw.cyc.com/2006/07/27/cyc/Individual> , <http://sw.cyc.com/2006/07/27/cyc/LongitudeLine> ;
	<http://sw.cyc.com/2006/07/27/cyc/prettyString-Canonical> "84th Meridian West" .

<http://sw.cyc.com/2006/07/27/cyc/85MMSmoothBoreCannon> <http://www.w3.org/2000/01/rdf-schema#comment> """A kind of #$Cannon
 common on #$Tank-Vehicles.""" ;
	a <http://sw.cyc.com/2006/07/27/cyc/WeaponType> , <http://sw.cyc.com/2006/07/27/cyc/ExistingObjectType> ;
	<http://sw.cyc.com/2006/07/27/cyc/prettyString-Canonical> "85 mm smooth bore cannon" ;
	<http://sw.cyc.com/2006/07/27/cyc/prettyString> "85 millimeter smooth bore gun" , "85 millimeter smooth bore guns" , "85 mm smooth bore gun" , "85 mm smooth bore guns" , "85 millimeter smooth bore cannon" , "85 millimeter smooth bore cannons" , "85 mm smooth bore cannons" ;
	<http://www.w3.org/2000/01/rdf-schema#subClassOf> <http://sw.cyc.com/2006/07/27/cyc/TankCannon> , <http://sw.cyc.com/2006/07/27/cyc/SmoothBoreWeapon> .

<http://sw.cyc.com/2006/07/27/cyc/85thMeridian-West> <http://www.w3.org/2000/01/rdf-schema#comment> "The 85th meridian west of the #$PrimeMeridian of #$PlanetEarth." ;
	a <http://sw.cyc.com/2006/07/27/cyc/Individual> , <http://sw.cyc.com/2006/07/27/cyc/LongitudeLine> ;
	<http://sw.cyc.com/2006/07/27/cyc/prettyString-Canonical> "85th Meridian West" .

<http://sw.cyc.com/2006/07/27/cyc/86thMeridian-West> <http://www.w3.org/2000/01/rdf-schema#comment> "The 86th meridian west of the #$PrimeMeridian of #$PlanetEarth." ;
	a <http://sw.cyc.com/2006/07/27/cyc/Individual> , <http://sw.cyc.com/2006/07/27/cyc/LongitudeLine> ;
	<http://sw.cyc.com/2006/07/27/cyc/prettyString-Canonical> "86th Meridian West" .

<http://sw.cyc.com/2006/07/27/cyc/87thMeridian-West> <http://www.w3.org/2000/01/rdf-schema#comment> "The 87th meridian west of the #$PrimeMeridian of #$PlanetEarth." ;
	a <http://sw.cyc.com/2006/07/27/cyc/Individual> , <http://sw.cyc.com/2006/07/27/cyc/LongitudeLine> ;
	<http://sw.cyc.com/2006/07/27/cyc/prettyString-Canonical> "87th Meridian West" .

<http://sw.cyc.com/2006/07/27/cyc/88thMeridian-West> <http://www.w3.org/2000/01/rdf-schema#comment> "The 88th meridian west of the #$PrimeMeridian of #$PlanetEarth." ;
	a <http://sw.cyc.com/2006/07/27/cyc/Individual> , <http://sw.cyc.com/2006/07/27/cyc/LongitudeLine> ;
	<http://sw.cyc.com/2006/07/27/cyc/prettyString-Canonical> "88th Meridian West" .

<http://sw.cyc.com/2006/07/27/cyc/89thMeridian-West> <http://www.w3.org/2000/01/rdf-schema#comment> "The 89th meridian west of the #$PrimeMeridian of #$PlanetEarth." ;
	a <http://sw.cyc.com/2006/07/27/cyc/Individual> , <http://sw.cyc.com/2006/07/27/cyc/LongitudeLine> ;
	<http://sw.cyc.com/2006/07/27/cyc/prettyString-Canonical> "89th Meridian West" .

<http://sw.cyc.com/2006/07/27/cyc/8ByteIntegerDatatype> <http://www.w3.org/2000/01/rdf-schema#comment> "The collection of all computer data types that employ exactly 8 bytes to represent some subset of the integers or values related to represnting integer values such as NAN. Note that this does not specify, for example, whether the data type represents positive integers only, or is in two's complement representation." ;
	a <http://sw.cyc.com/2006/07/27/cyc/FixedSizeComputerDatatypeType> , <http://sw.cyc.com/2006/07/27/cyc/SKSIDataTypeDescriptions-Topic> ;
	<http://sw.cyc.com/2006/07/27/cyc/prettyString-Canonical> "8-byte integer" ;
	<http://sw.cyc.com/2006/07/27/cyc/prettyString> "eight-byte integer" , "eight-byte integers" , "8-byte integers" ;
	<http://www.w3.org/2000/01/rdf-schema#subClassOf> <http://sw.cyc.com/2006/07/27/cyc/IntegerComputerNumber> , <http://sw.cyc.com/2006/07/27/cyc/ProgramObject> .

<http://sw.cyc.com/2006/07/27/cyc/8ByteRealDatatype> <http://www.w3.org/2000/01/rdf-schema#comment> "The collection of all computer data types that employ exactly 8 bytes to represent some subset of the real numbers." ;
	a <http://sw.cyc.com/2006/07/27/cyc/FixedSizeComputerDatatypeType> ;
	<http://sw.cyc.com/2006/07/27/cyc/prettyString-Canonical> "8 byte real datatype" ;
	<http://www.w3.org/2000/01/rdf-schema#subClassOf> <http://sw.cyc.com/2006/07/27/cyc/RealNumberDatatype> .

<http://sw.cyc.com/2006/07/27/cyc/8ByteTwosComplementInteger> a <http://sw.cyc.com/2006/07/27/cyc/TwosComplementIntegerDatatype> , <http://sw.cyc.com/2006/07/27/cyc/8ByteIntegerDatatype> ;
	<http://sw.cyc.com/2006/07/27/cyc/prettyString-Canonical> "8 Byte Twos Complement Integer" .

<http://sw.cyc.com/2006/07/27/cyc/8MMCamcorder> <http://www.w3.org/2000/01/rdf-schema#comment> """Camcorders which record on #$8MMCassettes.  These
types of #$AmateurVideoCameras usually need to be hooked up to the TV
directly to view the tapes.""" ;
	a <http://sw.cyc.com/2006/07/27/cyc/ExistingObjectType> , <http://sw.cyc.com/2006/07/27/cyc/SpatiallyDisjointObjectType> , <http://sw.cyc.com/2006/07/27/cyc/ArtifactTypeByGenericCategory> , <http://sw.cyc.com/2006/07/27/cyc/ManufacturedGoodsType> ;
	<http://sw.cyc.com/2006/07/27/cyc/prettyString-Canonical> "8mm camcorder" ;
	<http://sw.cyc.com/2006/07/27/cyc/prettyString> "8mm camcorders" ;
	<http://www.w3.org/2000/01/rdf-schema#subClassOf> <http://sw.cyc.com/2006/07/27/cyc/ManufacturedGoods> , <http://sw.cyc.com/2006/07/27/cyc/AmateurVideoCamera> .

<http://sw.cyc.com/2006/07/27/cyc/AmateurVideoCamera> <http://www.w3.org/2000/01/rdf-schema#comment> "The class of #$VideoCameras used by amateurs." ;
	a <http://sw.cyc.com/2006/07/27/cyc/ExistingObjectType> , <http://sw.cyc.com/2006/07/27/cyc/SpatiallyDisjointObjectType> , <http://sw.cyc.com/2006/07/27/cyc/ArtifactTypeByGenericCategory> , <http://sw.cyc.com/2006/07/27/cyc/ManufacturedGoodsType> ;
	<http://sw.cyc.com/2006/07/27/cyc/prettyString-Canonical> "camcorder" ;
	<http://sw.cyc.com/2006/07/27/cyc/prettyString> "cams" , "Cam" , "amateur video camera" , "amateur video cameras" , "camcorders" ;
	<http://www.w3.org/2000/01/rdf-schema#subClassOf> <http://sw.cyc.com/2006/07/27/cyc/ManufacturedGoods> , <http://sw.cyc.com/2006/07/27/cyc/VideoCamera> .

<http://sw.cyc.com/2006/07/27/cyc/ArtifactTypeByGenericCategory> <http://www.w3.org/2000/01/rdf-schema#comment> "An instance of #$SecondOrderCollection and a specialization of #$ArtifactType.  Each instance of #$ArtifactTypeByGenericCategory is a collection of #$Artifacts grouped together according to some feature(s) other than brand or model." ;
	a <http://sw.cyc.com/2006/07/27/cyc/SecondOrderCollection> ;
	<http://sw.cyc.com/2006/07/27/cyc/prettyString-Canonical> "kind of artifact not distinguished by brand or model" ;
	<http://sw.cyc.com/2006/07/27/cyc/prettyString> "kinds of artifact not distinguished by brand or model" ;
	<http://www.w3.org/2000/01/rdf-schema#subClassOf> <http://sw.cyc.com/2006/07/27/cyc/KEClarifyingCollectionType> , <http://sw.cyc.com/2006/07/27/cyc/ArtifactType> .

<http://sw.cyc.com/2006/07/27/cyc/ManufacturedGoodsType> <http://www.w3.org/2000/01/rdf-schema#comment> "The collection of all types of #$PartiallyTangible things that are usually/frequently commercially manufactured.  This is context dependent." ;
	a <http://sw.cyc.com/2006/07/27/cyc/AtemporalNecessarilyEssentialCollectionType> , <http://sw.cyc.com/2006/07/27/cyc/SecondOrderCollection> ;
	<http://sw.cyc.com/2006/07/27/cyc/prettyString-Canonical> "product type" ;
	<http://sw.cyc.com/2006/07/27/cyc/prettyString> "products" , "manufactured goods" , "product" , "product types" , "type of manufactured goods" , "types of manufactured goods" ;
	<http://www.w3.org/2000/01/rdf-schema#subClassOf> <http://sw.cyc.com/2006/07/27/cyc/FacetInstanceCollection> , <http://sw.cyc.com/2006/07/27/cyc/ArtifactType> , <http://sw.cyc.com/2006/07/27/cyc/TimeDependentCollection> ;
	<http://sw.cyc.com/2006/07/27/cyc/sharedNotes> <http://sw.cyc.com/2006/07/27/cyc/SharedNoteOnGenlsRelationsBetweenFacetingCollectionTypes> ;
	<http://www.w3.org/2002/07/owl#disjointWith> <http://sw.cyc.com/2006/07/27/cyc/PersonTypeByReligiousBackground> , <http://sw.cyc.com/2006/07/27/cyc/ServiceTypeFrequentlyForSale> ;
	<http://sw.cyc.com/2006/07/27/cyc/typeGenls> <http://sw.cyc.com/2006/07/27/cyc/ManufacturedGoods> .

<http://sw.cyc.com/2006/07/27/cyc/8MMCassette> <http://www.w3.org/2000/01/rdf-schema#comment> """8mm video cassettes.  Typically used only for
#$AmateurVideoCameras but usually of higher quality than other video medias
available to the amateur.  Must be played back from #$8MMCamcorder or copied to
a #$VHSCassette for playback on a #$VideoCassetteRecorder.""" ;
	a <http://sw.cyc.com/2006/07/27/cyc/ExistingObjectType> , <http://sw.cyc.com/2006/07/27/cyc/SpatiallyDisjointObjectType> , <http://sw.cyc.com/2006/07/27/cyc/ArtifactTypeByGenericCategory> ;
	<http://sw.cyc.com/2006/07/27/cyc/prettyString-Canonical> "8 mm cassette" ;
	<http://sw.cyc.com/2006/07/27/cyc/prettyString> "8 mm cassettes" ;
	<http://www.w3.org/2000/01/rdf-schema#subClassOf> <http://sw.cyc.com/2006/07/27/cyc/VideoCassette> .

<http://sw.cyc.com/2006/07/27/cyc/VideoCassette> <http://www.w3.org/2000/01/rdf-schema#comment> "Video cassette tapes, blank or not." ;
	a <http://sw.cyc.com/2006/07/27/cyc/ExistingObjectType> , <http://sw.cyc.com/2006/07/27/cyc/SpatiallyDisjointObjectType> , <http://sw.cyc.com/2006/07/27/cyc/ArtifactTypeByGenericCategory> ;
	<http://sw.cyc.com/2006/07/27/cyc/prettyString-Canonical> "videotape" ;
	<http://sw.cyc.com/2006/07/27/cyc/prettyString> "videotapes" , "video cassette" , "video cassettes" , "video" , "videos" ;
	<http://www.w3.org/2000/01/rdf-schema#subClassOf> <http://sw.cyc.com/2006/07/27/cyc/MagneticTapeCassette> .

<http://sw.cyc.com/2006/07/27/cyc/8-TheDigit> <http://www.w3.org/2000/01/rdf-schema#comment> "The numeral 8 of the Arabic Number system.  This is '8' as a #$Character-Abstract rather than the physical #$WrittenCharacter or the abstract mathematical #$Number-General." ;
	a <http://sw.cyc.com/2006/07/27/cyc/ArabicNumeral> ;
	<http://sw.cyc.com/2006/07/27/cyc/prettyString-Canonical> "the numeral 8" ;
	<http://sw.cyc.com/2006/07/27/cyc/prettyString> "the numerals 8" .

<http://sw.cyc.com/2006/07/27/cyc/8x8Inc> a <http://sw.cyc.com/2006/07/27/cyc/Individual> , <http://sw.cyc.com/2006/07/27/cyc/PubliclyHeldCorporation> ;
	<http://sw.cyc.com/2006/07/27/cyc/prettyString-Canonical> "8x 8, Inc." ;
	<http://sw.cyc.com/2006/07/27/cyc/prettyString> "8x 8" .

<http://sw.cyc.com/2006/07/27/cyc/9003Inc> a <http://sw.cyc.com/2006/07/27/cyc/Individual> , <http://sw.cyc.com/2006/07/27/cyc/SoftwareVendor> ;
	<http://sw.cyc.com/2006/07/27/cyc/prettyString-Canonical> "9003inc." .

<http://sw.cyc.com/2006/07/27/cyc/90thMeridian-West> <http://www.w3.org/2000/01/rdf-schema#comment> "The 90th meridian west of the #$PrimeMeridian of #$PlanetEarth." ;
	a <http://sw.cyc.com/2006/07/27/cyc/Individual> , <http://sw.cyc.com/2006/07/27/cyc/LongitudeLine> ;
	<http://sw.cyc.com/2006/07/27/cyc/prettyString-Canonical> "90th Meridian West" .

<http://sw.cyc.com/2006/07/27/cyc/989Studios> a <http://sw.cyc.com/2006/07/27/cyc/Individual> , <http://sw.cyc.com/2006/07/27/cyc/SoftwareVendor> ;
	<http://sw.cyc.com/2006/07/27/cyc/prettyString-Canonical> "989 Studios" .

<http://sw.cyc.com/2006/07/27/cyc/9-TheDigit> <http://www.w3.org/2000/01/rdf-schema#comment> "The numeral 9 of the Arabic Number system.  This is '9' as a #$Character-Abstract rather than the physical #$WrittenCharacter or the abstract mathematical #$Number-General." ;
	a <http://sw.cyc.com/2006/07/27/cyc/ArabicNumeral> ;
	<http://sw.cyc.com/2006/07/27/cyc/prettyString-Canonical> "the numeral 9" ;
	<http://sw.cyc.com/2006/07/27/cyc/prettyString> "the numerals 9" .

<http://sw.cyc.com/2006/07/27/cyc/A-123Engr-RRS> a <http://sw.cyc.com/2006/07/27/cyc/Individual> , <http://sw.cyc.com/2006/07/27/cyc/BlueUnit> , <http://sw.cyc.com/2006/07/27/cyc/EngineeringUnit-MilitarySpecialty> , <http://sw.cyc.com/2006/07/27/cyc/Company-MilitaryEchelon> ;
	<http://sw.cyc.com/2006/07/27/cyc/prettyString-Canonical> "A/123 Engr" ;
	<http://sw.cyc.com/2006/07/27/cyc/quotedIsa> <http://sw.cyc.com/2006/07/27/cyc/FACToryIrrelevantTerm> .

<http://sw.cyc.com/2006/07/27/cyc/A1Stats-TheProgram> a <http://sw.cyc.com/2006/07/27/cyc/UnversionedProgram> , <http://sw.cyc.com/2006/07/27/cyc/LocalProgram> , <http://sw.cyc.com/2006/07/27/cyc/UserProgram> ;
	<http://sw.cyc.com/2006/07/27/cyc/prettyString-Canonical> "Drummond Miles A1Stats" .

<http://sw.cyc.com/2006/07/27/cyc/A1WebServer-TheProgram> a <http://sw.cyc.com/2006/07/27/cyc/Individual> , <http://sw.cyc.com/2006/07/27/cyc/UnversionedProgram> , <http://sw.cyc.com/2006/07/27/cyc/WorldWideWebServerProgram> , <http://sw.cyc.com/2006/07/27/cyc/ServiceProgram> ;
	<http://sw.cyc.com/2006/07/27/cyc/prettyString-Canonical> "Robin Twombly A1 Web Server" .

<http://sw.cyc.com/2006/07/27/cyc/ServiceProgram> <http://www.w3.org/2000/01/rdf-schema#comment> "#$ServiceProgram is a specialization of #$ComputerProgram-CW.  It is the collection of programs whose associated running processes computer users typically do not interact with.  The configuration of these programs occurs at the system level and is typically not alterable at the user level.  For example, #$OpenSSH-TheProgram (sshd) has options that are configurable at the system level in a central location by someone with appropriate privileges, and whenever a user runs a process associated with that centrally configured program, the program's system configuration applies.  Note that #$UserProgram and #$ServiceProgram partition #$ComputerProgram-CW." ;
	a <http://www.w3.org/2002/07/owl#Class> , <http://sw.cyc.com/2006/07/27/cyc/ObjectType> , <http://sw.cyc.com/2006/07/27/cyc/AtemporalNecessarilyEssentialCollectionType> , <http://sw.cyc.com/2006/07/27/cyc/TemporalStuffType> ;
	<http://sw.cyc.com/2006/07/27/cyc/prettyString-Canonical> "daemon" ;
	<http://sw.cyc.com/2006/07/27/cyc/prettyString> "service programme" , "service program" , "service programs" , "service programz" , "daemons" ;
	<http://www.w3.org/2000/01/rdf-schema#subClassOf> <http://sw.cyc.com/2006/07/27/cyc/ApplicationProgram> ;
	<http://www.w3.org/2002/07/owl#disjointWith> <http://sw.cyc.com/2006/07/27/cyc/IndependentThing> .

<http://sw.cyc.com/2006/07/27/cyc/A2ps-TheSoftwarePackage> a <http://sw.cyc.com/2006/07/27/cyc/Individual> , <http://sw.cyc.com/2006/07/27/cyc/UnversionedProgram> , <http://sw.cyc.com/2006/07/27/cyc/PrintingProgram> , <http://sw.cyc.com/2006/07/27/cyc/SoftwarePackage> , <http://sw.cyc.com/2006/07/27/cyc/FileTranslationProgram> ;
	<http://sw.cyc.com/2006/07/27/cyc/prettyString-Canonical> "a2ps" .

<http://sw.cyc.com/2006/07/27/cyc/PrintingProgram> <http://www.w3.org/2000/01/rdf-schema#comment> "The collection of programs that send data to be printed to a printer." ;
	a <http://sw.cyc.com/2006/07/27/cyc/KEClarifyingCollectionType> , <http://sw.cyc.com/2006/07/27/cyc/ComputerProgramTypeByFunction> ;
	<http://sw.cyc.com/2006/07/27/cyc/prettyString-Canonical> "printing program" ;
	<http://sw.cyc.com/2006/07/27/cyc/prettyString> "printing programme" , "printing programs" , "printing programz" ;
	<http://www.w3.org/2000/01/rdf-schema#subClassOf> <http://sw.cyc.com/2006/07/27/cyc/UtilityProgram> .

<http://sw.cyc.com/2006/07/27/cyc/SoftwarePackage> <http://www.w3.org/2000/01/rdf-schema#comment> "#$SoftwarePackage is the collection of programs composed of loosely coupled component programs, possibly including an #$OperatingSystem, libraries, tool sets, or \"system software\"." ;
	a <http://www.w3.org/2002/07/owl#Class> , <http://sw.cyc.com/2006/07/27/cyc/ObjectType> , <http://sw.cyc.com/2006/07/27/cyc/AtemporalNecessarilyEssentialCollectionType> ;
	<http://sw.cyc.com/2006/07/27/cyc/prettyString-Canonical> "software package" ;
	<http://sw.cyc.com/2006/07/27/cyc/prettyString> "software packages" ;
	<http://www.w3.org/2000/01/rdf-schema#subClassOf> <http://sw.cyc.com/2006/07/27/cyc/SoftwareObject-Individual> .

<http://sw.cyc.com/2006/07/27/cyc/FileTranslationProgram> <http://www.w3.org/2000/01/rdf-schema#comment> "The subcollection of #$ComputerProgram-CWs whose instantiations alter the #$ComputerFileTypeByFormat of instances of #$ComputerFileCopy in some way. Typically instances of this collection will be programs which translate a file from one file format to another (#$JPEGFile to #$GIFFile for example).  The basic data is preserved in the translation, only the format in which the data is saved is changed." ;
	a <http://www.w3.org/2002/07/owl#Class> , <http://sw.cyc.com/2006/07/27/cyc/AtemporalNecessarilyEssentialCollectionType> , <http://sw.cyc.com/2006/07/27/cyc/KEClarifyingCollectionType> , <http://sw.cyc.com/2006/07/27/cyc/ComputerProgramTypeByFunction> ;
	<http://sw.cyc.com/2006/07/27/cyc/prettyString-Canonical> "file translation program" ;
	<http://sw.cyc.com/2006/07/27/cyc/prettyString> "file translation software" , "file translation programme" , "file translation programs" , "file translation programz" ;
	<http://www.w3.org/2000/01/rdf-schema#subClassOf> <http://sw.cyc.com/2006/07/27/cyc/UtilityProgram> .

<http://sw.cyc.com/2006/07/27/cyc/A2p-TheProgram> a <http://sw.cyc.com/2006/07/27/cyc/Individual> , <http://sw.cyc.com/2006/07/27/cyc/UnversionedProgram> , <http://sw.cyc.com/2006/07/27/cyc/LocalProgram> , <http://sw.cyc.com/2006/07/27/cyc/FileTranslationProgram> ;
	<http://sw.cyc.com/2006/07/27/cyc/prettyString-Canonical> "a2p" .

<http://sw.cyc.com/2006/07/27/cyc/A-5C-Fighter> <http://www.w3.org/2000/01/rdf-schema#comment> """A class of #$FighterPlane 
 currently (2000) used by #$China-PeoplesRepublic.""" ;
	a <http://sw.cyc.com/2006/07/27/cyc/WeaponType> , <http://sw.cyc.com/2006/07/27/cyc/ExistingObjectType> , <http://sw.cyc.com/2006/07/27/cyc/SpatiallyDisjointObjectType> , <http://sw.cyc.com/2006/07/27/cyc/ProductTypeByBrandVersion> .

<http://sw.cyc.com/2006/07/27/cyc/ComputerScienceConference> <http://www.w3.org/2000/01/rdf-schema#comment> "The collection of all #$ScientificConference dealing specifically with computer science." ;
	a <http://sw.cyc.com/2006/07/27/cyc/FirstOrderCollection> ;
	<http://sw.cyc.com/2006/07/27/cyc/prettyString-Canonical> "computer science conference" ;
	<http://sw.cyc.com/2006/07/27/cyc/prettyString> "computer science conferences" ;
	<http://www.w3.org/2000/01/rdf-schema#subClassOf> <http://sw.cyc.com/2006/07/27/cyc/ScientificConference> .

<http://sw.cyc.com/2006/07/27/cyc/TemporalObjectType> <http://www.w3.org/2000/01/rdf-schema#comment> """A specialization of #$ObjectType (q.v.) whose instances are all and only those collections that are temporally object-like. A collection <code>COL</code> is temporally object-like just in case it generally holds that any proper purely temporal parts (see #$timeSlices) of an instance of <code>COL</code> is not itself an instance of <code>COL</code>.  More precisely, a collection <code>COL</code> is an instance of #$TemporalObjectType just in case it satisfies the following: For any distinct <code>OBJ1</code> and <code>OBJ2</code>, if <code>(#$isa OBJ1 COL)</code> and <code>(#$timeSlices OBJ1 OBJ2)</code>, then <i>not</i> <code>(#$isa OBJ2 COL)</code>.
<p>
For example, none of the proper time-slices of a #$CalendarYear is itself a calendar year.  Likewise for #$TakingAStep.  So #$CalendarYear and #$TakingAStep are both instances of #$TemporalObjectType. Conversely, a proper time-slice of a given #$Date might itself be a #$Date (e.g. an hour has minutes and seconds as time-slices); so #$Date is <i>not</i> a temporal-object-type.
<p>
See #$TemporalStuffType for the disjoint notion of being temporally stuff-like.""" ;
	a <http://www.w3.org/2002/07/owl#Class> , <http://sw.cyc.com/2006/07/27/cyc/AtemporalNecessarilyEssentialCollectionType> , <http://sw.cyc.com/2006/07/27/cyc/Time-Topic> , <http://sw.cyc.com/2006/07/27/cyc/FacetingCollectionType> , <http://sw.cyc.com/2006/07/27/cyc/SecondOrderCollection> , <http://sw.cyc.com/2006/07/27/cyc/SetOrCollection> , <http://sw.cyc.com/2006/07/27/cyc/Top-Topic> , <http://sw.cyc.com/2006/07/27/cyc/ThingsWithTemporalExtent-Time-Topic> ;
	<http://sw.cyc.com/2006/07/27/cyc/prettyString-Canonical> "temporal object type" ;
	<http://sw.cyc.com/2006/07/27/cyc/prettyString> "type of temporally object-like thing" , "types of temporally object-like thing" , "temporal object types" ;
	<http://www.w3.org/2000/01/rdf-schema#subClassOf> <http://sw.cyc.com/2006/07/27/cyc/ObjectType> , <http://sw.cyc.com/2006/07/27/cyc/FirstOrderCollection> ;
	<http://www.w3.org/2002/07/owl#disjointWith> <http://sw.cyc.com/2006/07/27/cyc/TemporalStuffType> , <http://sw.cyc.com/2006/07/27/cyc/QuantityType> , <http://sw.cyc.com/2006/07/27/cyc/TaxBracket> ;
	<http://sw.cyc.com/2006/07/27/cyc/typeGenls> <http://sw.cyc.com/2006/07/27/cyc/TemporalThing> ;
	<http://sw.cyc.com/2006/07/27/cyc/facets-Generic> <http://sw.cyc.com/2006/07/27/cyc/TaskTypeBySide> .

<http://sw.cyc.com/2006/07/27/cyc/AAAI> a <http://sw.cyc.com/2006/07/27/cyc/Individual> , <http://sw.cyc.com/2006/07/27/cyc/ResearchOrganization> ;
	<http://sw.cyc.com/2006/07/27/cyc/prettyString-Canonical> "AAAI" .

<http://sw.cyc.com/2006/07/27/cyc/ResearchOrganization> <http://www.w3.org/2000/01/rdf-schema#comment> "A specialization of #$Organization.  Each instance of #$ResearchOrganization is an organization that carries out basic or applied research as its main function (or one of its main functions).  A given instance of #$ResearchOrganization may or may not be a commercial, or a governmental, organization.  Examples of #$ResearchOrganizations include  #$UnitedStatesSpaceProgram, Thomas J. Watson Research Laboratory at #$IBMInc, and the Hoover Institute." ;
	a <http://www.w3.org/2002/07/owl#Class> , <http://sw.cyc.com/2006/07/27/cyc/KEClarifyingCollectionType> , <http://sw.cyc.com/2006/07/27/cyc/OrganizationTypeByActivityType> , <http://sw.cyc.com/2006/07/27/cyc/OrganizationsByFunction-Organization-Topic> ;
	<http://sw.cyc.com/2006/07/27/cyc/prettyString-Canonical> "research organization" ;
	<http://sw.cyc.com/2006/07/27/cyc/prettyString> "research centre" , "research centres" , "research centers" , "research center" , "research institute" , "research institutes" , "research organisation" , "research organisations" , "research organizations" ;
	<http://www.w3.org/2000/01/rdf-schema#subClassOf> <http://sw.cyc.com/2006/07/27/cyc/Organization> , <http://sw.cyc.com/2006/07/27/cyc/Agent-NonGeographical> ;
	<http://sw.cyc.com/2006/07/27/cyc/quotedIsa> <http://sw.cyc.com/2006/07/27/cyc/TerrorismOntologyConstant> ;
	<http://www.w3.org/2002/07/owl#disjointWith> <http://sw.cyc.com/2006/07/27/cyc/ModernMilitaryUnit-Deployable> , <http://sw.cyc.com/2006/07/27/cyc/GeopoliticalEntity> , <http://sw.cyc.com/2006/07/27/cyc/EntertainmentOrRecreationOrganization> , <http://sw.cyc.com/2006/07/27/cyc/TravelOrganization> .

<http://sw.cyc.com/2006/07/27/cyc/AAAIPress> a <http://sw.cyc.com/2006/07/27/cyc/Individual> , <http://sw.cyc.com/2006/07/27/cyc/PublishingOrganization> , <http://sw.cyc.com/2006/07/27/cyc/Organization> .

<http://sw.cyc.com/2006/07/27/cyc/Aana-DistrictWesternSamoa> a <http://sw.cyc.com/2006/07/27/cyc/State-Geopolitical> ;
	<http://sw.cyc.com/2006/07/27/cyc/prettyString-Canonical> "A`ana" .

<http://sw.cyc.com/2006/07/27/cyc/AAONInc> a <http://sw.cyc.com/2006/07/27/cyc/Individual> , <http://sw.cyc.com/2006/07/27/cyc/PubliclyHeldCorporation> ;
	<http://sw.cyc.com/2006/07/27/cyc/prettyString-Canonical> "AAON, Inc." ;
	<http://sw.cyc.com/2006/07/27/cyc/prettyString> "AAON" .

<http://sw.cyc.com/2006/07/27/cyc/AARCorp-Corporation> a <http://sw.cyc.com/2006/07/27/cyc/Individual> ;
	<http://sw.cyc.com/2006/07/27/cyc/prettyString-Canonical> "AAR Corp" .

<http://sw.cyc.com/2006/07/27/cyc/Aardvark-TheTVShow> a <http://sw.cyc.com/2006/07/27/cyc/Individual> , <http://sw.cyc.com/2006/07/27/cyc/TVSeriesProduct> ;
	<http://sw.cyc.com/2006/07/27/cyc/prettyString-Canonical> "Aardvark" .

<http://sw.cyc.com/2006/07/27/cyc/Aargau-CantonSwitzerland> a <http://sw.cyc.com/2006/07/27/cyc/Individual> , <http://sw.cyc.com/2006/07/27/cyc/State-Geopolitical> , <http://sw.cyc.com/2006/07/27/cyc/GeographicalThing> ;
	<http://sw.cyc.com/2006/07/27/cyc/prettyString-Canonical> "Aargau" .

<http://sw.cyc.com/2006/07/27/cyc/AaronCarter> a <http://sw.cyc.com/2006/07/27/cyc/Individual> , <http://sw.cyc.com/2006/07/27/cyc/MaleHuman> ;
	<http://sw.cyc.com/2006/07/27/cyc/prettyString-Canonical> "Aaron Carter" ;
	<http://sw.cyc.com/2006/07/27/cyc/prettyString> "Carter" .

<http://sw.cyc.com/2006/07/27/cyc/AaronKwok> a <http://sw.cyc.com/2006/07/27/cyc/Individual> ;
	<http://sw.cyc.com/2006/07/27/cyc/prettyString-Canonical> "Aaron Kwok" ;
	<http://sw.cyc.com/2006/07/27/cyc/prettyString> "Kwok" .

<http://sw.cyc.com/2006/07/27/cyc/AaronLohr> a <http://sw.cyc.com/2006/07/27/cyc/Individual> , <http://sw.cyc.com/2006/07/27/cyc/MaleHuman> , <http://sw.cyc.com/2006/07/27/cyc/ActorInMovies> , <http://sw.cyc.com/2006/07/27/cyc/Actor> ;
	<http://sw.cyc.com/2006/07/27/cyc/prettyString-Canonical> "Aaron Lohr" ;
	<http://sw.cyc.com/2006/07/27/cyc/prettyString> "Lohr" .

<http://sw.cyc.com/2006/07/27/cyc/ActorInMovies> <http://www.w3.org/2000/01/rdf-schema#comment> "The collection of people whose job it is to act in movies." ;
	a <http://sw.cyc.com/2006/07/27/cyc/AtemporalNecessarilyEssentialCollectionType> , <http://sw.cyc.com/2006/07/27/cyc/PersonTypeByOccupation> , <http://sw.cyc.com/2006/07/27/cyc/ActorTypeByMedium> ;
	<http://sw.cyc.com/2006/07/27/cyc/prettyString-Canonical> "movie actor" ;
	<http://sw.cyc.com/2006/07/27/cyc/prettyString> "screen actor" , "screen actors" , "movie actors" ;
	<http://www.w3.org/2000/01/rdf-schema#subClassOf> <http://sw.cyc.com/2006/07/27/cyc/Actor> , <http://sw.cyc.com/2006/07/27/cyc/SentientAnimal> .

<http://sw.cyc.com/2006/07/27/cyc/Actor> <http://www.w3.org/2000/01/rdf-schema#comment> "The collection of people whose job it is to entertain others by taking on the roles of other characters in #$DramaticPerformances.  Note that an #$Actor may be #$Male or #$Female." ;
	a <http://sw.cyc.com/2006/07/27/cyc/ExistingObjectType> , <http://sw.cyc.com/2006/07/27/cyc/AtemporalNecessarilyEssentialCollectionType> , <http://sw.cyc.com/2006/07/27/cyc/Artist-PerformerTypeByPerformanceType> , <http://sw.cyc.com/2006/07/27/cyc/EntertainerTypeByActivity> , <http://sw.cyc.com/2006/07/27/cyc/PersonTypeByFacetedActivityType> ;
	<http://sw.cyc.com/2006/07/27/cyc/prettyString-Canonical> "actor" ;
	<http://sw.cyc.com/2006/07/27/cyc/prettyString> "thespian" , "thespians" , "actress" , "actresses" .

<http://sw.cyc.com/2006/07/27/cyc/AaronVsRuth-TheGame> <http://sw.cyc.com/2006/07/27/cyc/prettyString> "Aaron vs Ruth" .

<http://sw.cyc.com/2006/07/27/cyc/AastromBiosciencesInc> a <http://sw.cyc.com/2006/07/27/cyc/Individual> , <http://sw.cyc.com/2006/07/27/cyc/PubliclyHeldCorporation> ;
	<http://sw.cyc.com/2006/07/27/cyc/prettyString-Canonical> "Aastrom Biosciences, Inc." ;
	<http://sw.cyc.com/2006/07/27/cyc/prettyString> "Aastrom Biosciences" .

<http://sw.cyc.com/2006/07/27/cyc/AavidThermalTechnologiesInc> a <http://sw.cyc.com/2006/07/27/cyc/Individual> , <http://sw.cyc.com/2006/07/27/cyc/PubliclyHeldCorporation> ;
	<http://sw.cyc.com/2006/07/27/cyc/prettyString-Canonical> "Aavid Thermal Technologies, Inc." ;
	<http://sw.cyc.com/2006/07/27/cyc/prettyString> "Aavid Thermal Technologies" .

<http://sw.cyc.com/2006/07/27/cyc/AB-205-Helicopter> <http://www.w3.org/2000/01/rdf-schema#comment> "License-built version of the U.S. Bell 205 helicopter." ;
	a <http://sw.cyc.com/2006/07/27/cyc/ExistingObjectType> , <http://sw.cyc.com/2006/07/27/cyc/SpatiallyDisjointObjectType> ;
	<http://sw.cyc.com/2006/07/27/cyc/prettyString-Canonical> "AB-205 helicopter" ;
	<http://sw.cyc.com/2006/07/27/cyc/prettyString> "AB 205" , "AB-205" ;
	<http://www.w3.org/2000/01/rdf-schema#subClassOf> <http://sw.cyc.com/2006/07/27/cyc/Helicopter> .

<http://sw.cyc.com/2006/07/27/cyc/Helicopter> <http://www.w3.org/2000/01/rdf-schema#comment> "#$Helicopter is a specialization of #$RotaryWingAircraft and #$TransportationDevice-Vehicle.  Each instance of #$Helicopter is a self-powered mechanical device that hovers in the air using a rotary wing." ;
	a <http://sw.cyc.com/2006/07/27/cyc/ExistingObjectType> , <http://sw.cyc.com/2006/07/27/cyc/SpatiallyDisjointObjectType> , <http://sw.cyc.com/2006/07/27/cyc/ManufacturedGoodsType> , <http://sw.cyc.com/2006/07/27/cyc/KEClarifyingCollectionType> , <http://sw.cyc.com/2006/07/27/cyc/Transportation-Topic> , <http://sw.cyc.com/2006/07/27/cyc/CPOF-EquipmentClassificationType> ;
	<http://sw.cyc.com/2006/07/27/cyc/prettyString-Canonical> "helicopter" ;
	<http://sw.cyc.com/2006/07/27/cyc/prettyString> "Chopper" , "choppers" , "whirlybird" , "whirlybirds" , "helicopters" ;
	<http://www.w3.org/2000/01/rdf-schema#subClassOf> <http://sw.cyc.com/2006/07/27/cyc/ManufacturedGoods> , <http://sw.cyc.com/2006/07/27/cyc/FuelPoweredDevice> , <http://sw.cyc.com/2006/07/27/cyc/RotaryWingAircraft> , <http://sw.cyc.com/2006/07/27/cyc/TransportationContainerProduct> ;
	<http://sw.cyc.com/2006/07/27/cyc/quotedIsa> <http://sw.cyc.com/2006/07/27/cyc/TerrorismOntologyConstant> ;
	<http://sw.cyc.com/2006/07/27/cyc/siblingDisjointExceptions> <http://sw.cyc.com/2006/07/27/cyc/MilitaryAircraft> .

<http://sw.cyc.com/2006/07/27/cyc/AB-206-Helicopter> <http://www.w3.org/2000/01/rdf-schema#comment> "License-built version of the U.S. Bell 206 helicopter." ;
	a <http://sw.cyc.com/2006/07/27/cyc/ExistingObjectType> , <http://sw.cyc.com/2006/07/27/cyc/SpatiallyDisjointObjectType> ;
	<http://sw.cyc.com/2006/07/27/cyc/prettyString-Canonical> "AB-206 helicopter" ;
	<http://sw.cyc.com/2006/07/27/cyc/prettyString> "AB 206" , "AB-206" ;
	<http://www.w3.org/2000/01/rdf-schema#subClassOf> <http://sw.cyc.com/2006/07/27/cyc/Helicopter> .

<http://sw.cyc.com/2006/07/27/cyc/Abacavir> a <http://sw.cyc.com/2006/07/27/cyc/GenericPharmacyProductType-NameOnly> , <http://sw.cyc.com/2006/07/27/cyc/NucleosideReverseTrancriptaseInhibitorDrugClass> , <http://sw.cyc.com/2006/07/27/cyc/PharmaceuticalType> ;
	<http://sw.cyc.com/2006/07/27/cyc/prettyString-Canonical> "abacavir" ;
	<http://www.w3.org/2000/01/rdf-schema#subClassOf> <http://sw.cyc.com/2006/07/27/cyc/ManufacturedGoods> , <http://sw.cyc.com/2006/07/27/cyc/DrugProduct> .

<http://sw.cyc.com/2006/07/27/cyc/DrugProduct> <http://www.w3.org/2000/01/rdf-schema#comment> "A specialization of both #$Artifact and #$DrugSubstance.  Each instance of #$DrugProduct is a drug substance manufactured by some agent. Instances of #$DrugProduct include drugs prescribed by a physician, drugs purchased as over-the-counter medicines, and drugs used for recreational purposes (so #$AlcoholicBeverage, #$Nicotine, and #$Caffeine are specializations)." .

<http://sw.cyc.com/2006/07/27/cyc/Aba-Garment> <http://www.w3.org/2000/01/rdf-schema#subClassOf> <http://sw.cyc.com/2006/07/27/cyc/OuterGarment> , <http://sw.cyc.com/2006/07/27/cyc/EnvelopingCovering> .

<http://sw.cyc.com/2006/07/27/cyc/OuterGarment> <http://www.w3.org/2000/01/rdf-schema#comment> """A specialization of #$Garment.  Each instance of
#$OuterGarment is a garment designed to be worn 'on the outside' in public, or at least, one that may be appropriately worn in this
fashion.  Wearing a garment 'on the outside' means wearing it
uncovered by another garment.  #$OuterGarment is disjoint with
#$Underwear (q.v).  For the collection of 'overclothes' such as
#$Coats, i.e., #$OuterGarments meant to be worn on top of other
instances of #$OuterGarment, see #$OverGarment.""" ;
	a <http://sw.cyc.com/2006/07/27/cyc/ExistingObjectType> , <http://sw.cyc.com/2006/07/27/cyc/SpatiallyDisjointObjectType> , <http://sw.cyc.com/2006/07/27/cyc/SomethingToWearTypeByGenericCategory> ;
	<http://sw.cyc.com/2006/07/27/cyc/prettyString-Canonical> "outer garment" ;
	<http://sw.cyc.com/2006/07/27/cyc/prettyString> "outerwear" , "outer garments" ;
	<http://www.w3.org/2000/01/rdf-schema#subClassOf> <http://sw.cyc.com/2006/07/27/cyc/SomethingToWear> , <http://sw.cyc.com/2006/07/27/cyc/Garment> .

<http://sw.cyc.com/2006/07/27/cyc/EnvelopingCovering> <http://www.w3.org/2000/01/rdf-schema#comment> "The collection of coverings which envelope closely the object being      covered" ;
	a <http://sw.cyc.com/2006/07/27/cyc/ExistingObjectType> , <http://sw.cyc.com/2006/07/27/cyc/SpatiallyDisjointObjectType> ;
	<http://sw.cyc.com/2006/07/27/cyc/prettyString-Canonical> "enveloping covering" ;
	<http://sw.cyc.com/2006/07/27/cyc/prettyString> "enveloping coverings" ;
	<http://www.w3.org/2000/01/rdf-schema#subClassOf> <http://sw.cyc.com/2006/07/27/cyc/Covering-Object> .

<http://sw.cyc.com/2006/07/27/cyc/SomethingToWearTypeByGenericCategory> <http://www.w3.org/2000/01/rdf-schema#comment> "An instance of #$SecondOrderCollection. Each instance of #$SomethingToWearTypeByGenericCategory is a collection of instances of #$SomethingToWear, grouped together according to some feature(s) other than brand." ;
	a <http://sw.cyc.com/2006/07/27/cyc/SecondOrderCollection> ;
	<http://sw.cyc.com/2006/07/27/cyc/prettyString-Canonical> "something to wear type by generic category" ;
	<http://www.w3.org/2000/01/rdf-schema#subClassOf> <http://sw.cyc.com/2006/07/27/cyc/ArtifactTypeByGenericCategory> ;
	<http://sw.cyc.com/2006/07/27/cyc/typeGenls> <http://sw.cyc.com/2006/07/27/cyc/SomethingToWear> .

<http://sw.cyc.com/2006/07/27/cyc/AbandonedCamp> <http://www.w3.org/2000/01/rdf-schema#comment> "A specialization of #$Campsite and #$Abandoned-ExistentialStatus whose instances are abandoned encampments." ;
	a <http://sw.cyc.com/2006/07/27/cyc/ExistingObjectType> , <http://sw.cyc.com/2006/07/27/cyc/ArtifactualFeatureType> ;
	<http://sw.cyc.com/2006/07/27/cyc/prettyString-Canonical> "abandoned camp" ;
	<http://sw.cyc.com/2006/07/27/cyc/prettyString> "abandoned camps" ;
	<http://www.w3.org/2000/01/rdf-schema#subClassOf> <http://sw.cyc.com/2006/07/27/cyc/Abandoned-ExistentialStatus> , <http://sw.cyc.com/2006/07/27/cyc/Campsite> .

<http://sw.cyc.com/2006/07/27/cyc/Abandoned-ExistentialStatus> <http://www.w3.org/2000/01/rdf-schema#comment> """This instance of #$ConstructionArtifactTypeByExistentialStatus describes
instances of #$ConstructionArtifact that are no longer maintained, i.e., no
maintenance operations are conducted to preserve their operability.""" ;
	a <http://sw.cyc.com/2006/07/27/cyc/ConstructionArtifactTypeByExistentialStatus> ;
	<http://sw.cyc.com/2006/07/27/cyc/prettyString-Canonical> "abandoned existential status" ;
	<http://www.w3.org/2000/01/rdf-schema#subClassOf> <http://sw.cyc.com/2006/07/27/cyc/ConstructionArtifact> .

<http://sw.cyc.com/2006/07/27/cyc/Campsite> <http://www.w3.org/2000/01/rdf-schema#comment> "The region where people have temporarily set up lodging in the form of tents, sleeping bags, campfires, etc..  Also includes military style encampments.  Some campsites are campsites for no longer than the duration the tent is set up there.  Other campsites remain campsites for years, e.g. #$Campground." ;
	a <http://sw.cyc.com/2006/07/27/cyc/ExistingObjectType> , <http://sw.cyc.com/2006/07/27/cyc/SpatiallyDisjointObjectType> , <http://sw.cyc.com/2006/07/27/cyc/ArtifactualFeatureType> ;
	<http://sw.cyc.com/2006/07/27/cyc/prettyString-Canonical> "campsite" ;
	<http://sw.cyc.com/2006/07/27/cyc/prettyString> "Camp" , "camps" , "campsites" ;
	<http://www.w3.org/2000/01/rdf-schema#subClassOf> <http://sw.cyc.com/2006/07/27/cyc/NonNaturalThing> , <http://sw.cyc.com/2006/07/27/cyc/OutdoorLocation> , <http://sw.cyc.com/2006/07/27/cyc/HumanlyOccupiedSpatialObject> ;
	<http://www.w3.org/2002/07/owl#disjointWith> <http://sw.cyc.com/2006/07/27/cyc/Dock> .

<http://sw.cyc.com/2006/07/27/cyc/ArtifactualFeatureType> <http://www.w3.org/2000/01/rdf-schema#comment> """#$ArtifactualFeatureType is the collection of
#$CartographicFeatureTypes which are #$Artifacts, as opposed to
naturally occuring. Positive examples include #$WaterReservoir, #$Canal,
and #$Airfield. Negative examples include #$Mountain, #$Ocean, and
#$Mesa. Also see #$NaturalFeatureType, the corresponding collection
for naturally occuring feature types.""" ;
	a <http://sw.cyc.com/2006/07/27/cyc/AtemporalNecessarilyEssentialCollectionType> , <http://sw.cyc.com/2006/07/27/cyc/FacetingCollectionType> , <http://sw.cyc.com/2006/07/27/cyc/SecondOrderCollection> , <http://sw.cyc.com/2006/07/27/cyc/TerrainFeatureTaxonType> ;
	<http://sw.cyc.com/2006/07/27/cyc/prettyString-Canonical> "artifactual feature type" ;
	<http://www.w3.org/2000/01/rdf-schema#subClassOf> <http://sw.cyc.com/2006/07/27/cyc/ExistingObjectType> , <http://sw.cyc.com/2006/07/27/cyc/ArtifactTypeByGenericCategory> , <http://sw.cyc.com/2006/07/27/cyc/FirstOrderCollection> , <http://sw.cyc.com/2006/07/27/cyc/CartographicFeatureType> ;
	<http://sw.cyc.com/2006/07/27/cyc/typeGenls> <http://sw.cyc.com/2006/07/27/cyc/NonNaturalThing> .

<http://sw.cyc.com/2006/07/27/cyc/ConstructionArtifact> <http://www.w3.org/2000/01/rdf-schema#comment> "A specialization of #$Artifact.  Each instance of #$ConstructionArtifact is a structure designed and built by agents (human or otherwise).  This collection includes buildings and parts of buildings, as well as things like dams, railroad lines, and roads.  Examples include the #$RomanColiseum, the #$ArcDeTriomphe, #$HooverDam, the #$EmpireStateBuilding, and the #$HollywoodBowl.  Note that the collection #$ConstructionArtifact includes some instances (such as instances of the specialization #$MannedSpacecraft) that are not tied to a fixed location, as well as some instances (such as instances of the specialization #$BridgeSpan) that, although tied to a fixed location, are not free-standing artifacts.  #$FixedStructure, an important specialization of #$ConstructionArtifact, is the collection of free-standing construction artifacts that are tied to a fixed location." ;
	a <http://sw.cyc.com/2006/07/27/cyc/FirstOrderCollection> , <http://sw.cyc.com/2006/07/27/cyc/TemporalStuffType> , <http://sw.cyc.com/2006/07/27/cyc/Construction-Topic> , <http://sw.cyc.com/2006/07/27/cyc/TestOWLExportConcept> ;
	<http://sw.cyc.com/2006/07/27/cyc/prettyString-Canonical> "man-made structure" ;
	<http://sw.cyc.com/2006/07/27/cyc/prettyString> "construction" , "structure" , "structures" , "constructions" , "man-made structures" ;
	<http://www.w3.org/2000/01/rdf-schema#subClassOf> <http://sw.cyc.com/2006/07/27/cyc/Artifact> , <http://sw.cyc.com/2006/07/27/cyc/Place> , <http://sw.cyc.com/2006/07/27/cyc/Artifact-NonAgentive> , <http://sw.cyc.com/2006/07/27/cyc/Artifact-HumanCreated> , <http://sw.cyc.com/2006/07/27/cyc/DurableGood> , <http://sw.cyc.com/2006/07/27/cyc/HumanScaleObject> ;
	<http://sw.cyc.com/2006/07/27/cyc/quotedIsa> <http://sw.cyc.com/2006/07/27/cyc/TerrorismOntologyConstant> .

<http://sw.cyc.com/2006/07/27/cyc/ComputerProgram-CW> <http://www.w3.org/2000/01/rdf-schema#comment> """A specialization of #$PropositionalConceptualWork, #$ComputerFile-CW and #$SoftwareObject-Individual. Each instance of #$ComputerProgram-CW is a deliberately created abstract object composed of propositions that together constitute a list of instructions for computers to execute.  
<p>
Example instances include #$Emacs-TheProgram and #$LinuxKernel-TheProgram.
<p>
Instances of this collection are distinct from computer code and from both running and installed programs. The instructions that comprise an instance of #$ComputerProgram-CW can be expressed as abstract computer code (see #$ComputerCode), but no list of instructions expressed in code constitutes an instance of #$ComputerProgram-CW.  Rather, the code in which an instance of #$ComputerProgram-CW is expressed constitutes an instance of #$AbstractInformationStructure that can be related to the program it expresses using the predicate #$programCode.  More than one instance of #$ComputerCode can express the same instance of #$ComputerProgram-CW; for example,  a single instance of #$ComputerProgram-CW can be written in source code (see #$ComputerCode-Source) in several different computer languages, or it can be complied as a binary executable (see #$ComputerCode-Binary).  A physical instantiation of a #$ComputerProgram-CW is a #$ComputerProgramCopy which is an #$InformationBearingThing and is related to its #$ComputerProgram-CW by the predicate #$programCopies.  An instance of #$ComputerProgram-CW that is being executed is a #$ComputerProcessRunning, related to its #$ComputerProgram-CW by the predicate #$programOfProcess.""" ;
	a <http://sw.cyc.com/2006/07/27/cyc/ObjectType> , <http://sw.cyc.com/2006/07/27/cyc/TemporalStuffType> , <http://sw.cyc.com/2006/07/27/cyc/QAClarifyingCollectionType> , <http://sw.cyc.com/2006/07/27/cyc/InformationAndCWs-Topic> ;
	<http://sw.cyc.com/2006/07/27/cyc/prettyString-Canonical> "computer program" ;
	<http://sw.cyc.com/2006/07/27/cyc/prettyString> "code" , "software title" , "software titles" , "computer software" , "software programme" , "software program" , "software programs" , "software programz" , "prog" , "progz" , "proggies" , "progs" , "computer programme" , "computer programs" , "computer programz" , "programme" , "program" , "programs" , "software" , "programz" ;
	<http://www.w3.org/2000/01/rdf-schema#subClassOf> <http://sw.cyc.com/2006/07/27/cyc/ComputerFile-CW> , <http://sw.cyc.com/2006/07/27/cyc/SoftwareObject-Individual> ;
	<http://sw.cyc.com/2006/07/27/cyc/sharedNotes> <http://sw.cyc.com/2006/07/27/cyc/SharedNoteOnPrimaryFunctionOfComputerProgram-CWs> ;
	<http://sw.cyc.com/2006/07/27/cyc/facets-Generic> <http://sw.cyc.com/2006/07/27/cyc/ComputerProgramTypeByCreator> , <http://sw.cyc.com/2006/07/27/cyc/ComputerProgramTypeByDistribution> , <http://sw.cyc.com/2006/07/27/cyc/SoftwareTypeByInterfaceFeature> , <http://sw.cyc.com/2006/07/27/cyc/ComputerProgramTypeByPlatform> .

<http://sw.cyc.com/2006/07/27/cyc/ExistenceDependentTerminalCollection> <http://www.w3.org/2000/01/rdf-schema#comment> "A specialization of both #$ExistenceDependentCollection and #$NonInitialCollection  (qq.v.).  Each instance EDTC of #$ExistenceDependentTerminalCollection is a collection such that: (i) a thing can be an instance of EDTC only while the thing exists, (ii) once a thing becomes an instance of EDTC it necessarily remains so until the end of the thing's existence, (iii) nothing can be an instance of EDTC for its entire existence.  It follows from these conditions that (iv) nothing starts out as an instance of EDTC and (v) any instance of EDTC ceases to be such when it ceases to exist.  An example of an #$ExistenceDependentTerminalCollection is (#$GraduateFn #$College), the collection of college graduates.  Cf. #$ExistenceDependentInitialCollection." ;
	a <http://sw.cyc.com/2006/07/27/cyc/FacetingCollectionType> , <http://sw.cyc.com/2006/07/27/cyc/SecondOrderCollection> , <http://sw.cyc.com/2006/07/27/cyc/TimeIndependentCollection> ;
	<http://sw.cyc.com/2006/07/27/cyc/prettyString-Canonical> "existence dependent terminal collection" ;
	<http://www.w3.org/2000/01/rdf-schema#subClassOf> <http://sw.cyc.com/2006/07/27/cyc/NonInitialCollection> , <http://sw.cyc.com/2006/07/27/cyc/ExistenceDependentCollection> ;
	<http://www.w3.org/2002/07/owl#disjointWith> <http://sw.cyc.com/2006/07/27/cyc/IntermittentCollection> .

<http://sw.cyc.com/2006/07/27/cyc/Abasha-DistrictGeorgia> a <http://sw.cyc.com/2006/07/27/cyc/Individual> , <http://sw.cyc.com/2006/07/27/cyc/State-Geopolitical> ;
	<http://sw.cyc.com/2006/07/27/cyc/prettyString-Canonical> "Abasha" ;
	<http://sw.cyc.com/2006/07/27/cyc/prettyString> "Bashis Raioni" .

<http://sw.cyc.com/2006/07/27/cyc/Abatis> a <http://sw.cyc.com/2006/07/27/cyc/ArtifactualFeatureType> , <http://sw.cyc.com/2006/07/27/cyc/FirstOrderCollection> ;
	<http://sw.cyc.com/2006/07/27/cyc/prettyString-Canonical> "abati" ;
	<http://sw.cyc.com/2006/07/27/cyc/prettyString> "abatis" .

<http://sw.cyc.com/2006/07/27/cyc/LargeIncorporatedBusiness> <http://www.w3.org/2000/01/rdf-schema#comment> "A specialization of both #$LegalCorporation and #$Business.  Each instance of #$LargeIncorporatedBusiness is a relatively large (e.g., having at least several hundred employees) business corporation.  Specializations of #$LargeIncorporatedBusiness include #$ChainOrganization and #$MultinationalCorporation." ;
	a <http://sw.cyc.com/2006/07/27/cyc/ExistingObjectType> ;
	<http://sw.cyc.com/2006/07/27/cyc/prettyString-Canonical> "incorporated business" ;
	<http://sw.cyc.com/2006/07/27/cyc/prettyString> "incorporated businesses" ;
	<http://www.w3.org/2000/01/rdf-schema#subClassOf> <http://sw.cyc.com/2006/07/27/cyc/Business> , <http://sw.cyc.com/2006/07/27/cyc/LegalCorporation> ;
	<http://www.w3.org/2002/07/owl#disjointWith> <http://sw.cyc.com/2006/07/27/cyc/ServiceEstablishment> .

<http://sw.cyc.com/2006/07/27/cyc/ManufacturingOrganization> <http://www.w3.org/2000/01/rdf-schema#comment> "A specialization of #$Organization.  Each instance of #$ManufacturingOrganization is an organization whose main function (see #$MainFunction) is the manufacture or production of goods.  Instances of #$ManufacturingOrganization may be departments, suborganizations, companies, or conglomerate enterprises." ;
	a <http://sw.cyc.com/2006/07/27/cyc/OrganizationTypeByActivityType> , <http://sw.cyc.com/2006/07/27/cyc/OrganizationsByFunction-Organization-Topic> , <http://sw.cyc.com/2006/07/27/cyc/IndustrialConcept> ;
	<http://sw.cyc.com/2006/07/27/cyc/prettyString-Canonical> "producer" ;
	<http://sw.cyc.com/2006/07/27/cyc/prettyString> "producers" , "manufacturer" , "manufacturers" ;
	<http://www.w3.org/2000/01/rdf-schema#subClassOf> <http://sw.cyc.com/2006/07/27/cyc/CommercialOrganization> ;
	<http://sw.cyc.com/2006/07/27/cyc/quotedIsa> <http://sw.cyc.com/2006/07/27/cyc/WordNetWorkflowConstant-NotFullyReviewed> , <http://sw.cyc.com/2006/07/27/cyc/TerrorismOntologyConstant> ;
	<http://www.w3.org/2002/07/owl#disjointWith> <http://sw.cyc.com/2006/07/27/cyc/FinancialOrganization> , <http://sw.cyc.com/2006/07/27/cyc/TransportationOrganization> , <http://sw.cyc.com/2006/07/27/cyc/TravelOrganization> , <http://sw.cyc.com/2006/07/27/cyc/InsuranceOrganization> , <http://sw.cyc.com/2006/07/27/cyc/HealthcareOrganization> , <http://sw.cyc.com/2006/07/27/cyc/PoliticalParty> , <http://sw.cyc.com/2006/07/27/cyc/ProfessionalOffice> ;
	<http://sw.cyc.com/2006/07/27/cyc/facets-Generic> <http://sw.cyc.com/2006/07/27/cyc/ManufacturerTypeByFocalProductType> .

<http://sw.cyc.com/2006/07/27/cyc/PharmaceuticalCompany> <http://www.w3.org/2000/01/rdf-schema#comment> "Instances are companies which develop and produce drugs and other pharmaceutical products, such as medical devices. " ;
	a <http://sw.cyc.com/2006/07/27/cyc/BusinessTypeByActivityType> ;
	<http://sw.cyc.com/2006/07/27/cyc/prettyString-Canonical> "pharmaceutical company" ;
	<http://sw.cyc.com/2006/07/27/cyc/prettyString> "pharmaceutical companies" ;
	<http://www.w3.org/2000/01/rdf-schema#subClassOf> <http://sw.cyc.com/2006/07/27/cyc/ResearchOrganization> , <http://sw.cyc.com/2006/07/27/cyc/ManufacturingCompany> .

<http://sw.cyc.com/2006/07/27/cyc/HighTechManufacturingEnterprise> <http://www.w3.org/2000/01/rdf-schema#comment> "The colleciton of organizations (businesses) that manufacture high tech items." ;
	a <http://sw.cyc.com/2006/07/27/cyc/ExistingObjectType> , <http://sw.cyc.com/2006/07/27/cyc/QAClarifyingCollectionType> ;
	<http://sw.cyc.com/2006/07/27/cyc/prettyString-Canonical> "high tech manufacturer" ;
	<http://sw.cyc.com/2006/07/27/cyc/prettyString> "high tech manufacturing enterprise" , "high tech manufacturing enterprises" , "high tech company" , "high tech companies" , "high tech manufacturers" ;
	<http://www.w3.org/2000/01/rdf-schema#subClassOf> <http://sw.cyc.com/2006/07/27/cyc/ManufacturingCompany> , <http://sw.cyc.com/2006/07/27/cyc/TechnologyCompany> .

<http://sw.cyc.com/2006/07/27/cyc/Abbreviation> <http://www.w3.org/2000/01/rdf-schema#comment> "A shortened version of a written word or phrase. An #$Acronym is a specific type of abbreviation." ;
	a <http://sw.cyc.com/2006/07/27/cyc/ObjectType> ;
	<http://sw.cyc.com/2006/07/27/cyc/prettyString-Canonical> "abbreviation" ;
	<http://sw.cyc.com/2006/07/27/cyc/prettyString> "abbreviations" ;
	<http://www.w3.org/2000/01/rdf-schema#subClassOf> <http://sw.cyc.com/2006/07/27/cyc/ProperNameString> .

<http://sw.cyc.com/2006/07/27/cyc/abbreviationForCompoundString> <http://www.w3.org/2000/01/rdf-schema#comment> "(#$abbreviationForCompoundString LEXICALWORD STRING POS ABBREVIATION) means that ABBREVIATION is an abbreviation for the compound phrase picked out by POS part of speech of LEXICALWORD + STRING.  Example --  (#$abbreviationForCompoundString #$Mile-TheWord (#$TheList (\"per\" \"hour\")) #$CountNoun \"m/h\")." ;
	a <http://sw.cyc.com/2006/07/27/cyc/MultiWordForStringPred> , <http://sw.cyc.com/2006/07/27/cyc/QuaternaryPredicate> ;
	<http://sw.cyc.com/2006/07/27/cyc/prettyString-Canonical> "Abbreviation For Compound String" ;
	<http://sw.cyc.com/2006/07/27/cyc/quotedIsa> <http://sw.cyc.com/2006/07/27/cyc/CycLexiconPredicator> , <http://sw.cyc.com/2006/07/27/cyc/NLTerm> ;
	<http://www.w3.org/2000/01/rdf-schema#domain> <http://sw.cyc.com/2006/07/27/cyc/LexicalWord> .

<http://sw.cyc.com/2006/07/27/cyc/abbreviationForString> a <http://www.w3.org/2000/01/rdf-schema#Property> ;
	<http://sw.cyc.com/2006/07/27/cyc/prettyString-Canonical> "Abbreviation For String" ;
	<http://sw.cyc.com/2006/07/27/cyc/quotedIsa> <http://sw.cyc.com/2006/07/27/cyc/NLTerm> ;
	<http://www.w3.org/2000/01/rdf-schema#domain> <http://sw.cyc.com/2006/07/27/cyc/CharacterString> ;
	<http://sw.cyc.com/2006/07/27/cyc/arity> "2"^^<http://www.w3.org/2001/XMLSchema#long> ;
	<http://sw.cyc.com/2006/07/27/cyc/sharedNotes> <http://sw.cyc.com/2006/07/27/cyc/SharedNoteOnMultiWordPredicates> ;
	<http://www.w3.org/2000/01/rdf-schema#range> <http://sw.cyc.com/2006/07/27/cyc/CharacterString> .

<http://sw.cyc.com/2006/07/27/cyc/ProperNameString> <http://www.w3.org/2000/01/rdf-schema#comment> "A specialization of #$IDString. Each instance of this collection is a proper name considered as a character string. Instances of #$ProperNameString include city names (e.g. \"Dallas\"), person names (e.g. \"Douglas\" -- see #$HumanNameString), brand names (e.g. \"Jello\" -- see #$BrandName), company names (e.g. \"Apple\"), book titles, etc. Note that it is also possible to consider proper names not as character strings but as instances of #$LexicalWord -- for that, see #$Name and its specializations (and see #$nameSpelling to relate the two)." ;
	a <http://sw.cyc.com/2006/07/27/cyc/TermPhrasesConstraint> , <http://sw.cyc.com/2006/07/27/cyc/IDStringType> , <http://sw.cyc.com/2006/07/27/cyc/TitlesAndNames-Social-Topic> ;
	<http://sw.cyc.com/2006/07/27/cyc/prettyString-Canonical> "proper name string" ;
	<http://sw.cyc.com/2006/07/27/cyc/prettyString> "proper name strings" ;
	<http://www.w3.org/2000/01/rdf-schema#subClassOf> <http://sw.cyc.com/2006/07/27/cyc/IDString> ;
	<http://www.w3.org/2002/07/owl#disjointWith> <http://sw.cyc.com/2006/07/27/cyc/InternationalPostalCode> .

<http://sw.cyc.com/2006/07/27/cyc/abbreviationString-PN> <http://www.w3.org/2000/01/rdf-schema#comment> "(#$abbreviationString-PN THING STRING) means that STRING is a shortened form of the name for THING.  For example, \"Nov\" is short for \"November\".  Therefore one asserts (#$abbreviationString-PN #$November \"Nov\").  STRING will be treated as a proper noun (see #$ProperNoun)." ;
	a <http://sw.cyc.com/2006/07/27/cyc/ProperNamePredicate-Strict> , <http://sw.cyc.com/2006/07/27/cyc/StringIndexingSlot> , <http://sw.cyc.com/2006/07/27/cyc/ProperNamePredicateForNPParser> ;
	<http://sw.cyc.com/2006/07/27/cyc/prettyString-Canonical> "abbreviation" ;
	<http://sw.cyc.com/2006/07/27/cyc/quotedIsa> <http://sw.cyc.com/2006/07/27/cyc/CycLexiconPredicator> , <http://sw.cyc.com/2006/07/27/cyc/NLTerm> ;
	<http://www.w3.org/2000/01/rdf-schema#domain> <http://www.w3.org/2002/07/owl#Thing> ;
	<http://sw.cyc.com/2006/07/27/cyc/arity> "2"^^<http://www.w3.org/2001/XMLSchema#long> ;
	<http://sw.cyc.com/2006/07/27/cyc/sharedNotes> <http://sw.cyc.com/2006/07/27/cyc/SharedNoteOnProperNamePredicates> ;
	<http://www.w3.org/2000/01/rdf-schema#range> <http://sw.cyc.com/2006/07/27/cyc/Abbreviation> ;
	<http://www.w3.org/2000/01/rdf-schema#subPropertyOf> <http://sw.cyc.com/2006/07/27/cyc/properNameStrings> .

<http://sw.cyc.com/2006/07/27/cyc/properNameStrings> <http://www.w3.org/2000/01/rdf-schema#comment> "An #$NLPredicate that relates a #$Thing to a #$ProperNameString.  (#$properNameStrings THING STRING) means that STRING is a proper name for THING." ;
	a <http://sw.cyc.com/2006/07/27/cyc/StringIndexingSlot> ;
	<http://sw.cyc.com/2006/07/27/cyc/prettyString-Canonical> "proper name strings" ;
	<http://sw.cyc.com/2006/07/27/cyc/quotedIsa> <http://sw.cyc.com/2006/07/27/cyc/CycLexiconPredicator> , <http://sw.cyc.com/2006/07/27/cyc/NLTerm> ;
	<http://www.w3.org/2000/01/rdf-schema#domain> <http://www.w3.org/2002/07/owl#Thing> ;
	<http://sw.cyc.com/2006/07/27/cyc/arity> "2"^^<http://www.w3.org/2001/XMLSchema#long> ;
	<http://www.w3.org/2000/01/rdf-schema#range> <http://sw.cyc.com/2006/07/27/cyc/ProperNameString> ;
	<http://www.w3.org/2000/01/rdf-schema#subPropertyOf> <http://sw.cyc.com/2006/07/27/cyc/termStrings> .

<http://sw.cyc.com/2006/07/27/cyc/ProperNamePredicate-Strict> <http://www.w3.org/2000/01/rdf-schema#comment> "Elements of #$ProperNamePredicate-Strict are all the lexical predicates that can be used to register the information that a certain STRING is (one of the) name(s) of a certain FORT. This only includes predicates that are used for permanent and thorough lexification. Assertions using predicates that are members of this collection contain all the grammatical information that is necessary to deal with issues such as pluralization. Compare to #$ProperNamePredicate-Loose." ;
	a <http://sw.cyc.com/2006/07/27/cyc/KBDependentCollection> , <http://sw.cyc.com/2006/07/27/cyc/LinguisticObjectType> , <http://sw.cyc.com/2006/07/27/cyc/PredicateType> ;
	<http://sw.cyc.com/2006/07/27/cyc/prettyString-Canonical> "strict proper name predicate" ;
	<http://sw.cyc.com/2006/07/27/cyc/prettyString> "strict proper name predicates" ;
	<http://www.w3.org/2000/01/rdf-schema#subClassOf> <http://sw.cyc.com/2006/07/27/cyc/ProperNamePredicate-General> .

<http://sw.cyc.com/2006/07/27/cyc/StringIndexingSlot> a <http://sw.cyc.com/2006/07/27/cyc/KEClarifyingCollectionType> , <http://sw.cyc.com/2006/07/27/cyc/LinguisticObjectType> , <http://sw.cyc.com/2006/07/27/cyc/PredicateType> ;
	<http://sw.cyc.com/2006/07/27/cyc/prettyString-Canonical> "string indexing slot" ;
	<http://www.w3.org/2000/01/rdf-schema#subClassOf> <http://sw.cyc.com/2006/07/27/cyc/TermPhrasesConstraint> , <http://www.w3.org/2000/01/rdf-schema#Property> , <http://sw.cyc.com/2006/07/27/cyc/NLSemanticPredicate> .

<http://sw.cyc.com/2006/07/27/cyc/ProperNamePredicateForNPParser> <http://www.w3.org/2000/01/rdf-schema#comment> """The collection of all name predicates that are consulted in order
to build the lexical trie on which the Noun Phrase parser is presently 
(September 6, 2000) based""" ;
	a <http://sw.cyc.com/2006/07/27/cyc/KBDependentCollection> , <http://sw.cyc.com/2006/07/27/cyc/LinguisticObjectType> , <http://sw.cyc.com/2006/07/27/cyc/PredicateType> .

<http://sw.cyc.com/2006/07/27/cyc/PersonalizableWebPortal> <http://www.w3.org/2000/01/rdf-schema#comment> "A collection of #$WebPortals that permit the user to personalize or customize the #$WebPortal for his own interests or needs.  The #$PersonalizableWebPortal often has a different homepage from the main homepage of a #$SearchEngine.  For example, #$Yahoo-SearchEngine has different homepage from 'My Yahoo', which is an instance of #$PersonalizableWebPortal.  Yet, the instances of #$PersonalizableWebPortal are not collections of individualized #$WebPortals.  For example, #$Yahoo-PersonalizableWebPortal is not a collection containing Roland's MyYahoo or Michael's MyYahoo.  Instead, to create Roland's MyYahoo one would assert that Roland's MyYahoo is a #$WebPortal and is #$derivedConceptualWork from #$PersonalizableWebPortal." ;
	a <http://sw.cyc.com/2006/07/27/cyc/ComputerProgramTypeByFunction> ;
	<http://sw.cyc.com/2006/07/27/cyc/prettyString-Canonical> "customized portal" ;
	<http://sw.cyc.com/2006/07/27/cyc/prettyString> "web portal" , "web portals" , "personalized portal" , "personalized portals" , "customized portals" ;
	<http://www.w3.org/2000/01/rdf-schema#subClassOf> <http://sw.cyc.com/2006/07/27/cyc/WebPortal> .

<http://sw.cyc.com/2006/07/27/cyc/AbdaliyaOilField> <http://www.w3.org/2000/01/rdf-schema#comment> "An #$OilField located in #$Kuwait" ;
	a <http://sw.cyc.com/2006/07/27/cyc/Individual> , <http://sw.cyc.com/2006/07/27/cyc/OilField> ;
	<http://sw.cyc.com/2006/07/27/cyc/prettyString-Canonical> "the Abdaliya Oilfield" .

<http://sw.cyc.com/2006/07/27/cyc/OilField> <http://www.w3.org/2000/01/rdf-schema#comment> "A specialization of #$MineralField.  Each instance of #$OilField is a region -- developed or not -- that is naturally rich in petrolium.  For commercially developed oil fields, see the specialization #$OilField-Developed." ;
	a <http://sw.cyc.com/2006/07/27/cyc/ExistingObjectType> , <http://sw.cyc.com/2006/07/27/cyc/SpatiallyDisjointObjectType> , <http://sw.cyc.com/2006/07/27/cyc/ArtifactualFeatureType> , <http://sw.cyc.com/2006/07/27/cyc/AtemporalNecessarilyEssentialCollectionType> ;
	<http://sw.cyc.com/2006/07/27/cyc/prettyString-Canonical> "oil field" ;
	<http://sw.cyc.com/2006/07/27/cyc/prettyString> "oilfield" , "oilfields" , "oil fields" ;
	<http://www.w3.org/2000/01/rdf-schema#subClassOf> <http://sw.cyc.com/2006/07/27/cyc/MineralField> .

<http://sw.cyc.com/2006/07/27/cyc/AbdallahAzzam> <http://www.w3.org/2000/01/rdf-schema#comment> """The emir of Mekta al Khidemat, which helps train people
for fighting in Afghanistan.""" ;
	a <http://sw.cyc.com/2006/07/27/cyc/Individual> , <http://sw.cyc.com/2006/07/27/cyc/AdultMaleHuman> ;
	<http://sw.cyc.com/2006/07/27/cyc/prettyString-Canonical> "Abdallah Azzam" ;
	<http://sw.cyc.com/2006/07/27/cyc/prettyString> "Azzam" .

<http://sw.cyc.com/2006/07/27/cyc/AdultMaleHuman> <http://www.w3.org/2000/01/rdf-schema#comment> "A specialization of #$HumanAdult and #$MaleHuman.  Each instance of #$AdultMaleHuman is a man, i.e., an instance of #$HomoSapiens who is adult and male." ;
	a <http://sw.cyc.com/2006/07/27/cyc/ExistingObjectType> , <http://sw.cyc.com/2006/07/27/cyc/AtemporalNecessarilyEssentialCollectionType> , <http://sw.cyc.com/2006/07/27/cyc/KEClarifyingCollectionType> ;
	<http://sw.cyc.com/2006/07/27/cyc/prettyString-Canonical> "MAN" ;
	<http://sw.cyc.com/2006/07/27/cyc/prettyString> "fellow" , "fellows" , "male adult" , "male adults" , "adult male" , "adult males" , "men" ;
	<http://www.w3.org/2000/01/rdf-schema#subClassOf> <http://sw.cyc.com/2006/07/27/cyc/MaleHuman> , <http://sw.cyc.com/2006/07/27/cyc/HumanAdult> ;
	<http://sw.cyc.com/2006/07/27/cyc/facets-Covering> <http://sw.cyc.com/2006/07/27/cyc/ManTypeByShoeSize> ;
	<http://sw.cyc.com/2006/07/27/cyc/facets-Generic> <http://sw.cyc.com/2006/07/27/cyc/ManTypeByShoeSize> ;
	<http://sw.cyc.com/2006/07/27/cyc/requiredArg1Pred> <http://sw.cyc.com/2006/07/27/cyc/wearsSize> .

<http://sw.cyc.com/2006/07/27/cyc/AbdAlRahmanShalgam> a <http://sw.cyc.com/2006/07/27/cyc/AdultMaleHuman> ;
	<http://sw.cyc.com/2006/07/27/cyc/prettyString-Canonical> "Abd al-Rahman Shalgam" .

<http://sw.cyc.com/2006/07/27/cyc/AbdelazizRhouzlane-911FOAF> a <http://sw.cyc.com/2006/07/27/cyc/Individual> , <http://sw.cyc.com/2006/07/27/cyc/Person> .

<http://sw.cyc.com/2006/07/27/cyc/AbdelMunimAlKhabir> <http://sw.cyc.com/2006/07/27/cyc/prettyString> "Dr. Abdel Munim al-Khabir" , "al-Khabir" .

<http://sw.cyc.com/2006/07/27/cyc/AbdelRahmanShrewi> a <http://sw.cyc.com/2006/07/27/cyc/Individual> , <http://sw.cyc.com/2006/07/27/cyc/Person> ;
	<http://sw.cyc.com/2006/07/27/cyc/prettyString-Canonical> "Abdel Rahman Shrewi" ;
	<http://sw.cyc.com/2006/07/27/cyc/prettyString> "Shrewi" , "Abdel Shrewi" .

<http://sw.cyc.com/2006/07/27/cyc/Abdicating> <http://www.w3.org/2000/01/rdf-schema#comment> "A collection of events; a subcollection of #$Resigning. In each #$Abdicating, someone gives up, such as power, as of monarchs and emperors, or duties and obligations." ;
	a <http://sw.cyc.com/2006/07/27/cyc/FirstOrderCollection> ;
	<http://sw.cyc.com/2006/07/27/cyc/prettyString-Canonical> "Abdicating" ;
	<http://sw.cyc.com/2006/07/27/cyc/prettyString> "renounce" , "renounced" , "renounces" , "renouncing" , "have renounced" , "has renounced" , "will renounce" , "had renounced" , "will have renounced" , "Abdicate" , "Abdicated" , "Abdicates" , "have Abdicated" , "has Abdicated" , "will Abdicate" , "had Abdicated" , "will have Abdicated" ;
	<http://www.w3.org/2000/01/rdf-schema#subClassOf> <http://sw.cyc.com/2006/07/27/cyc/Resigning> ;
	<http://sw.cyc.com/2006/07/27/cyc/quotedIsa> <http://sw.cyc.com/2006/07/27/cyc/WordNetWorkflowConstant-NotFullyReviewed> .

<http://sw.cyc.com/2006/07/27/cyc/Resigning> <http://www.w3.org/2000/01/rdf-schema#comment> "Voluntarily leaving your job." ;
	a <http://sw.cyc.com/2006/07/27/cyc/TemporalObjectType> , <http://sw.cyc.com/2006/07/27/cyc/TypicalHumanActivityType-AtLeastOnce> ;
	<http://sw.cyc.com/2006/07/27/cyc/prettyString-Canonical> "resignation" ;
	<http://sw.cyc.com/2006/07/27/cyc/prettyString> "quit" , "quits" , "quitting" , "have quit" , "has quit" , "will quit" , "had quit" , "will have quit" , "resign" , "resigned" , "resigns" , "resigning" , "have resigned" , "has resigned" , "will resign" , "had resigned" , "will have resigned" , "resignations" ;
	<http://www.w3.org/2000/01/rdf-schema#subClassOf> <http://sw.cyc.com/2006/07/27/cyc/EmploymentTermination> ;
	<http://www.w3.org/2002/07/owl#disjointWith> <http://sw.cyc.com/2006/07/27/cyc/ExpellingFromMembership> .

<http://sw.cyc.com/2006/07/27/cyc/WordNetWorkflowConstant-NotFullyReviewed> <http://www.w3.org/2000/01/rdf-schema#comment> "The collection of all #$CycLConstants created from the import of concepts from #$WordNet-Version2_0 that have not yet been fully reviewed by a #$HumanCyclist." ;
	a <http://sw.cyc.com/2006/07/27/cyc/NonAbducibleCollection> , <http://sw.cyc.com/2006/07/27/cyc/KBDependentCollection> , <http://sw.cyc.com/2006/07/27/cyc/CycLExpressionType> ;
	<http://sw.cyc.com/2006/07/27/cyc/prettyString-Canonical> "word net workflow constant not fully reviewed" ;
	<http://www.w3.org/2000/01/rdf-schema#subClassOf> <http://sw.cyc.com/2006/07/27/cyc/WordNetWorkflowConstant> .

<http://sw.cyc.com/2006/07/27/cyc/Abdomen> <http://www.w3.org/2000/01/rdf-schema#comment> "Part of body between the chest and the pelvis" ;
	a <http://sw.cyc.com/2006/07/27/cyc/SpatiallyDisjointObjectType> , <http://sw.cyc.com/2006/07/27/cyc/AnimalBodyPartType> , <http://sw.cyc.com/2006/07/27/cyc/ExternalAnimalBodyRegionType> , <http://sw.cyc.com/2006/07/27/cyc/UniqueAnatomicalPartType> ;
	<http://sw.cyc.com/2006/07/27/cyc/prettyString-Canonical> "abdomen" ;
	<http://sw.cyc.com/2006/07/27/cyc/prettyString> "tummy" , "tummies" , "Belly" , "stomach" , "bellies" , "stomachs" , "abdomens" ;
	<http://www.w3.org/2000/01/rdf-schema#subClassOf> <http://sw.cyc.com/2006/07/27/cyc/SolidTangibleThing> , <http://sw.cyc.com/2006/07/27/cyc/AnimalBodyPart> , <http://sw.cyc.com/2006/07/27/cyc/ExternalAnatomicalPart> .

<http://sw.cyc.com/2006/07/27/cyc/SolidTangibleThing> <http://www.w3.org/2000/01/rdf-schema#comment> "An instance of #$ExistingStuffType, and a specialization of #$PartiallyTangible.  Each instance of #$SolidTangibleThing is a piece of stuff possessing many of the properties that matter in a solid state (see the constant #$Solid-StateOfMatter) exhibits (although not all instances of #$SolidTangibleThing are formally in a solid state).  Instances have a shape independent from their container, and, when deformed with sufficient force (which may be small for weak, brittle materials or high for materials that deform easily), they break.  Examples of #$SolidTangibleThings include: pieces of substances in a solid state of matter, such as ice cubes; solid mixtures like a quarter-dollar coin or a paper bag; and complex mixtures of biological origin that behave like solids, e.g., bone.  Note that some pieces of matter that are formally in a solid state (for example, pieces of clay) are not instances of #$SolidTangibleThing, since they do not readily break when deformed; for this reason, #$Solid-StateOfMatter is <i>not</i> a specialization of #$SolidTangibleThing.  Collections of the solid form of any type of stuff can be created using #$SolidFn (q.v.)." ;
	a <http://sw.cyc.com/2006/07/27/cyc/QAClarifyingCollectionType> , <http://sw.cyc.com/2006/07/27/cyc/TestOWLExportConcept> , <http://sw.cyc.com/2006/07/27/cyc/StatesOfMatter-Material-Topic> , <http://sw.cyc.com/2006/07/27/cyc/TangibleStuffStateType> , <http://sw.cyc.com/2006/07/27/cyc/DosageFormType> , <http://sw.cyc.com/2006/07/27/cyc/DosagePhysicalStateType> ;
	<http://sw.cyc.com/2006/07/27/cyc/prettyString-Canonical> "solid object" ;
	<http://sw.cyc.com/2006/07/27/cyc/prettyString> "solid stuff" , "solid objects" ;
	<http://www.w3.org/2000/01/rdf-schema#subClassOf> <http://sw.cyc.com/2006/07/27/cyc/Container-Underspecified> , <http://sw.cyc.com/2006/07/27/cyc/NonFluidlikeTangibleThing> , <http://sw.cyc.com/2006/07/27/cyc/ContainerIndependentShapedThing> ;
	<http://www.w3.org/2002/07/owl#disjointWith> <http://sw.cyc.com/2006/07/27/cyc/SemiSolidTangibleThing> , <http://sw.cyc.com/2006/07/27/cyc/FluidTangibleThing> .

<http://sw.cyc.com/2006/07/27/cyc/AnimalBodyPart> <http://www.w3.org/2000/01/rdf-schema#comment> "A specialization of #$AnimalBodyRegion.  Each instance of #$AnimalBodyPart is an anatomical part of some living animal, and thus is itself an instance of #$BiologicalLivingObject (q.v).  #$AnimalBodyPart includes both highly localized organs (for example, hearts) and physical systems composed of parts distributed throughout an animal's body (such as an animal's circulatory system and nervous system).  Note that severed limbs and removed organs are _not_ instances of this collection, since they are not _parts_ of some living animal." ;
	a <http://sw.cyc.com/2006/07/27/cyc/ExistingObjectType> .

<http://sw.cyc.com/2006/07/27/cyc/AbdominalAorta> <http://sw.cyc.com/2006/07/27/cyc/prettyString> "abdominal aortas" , "abdominal aortae" ;
	<http://www.w3.org/2000/01/rdf-schema#subClassOf> <http://sw.cyc.com/2006/07/27/cyc/SystemicArtery> ;
	<http://sw.cyc.com/2006/07/27/cyc/sharedNotes> <http://sw.cyc.com/2006/07/27/cyc/BeforeMajorChangesToAnatomicalParts> .

<http://sw.cyc.com/2006/07/27/cyc/SystemicArtery> <http://www.w3.org/2000/01/rdf-schema#comment> "The collection of all arteries which provide #$OxygenatedBlood from the #$Heart to the body.  This includes every #$Artery except pulmonary arteries (#$PulmonaryArtery-Generic) which carry #$DeoxygenatedBlood." ;
	a <http://sw.cyc.com/2006/07/27/cyc/AnimalBodyPartType> , <http://sw.cyc.com/2006/07/27/cyc/InternalAnimalBodyRegionType> ;
	<http://sw.cyc.com/2006/07/27/cyc/prettyString-Canonical> "systemic artery" ;
	<http://sw.cyc.com/2006/07/27/cyc/prettyString> "systemic arteries" ;
	<http://www.w3.org/2000/01/rdf-schema#subClassOf> <http://sw.cyc.com/2006/07/27/cyc/Artery> .

<http://sw.cyc.com/2006/07/27/cyc/InternalAnimalBodyRegionType> <http://www.w3.org/2000/01/rdf-schema#comment> "A #$SecondOrderCollection and a specialization of #$OrganismConstituentType.  Each instance of #$InternalAnimalBodyRegionType is a specialization of #$AnimalBodyRegion whose instances are, under normal circumstances, located completely within (i.e. #$in-ContCompletely) the outer surface of an animal.  Instances include #$Heart, #$Brain, and #$Bone-BodyPart. Non-instances include #$Head-AnimalBodyPart, #$Wing-AnimalBodyPart,and #$UpperBody-Human, which are instances of #$ExternalAnimalBodyRegionType (q.v.)." ;
	a <http://sw.cyc.com/2006/07/27/cyc/SecondOrderCollection> ;
	<http://sw.cyc.com/2006/07/27/cyc/prettyString-Canonical> "internal animal body region type" ;
	<http://www.w3.org/2000/01/rdf-schema#subClassOf> <http://sw.cyc.com/2006/07/27/cyc/FirstOrderCollection> , <http://sw.cyc.com/2006/07/27/cyc/OrganismConstituentType> ;
	<http://sw.cyc.com/2006/07/27/cyc/typeGenls> <http://sw.cyc.com/2006/07/27/cyc/AnimalBodyRegion> .

<http://sw.cyc.com/2006/07/27/cyc/BeforeMajorChangesToAnatomicalParts> <http://www.w3.org/2000/01/rdf-schema#comment> "Before making major changes to #$AnimalBodyPartTypes, make sure you are familiar with CYC's anatomical system including the homuncular system.  Note that some English words apply both to a region of a body and an internal structure inside it (e.g. elbow, hip, ...).  These CYC concepts should be kept separate and care should be taken that the correct one is used.  If something seems strange or wrong with assertions dealing with #$AnimalBodyPartTypes, please alert #$Foxvog (9/1997)." ;
	a <http://sw.cyc.com/2006/07/27/cyc/Individual> ;
	<http://sw.cyc.com/2006/07/27/cyc/prettyString-Canonical> "Before Major Changes To Anatomical Parts" ;
	<http://sw.cyc.com/2006/07/27/cyc/quotedIsa> <http://sw.cyc.com/2006/07/27/cyc/SharedNote> .

<http://sw.cyc.com/2006/07/27/cyc/AbdominalCavity> <http://www.w3.org/2000/01/rdf-schema#comment> "The collection of AbdominalCavities, or cavities within the #$Abdomen, that each contains the digestive #$Organs (#$Stomach, intestines, #$Liver, #$Spleen, #$Pancreas, etc.).  An #$AbdominalCavity includes its walls." ;
	a <http://sw.cyc.com/2006/07/27/cyc/SpatiallyDisjointObjectType> , <http://sw.cyc.com/2006/07/27/cyc/AnimalBodyPartType> , <http://sw.cyc.com/2006/07/27/cyc/UniqueAnatomicalPartType> , <http://sw.cyc.com/2006/07/27/cyc/InternalAnimalBodyRegionType> ;
	<http://sw.cyc.com/2006/07/27/cyc/prettyString-Canonical> "abdominal cavity" ;
	<http://sw.cyc.com/2006/07/27/cyc/prettyString> "abdomens" , "abdomen" , "abdominal cavities" ;
	<http://www.w3.org/2000/01/rdf-schema#subClassOf> <http://sw.cyc.com/2006/07/27/cyc/SolidTangibleThing> , <http://sw.cyc.com/2006/07/27/cyc/AnimalBodyPart> , <http://sw.cyc.com/2006/07/27/cyc/InternalAnatomicalPart> , <http://sw.cyc.com/2006/07/27/cyc/CavityWithWalls> ;
	<http://sw.cyc.com/2006/07/27/cyc/sharedNotes> <http://sw.cyc.com/2006/07/27/cyc/BeforeMajorChangesToAnatomicalParts> .

<http://sw.cyc.com/2006/07/27/cyc/InternalAnatomicalPart> <http://www.w3.org/2000/01/rdf-schema#comment> "#$InternalAnatomicalPart is a specialization of #$OrganismPart.  Each instance of #$InternalAnatomicalPart is a part of the internal anatomy of an organism.  Example subcollections include #$CirculatorySystem and #$MiddleEar." ;
	a <http://sw.cyc.com/2006/07/27/cyc/FirstOrderCollection> , <http://sw.cyc.com/2006/07/27/cyc/CandidateKBCompletenessNode> ;
	<http://sw.cyc.com/2006/07/27/cyc/prettyString-Canonical> "internal body part" ;
	<http://sw.cyc.com/2006/07/27/cyc/prettyString> "internal anatomical part" , "internal anatomical parts" , "internal body parts" ;
	<http://www.w3.org/2000/01/rdf-schema#subClassOf> <http://sw.cyc.com/2006/07/27/cyc/OrganismPart> ;
	<http://www.w3.org/2002/07/owl#disjointWith> <http://sw.cyc.com/2006/07/27/cyc/ExternalAnatomicalPart> , <http://sw.cyc.com/2006/07/27/cyc/IndependentThing> .

<http://sw.cyc.com/2006/07/27/cyc/CavityWithWalls> <http://www.w3.org/2000/01/rdf-schema#comment> "A specialization of #$PartiallyTangible and #$Cavity.  Each instance of #$CavityWithWalls is an individual that spatially subsumes both the intangible space region \"inside\" a cavity (see #$CavityInteriorRegion) and the surfaces that constitute the inner walls of the cavity.  Compare #$CavityWithWalls to the collection #$Cavity; some instances of #$Cavity have their walls as parts, and some do not." ;
	a <http://sw.cyc.com/2006/07/27/cyc/ExistingObjectType> , <http://sw.cyc.com/2006/07/27/cyc/SpatiallyDisjointObjectType> ;
	<http://sw.cyc.com/2006/07/27/cyc/prettyString-Canonical> "walled cavity" ;
	<http://sw.cyc.com/2006/07/27/cyc/prettyString> "walled cavities" ;
	<http://www.w3.org/2000/01/rdf-schema#subClassOf> <http://sw.cyc.com/2006/07/27/cyc/Cavity> .

<http://sw.cyc.com/2006/07/27/cyc/AbdominalExerciseDevice> <http://www.w3.org/2000/01/rdf-schema#comment> """This is the collection of devices
designed specifically to work the abdominal muscles.""" ;
	a <http://sw.cyc.com/2006/07/27/cyc/ExistingObjectType> , <http://sw.cyc.com/2006/07/27/cyc/SpatiallyDisjointObjectType> , <http://sw.cyc.com/2006/07/27/cyc/ArtifactTypeByFunction> ;
	<http://sw.cyc.com/2006/07/27/cyc/prettyString-Canonical> "ab machine" ;
	<http://sw.cyc.com/2006/07/27/cyc/prettyString> "abdominal exercise machine" , "abdominal exercise machines" , "abdominal machine" , "abdominal machines" , "ab exerciser" .

<http://sw.cyc.com/2006/07/27/cyc/AbducensNerve> a <http://sw.cyc.com/2006/07/27/cyc/SymmetricAnatomicalPartType> ;
	<http://sw.cyc.com/2006/07/27/cyc/prettyString-Canonical> "abducens nerve" ;
	<http://sw.cyc.com/2006/07/27/cyc/prettyString> "abducens nerves" , "sixth cranial nerve" , "sixth cranial nerves" , "abducent nerve" , "abducent nerves" ;
	<http://www.w3.org/2000/01/rdf-schema#subClassOf> <http://sw.cyc.com/2006/07/27/cyc/CranialNerve> , <http://sw.cyc.com/2006/07/27/cyc/MotorNerve> ;
	<http://sw.cyc.com/2006/07/27/cyc/sharedNotes> <http://sw.cyc.com/2006/07/27/cyc/BeforeMajorChangesToAnatomicalParts> .

<http://sw.cyc.com/2006/07/27/cyc/CranialNerve> <http://www.w3.org/2000/01/rdf-schema#comment> "The collection of all cranial #$Nerves.  In an individual #$CranialNerves appear as 12 pairs of #$Nerves extending from the #$Brain." ;
	a <http://sw.cyc.com/2006/07/27/cyc/AnimalBodyPartType> , <http://sw.cyc.com/2006/07/27/cyc/InternalAnimalBodyRegionType> ;
	<http://sw.cyc.com/2006/07/27/cyc/prettyString-Canonical> "cranial nerve" ;
	<http://sw.cyc.com/2006/07/27/cyc/prettyString> "cranial nerves" ;
	<http://www.w3.org/2000/01/rdf-schema#subClassOf> <http://sw.cyc.com/2006/07/27/cyc/Nerve> ;
	<http://sw.cyc.com/2006/07/27/cyc/siblingDisjointExceptions> <http://sw.cyc.com/2006/07/27/cyc/MotorNerve> , <http://sw.cyc.com/2006/07/27/cyc/SensoryNerve> .

<http://sw.cyc.com/2006/07/27/cyc/MotorNerve> <http://www.w3.org/2000/01/rdf-schema#comment> "The collection of all solely motor #$Nerves.  Each #$MotorNerve is a #$Nerve that #$innervates a #$Muscle by signalling for it to contract or relax.  A #$Nerve containing both motor and sensory #$Neurons is a #$SensoryMotorNerve." ;
	a <http://sw.cyc.com/2006/07/27/cyc/AnimalBodyPartType> , <http://sw.cyc.com/2006/07/27/cyc/InternalAnimalBodyRegionType> ;
	<http://sw.cyc.com/2006/07/27/cyc/prettyString-Canonical> "motor nerve" ;
	<http://sw.cyc.com/2006/07/27/cyc/prettyString> "motor nerves" ;
	<http://www.w3.org/2000/01/rdf-schema#subClassOf> <http://sw.cyc.com/2006/07/27/cyc/Nerve> , <http://sw.cyc.com/2006/07/27/cyc/DirectedAcyclicPathSystem> .

<http://sw.cyc.com/2006/07/27/cyc/SymmetricAnatomicalPartType> <http://www.w3.org/2000/01/rdf-schema#comment> "A collection of collections.  Instances are types of #$anatomicalParts of bilaterally symmetrical organisms (#$Organism-Whole) which occur in bilaterally symmetric pairs.  This is not intended to include broader categories like #$Tooth, #$Rib-AnimalBodyPart, or #$Finger, but the specific parts of which the organism only has two (EyeTooth, FifthRib, or #$RingFinger)." ;
	a <http://sw.cyc.com/2006/07/27/cyc/AtemporalNecessarilyEssentialCollectionType> , <http://sw.cyc.com/2006/07/27/cyc/SiblingDisjointCollectionType> , <http://sw.cyc.com/2006/07/27/cyc/FacetingCollectionType> , <http://sw.cyc.com/2006/07/27/cyc/SecondOrderCollection> , <http://sw.cyc.com/2006/07/27/cyc/Parts-Topic> ;
	<http://sw.cyc.com/2006/07/27/cyc/prettyString-Canonical> "type of symmetric anatomical part" ;
	<http://sw.cyc.com/2006/07/27/cyc/prettyString> "types of symmetric anatomical part" ;
	<http://www.w3.org/2000/01/rdf-schema#subClassOf> <http://sw.cyc.com/2006/07/27/cyc/AnimalBodyPartType> ;
	<http://www.w3.org/2002/07/owl#disjointWith> <http://sw.cyc.com/2006/07/27/cyc/UniqueAnatomicalPartType> .

<http://sw.cyc.com/2006/07/27/cyc/AbductingSomeone> <http://www.w3.org/2000/01/rdf-schema#comment> """A collection of events and a specialization of #$TakingAPersonPrisoner.  In each instance of #$AbductingSomeone, a #$Person is taken captive, moved somewhere, and held by another (or group of others).
<p>
Abductions are usually done illegally; see the specialization #$KidnappingSomeone. But note that this need not be the case.  For example, in certain circumstances a government agent might legally abduct a person for questioning; a parent might legally abduct a minor from the grounds of a religious cult; some people claim to have been abducted by aliens.
<p>
Note also that, while an abduction is typically done against the victim's will, this might not be the case if s/he is (say) unconscious, extremely ill, mentally disturbed, or very young.""" ;
	a <http://sw.cyc.com/2006/07/27/cyc/TemporalObjectType> ;
	<http://sw.cyc.com/2006/07/27/cyc/prettyString-Canonical> "abduction" ;
	<http://sw.cyc.com/2006/07/27/cyc/prettyString> "abduct" , "abducted" , "abducts" , "abducting" , "have abducted" , "has abducted" , "will abduct" , "had abducted" , "will have abducted" , "snatching" , "snatch" , "snatched" , "snatches" , "have snatched" , "has snatched" , "will snatch" , "had snatched" , "will have snatched" , "abductions" ;
	<http://www.w3.org/2000/01/rdf-schema#subClassOf> <http://sw.cyc.com/2006/07/27/cyc/ActsCommonlyConsideredCriminal> , <http://sw.cyc.com/2006/07/27/cyc/TakingAPersonPrisoner> .

<http://sw.cyc.com/2006/07/27/cyc/ActsCommonlyConsideredCriminal> <http://www.w3.org/2000/01/rdf-schema#comment> "A collection of actions.  Instances of #$ActsCommonlyConsideredCriminal are actions which are commonly considered illegal, i.e., in most legal systems.  The primary purpose of this collection is to group together types of actions such as #$Murder and #$Stealing-Generic, which are almost universally considered criminal.  However, individual instances of this collection are not necessarily instances of #$CriminalAct in every context or under every #$GovernmentCOC." ;
	a <http://sw.cyc.com/2006/07/27/cyc/FirstOrderCollection> , <http://sw.cyc.com/2006/07/27/cyc/QAClarifyingCollectionType> , <http://sw.cyc.com/2006/07/27/cyc/FocalTermSceneCandidate-Intermediate> ;
	<http://sw.cyc.com/2006/07/27/cyc/prettyString-Canonical> "possibly criminal act" ;
	<http://sw.cyc.com/2006/07/27/cyc/prettyString> "possibly criminal acts" ;
	<http://www.w3.org/2000/01/rdf-schema#subClassOf> <http://sw.cyc.com/2006/07/27/cyc/HumanActivity> .

<http://sw.cyc.com/2006/07/27/cyc/AspatialInformationStore> <http://www.w3.org/2000/01/rdf-schema#comment> "A specialization of #$AspatialThing, #$IntangibleIndividual, and #$InformationStore.  #$AspatialInformationStore is the collection of all information stores that have no spatial location.  Specializations of #$AspatialInformationStore include #$ConceptualWork, #$Microtheory, #$AbstractInformationStructure, and #$FieldOfStudy.  Although no instance of #$AspatialInformationStore has a spatial location, some instances can have multiple spatio-temporal \"embodiments\". For example, an instance of #$PropositionalInformationThing may be the content of several concrete documents, such as several instances of #$BookCopy (see #$containsInfoPropositional-IBT); and several distinct events, such as spoken utterances, may have a certain unique #$Proposition as their content (see #$containsInformation)." ;
	a <http://sw.cyc.com/2006/07/27/cyc/StuffType> , <http://sw.cyc.com/2006/07/27/cyc/InformationAndCWs-Topic> , <http://sw.cyc.com/2006/07/27/cyc/TestOWLExportConcept> ;
	<http://sw.cyc.com/2006/07/27/cyc/prettyString-Canonical> "information" ;
	<http://sw.cyc.com/2006/07/27/cyc/prettyString> "knowledge" , "info" , "data" , "datum" ;
	<http://www.w3.org/2000/01/rdf-schema#subClassOf> <http://sw.cyc.com/2006/07/27/cyc/IntangibleIndividual> , <http://sw.cyc.com/2006/07/27/cyc/AspatialThing> , <http://sw.cyc.com/2006/07/27/cyc/InformationStore> ;
	<http://www.w3.org/2002/07/owl#disjointWith> <http://sw.cyc.com/2006/07/27/cyc/Agent-Generic> ;
	<http://sw.cyc.com/2006/07/27/cyc/facets-Generic> <http://sw.cyc.com/2006/07/27/cyc/AISTypeByEvaluationTone> .

<http://sw.cyc.com/2006/07/27/cyc/CycHLSupportModule> <http://www.w3.org/2000/01/rdf-schema#comment> """A specialization of #$CycProgramModule-CW each instance of 
which is a code module within the Cyc system such that, for
a certain type of #$CycHLSupportDatastructure (q.v.) claiming 
that some #$CycLSentence has some truth value in some 
#$Microtheory, the code module can verify the validity of 
that support and generate a justification for it.""" ;
	a <http://sw.cyc.com/2006/07/27/cyc/ObjectType> , <http://sw.cyc.com/2006/07/27/cyc/KBDependentCollection> ;
	<http://sw.cyc.com/2006/07/27/cyc/prettyString-Canonical> "Cyc HL support module" ;
	<http://sw.cyc.com/2006/07/27/cyc/prettyString> "Cyc HL support modules" ;
	<http://www.w3.org/2000/01/rdf-schema#subClassOf> <http://sw.cyc.com/2006/07/27/cyc/CycProgramModule-CW> .

<http://sw.cyc.com/2006/07/27/cyc/uniquelyIdentifiedInType> <http://www.w3.org/2000/01/rdf-schema#comment> "(#$uniquelyIdentifiedInType AIT COL) means that there is an identifier ID such that (#$subLIdentifier AIT ID) which uniquely identifies AIT in the SubL programming environment among all instances of COL.  For example, in SubL, the symbol :TRUE-DEF uniquely identifies #$DefaultTrue among the other instances of #$CycHLTruthValue, so we would state both (#$uniquelyIdentifiedInType #$DefaultTrue #$CycHLTruthValue) and (#$subLIdentifier #$DefaultTrue (#$ExpandSubLFn NIL :TRUE-DEF))." ;
	a <http://www.w3.org/2000/01/rdf-schema#Property> ;
	<http://sw.cyc.com/2006/07/27/cyc/prettyString-Canonical> "Uniquely Identified In Type" ;
	<http://sw.cyc.com/2006/07/27/cyc/quotedIsa> <http://sw.cyc.com/2006/07/27/cyc/OpenCycDefinitionalPredicate> ;
	<http://www.w3.org/2000/01/rdf-schema#domain> <http://sw.cyc.com/2006/07/27/cyc/AspatialInformationStore> ;
	<http://sw.cyc.com/2006/07/27/cyc/arity> "2"^^<http://www.w3.org/2001/XMLSchema#long> ;
	<http://www.w3.org/2000/01/rdf-schema#range> <http://www.w3.org/2002/07/owl#Class> ;
	<http://www.w3.org/2000/01/rdf-schema#subPropertyOf> <http://www.w3.org/1999/02/22-rdf-syntax-ns#type> ;
	<http://sw.cyc.com/2006/07/27/cyc/arg2Genl> <http://sw.cyc.com/2006/07/27/cyc/AspatialInformationStore> .

<http://sw.cyc.com/2006/07/27/cyc/AbductionTest> <http://www.w3.org/2000/01/rdf-schema#comment> "A collection of tests, whose instances should test system functionality that is relevant to the way the abductive tactician works. The name of these test should usuallky begin with \"AbductionTest-\"." ;
	a <http://sw.cyc.com/2006/07/27/cyc/KBDependentCollection> , <http://sw.cyc.com/2006/07/27/cyc/KBContentTestSpecificationType> ;
	<http://sw.cyc.com/2006/07/27/cyc/prettyString-Canonical> "abduction test" ;
	<http://www.w3.org/2000/01/rdf-schema#subClassOf> <http://sw.cyc.com/2006/07/27/cyc/KBContentTest-FullySpecified> ;
	<http://sw.cyc.com/2006/07/27/cyc/quotedIsa> <http://sw.cyc.com/2006/07/27/cyc/TestQueryConstant> .

<http://sw.cyc.com/2006/07/27/cyc/KBContentTest-FullySpecified> <http://www.w3.org/2000/01/rdf-schema#comment> "Each instance of #$KBContentTest-FullySpecified is a specification for a CycL query and the expected query results." ;
	a <http://sw.cyc.com/2006/07/27/cyc/ObjectType> , <http://sw.cyc.com/2006/07/27/cyc/KBDependentCollection> ;
	<http://sw.cyc.com/2006/07/27/cyc/prettyString-Canonical> "specification for a CycL query and its expected results" ;
	<http://sw.cyc.com/2006/07/27/cyc/prettyString> "specifications for a CycL query and its expected results" ;
	<http://www.w3.org/2000/01/rdf-schema#subClassOf> <http://sw.cyc.com/2006/07/27/cyc/StructurallySpecificWork> , <http://sw.cyc.com/2006/07/27/cyc/KBContentTest-QuerySentenceSpecified> ;
	<http://sw.cyc.com/2006/07/27/cyc/quotedIsa> <http://sw.cyc.com/2006/07/27/cyc/TestQueryConstant> , <http://sw.cyc.com/2006/07/27/cyc/ProprietaryConstant> ;
	<http://sw.cyc.com/2006/07/27/cyc/facets-Generic> <http://sw.cyc.com/2006/07/27/cyc/KBContentTestTypeByOwner> .

<http://sw.cyc.com/2006/07/27/cyc/KBContentTestSpecificationType> <http://www.w3.org/2000/01/rdf-schema#comment> "Each instance of #$KBContentTestSpecificationType is a collection whose instances are individual KB content test definitions.  Instances of #$KBContentTestSpecificationType represent categories of tests grouped together because they test similar functionality, and which might sensibly be run as a unit." ;
	a <http://sw.cyc.com/2006/07/27/cyc/KBDependentCollection> , <http://sw.cyc.com/2006/07/27/cyc/SecondOrderCollection> ;
	<http://sw.cyc.com/2006/07/27/cyc/prettyString-Canonical> "type of specification for a CycL query and its expected results" ;
	<http://sw.cyc.com/2006/07/27/cyc/prettyString> "types of specification for a CycL query and its expected results" ;
	<http://www.w3.org/2000/01/rdf-schema#subClassOf> <http://sw.cyc.com/2006/07/27/cyc/ObjectType> , <http://sw.cyc.com/2006/07/27/cyc/KBDependentCollection> , <http://sw.cyc.com/2006/07/27/cyc/SoftwareTestSpecificationType> ;
	<http://sw.cyc.com/2006/07/27/cyc/quotedIsa> <http://sw.cyc.com/2006/07/27/cyc/TestQueryConstant> ;
	<http://sw.cyc.com/2006/07/27/cyc/typeGenls> <http://sw.cyc.com/2006/07/27/cyc/KBContentTest-FullySpecified> .

<http://sw.cyc.com/2006/07/27/cyc/AbductionTestQueryFolder> a <http://sw.cyc.com/2006/07/27/cyc/KEInteractionFolder> ;
	<http://sw.cyc.com/2006/07/27/cyc/prettyString-Canonical> "Abduction Test Query Folder" .

<http://sw.cyc.com/2006/07/27/cyc/KEInteractionFolder> <http://www.w3.org/2000/01/rdf-schema#comment> "Instances of this collection are (abstract) folders which organize pages of content (cf. #$PageTemplate) which should be used to facilitate interactions with a user." ;
	a <http://sw.cyc.com/2006/07/27/cyc/ObjectType> , <http://sw.cyc.com/2006/07/27/cyc/KBDependentCollection> ;
	<http://sw.cyc.com/2006/07/27/cyc/prettyString-Canonical> "Cyc ke interaction folder" ;
	<http://sw.cyc.com/2006/07/27/cyc/prettyString> "Cyc ke interaction folders" ;
	<http://www.w3.org/2000/01/rdf-schema#subClassOf> <http://sw.cyc.com/2006/07/27/cyc/KEInteractionResource> .

<http://sw.cyc.com/2006/07/27/cyc/TestQueryConstant> <http://www.w3.org/2000/01/rdf-schema#comment> "The collection of all terms that belong to the ontology of internal KB content tests in Cyc." ;
	a <http://www.w3.org/2002/07/owl#Class> , <http://sw.cyc.com/2006/07/27/cyc/CycLExpressionType> ;
	<http://sw.cyc.com/2006/07/27/cyc/prettyString-Canonical> "test query constant" ;
	<http://www.w3.org/2000/01/rdf-schema#subClassOf> <http://www.w3.org/2002/07/owl#Thing> , <http://sw.cyc.com/2006/07/27/cyc/CycLTerm> ;
	<http://sw.cyc.com/2006/07/27/cyc/quotedIsa> <http://sw.cyc.com/2006/07/27/cyc/TestQueryConstant> .

<http://sw.cyc.com/2006/07/27/cyc/abductiveExpansion> <http://www.w3.org/2000/01/rdf-schema#comment> "An instance of #$UnderstandingEnrichmentRelation.  (#$abductiveExpansion EXPLANANDUM HYP-EXPLANANS) means that if EXPLANANDUM is true, a good way to make sense of EXPLANANDUM is to postulate that HYP-EXPLANANS is true, and that HYP-EXPLANANS broadens the level of detail in terms of which EXPLANANDUM is understood.  For example, if it is true that someone applies toothpaste to a toothbrush (and that is our explanandum), and it is known that applications of toothpaste to toothbrushes are typical components of events in which one brushes one's own teeth, then a good way to make sense of the application of toothpaste to the toothbrush is to suppose (as a hypthothetical explanans) that there is an event of which the application is a component which is itself an event in which the applier is brushing her own teeth. (#$abductiveExpansion EXPLANANDUM HYP-EXPLANANS) also means that the truth of EXPLANANDUM is evidence (though generally not sufficient evidence) for the truth of HYP-EXPLANANS.  Thus, if a person applies toothpaste to a toothbrush, that is evidence that she is about to brush her teeth. It is possible that various legitimate values for HYP-EXPLANANS are mutually inconsistent for a single value of EXPLANANDUM -- perhaps the reason someone applies toothpaste to a toothbrush is to brush a dog's teeth." ;
	a <http://www.w3.org/2000/01/rdf-schema#Property> , <http://sw.cyc.com/2006/07/27/cyc/UnderstandingEnrichmentRelation> ;
	<http://sw.cyc.com/2006/07/27/cyc/prettyString-Canonical> "Abductive Expansion" ;
	<http://sw.cyc.com/2006/07/27/cyc/arity> "2"^^<http://www.w3.org/2001/XMLSchema#long> ;
	<http://www.w3.org/2000/01/rdf-schema#subPropertyOf> <http://sw.cyc.com/2006/07/27/cyc/abductivelyRelevant> ;
	<http://sw.cyc.com/2006/07/27/cyc/arg1QuotedIsa> <http://sw.cyc.com/2006/07/27/cyc/CycLSentence-Assertible> ;
	<http://sw.cyc.com/2006/07/27/cyc/arg2QuotedIsa> <http://sw.cyc.com/2006/07/27/cyc/CycLSentence-Assertible> ;
	<http://sw.cyc.com/2006/07/27/cyc/quotedArgument> "2"^^<http://www.w3.org/2001/XMLSchema#long> , "1"^^<http://www.w3.org/2001/XMLSchema#long> .

<http://sw.cyc.com/2006/07/27/cyc/arg1QuotedIsa> <http://www.w3.org/2000/01/rdf-schema#comment> "A binary #$Predicate (#$arg1QuotedIsa RELN COL) means that semantic well-formedness requires that the term given as the first argument to RELN must be an instance of the #$SubLExpressionType COL. That is, (RELN ARG1 ...) is semantically well-formed only if (#$quotedIsa ARG1 COL) holds." ;
	a <http://www.w3.org/2000/01/rdf-schema#Property> , <http://sw.cyc.com/2006/07/27/cyc/DefaultMonotonicPredicate> , <http://sw.cyc.com/2006/07/27/cyc/NonAbduciblePredicate> , <http://sw.cyc.com/2006/07/27/cyc/ArgQuotedIsaBinaryPredicate> ;
	<http://sw.cyc.com/2006/07/27/cyc/prettyString-Canonical> "Arg 1 Quoted Isa" ;
	<http://sw.cyc.com/2006/07/27/cyc/quotedIsa> <http://sw.cyc.com/2006/07/27/cyc/OpenCycDefinitionalPredicate> ;
	<http://www.w3.org/2000/01/rdf-schema#domain> <http://sw.cyc.com/2006/07/27/cyc/Relation> ;
	<http://sw.cyc.com/2006/07/27/cyc/arity> "2"^^<http://www.w3.org/2001/XMLSchema#long> ;
	<http://sw.cyc.com/2006/07/27/cyc/sharedNotes> <http://sw.cyc.com/2006/07/27/cyc/ArgumentTypeChecking-FORTSvsNonReifiedNATS> ;
	<http://www.w3.org/2000/01/rdf-schema#range> <http://sw.cyc.com/2006/07/27/cyc/SubLExpressionType> .

<http://sw.cyc.com/2006/07/27/cyc/AbductiveInferenceProcess> <http://www.w3.org/2000/01/rdf-schema#subClassOf> <http://sw.cyc.com/2006/07/27/cyc/Individual> , <http://sw.cyc.com/2006/07/27/cyc/Reasoning> .

<http://sw.cyc.com/2006/07/27/cyc/Reasoning> <http://www.w3.org/2000/01/rdf-schema#comment> "A sub-collection of #$Thinking. Each instance is thinking that is coherent and logical." ;
	a <http://www.w3.org/2002/07/owl#Class> , <http://sw.cyc.com/2006/07/27/cyc/FirstOrderCollection> ;
	<http://sw.cyc.com/2006/07/27/cyc/prettyString-Canonical> "logical argument" ;
	<http://sw.cyc.com/2006/07/27/cyc/prettyString> "reasoning" , "arguation" , "line of reasoning" , "lines of reasoning" , "logical arguments" ;
	<http://www.w3.org/2000/01/rdf-schema#subClassOf> <http://sw.cyc.com/2006/07/27/cyc/Thinking> ;
	<http://sw.cyc.com/2006/07/27/cyc/quotedIsa> <http://sw.cyc.com/2006/07/27/cyc/StubTerm> , <http://sw.cyc.com/2006/07/27/cyc/WordNetWorkflowConstant-NotFullyReviewed> , <http://sw.cyc.com/2006/07/27/cyc/PoorlyOntologized> .

<http://sw.cyc.com/2006/07/27/cyc/AbductorDigitiMinimi> <http://www.w3.org/2000/01/rdf-schema#comment> "The #$Collection of all instances of #$AbductorDigitiMinimi #$Muscle.  The #$AbductorDigitiMinimi abducts the #$LittleFinger away from the other #$Fingers parallel to the #$PalmOfHand." ;
	a <http://sw.cyc.com/2006/07/27/cyc/SpatiallyDisjointObjectType> , <http://sw.cyc.com/2006/07/27/cyc/InternalAnimalBodyRegionType> , <http://sw.cyc.com/2006/07/27/cyc/SymmetricAnatomicalPartType> ;
	<http://sw.cyc.com/2006/07/27/cyc/prettyString-Canonical> "abductor digiti minimi muscle" ;
	<http://sw.cyc.com/2006/07/27/cyc/prettyString> "abductor digiti minimi muscles" ;
	<http://www.w3.org/2000/01/rdf-schema#subClassOf> <http://sw.cyc.com/2006/07/27/cyc/SkeletalMuscle> ;
	<http://sw.cyc.com/2006/07/27/cyc/sharedNotes> <http://sw.cyc.com/2006/07/27/cyc/BeforeMajorChangesToAnatomicalParts> .

<http://sw.cyc.com/2006/07/27/cyc/SkeletalMuscle> <http://www.w3.org/2000/01/rdf-schema#comment> "The collection of #$Muscles which are connected at at least one end to a bone. Skeletal muscles are involved in movements of the #$SkeletalSystem." ;
	a <http://sw.cyc.com/2006/07/27/cyc/SpatiallyDisjointObjectType> , <http://sw.cyc.com/2006/07/27/cyc/AnimalBodyPartType> , <http://sw.cyc.com/2006/07/27/cyc/InternalAnimalBodyRegionType> ;
	<http://sw.cyc.com/2006/07/27/cyc/prettyString-Canonical> "skeletal muscle" ;
	<http://sw.cyc.com/2006/07/27/cyc/prettyString> "skeletal muscles" ;
	<http://www.w3.org/2000/01/rdf-schema#subClassOf> <http://sw.cyc.com/2006/07/27/cyc/StriatedMuscle> .

<http://sw.cyc.com/2006/07/27/cyc/AbductorPollicisBrevis> <http://www.w3.org/2000/01/rdf-schema#comment> "The #$Collection of all instances of #$AbductorPollicisBrevis#$Muscle.  The #$AbductorPollicisBrevis brings the #$Thumb into opposition." ;
	a <http://sw.cyc.com/2006/07/27/cyc/SpatiallyDisjointObjectType> , <http://sw.cyc.com/2006/07/27/cyc/InternalAnimalBodyRegionType> , <http://sw.cyc.com/2006/07/27/cyc/SymmetricAnatomicalPartType> ;
	<http://sw.cyc.com/2006/07/27/cyc/prettyString-Canonical> "abductor pollicis brevis muscle" ;
	<http://sw.cyc.com/2006/07/27/cyc/prettyString> "abductor pollicis brevis muscles" ;
	<http://www.w3.org/2000/01/rdf-schema#subClassOf> <http://sw.cyc.com/2006/07/27/cyc/SkeletalMuscle> ;
	<http://sw.cyc.com/2006/07/27/cyc/sharedNotes> <http://sw.cyc.com/2006/07/27/cyc/BeforeMajorChangesToAnatomicalParts> .

<http://sw.cyc.com/2006/07/27/cyc/AbductorPollicisLongus> <http://www.w3.org/2000/01/rdf-schema#comment> "The #$Collection of all instances of #$AbductorPollicisLongus #$Muscle.  The #$AbductorPollicisLongus abducts the #$Thumb in a radial direction." ;
	a <http://sw.cyc.com/2006/07/27/cyc/SpatiallyDisjointObjectType> , <http://sw.cyc.com/2006/07/27/cyc/InternalAnimalBodyRegionType> , <http://sw.cyc.com/2006/07/27/cyc/SymmetricAnatomicalPartType> ;
	<http://sw.cyc.com/2006/07/27/cyc/prettyString-Canonical> "abductor pollicis longus muscle" ;
	<http://sw.cyc.com/2006/07/27/cyc/prettyString> "abductor pollicis longus muscles" ;
	<http://www.w3.org/2000/01/rdf-schema#subClassOf> <http://sw.cyc.com/2006/07/27/cyc/SkeletalMuscle> ;
	<http://sw.cyc.com/2006/07/27/cyc/sharedNotes> <http://sw.cyc.com/2006/07/27/cyc/BeforeMajorChangesToAnatomicalParts> .

<http://sw.cyc.com/2006/07/27/cyc/AbdulAhadGuru> a <http://sw.cyc.com/2006/07/27/cyc/Individual> , <http://sw.cyc.com/2006/07/27/cyc/Person> ;
	<http://sw.cyc.com/2006/07/27/cyc/prettyString-Canonical> "Abdul Ahad Guru" ;
	<http://sw.cyc.com/2006/07/27/cyc/prettyString> "Abdul Guru" , "Guru" .

<http://sw.cyc.com/2006/07/27/cyc/AbdulAzizMoqrin> a <http://sw.cyc.com/2006/07/27/cyc/Individual> , <http://sw.cyc.com/2006/07/27/cyc/Person> ;
	<http://sw.cyc.com/2006/07/27/cyc/prettyString-Canonical> "Abdul Aziz Moqrin" ;
	<http://sw.cyc.com/2006/07/27/cyc/prettyString> "Moqrin" , "Abdul Moqrin" .

<http://sw.cyc.com/2006/07/27/cyc/AbdulHameedButt> a <http://sw.cyc.com/2006/07/27/cyc/Individual> , <http://sw.cyc.com/2006/07/27/cyc/Person> ;
	<http://sw.cyc.com/2006/07/27/cyc/prettyString-Canonical> "Abdul Hameed Butt" ;
	<http://sw.cyc.com/2006/07/27/cyc/prettyString> "Butt" , "Abdul Butt" .

<http://sw.cyc.com/2006/07/27/cyc/AbdulKalam> a <http://sw.cyc.com/2006/07/27/cyc/AdultMaleHuman> ;
	<http://sw.cyc.com/2006/07/27/cyc/prettyString-Canonical> "Abdul Kalam" ;
	<http://sw.cyc.com/2006/07/27/cyc/prettyString> "Kalam" .

<http://sw.cyc.com/2006/07/27/cyc/AbdulKarimNasrallah> a <http://sw.cyc.com/2006/07/27/cyc/Person> ;
	<http://sw.cyc.com/2006/07/27/cyc/prettyString-Canonical> "Sayyed Abdul Karim Nasrallah" ;
	<http://sw.cyc.com/2006/07/27/cyc/prettyString> "Abdul Nasrallah" , "Abdul K. Nasrallah" , "Abdul Karim Nasrallah" .

<http://sw.cyc.com/2006/07/27/cyc/AbdullahIbnAbdAl-AzizAl-Saud> a <http://sw.cyc.com/2006/07/27/cyc/Individual> , <http://sw.cyc.com/2006/07/27/cyc/HomoSapiens> ;
	<http://sw.cyc.com/2006/07/27/cyc/prettyString-Canonical> "Abdullah ibn Abd al-Aziz al-Sa'ud" .

<http://sw.cyc.com/2006/07/27/cyc/AbdullahSalimAl-Badri> a <http://sw.cyc.com/2006/07/27/cyc/Individual> , <http://sw.cyc.com/2006/07/27/cyc/HomoSapiens> ;
	<http://sw.cyc.com/2006/07/27/cyc/prettyString-Canonical> "Abdullah Salim Al-Badri" .

<http://sw.cyc.com/2006/07/27/cyc/AbdulMajeedDar> a <http://sw.cyc.com/2006/07/27/cyc/Individual> , <http://sw.cyc.com/2006/07/27/cyc/Person> ;
	<http://sw.cyc.com/2006/07/27/cyc/prettyString-Canonical> "Abdul Majeed Dar" ;
	<http://sw.cyc.com/2006/07/27/cyc/prettyString> "DAR" , "Abdul Dar" .

<http://sw.cyc.com/2006/07/27/cyc/AbdulRahimMaluah> a <http://sw.cyc.com/2006/07/27/cyc/Individual> , <http://sw.cyc.com/2006/07/27/cyc/Person> ;
	<http://sw.cyc.com/2006/07/27/cyc/prettyString-Canonical> "Abdul Rahim Maluah" ;
	<http://sw.cyc.com/2006/07/27/cyc/prettyString> "Abdul Maluah" , "Maluah" .

<http://sw.cyc.com/2006/07/27/cyc/AbdulRasoolSayyaf> <http://www.w3.org/2000/01/rdf-schema#comment> "Leader of the jihad in Afghanistan, according to  al Ridi." ;
	a <http://sw.cyc.com/2006/07/27/cyc/Individual> , <http://sw.cyc.com/2006/07/27/cyc/AdultMaleHuman> , <http://sw.cyc.com/2006/07/27/cyc/AfghanPerson> , <http://sw.cyc.com/2006/07/27/cyc/Leader> ;
	<http://sw.cyc.com/2006/07/27/cyc/prettyString-Canonical> "Abdul Rasool Sayyaf" .

<http://sw.cyc.com/2006/07/27/cyc/AfghanPerson> <http://www.w3.org/2000/01/rdf-schema#comment> "The collection of people who are #$citizens of #$Afghanistan, or who participate in its #$NationalCulture." ;
	a <http://sw.cyc.com/2006/07/27/cyc/NationalityGroupsInTheRegion-HormuzArea-Topic> , <http://sw.cyc.com/2006/07/27/cyc/TKBNationalityList> , <http://sw.cyc.com/2006/07/27/cyc/PersonTypeByGeoPoliticalAffiliation> , <http://sw.cyc.com/2006/07/27/cyc/PersonTypeByNationality> ;
	<http://sw.cyc.com/2006/07/27/cyc/prettyString-Canonical> "afghan" ;
	<http://sw.cyc.com/2006/07/27/cyc/prettyString> "afghans" , "Afghan person" , "Afghan people" , "Afghan persons" ;
	<http://www.w3.org/2000/01/rdf-schema#subClassOf> <http://sw.cyc.com/2006/07/27/cyc/Person> , <http://sw.cyc.com/2006/07/27/cyc/AsianCitizenOrSubject> .

<http://sw.cyc.com/2006/07/27/cyc/Leader> <http://www.w3.org/2000/01/rdf-schema#comment> "A collection of persons.  Each instance of #$Leader is a person who heads an instance of #$Organization.  Typically, a leader of an organization makes major decisions on behalf of the whole organization, has the authority to direct the organization's personnel to carry out those decisions, and is empowered to engage or negotiate with external agents to achieve the organization's goals.  This collection includes leaders of sub-organizations of larger organizations, such as department heads within larger organizations.  Note that a single person may be a leader in more than one organization.  See also the predicates #$hasLeaders and #$seniorExecutives, and the collection #$Manager." ;
	a <http://sw.cyc.com/2006/07/27/cyc/ExistingObjectType> , <http://www.w3.org/2002/07/owl#Class> , <http://sw.cyc.com/2006/07/27/cyc/ObjectType> , <http://sw.cyc.com/2006/07/27/cyc/FirstOrderCollection> , <http://sw.cyc.com/2006/07/27/cyc/TemporalStuffType> , <http://sw.cyc.com/2006/07/27/cyc/PeopleRelatedToOrganizations-Organization-Topic> ;
	<http://sw.cyc.com/2006/07/27/cyc/prettyString-Canonical> "leader" ;
	<http://sw.cyc.com/2006/07/27/cyc/prettyString> "Head" , "chieftain" , "chieftains" , "leaders" , "heads" , "chief" , "sarpanches" .

<http://sw.cyc.com/2006/07/27/cyc/AberdeenProvingGround> <http://sw.cyc.com/2006/07/27/cyc/prettyString> "Aberdeen" .

<http://sw.cyc.com/2006/07/27/cyc/NBCWeaponStorageFacility> <http://www.w3.org/2000/01/rdf-schema#comment> "#$NBCWeaponStorageFacility is the collection of storage facilities where nuclear, biological, or chemical weapons are typically stored." ;
	a <http://sw.cyc.com/2006/07/27/cyc/ExistingObjectType> , <http://sw.cyc.com/2006/07/27/cyc/SpatiallyDisjointObjectType> , <http://sw.cyc.com/2006/07/27/cyc/ArtifactualFeatureType> , <http://sw.cyc.com/2006/07/27/cyc/QAClarifyingCollectionType> , <http://sw.cyc.com/2006/07/27/cyc/MilitaryFacilityConcept> ;
	<http://sw.cyc.com/2006/07/27/cyc/prettyString-Canonical> "NBC weapon storage facility" ;
	<http://sw.cyc.com/2006/07/27/cyc/prettyString> "NBC weapons storage site" , "NBC weapons storage sites" , "NBC weapon storage facilities" ;
	<http://www.w3.org/2000/01/rdf-schema#subClassOf> <http://sw.cyc.com/2006/07/27/cyc/StorageFacility> , <http://sw.cyc.com/2006/07/27/cyc/MilitaryFacility> .

<http://sw.cyc.com/2006/07/27/cyc/ProvingGround> <http://www.w3.org/2000/01/rdf-schema#comment> """A tract of land used by a military organization for the testing and
development of various kinds of military hardware and weapons
systems.""" ;
	a <http://sw.cyc.com/2006/07/27/cyc/ExistingObjectType> , <http://sw.cyc.com/2006/07/27/cyc/SpatiallyDisjointObjectType> , <http://sw.cyc.com/2006/07/27/cyc/ArtifactualFeatureType> ;
	<http://sw.cyc.com/2006/07/27/cyc/prettyString-Canonical> "proving ground" ;
	<http://sw.cyc.com/2006/07/27/cyc/prettyString> "proving grounds" ;
	<http://www.w3.org/2000/01/rdf-schema#subClassOf> <http://sw.cyc.com/2006/07/27/cyc/NonNaturalThing> , <http://sw.cyc.com/2006/07/27/cyc/OutdoorLocation> .

<http://sw.cyc.com/2006/07/27/cyc/AbeVigoda> a <http://sw.cyc.com/2006/07/27/cyc/Individual> ;
	<http://sw.cyc.com/2006/07/27/cyc/prettyString-Canonical> "Abe Vigoda" ;
	<http://sw.cyc.com/2006/07/27/cyc/prettyString> "Vigoda" .

<http://sw.cyc.com/2006/07/27/cyc/AbgenixInc> a <http://sw.cyc.com/2006/07/27/cyc/Individual> , <http://sw.cyc.com/2006/07/27/cyc/PubliclyHeldCorporation> ;
	<http://sw.cyc.com/2006/07/27/cyc/prettyString-Canonical> "Abgenix Inc" .

<http://sw.cyc.com/2006/07/27/cyc/Abhorrence> <http://www.w3.org/2000/01/rdf-schema#comment> "Extreme repugnance felt towards a person or thing, typically resulting in strenuous efforts to avoid it." ;
	a <http://sw.cyc.com/2006/07/27/cyc/EmotionalQuantityType> , <http://sw.cyc.com/2006/07/27/cyc/AtemporalNecessarilyEssentialCollectionType> ;
	<http://sw.cyc.com/2006/07/27/cyc/prettyString-Canonical> "abhorrence" ;
	<http://www.w3.org/2000/01/rdf-schema#subClassOf> <http://sw.cyc.com/2006/07/27/cyc/Disgust> , <http://sw.cyc.com/2006/07/27/cyc/Dissatisfaction> , <http://sw.cyc.com/2006/07/27/cyc/Hate> .

<http://sw.cyc.com/2006/07/27/cyc/Disgust> <http://www.w3.org/2000/01/rdf-schema#comment> "A feeling of repulsion or aversion towards something considered distasteful or repugnant.  This is a #$Collection --- for an explanation of that, see #$Happiness.  Some more specialized #$FeelingTypes than #$Disgust include feelings of #$Abhorrence." ;
	a <http://sw.cyc.com/2006/07/27/cyc/EmotionalQuantityType> , <http://sw.cyc.com/2006/07/27/cyc/AtemporalNecessarilyEssentialCollectionType> , <http://sw.cyc.com/2006/07/27/cyc/SomeEmotionsAboutAttractionAndDislike-Emotion-Topic> ;
	<http://sw.cyc.com/2006/07/27/cyc/prettyString-Canonical> "disgust" ;
	<http://www.w3.org/2000/01/rdf-schema#subClassOf> <http://sw.cyc.com/2006/07/27/cyc/Dislike> .

<http://sw.cyc.com/2006/07/27/cyc/Dissatisfaction> <http://www.w3.org/2000/01/rdf-schema#comment> "Feeling of discontent, due to a lack of fulfillment of an agent's desires, needs, or requirements.  This is a collection; for an explanation of a typical #$FeelingType, see #$Happiness.   Some more specialized #$FeelingTypes than #$Dissatisfaction are #$Disappointment, #$Frustration, #$Impatience, #$Anger, etc. " ;
	a <http://sw.cyc.com/2006/07/27/cyc/EmotionalQuantityType> , <http://sw.cyc.com/2006/07/27/cyc/AtemporalNecessarilyEssentialCollectionType> , <http://sw.cyc.com/2006/07/27/cyc/SomeEmotionsAboutTheRealizationOfExpectations-Emotion-Topic> ;
	<http://sw.cyc.com/2006/07/27/cyc/prettyString-Canonical> "dissatisfaction" ;
	<http://www.w3.org/2000/01/rdf-schema#subClassOf> <http://sw.cyc.com/2006/07/27/cyc/FeelingAttribute> , <http://sw.cyc.com/2006/07/27/cyc/Unhappiness> .

<http://sw.cyc.com/2006/07/27/cyc/Hate> <http://www.w3.org/2000/01/rdf-schema#comment> "An intense feeling of hostility and aversion, usually deriving from fear, anger, or a sense of injury, and usually coupled with enmity and malice.  This is a #$Collection --- for an explanation of that, see #$Happiness." ;
	a <http://sw.cyc.com/2006/07/27/cyc/EmotionalQuantityType> , <http://sw.cyc.com/2006/07/27/cyc/AtemporalNecessarilyEssentialCollectionType> , <http://sw.cyc.com/2006/07/27/cyc/SomeEmotionsAboutAttractionAndDislike-Emotion-Topic> , <http://sw.cyc.com/2006/07/27/cyc/Emotion-Topic> ;
	<http://sw.cyc.com/2006/07/27/cyc/prettyString-Canonical> "hatred" ;
	<http://sw.cyc.com/2006/07/27/cyc/prettyString> "animosity" , "hate" ;
	<http://www.w3.org/2000/01/rdf-schema#subClassOf> <http://sw.cyc.com/2006/07/27/cyc/Dislike> , <http://sw.cyc.com/2006/07/27/cyc/Hostility> .

<http://sw.cyc.com/2006/07/27/cyc/EmotionalQuantityType> <http://www.w3.org/2000/01/rdf-schema#comment> "The collection of all specializations of #$EmotionalQuantity (currently named '#$FeelingAttribute')." ;
	a <http://sw.cyc.com/2006/07/27/cyc/AtemporalNecessarilyEssentialCollectionType> , <http://sw.cyc.com/2006/07/27/cyc/KEClarifyingCollectionType> , <http://sw.cyc.com/2006/07/27/cyc/FacetingCollectionType> , <http://sw.cyc.com/2006/07/27/cyc/SecondOrderCollection> , <http://sw.cyc.com/2006/07/27/cyc/TopLevelAffectCollections-Emotion-Topic> ;
	<http://sw.cyc.com/2006/07/27/cyc/prettyString-Canonical> "type of emotion" ;
	<http://sw.cyc.com/2006/07/27/cyc/prettyString> "kind of emotion" , "kinds of emotion" , "types of emotion" ;
	<http://www.w3.org/2000/01/rdf-schema#subClassOf> <http://sw.cyc.com/2006/07/27/cyc/PrimitiveOrderedQuantityType> .

<http://sw.cyc.com/2006/07/27/cyc/AbilityOfToTypeFn> a <http://sw.cyc.com/2006/07/27/cyc/BinaryFunction> , <http://sw.cyc.com/2006/07/27/cyc/IndividualDenotingFunction> ;
	<http://sw.cyc.com/2006/07/27/cyc/prettyString-Canonical> "Ability Of To Type Fn" ;
	<http://www.w3.org/2000/01/rdf-schema#domain> <http://sw.cyc.com/2006/07/27/cyc/Agent-Generic> ;
	<http://sw.cyc.com/2006/07/27/cyc/arity> "2"^^<http://www.w3.org/2001/XMLSchema#long> ;
	<http://www.w3.org/2000/01/rdf-schema#range> <http://www.w3.org/2002/07/owl#Class> ;
	<http://sw.cyc.com/2006/07/27/cyc/resultIsa> <http://sw.cyc.com/2006/07/27/cyc/AgentCapacityQuantity> ;
	<http://sw.cyc.com/2006/07/27/cyc/arg2Genl> <http://sw.cyc.com/2006/07/27/cyc/Event> .

<http://sw.cyc.com/2006/07/27/cyc/arg2Genl> <http://www.w3.org/2000/01/rdf-schema#comment> "A binary #$ArgGenlPredicate (q.v.).  <code>(#$arg2Genl RELN COL)</code>  means that semantic well-formedness requires that anything given as the second argument to <code>RELN</code> must be a subcollection of <code>COL</code>.  That is, <code>(RELN ARG1 ARG2</code> ...) is semantically well-formed only if <code>(#$genls ARG2 COL)</code> holds.  For an  explanation of semantic well-formedness, see #$CycLExpression-Assertible and its specializations.  See #$argGenl for a similar but more flexible ternary  predicate." ;
	a <http://sw.cyc.com/2006/07/27/cyc/DefaultMonotonicPredicate> , <http://sw.cyc.com/2006/07/27/cyc/IntangibleObjectRelatingPredicate> , <http://sw.cyc.com/2006/07/27/cyc/NonAbduciblePredicate> , <http://sw.cyc.com/2006/07/27/cyc/ArgumentGenl-Fundamental-Topic> , <http://sw.cyc.com/2006/07/27/cyc/ArgGenlBinaryPredicate> ;
	<http://sw.cyc.com/2006/07/27/cyc/prettyString-Canonical> "Arg 2 Genl" ;
	<http://sw.cyc.com/2006/07/27/cyc/quotedIsa> <http://sw.cyc.com/2006/07/27/cyc/OpenCycDefinitionalPredicate> ;
	<http://www.w3.org/2000/01/rdf-schema#domain> <http://sw.cyc.com/2006/07/27/cyc/Relation> ;
	<http://sw.cyc.com/2006/07/27/cyc/arity> "2"^^<http://www.w3.org/2001/XMLSchema#long> ;
	<http://sw.cyc.com/2006/07/27/cyc/sharedNotes> <http://sw.cyc.com/2006/07/27/cyc/ArgumentTypeChecking-FORTSvsNonReifiedNATS> ;
	<http://www.w3.org/2000/01/rdf-schema#range> <http://www.w3.org/2002/07/owl#Class> ;
	<http://www.w3.org/2000/01/rdf-schema#subPropertyOf> <http://sw.cyc.com/2006/07/27/cyc/relationExplicitlyInvokesTypeDerivatively-ArgGenl> ;
	<http://sw.cyc.com/2006/07/27/cyc/arg2Genl> <http://www.w3.org/2002/07/owl#Thing> ;
	<http://sw.cyc.com/2006/07/27/cyc/arg1Format> <http://sw.cyc.com/2006/07/27/cyc/SetTheFormat> ;
	<http://sw.cyc.com/2006/07/27/cyc/arg2Format> <http://sw.cyc.com/2006/07/27/cyc/SetTheFormat> ;
	<http://sw.cyc.com/2006/07/27/cyc/negationPreds> <http://sw.cyc.com/2006/07/27/cyc/arg2NotGenl> ;
	<http://sw.cyc.com/2006/07/27/cyc/oldConstantName> "argumentTwoGenls" ;
	<http://sw.cyc.com/2006/07/27/cyc/constrainsArg> "2"^^<http://www.w3.org/2001/XMLSchema#long> .

<http://sw.cyc.com/2006/07/27/cyc/Event> <http://www.w3.org/2000/01/rdf-schema#comment> """An important specialization of #$Situation and thus also of #$IntangibleIndividual and #$TemporallyExistingThing (qq.v).  Each instance of #$Event is a dynamic situation in which the state of the world changes; each instance is something one would say \"happens\".  Events are intangible because they are changes <i>per se</i>, not tangible objects that effect and undergo changes.
<p>
Notable specializations of #$Event include #$Event-Localized, #$PhysicalEvent, #$Action, and #$GeneralizedTransfer.
<p>
#$Events should not be confused with #$TimeIntervals (q.v.).  The temporal bounds of events are delineated by time intervals, but in contrast to many events time intervals have no spatial location or extent.""" ;
	a <http://sw.cyc.com/2006/07/27/cyc/FirstOrderCollection> , <http://sw.cyc.com/2006/07/27/cyc/TemporalStuffType> , <http://sw.cyc.com/2006/07/27/cyc/Time-Topic> , <http://sw.cyc.com/2006/07/27/cyc/TestOWLExportConcept> , <http://sw.cyc.com/2006/07/27/cyc/Top-Topic> , <http://sw.cyc.com/2006/07/27/cyc/ClarifyingCollectionType> , <http://sw.cyc.com/2006/07/27/cyc/ThingsWithTemporalExtent-Time-Topic> ;
	<http://sw.cyc.com/2006/07/27/cyc/prettyString-Canonical> "event" ;
	<http://sw.cyc.com/2006/07/27/cyc/prettyString> "occurrence" , "occurrences" , "occasion" , "occasions" , "incident" , "incidents" , "events" ;
	<http://www.w3.org/2000/01/rdf-schema#subClassOf> <http://sw.cyc.com/2006/07/27/cyc/Situation> , <http://sw.cyc.com/2006/07/27/cyc/Landmark-Underspecified> ;
	<http://sw.cyc.com/2006/07/27/cyc/quotedIsa> <http://sw.cyc.com/2006/07/27/cyc/WordNetWorkflowConstant-NotFullyReviewed> , <http://sw.cyc.com/2006/07/27/cyc/TerrorismOntologyConstant> ;
	<http://sw.cyc.com/2006/07/27/cyc/sharedNotes> <http://sw.cyc.com/2006/07/27/cyc/SharedNoteOnEventRepresentation> ;
	<http://www.w3.org/2002/07/owl#disjointWith> <http://sw.cyc.com/2006/07/27/cyc/AspatialInformationStore> , <http://sw.cyc.com/2006/07/27/cyc/Issue> , <http://sw.cyc.com/2006/07/27/cyc/CavityOrContainer> , <http://sw.cyc.com/2006/07/27/cyc/PositiveDimensionalThing> , <http://sw.cyc.com/2006/07/27/cyc/PostalCodeRegion> ;
	<http://sw.cyc.com/2006/07/27/cyc/requiredActorSlots> <http://sw.cyc.com/2006/07/27/cyc/actors> .

<http://sw.cyc.com/2006/07/27/cyc/BinaryFunction> <http://www.w3.org/2000/01/rdf-schema#comment> "A specialization of both #$BinaryRelation and #$Function-Denotational.  An instance of #$Function-Denotational FUNC is an instance of #$BinaryFunction if and only if FUNC has an #$arity of 2." ;
	a <http://www.w3.org/2002/07/owl#Class> , <http://sw.cyc.com/2006/07/27/cyc/AtemporalNecessarilyEssentialCollectionType> , <http://sw.cyc.com/2006/07/27/cyc/FixedArityFunctionTypeByArity> , <http://sw.cyc.com/2006/07/27/cyc/FunctionTypeByArity> ;
	<http://sw.cyc.com/2006/07/27/cyc/prettyString-Canonical> "binary function" ;
	<http://sw.cyc.com/2006/07/27/cyc/prettyString> "two-place function" , "two-place functions" , "binary functions" ;
	<http://www.w3.org/2000/01/rdf-schema#subClassOf> <http://sw.cyc.com/2006/07/27/cyc/Function-Denotational> , <http://sw.cyc.com/2006/07/27/cyc/BinaryRelation> , <http://sw.cyc.com/2006/07/27/cyc/FixedArityFunction> ;
	<http://sw.cyc.com/2006/07/27/cyc/collectionConventionMt> <http://sw.cyc.com/2006/07/27/cyc/UniversalVocabularyMt> .

<http://sw.cyc.com/2006/07/27/cyc/IndividualDenotingFunction> <http://www.w3.org/2000/01/rdf-schema#comment> """The subcollection of #$Function-Denotational whose instances, when applied to any appropriate
(sequence of) arguments, return instances of #$Individual.  Examples include #$PerimeterFn, #$GovernmentFn, and #$CavityInteriorRegionFn. See also the collections #$CollectionDenotingFunction and #$SetDenotingFunction.""" ;
	a <http://sw.cyc.com/2006/07/27/cyc/AtemporalNecessarilyEssentialCollectionType> , <http://sw.cyc.com/2006/07/27/cyc/FunctionTypeByRangeType> , <http://sw.cyc.com/2006/07/27/cyc/Functions-Fundamental-Topic> ;
	<http://sw.cyc.com/2006/07/27/cyc/prettyString-Canonical> "individual-denoting function" ;
	<http://sw.cyc.com/2006/07/27/cyc/prettyString> "individual-denoting functions" ;
	<http://www.w3.org/2000/01/rdf-schema#subClassOf> <http://sw.cyc.com/2006/07/27/cyc/Function-Denotational> .

<http://sw.cyc.com/2006/07/27/cyc/AbilityOfTypeToTypeFn> <http://www.w3.org/2000/01/rdf-schema#comment> "(#$AbilityOfTypeToTypeFn AGTTYPE TYPE) refers to the ability to engage in the spec of #$Event TYPE, that instances of AGTTYPE typically share.  For example, (#$AbilityOfTypeToTypeFn #$BasketballPlayer (#$PlayingFn #$Basketball-TheGame)) is the ability of basketball players have to play basketball." ;
	a <http://sw.cyc.com/2006/07/27/cyc/ReifiableFunction> , <http://sw.cyc.com/2006/07/27/cyc/BinaryFunction> , <http://sw.cyc.com/2006/07/27/cyc/IndividualDenotingFunction> ;
	<http://sw.cyc.com/2006/07/27/cyc/prettyString-Canonical> "Ability Of Type To Type Fn" ;
	<http://www.w3.org/2000/01/rdf-schema#domain> <http://www.w3.org/2002/07/owl#Class> ;
	<http://sw.cyc.com/2006/07/27/cyc/arity> "2"^^<http://www.w3.org/2001/XMLSchema#long> ;
	<http://www.w3.org/2000/01/rdf-schema#range> <http://www.w3.org/2002/07/owl#Class> ;
	<http://sw.cyc.com/2006/07/27/cyc/resultIsa> <http://sw.cyc.com/2006/07/27/cyc/AgentCapacityQuantity> .

<http://sw.cyc.com/2006/07/27/cyc/AbingtonBancorpInc> a <http://sw.cyc.com/2006/07/27/cyc/PubliclyHeldCorporation> ;
	<http://sw.cyc.com/2006/07/27/cyc/prettyString-Canonical> "Abington Bancorp Inc" .

<http://sw.cyc.com/2006/07/27/cyc/ABIOMEDInc> a <http://sw.cyc.com/2006/07/27/cyc/Individual> , <http://sw.cyc.com/2006/07/27/cyc/PubliclyHeldCorporation> ;
	<http://sw.cyc.com/2006/07/27/cyc/prettyString-Canonical> "ABIOMED" .

<http://sw.cyc.com/2006/07/27/cyc/Abitibi-Price-Corporation> a <http://sw.cyc.com/2006/07/27/cyc/Individual> ;
	<http://sw.cyc.com/2006/07/27/cyc/prettyString-Canonical> "Abitibi-Price" .

<http://sw.cyc.com/2006/07/27/cyc/Abkhazia-RegionGeorgia> a <http://sw.cyc.com/2006/07/27/cyc/Individual> , <http://sw.cyc.com/2006/07/27/cyc/State-Geopolitical> , <http://sw.cyc.com/2006/07/27/cyc/GeographicalThing> ;
	<http://sw.cyc.com/2006/07/27/cyc/prettyString-Canonical> "Abkhazia" .

<http://sw.cyc.com/2006/07/27/cyc/AbkhazLanguage> <http://www.w3.org/2000/01/rdf-schema#comment> "A language of the northern Caucasus group." ;
	a <http://sw.cyc.com/2006/07/27/cyc/Individual> , <http://sw.cyc.com/2006/07/27/cyc/NorthernCaucasianLanguageFamily> , <http://sw.cyc.com/2006/07/27/cyc/NaturalLanguage> , <http://sw.cyc.com/2006/07/27/cyc/LivingLanguage> , <http://sw.cyc.com/2006/07/27/cyc/LanguagesSpokenInCountries-HormuzArea-Topic> ;
	<http://sw.cyc.com/2006/07/27/cyc/prettyString-Canonical> "Abkhaz" ;
	<http://sw.cyc.com/2006/07/27/cyc/prettyString> "Abxazo" .

<http://sw.cyc.com/2006/07/27/cyc/NorthernCaucasianLanguageFamily> <http://www.w3.org/2000/01/rdf-schema#comment> "Languages of southeastern Russia, including that of the fabled Circassian maidens" ;
	a <http://sw.cyc.com/2006/07/27/cyc/LanguageFamilyType> ;
	<http://sw.cyc.com/2006/07/27/cyc/prettyString-Canonical> "the Northern Caucasian language family" ;
	<http://sw.cyc.com/2006/07/27/cyc/prettyString> "Northern Caucasian language" , "Northern Caucasian languages" ;
	<http://www.w3.org/2000/01/rdf-schema#subClassOf> <http://sw.cyc.com/2006/07/27/cyc/CaucasianLanguageFamily> .

<http://sw.cyc.com/2006/07/27/cyc/NaturalLanguage> <http://www.w3.org/2000/01/rdf-schema#comment> "A specialization of #$Language.  Each instance of #$NaturalLanguage is a language which is used for human communication, and which has evolved naturally. (It is disjoint with #$ConstructedLanguage.) Instances thus include dead languages such as Ancient Greek and Latin, but concocted languages such as Esperanto are not included." ;
	a <http://sw.cyc.com/2006/07/27/cyc/ObjectType> , <http://sw.cyc.com/2006/07/27/cyc/AtemporalNecessarilyEssentialCollectionType> , <http://sw.cyc.com/2006/07/27/cyc/KEClarifyingCollectionType> , <http://sw.cyc.com/2006/07/27/cyc/Linguistic-Topic> ;
	<http://sw.cyc.com/2006/07/27/cyc/prettyString-Canonical> "natural language" ;
	<http://sw.cyc.com/2006/07/27/cyc/prettyString> "natural languages" ;
	<http://www.w3.org/2000/01/rdf-schema#subClassOf> <http://sw.cyc.com/2006/07/27/cyc/HumanLanguage> ;
	<http://www.w3.org/2002/07/owl#disjointWith> <http://sw.cyc.com/2006/07/27/cyc/Artifact-Generic> .

<http://sw.cyc.com/2006/07/27/cyc/LivingLanguage> <http://www.w3.org/2000/01/rdf-schema#comment> "A specialization of #$NaturalLanguage.  An instance of #$NaturalLanguage is an instance of #$LivingLanguage just in case it has at least one extant native speaker." ;
	a <http://sw.cyc.com/2006/07/27/cyc/AtemporalNecessarilyEssentialCollectionType> , <http://sw.cyc.com/2006/07/27/cyc/Linguistic-Topic> , <http://sw.cyc.com/2006/07/27/cyc/LanguageGroupingType> ;
	<http://sw.cyc.com/2006/07/27/cyc/prettyString-Canonical> "living language" ;
	<http://sw.cyc.com/2006/07/27/cyc/prettyString> "living languages" ;
	<http://www.w3.org/2000/01/rdf-schema#subClassOf> <http://sw.cyc.com/2006/07/27/cyc/NaturalLanguage> ;
	<http://sw.cyc.com/2006/07/27/cyc/requiredArg2Pred> <http://sw.cyc.com/2006/07/27/cyc/nativeLanguage> .

<http://sw.cyc.com/2006/07/27/cyc/LanguagesSpokenInCountries-HormuzArea-Topic> a <http://sw.cyc.com/2006/07/27/cyc/KBDependentCollection> , <http://sw.cyc.com/2006/07/27/cyc/CycVocabularyTopic> ;
	<http://sw.cyc.com/2006/07/27/cyc/prettyString-Canonical> "languages spoken in countries hormuz area topic" ;
	<http://www.w3.org/2000/01/rdf-schema#subClassOf> <http://sw.cyc.com/2006/07/27/cyc/HormuzArea-Topic> .

<http://sw.cyc.com/2006/07/27/cyc/Ablation> <http://www.w3.org/2000/01/rdf-schema#comment> "A collection of events.  In an #$Ablation, a (usually relatively thin) layer of material is removed from the surface of an object." ;
	a <http://sw.cyc.com/2006/07/27/cyc/ChangeOfState-Topic> , <http://sw.cyc.com/2006/07/27/cyc/Transform-Topic> , <http://sw.cyc.com/2006/07/27/cyc/TemporalStuffType> .

<http://sw.cyc.com/2006/07/27/cyc/AbleMinded> <http://sw.cyc.com/2006/07/27/cyc/prettyString> "able-minded" , "more able-minded" , "most able-minded" ;
	<http://www.w3.org/2000/01/rdf-schema#subClassOf> <http://sw.cyc.com/2006/07/27/cyc/SentientAnimal> , <http://sw.cyc.com/2006/07/27/cyc/IntelligentAgent> .

<http://sw.cyc.com/2006/07/27/cyc/SentientAnimal> <http://www.w3.org/2000/01/rdf-schema#comment> "A subset of #$Animal, the collection of all animals which have a mind and are capable of conscious thought, or at least are best treated as such if you have to deal with them." ;
	a <http://sw.cyc.com/2006/07/27/cyc/ExistingObjectType> , <http://sw.cyc.com/2006/07/27/cyc/AnimalsByMiscellaneousCriteria-Biology-Topic> ;
	<http://sw.cyc.com/2006/07/27/cyc/prettyString-Canonical> "sentient animal" ;
	<http://sw.cyc.com/2006/07/27/cyc/prettyString> "sentient animals" ;
	<http://www.w3.org/2000/01/rdf-schema#subClassOf> <http://sw.cyc.com/2006/07/27/cyc/Animal> , <http://sw.cyc.com/2006/07/27/cyc/Sentient> ;
	<http://sw.cyc.com/2006/07/27/cyc/facets-Generic> <http://sw.cyc.com/2006/07/27/cyc/AnimalTypeByMentalState> .

<http://sw.cyc.com/2006/07/27/cyc/IntelligentAgent> <http://www.w3.org/2000/01/rdf-schema#comment> """A specialization of #$Agent-Generic and #$InformationStore (qq.v.).  An agent is an #$IntelligentAgent if and only if it is capable of knowing and acting, and capable of employing its knowledge in its actions.  An intelligent agent typically #$knowsAbout certain things, and its #$beliefs concerning those things influences its actions.  As with agents generally, an intelligent agent might either be a single individual, such as a person, or a group consisting of two or more individual agents, such as a business or government organization.  Specializations of #$IntelligentAgent include #$SocialBeing and #$MultiIndividualAgent-Intelligent.
<p>
Note that non-human #$Vertebrates that are sentient and somewhat intelligent, such as (arguably) cats and horses, can be considered intelligent agents in some contexts.""" ;
	a <http://sw.cyc.com/2006/07/27/cyc/ObjectType> , <http://sw.cyc.com/2006/07/27/cyc/TemporalStuffType> , <http://sw.cyc.com/2006/07/27/cyc/TestOWLExportConcept> , <http://sw.cyc.com/2006/07/27/cyc/Agents-Topic> ;
	<http://sw.cyc.com/2006/07/27/cyc/prettyString-Canonical> "intelligent agent" ;
	<http://sw.cyc.com/2006/07/27/cyc/prettyString> "intelligent agents" ;
	<http://www.w3.org/2000/01/rdf-schema#subClassOf> <http://sw.cyc.com/2006/07/27/cyc/Agent-Generic> , <http://sw.cyc.com/2006/07/27/cyc/InformationStore> ;
	<http://www.w3.org/2002/07/owl#disjointWith> <http://sw.cyc.com/2006/07/27/cyc/Statement> , <http://sw.cyc.com/2006/07/27/cyc/VisualPattern> , <http://sw.cyc.com/2006/07/27/cyc/Secretion-Bodily> , <http://sw.cyc.com/2006/07/27/cyc/VegetableMatter> , <http://sw.cyc.com/2006/07/27/cyc/EnergyStuff> ;
	<http://sw.cyc.com/2006/07/27/cyc/facets-Generic> <http://sw.cyc.com/2006/07/27/cyc/AgentTypeByEmotionalState> , <http://sw.cyc.com/2006/07/27/cyc/IntelligentAgentTypeByBeliefSystem> , <http://sw.cyc.com/2006/07/27/cyc/PersonTypeByMentalFeature> .

<http://sw.cyc.com/2006/07/27/cyc/AnimalTypeByMentalState> <http://www.w3.org/2000/01/rdf-schema#comment> "A collection of collections.  Each instance of #$AnimalTypeByMentalState is a subcollection of #$SentientAnimal whose instances share a mental state." ;
	a <http://sw.cyc.com/2006/07/27/cyc/FacetingCollectionType> , <http://sw.cyc.com/2006/07/27/cyc/SecondOrderCollection> ;
	<http://sw.cyc.com/2006/07/27/cyc/prettyString-Canonical> "mental state attribute" ;
	<http://www.w3.org/2000/01/rdf-schema#subClassOf> <http://sw.cyc.com/2006/07/27/cyc/FacetInstanceCollection> , <http://sw.cyc.com/2006/07/27/cyc/PersonTypeByMentalFeature> ;
	<http://sw.cyc.com/2006/07/27/cyc/sharedNotes> <http://sw.cyc.com/2006/07/27/cyc/SharedNoteOnGenlsRelationsBetweenFacetingCollectionTypes> ;
	<http://sw.cyc.com/2006/07/27/cyc/typeGenls> <http://sw.cyc.com/2006/07/27/cyc/SentientAnimal> .

<http://sw.cyc.com/2006/07/27/cyc/AbleTelcomHoldingCorp> a <http://sw.cyc.com/2006/07/27/cyc/Individual> , <http://sw.cyc.com/2006/07/27/cyc/PubliclyHeldCorporation> ;
	<http://sw.cyc.com/2006/07/27/cyc/prettyString-Canonical> "Able Telcom Holding Corp" .

<http://sw.cyc.com/2006/07/27/cyc/Able-TheSuffix> <http://www.w3.org/2000/01/rdf-schema#comment> """The suffix \"able\" (\"ible\") means something like *of the kind that
can be V-ed*. It converts (passive) #$Verbs to #$Adjectives. Example: (#$derivedUsingSuffix #$Breakable-TheWord #$Able-TheSuffix).""" ;
	a <http://sw.cyc.com/2006/07/27/cyc/Individual> , <http://sw.cyc.com/2006/07/27/cyc/LexicalSuffix> , <http://sw.cyc.com/2006/07/27/cyc/EnglishDerivationalSuffix> , <http://sw.cyc.com/2006/07/27/cyc/ProductiveLexicalAffix> , <http://sw.cyc.com/2006/07/27/cyc/DeverbalAdjectiveProducingSuffix> ;
	<http://sw.cyc.com/2006/07/27/cyc/prettyString-Canonical> "able suffix" ;
	<http://sw.cyc.com/2006/07/27/cyc/prettyString> "able suffixes" .

<http://sw.cyc.com/2006/07/27/cyc/Ably-TheSuffix> a <http://sw.cyc.com/2006/07/27/cyc/EnglishDerivationalSuffix> , <http://sw.cyc.com/2006/07/27/cyc/DeAdjectivalAdverbProducingSuffix> ;
	<http://sw.cyc.com/2006/07/27/cyc/prettyString-Canonical> "ibly suffix" ;
	<http://sw.cyc.com/2006/07/27/cyc/prettyString> "ably suffix" , "ably suffixes" , "ibly suffixes" ;
	<http://sw.cyc.com/2006/07/27/cyc/quotedIsa> <http://sw.cyc.com/2006/07/27/cyc/NLMorphologyTerm> .

<http://sw.cyc.com/2006/07/27/cyc/DeAdjectivalAdverbProducingSuffix> <http://www.w3.org/2000/01/rdf-schema#comment> "The collection of suffixes which serve to convert #$Adjectives into #$Adverbs. Example: #$Commendable-TheWord + #$Ably-TheSuffix = #$Commendably-TheWord." ;
	a <http://sw.cyc.com/2006/07/27/cyc/NLMorphologyCollection> , <http://sw.cyc.com/2006/07/27/cyc/SuffixCategory> , <http://sw.cyc.com/2006/07/27/cyc/LinguisticObjectType> ;
	<http://sw.cyc.com/2006/07/27/cyc/prettyString-Canonical> "de-adjectival adverb suffix" ;
	<http://sw.cyc.com/2006/07/27/cyc/prettyString> "de-adjectival adverb suffixes" ;
	<http://www.w3.org/2000/01/rdf-schema#subClassOf> <http://sw.cyc.com/2006/07/27/cyc/AdverbProducingSuffix> , <http://sw.cyc.com/2006/07/27/cyc/CategoryChangingAffix> , <http://sw.cyc.com/2006/07/27/cyc/DeAdjectivalSuffix> ;
	<http://sw.cyc.com/2006/07/27/cyc/quotedIsa> <http://sw.cyc.com/2006/07/27/cyc/NLTerm> , <http://sw.cyc.com/2006/07/27/cyc/NLMorphologyTerm> .

<http://sw.cyc.com/2006/07/27/cyc/ABMIndustriesIncorporated> a <http://sw.cyc.com/2006/07/27/cyc/Individual> , <http://sw.cyc.com/2006/07/27/cyc/PubliclyHeldCorporation> ;
	<http://sw.cyc.com/2006/07/27/cyc/prettyString-Canonical> "ABM Industries Incorporated" .

<http://sw.cyc.com/2006/07/27/cyc/ABNAMROHoldingNV> a <http://sw.cyc.com/2006/07/27/cyc/Individual> , <http://sw.cyc.com/2006/07/27/cyc/PubliclyHeldCorporation> ;
	<http://sw.cyc.com/2006/07/27/cyc/prettyString-Canonical> "ABNAMRO Holding NV" .

<http://sw.cyc.com/2006/07/27/cyc/abnormal> <http://www.w3.org/2000/01/rdf-schema#comment> """A binary #$MetaKnowledgePredicate that is used to state exceptions to a given general #$CycLAssertion.  Typically, an #$abnormal assertion will be the result of the #$CycCanonicalizer having \"transformed\" a sentence asserted at the EL level that was built from an #$ExceptionPredicate (i.e. #$exceptWhen or #$exceptFor).  While perhaps less common-sensically intuitive than #$exceptWhen or #$exceptFor, #$abnormal facilitates an efficient and uniform handling of exceptions.
<p>
Here, in more detail, is how #$abnormal is used.  Every default rule in our system, schematically:
<p>
P[X1 ... Xn] -> Q[X1 ... Xn]
<p>
(with X1, ..., Xn free in both P and Q) is implicitly treated as
<p>
(not (\"abnormal-for-this-rule\" X1 ... Xn)) & (P[X1 ... Xn] -> Q[X1 ... Xn]) .
<p>
Thus rules without exceptions need never incur the overhead of default reasoning.  Since a different \"abnormality\" relation would otherwise be needed for every default rule in the system, we use instead a single predicate -- #$abnormal -- which takes the rule in question as an argument.  And the other argument to #$abnormal is a #$List of variables (or of a single closed term) over which abnormality is computed; this allows #$abnormal to be binary rather than variable-arity.  Hence a sentence of the form
<p>
(#$exceptWhen EXCEPTION RULE) ,
<p>
in which each of the variables X1, ..., Xn occurs free in both EXCEPTION and RULE, gets canonicalized to an #$implies rule that concludes to an #$abnormal sentence:
<p>
<pre>
(#$implies
  EXCEPTION
  (#$abnormal (#$TheList X1 .... Xn) RULE)) .
</pre>
<p>
And a sentence of the form
<p>
(#$exceptFor TERM RULE) ,
<p>
in which exactly one variable X occurs free in RULE, gets canonicalized to a sentence of the form
<p>
(#$abnormal (#$TheList TERM) RULE) .
<p>
See also #$pragmaticallyNormal.""" ;
	a <http://www.w3.org/2000/01/rdf-schema#Property> , <http://sw.cyc.com/2006/07/27/cyc/DefaultReasoning-Fundamental-Topic> , <http://sw.cyc.com/2006/07/27/cyc/DefaultMonotonicPredicate> , <http://sw.cyc.com/2006/07/27/cyc/MetaKnowledgePredicate> ;
	<http://sw.cyc.com/2006/07/27/cyc/prettyString-Canonical> "abnormal" ;
	<http://www.w3.org/2000/01/rdf-schema#domain> <http://sw.cyc.com/2006/07/27/cyc/List> ;
	<http://sw.cyc.com/2006/07/27/cyc/arity> "2"^^<http://www.w3.org/2001/XMLSchema#long> ;
	<http://sw.cyc.com/2006/07/27/cyc/sharedNotes> <http://sw.cyc.com/2006/07/27/cyc/MetaAssertionsForPolycanonicalizingAssertions> , <http://sw.cyc.com/2006/07/27/cyc/NoteOnExceptionsAndOldConclusions> , <http://sw.cyc.com/2006/07/27/cyc/NoteAboutExceptionCheckingDuringInference> ;
	<http://sw.cyc.com/2006/07/27/cyc/arg2QuotedIsa> <http://sw.cyc.com/2006/07/27/cyc/CycLAssertion> ;
	<http://sw.cyc.com/2006/07/27/cyc/quotedArgument> "2"^^<http://www.w3.org/2001/XMLSchema#long> ;
	<http://www.w3.org/2000/01/rdf-schema#seeAlso> <http://sw.cyc.com/2006/07/27/cyc/pragmaticallyNormal> , <http://sw.cyc.com/2006/07/27/cyc/meetsPragmaticRequirement> .

<http://sw.cyc.com/2006/07/27/cyc/List> <http://www.w3.org/2000/01/rdf-schema#comment> "A specialization of #$Tuple.  Each instance of #$List is a  finite sequence of things with a first and last member-position, with each member-position other than the last having a successor member-position.   As with tuples generally, lists allow for repetition of their members, so that the same item can appear at multiple member-positions in the same list.  A list can be represented formally as a function from a finite index set of counting numbers, beginning with one, into the domain of all #$Things (but note that #$Lists are _not_ explicitly represented as functions in the Cyc ontology).  Unlike an instance of #$Series (q.v.), a list is purely abstract (i.e. both aspatial and atemporal), and the only implied relation between an item and its successor in a list is the successor relation of the list itself.  Technically, #$List is more specific than #$Tuple only in that the index set (see #$tupleIndexSet) for a given list must be the counting numbers in their usual order (or some initial segment thereof), whereas the index set for a tuple, generally speaking, might be any set whatsoever." ;
	a <http://www.w3.org/2002/07/owl#Class> , <http://sw.cyc.com/2006/07/27/cyc/AtemporalNecessarilyEssentialCollectionType> , <http://sw.cyc.com/2006/07/27/cyc/StuffType> , <http://sw.cyc.com/2006/07/27/cyc/Group-Topic> ;
	<http://sw.cyc.com/2006/07/27/cyc/prettyString-Canonical> "List" ;
	<http://sw.cyc.com/2006/07/27/cyc/prettyString> "lists" , "list of things" ;
	<http://www.w3.org/2000/01/rdf-schema#subClassOf> <http://sw.cyc.com/2006/07/27/cyc/List> , <http://sw.cyc.com/2006/07/27/cyc/Tuple> ;
	<http://sw.cyc.com/2006/07/27/cyc/oldConstantName> "List" ;
	<http://sw.cyc.com/2006/07/27/cyc/collectionConventionMt> <http://sw.cyc.com/2006/07/27/cyc/UniversalVocabularyMt> ;
	<http://www.w3.org/2002/07/owl#equivalentClass> <http://sw.cyc.com/2006/07/27/cyc/List> .

<http://sw.cyc.com/2006/07/27/cyc/CycLAssertion> <http://www.w3.org/2000/01/rdf-schema#comment> "The collection of semantically well-formed #$CycLSentences asserted to the Cyc Knowledge Base.  Each instance of #$CycLAssertion is either (1) an HL assertion, i.e. a CycL sentence that corresponds to a data structure actually in the Cyc KB), or (2) an EL assertion : an Epistemological Level CycL sentence that can be canonicalized into one or more already extant HL assertions.  #$CycLAssertion is used as a quoted argument type constraint for certain meta-predicates, such as #$overrides." ;
	a <http://www.w3.org/2002/07/owl#Class> , <http://sw.cyc.com/2006/07/27/cyc/CycLExpressionType> , <http://sw.cyc.com/2006/07/27/cyc/AtemporalNecessarilyEssentialCollectionType> , <http://sw.cyc.com/2006/07/27/cyc/PragmaticallyDecontextualizedCollection> , <http://sw.cyc.com/2006/07/27/cyc/SubsetsOfComputationalObject-Math-Topic> ;
	<http://sw.cyc.com/2006/07/27/cyc/prettyString-Canonical> "CycL assertion" ;
	<http://sw.cyc.com/2006/07/27/cyc/prettyString> "Assertion" , "Cyc assertion" , "Cyc assertions" .

<http://sw.cyc.com/2006/07/27/cyc/Abnormal-Unusual> <http://sw.cyc.com/2006/07/27/cyc/prettyString> "atypical" , "more atypical" , "most atypical" ;
	<http://www.w3.org/2000/01/rdf-schema#subClassOf> <http://sw.cyc.com/2006/07/27/cyc/TemporalThing> .

<http://sw.cyc.com/2006/07/27/cyc/ThingByNormalityInContext> <http://www.w3.org/2000/01/rdf-schema#comment> "The collection of types of things by their normality in some (normally) highly restrained context.  The context need not be reified, but merely implied by the predicate (#$normalityOfThing or #$normalityForAgent) used for attributing such a normality to the thing.  Normality is (at least currently) a squishily-defined concept, and it is certainly dependent on the observer and context about which the assertion is made.  Normality is different from but related to frequency (e.g. #$frequencyOfActionType, #$Frequency). For example, I might see my pet exotic fish every day, but the fish still is #$Exotic-Unusual in Austin, although it may not be on a Belizian reef.  To make assertions involving normality, use #$normalityOfThing or #$normalityForAgent." ;
	a <http://sw.cyc.com/2006/07/27/cyc/CollectionType> ;
	<http://sw.cyc.com/2006/07/27/cyc/prettyString-Canonical> "thing by normality in context" ;
	<http://www.w3.org/2000/01/rdf-schema#subClassOf> <http://www.w3.org/2002/07/owl#Class> .

<http://sw.cyc.com/2006/07/27/cyc/aboardTransporter> <http://www.w3.org/2000/01/rdf-schema#comment> "(#$aboardTransporter THING TRANSPORT) says that the #$PartiallyTangible object THING is aboard the #$TransportationDevice TRANSPORT, which means that THING will move wherever TRANSPORT moves.  This predicate covers a wide range of physical relations to transporters, such as a pilot in an airplane, a dog in the bed of a pickup truck, and a torpedo in a submarine." ;
	a <http://www.w3.org/2002/07/owl#TransitiveProperty> , <http://sw.cyc.com/2006/07/27/cyc/CoexistingObjectsPredicate> , <http://sw.cyc.com/2006/07/27/cyc/AsymmetricBinaryPredicate> ;
	<http://sw.cyc.com/2006/07/27/cyc/prettyString-Canonical> "Aboard Transporter" ;
	<http://www.w3.org/2000/01/rdf-schema#domain> <http://sw.cyc.com/2006/07/27/cyc/PartiallyTangible> ;
	<http://sw.cyc.com/2006/07/27/cyc/arity> "2"^^<http://www.w3.org/2001/XMLSchema#long> ;
	<http://www.w3.org/2000/01/rdf-schema#range> <http://sw.cyc.com/2006/07/27/cyc/TransportationDevice> ;
	<http://www.w3.org/2000/01/rdf-schema#subPropertyOf> <http://sw.cyc.com/2006/07/27/cyc/movesWith> , <http://sw.cyc.com/2006/07/27/cyc/objectFoundInLocation> ;
	<http://sw.cyc.com/2006/07/27/cyc/negationInverse> <http://sw.cyc.com/2006/07/27/cyc/aboardTransporter> .

<http://sw.cyc.com/2006/07/27/cyc/TransportationDevice> <http://www.w3.org/2000/01/rdf-schema#comment> "A specialization of both #$Conveyance and #$PhysicalDevice.  Each instance of #$TransportationDevice is an artifact designed to move an object from one location to another, by (for example) carrying, pulling, or pushing the transported object.  Instances of this collection may or may not have their own power source (see #$SelfPoweredDevice).  Those that do, such as automobiles and speedboats, constitute the specialization #$TransportationDevice-Vehicle.  Other transportation devices (for example, instances of #$Wheelbarrow or #$Bicycle) require an external motive force.  Because #$transporter and #$transportees are specializations of #$objectMoving, it follows that any object in the role of #$transporter moves as a whole with those objects playing the role of #$transportees.  Consequently, since any instance of #$TransportationDevice has playing the role of #$transporter as its intended function, stationary objects which cause motion, such as conveyor belts, escalators, rocket launchers, and slingshots, are excluded from the collection #$TransportationDevice. Although they facilitate travel, ice skates, shoes, skis and other instances of #$WearableConveyance are also excluded from the collection #$TransportationDevice, since they are devices which are worn rather than ridden on, ridden with, or ridden in." ;
	a <http://sw.cyc.com/2006/07/27/cyc/ExistingObjectType> , <http://sw.cyc.com/2006/07/27/cyc/SpatiallyDisjointObjectType> , <http://sw.cyc.com/2006/07/27/cyc/FirstOrderCollection> , <http://sw.cyc.com/2006/07/27/cyc/ArtifactTypeByFunction> , <http://sw.cyc.com/2006/07/27/cyc/CDETagTranslationConstant> , <http://sw.cyc.com/2006/07/27/cyc/SaffronSituationTypeConstant> , <http://sw.cyc.com/2006/07/27/cyc/SpecializationsOfPhysicalDevice-Device-Topic> , <http://sw.cyc.com/2006/07/27/cyc/Transportation-Topic> ;
	<http://sw.cyc.com/2006/07/27/cyc/prettyString-Canonical> "transportation device" ;
	<http://sw.cyc.com/2006/07/27/cyc/prettyString> "transportation devices" ;
	<http://www.w3.org/2000/01/rdf-schema#subClassOf> <http://sw.cyc.com/2006/07/27/cyc/Artifact-NonAgentive> , <http://sw.cyc.com/2006/07/27/cyc/PhysicalDevice> , <http://sw.cyc.com/2006/07/27/cyc/Conveyance> ;
	<http://sw.cyc.com/2006/07/27/cyc/quotedIsa> <http://sw.cyc.com/2006/07/27/cyc/TerrorismOntologyConstant> ;
	<http://www.w3.org/2002/07/owl#disjointWith> <http://sw.cyc.com/2006/07/27/cyc/GeographicalThing> , <http://sw.cyc.com/2006/07/27/cyc/NaturalTangibleStuff> , <http://sw.cyc.com/2006/07/27/cyc/SmallArm-Weapon> , <http://sw.cyc.com/2006/07/27/cyc/PathArtifactSystem> , <http://sw.cyc.com/2006/07/27/cyc/NavigationDevice> , <http://sw.cyc.com/2006/07/27/cyc/AlarmDevice> , <http://sw.cyc.com/2006/07/27/cyc/InformationRecordingDevice> , <http://sw.cyc.com/2006/07/27/cyc/StationeryProduct> , <http://sw.cyc.com/2006/07/27/cyc/Clothing-Generic> , <http://sw.cyc.com/2006/07/27/cyc/NonPoweredDevice> , <http://sw.cyc.com/2006/07/27/cyc/Decoration> , <http://sw.cyc.com/2006/07/27/cyc/ComputationalSystem> , <http://sw.cyc.com/2006/07/27/cyc/RecordingOfWaveIBT> , <http://sw.cyc.com/2006/07/27/cyc/TextualMaterial> , <http://sw.cyc.com/2006/07/27/cyc/Wire> , <http://sw.cyc.com/2006/07/27/cyc/PlumbingFixture> , <http://sw.cyc.com/2006/07/27/cyc/ControlDevice> , <http://sw.cyc.com/2006/07/27/cyc/MeasuringDevice> , <http://sw.cyc.com/2006/07/27/cyc/TravelAccessory> .

<http://sw.cyc.com/2006/07/27/cyc/movesWith> <http://www.w3.org/2000/01/rdf-schema#comment> "<code>(#$movesWith MOVED MOVER)</code> means that if <code>MOVER</code> undergoes translation (see #$Movement-TranslationEvent) then <code>MOVED</code> by default also undergoes a translation in the same direction and same speed.  However, this default is defeated if <code>MOVED</code> is undergoing motion relative to <code>MOVER</code>. For example, a person would #$movesWith the Titanic if they were #$on-Physical it.  However, if <code>MOVED</code> is moving relative to <code>MOVER</code>, then its 'absolute' motion is computed by subtracting its motion relative to <code>MOVER</code> from the 'absolute' motion vector of <code>MOVER</code>." ;
	a <http://sw.cyc.com/2006/07/27/cyc/CoexistingObjectsPredicate> , <http://www.w3.org/2002/07/owl#SymmetricProperty> , <http://sw.cyc.com/2006/07/27/cyc/ReflexiveBinaryPredicate> ;
	<http://sw.cyc.com/2006/07/27/cyc/prettyString-Canonical> "Moves With" ;
	<http://www.w3.org/2000/01/rdf-schema#domain> <http://sw.cyc.com/2006/07/27/cyc/SpatialThing-Localized> ;
	<http://sw.cyc.com/2006/07/27/cyc/arity> "2"^^<http://www.w3.org/2001/XMLSchema#long> ;
	<http://www.w3.org/2000/01/rdf-schema#range> <http://sw.cyc.com/2006/07/27/cyc/SpatialThing-Localized> ;
	<http://www.w3.org/2000/01/rdf-schema#subPropertyOf> <http://sw.cyc.com/2006/07/27/cyc/temporallyCoexist> , <http://sw.cyc.com/2006/07/27/cyc/near> ;
	<http://sw.cyc.com/2006/07/27/cyc/arg1Format> <http://sw.cyc.com/2006/07/27/cyc/SetTheFormat> ;
	<http://sw.cyc.com/2006/07/27/cyc/arg2Format> <http://sw.cyc.com/2006/07/27/cyc/SetTheFormat> .

<http://sw.cyc.com/2006/07/27/cyc/objectFoundInLocation> <http://www.w3.org/2000/01/rdf-schema#comment> "A #$CoexistingObjectsPredicate and specialization of #$inRegion (q.v.).  <code>(#$objectFoundInLocation OBJ LOC)</code> means that <code>OBJ</code> has the location <code>LOC</code>.  <code>OBJ</code> might or might not be a physical part (see #$physicalDecompositions) of <code>LOC</code>, but <code>LOC</code> must <i>not</i> be a part of <code>OBJ</code>.  For example, <code>(#$objectFoundInLocation #$PietaStatue-Michelangelo #$StPetersBasilica)</code> is true." ;
	a <http://www.w3.org/2002/07/owl#TransitiveProperty> , <http://sw.cyc.com/2006/07/27/cyc/CoexistingObjectsPredicate> , <http://www.w3.org/2002/07/owl#SymmetricProperty> , <http://sw.cyc.com/2006/07/27/cyc/AntiSymmetricBinaryPredicate> , <http://sw.cyc.com/2006/07/27/cyc/IrreflexiveBinaryPredicate> , <http://sw.cyc.com/2006/07/27/cyc/RelativeLocationalPredicate> , <http://sw.cyc.com/2006/07/27/cyc/ClimateConcept> , <http://sw.cyc.com/2006/07/27/cyc/RelationalNounSlot> , <http://sw.cyc.com/2006/07/27/cyc/ProximityAndLocation-Spatial-Topic> , <http://sw.cyc.com/2006/07/27/cyc/BBNRelationTypePredicate> ;
	<http://sw.cyc.com/2006/07/27/cyc/prettyString-Canonical> "location" ;
	<http://sw.cyc.com/2006/07/27/cyc/prettyString> "locations" , "site" , "sites" , "whereabouts" ;
	<http://www.w3.org/2000/01/rdf-schema#domain> <http://sw.cyc.com/2006/07/27/cyc/SpatialThing-Localized> , <http://sw.cyc.com/2006/07/27/cyc/SpatialThing-NonSituational> ;
	<http://sw.cyc.com/2006/07/27/cyc/arity> "2"^^<http://www.w3.org/2001/XMLSchema#long> ;
	<http://www.w3.org/2000/01/rdf-schema#range> <http://sw.cyc.com/2006/07/27/cyc/SpatialThing-Localized> , <http://sw.cyc.com/2006/07/27/cyc/SpatialThing-NonSituational> ;
	<http://www.w3.org/2000/01/rdf-schema#subPropertyOf> <http://sw.cyc.com/2006/07/27/cyc/temporallyCoexist> .

<http://sw.cyc.com/2006/07/27/cyc/Abortion-Intentional> <http://sw.cyc.com/2006/07/27/cyc/prettyString> "aborting" , "have aborted" , "has aborted" , "will abort" , "had aborted" , "will have aborted" , "abortions" ;
	<http://www.w3.org/2000/01/rdf-schema#subClassOf> <http://sw.cyc.com/2006/07/27/cyc/PregnancyEndingEvent> , <http://sw.cyc.com/2006/07/27/cyc/IntelligentAgentActivity> , <http://sw.cyc.com/2006/07/27/cyc/BiologicalDestructionEvent> , <http://sw.cyc.com/2006/07/27/cyc/MedicalTreatmentEvent> .

<http://sw.cyc.com/2006/07/27/cyc/PregnancyEndingEvent> <http://www.w3.org/2000/01/rdf-schema#comment> "A specialization of #$IntrinsicStateChangeEvent and #$AnimalActivity. Each instance of this collection is an event which terminates a #$Pregnancy. Notable specializations of this collection include birth (cf. #$BirthEvent), abortion (cf. #$Abortion-Intentional), and #$Miscarriage." ;
	a <http://sw.cyc.com/2006/07/27/cyc/TemporalObjectType> , <http://sw.cyc.com/2006/07/27/cyc/QAClarifyingCollectionType> , <http://sw.cyc.com/2006/07/27/cyc/BiologicalEvents-Biology-Topic> ;
	<http://sw.cyc.com/2006/07/27/cyc/prettyString-Canonical> "pregnancy ending event" ;
	<http://sw.cyc.com/2006/07/27/cyc/prettyString> "end a pregnancy" , "ended a pregnancy" , "ends a pregnancy" , "ending a pregnancy" , "have ended a pregnancy" , "has ended a pregnancy" , "will end a pregnancy" , "had ended a pregnancy" , "will have ended a pregnancy" , "pregnancy ending events" ;
	<http://www.w3.org/2000/01/rdf-schema#subClassOf> <http://sw.cyc.com/2006/07/27/cyc/IntrinsicStateChangeEvent> , <http://sw.cyc.com/2006/07/27/cyc/AnimalActivity> .

<http://sw.cyc.com/2006/07/27/cyc/IntelligentAgentActivity> <http://www.w3.org/2000/01/rdf-schema#comment> "A specialization of #$Action (q.v.).  Every instance of #$IntelligentAgentActivity is an action, each of whose \"doers\" (see #$doneBy and #$animateDoers) is either an #$IntelligentAgent or a group of such agents (i.e. a #$Group all of whose members are intelligent agents).  Specializations of this collection include #$HumanActivity and #$Reading." ;
	a <http://sw.cyc.com/2006/07/27/cyc/TemporalStuffType> ;
	<http://sw.cyc.com/2006/07/27/cyc/prettyString-Canonical> "intelligent agent activity" ;
	<http://sw.cyc.com/2006/07/27/cyc/prettyString> "intelligent agent activities" ;
	<http://www.w3.org/2000/01/rdf-schema#subClassOf> <http://sw.cyc.com/2006/07/27/cyc/Action> .

<http://sw.cyc.com/2006/07/27/cyc/BiologicalDestructionEvent> <http://www.w3.org/2000/01/rdf-schema#comment> "A specialization of both #$PhysicalDestructionEvent and #$BiologicalProcess.  In each instance  of #$BiologicalDestructionEvent, some instance(s) of  #$BiologicalLivingObject (q.v.) are destroyed.  Notable  specializations of #$BiologicalDestructionEvent include #$BiologicalCatabolismEvent, #$DigestionEvent, and #$BiologicalDecompositionEvent." ;
	a <http://sw.cyc.com/2006/07/27/cyc/Transform-Topic> , <http://sw.cyc.com/2006/07/27/cyc/TemporalStuffType> , <http://sw.cyc.com/2006/07/27/cyc/BiologicalEvents-Biology-Topic> , <http://sw.cyc.com/2006/07/27/cyc/Biology-Topic> ;
	<http://sw.cyc.com/2006/07/27/cyc/prettyString-Canonical> "biological destruction" ;
	<http://www.w3.org/2000/01/rdf-schema#subClassOf> <http://sw.cyc.com/2006/07/27/cyc/PhysicalDestructionEvent> , <http://sw.cyc.com/2006/07/27/cyc/BiologicalProcess> ;
	<http://www.w3.org/2002/07/owl#disjointWith> <http://sw.cyc.com/2006/07/27/cyc/TakingCareOfPeople> .

<http://sw.cyc.com/2006/07/27/cyc/MedicalTreatmentEvent> <http://www.w3.org/2000/01/rdf-schema#comment> "A subcollection of #$MedicalCareEvent.  Each instance of #$MedicalTreatmentEvent is a procedure performed by one or more medical professionals to alleviate or ameliorate a #$PhysiologicalCondition (q.v.)." ;
	a <http://sw.cyc.com/2006/07/27/cyc/FirstOrderCollection> , <http://sw.cyc.com/2006/07/27/cyc/ChangeOfState-Topic> , <http://sw.cyc.com/2006/07/27/cyc/KEClarifyingCollectionType> , <http://sw.cyc.com/2006/07/27/cyc/MedicalCareEvents-GeneralMedicine-Topic> , <http://sw.cyc.com/2006/07/27/cyc/Medicine-Other-Topic> ;
	<http://sw.cyc.com/2006/07/27/cyc/prettyString-Canonical> "medical treatment" ;
	<http://sw.cyc.com/2006/07/27/cyc/prettyString> "treatment" , "health care" , "treated" , "treating" , "have treated" , "has treated" , "will treat" , "had treated" , "will have treated" , "procedure" , "procedures" , "therapy" , "treatments" , "medical" , "medical treatments" , "treat" , "treats" ;
	<http://www.w3.org/2000/01/rdf-schema#subClassOf> <http://sw.cyc.com/2006/07/27/cyc/ServiceEvent> , <http://sw.cyc.com/2006/07/27/cyc/MedicalCareEvent> .

<http://sw.cyc.com/2006/07/27/cyc/above-Directly> a <http://www.w3.org/2002/07/owl#TransitiveProperty> , <http://sw.cyc.com/2006/07/27/cyc/CoexistingObjectsPredicate> , <http://sw.cyc.com/2006/07/27/cyc/AsymmetricBinaryPredicate> , <http://sw.cyc.com/2006/07/27/cyc/RelativeLocationalPredicate> , <http://sw.cyc.com/2006/07/27/cyc/RelativePositionsOfObjects-Spatial-Topic> ;
	<http://sw.cyc.com/2006/07/27/cyc/prettyString-Canonical> "Above-Directly" ;
	<http://www.w3.org/2000/01/rdf-schema#domain> <http://sw.cyc.com/2006/07/27/cyc/SpatialThing-Localized> ;
	<http://sw.cyc.com/2006/07/27/cyc/arity> "2"^^<http://www.w3.org/2001/XMLSchema#long> ;
	<http://www.w3.org/2000/01/rdf-schema#range> <http://sw.cyc.com/2006/07/27/cyc/SpatialThing-Localized> ;
	<http://www.w3.org/2000/01/rdf-schema#subPropertyOf> <http://sw.cyc.com/2006/07/27/cyc/above-Generally> ;
	<http://sw.cyc.com/2006/07/27/cyc/arg1Format> <http://sw.cyc.com/2006/07/27/cyc/SetTheFormat> ;
	<http://sw.cyc.com/2006/07/27/cyc/arg2Format> <http://sw.cyc.com/2006/07/27/cyc/SetTheFormat> ;
	<http://sw.cyc.com/2006/07/27/cyc/negationInverse> <http://sw.cyc.com/2006/07/27/cyc/above-Directly> .

<http://sw.cyc.com/2006/07/27/cyc/above-Generally> <http://www.w3.org/2000/01/rdf-schema#comment> "(#$above-Generally OBJ1 OBJ2) means that the #$SpatialThing-Localized OBJ1 is more or less above the #$SpatialThing-Localized OBJ2. To be more precise: if OBJ1 is within a cone-shaped set of vectors within about 45 degrees of #$Up-Directly pointing up from OBJ2 (see #$Up-Generally), then (#$above-Generally OBJ1 OBJ2) holds. This is a more general predicate than #$above-Directly (q.v.), but it is a more specialized predicate than #$above-Higher (q.v.). It probably most closely conforms to the English word \"above.\"" ;
	a <http://www.w3.org/2002/07/owl#TransitiveProperty> , <http://sw.cyc.com/2006/07/27/cyc/CoexistingObjectsPredicate> , <http://sw.cyc.com/2006/07/27/cyc/AsymmetricBinaryPredicate> , <http://sw.cyc.com/2006/07/27/cyc/RelativeLocationalPredicate> , <http://sw.cyc.com/2006/07/27/cyc/RelativePositionsOfObjects-Spatial-Topic> ;
	<http://sw.cyc.com/2006/07/27/cyc/prettyString-Canonical> "above" ;
	<http://www.w3.org/2000/01/rdf-schema#domain> <http://sw.cyc.com/2006/07/27/cyc/SpatialThing-Localized> ;
	<http://sw.cyc.com/2006/07/27/cyc/arity> "2"^^<http://www.w3.org/2001/XMLSchema#long> ;
	<http://sw.cyc.com/2006/07/27/cyc/sharedNotes> <http://sw.cyc.com/2006/07/27/cyc/NoteOnCycMergedOntologyConstants> ;
	<http://www.w3.org/2000/01/rdf-schema#range> <http://sw.cyc.com/2006/07/27/cyc/SpatialThing-Localized> ;
	<http://www.w3.org/2000/01/rdf-schema#subPropertyOf> <http://sw.cyc.com/2006/07/27/cyc/above-Higher> , <http://sw.cyc.com/2006/07/27/cyc/over-UnderspecifiedLocation> ;
	<http://sw.cyc.com/2006/07/27/cyc/arg1Format> <http://sw.cyc.com/2006/07/27/cyc/openEntryFormatInArgs> ;
	<http://sw.cyc.com/2006/07/27/cyc/arg2Format> <http://sw.cyc.com/2006/07/27/cyc/openEntryFormatInArgs> ;
	<http://sw.cyc.com/2006/07/27/cyc/negationInverse> <http://sw.cyc.com/2006/07/27/cyc/above-Generally> ;
	<http://sw.cyc.com/2006/07/27/cyc/negationPreds> <http://sw.cyc.com/2006/07/27/cyc/under-UnderspecifiedLocation> .

<http://sw.cyc.com/2006/07/27/cyc/RelativeLocationalPredicate> <http://www.w3.org/2000/01/rdf-schema#comment> """A specialization of #$LocationalPredicate (q.v.).  Each instance of #$RelativeLocationalPredicate relates two (or, occasionally, more) spatial things in terms of their relative locations with respect to one another, and does so in a way that does not simply amount to relating a spatial thing to a space region in which it is embedded.  (Cf. #$AbsoluteLocationalPredicate.)  
<p>
Many relative-location predicates can take any #$SpatialThings (or at least any instances of #$SpatialThing-Localized) as arguments.  For example, #$touches-Directly holds of any two spatial things that either spatially intersect or are in direct spatial contact.  Other relative-location predicates have one or more of their argument-places restricted to tangible things of some sort (see #$PartiallyTangible); e.g. #$pathThroughRegion and #$abutsSurface.  Still others (the so-called #$SpaceRegionPredicates) only relate #$SpaceRegions to each other; e.g. #$overlappingSpaceRegions and #$properPartOfSpaceRegion.""" ;
	a <http://sw.cyc.com/2006/07/27/cyc/KEClarifyingCollectionType> , <http://sw.cyc.com/2006/07/27/cyc/PredicateType> ;
	<http://sw.cyc.com/2006/07/27/cyc/prettyString-Canonical> "relative locational predicate" ;
	<http://www.w3.org/2000/01/rdf-schema#subClassOf> <http://sw.cyc.com/2006/07/27/cyc/LocationalPredicate> .

<http://sw.cyc.com/2006/07/27/cyc/RelativePositionsOfObjects-Spatial-Topic> a <http://sw.cyc.com/2006/07/27/cyc/KBDependentCollection> , <http://sw.cyc.com/2006/07/27/cyc/CycVocabularyTopic> ;
	<http://sw.cyc.com/2006/07/27/cyc/prettyString-Canonical> "relative positions of objects spatial topic" ;
	<http://www.w3.org/2000/01/rdf-schema#subClassOf> <http://sw.cyc.com/2006/07/27/cyc/Spatial-Topic> .

<http://sw.cyc.com/2006/07/27/cyc/AboveFreezingOnEarth> <http://www.w3.org/2000/01/rdf-schema#comment> "#$AboveFreezingOnEarth is a generic temperature quantity that includes the range of naturally occurring above-freezing temperatures on the surface of the #$PlanetEarth.  Approx. 32 to 130 degrees Fahrenheit." ;
	a <http://sw.cyc.com/2006/07/27/cyc/NonNumericScalarQuantity> , <http://sw.cyc.com/2006/07/27/cyc/ClimateConcept> , <http://sw.cyc.com/2006/07/27/cyc/GenericQuantity> , <http://sw.cyc.com/2006/07/27/cyc/Temperature> ;
	<http://sw.cyc.com/2006/07/27/cyc/prettyString-Canonical> "above freezing" ;
	<http://sw.cyc.com/2006/07/27/cyc/prettyString> "more above freezing" , "most above freezing" .

<http://sw.cyc.com/2006/07/27/cyc/ClimateConcept> <http://www.w3.org/2000/01/rdf-schema#comment> "A #$ConceptTypeByDomain (q.v.).  Instances of #$ClimateConcept are collections and relations having to do with climate.  Specializations of #$AnnualClimateCycle, those specializations of #$GeographicalRegion that are closely associated with particular climates, and relations used for describing the locations, meteorological features, inhabitants,  and other features of regions in various types of climates are instances of this collection." ;
	a <http://sw.cyc.com/2006/07/27/cyc/ConceptTypeByDomain> ;
	<http://sw.cyc.com/2006/07/27/cyc/prettyString-Canonical> "climate concept" ;
	<http://sw.cyc.com/2006/07/27/cyc/prettyString> "the climate domain" , "climate concepts" ;
	<http://www.w3.org/2000/01/rdf-schema#subClassOf> <http://www.w3.org/2002/07/owl#Thing> .

<http://sw.cyc.com/2006/07/27/cyc/GenericQuantity> <http://www.w3.org/2000/01/rdf-schema#comment> """A specialization of #$NonNumericScalarQuantity (q.v.).  Each instance of #$GenericQuantity is a properly interval-like, generic or approximate measure that is not numerically specified.  (Cf. #$MeasurableQuantity).
<p>
For example, (#$HighAmountFn #$Elasticity) is a \"high amount of elasticity\" (with respect to some contextually-determined, conventional elasticity scale), but is not explicitly associated with any particular number or numbers.  (But see #$NoteAboutGivingGenericValueFunctionsNumericValues.)
<p>
The values returned by #$GenericValueFunctions (such as #$HighAmountFn) are all instances of #$GenericQuantity.""" ;
	a <http://sw.cyc.com/2006/07/27/cyc/ObjectType> , <http://sw.cyc.com/2006/07/27/cyc/AtemporalNecessarilyEssentialCollectionType> , <http://sw.cyc.com/2006/07/27/cyc/KEClarifyingCollectionType> ;
	<http://sw.cyc.com/2006/07/27/cyc/prettyString-Canonical> "generic quantity" ;
	<http://sw.cyc.com/2006/07/27/cyc/prettyString> "Extent" , "extents" , "generic quantities" ;
	<http://www.w3.org/2000/01/rdf-schema#subClassOf> <http://sw.cyc.com/2006/07/27/cyc/NonNumericScalarQuantity> .

<http://sw.cyc.com/2006/07/27/cyc/Temperature> <http://www.w3.org/2000/01/rdf-schema#comment> "A specialization of #$PhysicalQuantity.  Each instance of #$Temperature is the degree of \"hotness\" - or, more precisely, the potential for heat transfer - of some physical thing (<i>i.e.</i> some instance of #$PartiallyTangible).  An instance of #$Temperature may be either a fixed interval, such as 98.6 degrees Fahrenheit (cf. #$UnitOfTemperature), or a range, such as #$HumanHabitableTemperature or #$TooHotToTouch." ;
	a <http://sw.cyc.com/2006/07/27/cyc/AtemporalNecessarilyEssentialCollectionType> , <http://sw.cyc.com/2006/07/27/cyc/UnitOfMeasureConcept> , <http://sw.cyc.com/2006/07/27/cyc/ScalarIntervals-Quantity-Topic> , <http://sw.cyc.com/2006/07/27/cyc/PrimitiveMeasurableQuantityType> , <http://sw.cyc.com/2006/07/27/cyc/WeatherAttributes-Weather-Topic> , <http://sw.cyc.com/2006/07/27/cyc/Weather-Topic> ;
	<http://sw.cyc.com/2006/07/27/cyc/prettyString-Canonical> "temperature" ;
	<http://sw.cyc.com/2006/07/27/cyc/prettyString> "temperatures" ;
	<http://www.w3.org/2000/01/rdf-schema#subClassOf> <http://sw.cyc.com/2006/07/27/cyc/PhysicalQuantity> , <http://sw.cyc.com/2006/07/27/cyc/OneDimensionalQuantity> , <http://sw.cyc.com/2006/07/27/cyc/NonAspectualQuantity> ;
	<http://www.w3.org/2002/07/owl#disjointWith> <http://sw.cyc.com/2006/07/27/cyc/Rate> , <http://sw.cyc.com/2006/07/27/cyc/Volume> , <http://sw.cyc.com/2006/07/27/cyc/AngularDistance> , <http://sw.cyc.com/2006/07/27/cyc/Pressure> , <http://sw.cyc.com/2006/07/27/cyc/IntervalOnNumberLine> , <http://sw.cyc.com/2006/07/27/cyc/Voltage> , <http://sw.cyc.com/2006/07/27/cyc/Molarity> , <http://sw.cyc.com/2006/07/27/cyc/ElectricalCharge> .

<http://sw.cyc.com/2006/07/27/cyc/above-Higher> <http://www.w3.org/2000/01/rdf-schema#comment> "(#$above-Higher HIGH-OBJ LOW-OBJ) means that HIGH-OBJ is at a greater altitude (from some common reference point) than LOW-OBJ.  In terrestrial contexts (see #$TerrestrialFrameOfReferenceMt), (#$above-Higher HIGH-OBJ LOW-OBJ) typically means that HIGH-OBJ-A is at a greater altitude above sea level (see the predicate #$altitudeAboveSeaLevel) than LOW-OBJ." ;
	a <http://www.w3.org/2002/07/owl#TransitiveProperty> , <http://sw.cyc.com/2006/07/27/cyc/CoexistingObjectsPredicate> , <http://sw.cyc.com/2006/07/27/cyc/AsymmetricBinaryPredicate> , <http://sw.cyc.com/2006/07/27/cyc/RelativeLocationalPredicate> , <http://sw.cyc.com/2006/07/27/cyc/RelativePositionsOfObjects-Spatial-Topic> ;
	<http://sw.cyc.com/2006/07/27/cyc/prettyString-Canonical> "Above-Higher" ;
	<http://www.w3.org/2000/01/rdf-schema#domain> <http://sw.cyc.com/2006/07/27/cyc/SpatialThing-Localized> ;
	<http://sw.cyc.com/2006/07/27/cyc/arity> "2"^^<http://www.w3.org/2001/XMLSchema#long> ;
	<http://www.w3.org/2000/01/rdf-schema#range> <http://sw.cyc.com/2006/07/27/cyc/SpatialThing-Localized> ;
	<http://www.w3.org/2000/01/rdf-schema#subPropertyOf> <http://sw.cyc.com/2006/07/27/cyc/temporallyCoexist> ;
	<http://sw.cyc.com/2006/07/27/cyc/arg1Format> <http://sw.cyc.com/2006/07/27/cyc/openEntryFormatInArgs> ;
	<http://sw.cyc.com/2006/07/27/cyc/arg2Format> <http://sw.cyc.com/2006/07/27/cyc/openEntryFormatInArgs> ;
	<http://sw.cyc.com/2006/07/27/cyc/negationInverse> <http://sw.cyc.com/2006/07/27/cyc/above-Higher> .

<http://sw.cyc.com/2006/07/27/cyc/over-UnderspecifiedLocation> <http://www.w3.org/2000/01/rdf-schema#comment> """(#$over-UnderspecifiedLocation ACT LOC) states that an abstract
locational relation holds between ACT and LOC, where LOC is a
#$Location-Underspecified and ACT is some action requiring some kind of
abstract 'floor' or lower boundary. We can say 'the path went over the
mountain', 'the game went over 90 minutes' (90 minutes being an abstract
location by virtue of being an abstract container), etc.""" ;
	a <http://www.w3.org/2002/07/owl#TransitiveProperty> , <http://sw.cyc.com/2006/07/27/cyc/AsymmetricBinaryPredicate> , <http://sw.cyc.com/2006/07/27/cyc/UnderspecifiedPrepositionPredicate> ;
	<http://sw.cyc.com/2006/07/27/cyc/prettyString-Canonical> "over" ;
	<http://sw.cyc.com/2006/07/27/cyc/quotedIsa> <http://sw.cyc.com/2006/07/27/cyc/NLTerm> ;
	<http://www.w3.org/2000/01/rdf-schema#domain> <http://sw.cyc.com/2006/07/27/cyc/Individual> ;
	<http://sw.cyc.com/2006/07/27/cyc/arity> "2"^^<http://www.w3.org/2001/XMLSchema#long> ;
	<http://sw.cyc.com/2006/07/27/cyc/sharedNotes> <http://sw.cyc.com/2006/07/27/cyc/SharedNoteOnIntermediateVocabulary> ;
	<http://www.w3.org/2000/01/rdf-schema#range> <http://sw.cyc.com/2006/07/27/cyc/Individual> ;
	<http://sw.cyc.com/2006/07/27/cyc/negationInverse> <http://sw.cyc.com/2006/07/27/cyc/over-UnderspecifiedLocation> .

<http://sw.cyc.com/2006/07/27/cyc/negationPreds> <http://www.w3.org/2000/01/rdf-schema#comment> """A #$MetaPredicate for stating that two predicates are logical \"contraries\" of one another.  <code>(#$negationPreds PRED1 PRED2)</code> means that if <code>PRED1</code> holds among a given sequence of things, then <code>PRED2</code> does <i>not</i> hold among that sequence (and vice versa).  Thus it is equivalent to 

<pre>  (#$not (#$and (PRED1 . ARGS) (PRED2 . ARGS))) .</pre>  

For example, (#$negationPreds #$owns #$rents) holds, as one cannot both own and rent a given thing at the same time.   
<p>
Note that the argument types of <code>PRED1</code> and <code>PRED2</code> need not be the same, they merely must not be disjoint.  Note also that <code>PRED1</code> and <code>PRED2</code> are constrained (see e.g. #$interArgIsa) either to both having the same fixed-arity (see #$FixedArityRelation) or to both having variable-arity (see #$VariableArityRelations).     
<p>
See also #$genlPreds and #$negationInverse.""" ;
	a <http://www.w3.org/2002/07/owl#TransitiveProperty> , <http://www.w3.org/2002/07/owl#SymmetricProperty> , <http://sw.cyc.com/2006/07/27/cyc/IrreflexiveBinaryPredicate> , <http://sw.cyc.com/2006/07/27/cyc/DefaultMonotonicPredicate> , <http://sw.cyc.com/2006/07/27/cyc/RuleMacroPredicate> , <http://sw.cyc.com/2006/07/27/cyc/RelationalNounSlot> , <http://sw.cyc.com/2006/07/27/cyc/MetaPredicate> , <http://sw.cyc.com/2006/07/27/cyc/TaxonomicSlotForPredicates> , <http://sw.cyc.com/2006/07/27/cyc/HLPredicate> , <http://sw.cyc.com/2006/07/27/cyc/NegationRelations-Fundamental-Topic> ;
	<http://sw.cyc.com/2006/07/27/cyc/prettyString-Canonical> "mutually-negating predicate" ;
	<http://sw.cyc.com/2006/07/27/cyc/prettyString> "mutually-negating predicates" ;
	<http://sw.cyc.com/2006/07/27/cyc/quotedIsa> <http://sw.cyc.com/2006/07/27/cyc/OpenCycDefinitionalPredicate> ;
	<http://www.w3.org/2000/01/rdf-schema#domain> <http://sw.cyc.com/2006/07/27/cyc/Predicate> ;
	<http://sw.cyc.com/2006/07/27/cyc/arity> "2"^^<http://www.w3.org/2001/XMLSchema#long> ;
	<http://www.w3.org/2000/01/rdf-schema#range> <http://sw.cyc.com/2006/07/27/cyc/Predicate> ;
	<http://sw.cyc.com/2006/07/27/cyc/arg1Format> <http://sw.cyc.com/2006/07/27/cyc/SetTheFormat> ;
	<http://sw.cyc.com/2006/07/27/cyc/arg2Format> <http://sw.cyc.com/2006/07/27/cyc/SetTheFormat> ;
	<http://sw.cyc.com/2006/07/27/cyc/genlInverse> <http://sw.cyc.com/2006/07/27/cyc/negationPreds> .

<http://sw.cyc.com/2006/07/27/cyc/under-UnderspecifiedLocation> <http://www.w3.org/2000/01/rdf-schema#comment> "(#$under-UnderspecifiedLocation ACT LOC) states that an abstract locational relation holds between ACT and LOC, where LOC is a #$Location-Underspecified and ACT is some action requiring some kind of abstract 'ceiling' or upper boundary. We can say 'the path ran under the highway', 'the game ran under 90 minutes' (90 minutes being an abstract location by virtue of being an abstract container), etc." ;
	a <http://www.w3.org/2002/07/owl#TransitiveProperty> , <http://sw.cyc.com/2006/07/27/cyc/AsymmetricBinaryPredicate> , <http://sw.cyc.com/2006/07/27/cyc/UnderspecifiedPrepositionPredicate> ;
	<http://sw.cyc.com/2006/07/27/cyc/prettyString-Canonical> "under" ;
	<http://sw.cyc.com/2006/07/27/cyc/quotedIsa> <http://sw.cyc.com/2006/07/27/cyc/NLTerm> ;
	<http://www.w3.org/2000/01/rdf-schema#domain> <http://sw.cyc.com/2006/07/27/cyc/Individual> ;
	<http://sw.cyc.com/2006/07/27/cyc/arity> "2"^^<http://www.w3.org/2001/XMLSchema#long> ;
	<http://sw.cyc.com/2006/07/27/cyc/sharedNotes> <http://sw.cyc.com/2006/07/27/cyc/SharedNoteOnIntermediateVocabulary> ;
	<http://www.w3.org/2000/01/rdf-schema#range> <http://sw.cyc.com/2006/07/27/cyc/Individual> ;
	<http://sw.cyc.com/2006/07/27/cyc/negationInverse> <http://sw.cyc.com/2006/07/27/cyc/under-UnderspecifiedLocation> .

<http://sw.cyc.com/2006/07/27/cyc/NoteOnCycMergedOntologyConstants> <http://www.w3.org/2000/01/rdf-schema#comment> "This constant represents an important concept in the SENSUS Ontology developed by ISI, and has been mapped into the CYC Merged Ontology for the DARPA HPKB Project." ;
	a <http://sw.cyc.com/2006/07/27/cyc/Individual> ;
	<http://sw.cyc.com/2006/07/27/cyc/prettyString-Canonical> "Note On Cyc Merged Ontology Constants" ;
	<http://sw.cyc.com/2006/07/27/cyc/quotedIsa> <http://sw.cyc.com/2006/07/27/cyc/SharedNote> .

<http://sw.cyc.com/2006/07/27/cyc/AboveGround> <http://www.w3.org/2000/01/rdf-schema#comment> "The collection of instances of #$SpatialThing-Localized  that are resting on the surface of the ground of a particular place." ;
	a <http://sw.cyc.com/2006/07/27/cyc/SpatialThingTypeByGenericLocation> , <http://sw.cyc.com/2006/07/27/cyc/SundrySpatialConcepts-Spatial-Topic> ;
	<http://sw.cyc.com/2006/07/27/cyc/prettyString-Canonical> "aboveground thing" ;
	<http://sw.cyc.com/2006/07/27/cyc/prettyString> "aboveground" , "more aboveground" , "most aboveground" ;
	<http://www.w3.org/2000/01/rdf-schema#subClassOf> <http://sw.cyc.com/2006/07/27/cyc/SpatialThing-Localized> .

<http://sw.cyc.com/2006/07/27/cyc/AboveGroundFuelStorageTank> <http://www.w3.org/2000/01/rdf-schema#comment> "Each instance of #$AboveGroundFuelStorageTank is a large, cylindrical tank intended for the storage of #$Oil, #$GasolineFuel or other liquid petrochemicals.  The capacity of these tanks can range upwards of 10,000 gallons." ;
	a <http://sw.cyc.com/2006/07/27/cyc/ExistingObjectType> , <http://sw.cyc.com/2006/07/27/cyc/SpatiallyDisjointObjectType> , <http://sw.cyc.com/2006/07/27/cyc/ArtifactualFeatureType> ;
	<http://sw.cyc.com/2006/07/27/cyc/prettyString-Canonical> "above-ground fuel storage tank" ;
	<http://sw.cyc.com/2006/07/27/cyc/prettyString> "above-ground fuel storage tanks" ;
	<http://www.w3.org/2000/01/rdf-schema#subClassOf> <http://sw.cyc.com/2006/07/27/cyc/FixedStructure> , <http://sw.cyc.com/2006/07/27/cyc/HollowCylindricalObject> , <http://sw.cyc.com/2006/07/27/cyc/FuelTank> .

<http://sw.cyc.com/2006/07/27/cyc/FixedStructure> <http://www.w3.org/2000/01/rdf-schema#comment> "#$FixedStructure is a specialization of #$ConstructionArtifact.  Each instance of #$FixedStructure is a human-constructed, freestanding object that exists in a fixed location.  Examples include buildings, pyramids, the Great Wall of China, dams, bridges, elevated roadways, and canals. Such structures may have parts which are also instances of #$FixedStructure (e.g. bridge pilings) and parts which are not freestanding (e.g. the span of a bridge, or a room in a building)." ;
	a <http://sw.cyc.com/2006/07/27/cyc/ExistingObjectType> , <http://sw.cyc.com/2006/07/27/cyc/SpatiallyDisjointObjectType> , <http://sw.cyc.com/2006/07/27/cyc/Construction-Topic> ;
	<http://sw.cyc.com/2006/07/27/cyc/prettyString-Canonical> "fixed freestanding structure" ;
	<http://sw.cyc.com/2006/07/27/cyc/prettyString> "free-standing structure" , "free-standing structures" , "fixed free-standing structure" , "fixed free-standing structures" , "freestanding structure" , "freestanding structures" , "fixed structure" , "fixed structures" , "fixed freestanding structures" ;
	<http://www.w3.org/2000/01/rdf-schema#subClassOf> <http://sw.cyc.com/2006/07/27/cyc/GeographicalThing> , <http://sw.cyc.com/2006/07/27/cyc/ConstructionArtifact> , <http://sw.cyc.com/2006/07/27/cyc/Place-NonAgent> ;
	<http://sw.cyc.com/2006/07/27/cyc/quotedIsa> <http://sw.cyc.com/2006/07/27/cyc/TerrorismOntologyConstant> ;
	<http://www.w3.org/2002/07/owl#disjointWith> <http://sw.cyc.com/2006/07/27/cyc/TransportationDevice> , <http://sw.cyc.com/2006/07/27/cyc/TransportationContainerProduct> .

<http://sw.cyc.com/2006/07/27/cyc/HollowCylindricalObject> <http://www.w3.org/2000/01/rdf-schema#comment> """A specialization of #$SolidTangibleThing; instances are characterized
by a cylindrical, single-walled structure and a hollow interior.
Examples include #$GunBarrels and #$Bottles.  The structure
in question must be 'long' enough to justify the appelation of 'hollow'.
Borderline non-cases might include two-dimensional ringlike structures like
wedding-rings.""" ;
	a <http://sw.cyc.com/2006/07/27/cyc/ExistingObjectType> ;
	<http://sw.cyc.com/2006/07/27/cyc/prettyString-Canonical> "hollow cylindrical object" ;
	<http://sw.cyc.com/2006/07/27/cyc/prettyString> "hollow cylindrical objects" ;
	<http://www.w3.org/2000/01/rdf-schema#subClassOf> <http://sw.cyc.com/2006/07/27/cyc/SolidTangibleThing> , <http://sw.cyc.com/2006/07/27/cyc/Hollow> , <http://sw.cyc.com/2006/07/27/cyc/ContainerShapedObject> ;
	<http://www.w3.org/2002/07/owl#disjointWith> <http://sw.cyc.com/2006/07/27/cyc/SheetOfSomeStuff> .

<http://sw.cyc.com/2006/07/27/cyc/FuelTank> <http://www.w3.org/2000/01/rdf-schema#comment> "Any tank used to contain a FuelSubstance." .

<http://sw.cyc.com/2006/07/27/cyc/above-Overhead> a <http://sw.cyc.com/2006/07/27/cyc/RelativeLocationalPredicate> , <http://sw.cyc.com/2006/07/27/cyc/RelativePositionsOfObjects-Spatial-Topic> ;
	<http://sw.cyc.com/2006/07/27/cyc/prettyString-Canonical> "Above-Overhead" ;
	<http://www.w3.org/2000/01/rdf-schema#domain> <http://sw.cyc.com/2006/07/27/cyc/SpatialThing-Localized> ;
	<http://sw.cyc.com/2006/07/27/cyc/arity> "2"^^<http://www.w3.org/2001/XMLSchema#long> ;
	<http://www.w3.org/2000/01/rdf-schema#range> <http://sw.cyc.com/2006/07/27/cyc/SpatialThing-Localized> ;
	<http://www.w3.org/2000/01/rdf-schema#subPropertyOf> <http://sw.cyc.com/2006/07/27/cyc/above-Directly> ;
	<http://sw.cyc.com/2006/07/27/cyc/arg1Format> <http://sw.cyc.com/2006/07/27/cyc/SetTheFormat> ;
	<http://sw.cyc.com/2006/07/27/cyc/arg2Format> <http://sw.cyc.com/2006/07/27/cyc/SetTheFormat> ;
	<http://sw.cyc.com/2006/07/27/cyc/negationInverse> <http://sw.cyc.com/2006/07/27/cyc/above-Overhead> ;
	<http://sw.cyc.com/2006/07/27/cyc/negationPreds> <http://sw.cyc.com/2006/07/27/cyc/touches> .

<http://sw.cyc.com/2006/07/27/cyc/touches> <http://www.w3.org/2000/01/rdf-schema#comment> """A #$RelativeLocationalPredicate and specialization of #$near that holds between certain tangible objects.  <code>(#$touches OBJ1 OBJ2)</code> means that <code>OBJ1</code> and <code>OBJ2</code> are in contact, either directly or indirectly.  Two spatial things are directly in contact just in case there is nothing between them; to indicate that such a situation obtains between two spatial things, use the specialization #$touches-Directly.  Two spatial things touch indirectly if there is only a very thin object or substance between them.  Here 'very thin' means that the distance between the surfaces of the two spatial things is very much less than the distance between their center points.  
<p>
Here are some examples in which #$touches holds: an airplane touches the air around it; my feet touch the floor (even though I am wearing shoes); a blanket touches the person sleeping under it (even if there is a sheet); a hovercraft touches the water (even though a cushion of air is between it and the water).""" ;
	a <http://www.w3.org/2002/07/owl#TransitiveProperty> , <http://www.w3.org/2002/07/owl#SymmetricProperty> , <http://sw.cyc.com/2006/07/27/cyc/ReflexiveBinaryPredicate> , <http://sw.cyc.com/2006/07/27/cyc/RelativeLocationalPredicate> , <http://sw.cyc.com/2006/07/27/cyc/ProximityAndLocation-Spatial-Topic> , <http://sw.cyc.com/2006/07/27/cyc/LinearObjectConcept> , <http://sw.cyc.com/2006/07/27/cyc/SpatialThingPredicate> , <http://sw.cyc.com/2006/07/27/cyc/MereotopologyConcept> ;
	<http://sw.cyc.com/2006/07/27/cyc/prettyString-Canonical> "touching an object" ;
	<http://sw.cyc.com/2006/07/27/cyc/prettyString> "touch an object" , "touched an object" , "touches an object" , "have touched an object" , "has touched an object" , "will touch an object" , "had touched an object" , "will have touched an object" ;
	<http://www.w3.org/2000/01/rdf-schema#domain> <http://sw.cyc.com/2006/07/27/cyc/SpatialThing> ;
	<http://sw.cyc.com/2006/07/27/cyc/arity> "2"^^<http://www.w3.org/2001/XMLSchema#long> ;
	<http://www.w3.org/2000/01/rdf-schema#range> <http://sw.cyc.com/2006/07/27/cyc/SpatialThing> ;
	<http://www.w3.org/2000/01/rdf-schema#subPropertyOf> <http://sw.cyc.com/2006/07/27/cyc/near> ;
	<http://sw.cyc.com/2006/07/27/cyc/arg1Format> <http://sw.cyc.com/2006/07/27/cyc/SetTheFormat> ;
	<http://sw.cyc.com/2006/07/27/cyc/arg2Format> <http://sw.cyc.com/2006/07/27/cyc/SetTheFormat> ;
	<http://sw.cyc.com/2006/07/27/cyc/negationPreds> <http://sw.cyc.com/2006/07/27/cyc/spatiallySeparated> ;
	<http://sw.cyc.com/2006/07/27/cyc/genlInverse> <http://sw.cyc.com/2006/07/27/cyc/touches> .

<http://sw.cyc.com/2006/07/27/cyc/above-Touching> <http://www.w3.org/2000/01/rdf-schema#comment> """A binary #$SpatialPredicate that is a
specialization of both #$above-Directly and #$touches (qq.v.).
(#$above-Touching ABOVE BELOW) means that ABOVE is located over 
BELOW and they are touching.  Examples of things related by
#$above-Touching include a person and a chair s/he is sitting on, 
a boat and the on water it floats on, and a hat and the head 
wearing it.  Note that it need _not_ be the case that every point 
of ABOVE is higher than every point of BELOW.""" ;
	a <http://www.w3.org/2002/07/owl#TransitiveProperty> , <http://sw.cyc.com/2006/07/27/cyc/CoexistingObjectsPredicate> , <http://sw.cyc.com/2006/07/27/cyc/AsymmetricBinaryPredicate> , <http://sw.cyc.com/2006/07/27/cyc/RelativeLocationalPredicate> , <http://sw.cyc.com/2006/07/27/cyc/RelativePositionsOfObjects-Spatial-Topic> , <http://sw.cyc.com/2006/07/27/cyc/PredicateOrCollection-UsedInUCTRepresentation> ;
	<http://sw.cyc.com/2006/07/27/cyc/prettyString-Canonical> "Above-Touching" ;
	<http://www.w3.org/2000/01/rdf-schema#domain> <http://sw.cyc.com/2006/07/27/cyc/SpatialThing-Localized> ;
	<http://sw.cyc.com/2006/07/27/cyc/arity> "2"^^<http://www.w3.org/2001/XMLSchema#long> ;
	<http://www.w3.org/2000/01/rdf-schema#range> <http://sw.cyc.com/2006/07/27/cyc/SpatialThing-Localized> ;
	<http://www.w3.org/2000/01/rdf-schema#subPropertyOf> <http://sw.cyc.com/2006/07/27/cyc/temporallyCoexist> , <http://sw.cyc.com/2006/07/27/cyc/above-Directly> , <http://sw.cyc.com/2006/07/27/cyc/touches> ;
	<http://sw.cyc.com/2006/07/27/cyc/negationInverse> <http://sw.cyc.com/2006/07/27/cyc/above-Directly> , <http://sw.cyc.com/2006/07/27/cyc/above-Touching> .

<http://sw.cyc.com/2006/07/27/cyc/PredicateOrCollection-UsedInUCTRepresentation> a <http://www.w3.org/2002/07/owl#Class> ;
	<http://sw.cyc.com/2006/07/27/cyc/prettyString-Canonical> "predicate or collection used in UCT representation" ;
	<http://www.w3.org/2000/01/rdf-schema#subClassOf> <http://www.w3.org/2002/07/owl#Thing> .

<http://sw.cyc.com/2006/07/27/cyc/AbqaiqOilField> <http://www.w3.org/2000/01/rdf-schema#comment> "An #$OilField located in #$SaudiArabia" ;
	a <http://sw.cyc.com/2006/07/27/cyc/Individual> , <http://sw.cyc.com/2006/07/27/cyc/OilField> ;
	<http://sw.cyc.com/2006/07/27/cyc/prettyString-Canonical> "the Abqaiq Oilfield" ;
	<http://sw.cyc.com/2006/07/27/cyc/prettyString> "Abqaiq" .

<http://sw.cyc.com/2006/07/27/cyc/Abqaiq-YanbuPipeline> <http://www.w3.org/2000/01/rdf-schema#comment> "A gas pipeline in the Middle East. It is important for reasoning about situations described in specializations of #$HPKBVocabMt." ;
	a <http://sw.cyc.com/2006/07/27/cyc/Individual> , <http://sw.cyc.com/2006/07/27/cyc/GasPipeline> ;
	<http://sw.cyc.com/2006/07/27/cyc/prettyString-Canonical> "Abqaiq-Yanbu Pipeline" ;
	<http://sw.cyc.com/2006/07/27/cyc/prettyString> "Abqaiq-Yanbu NGL line" .

<http://sw.cyc.com/2006/07/27/cyc/GasPipeline> <http://www.w3.org/2000/01/rdf-schema#comment> "The collection of #$Pipelines whose primary function is the transportation of #$NaturalGas.  See also #$OilPipeline." ;
	a <http://sw.cyc.com/2006/07/27/cyc/ExistingObjectType> , <http://sw.cyc.com/2006/07/27/cyc/ArtifactualFeatureType> ;
	<http://sw.cyc.com/2006/07/27/cyc/prettyString-Canonical> "gas pipeline" ;
	<http://sw.cyc.com/2006/07/27/cyc/prettyString> "gas pipelines" ;
	<http://www.w3.org/2000/01/rdf-schema#subClassOf> <http://sw.cyc.com/2006/07/27/cyc/FixedStructure> , <http://sw.cyc.com/2006/07/27/cyc/InfrastructureProduct> , <http://sw.cyc.com/2006/07/27/cyc/TransportFacility> , <http://sw.cyc.com/2006/07/27/cyc/PathArtifact> , <http://sw.cyc.com/2006/07/27/cyc/Pipeline> ;
	<http://sw.cyc.com/2006/07/27/cyc/quotedIsa> <http://sw.cyc.com/2006/07/27/cyc/TerrorismOntologyConstant> .

<http://sw.cyc.com/2006/07/27/cyc/AbradingSomething> <http://www.w3.org/2000/01/rdf-schema#comment> "A collection of events.  In an #$AbradingSomething event, the surface of some object is gradually worn away by scraping or similar physical contact involving friction.  Devices used in elements of #$AbradingSomething include files and sand paper; elements of #$AbradingSomething would include the event in which Howard Hughes sanded down the Spruce Goose for the last time, the event in which Lucy Ricardo filed her fingernails just before her singing debut at Rickie's club, etc." ;
	a <http://sw.cyc.com/2006/07/27/cyc/ChangeOfState-Topic> , <http://sw.cyc.com/2006/07/27/cyc/TemporalStuffType> ;
	<http://sw.cyc.com/2006/07/27/cyc/prettyString-Canonical> "abrading event" ;
	<http://sw.cyc.com/2006/07/27/cyc/prettyString> "abrasion" , "abrade" , "abraded" , "abrades" , "abrading" , "have abraded" , "has abraded" , "will abrade" , "will have abraded" , "abrading events" ;
	<http://www.w3.org/2000/01/rdf-schema#subClassOf> <http://sw.cyc.com/2006/07/27/cyc/Ablation> , <http://sw.cyc.com/2006/07/27/cyc/Rubbing> .

<http://sw.cyc.com/2006/07/27/cyc/Rubbing> <http://www.w3.org/2000/01/rdf-schema#comment> "A collection of events.  An instance of #$Rubbing is an event in which the #$objectActedOn is rubbed." ;
	a <http://sw.cyc.com/2006/07/27/cyc/DurativeEventType> , <http://sw.cyc.com/2006/07/27/cyc/SomeImportantMovement-RelatedPredicates-Movement-Topic> , <http://sw.cyc.com/2006/07/27/cyc/Movement-Topic> ;
	<http://sw.cyc.com/2006/07/27/cyc/prettyString-Canonical> "rubbing" ;
	<http://sw.cyc.com/2006/07/27/cyc/prettyString> "rub" , "rubbed" , "rubs" , "have rubbed" , "has rubbed" , "will rub" , "had rubbed" , "will have rubbed" ;
	<http://www.w3.org/2000/01/rdf-schema#subClassOf> <http://sw.cyc.com/2006/07/27/cyc/Sliding-Generic> , <http://sw.cyc.com/2006/07/27/cyc/FrictionProcess> ;
	<http://www.w3.org/2002/07/owl#disjointWith> <http://sw.cyc.com/2006/07/27/cyc/FrictionlessMotion> , <http://sw.cyc.com/2006/07/27/cyc/Sliding-LowFriction> .

<http://sw.cyc.com/2006/07/27/cyc/AbradingTeeth> <http://www.w3.org/2000/01/rdf-schema#comment> "The process of scraping or wearing away the surface of teeth." ;
	a <http://sw.cyc.com/2006/07/27/cyc/TemporalStuffType> ;
	<http://sw.cyc.com/2006/07/27/cyc/prettyString-Canonical> "abrading teeth" ;
	<http://www.w3.org/2000/01/rdf-schema#subClassOf> <http://sw.cyc.com/2006/07/27/cyc/AbradingSomething> .

<http://sw.cyc.com/2006/07/27/cyc/AbrahamBenrubi> a <http://sw.cyc.com/2006/07/27/cyc/Individual> , <http://sw.cyc.com/2006/07/27/cyc/MaleHuman> , <http://sw.cyc.com/2006/07/27/cyc/Actor> ;
	<http://sw.cyc.com/2006/07/27/cyc/prettyString-Canonical> "Abraham Benrubi" ;
	<http://sw.cyc.com/2006/07/27/cyc/prettyString> "Benrubi" .

<http://sw.cyc.com/2006/07/27/cyc/AbrahamLincoln> <http://www.w3.org/2000/01/rdf-schema#comment> "Abraham Lincoln (1809-1865),  born in #$Kentucky-State, practiced law in the #$CityOfSpringfieldIL (#$Illinois-State) and held several public offices there.  #$AbrahamLincoln was elected the 16th president of the United States and he was the Union's leader during the #$UnitedStatesCivilWar.  He was assassinated by the actor #$JohnWilkesBooth." ;
	a <http://sw.cyc.com/2006/07/27/cyc/Individual> , <http://sw.cyc.com/2006/07/27/cyc/TemporalThing> , <http://sw.cyc.com/2006/07/27/cyc/FamousHuman> , <http://sw.cyc.com/2006/07/27/cyc/HistoricHuman> , <http://sw.cyc.com/2006/07/27/cyc/CensusGroupOfCaucasians> ;
	<http://sw.cyc.com/2006/07/27/cyc/prettyString-Canonical> "Abe Lincoln" ;
	<http://sw.cyc.com/2006/07/27/cyc/prettyString> "Abraham Lincoln" , "Lincoln" .

<http://sw.cyc.com/2006/07/27/cyc/FamousHuman> <http://www.w3.org/2000/01/rdf-schema#comment> "A specialization of #$HomoSapiens.  This is the collection of all human beings that are #$Famous (i.e. identifiable by a large number of other human beings). See also #$HistoricHuman." ;
	a <http://sw.cyc.com/2006/07/27/cyc/ExistingObjectType> , <http://www.w3.org/2002/07/owl#Class> , <http://sw.cyc.com/2006/07/27/cyc/AtemporalNecessarilyEssentialCollectionType> , <http://sw.cyc.com/2006/07/27/cyc/KEClarifyingCollectionType> , <http://sw.cyc.com/2006/07/27/cyc/IntermittentCollection> ;
	<http://sw.cyc.com/2006/07/27/cyc/prettyString-Canonical> "famous person" ;
	<http://sw.cyc.com/2006/07/27/cyc/prettyString> "stars" , "Star" , "superstar" , "superstars" , "celeb" , "celebs" , "public figure" , "public figures" , "famous people" , "famous persons" , "human whose Renown Level has been infamy" , "humans whose Renown Level has been infamy" , "human being whose Renown Level has been infamy" , "homo sapiens whose Renown Level has been infamy" , "human whose Renown Level is infamy" , "humans whose Renown Level is infamy" , "human being whose Renown Level is infamy" , "homo sapiens whose Renown Level is infamy" , "personality" , "personalities" .

<http://sw.cyc.com/2006/07/27/cyc/ABRInformationServicesInc> <http://sw.cyc.com/2006/07/27/cyc/prettyString-Canonical> "ABR Information Services, Inc." ;
	<http://sw.cyc.com/2006/07/27/cyc/prettyString> "ABR Information Services" .

<http://sw.cyc.com/2006/07/27/cyc/AbrinToxin> <http://www.w3.org/2000/01/rdf-schema#comment> "A #$ToxinBioAgentType. #$AbrinToxin is derived from the Rosary Pea. It is closely related to #$RicinToxin." ;
	a <http://sw.cyc.com/2006/07/27/cyc/ExistingStuffType> , <http://sw.cyc.com/2006/07/27/cyc/ToxinBioAgentType> ;
	<http://sw.cyc.com/2006/07/27/cyc/prettyString-Canonical> "abrin" ;
	<http://www.w3.org/2000/01/rdf-schema#subClassOf> <http://sw.cyc.com/2006/07/27/cyc/Powder> , <http://sw.cyc.com/2006/07/27/cyc/BiologicalToxin> .

<http://sw.cyc.com/2006/07/27/cyc/Powder> <http://www.w3.org/2000/01/rdf-schema#comment> "A specialization of #$Granular.  Instances of #$Powder are composed of many fine particles and are #$FluidTangibleThing." ;
	a <http://sw.cyc.com/2006/07/27/cyc/PartiallyTangibleTypeByPhysicalStructuralFeature> , <http://sw.cyc.com/2006/07/27/cyc/TangibleStuffStateType> , <http://sw.cyc.com/2006/07/27/cyc/DosageFormType> , <http://sw.cyc.com/2006/07/27/cyc/StructuralAttributes-Material-Topic> ;
	<http://sw.cyc.com/2006/07/27/cyc/prettyString-Canonical> "powder" ;
	<http://sw.cyc.com/2006/07/27/cyc/prettyString> "powdery" , "more powdery" , "most powdery" ;
	<http://www.w3.org/2000/01/rdf-schema#subClassOf> <http://sw.cyc.com/2006/07/27/cyc/InanimateObject> , <http://sw.cyc.com/2006/07/27/cyc/Opaque> , <http://sw.cyc.com/2006/07/27/cyc/Granular> ;
	<http://www.w3.org/2002/07/owl#disjointWith> <http://sw.cyc.com/2006/07/27/cyc/Water> .

<http://sw.cyc.com/2006/07/27/cyc/BiologicalToxin> <http://www.w3.org/2000/01/rdf-schema#comment> "A #$ToxicSubstance produced by some #$Organism-Whole. An example is the toxin produced by the bacterium Clostridium botulinum; the toxin is responsible for the cluster of effects seen in #$Botulism." ;
	a <http://sw.cyc.com/2006/07/27/cyc/ExistingStuffType> ;
	<http://sw.cyc.com/2006/07/27/cyc/prettyString-Canonical> "biological toxin" ;
	<http://sw.cyc.com/2006/07/27/cyc/prettyString> "biological toxins" ;
	<http://www.w3.org/2000/01/rdf-schema#subClassOf> <http://sw.cyc.com/2006/07/27/cyc/ToxicSubstance> , <http://sw.cyc.com/2006/07/27/cyc/NaturalTangibleStuff> , <http://sw.cyc.com/2006/07/27/cyc/BiologicalAgentStuff> ;
	<http://www.w3.org/2002/07/owl#disjointWith> <http://sw.cyc.com/2006/07/27/cyc/LivingBiologicalAgent> .

<http://sw.cyc.com/2006/07/27/cyc/ToxinBioAgentType> <http://www.w3.org/2000/01/rdf-schema#comment> "#$ToxinBioAgentType is a specialization of #$BiologicalAgentType. Instances of #$ToxinBioAgentType are types of biological toxins that could potentially be used as biological agents in biological warfare." ;
	a <http://sw.cyc.com/2006/07/27/cyc/FacetingCollectionType> , <http://sw.cyc.com/2006/07/27/cyc/SecondOrderCollection> , <http://sw.cyc.com/2006/07/27/cyc/DisjointCollectionType> ;
	<http://sw.cyc.com/2006/07/27/cyc/prettyString-Canonical> "biological toxin agent type" ;
	<http://sw.cyc.com/2006/07/27/cyc/prettyString> "type of biological toxin agent" , "types of biological toxin agent" , "biological toxin agent types" ;
	<http://www.w3.org/2000/01/rdf-schema#subClassOf> <http://sw.cyc.com/2006/07/27/cyc/ExistingStuffType> , <http://sw.cyc.com/2006/07/27/cyc/BiologicalAgentType> ;
	<http://sw.cyc.com/2006/07/27/cyc/typeGenls> <http://sw.cyc.com/2006/07/27/cyc/BiologicalToxin> .

<http://sw.cyc.com/2006/07/27/cyc/AbrumiZahed> a <http://sw.cyc.com/2006/07/27/cyc/Person> ;
	<http://sw.cyc.com/2006/07/27/cyc/prettyString-Canonical> "Abrumi Zahed" ;
	<http://sw.cyc.com/2006/07/27/cyc/prettyString> "Zahed" .

<http://sw.cyc.com/2006/07/27/cyc/Abruzzi-RegionItaly> a <http://sw.cyc.com/2006/07/27/cyc/Individual> , <http://sw.cyc.com/2006/07/27/cyc/State-Geopolitical> , <http://sw.cyc.com/2006/07/27/cyc/GeographicalThing> ;
	<http://sw.cyc.com/2006/07/27/cyc/prettyString-Canonical> "Abruzzi" .

<http://sw.cyc.com/2006/07/27/cyc/AbscronRayonuAzerbaijan> a <http://sw.cyc.com/2006/07/27/cyc/Individual> , <http://sw.cyc.com/2006/07/27/cyc/GeographicalThing> , <http://sw.cyc.com/2006/07/27/cyc/GeopoliticalEntity> , <http://sw.cyc.com/2006/07/27/cyc/GeographicalRegion> ;
	<http://sw.cyc.com/2006/07/27/cyc/prettyString-Canonical> "Abscron Rayonu" .

<http://sw.cyc.com/2006/07/27/cyc/GeopoliticalEntity> <http://www.w3.org/2000/01/rdf-schema#comment> """A specialization of #$Organization and of #$LegalAgent and of #$GeographicalAgent; instances of this collection control #$GeographicalRegions.  Each instance of #$GeopoliticalEntity includes a governing body, but is more than just that governing body.  
<p>
Important subcollections include #$Country, #$IndependentCountry, #$State-Geopolitical, #$City, and #$Province.  Instances include #$CityOfTokyoJapan, #$BronxNY-Borough, #$Alaska-State, #$Rwanda, #$Singapore, #$InnerMongolia, #$Somerset-CountyEngland, and #$Taiwan-RepublicOfChina.  
<p>
A central feature of this collection is that geopolitical-entities (indeed, all  #$GeographicalAgents) are viewed in two significantly different ways with respect to two different types of geography-related microtheories.  In a \"physical\" geography microtheory (i.e. #$PhysicalGeographyMt and its submicrotheories), geopolitical-entities are clearly distinguished from the regions they control.  (#$TerritoryFn <b>GEO-POL</b>) is used in these contexts to denote the land mass (a #$GeopoliticalRegion) of a given geopolitical-entity <b>GEO-POL</b>.  In a \"dualist\" geography microtheory (i.e. #$DualistGeopoliticalMt and its submicrotheories), on the other hand, geopolitical-entities are viewed as being <i>both</i> agents <i>and</i> land masses (i.e. #$GeographicalRegions).  Thus, there is little need for #$TerritoryFn in the latter sort of context.  (Despite their somewhat paradoxical flavor, dualist microtheories arguably allow Cyc to mimic commonsense reasoning about geopolitical entities and regions more closely than do the stricter physicalist microtheories.)  There are also some \"generic\" geography microtheories (e.g. #$WorldGeographyMt and #$UnitedStatesGeographyMt) which are neutral with respect to the physical and dualist views.  
<p>
Also see the shared-note for this constant.""" ;
	a <http://sw.cyc.com/2006/07/27/cyc/ArtifactualFeatureType> , <http://sw.cyc.com/2006/07/27/cyc/AtemporalNecessarilyEssentialCollectionType> , <http://sw.cyc.com/2006/07/27/cyc/QAClarifyingCollectionType> , <http://sw.cyc.com/2006/07/27/cyc/OrganizationByEntityType> , <http://sw.cyc.com/2006/07/27/cyc/BBNEntityType> , <http://sw.cyc.com/2006/07/27/cyc/GeopoliticalEntities-Geography-Topic> ;
	<http://sw.cyc.com/2006/07/27/cyc/prettyString-Canonical> "political entity" ;
	<http://sw.cyc.com/2006/07/27/cyc/prettyString> "Domain" , "political geographic region" , "political geographic regions" , "geopolitical entity" , "geopolitical entities" , "demesne" , "demesnes" , "domains" , "political entities" , "land" .

<http://sw.cyc.com/2006/07/27/cyc/AbsoluteGoalSuccess> a <http://sw.cyc.com/2006/07/27/cyc/GoalSituationBySuccessStatus> ;
	<http://sw.cyc.com/2006/07/27/cyc/prettyString-Canonical> "absolute goal success" ;
	<http://www.w3.org/2000/01/rdf-schema#subClassOf> <http://sw.cyc.com/2006/07/27/cyc/MentalSituation> .

<http://sw.cyc.com/2006/07/27/cyc/MentalSituation> <http://www.w3.org/2000/01/rdf-schema#comment> "A specialization of #$Situation. Each instance of #$MentalSituation is a mental situation such as a person seeing the color red, or believing that his enemies control the CIA, or desiring that Fidel Castro shave his beard. An important subcollection of this collection is #$AtLeastPartiallyMentalEvent whice is the collection of mental situations that are events, such as thinking about something or tasting something. Other instances of #$MentalSituation are more \"long-standing\" and stable, and hence also instances of #$StaticSituation, e.g., believing something, or having some goal. Cf. #$MentalSituationFn." ;
	a <http://sw.cyc.com/2006/07/27/cyc/ObjectType> ;
	<http://sw.cyc.com/2006/07/27/cyc/prettyString-Canonical> "mental situation" ;
	<http://sw.cyc.com/2006/07/27/cyc/prettyString> "psychological feature" , "psychological features" , "mental situations" ;
	<http://www.w3.org/2000/01/rdf-schema#subClassOf> <http://sw.cyc.com/2006/07/27/cyc/Situation> ;
	<http://sw.cyc.com/2006/07/27/cyc/quotedIsa> <http://sw.cyc.com/2006/07/27/cyc/WordNetWorkflowConstant-NotFullyReviewed> .

<http://sw.cyc.com/2006/07/27/cyc/GoalSituationBySuccessStatus> <http://www.w3.org/2000/01/rdf-schema#comment> """#$GoalSituationBySuccessStatus is a collection of collections.  Each instance is a collection of #$GoalSituations that share a similar success status.  These instances represent statuses that
can apply to #$GoalSituations to describe whether a given goal is
successful, actively being pursued, relevant to the current state of
affairs etc.""" ;
	a <http://sw.cyc.com/2006/07/27/cyc/AtemporalNecessarilyEssentialCollectionType> , <http://sw.cyc.com/2006/07/27/cyc/CollectionType> ;
	<http://sw.cyc.com/2006/07/27/cyc/prettyString-Canonical> "goal situation by success status" ;
	<http://www.w3.org/2000/01/rdf-schema#subClassOf> <http://www.w3.org/2002/07/owl#Class> .

<http://sw.cyc.com/2006/07/27/cyc/AbsoluteLocationalPredicate> <http://www.w3.org/2000/01/rdf-schema#comment> """A specialization of #$LocationalPredicate (q.v.) instances of which are used to relate spatial things to their locations in space.  Each instance of #$AbsoluteLocationalPredicate is a binary predicate that relates spatial things (including at least some that are not themselves pure space regions) to #$SpaceRegions in which they are (wholly or partly) embedded.  
<p>
By stipulation, the first argument-place of an #$AbsoluteLocationalPredicate is constrained to instances of #$SpatialThing or some specialization thereof, but is <i>not</i> constrained so tightly as to only admit instances of #$SpaceRegion.  Conversely, the second argument-place is constrained to instances of #$SpaceRegion or some specialization thereof.
<p>
Examples of absolute-location predicates include #$exactlyLocatedAt-Spatial, #$partiallyLocatedAt-Spatial, and #$locatedAtPoint-SurfaceGeographical.
<p>
Cf. #$RelativeLocationalPredicate.""" ;
	a <http://sw.cyc.com/2006/07/27/cyc/KEClarifyingCollectionType> , <http://sw.cyc.com/2006/07/27/cyc/PredicateTypeByTopic> ;
	<http://sw.cyc.com/2006/07/27/cyc/prettyString-Canonical> "absolute locational predicate" ;
	<http://sw.cyc.com/2006/07/27/cyc/prettyString> "absolute locational predicates" ;
	<http://www.w3.org/2000/01/rdf-schema#subClassOf> <http://www.w3.org/2000/01/rdf-schema#Property> , <http://sw.cyc.com/2006/07/27/cyc/LocationalPredicate> ;
	<http://www.w3.org/2002/07/owl#disjointWith> <http://sw.cyc.com/2006/07/27/cyc/RelativeLocationalPredicate> .

<http://sw.cyc.com/2006/07/27/cyc/LocationalPredicate> <http://www.w3.org/2000/01/rdf-schema#comment> "A specialization of #$SpatialPredicate whose instances are used to indicate the locations of #$SpatialThings within a particular frame of reference.  #$AbsoluteLocationalPredicates (q.v.) are used to indicate a spatial thing's location by giving a pure #$SpaceRegion in which it is embedded.  #$RelativeLocationalPredicates (q.v.) are used to indicate the relative locations of two or more spatial things with respect to one another." ;
	a <http://sw.cyc.com/2006/07/27/cyc/KEClarifyingCollectionType> , <http://sw.cyc.com/2006/07/27/cyc/PredicateTypeByTopic> ;
	<http://sw.cyc.com/2006/07/27/cyc/prettyString-Canonical> "locational predicate" ;
	<http://www.w3.org/2000/01/rdf-schema#subClassOf> <http://sw.cyc.com/2006/07/27/cyc/SpatialPredicate> .

<http://sw.cyc.com/2006/07/27/cyc/PredicateTypeByTopic> <http://www.w3.org/2000/01/rdf-schema#comment> "#$PredicateTypeByTopic is a specialization of #$PredicateType.  Each instance of #$PredicateTypeByTopic is a collection of predicates each instance of which, when used in an arg0 slot to form a sentence, forms a sentence that is \"about\" some particular sort of thing.  For example, #$PurposePredicate is an instance of #$PredicateTypeByTopic because instances of #$PurposePredicate are used to form sentences about purposes or goals.  Similarly, #$ComparisonPredicates are predicates that are \"about\" how one thing or type of thing compares to another, and so #$ComparisonPredicate is an instance of #$PredicateTypeByTopic." ;
	a <http://sw.cyc.com/2006/07/27/cyc/FacetingCollectionType> , <http://sw.cyc.com/2006/07/27/cyc/SecondOrderCollection> ;
	<http://sw.cyc.com/2006/07/27/cyc/prettyString-Canonical> "predicate type by topic" ;
	<http://www.w3.org/2000/01/rdf-schema#subClassOf> <http://sw.cyc.com/2006/07/27/cyc/CycVocabularyTopic> , <http://sw.cyc.com/2006/07/27/cyc/FacetInstanceCollection> , <http://sw.cyc.com/2006/07/27/cyc/PredicateType> ;
	<http://sw.cyc.com/2006/07/27/cyc/sharedNotes> <http://sw.cyc.com/2006/07/27/cyc/SharedNoteOnGenlsRelationsBetweenFacetingCollectionTypes> ;
	<http://sw.cyc.com/2006/07/27/cyc/typeGenls> <http://sw.cyc.com/2006/07/27/cyc/Predicate> .

<http://sw.cyc.com/2006/07/27/cyc/AbsolutelyFabulous-TheTVShow> a <http://sw.cyc.com/2006/07/27/cyc/Individual> , <http://sw.cyc.com/2006/07/27/cyc/TVSeriesProduct> ;
	<http://sw.cyc.com/2006/07/27/cyc/prettyString-Canonical> "Absolutely Fabulous" .

<http://sw.cyc.com/2006/07/27/cyc/AbsolutePathname> <http://www.w3.org/2000/01/rdf-schema#comment> "#$AbsolutePathname is the collection of computer filesystem pathnames (c.f. #$Pathname) that start at the root directory (e.g. on Unix, these always begin with a slash '/' character)." ;
	a <http://sw.cyc.com/2006/07/27/cyc/IDStringType> ;
	<http://sw.cyc.com/2006/07/27/cyc/prettyString-Canonical> "absolute pathname" ;
	<http://www.w3.org/2000/01/rdf-schema#subClassOf> <http://sw.cyc.com/2006/07/27/cyc/Pathname> .

<http://sw.cyc.com/2006/07/27/cyc/Pathname> <http://www.w3.org/2000/01/rdf-schema#comment> "#$Pathname is the collection of computer filesystem pathnames.  Pathnames are intended to identify directories or files on a given filesystem.  For example, 'file:/cyc/ke/' is a pathname which denotes a directory on the #$Cycorp unix filesystem.  'file:/cyc/ke/temp.txt' is a pathname which denotes a file on the Cycorp unix filesystem.  Similarly, 'file:/cyc/foobar/' is a syntactically legal pathname.  However, because 'file:/cyc/foobar/' is not a directory on the #$Cycorp unix filesystem (well, at least it currently (Jan 2000) isn't), it is not a semantically valid pathname.  The file: is required at the beginning of the name because the browser currently (Sept 2000) will only hotlink to a URL if http: or file: is prepended.  We desire hotlinks for all the uses of #$Pathname in the system currently.  If the universality of this desire lessens, perhaps someday we will want 'HotlinkedPathname' and 'NotHotlinkedPathname'.  #$salientCycorpPathname and relata should have hotlinked pathnames." ;
	a <http://sw.cyc.com/2006/07/27/cyc/IDStringType> , <http://sw.cyc.com/2006/07/27/cyc/FileManagement-Topic> ;
	<http://sw.cyc.com/2006/07/27/cyc/prettyString-Canonical> "pathname" ;
	<http://sw.cyc.com/2006/07/27/cyc/prettyString> "pathnames" ;
	<http://www.w3.org/2000/01/rdf-schema#subClassOf> <http://sw.cyc.com/2006/07/27/cyc/CycLConstant> , <http://sw.cyc.com/2006/07/27/cyc/ComputerNetworkContactInfoString> .

<http://sw.cyc.com/2006/07/27/cyc/IDStringType> <http://www.w3.org/2000/01/rdf-schema#comment> "A collection of collections and a specialization of #$ObjectType.  Each instance of #$IDStringType is a collection of character strings which is a specialization of #$IDString (q.v.).  A few notable instances of #$IDStringType are #$ProductName, #$ProductVersion, #$EMailAddress, #$PhoneNumber, #$PostalCode." ;
	a <http://sw.cyc.com/2006/07/27/cyc/AtemporalNecessarilyEssentialCollectionType> , <http://sw.cyc.com/2006/07/27/cyc/FacetingCollectionType> , <http://sw.cyc.com/2006/07/27/cyc/SecondOrderCollection> , <http://sw.cyc.com/2006/07/27/cyc/Addresses-Geography-Topic> , <http://sw.cyc.com/2006/07/27/cyc/CharacterStringRelatedConstants-Db-Topic> ;
	<http://sw.cyc.com/2006/07/27/cyc/prettyString-Canonical> "type of ID string" ;
	<http://sw.cyc.com/2006/07/27/cyc/prettyString> "ID string type" , "ID string types" , "types of ID string" ;
	<http://www.w3.org/2000/01/rdf-schema#subClassOf> <http://sw.cyc.com/2006/07/27/cyc/ObjectType> , <http://sw.cyc.com/2006/07/27/cyc/CharacterStringType> ;
	<http://www.w3.org/2002/07/owl#disjointWith> <http://sw.cyc.com/2006/07/27/cyc/MicrotheoryType> , <http://sw.cyc.com/2006/07/27/cyc/TemporalStuffType> , <http://sw.cyc.com/2006/07/27/cyc/SpatialThingTypeByShape> , <http://sw.cyc.com/2006/07/27/cyc/MatterTypeByPhysicalState> ;
	<http://sw.cyc.com/2006/07/27/cyc/typeGenls> <http://sw.cyc.com/2006/07/27/cyc/IDString> .

<http://sw.cyc.com/2006/07/27/cyc/AbsolutePower-TheMovie> a <http://sw.cyc.com/2006/07/27/cyc/Individual> , <http://sw.cyc.com/2006/07/27/cyc/ThrillerMovie> ;
	<http://sw.cyc.com/2006/07/27/cyc/prettyString-Canonical> "Absolute Power" .

<http://sw.cyc.com/2006/07/27/cyc/ThrillerMovie> <http://www.w3.org/2000/01/rdf-schema#comment> "#$ThrillerMovie is a collection of instances of #$Movie-CW, each of which relates a thrilling story." ;
	a <http://sw.cyc.com/2006/07/27/cyc/MovieTypeByGenre> ;
	<http://sw.cyc.com/2006/07/27/cyc/prettyString-Canonical> "thriller movie" ;
	<http://sw.cyc.com/2006/07/27/cyc/prettyString> "thriller movies" ;
	<http://www.w3.org/2000/01/rdf-schema#subClassOf> <http://sw.cyc.com/2006/07/27/cyc/Movie-CW> , <http://sw.cyc.com/2006/07/27/cyc/PropositionalConceptualWork-ThrillerGenre> .

<http://sw.cyc.com/2006/07/27/cyc/ScalarInterval> <http://www.w3.org/2000/01/rdf-schema#comment> """A specialization of #$TupleOfIntervals (q.v.).  Roughly put, this is the collection of all things that can be ranked according to some one-dimensional scale.  Instances of #$ScalarInterval are numbers or quantities possessing only sign and magnitude.  They are construed as <i>one-tuples</i> (see #$Tuple) of intervals.  They are to be contrasted with #$VectorIntervals (q.v.), which possess a direction as well as a magnitude, and are construed as two-membered tuples of intervals.
<p>
#$ScalarInterval is partitioned into the two collections #$NumericInterval (which is the collection of numbers and number-ranges of all kinds) and #$Quantity (qq.v).  A #$Quantity is usually specified with a numeric-interval, as with (#$Meter 3)), but it might also be given in a generically-ranked way, as with (#$HighAmountFn #$Happiness); see the specializations #$MeasurableQuantity and #$NonNumericQuantity.  The magnitude of a scalar might be given by a specific number (see #$ScalarPointValue) or by a proper range of numbers (see #$ScalarProperInterval).
<p>
Note that the instances of #$MathematicalFunctionOnScalars (q.v.), which include artithmetic functions such as addition (see #$PlusFn) and division (see #$QuotientFn), are defined broadly so as to apply not only to numbers, but to (numerically-measured) scalar intervals generally.  Thus (#$PlusFn (#$Meter 3) (#$Meter 5)) is equal to (#$Meter 8).""" ;
	a <http://www.w3.org/2002/07/owl#Class> , <http://sw.cyc.com/2006/07/27/cyc/ObjectType> , <http://sw.cyc.com/2006/07/27/cyc/AtemporalNecessarilyEssentialCollectionType> , <http://sw.cyc.com/2006/07/27/cyc/ScalarIntervals-Quantity-Topic> , <http://sw.cyc.com/2006/07/27/cyc/TestOWLExportConcept> , <http://sw.cyc.com/2006/07/27/cyc/SubsetsOfMathematicalThing-Math-Topic> ;
	<http://sw.cyc.com/2006/07/27/cyc/prettyString-Canonical> "QUANTITY" ;
	<http://sw.cyc.com/2006/07/27/cyc/prettyString> "quantum" , "quantums" , "amount" , "amounts" , "quantities" ;
	<http://www.w3.org/2000/01/rdf-schema#subClassOf> <http://sw.cyc.com/2006/07/27/cyc/Container-Underspecified> , <http://sw.cyc.com/2006/07/27/cyc/ScalarOrVectorInterval> ;
	<http://sw.cyc.com/2006/07/27/cyc/sharedNotes> <http://sw.cyc.com/2006/07/27/cyc/SharedNoteAboutScalarIntervalArithmetic> ;
	<http://www.w3.org/2002/07/owl#disjointWith> <http://sw.cyc.com/2006/07/27/cyc/VectorInterval> , <http://sw.cyc.com/2006/07/27/cyc/Path-Generic> , <http://sw.cyc.com/2006/07/27/cyc/Proposition> ;
	<http://sw.cyc.com/2006/07/27/cyc/collectionConventionMt> <http://sw.cyc.com/2006/07/27/cyc/UniversalVocabularyMt> .

<http://sw.cyc.com/2006/07/27/cyc/UnitOfMeasureConcept> <http://www.w3.org/2000/01/rdf-schema#comment> "A #$ConceptTypeByDomain (q.v.).  Instances of #$UnitOfMeasureConcept are collections and relations having to do with unit of measurement functions and the kinds of quantities they return as values.  Important specializations and instances of #$UnitOfMeasure, major specializations or #$ScalarInterval, and relations that are important to measurement theory are instances of this collection." ;
	a <http://sw.cyc.com/2006/07/27/cyc/ConceptTypeByDomain> ;
	<http://sw.cyc.com/2006/07/27/cyc/prettyString-Canonical> "unit of measure concept" ;
	<http://sw.cyc.com/2006/07/27/cyc/prettyString> "the unit of measure domain" , "unit of measure concepts" ;
	<http://www.w3.org/2000/01/rdf-schema#subClassOf> <http://www.w3.org/2002/07/owl#Thing> .

<http://sw.cyc.com/2006/07/27/cyc/SKSISupportedFunction> <http://www.w3.org/2000/01/rdf-schema#comment> """This is the collection of evaluatable functions which are
supported by SKSI in the sense that they are translatable to their SQL
equivalents.""" ;
	a <http://sw.cyc.com/2006/07/27/cyc/NonAbducibleCollection> , <http://sw.cyc.com/2006/07/27/cyc/FunctionType> ;
	<http://sw.cyc.com/2006/07/27/cyc/prettyString-Canonical> "SKSI supported function" ;
	<http://www.w3.org/2000/01/rdf-schema#subClassOf> <http://sw.cyc.com/2006/07/27/cyc/Function-Denotational> , <http://sw.cyc.com/2006/07/27/cyc/SKSISupportedOperator> ;
	<http://www.w3.org/2002/07/owl#disjointWith> <http://sw.cyc.com/2006/07/27/cyc/SKSISupportedComparisonPredicate> .

<http://sw.cyc.com/2006/07/27/cyc/MathematicalFunctionOnScalars> <http://www.w3.org/2000/01/rdf-schema#comment> """A specialization of #$ScalarDenotingFunction (q.v.).  Each instance of #$MathematicalFunctionOnScalars is a function that takes one or more #$ScalarIntervals (q.v.) as its argument(s), and returns a scalar interval as its value.
<p>
Most currently-reified instances of #$MathematicalFunctionOnScalars are applicable both to pure numbers (see #$NumericInterval) and to quantities (see esp. #$MeasurableQuantity).  For example, #$PlusFn can be used to add real numbers together and to add distances together.  But some mathematical functions on scalars (e.g. #$ExponentFn and #$LogFn) are defined only for numeric-intervals. And some (e.g. some #$TrigonometricFunctions) take numbers as arguments and return
quantities, or vice versa.
<p>
Other instances of this collection include #$TimesFn, #$SineFn and #$AbsoluteValueFn.""" ;
	a <http://sw.cyc.com/2006/07/27/cyc/ArithmeticFunctions-Math-Topic> , <http://sw.cyc.com/2006/07/27/cyc/FunctionType> ;
	<http://sw.cyc.com/2006/07/27/cyc/prettyString-Canonical> "function from quantities to quantities" ;
	<http://sw.cyc.com/2006/07/27/cyc/prettyString> "functions from quantities to quantities" ;
	<http://www.w3.org/2000/01/rdf-schema#subClassOf> <http://sw.cyc.com/2006/07/27/cyc/EvaluatableFunction> , <http://sw.cyc.com/2006/07/27/cyc/ScalarDenotingFunction> ;
	<http://www.w3.org/2002/07/owl#disjointWith> <http://sw.cyc.com/2006/07/27/cyc/DateDenotingFunction> .

<http://sw.cyc.com/2006/07/27/cyc/ArithmeticFunctions-Math-Topic> a <http://sw.cyc.com/2006/07/27/cyc/KBDependentCollection> , <http://sw.cyc.com/2006/07/27/cyc/CycVocabularyTopic> ;
	<http://sw.cyc.com/2006/07/27/cyc/prettyString-Canonical> "arithmetic functions math topic" ;
	<http://www.w3.org/2000/01/rdf-schema#subClassOf> <http://sw.cyc.com/2006/07/27/cyc/Math-Topic> .

<http://sw.cyc.com/2006/07/27/cyc/oldConstantName> <http://www.w3.org/2000/01/rdf-schema#comment> """This bookkeeping predicate relates a CycL constant to a former \"name\" of that constant.  More accurately, (#$oldConstantName CONSTANT STRING) means that the underlying data structure currently associated with the CycL expression CONSTANT was formerly associated instead with the SubL string STRING.  If CONSTANT has undergone multiple \"renames\", STRING will 
normally be its most recent former \"name\".  While #$oldConstantName sentences 
can be asserted and edited by hand, they are asserted automatically when a Rename is done in the Knowledge Base.""" ;
	a <http://www.w3.org/2000/01/rdf-schema#Property> , <http://sw.cyc.com/2006/07/27/cyc/MetaKnowledgePredicate> , <http://sw.cyc.com/2006/07/27/cyc/BookkeepingPredicate> , <http://sw.cyc.com/2006/07/27/cyc/DocumentationPredicate> , <http://sw.cyc.com/2006/07/27/cyc/BookkeepingPredicateForAnyThing> , <http://sw.cyc.com/2006/07/27/cyc/Doc-Topic> ;
	<http://sw.cyc.com/2006/07/27/cyc/prettyString-Canonical> "Old Constant Name" ;
	<http://sw.cyc.com/2006/07/27/cyc/arity> "2"^^<http://www.w3.org/2001/XMLSchema#long> ;
	<http://sw.cyc.com/2006/07/27/cyc/arg1QuotedIsa> <http://sw.cyc.com/2006/07/27/cyc/CycLConstant> ;
	<http://sw.cyc.com/2006/07/27/cyc/arg2QuotedIsa> <http://www.w3.org/2001/XMLSchema#string> ;
	<http://sw.cyc.com/2006/07/27/cyc/quotedArgument> "2"^^<http://www.w3.org/2001/XMLSchema#long> , "1"^^<http://www.w3.org/2001/XMLSchema#long> ;
	<http://sw.cyc.com/2006/07/27/cyc/definingMt> <http://sw.cyc.com/2006/07/27/cyc/BookkeepingMt> .

<http://sw.cyc.com/2006/07/27/cyc/NonNegativeScalarInterval> <http://www.w3.org/2000/01/rdf-schema#comment> "A specialization of #$ScalarInterval.  An instance INTERVAL of #$ScalarInterval is also an instance of #$NonNegativeScalarInterval just in case INTERVAL is a non-negative number or quantity.  Instances of #$NonNegativeScalarInterval include all instances of #$NonNegativeNumber (q.v.), as well as non-negative quantities such as (#$Meter 212), (#$Kilogram 5), and (#$SecondsDuration 0)." ;
	a <http://www.w3.org/2002/07/owl#Class> , <http://sw.cyc.com/2006/07/27/cyc/FirstOrderCollection> , <http://sw.cyc.com/2006/07/27/cyc/AtemporalNecessarilyEssentialCollectionType> ;
	<http://sw.cyc.com/2006/07/27/cyc/prettyString-Canonical> "non-negative quantity or number" ;
	<http://sw.cyc.com/2006/07/27/cyc/prettyString> "quantity or number greater than or equal to zero" .

<http://sw.cyc.com/2006/07/27/cyc/AbsorptionEvent> a <http://sw.cyc.com/2006/07/27/cyc/TemporalObjectType> , <http://sw.cyc.com/2006/07/27/cyc/TemporalStuffType> ;
	<http://sw.cyc.com/2006/07/27/cyc/prettyString-Canonical> "absorption" ;
	<http://sw.cyc.com/2006/07/27/cyc/prettyString> "absorb" , "absorbed" , "absorbs" , "absorbing" , "have absorbed" , "has absorbed" , "had absorbed" , "will have absorbed" , "taking in" , "take in" , "took in" , "taken in" , "takes in" , "have taken in" , "has taken in" , "will take in" , "had taken in" , "will have taken in" , "Will Absorb" ;
	<http://www.w3.org/2000/01/rdf-schema#subClassOf> <http://sw.cyc.com/2006/07/27/cyc/FluidFlow-Complete> , <http://sw.cyc.com/2006/07/27/cyc/FluidFlow-Translation> , <http://sw.cyc.com/2006/07/27/cyc/TransferIn> ;
	<http://sw.cyc.com/2006/07/27/cyc/quotedIsa> <http://sw.cyc.com/2006/07/27/cyc/WordNetWorkflowConstant-NotFullyReviewed> ;
	<http://www.w3.org/2002/07/owl#disjointWith> <http://sw.cyc.com/2006/07/27/cyc/ConsciousActivity> .

<http://sw.cyc.com/2006/07/27/cyc/ConsciousActivity> <http://www.w3.org/2000/01/rdf-schema#comment> "This is the collection of all activities which are performed in a state of consciousness, that is, the animal performing the action is not sleeping, in a coma, or otherwise unconscious." ;
	a <http://sw.cyc.com/2006/07/27/cyc/AnimalCapabilityType> ;
	<http://sw.cyc.com/2006/07/27/cyc/prettyString-Canonical> "conscious activity" ;
	<http://sw.cyc.com/2006/07/27/cyc/prettyString> "conscious activities" ;
	<http://www.w3.org/2000/01/rdf-schema#subClassOf> <http://sw.cyc.com/2006/07/27/cyc/AtLeastPartiallyMentalEvent> ;
	<http://www.w3.org/2002/07/owl#disjointWith> <http://sw.cyc.com/2006/07/27/cyc/StateOfUnconsciousness> .

<http://sw.cyc.com/2006/07/27/cyc/FluidFlow-Complete> <http://www.w3.org/2000/01/rdf-schema#comment> "Instances of #$FluidFlow-Complete represent the motion of a piece of fluid from being entirely `at' (see #$objectFoundInLocation) the #$fromLocation to entirely `at' the #$toLocation.  Thus when we say, `The river flowed from West Egg to East Egg' we don't mean the same thing as `The entire river left West Egg and went to East Egg'.  Therefore, #$FluidFlow-Complete is not the correct motion event to use.  Instead, #$FluidFlow-Translation is.  However, if we wish to say, `Joe pumped all the water out of the bilge and into the ocean' we do mean the same thing that #$FluidFlow-Complete entails." ;
	a <http://sw.cyc.com/2006/07/27/cyc/TemporalStuffType> ;
	<http://sw.cyc.com/2006/07/27/cyc/prettyString-Canonical> "conducting" ;
	<http://sw.cyc.com/2006/07/27/cyc/prettyString> "conduct" , "conducted" , "conducts" , "have conducted" , "has conducted" , "will conduct" , "had conducted" , "will have conducted" ;
	<http://www.w3.org/2000/01/rdf-schema#subClassOf> <http://sw.cyc.com/2006/07/27/cyc/FluidFlow-Translation> , <http://sw.cyc.com/2006/07/27/cyc/Translation-Complete> .

<http://sw.cyc.com/2006/07/27/cyc/FluidFlow-Translation> <http://www.w3.org/2000/01/rdf-schema#comment> """A specialization of both #$FluidFlowEvent and #$Movement-TranslationEvent (qq.v.). In each instance of #$FluidFlow-Translation, the moving object (see the predicate #$objectMoving) is an instance of #$FluidTangibleThing (i.e. a portion of some fluid, such as a quart of milk) rather than a discrete solid object.  At least some of the moving object leaves its original position (see the predicate #$fromLocation) and some arrives at the destination (see the predicate #$toLocation), but it is not necessary that all of the moving object go from the origin to the destination.  Instances of #$FluidFlow-Translation include rivers flowing or winds blowing or air filling one's lungs when one takes a breath.  Other instances of #$FluidFlow-Translation include flows of #$GranularFluids (q.v.), such as sand or drifting snow, that are 
composed of multiple solid particles.""" ;
	a <http://sw.cyc.com/2006/07/27/cyc/ProcessType> , <http://sw.cyc.com/2006/07/27/cyc/CumulativeEventType> .

<http://sw.cyc.com/2006/07/27/cyc/Abstinence> <http://sw.cyc.com/2006/07/27/cyc/quotedIsa> <http://sw.cyc.com/2006/07/27/cyc/StubTerm> .

<http://sw.cyc.com/2006/07/27/cyc/Inaction> a <http://www.w3.org/2002/07/owl#Class> , <http://sw.cyc.com/2006/07/27/cyc/FirstOrderCollection> ;
	<http://sw.cyc.com/2006/07/27/cyc/prettyString-Canonical> "inaction" ;
	<http://www.w3.org/2000/01/rdf-schema#subClassOf> <http://sw.cyc.com/2006/07/27/cyc/Situation> ;
	<http://sw.cyc.com/2006/07/27/cyc/quotedIsa> <http://sw.cyc.com/2006/07/27/cyc/StubTerm> .

<http://sw.cyc.com/2006/07/27/cyc/AbstractIndividual> <http://www.w3.org/2000/01/rdf-schema#comment> "A specialization of #$AbstractThing and #$IntangibleIndividual (q.v.).  This is the collection of all abstract (i.e. aspatial, atemporal) individuals.  Specializations of #$AbstractIndividual include #$Relation, #$Tuple, and #$AbstractStructure." ;
	a <http://sw.cyc.com/2006/07/27/cyc/FirstOrderCollection> , <http://sw.cyc.com/2006/07/27/cyc/AtemporalNecessarilyEssentialCollectionType> ;
	<http://sw.cyc.com/2006/07/27/cyc/prettyString-Canonical> "abstract individual" ;
	<http://sw.cyc.com/2006/07/27/cyc/prettyString> "abstract individuals" , "individual that has been also abstract thing" , "item that has been also abstract thing" , "items that has been also abstract thing" , "piece that has been also abstract thing" , "pieces that has been also abstract thing" , "article that has been also abstract thing" , "element that has been also abstract thing" , "articles that has been also abstract thing" , "elements that has been also abstract thing" , "individuals that has been also abstract thing" , "individual object that has been also abstract thing" , "individual that is also abstract thing" , "item that is also abstract thing" , "items that is also abstract thing" , "piece that is also abstract thing" , "pieces that is also abstract thing" , "article that is also abstract thing" , "element that is also abstract thing" , "articles that is also abstract thing" , "elements that is also abstract thing" , "individuals that is also abstract thing" , "individual object that is also abstract thing" ;
	<http://www.w3.org/2000/01/rdf-schema#subClassOf> <http://sw.cyc.com/2006/07/27/cyc/IntangibleIndividual> , <http://sw.cyc.com/2006/07/27/cyc/AbstractThing> .

<http://sw.cyc.com/2006/07/27/cyc/AbstractThing> <http://www.w3.org/2000/01/rdf-schema#comment> "A specialization of both #$AtemporalThing and #$AspatialThing (qq.v.).  The collection of things that are \"abstract\", in the sense of having neither temporal nor spatial extent or location.  Specializations of #$AbstractThing include #$SetOrCollection, #$Number-General, #$Relation, and #$Proposition (qq.v.).  Note that a set or collection is considered an abstract thing even if its elements are not abstract." ;
	a <http://sw.cyc.com/2006/07/27/cyc/AtemporalNecessarilyEssentialCollectionType> , <http://sw.cyc.com/2006/07/27/cyc/VariedOrderCollection> ;
	<http://sw.cyc.com/2006/07/27/cyc/prettyString-Canonical> "abstract thing" ;
	<http://www.w3.org/2000/01/rdf-schema#subClassOf> <http://sw.cyc.com/2006/07/27/cyc/AtemporalThing> , <http://sw.cyc.com/2006/07/27/cyc/AspatialThing> .

<http://sw.cyc.com/2006/07/27/cyc/abstractInfoAbout> <http://www.w3.org/2000/01/rdf-schema#comment> "(#$abstractInfoAbout INFO TERM) means that the #$AspatialInformationStore INFO contains information about TERM.  The information does not *necessarily* have propositional content; a picture may convey abstract information concerning the way someone looks, but 'the way someone looks' need not be expressible propositionally." ;
	a <http://www.w3.org/2000/01/rdf-schema#Property> ;
	<http://sw.cyc.com/2006/07/27/cyc/prettyString-Canonical> "Abstract Info About" ;
	<http://www.w3.org/2000/01/rdf-schema#domain> <http://sw.cyc.com/2006/07/27/cyc/AspatialInformationStore> ;
	<http://sw.cyc.com/2006/07/27/cyc/arity> "2"^^<http://www.w3.org/2001/XMLSchema#long> ;
	<http://www.w3.org/2000/01/rdf-schema#range> <http://www.w3.org/2002/07/owl#Thing> .

<http://sw.cyc.com/2006/07/27/cyc/AbstractInformationStructure> <http://www.w3.org/2000/01/rdf-schema#comment> "A specialization of #$AbstractStructure.  Each instance of #$AbstractInformationStructure is an abstract individual comprising abstract symbols and relations between them. Important specializations of this collection include #$CharacterString and #$Sentence. #$AbstractInformationStructure also includes abstract diagrams, graphs, and bit strings. The collection can be more precisely defined as follows: Each #$AbstractInformationStructure is such that each of its physical instantiations (see #$instantiationOfAIS) consists of instantiations of instances of #$AtomicSymbol-Abstract, arranged in a certain way. For example, the abstract sentence 'The pig flies' is an #$AbstractInformationStructure. Each written instantiation of it consists of an instantiation of the words (symbols) 'The', 'pig' and 'flies', written in that order. (If the #$AbstractInformationStructure 'The pig flies' were spoken, the same words would appear in the same order, i.e. 'The' first, etc., but the sequence would be determined by the arrangement of the spoken words in time, rather than space.) Likewise with abstract diagrams, graphs, etc. Each of these is such that its physical instantiations consist of arrangements of instantiations of instances of #$AtomicSymbol-Abstract. A hard copy of a wiring diagram consists of a group of concrete symbols representing various circuit components, in which these symbols are spatially arranged in a certain in way. The arrangement of the concrete symbols in an instantiation of an #$AbstractInformationStructure is not always a simple matter of arrangement in space or time. The sequence of symbols '0010010111011001' can be instantiated in written, spoken, or electronic forms. In the last case, the order of the symbols is determined by conventions concerning the electronic medium in which it is stored, rather than by any common criterion for precedence or subsequence in space or time." ;
	a <http://sw.cyc.com/2006/07/27/cyc/FirstOrderCollection> ;
	<http://sw.cyc.com/2006/07/27/cyc/prettyString-Canonical> "AIS" ;
	<http://www.w3.org/2000/01/rdf-schema#subClassOf> <http://sw.cyc.com/2006/07/27/cyc/AbstractStructure> ;
	<http://sw.cyc.com/2006/07/27/cyc/quotedIsa> <http://sw.cyc.com/2006/07/27/cyc/DocumentStructureRepresentationConstant> .

<http://sw.cyc.com/2006/07/27/cyc/AbstractStructure> <http://www.w3.org/2000/01/rdf-schema#comment> "This collection was reified prior to completing its basic representation in order to facilitate the loading of files on which it depends." ;
	a <http://sw.cyc.com/2006/07/27/cyc/FirstOrderCollection> ;
	<http://www.w3.org/2000/01/rdf-schema#subClassOf> <http://sw.cyc.com/2006/07/27/cyc/AspatialInformationStore> , <http://sw.cyc.com/2006/07/27/cyc/AbstractIndividual> ;
	<http://sw.cyc.com/2006/07/27/cyc/quotedIsa> <http://sw.cyc.com/2006/07/27/cyc/DocumentStructureRepresentationConstant> .

<http://sw.cyc.com/2006/07/27/cyc/DocumentStructureRepresentationConstant> <http://www.w3.org/2000/01/rdf-schema#comment> "The collection of instances of #$CycLConstant used to represent the structure of documents." ;
	a <http://sw.cyc.com/2006/07/27/cyc/NonAbducibleCollection> , <http://sw.cyc.com/2006/07/27/cyc/KBDependentCollection> , <http://sw.cyc.com/2006/07/27/cyc/TextLearnerConstantTypeByFunctionalArea> ;
	<http://sw.cyc.com/2006/07/27/cyc/prettyString-Canonical> "document structure representation constant" ;
	<http://www.w3.org/2000/01/rdf-schema#subClassOf> <http://sw.cyc.com/2006/07/27/cyc/CycLConstant> .

<http://sw.cyc.com/2006/07/27/cyc/AbstractLexiconSpecification> <http://www.w3.org/2000/01/rdf-schema#comment> "The base class from which all useful lexicons are derived.  Because it is an abstract class, it should not be expected to be fully functional, and should not be used in applications, except for inheritance purposes." ;
	a <http://sw.cyc.com/2006/07/27/cyc/ObjectType> , <http://sw.cyc.com/2006/07/27/cyc/TemporalStuffType> ;
	<http://sw.cyc.com/2006/07/27/cyc/prettyString-Canonical> "abstract lexicon specification" ;
	<http://www.w3.org/2000/01/rdf-schema#subClassOf> <http://sw.cyc.com/2006/07/27/cyc/Individual> , <http://sw.cyc.com/2006/07/27/cyc/NormativeSpecification> .

<http://sw.cyc.com/2006/07/27/cyc/NormativeSpecification> <http://www.w3.org/2000/01/rdf-schema#comment> "The common sub-collection of both #$Specification and #$Criterion.  Each instyance of #$NormativeSpecification is a conceptual work that describes how something should be.  The instances can refer to instances or whole sub-collections of #$Situation or #$SomethingExisting.  Thus, the conceptual work associated with an instance of #$Blueprint is an instance of #$NormativeSpecification because it describes what the properties of the resultant building should be.  Familiar specializations of #$NormativeSpecification include #$Agreement, #$Obligation, and #$Instructions." ;
	a <http://sw.cyc.com/2006/07/27/cyc/ObjectType> ;
	<http://sw.cyc.com/2006/07/27/cyc/prettyString-Canonical> "plan" ;
	<http://sw.cyc.com/2006/07/27/cyc/prettyString> "plans" , "Designs" , "design" , "norms" , "Norm" ;
	<http://www.w3.org/2000/01/rdf-schema#subClassOf> <http://sw.cyc.com/2006/07/27/cyc/Specification> , <http://sw.cyc.com/2006/07/27/cyc/Criterion> ;
	<http://sw.cyc.com/2006/07/27/cyc/quotedIsa> <http://sw.cyc.com/2006/07/27/cyc/AssignmentOntologyConstant> ;
	<http://sw.cyc.com/2006/07/27/cyc/facets-Covering> <http://sw.cyc.com/2006/07/27/cyc/NormativeSpecificationTypeBySatisfactionMethod> .

<http://sw.cyc.com/2006/07/27/cyc/AbstractNounProducingSuffix> <http://www.w3.org/2000/01/rdf-schema#comment> "The collection of suffixes which serve to convert words into abstract nouns. These are generally #$MassNouns. Example: #$Friend-TheWord + #$Ship-TheSuffix = #$Friendship-TheWord." ;
	a <http://sw.cyc.com/2006/07/27/cyc/NLMorphologyCollection> , <http://sw.cyc.com/2006/07/27/cyc/SuffixCategory> , <http://sw.cyc.com/2006/07/27/cyc/LinguisticObjectType> ;
	<http://sw.cyc.com/2006/07/27/cyc/prettyString-Canonical> "abstract-noun-creating suffix" ;
	<http://sw.cyc.com/2006/07/27/cyc/prettyString> "abstract-noun-creating suffixes" ;
	<http://www.w3.org/2000/01/rdf-schema#subClassOf> <http://sw.cyc.com/2006/07/27/cyc/NounProducingSuffix> ;
	<http://sw.cyc.com/2006/07/27/cyc/quotedIsa> <http://sw.cyc.com/2006/07/27/cyc/NLTerm> , <http://sw.cyc.com/2006/07/27/cyc/NLMorphologyTerm> .

<http://sw.cyc.com/2006/07/27/cyc/NounProducingSuffix> <http://www.w3.org/2000/01/rdf-schema#comment> "The collection of suffixes which serve to convert words into #$Nouns. Example: #$Friend-TheWord + #$Ship-TheSuffix = #$Friendship-TheWord." ;
	a <http://sw.cyc.com/2006/07/27/cyc/NLMorphologyCollection> , <http://sw.cyc.com/2006/07/27/cyc/SuffixCategory> , <http://sw.cyc.com/2006/07/27/cyc/LinguisticObjectType> ;
	<http://sw.cyc.com/2006/07/27/cyc/prettyString-Canonical> "noun-creating suffix" ;
	<http://sw.cyc.com/2006/07/27/cyc/prettyString> "noun-creating suffixes" ;
	<http://www.w3.org/2000/01/rdf-schema#subClassOf> <http://sw.cyc.com/2006/07/27/cyc/DerivationalSuffix> , <http://sw.cyc.com/2006/07/27/cyc/NounProducingAffix> ;
	<http://sw.cyc.com/2006/07/27/cyc/quotedIsa> <http://sw.cyc.com/2006/07/27/cyc/NLTerm> , <http://sw.cyc.com/2006/07/27/cyc/NLMorphologyTerm> .

<http://sw.cyc.com/2006/07/27/cyc/NLMorphologyCollection> <http://www.w3.org/2000/01/rdf-schema#comment> "The collection of #$NLCollections used in representing NL morphology." ;
	a <http://www.w3.org/2002/07/owl#Class> , <http://sw.cyc.com/2006/07/27/cyc/AtemporalNecessarilyEssentialCollectionType> .

<http://sw.cyc.com/2006/07/27/cyc/AbuAyoubAlIraqi> a <http://sw.cyc.com/2006/07/27/cyc/Individual> , <http://sw.cyc.com/2006/07/27/cyc/AdultMaleHuman> , <http://sw.cyc.com/2006/07/27/cyc/Leader> , <http://sw.cyc.com/2006/07/27/cyc/IraqiPerson> ;
	<http://sw.cyc.com/2006/07/27/cyc/prettyString-Canonical> "Abu Ayou al-Iraqi" .

<http://sw.cyc.com/2006/07/27/cyc/IraqiPerson> <http://www.w3.org/2000/01/rdf-schema#comment> "The collection of people who are #$citizens of #$Iraq, or participate in its #$NationalCulture." ;
	a <http://sw.cyc.com/2006/07/27/cyc/NationalityGroupsInTheRegion-HormuzArea-Topic> , <http://sw.cyc.com/2006/07/27/cyc/TKBNationalityList> , <http://sw.cyc.com/2006/07/27/cyc/PersonTypeByGeoPoliticalAffiliation> , <http://sw.cyc.com/2006/07/27/cyc/PersonTypeByNationality> ;
	<http://sw.cyc.com/2006/07/27/cyc/prettyString-Canonical> "Iraqi" ;
	<http://sw.cyc.com/2006/07/27/cyc/prettyString> "Iraqi person" , "Iraqi people" , "Iraqi persons" , "Iraqis" ;
	<http://www.w3.org/2000/01/rdf-schema#subClassOf> <http://sw.cyc.com/2006/07/27/cyc/Person> , <http://sw.cyc.com/2006/07/27/cyc/AsianCitizenOrSubject> .

<http://sw.cyc.com/2006/07/27/cyc/AbuBakrAlSadeekCamp> <http://www.w3.org/2000/01/rdf-schema#comment> """A camp in Khost, Afghanistan. AlFadl stayed there for 
two weeks to be trained in running traing camps.""" ;
	a <http://sw.cyc.com/2006/07/27/cyc/Individual> , <http://sw.cyc.com/2006/07/27/cyc/TrainingCamp> , <http://sw.cyc.com/2006/07/27/cyc/ShelterConstruction> ;
	<http://sw.cyc.com/2006/07/27/cyc/prettyString-Canonical> "the Abu Bakr al Sadeek Camp" ;
	<http://sw.cyc.com/2006/07/27/cyc/prettyString> "Abu Bakr al Sadeek camp" , "Abu Bakr al Sadeek" .

<http://sw.cyc.com/2006/07/27/cyc/TrainingCamp> <http://www.w3.org/2000/01/rdf-schema#comment> "The collection of encampments used primarily for training." ;
	a <http://sw.cyc.com/2006/07/27/cyc/ExistingObjectType> , <http://sw.cyc.com/2006/07/27/cyc/SpatiallyDisjointObjectType> , <http://sw.cyc.com/2006/07/27/cyc/ArtifactualFeatureType> ;
	<http://sw.cyc.com/2006/07/27/cyc/prettyString-Canonical> "training camp" ;
	<http://sw.cyc.com/2006/07/27/cyc/prettyString> "training camps" ;
	<http://www.w3.org/2000/01/rdf-schema#subClassOf> <http://sw.cyc.com/2006/07/27/cyc/GroundsOfOrganization> , <http://sw.cyc.com/2006/07/27/cyc/HumanlyOccupiedSpatialObject> , <http://sw.cyc.com/2006/07/27/cyc/Facility-Generic> .

<http://sw.cyc.com/2006/07/27/cyc/ShelterConstruction> <http://www.w3.org/2000/01/rdf-schema#comment> "A specialization of #$ConstructionArtifact.  Each instance of #$ShelterConstruction is an artifact built by some agent, including but not limited to humans, and intended for use as a shelter.  Instances of #$ShelterConstruction include bird nests, termite mounds, beaver dams, the #$SydneyOperaHouse, the #$PalaceOfFineArts-SanFrancisco, and the #$NewYorkHiltonAtBroadway." ;
	a <http://sw.cyc.com/2006/07/27/cyc/ExistingObjectType> , <http://sw.cyc.com/2006/07/27/cyc/SpatiallyDisjointObjectType> , <http://sw.cyc.com/2006/07/27/cyc/Construction-Topic> ;
	<http://sw.cyc.com/2006/07/27/cyc/prettyString-Canonical> "shelter" ;
	<http://sw.cyc.com/2006/07/27/cyc/prettyString> "dugout" , "dugouts" , "habitation" , "habitations" , "sanctuary" , "sanctuaries" , "refuge" , "refuges" , "shelters" ;
	<http://www.w3.org/2000/01/rdf-schema#subClassOf> <http://sw.cyc.com/2006/07/27/cyc/ConstructionArtifact> , <http://sw.cyc.com/2006/07/27/cyc/Facility-Generic> , <http://sw.cyc.com/2006/07/27/cyc/ShelteringArtifact> ;
	<http://www.w3.org/2002/07/owl#disjointWith> <http://sw.cyc.com/2006/07/27/cyc/Weapon> , <http://sw.cyc.com/2006/07/27/cyc/CornerOnObject> , <http://sw.cyc.com/2006/07/27/cyc/Dock> , <http://sw.cyc.com/2006/07/27/cyc/PathArtifactSystem> , <http://sw.cyc.com/2006/07/27/cyc/TopographicalFeature> , <http://sw.cyc.com/2006/07/27/cyc/OutdoorRecreationArea> , <http://sw.cyc.com/2006/07/27/cyc/Shipyard> , <http://sw.cyc.com/2006/07/27/cyc/MeasuringDevice> , <http://sw.cyc.com/2006/07/27/cyc/Quarry> , <http://sw.cyc.com/2006/07/27/cyc/Terrace-Topographical> , <http://sw.cyc.com/2006/07/27/cyc/FlowerBed> , <http://sw.cyc.com/2006/07/27/cyc/InnerTube> , <http://sw.cyc.com/2006/07/27/cyc/LuggageSet> .

<http://sw.cyc.com/2006/07/27/cyc/AbuBurhanAlIraqi> <http://www.w3.org/2000/01/rdf-schema#comment> """Al Qaeda member.  Attended the first Al Qaeda formation
meeting in Khost, Afghanistan.""" ;
	a <http://sw.cyc.com/2006/07/27/cyc/Individual> , <http://sw.cyc.com/2006/07/27/cyc/AdultMaleHuman> ;
	<http://sw.cyc.com/2006/07/27/cyc/prettyString-Canonical> "Abu Burhan al-Iraqi" ;
	<http://sw.cyc.com/2006/07/27/cyc/prettyString> "Abu Burhan" .

<http://sw.cyc.com/2006/07/27/cyc/AbuDhabi-Emirate> <http://www.w3.org/2000/01/rdf-schema#comment> "The Emirate of Abu Dhabi (or Abu Zaby), the largest and richest of the #$UnitedArabEmirates.  Abu Dhabi's main geographic part is north of #$SaudiArabia, southeast of #$Qatar and southwest of #$Dubai-Emirate, but it has some #$Enclaves to the north, including one disputed with #$Ajman-Emirate." ;
	a <http://sw.cyc.com/2006/07/27/cyc/Individual> , <http://sw.cyc.com/2006/07/27/cyc/CountrySubsidiary> , <http://sw.cyc.com/2006/07/27/cyc/Emirate-Geopolitical> , <http://sw.cyc.com/2006/07/27/cyc/CountriesInThePersianGulf-HormuzArea-Topic> ;
	<http://sw.cyc.com/2006/07/27/cyc/prettyString-Canonical> "Abu Dhabi" ;
	<http://sw.cyc.com/2006/07/27/cyc/prettyString> "Abu Zaby" , "Abu Zabi" .

<http://sw.cyc.com/2006/07/27/cyc/CountrySubsidiary> <http://www.w3.org/2000/01/rdf-schema#comment> "A specialization of #$GeopoliticalEntity.  Each instance of #$CountrySubsidiary is a political region that is a direct subsidiary of some country.  This collection includes states, provinces, territories, and some special districts such as Washington, D.C." ;
	a <http://sw.cyc.com/2006/07/27/cyc/ExistingObjectType> , <http://sw.cyc.com/2006/07/27/cyc/ArtifactualFeatureType> , <http://sw.cyc.com/2006/07/27/cyc/AtemporalNecessarilyEssentialCollectionType> , <http://sw.cyc.com/2006/07/27/cyc/GeopoliticalEntities-Geography-Topic> ;
	<http://sw.cyc.com/2006/07/27/cyc/prettyString-Canonical> "country subsidiary" ;
	<http://sw.cyc.com/2006/07/27/cyc/prettyString> "district" , "districts" , "country subsidiaries" ;
	<http://www.w3.org/2000/01/rdf-schema#subClassOf> <http://sw.cyc.com/2006/07/27/cyc/GeopoliticalEntity> , <http://sw.cyc.com/2006/07/27/cyc/NonNaturalThing> ;
	<http://sw.cyc.com/2006/07/27/cyc/facets-Generic> <http://sw.cyc.com/2006/07/27/cyc/CountrySubsidiaryTypeByAdministrativeDivision> .

<http://sw.cyc.com/2006/07/27/cyc/AbuDoha> <http://sw.cyc.com/2006/07/27/cyc/prettyString> "Amar Doha" , "Doha Doha" , "Rashid Bukhalfa" , "Rashid Makhlolif" , "Rashid Doha" , "Amar Bukhalfa" , "Doha Bukhalfa" , "Haydar Bukhalfa" , "Abu Bukhalfa" , "Bukhalfa" , "Makhlolif" , "Amar Makhlolif" , "Rachid" , "Amar Maklolif" , "the Doctor" , "Dr. Haider" , "Amar Makhlulif" , "Haydar Abu Doha" , "Haydar Doha" , "Doha" .

<http://sw.cyc.com/2006/07/27/cyc/IslamicNationalist> <http://www.w3.org/2000/01/rdf-schema#comment> "The collection of all persons whose belief system is Islamic Nationalism." ;
	a <http://sw.cyc.com/2006/07/27/cyc/ExistingObjectType> , <http://www.w3.org/2002/07/owl#Class> , <http://sw.cyc.com/2006/07/27/cyc/FirstOrderCollection> , <http://sw.cyc.com/2006/07/27/cyc/SetOrCollection> , <http://sw.cyc.com/2006/07/27/cyc/PersonTypeByBeliefSystem> ;
	<http://sw.cyc.com/2006/07/27/cyc/prettyString-Canonical> "Islamic nationalist" ;
	<http://sw.cyc.com/2006/07/27/cyc/prettyString> "Islamic nationalism mortal" , "Islamic nationalist ideology mortal" , "Islamic nationalism layman" , "Islamic nationalist ideology layman" , "Islamic nationalism laymen" , "Islamic nationalist ideology laymen" , "Islamic nationalism persons" , "Islamic nationalist ideology persons" , "Islamic nationalism mortals" , "Islamic nationalist ideology mortals" , "Islamic nationalism human thing" , "Islamic nationalist ideology human thing" , "person whose belief systems have included Islamic nationalism" , "Islamic nationalists" , "human whose belief systems have included Islamic nationalism" , "people whose belief systems have included Islamic nationalism" , "mortal whose belief systems have included Islamic nationalism" , "layman whose belief systems have included Islamic nationalism" , "laymen whose belief systems have included Islamic nationalism" , "persons whose belief systems have included Islamic nationalism" , "mortals whose belief systems have included Islamic nationalism" , "humaner whose belief systems have included Islamic nationalism" , "humanest whose belief systems have included Islamic nationalism" .

<http://sw.cyc.com/2006/07/27/cyc/AbuHul-PLOLeader> <http://sw.cyc.com/2006/07/27/cyc/prettyString-Canonical> "Abu Hul" .

<http://sw.cyc.com/2006/07/27/cyc/AbuIbrahimAlIraqi> <http://www.w3.org/2000/01/rdf-schema#comment> "Al Qaida member, and member of the Shura Council" ;
	a <http://sw.cyc.com/2006/07/27/cyc/Individual> , <http://sw.cyc.com/2006/07/27/cyc/AdultMaleHuman> , <http://sw.cyc.com/2006/07/27/cyc/IraqiPerson> ;
	<http://sw.cyc.com/2006/07/27/cyc/prettyString-Canonical> "Abu Ibrahim al-Iraqi" ;
	<http://sw.cyc.com/2006/07/27/cyc/prettyString> "Abu Ibrahim" .

<http://sw.cyc.com/2006/07/27/cyc/AbuIyad-PLOLeader> <http://www.w3.org/2000/01/rdf-schema#comment> "Abu Iyad, deputy chief of the PLO, who was assassinated in 1991." ;
	a <http://sw.cyc.com/2006/07/27/cyc/Individual> , <http://sw.cyc.com/2006/07/27/cyc/Leader> ;
	<http://sw.cyc.com/2006/07/27/cyc/prettyString-Canonical> "Seif Allah Ben Hasin" ;
	<http://sw.cyc.com/2006/07/27/cyc/prettyString> "Abu Iyyad" , "Seif Ben Hasin" , "Ben Hasin" , "Seif A. Ben Hasin" .

<http://sw.cyc.com/2006/07/27/cyc/AbujaCapitalTerritoryNigeria> a <http://sw.cyc.com/2006/07/27/cyc/Individual> , <http://sw.cyc.com/2006/07/27/cyc/GeographicalThing> , <http://sw.cyc.com/2006/07/27/cyc/FederalDistrict> ;
	<http://sw.cyc.com/2006/07/27/cyc/prettyString-Canonical> "Abuja Capital Territory" .

<http://sw.cyc.com/2006/07/27/cyc/FederalDistrict> <http://www.w3.org/2000/01/rdf-schema#comment> "The collection of all federal districts.  Each instance of #$FederalDistrict is a #$CountrySubsidiary which answers directly to the government of the #$Country without being part of any intermediate body.  A #$FederalDistrict usually contains the #$capitalCity of the #$Country." ;
	a <http://sw.cyc.com/2006/07/27/cyc/ExistingObjectType> , <http://sw.cyc.com/2006/07/27/cyc/ArtifactualFeatureType> ;
	<http://sw.cyc.com/2006/07/27/cyc/prettyString-Canonical> "federal district" ;
	<http://sw.cyc.com/2006/07/27/cyc/prettyString> "federal districts" ;
	<http://www.w3.org/2000/01/rdf-schema#subClassOf> <http://sw.cyc.com/2006/07/27/cyc/CountrySubsidiary> , <http://sw.cyc.com/2006/07/27/cyc/NonNaturalThing> .

<http://sw.cyc.com/2006/07/27/cyc/AbuJaffar> <http://www.w3.org/2000/01/rdf-schema#comment> "#$AhmedRessam testified that #$AbuJaffar is one of the leaders of the Algerian group which met at the #$KahldenCamp, a terrorist training camp in Afghanistan." ;
	a <http://sw.cyc.com/2006/07/27/cyc/Individual> , <http://sw.cyc.com/2006/07/27/cyc/AdultMaleHuman> , <http://sw.cyc.com/2006/07/27/cyc/Leader> , <http://sw.cyc.com/2006/07/27/cyc/IntelligentAgent> , <http://sw.cyc.com/2006/07/27/cyc/IslamicNationalist> , <http://sw.cyc.com/2006/07/27/cyc/AlgerianPerson> ;
	<http://sw.cyc.com/2006/07/27/cyc/prettyString-Canonical> "Abu Jaffar" ;
	<http://sw.cyc.com/2006/07/27/cyc/prettyString> "Jaffar" .

<http://sw.cyc.com/2006/07/27/cyc/AbuKhaleedAlMadani> <http://www.w3.org/2000/01/rdf-schema#comment> "Al Qaida member, and member of the military committee" ;
	a <http://sw.cyc.com/2006/07/27/cyc/Individual> , <http://sw.cyc.com/2006/07/27/cyc/AdultMaleHuman> ;
	<http://sw.cyc.com/2006/07/27/cyc/prettyString-Canonical> "Abu Khaleed al-Madani" .

<http://sw.cyc.com/2006/07/27/cyc/AbuKharab> a <http://sw.cyc.com/2006/07/27/cyc/Individual> , <http://sw.cyc.com/2006/07/27/cyc/Person> ;
	<http://sw.cyc.com/2006/07/27/cyc/prettyString-Canonical> "Abu Kharab" ;
	<http://sw.cyc.com/2006/07/27/cyc/prettyString> "Kharab" .

<http://sw.cyc.com/2006/07/27/cyc/AbuKheirElMasry> <http://www.w3.org/2000/01/rdf-schema#comment> """An instructor at the Jihad Wal Camp, he teaches the use
and making of explosives.""" ;
	a <http://sw.cyc.com/2006/07/27/cyc/Individual> , <http://sw.cyc.com/2006/07/27/cyc/AdultMaleHuman> , <http://sw.cyc.com/2006/07/27/cyc/EgyptianPerson> ;
	<http://sw.cyc.com/2006/07/27/cyc/prettyString-Canonical> "Abu Kheir el Masry" .

<http://sw.cyc.com/2006/07/27/cyc/AbulAbbas> a <http://sw.cyc.com/2006/07/27/cyc/Individual> , <http://sw.cyc.com/2006/07/27/cyc/Person> ;
	<http://sw.cyc.com/2006/07/27/cyc/prettyString-Canonical> "Abul Abbas" ;
	<http://sw.cyc.com/2006/07/27/cyc/prettyString> "Abbas" .

<http://sw.cyc.com/2006/07/27/cyc/AbuMadiGasField> a <http://sw.cyc.com/2006/07/27/cyc/Individual> , <http://sw.cyc.com/2006/07/27/cyc/GasField> ;
	<http://sw.cyc.com/2006/07/27/cyc/prettyString-Canonical> "the Abu Madi gas Field" ;
	<http://sw.cyc.com/2006/07/27/cyc/prettyString> "Abu Madi" .

<http://sw.cyc.com/2006/07/27/cyc/GasField> <http://www.w3.org/2000/01/rdf-schema#comment> """The collection of regions which are naturally
rich in deposits of #$NaturalGas.  Once a #$GasField is producing
#$NaturalGas, it ought to be considered a #$GasField-Developed. #$JulieF.""" ;
	a <http://sw.cyc.com/2006/07/27/cyc/ExistingObjectType> , <http://sw.cyc.com/2006/07/27/cyc/SpatiallyDisjointObjectType> , <http://sw.cyc.com/2006/07/27/cyc/ArtifactualFeatureType> ;
	<http://sw.cyc.com/2006/07/27/cyc/prettyString-Canonical> "gas field" ;
	<http://sw.cyc.com/2006/07/27/cyc/prettyString> "gas fields" ;
	<http://www.w3.org/2000/01/rdf-schema#subClassOf> <http://sw.cyc.com/2006/07/27/cyc/NonNaturalThing> , <http://sw.cyc.com/2006/07/27/cyc/MineralField> .

<http://sw.cyc.com/2006/07/27/cyc/AbuMosabAlSaudi> a <http://sw.cyc.com/2006/07/27/cyc/Individual> , <http://sw.cyc.com/2006/07/27/cyc/AdultMaleHuman> , <http://sw.cyc.com/2006/07/27/cyc/SaudiPerson> ;
	<http://sw.cyc.com/2006/07/27/cyc/prettyString-Canonical> "Abu Mosab al-Saudi" .

<http://sw.cyc.com/2006/07/27/cyc/SaudiPerson> <http://www.w3.org/2000/01/rdf-schema#comment> "The collection of people who are #$citizens of #$SaudiArabia, or participate in its #$NationalCulture." ;
	a <http://sw.cyc.com/2006/07/27/cyc/NationalityGroupsInTheRegion-HormuzArea-Topic> , <http://sw.cyc.com/2006/07/27/cyc/TKBNationalityList> , <http://sw.cyc.com/2006/07/27/cyc/PersonTypeByNationality> ;
	<http://sw.cyc.com/2006/07/27/cyc/prettyString-Canonical> "Saudi" ;
	<http://sw.cyc.com/2006/07/27/cyc/prettyString> "Saudi person" , "Saudi people" , "Saudi persons" , "Saudi Arabian person" , "Saudi Arabian people" , "Saudi Arabian persons" , "Saudi Arabian" , "Saudi Arabians" , "Saudis" ;
	<http://www.w3.org/2000/01/rdf-schema#subClassOf> <http://sw.cyc.com/2006/07/27/cyc/AsianCitizenOrSubject> , <http://sw.cyc.com/2006/07/27/cyc/PersonWithNationality> .

<http://sw.cyc.com/2006/07/27/cyc/AbuMusabAlSudani> <http://www.w3.org/2000/01/rdf-schema#comment> """An opponent of Saddiq al-Mahdi, he encouraged al-Fadl
to infiltrate the Umma Party (al-Mahdi's political party),
question him about Party matters, and then kill him.""" ;
	a <http://sw.cyc.com/2006/07/27/cyc/Individual> , <http://sw.cyc.com/2006/07/27/cyc/AdultMaleHuman> , <http://sw.cyc.com/2006/07/27/cyc/SudanPerson> ;
	<http://sw.cyc.com/2006/07/27/cyc/prettyString-Canonical> "Abu Musab al-Sudani" ;
	<http://sw.cyc.com/2006/07/27/cyc/prettyString> "Abu Musab" .

<http://sw.cyc.com/2006/07/27/cyc/AbuMusabAlSuri> <http://www.w3.org/2000/01/rdf-schema#comment> "The emir of #$JamaateJihalAlSuri." ;
	a <http://sw.cyc.com/2006/07/27/cyc/Individual> , <http://sw.cyc.com/2006/07/27/cyc/AdultMaleHuman> , <http://sw.cyc.com/2006/07/27/cyc/Leader> , <http://sw.cyc.com/2006/07/27/cyc/SyrianPerson> , <http://sw.cyc.com/2006/07/27/cyc/BlondeHairedHuman> ;
	<http://sw.cyc.com/2006/07/27/cyc/prettyString-Canonical> "Abu Musab al-Suri" ;
	<http://sw.cyc.com/2006/07/27/cyc/prettyString> "Abu Musab" , "the organizational head of Jamaate Jihal al-Suri" , "Jamaate Jihal al-Suri's organizational head" .

<http://sw.cyc.com/2006/07/27/cyc/SyrianPerson> <http://www.w3.org/2000/01/rdf-schema#comment> "The collection of people who are #$citizens of #$Syria, or participate in its #$NationalCulture." ;
	a <http://sw.cyc.com/2006/07/27/cyc/TestOWLExportConcept> , <http://sw.cyc.com/2006/07/27/cyc/NationalityGroupsInTheRegion-HormuzArea-Topic> , <http://sw.cyc.com/2006/07/27/cyc/TKBNationalityList> , <http://sw.cyc.com/2006/07/27/cyc/PersonTypeByNationality> ;
	<http://sw.cyc.com/2006/07/27/cyc/prettyString-Canonical> "Syrian" ;
	<http://sw.cyc.com/2006/07/27/cyc/prettyString> "Syriac" , "Syriac person" , "Syriac people" , "Syriac persons" , "Syrian person" , "Syrian people" , "Syrian persons" , "Syrians" ;
	<http://www.w3.org/2000/01/rdf-schema#subClassOf> <http://sw.cyc.com/2006/07/27/cyc/AsianCitizenOrSubject> , <http://sw.cyc.com/2006/07/27/cyc/PersonWithNationality> .

<http://sw.cyc.com/2006/07/27/cyc/BlondeHairedHuman> <http://www.w3.org/2000/01/rdf-schema#comment> "The collection of all #$HomoSapiens with #$Blonde-HairColor evident on the head.  The color may be natural or dyed, and it may include woven hair.  Removable wigs are excluded from consideration in determining this class of people." ;
	a <http://sw.cyc.com/2006/07/27/cyc/HumanTypeByHairColor> ;
	<http://sw.cyc.com/2006/07/27/cyc/prettyString-Canonical> "blonde person" ;
	<http://sw.cyc.com/2006/07/27/cyc/prettyString> "blonde" , "blondie" , "blondies" , "blond" , "blonds" , "blondes" , "blonde people" , "blonde persons" ;
	<http://www.w3.org/2000/01/rdf-schema#subClassOf> <http://sw.cyc.com/2006/07/27/cyc/HomoSapiens> .

<http://sw.cyc.com/2006/07/27/cyc/AbuMusaConflict-1992> <http://www.w3.org/2000/01/rdf-schema#comment> "A #$TerritorialDispute between #$Iran and #$UnitedArabEmirates over #$AbuMusaIsland." ;
	a <http://sw.cyc.com/2006/07/27/cyc/Individual> , <http://sw.cyc.com/2006/07/27/cyc/InternationalTerritorialDispute> ;
	<http://sw.cyc.com/2006/07/27/cyc/prettyString-Canonical> "Abu Musa Conflict 1992" .

<http://sw.cyc.com/2006/07/27/cyc/InternationalTerritorialDispute> <http://www.w3.org/2000/01/rdf-schema#comment> "A collection of events, a subset of #$ConflictEvent and #$InternationalConflict. In each instance, there are at least two instances of #$Country, who both claim legal control over some place, in such a way that their claims come into conflict. The dispute between the #$UnitedKingdomOfGreatBritainAndNorthernIreland and #$Argentina over who controlled the #$FalklandIslands would be an instance.  While both the #$CityOfAustinTX and #$Texas-State claiming control over parts of Travis County would not, since the claims are not in conflict and the dispute is not at the international level." ;
	a <http://sw.cyc.com/2006/07/27/cyc/FirstOrderCollection> ;
	<http://sw.cyc.com/2006/07/27/cyc/prettyString-Canonical> "international territorial dispute" ;
	<http://sw.cyc.com/2006/07/27/cyc/prettyString> "international territorial disputes" ;
	<http://www.w3.org/2000/01/rdf-schema#subClassOf> <http://sw.cyc.com/2006/07/27/cyc/DisputeEvent> , <http://sw.cyc.com/2006/07/27/cyc/InternationalConflict> .

<http://sw.cyc.com/2006/07/27/cyc/AbuMusaIncidentMt> <http://www.w3.org/2000/01/rdf-schema#comment> "A #$Microtheory containing information about the 1992 conflict between Iran and the UAE over Abu Musa Island.  This           Factsheet is available online at http://www.iet.com/Projects/HPKB/Y2/." ;
	<http://sw.cyc.com/2006/07/27/cyc/genlMt> <http://sw.cyc.com/2006/07/27/cyc/BaseKB> , <http://sw.cyc.com/2006/07/27/cyc/HPKB-CF-ReasoningMt> .

<http://sw.cyc.com/2006/07/27/cyc/AbuQirBay> a <http://sw.cyc.com/2006/07/27/cyc/Bay> ;
	<http://sw.cyc.com/2006/07/27/cyc/prettyString-Canonical> "Abu Qir Bay" ;
	<http://sw.cyc.com/2006/07/27/cyc/prettyString> "Abu Qir" , "Aboukir" , "Aboukir Bay" .

<http://sw.cyc.com/2006/07/27/cyc/Bay> <http://www.w3.org/2000/01/rdf-schema#comment> "A specialization of #$BodyOfWater.  Each instance of #$Bay is an inlet of a sea or lake, and is usually smaller than a #$Gulf." ;
	a <http://sw.cyc.com/2006/07/27/cyc/ExistingObjectType> , <http://sw.cyc.com/2006/07/27/cyc/QAClarifyingCollectionType> , <http://sw.cyc.com/2006/07/27/cyc/NaturalFeatureType> , <http://sw.cyc.com/2006/07/27/cyc/WaterBodyConcept> ;
	<http://sw.cyc.com/2006/07/27/cyc/prettyString-Canonical> "BAY" ;
	<http://sw.cyc.com/2006/07/27/cyc/prettyString> "bays" ;
	<http://www.w3.org/2000/01/rdf-schema#subClassOf> <http://sw.cyc.com/2006/07/27/cyc/BodyOfWater> , <http://sw.cyc.com/2006/07/27/cyc/NaturalThing> .

<http://sw.cyc.com/2006/07/27/cyc/AbuQir-NorthAbuQir-GasField> a <http://sw.cyc.com/2006/07/27/cyc/Individual> , <http://sw.cyc.com/2006/07/27/cyc/GasField> ;
	<http://sw.cyc.com/2006/07/27/cyc/prettyString-Canonical> "the Abu Qir-North Abu Qir-gas Field" ;
	<http://sw.cyc.com/2006/07/27/cyc/prettyString> "Abu Qir/North Abu Qir" .

<http://sw.cyc.com/2006/07/27/cyc/AbuRidaAlSuri> <http://www.w3.org/2000/01/rdf-schema#comment> "Al Qaida member." ;
	a <http://sw.cyc.com/2006/07/27/cyc/Individual> , <http://sw.cyc.com/2006/07/27/cyc/AdultMaleHuman> , <http://sw.cyc.com/2006/07/27/cyc/SyrianPerson> ;
	<http://sw.cyc.com/2006/07/27/cyc/prettyString-Canonical> "Abu Rida al-Suri" .

<http://sw.cyc.com/2006/07/27/cyc/AbuSaafaOilField> <http://www.w3.org/2000/01/rdf-schema#comment> "An #$OilField located in #$SaudiArabia" ;
	a <http://sw.cyc.com/2006/07/27/cyc/Individual> , <http://sw.cyc.com/2006/07/27/cyc/OilField> ;
	<http://sw.cyc.com/2006/07/27/cyc/prettyString-Canonical> "the Abu Saafa Oilfield" ;
	<http://sw.cyc.com/2006/07/27/cyc/prettyString> "Abu Saafa" .

<http://sw.cyc.com/2006/07/27/cyc/Abuse-TheGame> a <http://sw.cyc.com/2006/07/27/cyc/Individual> , <http://sw.cyc.com/2006/07/27/cyc/UnversionedProgram> , <http://sw.cyc.com/2006/07/27/cyc/ComputerGameProgram> , <http://sw.cyc.com/2006/07/27/cyc/Freeware> , <http://sw.cyc.com/2006/07/27/cyc/OpenSourceComputerProgram> ;
	<http://sw.cyc.com/2006/07/27/cyc/prettyString-Canonical> "abuse.console" ;
	<http://sw.cyc.com/2006/07/27/cyc/prettyString> "Abuse" .

<http://sw.cyc.com/2006/07/27/cyc/Freeware> <http://www.w3.org/2000/01/rdf-schema#comment> "This collection includes all instances of Freeware, software which is available free of charge." ;
	a <http://sw.cyc.com/2006/07/27/cyc/AtemporalNecessarilyEssentialCollectionType> , <http://sw.cyc.com/2006/07/27/cyc/KEClarifyingCollectionType> , <http://sw.cyc.com/2006/07/27/cyc/ComputerProgramTypeByDistribution> ;
	<http://sw.cyc.com/2006/07/27/cyc/prettyString-Canonical> "freeware" ;
	<http://www.w3.org/2000/01/rdf-schema#subClassOf> <http://sw.cyc.com/2006/07/27/cyc/ComputerProgram-CW> , <http://sw.cyc.com/2006/07/27/cyc/FreeThing> ;
	<http://www.w3.org/2002/07/owl#disjointWith> <http://sw.cyc.com/2006/07/27/cyc/MarketedComputerProgram> .

<http://sw.cyc.com/2006/07/27/cyc/OpenSourceComputerProgram> <http://www.w3.org/2000/01/rdf-schema#comment> "A specialization of #$ComputerProgram-CW. #$OpenSourceComputerProgram is the collection of programs for which the #$ComputerCode-Source is available to anyone who owns a copy of the program.  That means owners are free to run, copy, distribute, study, change, and improve the software.  Some prominent instances of #$OpenSourceComputerProgram are the #$ApacheWebServer -- which operates a significant number of the world's web sites, #$BIND-TheProgram -- that provides the domain name service for the Internet, the #$Linux operating system, GNU software packages, and many computer games." ;
	a <http://sw.cyc.com/2006/07/27/cyc/AtemporalNecessarilyEssentialCollectionType> , <http://sw.cyc.com/2006/07/27/cyc/KEClarifyingCollectionType> , <http://sw.cyc.com/2006/07/27/cyc/ComputerProgramTypeByDistribution> ;
	<http://sw.cyc.com/2006/07/27/cyc/prettyString-Canonical> "open source program" ;
	<http://sw.cyc.com/2006/07/27/cyc/prettyString> "open source software" .

<http://sw.cyc.com/2006/07/27/cyc/AbutilonEremitopetalum> a <http://sw.cyc.com/2006/07/27/cyc/BiologicalSpecies> , <http://sw.cyc.com/2006/07/27/cyc/Endangered-OrganismTypeByExistentialThreatLevel> ;
	<http://sw.cyc.com/2006/07/27/cyc/prettyString-Canonical> "Abutilon eremitopetalum" ;
	<http://www.w3.org/2000/01/rdf-schema#subClassOf> <http://sw.cyc.com/2006/07/27/cyc/Plant> ;
	<http://sw.cyc.com/2006/07/27/cyc/superTaxons> <http://sw.cyc.com/2006/07/27/cyc/Plant> .

<http://sw.cyc.com/2006/07/27/cyc/Plant> <http://www.w3.org/2000/01/rdf-schema#comment> "The collection of all individual plants, an instance of #$OrganismClassificationType and a specialization of #$EukaryoticOrganism.  #$Plant is a member of the #$BiologicalKingdom and contains the primary subjects of #$Botany.  The instances of this collections are typically stationary, living, whole organisms; the cells of plants generally lack cholesterol and have cell walls that include substances of #$Cellulose.  Most, though not all, plants are capable of making sugars by #$Photosynthesis-Plant processes and have green parts.  Some example subsets of #$Plant are the collections #$RoseBush, #$SpruceTree, and #$Moss." ;
	a <http://sw.cyc.com/2006/07/27/cyc/SpatiallyDisjointObjectType> , <http://sw.cyc.com/2006/07/27/cyc/KEClarifyingCollectionType> , <http://sw.cyc.com/2006/07/27/cyc/CandidateKBCompletenessNode> , <http://sw.cyc.com/2006/07/27/cyc/OrganismByTaxonomicKingdom-Biology-Topic> , <http://sw.cyc.com/2006/07/27/cyc/BiologicalKingdom> ;
	<http://sw.cyc.com/2006/07/27/cyc/prettyString-Canonical> "Plant" ;
	<http://sw.cyc.com/2006/07/27/cyc/prettyString> "plants" , "greenery" ;
	<http://www.w3.org/2000/01/rdf-schema#subClassOf> <http://sw.cyc.com/2006/07/27/cyc/EukaryoticOrganism> , <http://sw.cyc.com/2006/07/27/cyc/PlantBLO> , <http://sw.cyc.com/2006/07/27/cyc/TopAndBottomSidedObject> , <http://sw.cyc.com/2006/07/27/cyc/VegetableMatter> .

<http://sw.cyc.com/2006/07/27/cyc/BiologicalSpecies> <http://www.w3.org/2000/01/rdf-schema#comment> "An instance of #$BiologicalTaxonType. Each instance of #$BiologicalSpecies is the most general taxon from which two breeding organisms of appropriate sexes can conceivably produce fertile offspring, or, in the case of asexual reproduction, is conventionally defined.  Members of different species of animals cannot produce fertile offspring by interbreeding.  If there are only two breeds of a given species and one breed becomes extinct, the second breed by virtue of that fact becomes an instance of #$BiologicalSpecies -- since the only organisms instances can breed with to produce fertile offspring are, at that point, members of that collection.  An instance of #$BiologicalSpecies has members who all have significant traits in common, and members of each biological species have other members as parents.  Exceptions occur when a species is conventionally defined to start since parenthood could conceivably be traced back billions of years, yet new species came into existence.  In biological taxonomy, related species are grouped into a particular instance of #$BiologicalGenus.  Some genera have only a single species, but they remain different taxons." ;
	a <http://sw.cyc.com/2006/07/27/cyc/KEClarifyingCollectionType> , <http://sw.cyc.com/2006/07/27/cyc/FacetingCollectionType> , <http://sw.cyc.com/2006/07/27/cyc/DisjointCollectionType> , <http://sw.cyc.com/2006/07/27/cyc/Biology-Topic> , <http://sw.cyc.com/2006/07/27/cyc/BiologicalTaxonType> ;
	<http://sw.cyc.com/2006/07/27/cyc/prettyString-Canonical> "species" ;
	<http://sw.cyc.com/2006/07/27/cyc/prettyString> "variety" , "varieties" , "biological species" ;
	<http://www.w3.org/2000/01/rdf-schema#subClassOf> <http://sw.cyc.com/2006/07/27/cyc/KEClarifyingCollectionType> , <http://sw.cyc.com/2006/07/27/cyc/FacetInstanceCollection> , <http://sw.cyc.com/2006/07/27/cyc/BiologicalTaxon> ;
	<http://sw.cyc.com/2006/07/27/cyc/sharedNotes> <http://sw.cyc.com/2006/07/27/cyc/SharedNoteOnGenlsRelationsBetweenFacetingCollectionTypes> ;
	<http://sw.cyc.com/2006/07/27/cyc/typeGenls> <http://sw.cyc.com/2006/07/27/cyc/Organism-Whole> .

<http://sw.cyc.com/2006/07/27/cyc/Endangered-OrganismTypeByExistentialThreatLevel> <http://www.w3.org/2000/01/rdf-schema#comment> "The collection of #$BiologicalSpecies and other #$OrganismClassificationTypes that are endangered (at risk of extinction)." ;
	a <http://sw.cyc.com/2006/07/27/cyc/SecondOrderCollection> , <http://sw.cyc.com/2006/07/27/cyc/TestOWLExportConcept> , <http://sw.cyc.com/2006/07/27/cyc/ClarifyingCollectionType> , <http://sw.cyc.com/2006/07/27/cyc/OrganismTypeByExistentialThreatLevel> ;
	<http://sw.cyc.com/2006/07/27/cyc/prettyString-Canonical> "endangered species" ;
	<http://www.w3.org/2000/01/rdf-schema#subClassOf> <http://sw.cyc.com/2006/07/27/cyc/OrganismClassificationType> , <http://sw.cyc.com/2006/07/27/cyc/NonEmptyCollection> .

<http://sw.cyc.com/2006/07/27/cyc/superTaxons> <http://www.w3.org/2000/01/rdf-schema#comment> "A specialization of #$genls used to relate instances of #$BiologicalTaxon.  <code>(#$superTaxons TAXON SUPERTAXON)</code> means that <code>SUPERTAXON</code> is above the more specific <code>TAXON</code> in the biological taxon hierarchy; i.e. the later taxon is more general and inclusive than the former.  Every instance of <code>TAXON</code> must therefore also be an instance of <code>SUPERTAXON</code>.  For example, (#$superTaxons #$DomesticCat #$FelisGenus) holds.  See also #$taxonMembers." ;
	a <http://www.w3.org/2002/07/owl#TransitiveProperty> , <http://sw.cyc.com/2006/07/27/cyc/AsymmetricBinaryPredicate> , <http://sw.cyc.com/2006/07/27/cyc/FirstOrderCollectionPredicate> , <http://sw.cyc.com/2006/07/27/cyc/RuleMacroPredicate> , <http://sw.cyc.com/2006/07/27/cyc/RelationalNounSlot> , <http://sw.cyc.com/2006/07/27/cyc/Biology-Topic> , <http://sw.cyc.com/2006/07/27/cyc/VocabularyDefiningPredicate> ;
	<http://sw.cyc.com/2006/07/27/cyc/prettyString-Canonical> "Super Taxons" ;
	<http://sw.cyc.com/2006/07/27/cyc/quotedIsa> <http://sw.cyc.com/2006/07/27/cyc/OpenCycDefinitionalPredicate> , <http://sw.cyc.com/2006/07/27/cyc/DefinitionalPredicate> ;
	<http://www.w3.org/2000/01/rdf-schema#domain> <http://sw.cyc.com/2006/07/27/cyc/BiologicalTaxon> ;
	<http://sw.cyc.com/2006/07/27/cyc/arity> "2"^^<http://www.w3.org/2001/XMLSchema#long> ;
	<http://www.w3.org/2000/01/rdf-schema#range> <http://sw.cyc.com/2006/07/27/cyc/BiologicalTaxon> ;
	<http://www.w3.org/2000/01/rdf-schema#subPropertyOf> <http://www.w3.org/2000/01/rdf-schema#subClassOf> ;
	<http://sw.cyc.com/2006/07/27/cyc/arg1Genl> <http://sw.cyc.com/2006/07/27/cyc/Organism-Whole> ;
	<http://sw.cyc.com/2006/07/27/cyc/arg2Genl> <http://sw.cyc.com/2006/07/27/cyc/Organism-Whole> ;
	<http://sw.cyc.com/2006/07/27/cyc/arg1Format> <http://sw.cyc.com/2006/07/27/cyc/SetTheFormat> ;
	<http://sw.cyc.com/2006/07/27/cyc/arg2Format> <http://sw.cyc.com/2006/07/27/cyc/SetTheFormat> ;
	<http://sw.cyc.com/2006/07/27/cyc/negationInverse> <http://sw.cyc.com/2006/07/27/cyc/superTaxons> ;
	<http://sw.cyc.com/2006/07/27/cyc/typedGenlPreds> <http://www.w3.org/2000/01/rdf-schema#subClassOf> ;
	<http://sw.cyc.com/2006/07/27/cyc/genlInverse> <http://sw.cyc.com/2006/07/27/cyc/taxonMembers> .

<http://sw.cyc.com/2006/07/27/cyc/AbutilonSandwicense> a <http://sw.cyc.com/2006/07/27/cyc/SpatiallyDisjointObjectType> , <http://sw.cyc.com/2006/07/27/cyc/BiologicalSpecies> , <http://sw.cyc.com/2006/07/27/cyc/Endangered-OrganismTypeByExistentialThreatLevel> ;
	<http://sw.cyc.com/2006/07/27/cyc/prettyString-Canonical> "Abutilon sandwicense" ;
	<http://www.w3.org/2000/01/rdf-schema#subClassOf> <http://sw.cyc.com/2006/07/27/cyc/Plant> ;
	<http://sw.cyc.com/2006/07/27/cyc/superTaxons> <http://sw.cyc.com/2006/07/27/cyc/Plant> .

<http://sw.cyc.com/2006/07/27/cyc/abutsSurface> <http://www.w3.org/2000/01/rdf-schema#comment> "(#$abutsSurface OBJ1 OBJ2) means that an end of #$LongAndThin OBJ1 is in contact with the surface of OBJ2." ;
	a <http://sw.cyc.com/2006/07/27/cyc/CoexistingObjectsPredicate> , <http://sw.cyc.com/2006/07/27/cyc/RelativeLocationalPredicate> , <http://sw.cyc.com/2006/07/27/cyc/InterExistingObjectPredicate> ;
	<http://sw.cyc.com/2006/07/27/cyc/prettyString-Canonical> "Abuts Surface" ;
	<http://www.w3.org/2000/01/rdf-schema#domain> <http://sw.cyc.com/2006/07/27/cyc/PartiallyTangible> ;
	<http://sw.cyc.com/2006/07/27/cyc/arity> "2"^^<http://www.w3.org/2001/XMLSchema#long> ;
	<http://www.w3.org/2000/01/rdf-schema#range> <http://sw.cyc.com/2006/07/27/cyc/PartiallyTangible> ;
	<http://www.w3.org/2000/01/rdf-schema#subPropertyOf> <http://sw.cyc.com/2006/07/27/cyc/temporallyCoexist> , <http://sw.cyc.com/2006/07/27/cyc/touchesAtEnd> .

<http://sw.cyc.com/2006/07/27/cyc/touchesAtEnd> <http://www.w3.org/2000/01/rdf-schema#comment> "(#$touchesAtEnd OBJ1 OBJ2) means that an end of OBJ1 #$touches OBJ2.  If the two objects are #$connectedTo each other at this point, the more specific #$Predicate, #$connectedAtEnd applies." ;
	a <http://www.w3.org/2000/01/rdf-schema#Property> , <http://sw.cyc.com/2006/07/27/cyc/RelativeLocationalPredicate> , <http://sw.cyc.com/2006/07/27/cyc/PredicateOrCollection-UsedInUCTRepresentation> , <http://sw.cyc.com/2006/07/27/cyc/SpatialCotemporalPredicate> ;
	<http://sw.cyc.com/2006/07/27/cyc/prettyString-Canonical> "Touches At End" ;
	<http://www.w3.org/2000/01/rdf-schema#domain> <http://sw.cyc.com/2006/07/27/cyc/SpatialThing> ;
	<http://sw.cyc.com/2006/07/27/cyc/arity> "2"^^<http://www.w3.org/2001/XMLSchema#long> ;
	<http://www.w3.org/2000/01/rdf-schema#range> <http://sw.cyc.com/2006/07/27/cyc/SpatialThing> ;
	<http://www.w3.org/2000/01/rdf-schema#subPropertyOf> <http://sw.cyc.com/2006/07/27/cyc/touches> .

<http://sw.cyc.com/2006/07/27/cyc/InterExistingObjectPredicate> <http://www.w3.org/2000/01/rdf-schema#comment> "A specialization of both #$ObjectPredicate (q.v.) and #$BinaryPredicate.  Each instance of #$InterExistingObjectPredicate is a binary predicate that only relates pairs of #$SomethingExistings to each other.  Thus both argument-places of such a predicate are constrained to instances (see #$argIsa) of #$SomethingExisting or some specialization thereof.  Instances of #$InterExistingObjectPredicate include #$derivedFrom, #$cohabitants, #$capitalCity, and #$electricallyConnectedTo." .

<http://sw.cyc.com/2006/07/27/cyc/Abysm-MusicGroup> a <http://sw.cyc.com/2006/07/27/cyc/ProgressiveMusicPerformer> ;
	<http://sw.cyc.com/2006/07/27/cyc/prettyString-Canonical> "Abysm" .

<http://sw.cyc.com/2006/07/27/cyc/ProgressiveMusicPerformer> <http://www.w3.org/2000/01/rdf-schema#comment> "The collection of bands and solo artists that perform progressive music." ;
	a <http://sw.cyc.com/2006/07/27/cyc/MusicalPerformanceAgentTypeByGenre> ;
	<http://sw.cyc.com/2006/07/27/cyc/prettyString-Canonical> "progressive music performer" ;
	<http://www.w3.org/2000/01/rdf-schema#subClassOf> <http://sw.cyc.com/2006/07/27/cyc/MusicPerformanceAgent> .

<http://sw.cyc.com/2006/07/27/cyc/AbyssalPlain> <http://www.w3.org/2000/01/rdf-schema#comment> "An #$AbyssalPlain is any of the great flat sediment-covered areas of ocean floor." ;
	a <http://sw.cyc.com/2006/07/27/cyc/ExistingObjectType> , <http://sw.cyc.com/2006/07/27/cyc/UnderseaTerrainFeatureType> , <http://sw.cyc.com/2006/07/27/cyc/CartographicFeatureType> ;
	<http://sw.cyc.com/2006/07/27/cyc/prettyString-Canonical> "abyssal plain" ;
	<http://sw.cyc.com/2006/07/27/cyc/prettyString> "abyssal plains" ;
	<http://www.w3.org/2000/01/rdf-schema#subClassOf> <http://sw.cyc.com/2006/07/27/cyc/UnderwaterTopographicalFeature> , <http://sw.cyc.com/2006/07/27/cyc/Place> .

<http://sw.cyc.com/2006/07/27/cyc/UnderwaterTopographicalFeature> <http://www.w3.org/2000/01/rdf-schema#comment> "A collection of geographical regions and a specialization of #$LandTopographicalFeature and #$UnderwaterLocation. Each instance of #$UnderwaterTopographicalFeature is a region of land under a body of water and is distinguishable from surrounding regions by salient physical differences in surface texture, three-dimensional shape, or elevation." ;
	a <http://sw.cyc.com/2006/07/27/cyc/FirstOrderCollection> , <http://sw.cyc.com/2006/07/27/cyc/NaturalFeatureType> ;
	<http://sw.cyc.com/2006/07/27/cyc/prettyString-Canonical> "underwater topographical feature" ;
	<http://www.w3.org/2000/01/rdf-schema#subClassOf> <http://sw.cyc.com/2006/07/27/cyc/NaturalThing> , <http://sw.cyc.com/2006/07/27/cyc/LandTopographicalFeature> , <http://sw.cyc.com/2006/07/27/cyc/UnderwaterLocation> ;
	<http://www.w3.org/2002/07/owl#disjointWith> <http://sw.cyc.com/2006/07/27/cyc/FloodedArea> .

<http://sw.cyc.com/2006/07/27/cyc/Place> <http://www.w3.org/2000/01/rdf-schema#comment> "A specialization of #$EnduringThing-Localized.  Each instance of #$Place is a spatial thing which has a relatively permanent location. Thus, in a given microtheory, each #$Place is stationary with respect to the frame of reference of that microtheory." ;
	a <http://sw.cyc.com/2006/07/27/cyc/FirstOrderCollection> , <http://sw.cyc.com/2006/07/27/cyc/QAClarifyingCollectionType> , <http://sw.cyc.com/2006/07/27/cyc/CartographicFeatureType> , <http://sw.cyc.com/2006/07/27/cyc/Objects-Spatial-Topic> ;
	<http://sw.cyc.com/2006/07/27/cyc/prettyString-Canonical> "place" ;
	<http://sw.cyc.com/2006/07/27/cyc/prettyString> "places" , "point" , "points" , "site" , "sites" , "spot" , "spots" ;
	<http://www.w3.org/2000/01/rdf-schema#subClassOf> <http://sw.cyc.com/2006/07/27/cyc/EnduringThing-Localized> , <http://sw.cyc.com/2006/07/27/cyc/Location-Underspecified> ;
	<http://www.w3.org/2002/07/owl#disjointWith> <http://sw.cyc.com/2006/07/27/cyc/Agent-Generic> , <http://sw.cyc.com/2006/07/27/cyc/DrugSubstance> , <http://sw.cyc.com/2006/07/27/cyc/OrganismPart> , <http://sw.cyc.com/2006/07/27/cyc/EdibleStuff> , <http://sw.cyc.com/2006/07/27/cyc/Device-OneTimeUse> .

<http://sw.cyc.com/2006/07/27/cyc/UnderseaTerrainFeatureType> <http://www.w3.org/2000/01/rdf-schema#comment> "A collection of collections.  Instances of #$UnderseaTerrainFeatureType are collections of terrain features which can be found on the ocean floor." ;
	a <http://sw.cyc.com/2006/07/27/cyc/TerrainFeatureTaxonType> ;
	<http://sw.cyc.com/2006/07/27/cyc/prettyString-Canonical> "undersea terrain feature type" ;
	<http://www.w3.org/2000/01/rdf-schema#subClassOf> <http://sw.cyc.com/2006/07/27/cyc/FirstOrderCollection> , <http://sw.cyc.com/2006/07/27/cyc/CartographicFeatureType> .

<http://sw.cyc.com/2006/07/27/cyc/CartographicFeatureType> <http://www.w3.org/2000/01/rdf-schema#comment> "A #$SecondOrderCollection.  Each instance of #$CartographicFeatureType is a specialization of #$Place whose instances are often displayed on maps or conceptualized cartographically." ;
	a <http://sw.cyc.com/2006/07/27/cyc/NonAbducibleCollection> , <http://sw.cyc.com/2006/07/27/cyc/AtemporalNecessarilyEssentialCollectionType> , <http://sw.cyc.com/2006/07/27/cyc/SecondOrderCollection> ;
	<http://sw.cyc.com/2006/07/27/cyc/prettyString-Canonical> "cartographic feature type" ;
	<http://www.w3.org/2000/01/rdf-schema#subClassOf> <http://sw.cyc.com/2006/07/27/cyc/FirstOrderCollection> , <http://sw.cyc.com/2006/07/27/cyc/TemporalStuffType> ;
	<http://sw.cyc.com/2006/07/27/cyc/typeGenls> <http://sw.cyc.com/2006/07/27/cyc/Place> .

<http://sw.cyc.com/2006/07/27/cyc/AbyssIncidentAtEuropa-TheGame> a <http://sw.cyc.com/2006/07/27/cyc/Individual> , <http://sw.cyc.com/2006/07/27/cyc/AdventureGameProgram> ;
	<http://sw.cyc.com/2006/07/27/cyc/prettyString-Canonical> "Abyss: Incident at Europa" ;
	<http://sw.cyc.com/2006/07/27/cyc/prettyString> "The Abyss: Incident At Europa" , "The Abyss Incident At Europa" .

<http://sw.cyc.com/2006/07/27/cyc/AdventureGameProgram> <http://www.w3.org/2000/01/rdf-schema#comment> "The collection of all  #$ComputerGamePrograms which are 'adventure' games." ;
	a <http://sw.cyc.com/2006/07/27/cyc/KEClarifyingCollectionType> , <http://sw.cyc.com/2006/07/27/cyc/ComputerProgramTypeByFunction> ;
	<http://sw.cyc.com/2006/07/27/cyc/prettyString-Canonical> "adventure game" ;
	<http://sw.cyc.com/2006/07/27/cyc/prettyString> "adventure games" ;
	<http://www.w3.org/2000/01/rdf-schema#subClassOf> <http://sw.cyc.com/2006/07/27/cyc/ComputerGameProgram> ;
	<http://sw.cyc.com/2006/07/27/cyc/siblingDisjointExceptions> <http://sw.cyc.com/2006/07/27/cyc/ActionGameProgram> .

<http://sw.cyc.com/2006/07/27/cyc/Abyssinian-Cat> <http://www.w3.org/2000/01/rdf-schema#comment> "Each #$Abyssinian-Cat is a slender shorthaired cat with a reddish coat, having tabby-like markings. " ;
	a <http://sw.cyc.com/2006/07/27/cyc/CatTypeByBreed> ;
	<http://sw.cyc.com/2006/07/27/cyc/prettyString-Canonical> "Abyssinian cat" ;
	<http://sw.cyc.com/2006/07/27/cyc/prettyString> "Abyssinians" .

<http://sw.cyc.com/2006/07/27/cyc/AcademicBookReport> <http://www.w3.org/2000/01/rdf-schema#subClassOf> <http://sw.cyc.com/2006/07/27/cyc/ProseLiteraryWork-CW> , <http://sw.cyc.com/2006/07/27/cyc/AcademicComposition> .

<http://sw.cyc.com/2006/07/27/cyc/ProseLiteraryWork-CW> <http://www.w3.org/2000/01/rdf-schema#comment> "The collection of all #$PropositionalConceptualWorks which are prose. Including all instances of #$Article-PCW, #$AcademicEssay, #$Novel-CW." ;
	a <http://sw.cyc.com/2006/07/27/cyc/ObjectType> , <http://sw.cyc.com/2006/07/27/cyc/TKBFullySpecifiedSourceType> ;
	<http://sw.cyc.com/2006/07/27/cyc/prettyString-Canonical> "prose literary work" ;
	<http://www.w3.org/2000/01/rdf-schema#subClassOf> <http://sw.cyc.com/2006/07/27/cyc/LiteraryWork-CW> , <http://sw.cyc.com/2006/07/27/cyc/TKBFullySpecifiedSource> .

<http://sw.cyc.com/2006/07/27/cyc/AcademicComposition> <http://www.w3.org/2000/01/rdf-schema#comment> "The collection of all book reports, essays, term papers, etc. written and/or intended to be submitted by #$Students in fulfillment of #$HomeworkAssignments." ;
	a <http://sw.cyc.com/2006/07/27/cyc/ObjectType> ;
	<http://sw.cyc.com/2006/07/27/cyc/prettyString-Canonical> "paper" ;
	<http://sw.cyc.com/2006/07/27/cyc/prettyString> "composition" , "compositions" , "papers" ;
	<http://www.w3.org/2000/01/rdf-schema#subClassOf> <http://sw.cyc.com/2006/07/27/cyc/PropositionalConceptualWork> .

<http://sw.cyc.com/2006/07/27/cyc/PropositionalConceptualWork> <http://www.w3.org/2000/01/rdf-schema#comment> "A specialization of #$ConceptualWork. Each instance of #$PropositionalConceptualWork is an abstract work constituted at least in part by propositional information.  Propositional information is information which has a truth value in some context (see #$Proposition).  Typically, instances of #$PropositionalConceptualWork will be works whose instantiations are composed of (or merely contain) one or more spoken or written sentences. Positive examples of #$PropositionalConceptualWork include any instances of #$ProseLiteraryWork-CW (including instances of #$AcademicEssay and #$ExpositoryArticle).  A positive example that is <i>not</i> a literary work is any instance of #$MusicalComposition that has lyrics that express propositions; another positive example is a mostly graphical advertisement that also includes text that expresses propositions." ;
	a <http://sw.cyc.com/2006/07/27/cyc/ObjectType> , <http://sw.cyc.com/2006/07/27/cyc/TemporalStuffType> , <http://sw.cyc.com/2006/07/27/cyc/CandidateKBCompletenessNode> ;
	<http://sw.cyc.com/2006/07/27/cyc/prettyString-Canonical> "written work" ;
	<http://sw.cyc.com/2006/07/27/cyc/prettyString> "written works" , "propositional conceptual work" , "propositional conceptual works" , "publication" , "publications" ;
	<http://www.w3.org/2000/01/rdf-schema#subClassOf> <http://sw.cyc.com/2006/07/27/cyc/ConceptualWork> ;
	<http://sw.cyc.com/2006/07/27/cyc/facets-Covering> <http://sw.cyc.com/2006/07/27/cyc/PropositionalConceptualWorkTypeByStyle> ;
	<http://sw.cyc.com/2006/07/27/cyc/facets-Generic> <http://sw.cyc.com/2006/07/27/cyc/PCWTypeByGenre> ;
	<http://sw.cyc.com/2006/07/27/cyc/requiredArg1Pred> <http://sw.cyc.com/2006/07/27/cyc/topicOfPCW> .

<http://sw.cyc.com/2006/07/27/cyc/academicCourseLevel> <http://www.w3.org/2000/01/rdf-schema#comment> """(#$academicCourseLevel COURSE COURSE-LEVEL) holds just in case COURSE is 
designed for students who are at the education level corresponding to COURSE-LEVEL.  For 
instance, if (#$academicCourseLevel McXFall02Phil101A-Sec1 #$FreshmanCourseLevel) holds,
then McXFall02Phil101A-Sec1 is designed for persons, PERSON such that 
(#$educationLevel PERSON #$FreshmanLevel).""" ;
	a <http://www.w3.org/2000/01/rdf-schema#Property> ;
	<http://sw.cyc.com/2006/07/27/cyc/prettyString-Canonical> "Academic Course Level" ;
	<http://www.w3.org/2000/01/rdf-schema#domain> <http://sw.cyc.com/2006/07/27/cyc/Course-Academic> ;
	<http://sw.cyc.com/2006/07/27/cyc/arity> "2"^^<http://www.w3.org/2001/XMLSchema#long> ;
	<http://www.w3.org/2000/01/rdf-schema#range> <http://sw.cyc.com/2006/07/27/cyc/CourseTypeByLevel> ;
	<http://www.w3.org/2000/01/rdf-schema#subPropertyOf> <http://www.w3.org/1999/02/22-rdf-syntax-ns#type> ;
	<http://sw.cyc.com/2006/07/27/cyc/arg2Genl> <http://sw.cyc.com/2006/07/27/cyc/Course-Academic> ;
	<http://sw.cyc.com/2006/07/27/cyc/typedGenlPreds> <http://www.w3.org/1999/02/22-rdf-syntax-ns#type> .

<http://sw.cyc.com/2006/07/27/cyc/Course-Academic> <http://www.w3.org/2000/01/rdf-schema#comment> "A specialization of #$Education.  This is the collection of academic courses.  Each instance is a temporally discontinuous event consisting of the events that constitute an academic course of study.  Going to the football game on some school night doesn't count as a subevent of an instance of this collection, but doing one's homework probably does.  Important specializations include: #$Course-Collegiate, #$HighSchoolCourseLevel, and #$ElementaryCourseLevel as well as  their specializations." ;
	a <http://www.w3.org/2002/07/owl#Class> ;
	<http://sw.cyc.com/2006/07/27/cyc/prettyString-Canonical> "course-academic" ;
	<http://www.w3.org/2000/01/rdf-schema#subClassOf> <http://sw.cyc.com/2006/07/27/cyc/Education> .

<http://sw.cyc.com/2006/07/27/cyc/CourseTypeByLevel> <http://www.w3.org/2000/01/rdf-schema#comment> """the collection of specializations of Course-Academic that includes all and only those collections that represent the academic level of a course.  This collection includes:
#$FreshmanCourseLevel, #$EleventhGradeCourseLevel, #$FirstGradeCourseLevel, etc..""" ;
	a <http://sw.cyc.com/2006/07/27/cyc/CollectionType> ;
	<http://sw.cyc.com/2006/07/27/cyc/prettyString-Canonical> "course type by level" ;
	<http://www.w3.org/2000/01/rdf-schema#subClassOf> <http://sw.cyc.com/2006/07/27/cyc/FirstOrderCollection> ;
	<http://sw.cyc.com/2006/07/27/cyc/typeGenls> <http://sw.cyc.com/2006/07/27/cyc/Course-Academic> .

<http://sw.cyc.com/2006/07/27/cyc/typedGenlPreds> <http://www.w3.org/2000/01/rdf-schema#comment> """A #$TaxonomicSlotForPredicates that is a specialization of #$genlPreds (q.v.).  <code>(#$typedGenlPreds SPECPRED GENLPRED)</code> means that <code>GENLPRED</code> is a more general version of <code>SPECPRED</code> that allows for more general argument types.  Futhermore, any sequence of things that stand in the relation <code>GENLPRED</code> and that satisfy all of the respective argument-constraints on <code>SPECPRED</code> also stand in the relation <code>SPECPRED</code>.  More precisely, the #$typedGenlPreds sentence above entails each of the following: 
<pre>
1. GENLPRED is a generalization of SPECPRED (see #$genlPreds). 

2. The individual argument-type constraints (see #$ArgIsaPredicate 
   and #$ArgGenlPredicate) on SPECPRED are all at least as narrow 
   as, and in at least one argument-place narrower than, the 
   corresponding constraints on GENLPRED. 

3. For any list of things ARGS such that (GENLPRED . ARGS) 
   holds and where the items in ARGS satisfy both (a) the 
   respective individual argument-type constraints on the 
   corresponding argument-places of SPECPRED and (b) any 
   <i>inter-argument</i> constraints (see #$InterArgTypePredicate) 
   on SPECPRED, (SPECPRED . ARGS) holds.
</pre>
For example, <code>(#$typedGenlPreds #$sisters #$siblings)</code> entails that if <code>(#$siblings John Alex)</code> holds and Alex is a #$FemaleAnimal (and thus satisfies the relatively narrower type-constraint on the second argument of #$sisters), then <code>(#$sisters John Alex)</code> holds.""" ;
	a <http://www.w3.org/2002/07/owl#TransitiveProperty> , <http://sw.cyc.com/2006/07/27/cyc/AntiSymmetricBinaryPredicate> , <http://sw.cyc.com/2006/07/27/cyc/ReflexiveBinaryPredicate> , <http://sw.cyc.com/2006/07/27/cyc/DefaultMonotonicPredicate> , <http://sw.cyc.com/2006/07/27/cyc/RuleMacroPredicate> , <http://sw.cyc.com/2006/07/27/cyc/MetaPredicate> , <http://sw.cyc.com/2006/07/27/cyc/VocabularyDefiningPredicate> , <http://sw.cyc.com/2006/07/27/cyc/TaxonomicSlotForPredicates> , <http://sw.cyc.com/2006/07/27/cyc/NLParsingDirectivePredicate> ;
	<http://sw.cyc.com/2006/07/27/cyc/prettyString-Canonical> "Typed Genl Preds" ;
	<http://sw.cyc.com/2006/07/27/cyc/quotedIsa> <http://sw.cyc.com/2006/07/27/cyc/OpenCycDefinitionalPredicate> , <http://sw.cyc.com/2006/07/27/cyc/DefinitionalPredicate> ;
	<http://www.w3.org/2000/01/rdf-schema#domain> <http://sw.cyc.com/2006/07/27/cyc/Predicate> ;
	<http://sw.cyc.com/2006/07/27/cyc/arity> "2"^^<http://www.w3.org/2001/XMLSchema#long> ;
	<http://www.w3.org/2000/01/rdf-schema#range> <http://sw.cyc.com/2006/07/27/cyc/Predicate> ;
	<http://www.w3.org/2000/01/rdf-schema#subPropertyOf> <http://www.w3.org/2000/01/rdf-schema#subPropertyOf> ;
	<http://sw.cyc.com/2006/07/27/cyc/arg1Format> <http://sw.cyc.com/2006/07/27/cyc/SetTheFormat> ;
	<http://sw.cyc.com/2006/07/27/cyc/arg2Format> <http://sw.cyc.com/2006/07/27/cyc/SetTheFormat> .

<http://sw.cyc.com/2006/07/27/cyc/AcademicCycles-Time-CSC> a <http://sw.cyc.com/2006/07/27/cyc/List> , <http://sw.cyc.com/2006/07/27/cyc/CycSubjectClump> ;
	<http://sw.cyc.com/2006/07/27/cyc/prettyString-Canonical> "Academic Cycles Time CSC" .

<http://sw.cyc.com/2006/07/27/cyc/CycSubjectClump> a <http://www.w3.org/2002/07/owl#Class> ;
	<http://sw.cyc.com/2006/07/27/cyc/prettyString-Canonical> "cyc subject clump" ;
	<http://www.w3.org/2000/01/rdf-schema#subClassOf> <http://www.w3.org/2002/07/owl#Thing> ;
	<http://sw.cyc.com/2006/07/27/cyc/quotedIsa> <http://sw.cyc.com/2006/07/27/cyc/DocumentationConstant> .

<http://sw.cyc.com/2006/07/27/cyc/AcademicCycles-Time-Topic> a <http://sw.cyc.com/2006/07/27/cyc/KBDependentCollection> , <http://sw.cyc.com/2006/07/27/cyc/CycVocabularyTopic> ;
	<http://sw.cyc.com/2006/07/27/cyc/prettyString-Canonical> "academic cycles time topic" ;
	<http://www.w3.org/2000/01/rdf-schema#subClassOf> <http://sw.cyc.com/2006/07/27/cyc/Time-Topic> .

<http://sw.cyc.com/2006/07/27/cyc/Time-Topic> a <http://sw.cyc.com/2006/07/27/cyc/KBDependentCollection> , <http://sw.cyc.com/2006/07/27/cyc/CycVocabularyTopLevelTopic> ;
	<http://sw.cyc.com/2006/07/27/cyc/prettyString-Canonical> "time-topic" ;
	<http://www.w3.org/2000/01/rdf-schema#subClassOf> <http://www.w3.org/2002/07/owl#Thing> .

<http://sw.cyc.com/2006/07/27/cyc/CycVocabularyTopic> <http://www.w3.org/2000/01/rdf-schema#comment> "An instance of #$FacetingCollectionType and a specialization of #$Topic.  Each instance of #$CycVocabularyTopic is a collection of #$Things falling under a topic for which some Cyc Vocabulary exists.  #$Topic is neither a strict [#$facets-Strict] nor a covering [#$facets-Covering] faceting of #$Thing: many #$Things may be instances of no #$Topic, or of multiple #$Topics." .

<http://sw.cyc.com/2006/07/27/cyc/AcademicOrganization> a <http://sw.cyc.com/2006/07/27/cyc/ExistingObjectType> ;
	<http://sw.cyc.com/2006/07/27/cyc/prettyString-Canonical> "academic organization" ;
	<http://sw.cyc.com/2006/07/27/cyc/prettyString> "academic organisation" , "academic organisations" , "academic organizations" ;
	<http://www.w3.org/2000/01/rdf-schema#subClassOf> <http://sw.cyc.com/2006/07/27/cyc/EducationalOrganization> .

<http://sw.cyc.com/2006/07/27/cyc/DepartmentTypeByFunction> <http://www.w3.org/2000/01/rdf-schema#comment> """A collection of collections and a specialization of #$OrganizationType.  Each instance of
#$DepartmentTypeByFunction is a collection of #$Departments 
(q.v.) whose instances are distinguished by the fact that 
they perform a certain function for an organization (e.g. 
#$BudgetDepartment and #$ShippingAndReceivingDepartment).  
See also #$DepartmentTypeByOrganization.""" ;
	a <http://sw.cyc.com/2006/07/27/cyc/SiblingDisjointCollectionType> , <http://sw.cyc.com/2006/07/27/cyc/FacetingCollectionType> , <http://sw.cyc.com/2006/07/27/cyc/SecondOrderCollection> ;
	<http://sw.cyc.com/2006/07/27/cyc/prettyString-Canonical> "type of department by function" ;
	<http://sw.cyc.com/2006/07/27/cyc/prettyString> "types of department by function" ;
	<http://www.w3.org/2000/01/rdf-schema#subClassOf> <http://sw.cyc.com/2006/07/27/cyc/FacetInstanceCollection> , <http://sw.cyc.com/2006/07/27/cyc/OrganizationType> ;
	<http://sw.cyc.com/2006/07/27/cyc/sharedNotes> <http://sw.cyc.com/2006/07/27/cyc/SharedNoteOnGenlsRelationsBetweenFacetingCollectionTypes> ;
	<http://sw.cyc.com/2006/07/27/cyc/typeGenls> <http://sw.cyc.com/2006/07/27/cyc/SomethingExisting> , <http://sw.cyc.com/2006/07/27/cyc/Department> .

<http://sw.cyc.com/2006/07/27/cyc/PartsOfOrganizations-Organization-Topic> a <http://sw.cyc.com/2006/07/27/cyc/KBDependentCollection> , <http://sw.cyc.com/2006/07/27/cyc/CycVocabularyTopic> ;
	<http://sw.cyc.com/2006/07/27/cyc/prettyString-Canonical> "parts of organizations organization topic" ;
	<http://www.w3.org/2000/01/rdf-schema#subClassOf> <http://sw.cyc.com/2006/07/27/cyc/Organization-Topic> .

<http://sw.cyc.com/2006/07/27/cyc/OrganizationTypeByActivityType> <http://www.w3.org/2000/01/rdf-schema#comment> "A #$FacetingCollectionType.  Each instance of #$OrganizationTypeByActivityType is a specialization of #$Organization whose instances engage in the same type of activity.  Instances of #$OrganizationTypeByActivityType include #$ResearchOrganization, #$SellingOrganization, and #$ServiceOrganization." ;
	a <http://sw.cyc.com/2006/07/27/cyc/FacetingCollectionType> , <http://sw.cyc.com/2006/07/27/cyc/SecondOrderCollection> ;
	<http://sw.cyc.com/2006/07/27/cyc/prettyString-Canonical> "type of organization classified by activity" ;
	<http://sw.cyc.com/2006/07/27/cyc/prettyString> "types of organization classified by activity" ;
	<http://www.w3.org/2000/01/rdf-schema#subClassOf> <http://sw.cyc.com/2006/07/27/cyc/FacetInstanceCollection> , <http://sw.cyc.com/2006/07/27/cyc/OrganizationType> ;
	<http://sw.cyc.com/2006/07/27/cyc/sharedNotes> <http://sw.cyc.com/2006/07/27/cyc/SharedNoteOnGenlsRelationsBetweenFacetingCollectionTypes> ;
	<http://www.w3.org/2002/07/owl#disjointWith> <http://sw.cyc.com/2006/07/27/cyc/AcademicDepartmentTypeBySubject> , <http://sw.cyc.com/2006/07/27/cyc/PhysiologicalConditionType> , <http://sw.cyc.com/2006/07/27/cyc/PersonTypeByCulture> ;
	<http://sw.cyc.com/2006/07/27/cyc/typeGenls> <http://sw.cyc.com/2006/07/27/cyc/Organization> .

<http://sw.cyc.com/2006/07/27/cyc/FacetInstanceCollection> <http://www.w3.org/2000/01/rdf-schema#comment> "A #$CollectionType.  Each instance of #$FacetInstanceCollection is a collection that is an instance of a #$FacetingCollectionType (q.v.).  For example, the facet-instance-collection (#$WineOfVintageFn (#$YearFn 1926)) is an instance of the faceting-collection-type #$WineTypeByVintage." ;
	a <http://sw.cyc.com/2006/07/27/cyc/CollectionType> ;
	<http://sw.cyc.com/2006/07/27/cyc/prettyString-Canonical> "facet collection" ;
	<http://sw.cyc.com/2006/07/27/cyc/prettyString> "facet instance collection" , "facet instance collections" , "facet collections" ;
	<http://www.w3.org/2000/01/rdf-schema#subClassOf> <http://www.w3.org/2002/07/owl#Class> .

<http://sw.cyc.com/2006/07/27/cyc/SiblingDisjointCollectionType> <http://www.w3.org/2000/01/rdf-schema#comment> """A #$KBDependentCollection of collections of  collections (and thus an instance of #$CollectionTypeType and a specialization of #$CollectionType).  A sibling-disjoint collection type is such that its known  (i.e. KB-represented) instances are collections that -- save for any that are related to each other by  #$genls and any that are explicitly asserted to be exceptions (see  #$siblingDisjointExceptions) -- are disjoint from each other. 
<p>
More precisely, each instance <code>SIB</code> of #$SiblingDisjointCollectionType is a collection of collections that has the following KB-dependent property: 
<p>
For any two known instances <code>COL1</code> and <code>COL2</code> of   <code>SIB</code>, at least one of the following is known to hold: 
<pre>
  (a) (#$genls COL1 COL2)
  (b) (#$genls COL2 COL1)
  (c) (#$siblingDisjointExceptions COL1 COL2)
  (d) (#$disjointWith COL1 COL2)
</pre>  
Moreover, note that if <code>MT</code> is a context (see #$Microtheory) in which (i) both <code>(#$isa COL1 SIB)</code> and <code>(#$isa COL2 SIB)</code> hold and (ii)  neither <code>(#$genls COL1 COL2)</code> nor <code>(#$genls COL2 COL1)</code> nor <code>(#$siblingDisjointExceptions COL1 COL2)</code> is known to hold (see #$knownSentence), then 
<code>(#$disjointWith COL1 COL2)</code> holds by default in <code>MT</code>.   
<p>
For example, in #$BiologyMt both #$Person and #$Dog are instances of the  sibling-disjoint collection type #$BiologicalSpecies, while neither  (#$genls #$Person #$Dog) nor (#$genls #$Dog #$Person) nor  (#$siblingDisjointExceptions #$Person #$Dog) is known to hold in that  context; consequently, (#$disjointWith #$Person #$Dog) holds by default  in #$BiologyMt.  Instances of #$SiblingDisjointCollectionType include  #$BiologicalTaxon (and its specializations), #$OrganismPartType, and #$RelationshipTypeByArity.
<p>
See the generalization #$SiblingDisjointSetOrCollectionType.  Also cf. the stronger notion of #$DisjointCollectionType.""" ;
	a <http://www.w3.org/2002/07/owl#Class> , <http://sw.cyc.com/2006/07/27/cyc/KBDependentCollection> , <http://sw.cyc.com/2006/07/27/cyc/AtemporalNecessarilyEssentialCollectionType> , <http://sw.cyc.com/2006/07/27/cyc/VariedOrderCollection> , <http://sw.cyc.com/2006/07/27/cyc/FacetingCollectionType> , <http://sw.cyc.com/2006/07/27/cyc/CollectionTypeType> , <http://sw.cyc.com/2006/07/27/cyc/CollectionTypeTypeByDisjointness> , <http://sw.cyc.com/2006/07/27/cyc/DisjointCollections-Fundamental-Topic> .

<http://sw.cyc.com/2006/07/27/cyc/AcademicQuarter> a <http://sw.cyc.com/2006/07/27/cyc/SpatiallyDisjointObjectType> , <http://sw.cyc.com/2006/07/27/cyc/TemporalObjectType> , <http://sw.cyc.com/2006/07/27/cyc/AcademicCycles-Time-Topic> , <http://sw.cyc.com/2006/07/27/cyc/ConventionalClassificationType> ;
	<http://sw.cyc.com/2006/07/27/cyc/prettyString-Canonical> "academic quarter" ;
	<http://sw.cyc.com/2006/07/27/cyc/prettyString> "quarter" , "quarters" , "academic quarters" ;
	<http://www.w3.org/2000/01/rdf-schema#subClassOf> <http://sw.cyc.com/2006/07/27/cyc/AcademicTerm> , <http://sw.cyc.com/2006/07/27/cyc/Container-Underspecified> ;
	<http://www.w3.org/2002/07/owl#disjointWith> <http://sw.cyc.com/2006/07/27/cyc/AcademicSemester> , <http://sw.cyc.com/2006/07/27/cyc/AcademicYear> .

<http://sw.cyc.com/2006/07/27/cyc/AcademicSemester> <http://www.w3.org/2000/01/rdf-schema#comment> "A specialization of #$AcademicTerm. Each instance of this collection is an occurrence consisting of the complex of scheduled activities taking place at an educational institution over a roughly 4-month long period.  This is not a collection of pure time intervals: note that, for example, the 2003 spring semesters at Boston University and at the University of Texas, Austin are represented by distinct, though of course temporally overlapping, instances." ;
	a <http://sw.cyc.com/2006/07/27/cyc/SpatiallyDisjointObjectType> , <http://sw.cyc.com/2006/07/27/cyc/TemporalObjectType> , <http://sw.cyc.com/2006/07/27/cyc/AcademicCycles-Time-Topic> , <http://sw.cyc.com/2006/07/27/cyc/ConventionalClassificationType> ;
	<http://sw.cyc.com/2006/07/27/cyc/prettyString-Canonical> "semester" ;
	<http://sw.cyc.com/2006/07/27/cyc/prettyString> "semesters" ;
	<http://www.w3.org/2000/01/rdf-schema#subClassOf> <http://sw.cyc.com/2006/07/27/cyc/AcademicTerm> , <http://sw.cyc.com/2006/07/27/cyc/Container-Underspecified> ;
	<http://www.w3.org/2002/07/owl#disjointWith> <http://sw.cyc.com/2006/07/27/cyc/AcademicYear> , <http://sw.cyc.com/2006/07/27/cyc/AcademicTrimester> .

<http://sw.cyc.com/2006/07/27/cyc/AcademicYear> <http://www.w3.org/2000/01/rdf-schema#comment> "Each instance of this collection is an annually recurring occurrence comprising the planned yearly activities at an educational institution. Thus, things of the form StanfordAcademicYear1997 and UCLAAcademicYear1997 are distinct instances of #$AcademicYear, even though they may occupy the same temporal extent (i.e., the same #$TimeInterval)." ;
	a <http://sw.cyc.com/2006/07/27/cyc/SpatiallyDisjointObjectType> , <http://sw.cyc.com/2006/07/27/cyc/TemporalObjectType> , <http://sw.cyc.com/2006/07/27/cyc/AcademicCycles-Time-Topic> , <http://sw.cyc.com/2006/07/27/cyc/ConventionalClassificationType> ;
	<http://sw.cyc.com/2006/07/27/cyc/prettyString-Canonical> "academic year" ;
	<http://sw.cyc.com/2006/07/27/cyc/prettyString> "school year" , "school years" , "academic years" ;
	<http://www.w3.org/2000/01/rdf-schema#subClassOf> <http://sw.cyc.com/2006/07/27/cyc/AcademicTerm> , <http://sw.cyc.com/2006/07/27/cyc/Container-Underspecified> .

<http://sw.cyc.com/2006/07/27/cyc/AcademicTerm> <http://www.w3.org/2000/01/rdf-schema#comment> "A specialization of #$Situation-Localized. An instance of this collection is the complex of planned activities constituting an academic term at a given educational institution: e.g., the 2003 spring semester at the University of Texas, Austin (cf. #$AcademicSemester). Note that this is not a pure time interval. A certain course, for instance, is a part (cf. #$subSituations) of a certain academic term. Salient specializations are #$AcademicYear and #$AcademicQuarter (qq.v)." ;
	a <http://sw.cyc.com/2006/07/27/cyc/SpatiallyDisjointObjectType> , <http://sw.cyc.com/2006/07/27/cyc/TemporalObjectType> , <http://sw.cyc.com/2006/07/27/cyc/AcademicCycles-Time-Topic> , <http://sw.cyc.com/2006/07/27/cyc/RegularlyRepeatedEventType> ;
	<http://sw.cyc.com/2006/07/27/cyc/prettyString-Canonical> "academic term" ;
	<http://www.w3.org/2000/01/rdf-schema#subClassOf> <http://sw.cyc.com/2006/07/27/cyc/Situation-Localized> , <http://sw.cyc.com/2006/07/27/cyc/Container-Underspecified> .

<http://sw.cyc.com/2006/07/27/cyc/Container-Underspecified> <http://www.w3.org/2000/01/rdf-schema#comment> "The collection of objects, tangible or otherwise, which are typically conceptualized by human beings for purposes of common-sense reasoning as containers. Thus, #$Container-Underspecified includes not only the set of all physical containers, like boxes and suitcases, but metaphoric containers as well (such as the #$Mind, which is a container of ideas; the #$Heart, which is a container of emotions; the #$Spleen, a container of anger, sentences, which are containers of words, arguments, which are containers of propositions, etc.)." ;
	a <http://sw.cyc.com/2006/07/27/cyc/KBDependentCollection> , <http://sw.cyc.com/2006/07/27/cyc/VariedOrderCollection> , <http://sw.cyc.com/2006/07/27/cyc/UnderspecifiedCollectionType> ;
	<http://sw.cyc.com/2006/07/27/cyc/prettyString-Canonical> "container underspecified" ;
	<http://www.w3.org/2000/01/rdf-schema#subClassOf> <http://sw.cyc.com/2006/07/27/cyc/Region-Underspecified> .

<http://sw.cyc.com/2006/07/27/cyc/ConventionalClassificationType> <http://www.w3.org/2000/01/rdf-schema#comment> "A collection of collections.  Each instance of #$ConventionalClassificationType is a collection that corresponds to a category in some agreed-upon or conventional classification system (see #$ClassificationSystem) used by people.  In such systems, a change or reclassification is possible by a decision of an authority, or by a changed social agreement or custom, without changing the intrinsic natures of the actual objects in the category.   #$ConventionalClassificationTypes include categories in biological taxonomy, standard classifications in data dictionaries and thesauri, cultural taboo classes, military doctrinal classes, and named calendar intervals." ;
	a <http://sw.cyc.com/2006/07/27/cyc/CollectionType> , <http://sw.cyc.com/2006/07/27/cyc/VariedOrderCollection> , <http://sw.cyc.com/2006/07/27/cyc/FacetingCollectionType> , <http://sw.cyc.com/2006/07/27/cyc/InformationAndCWs-Topic> , <http://sw.cyc.com/2006/07/27/cyc/CandidateKBCompletenessNode> ;
	<http://sw.cyc.com/2006/07/27/cyc/prettyString-Canonical> "conventional classification type" ;
	<http://sw.cyc.com/2006/07/27/cyc/prettyString> "conventional classification types" ;
	<http://www.w3.org/2000/01/rdf-schema#subClassOf> <http://www.w3.org/2002/07/owl#Class> ;
	<http://sw.cyc.com/2006/07/27/cyc/sharedNotes> <http://sw.cyc.com/2006/07/27/cyc/NoteOnCycMergedOntologyConstants> ;
	<http://www.w3.org/2002/07/owl#disjointWith> <http://sw.cyc.com/2006/07/27/cyc/OrganismConstituentType> .

<http://sw.cyc.com/2006/07/27/cyc/AcademicTrimester> <http://www.w3.org/2000/01/rdf-schema#comment> "A specialization of #$AcademicTerm. Each instance of this collection is an occurrence consisting of the complex of scheduled activities taking place at an educational institution over a roughly 3-month long period.  This is not a collection of pure time intervals: note that, for example, the 2003 summer trimester at the University of Wellington and at Otago University would be represented by distinct, though most likely temporally overlapping, instances." ;
	a <http://sw.cyc.com/2006/07/27/cyc/SpatiallyDisjointObjectType> , <http://sw.cyc.com/2006/07/27/cyc/TemporalObjectType> , <http://sw.cyc.com/2006/07/27/cyc/AcademicCycles-Time-Topic> , <http://sw.cyc.com/2006/07/27/cyc/ConventionalClassificationType> ;
	<http://sw.cyc.com/2006/07/27/cyc/prettyString-Canonical> "trimester" ;
	<http://sw.cyc.com/2006/07/27/cyc/prettyString> "trimesters" ;
	<http://www.w3.org/2000/01/rdf-schema#subClassOf> <http://sw.cyc.com/2006/07/27/cyc/Container-Underspecified> ;
	<http://www.w3.org/2002/07/owl#disjointWith> <http://sw.cyc.com/2006/07/27/cyc/AcademicYear> .

<http://sw.cyc.com/2006/07/27/cyc/RegularlyRepeatedEventType> <http://www.w3.org/2000/01/rdf-schema#comment> """A specialization of #$RepeatedEventType (q.v.).  Each instance of #$RegularlyRepeatedEventType is a collection of events whose instances typically occur along with other instances of the same event-type at more or less regular intervals.  These regular occurrences might be the result of natural phenomena (e.g. the sunrise), human convention (e.g. the execution of a dance step within a given dancing event), or a combination of both (e.g. the annual celebration of Oktoberfest).
<p>
Other examples of #$RegularlyRepeatedEventType are #$OlympicGames, #$AcademicTerm, and #$TakingABreath.
<p>
See also #$IterativeEvent and #$IterativeEventType.""" ;
	a <http://sw.cyc.com/2006/07/27/cyc/SecondOrderCollection> , <http://sw.cyc.com/2006/07/27/cyc/RepeatedEvents-Time-Topic> ;
	<http://sw.cyc.com/2006/07/27/cyc/prettyString-Canonical> "periodic event" ;
	<http://sw.cyc.com/2006/07/27/cyc/prettyString> "regular" , "more regular" , "most regular" , "periodic" , "more periodic" , "most periodic" , "periodic events" ;
	<http://www.w3.org/2000/01/rdf-schema#subClassOf> <http://sw.cyc.com/2006/07/27/cyc/RepeatedEventType> .

<http://sw.cyc.com/2006/07/27/cyc/AcademicTest> <http://www.w3.org/2000/01/rdf-schema#comment> "The collection of #$PropositionalInformationThings whose instances are usually a set of questions designed to test a student's understanding of a certain subject.  See #$AcademicTesting." ;
	a <http://sw.cyc.com/2006/07/27/cyc/ObjectType> ;
	<http://sw.cyc.com/2006/07/27/cyc/prettyString-Canonical> "academic test" ;
	<http://sw.cyc.com/2006/07/27/cyc/prettyString> "academic tests" ;
	<http://www.w3.org/2000/01/rdf-schema#subClassOf> <http://sw.cyc.com/2006/07/27/cyc/NonfictionalPCW> .

<http://sw.cyc.com/2006/07/27/cyc/NonfictionalPCW> <http://www.w3.org/2000/01/rdf-schema#comment> "The collection of all #$PropositionalConceptualWorks that are nonfictional." ;
	a <http://sw.cyc.com/2006/07/27/cyc/ObjectType> ;
	<http://sw.cyc.com/2006/07/27/cyc/prettyString-Canonical> "nonfictional pcw" ;
	<http://www.w3.org/2000/01/rdf-schema#subClassOf> <http://sw.cyc.com/2006/07/27/cyc/PropositionalConceptualWork> .

<http://sw.cyc.com/2006/07/27/cyc/AcademicTesting> <http://www.w3.org/2000/01/rdf-schema#comment> "The collection of #$PerformanceTesting events in which some #$IntelligentAgent measures some aspect of another agent's academic achievement using a generic method to collect and analyze the relevant data.  #$AcademicTests are generic in the sense that individual such tests are not tailored to the person tested.  They typically consist of a series of questions that the student must answer." ;
	a <http://sw.cyc.com/2006/07/27/cyc/FirstOrderCollection> ;
	<http://sw.cyc.com/2006/07/27/cyc/prettyString-Canonical> "academic testing" ;
	<http://sw.cyc.com/2006/07/27/cyc/prettyString> "examinations" , "quiz" , "quizzed" , "quizzes" , "quizzing" , "have quizzed" , "has quizzed" , "will quiz" , "had quizzed" , "will have quizzed" , "exam" , "exams" , "test" , "tested" , "tests" , "testing" , "have tested" , "has tested" , "will test" , "had tested" , "will have tested" , "examination" ;
	<http://www.w3.org/2000/01/rdf-schema#subClassOf> <http://sw.cyc.com/2006/07/27/cyc/PerformanceTesting> .

<http://sw.cyc.com/2006/07/27/cyc/AcademyAward> <http://sw.cyc.com/2006/07/27/cyc/prettyString-Canonical> "Academy Award" ;
	<http://sw.cyc.com/2006/07/27/cyc/prettyString> "Oscar" , "Oscars" , "Oscar Award" , "Oscar Awards" , "Academy Awards" ;
	<http://www.w3.org/2000/01/rdf-schema#subClassOf> <http://sw.cyc.com/2006/07/27/cyc/AwardPractice> .

<http://sw.cyc.com/2006/07/27/cyc/AcademyAwardFn> <http://www.w3.org/2000/01/rdf-schema#comment> "(#$AcademyAwardFn CATEGORY YEAR) denotes the Academy Award given in the #$AcademyAwardCategory CATEGORY for the #$CalendarYear YEAR.  Note that there is one award per year.  The award may be shared, in which case two Oscar statues will be given (more if collaborators are involved).  See also #$AcademyAward." ;
	a <http://sw.cyc.com/2006/07/27/cyc/ReifiableFunction> , <http://sw.cyc.com/2006/07/27/cyc/BinaryFunction> , <http://sw.cyc.com/2006/07/27/cyc/IndividualDenotingFunction> ;
	<http://sw.cyc.com/2006/07/27/cyc/prettyString-Canonical> "Academy Award Fn" ;
	<http://www.w3.org/2000/01/rdf-schema#domain> <http://sw.cyc.com/2006/07/27/cyc/AcademyAwardCategory> ;
	<http://sw.cyc.com/2006/07/27/cyc/arity> "2"^^<http://www.w3.org/2001/XMLSchema#long> ;
	<http://www.w3.org/2000/01/rdf-schema#range> <http://sw.cyc.com/2006/07/27/cyc/CalendarYear> ;
	<http://sw.cyc.com/2006/07/27/cyc/resultIsaArg> "1"^^<http://www.w3.org/2001/XMLSchema#long> ;
	<http://sw.cyc.com/2006/07/27/cyc/resultIsa> <http://sw.cyc.com/2006/07/27/cyc/AcademyAward> .

<http://sw.cyc.com/2006/07/27/cyc/CalendarYear> <http://www.w3.org/2000/01/rdf-schema#comment> "A subcollection of #$Date (q.v.) and an instance of #$CalendarCoveringType (q.v.).  Each instance of #$CalendarYear is a year in some particular calendar.  Examples include #$TheYear1972 and (#$YearFn 2001).  Note that (as with any instance of an instance of calendar-covering-type) a given calendar-year is a temporally-continuous individual that occurs only _once_; e.g. it is not something that recurs each century or each millenium." ;
	a <http://sw.cyc.com/2006/07/27/cyc/NormalTimeParameter> , <http://sw.cyc.com/2006/07/27/cyc/DateFunctions-Time-Topic> , <http://sw.cyc.com/2006/07/27/cyc/CalendarCoveringType> , <http://sw.cyc.com/2006/07/27/cyc/ConventionallyClassifiedTimeIntervalSeries-CoveringAndDisjoint> , <http://sw.cyc.com/2006/07/27/cyc/TimeOfYearType> ;
	<http://sw.cyc.com/2006/07/27/cyc/prettyString-Canonical> "year" ;
	<http://sw.cyc.com/2006/07/27/cyc/prettyString> "calendar year" , "calendar years" , "years" ;
	<http://www.w3.org/2000/01/rdf-schema#subClassOf> <http://www.w3.org/2001/XMLSchema#date> ;
	<http://sw.cyc.com/2006/07/27/cyc/definingTimeUnit> <http://sw.cyc.com/2006/07/27/cyc/YearsDuration> .

<http://sw.cyc.com/2006/07/27/cyc/AwardPractice> <http://www.w3.org/2000/01/rdf-schema#comment> "A collection of intangibles.  Each instance of #$AwardPractice is a distinction bestowed upon someone or something by an appropriately authorized agent, generally in recognition of some accomplishment and often as a result of a competitive process.  Awards may be given to people, books, buildings, cities, etc.  Note that this collection represents the awards themselves rather than tangible symbols of awards, such as medals or Oscar statuettes.  Nor do its instances represent any money that might accompany an award.  See also #$SymbolicObject, #$Token-Physical." ;
	a <http://sw.cyc.com/2006/07/27/cyc/ObjectType> , <http://sw.cyc.com/2006/07/27/cyc/CandidateKBCompletenessNode> ;
	<http://sw.cyc.com/2006/07/27/cyc/prettyString-Canonical> "award" ;
	<http://sw.cyc.com/2006/07/27/cyc/prettyString> "accolade" , "accolades" , "prize" , "prizes" , "honour" , "honor" , "honours" , "honors" , "awards" ;
	<http://www.w3.org/2000/01/rdf-schema#subClassOf> <http://sw.cyc.com/2006/07/27/cyc/DevisedPracticeOrWork> ;
	<http://www.w3.org/2002/07/owl#disjointWith> <http://sw.cyc.com/2006/07/27/cyc/ConceptualWork> , <http://sw.cyc.com/2006/07/27/cyc/CommunicationConvention> .

<http://sw.cyc.com/2006/07/27/cyc/academyAwardNominee> <http://www.w3.org/2000/01/rdf-schema#comment> "(#$academyAwardNominee AWARD NOMINEE MOVIE) means that NOMINEE was nominated for the #$AcademyAward AWARD, for work on the film MOVIE. Note that the year of the nomination will be contained in the name of the term used for AWARD.  See also #$AcademyAwardFn." ;
	a <http://sw.cyc.com/2006/07/27/cyc/TernaryPredicate> , <http://sw.cyc.com/2006/07/27/cyc/MoviePredicate> , <http://sw.cyc.com/2006/07/27/cyc/Entertainment-Topic> .

<http://sw.cyc.com/2006/07/27/cyc/AcademyAwardWinner-Template> <http://sw.cyc.com/2006/07/27/cyc/prettyString-Canonical> "Academy Award Winner Template" .

<http://sw.cyc.com/2006/07/27/cyc/AcademyInsuranceGroup-Corporation> a <http://sw.cyc.com/2006/07/27/cyc/Individual> ;
	<http://sw.cyc.com/2006/07/27/cyc/prettyString-Canonical> "Academy Insurance Group" .

<http://sw.cyc.com/2006/07/27/cyc/AcademyOfMotionPictureArtsAndSciences> <http://www.w3.org/2000/01/rdf-schema#comment> "A professional organization, based in California, that promotes the development of motion picture arts and sciences by sponsoring awards, education, and research.  See also #$AcademyAward." ;
	a <http://sw.cyc.com/2006/07/27/cyc/Individual> , <http://sw.cyc.com/2006/07/27/cyc/ProfessionalAssociation> ;
	<http://sw.cyc.com/2006/07/27/cyc/prettyString-Canonical> "Academy of Motion Picture Arts and Sciences" .

<http://sw.cyc.com/2006/07/27/cyc/ProfessionalAssociation> <http://www.w3.org/2000/01/rdf-schema#comment> "A collection of organizations.  Each element of #$ProfessionalOrganization is a group consisting of professionally trained, white-collar workers as members.  Usually, the members of a particular professional organization belong to a single profession (or a related group of professions).  Examples: #$AmericanMedicalAssociation, #$AmericanOsteopathyAssociation." ;
	a <http://sw.cyc.com/2006/07/27/cyc/ExistingObjectType> , <http://sw.cyc.com/2006/07/27/cyc/MiscellaneousOrganizationConstants-Organization-Topic> ;
	<http://sw.cyc.com/2006/07/27/cyc/prettyString-Canonical> "Professional society" ;
	<http://sw.cyc.com/2006/07/27/cyc/prettyString> "professional organization" , "professional organisation" , "professional organisations" , "professional organizations" , "professional association" , "professional associations" , "Professional societies" ;
	<http://www.w3.org/2000/01/rdf-schema#subClassOf> <http://sw.cyc.com/2006/07/27/cyc/AdvocacyOrganization> , <http://sw.cyc.com/2006/07/27/cyc/WorkersOrganization> , <http://sw.cyc.com/2006/07/27/cyc/ProfessionalOrganization> ;
	<http://www.w3.org/2002/07/owl#disjointWith> <http://sw.cyc.com/2006/07/27/cyc/ActivityTypeFocusGroup> , <http://sw.cyc.com/2006/07/27/cyc/FoodAndBeverageOrganization> .

<http://sw.cyc.com/2006/07/27/cyc/AcadiaNationalPark> a <http://sw.cyc.com/2006/07/27/cyc/Individual> , <http://sw.cyc.com/2006/07/27/cyc/NationalPark> ;
	<http://sw.cyc.com/2006/07/27/cyc/prettyString-Canonical> "Acadia" ;
	<http://sw.cyc.com/2006/07/27/cyc/prettyString> "Acadia National Park" .

<http://sw.cyc.com/2006/07/27/cyc/NationalPark> <http://www.w3.org/2000/01/rdf-schema#comment> "A specialization of #$WildernessPark.  Each instance of #$NationalPark is a park in the wilderness that is managed by the national government of the country in which it is located." ;
	a <http://sw.cyc.com/2006/07/27/cyc/ExistingObjectType> , <http://sw.cyc.com/2006/07/27/cyc/SpatiallyDisjointObjectType> , <http://sw.cyc.com/2006/07/27/cyc/ArtifactualFeatureType> ;
	<http://sw.cyc.com/2006/07/27/cyc/prettyString-Canonical> "national park" ;
	<http://sw.cyc.com/2006/07/27/cyc/prettyString> "national parks" ;
	<http://www.w3.org/2000/01/rdf-schema#subClassOf> <http://sw.cyc.com/2006/07/27/cyc/TouristAttraction> , <http://sw.cyc.com/2006/07/27/cyc/WildernessPark> .

<http://sw.cyc.com/2006/07/27/cyc/AcadiaRealtyTrust> a <http://sw.cyc.com/2006/07/27/cyc/Individual> , <http://sw.cyc.com/2006/07/27/cyc/PubliclyHeldCorporation> ;
	<http://sw.cyc.com/2006/07/27/cyc/prettyString-Canonical> "Acadia Realty Trust" .

<http://sw.cyc.com/2006/07/27/cyc/AcajutlaMexicanRestaurant-Washington-FoodServiceEstablishment> <http://sw.cyc.com/2006/07/27/cyc/prettyString-Canonical> "Acajutla Mexican Restaurant - Washington" .

<http://sw.cyc.com/2006/07/27/cyc/Acanthite> a <http://sw.cyc.com/2006/07/27/cyc/ExistingStuffType> ;
	<http://sw.cyc.com/2006/07/27/cyc/prettyString-Canonical> "acanthite" ;
	<http://www.w3.org/2000/01/rdf-schema#subClassOf> <http://sw.cyc.com/2006/07/27/cyc/Mineral> .

<http://sw.cyc.com/2006/07/27/cyc/Mineral> <http://www.w3.org/2000/01/rdf-schema#comment> "A specialization of #$InanimateObject-Natural.  Each instance of #$Mineral is a piece of homogeneous inorganic physical substance that has a crystalline structure.  Specializations of #$Mineral include the collections #$Diamond, #$Turquoise-Gem, #$Jade-Gem, and #$Corundum." ;
	a <http://sw.cyc.com/2006/07/27/cyc/ExistingStuffType> , <http://sw.cyc.com/2006/07/27/cyc/CommonSubstances-Material-Topic> ;
	<http://sw.cyc.com/2006/07/27/cyc/prettyString-Canonical> "Mineral" ;
	<http://sw.cyc.com/2006/07/27/cyc/prettyString> "minerals" ;
	<http://www.w3.org/2000/01/rdf-schema#subClassOf> <http://sw.cyc.com/2006/07/27/cyc/Crystalline> , <http://sw.cyc.com/2006/07/27/cyc/InorganicMaterial> .

<http://sw.cyc.com/2006/07/27/cyc/ACappellaMusicPerformers> <http://www.w3.org/2000/01/rdf-schema#comment> "The collection of individuals or groups that perform a cappella music." ;
	a <http://sw.cyc.com/2006/07/27/cyc/ExistingObjectType> , <http://sw.cyc.com/2006/07/27/cyc/ObjectType> ;
	<http://sw.cyc.com/2006/07/27/cyc/prettyString-Canonical> "A cappella music performers" .

<http://sw.cyc.com/2006/07/27/cyc/accedingTo> a <http://www.w3.org/2000/01/rdf-schema#Property> ;
	<http://sw.cyc.com/2006/07/27/cyc/prettyString-Canonical> "Acceding To" ;
	<http://www.w3.org/2000/01/rdf-schema#domain> <http://sw.cyc.com/2006/07/27/cyc/Accepting-CommunicationAct> ;
	<http://sw.cyc.com/2006/07/27/cyc/arity> "2"^^<http://www.w3.org/2001/XMLSchema#long> ;
	<http://www.w3.org/2000/01/rdf-schema#range> <http://sw.cyc.com/2006/07/27/cyc/PropositionalInformationThing> .

<http://sw.cyc.com/2006/07/27/cyc/Accepting-CommunicationAct> <http://www.w3.org/2000/01/rdf-schema#comment> "An acknowledgement in which the performer affirms what was communicated to them in a prior communication." ;
	a <http://sw.cyc.com/2006/07/27/cyc/TemporalObjectType> ;
	<http://sw.cyc.com/2006/07/27/cyc/prettyString-Canonical> "accepting communication act" ;
	<http://www.w3.org/2000/01/rdf-schema#subClassOf> <http://sw.cyc.com/2006/07/27/cyc/Acknowledging-CommunicationAct> .

<http://sw.cyc.com/2006/07/27/cyc/AcceleratedX-TheProgram> <http://www.w3.org/2000/01/rdf-schema#comment> "A popular commercial X server available from Xi Graphics. " ;
	a <http://sw.cyc.com/2006/07/27/cyc/Individual> , <http://sw.cyc.com/2006/07/27/cyc/UnversionedProgram> , <http://sw.cyc.com/2006/07/27/cyc/LocalProgram> ;
	<http://sw.cyc.com/2006/07/27/cyc/prettyString-Canonical> "Accelerated X" .

<http://sw.cyc.com/2006/07/27/cyc/Accelerating-Rotational> <http://www.w3.org/2000/01/rdf-schema#comment> "#$Accelerating-Rotational occurs whenever the angular velocity of the #$objectMoving changes, e.g. spinning faster or slower or changing the axis along which spinning occurs." ;
	a <http://sw.cyc.com/2006/07/27/cyc/TemporalStuffType> ;
	<http://sw.cyc.com/2006/07/27/cyc/prettyString-Canonical> "accelerating rotational" ;
	<http://www.w3.org/2000/01/rdf-schema#subClassOf> <http://sw.cyc.com/2006/07/27/cyc/Movement-Rotation> .

<http://sw.cyc.com/2006/07/27/cyc/Movement-Rotation> <http://www.w3.org/2000/01/rdf-schema#comment> "A specialization of #$MovementEvent.  In each instance of  #$Movement-Rotation the most salient moving object (see  #$primaryObjectMoving) rotates (see #$objectRotating). That is, the object rotates about an axis (see  #$axisOfRotation) that spatially intersects it (or goes  through a hole in it).  Examples include the daily  rotation of the Earth on its axis and the rotation of a  clock hand about its fastened end.  A non-example is the  orbiting of the Earth around the sun, as the axis of the  orbit does not spatially intersect the Earth." ;
	a <http://sw.cyc.com/2006/07/27/cyc/QAClarifyingCollectionType> .

<http://sw.cyc.com/2006/07/27/cyc/AccelerationClause> <http://sw.cyc.com/2006/07/27/cyc/prettyString-Canonical> "acceleration clause" ;
	<http://sw.cyc.com/2006/07/27/cyc/prettyString> "acceleration clauses" ;
	<http://www.w3.org/2000/01/rdf-schema#subClassOf> <http://sw.cyc.com/2006/07/27/cyc/Obligation> .

<http://sw.cyc.com/2006/07/27/cyc/Obligation> <http://www.w3.org/2000/01/rdf-schema#comment> "A specialization of #$NormativeSpecification.  Each instance of the collection #$Obligation is specification of what some agent (related to the obligation via #$obligatedAgents (q.v.)) is obliged to do, or make true, for one or more other agents or possibly 'for' society in general.  An obligation is the most general case of some agent owing something to another.  Obligations may be undertaken in conjunction with various kinds of #$Agreements.   Unlike an agreement, however, an obligation need not have a second known party (though some do).  An obligation can exist and be understood without identifying another particular agent as the 'holder' of the obligation -- and that may be true, even if the beneficiary (#$obligationOwedTo) can be identified.  For example, assuming that parents have an obligation to care for their children, it is not clear with whom a parent has 'agreed' to take care of his or her child.  Some common ways to incur an obligation are through social transactions (e.g. family duties, friendship, favors) or through financial transactions (e.g. a #$PaymentObligation).   In addition, obligations may be imposed on those who are subject to one or more instances of #$CodeOfConduct, e.g. #$SportsRulesOf-BoxingSportsEvent or #$OfficeCodeOfConductMt." ;
	a <http://sw.cyc.com/2006/07/27/cyc/TemporalStuffType> , <http://sw.cyc.com/2006/07/27/cyc/SomeSampleKindsOfAgreements-Agreement-Topic> , <http://sw.cyc.com/2006/07/27/cyc/Mt-Topic> , <http://sw.cyc.com/2006/07/27/cyc/SomeTypesOfMicrotheories-MtExpansion-Topic> ;
	<http://sw.cyc.com/2006/07/27/cyc/prettyString-Canonical> "obligation" ;
	<http://sw.cyc.com/2006/07/27/cyc/prettyString> "commitment" , "mandates" , "mandate" , "onus" , "onuses" , "restriction" , "restrictions" , "commitments" , "obligations" ;
	<http://www.w3.org/2000/01/rdf-schema#subClassOf> <http://sw.cyc.com/2006/07/27/cyc/NormativeSpecification> ;
	<http://www.w3.org/2002/07/owl#disjointWith> <http://sw.cyc.com/2006/07/27/cyc/Proposal> ;
	<http://sw.cyc.com/2006/07/27/cyc/facets-Generic> <http://sw.cyc.com/2006/07/27/cyc/JointStaffResponsibilityType> .

<http://sw.cyc.com/2006/07/27/cyc/Acceleration> <http://www.w3.org/2000/01/rdf-schema#comment> "Acceleration is the change in speed of an object per unit time.  It is a measurable physical quantity, measured in units such as MilesPerHourPerSecond." ;
	a <http://sw.cyc.com/2006/07/27/cyc/AtemporalNecessarilyEssentialCollectionType> , <http://sw.cyc.com/2006/07/27/cyc/UnitOfMeasureConcept> , <http://sw.cyc.com/2006/07/27/cyc/DerivedMeasurableQuantityType> , <http://sw.cyc.com/2006/07/27/cyc/ScalarIntervals-Quantity-Topic> ;
	<http://sw.cyc.com/2006/07/27/cyc/prettyString-Canonical> "acceleration" ;
	<http://sw.cyc.com/2006/07/27/cyc/prettyString> "accelerations" ;
	<http://www.w3.org/2000/01/rdf-schema#subClassOf> <http://sw.cyc.com/2006/07/27/cyc/Rate> , <http://sw.cyc.com/2006/07/27/cyc/PhysicalQuantity> , <http://sw.cyc.com/2006/07/27/cyc/ThreeDimensionalQuantity> .

<http://sw.cyc.com/2006/07/27/cyc/AccelerationDueToGravity> <http://www.w3.org/2000/01/rdf-schema#comment> "A specialization of #$Acceleration. #$AccelerationDueToGravity is the collection of all accelerations that are accelerations of objects due to gravity. See #$accelerationDueToGravityOnPlanetaryBody." ;
	a <http://www.w3.org/2002/07/owl#Class> , <http://sw.cyc.com/2006/07/27/cyc/FirstOrderCollection> , <http://sw.cyc.com/2006/07/27/cyc/SetOrCollection> , <http://sw.cyc.com/2006/07/27/cyc/DerivedMeasurableQuantityType> ;
	<http://sw.cyc.com/2006/07/27/cyc/prettyString-Canonical> "acceleration due to gravity" ;
	<http://sw.cyc.com/2006/07/27/cyc/prettyString> "acceleration that has been Acceleration Due To Gravity On Planetary Body of a planetary body" , "accelerations that has been Acceleration Due To Gravity On Planetary Body of a planetary body" , "accelerations that is Acceleration Due To Gravity On Planetary Body of a planetary body" ;
	<http://www.w3.org/2000/01/rdf-schema#subClassOf> <http://sw.cyc.com/2006/07/27/cyc/Acceleration> , <http://sw.cyc.com/2006/07/27/cyc/MultiDimensionalQuantity> ;
	<http://sw.cyc.com/2006/07/27/cyc/quotedIsa> <http://sw.cyc.com/2006/07/27/cyc/WordNetWorkflowConstant-NotFullyReviewed> .

<http://sw.cyc.com/2006/07/27/cyc/MultiDimensionalQuantity> <http://www.w3.org/2000/01/rdf-schema#comment> """A specialization of #$MeasurableQuantity (q.v.).  Each instance of #$MultiDimensionalQuantity is a measurable quantity that is defined as the product or ratio of other quantities.  For example, (#$MilesPerHour 65) is a multi-dimensional quantity obtainable by dividing (#$Mile 65) by (#$HoursDuration 1), and (#$CubicMeter 8) is a derived quantity obtainable by multiplying (#$Meter 2) by itself twice.  In contrast, (#$Mile 65), (#$HoursDuration 1), and (#$Meter 2) are all instances of #$OneDimensionalQuantity (cf.).
<p>
Each multi-dimensional quantity is in principle equal to the result of applying some (reified or otherwise) #$MultiDimensionalUnitOfMeasure (q.v.) to some number or other #$NumericInterval (or pair of numeric-intervals).
<p>
When a <i>one-dimensional</i> quantity is multiplied or divided by another one-dimensional quantity, the result is always a multi-dimensional quantity.  But note that this is <i>not</i> true of the results of multiplying and dividing quantities generally.  For example, (#$ProductFn (#$MilesPerHour 65) (#$HoursDuration 1)) is equal to the one-dimensional quantity (#$Mile 65).)
<p>
Specializations of #$MultiDimensionalQuantity include #$TwoDimensionalQuantity and #$ThreeDimensionalQuantity.""" ;
	a <http://sw.cyc.com/2006/07/27/cyc/AtemporalNecessarilyEssentialCollectionType> ;
	<http://sw.cyc.com/2006/07/27/cyc/prettyString-Canonical> "multi dimensional quantity" ;
	<http://www.w3.org/2000/01/rdf-schema#subClassOf> <http://sw.cyc.com/2006/07/27/cyc/MeasurableQuantity> .

<http://sw.cyc.com/2006/07/27/cyc/SetOrCollection> <http://www.w3.org/2000/01/rdf-schema#comment> "A specialization of #$MathematicalThing.  Something is an instance of #$SetOrCollection just in case it is a collection (i.e. an instance of #$Collection) or a mathematical set (i.e. an instance of #$Set-Mathematical).  Instances of #$Set-Mathematical and instances of #$Collection (and thus instances of #$SetOrCollection) share some basic common features.  All instances of #$Collection and all instances of #$Set-Mathematical (and thus all instances of #$SetOrCollection) are abstract entities, lacking spatial and temporal properties.  Nearly all instances of #$Collection (except \"empty\" collections) and nearly all instances of #$Set-Mathematical (except the empty set; see #$TheEmptySet) have \"elements\" (i.e. instances or members; see #$elementOf); hence set-or-collections may stand to one another in generalized set-theoretic relations such as #$subsetOf and #$disjointWith (qq.v.).  (It is this shared feature of having elements that provides the basic rationale for reifying the collection #$SetOrCollection.)  Nevertheless, sets and collections differ in two important ways.  First, each collection is intrinsically associated with an intensional criterion for membership -- a more or less natural property (or group of properties) possessed by all of (and only) its elements.  Collections are thus akin to kinds.  In contrast, the elements of a set are not required to be homogeneous in any respect: any things whatsoever may together constitute the elements of a set.  The second major difference between sets and collections is that no two distinct sets can be coextensional (i.e. have exactly the same elements; see #$coExtensional).  Sets can thus be identified purely on the basis of their extensions (see #$extent).  Collections, on the other hand, are individuated by their intensional criteria for membership.  So collections that have exactly the same elements might nevertheless be distinct, differing in their respective membership criteria.  (Note that the general relationship between collections and their \"intensional criteria for membership\" in the above sense is not something that is currently represented explicitly in the Knowledge Base (though this seems a worthwhile area for future work); still the #$comment and other \"definitional\" assertions on a given collection should ideally convey a reasonably clear and precise idea of its associated membership criterion.)" ;
	a <http://www.w3.org/2002/07/owl#Class> , <http://sw.cyc.com/2006/07/27/cyc/AtemporalNecessarilyEssentialCollectionType> , <http://sw.cyc.com/2006/07/27/cyc/VariedOrderCollection> , <http://sw.cyc.com/2006/07/27/cyc/SetOrCollectionType> , <http://sw.cyc.com/2006/07/27/cyc/SubsetsOfMathematicalThing-Math-Topic> ;
	<http://sw.cyc.com/2006/07/27/cyc/prettyString-Canonical> "intensional or extensional set" ;
	<http://sw.cyc.com/2006/07/27/cyc/prettyString> "the union of { types of thing, sets }" , "intensional or extensional sets" ;
	<http://www.w3.org/2000/01/rdf-schema#subClassOf> <http://www.w3.org/2002/07/owl#Thing> , <http://sw.cyc.com/2006/07/27/cyc/AbstractThing> , <http://sw.cyc.com/2006/07/27/cyc/MathematicalThing> ;
	<http://sw.cyc.com/2006/07/27/cyc/facets-Covering> <http://sw.cyc.com/2006/07/27/cyc/SetOrCollectionTypeByCardinality> ;
	<http://sw.cyc.com/2006/07/27/cyc/requiredArg1Pred> <http://sw.cyc.com/2006/07/27/cyc/subsetOf> ;
	<http://sw.cyc.com/2006/07/27/cyc/collectionConventionMt> <http://sw.cyc.com/2006/07/27/cyc/UniversalVocabularyMt> .

<http://sw.cyc.com/2006/07/27/cyc/DerivedMeasurableQuantityType> <http://www.w3.org/2000/01/rdf-schema#comment> """A collection of collections and a specialization of both #$MeasurableScalarIntervalType and #$TotallyOrderedQuantityType (qq.v.).  Each instance of #$DerivedMeasurableQuantityType is a totally-ordered collection of instances of #$MultiDimensionalQuantity: measurable quantities that are derived from some more basic quantities (via e.g. #$ProductFn or #$QuotientFn).   Examples include #$Volume, #$Area, and #$Acceleration.
<p>
Cf. #$PrimitiveMeasurableQuantityType.""" ;
	a <http://sw.cyc.com/2006/07/27/cyc/AtemporalNecessarilyEssentialCollectionType> , <http://sw.cyc.com/2006/07/27/cyc/SiblingDisjointCollectionType> , <http://sw.cyc.com/2006/07/27/cyc/FacetingCollectionType> , <http://sw.cyc.com/2006/07/27/cyc/SecondOrderCollection> , <http://sw.cyc.com/2006/07/27/cyc/Math-Topic> , <http://sw.cyc.com/2006/07/27/cyc/UnitsOfMeasure-Quantity-Topic> ;
	<http://sw.cyc.com/2006/07/27/cyc/prettyString-Canonical> "type of derived numeric scalar interval" ;
	<http://sw.cyc.com/2006/07/27/cyc/prettyString> "types of derived numeric scalar interval" ;
	<http://www.w3.org/2000/01/rdf-schema#subClassOf> <http://sw.cyc.com/2006/07/27/cyc/MeasurableQuantityType> ;
	<http://www.w3.org/2002/07/owl#disjointWith> <http://sw.cyc.com/2006/07/27/cyc/PrimitiveMeasurableQuantityType> ;
	<http://sw.cyc.com/2006/07/27/cyc/typeGenls> <http://sw.cyc.com/2006/07/27/cyc/MultiDimensionalQuantity> .

<http://sw.cyc.com/2006/07/27/cyc/accelerationDueToGravityOnPlanetaryBody> <http://www.w3.org/2000/01/rdf-schema#comment> "<code>(#$accelerationDueToGravityOnPlanetaryBody BODY RATE)</code> means that near the surace of the planetary body <code>BODY</code>, the force of gravity causes objects to accelerate at <code>RATE</code> towards the center of mass of <code>BODY</code>.  For example, (#$accelerationDueToGravityOnPlanetaryBody   #$PlanetEarth (#$MetersPerSecondPerSecond 9.80619)) is true." ;
	a <http://www.w3.org/2000/01/rdf-schema#Property> , <http://sw.cyc.com/2006/07/27/cyc/BinaryQuantityPredicate> , <http://sw.cyc.com/2006/07/27/cyc/FunctionalSlot> ;
	<http://sw.cyc.com/2006/07/27/cyc/prettyString-Canonical> "Acceleration Due To Gravity On Planetary Body" ;
	<http://www.w3.org/2000/01/rdf-schema#domain> <http://sw.cyc.com/2006/07/27/cyc/PlanetaryBody> ;
	<http://sw.cyc.com/2006/07/27/cyc/arity> "2"^^<http://www.w3.org/2001/XMLSchema#long> ;
	<http://www.w3.org/2000/01/rdf-schema#range> <http://sw.cyc.com/2006/07/27/cyc/Acceleration> .

<http://sw.cyc.com/2006/07/27/cyc/PlanetaryBody> <http://www.w3.org/2000/01/rdf-schema#comment> "A collection of heavenly bodies.  Each element of #$PlanetaryBody is an entity spacially distinct from other heavenly bodies that does not emit radiation due to internal fusion processes." ;
	a <http://sw.cyc.com/2006/07/27/cyc/ExistingObjectType> , <http://sw.cyc.com/2006/07/27/cyc/SpatiallyDisjointObjectType> , <http://sw.cyc.com/2006/07/27/cyc/KEClarifyingCollectionType> , <http://sw.cyc.com/2006/07/27/cyc/Geography-Topic> ;
	<http://sw.cyc.com/2006/07/27/cyc/prettyString-Canonical> "planetary body" ;
	<http://sw.cyc.com/2006/07/27/cyc/prettyString> "planetary bodies" ;
	<http://www.w3.org/2000/01/rdf-schema#subClassOf> <http://sw.cyc.com/2006/07/27/cyc/AstronomicalBody> .

<http://sw.cyc.com/2006/07/27/cyc/BinaryQuantityPredicate> <http://www.w3.org/2000/01/rdf-schema#comment> """A specialization of #$BinaryPredicate and #$IntangibleObjectPredicate whose instances relate things to quantities.  A binary predicate is an instance of #$BinaryQuantityPredicate if and only if its #$arg1Isa or its #$arg2Isa (or both) is a specialization of #$Quantity.  Examples include #$sizeParameterOfObject, #$followingValue, #$lifeExpectancy, and many others.  
<p>
Note that if a binary quantity predicate is such that (i) its #$arg2Format is #$intervalEntryFormatInArgs and (ii) its #$arg1Isa is <i>not</i> a specialization of #$Quantity, it is an instance of the more specialized collection #$QuantitySlot.""" ;
	a <http://sw.cyc.com/2006/07/27/cyc/AtemporalNecessarilyEssentialCollectionType> , <http://sw.cyc.com/2006/07/27/cyc/PredicateType> ;
	<http://sw.cyc.com/2006/07/27/cyc/prettyString-Canonical> "binary quantity predicate" .

<http://sw.cyc.com/2006/07/27/cyc/accelerationOfObject-Translation> <http://www.w3.org/2000/01/rdf-schema#domain> <http://sw.cyc.com/2006/07/27/cyc/SpatialThing> ;
	<http://sw.cyc.com/2006/07/27/cyc/arity> "2"^^<http://www.w3.org/2001/XMLSchema#long> ;
	<http://www.w3.org/2000/01/rdf-schema#range> <http://sw.cyc.com/2006/07/27/cyc/Acceleration> ;
	<http://sw.cyc.com/2006/07/27/cyc/arg2Format> <http://sw.cyc.com/2006/07/27/cyc/intervalEntryFormatInArgs> ;
	<http://sw.cyc.com/2006/07/27/cyc/functionalInArgs> "2"^^<http://www.w3.org/2001/XMLSchema#long> ;
	<http://sw.cyc.com/2006/07/27/cyc/intervalEntryFormatInArgs> "2"^^<http://www.w3.org/2001/XMLSchema#long> .

<http://sw.cyc.com/2006/07/27/cyc/intervalEntryFormatInArgs> <http://www.w3.org/2000/01/rdf-schema#comment> """An instance of #$SpecificEntryFormatPredicate (q.v.) that is used only with argument-places that are constrained to instances (see #$argIsa) of either #$ScalarInterval or #$TimeInterval or some specialization of either.  (#$intervalEntryFormatInArgs PRED N) means that, for any particular way of fixing the other arguments to PRED besides the Nth, for any two intervals such that if either one is taken as the Nth argument PRED holds of those arguments, those intervals must \"overlap\" (see #$quantityIntersects and #$temporallyIntersects).  That is, if the sequences <... ARGN ...> and <... ARGN-PRIME ...> differ at most in their Nth items and both (PRED ... ARGN ...) and (PRED ... ARGN-PRIME ...) hold, then (i) if (#$argIsa PRED N #$ScalarInterval) then (#$quantityIntersects ARGN ARGN-PRIME) holds and (ii) if (#$argIsa PRED N #$TimeInterval) then (#$temporallyIntersects ARGN ARGN-PRIME) holds.   

For example, #$intervalEntryFormatInArgs holds of #$bodyTemperature with respect to its second argument-place because, while a given creature (at a given moment in time) has a single exact (see #$ScalarPointValue) body temperature, we want the predicate #$bodyTemperature to be flexible enough to allow us to specify this temperature with varying degrees of precision (e.g. as \"98.6 degrees Fahrenheit\" or as \"between 98 and 99 degrees Fahrenheit\" or as \"less than 100 degrees Fahrenheit\").

For another example, #$intervalEntryFormatInArgs holds of #$foundingDate with respect to its second argument-place because, while a given city has a single exact (see #$startingPoint) time when it was founded, we want the predicate #$foundingDate to be flexible enough to allow us to specify this date with varying degrees of precision (e.g. as \"June 14, 1964,\" \"June 1964,\" or simply \"1964\").

Note that many interval-entry format argument-places that are constrained to time-intervals have #$Date as their asserted #$argIsa constraint.""" ;
	a <http://sw.cyc.com/2006/07/27/cyc/IntangibleObjectRelatingPredicate> , <http://sw.cyc.com/2006/07/27/cyc/MetaPredicate> , <http://sw.cyc.com/2006/07/27/cyc/SpecificEntryFormatPredicate> ;
	<http://sw.cyc.com/2006/07/27/cyc/prettyString-Canonical> "Interval Entry Format In Args" ;
	<http://sw.cyc.com/2006/07/27/cyc/quotedIsa> <http://sw.cyc.com/2006/07/27/cyc/OpenCycDefinitionalPredicate> ;
	<http://www.w3.org/2000/01/rdf-schema#domain> <http://sw.cyc.com/2006/07/27/cyc/FunctionalPredicate> ;
	<http://sw.cyc.com/2006/07/27/cyc/arity> "2"^^<http://www.w3.org/2001/XMLSchema#long> ;
	<http://www.w3.org/2000/01/rdf-schema#range> <http://sw.cyc.com/2006/07/27/cyc/PositiveInteger> ;
	<http://www.w3.org/2000/01/rdf-schema#subPropertyOf> <http://sw.cyc.com/2006/07/27/cyc/functionalInArgs> .

<http://sw.cyc.com/2006/07/27/cyc/MeasurableQuantitySlot> <http://www.w3.org/2000/01/rdf-schema#comment> """A specialization of #$QuantitySlot (q.v.).  Each instance of #$QuantitySlot is a binary predicate that is used to attribute a property to a thing, by relating it to a #$MeasurableQuantity (q.v.) of some sort, such as a #$Distance, a #$Speed, or a #$Time-Quantity.
<p>
Instances of #$MeasurableQuantitySlot include #$lengthOfObject and #$duration.
<p>
See also #$NonNumericQuantitySlot.""" ;
	a <http://sw.cyc.com/2006/07/27/cyc/AtemporalNecessarilyEssentialCollectionType> , <http://sw.cyc.com/2006/07/27/cyc/PredicateType> ;
	<http://sw.cyc.com/2006/07/27/cyc/prettyString-Canonical> "measure" ;
	<http://sw.cyc.com/2006/07/27/cyc/prettyString> "measures" ;
	<http://www.w3.org/2000/01/rdf-schema#subClassOf> <http://sw.cyc.com/2006/07/27/cyc/QuantitySlot> .

<http://sw.cyc.com/2006/07/27/cyc/accelerationOfObject-Vector> <http://www.w3.org/2000/01/rdf-schema#comment> "This predicate relates an object to the vector that expresses the magnitude and direction of its acceleration. <code>(#$accelerationOfObject-Direction OBJECT VECTOR)</code> means that the acceleration of <code>OBJECT</code> has the vector direction and magnitude of <code>VECTOR</code>. See also #$accelerationOfObject-Translation and #$accelerationOfObject-Direction." ;
	a <http://www.w3.org/2000/01/rdf-schema#Property> , <http://sw.cyc.com/2006/07/27/cyc/FunctionalSlot> , <http://sw.cyc.com/2006/07/27/cyc/TemporalExistencePredicate> ;
	<http://sw.cyc.com/2006/07/27/cyc/prettyString-Canonical> "Acceleration Of Object Vector" ;
	<http://www.w3.org/2000/01/rdf-schema#domain> <http://sw.cyc.com/2006/07/27/cyc/SpatialThing> ;
	<http://sw.cyc.com/2006/07/27/cyc/arity> "2"^^<http://www.w3.org/2001/XMLSchema#long> ;
	<http://www.w3.org/2000/01/rdf-schema#range> <http://sw.cyc.com/2006/07/27/cyc/LinearAccelerationVector> .

<http://sw.cyc.com/2006/07/27/cyc/LinearAccelerationVector> <http://www.w3.org/2000/01/rdf-schema#comment> "A #$VectorIntervalType and specialization of #$VectorInterval.  Each instance of #$LinearAccelerationVector is a #$Tuple consisting of an #$Acceleration and a #$Direction." ;
	a <http://sw.cyc.com/2006/07/27/cyc/AtemporalNecessarilyEssentialCollectionType> , <http://sw.cyc.com/2006/07/27/cyc/VectorIntervalType> , <http://sw.cyc.com/2006/07/27/cyc/TotallyOrderedCollection> ;
	<http://sw.cyc.com/2006/07/27/cyc/prettyString-Canonical> "acceleration vector" ;
	<http://sw.cyc.com/2006/07/27/cyc/prettyString> "acceleration vectors" ;
	<http://www.w3.org/2000/01/rdf-schema#subClassOf> <http://sw.cyc.com/2006/07/27/cyc/VectorInterval> .

<http://sw.cyc.com/2006/07/27/cyc/AccelInternationalCorporation> a <http://sw.cyc.com/2006/07/27/cyc/Individual> , <http://sw.cyc.com/2006/07/27/cyc/PubliclyHeldCorporation> ;
	<http://sw.cyc.com/2006/07/27/cyc/prettyString-Canonical> "Accel International Corporation" .

<http://sw.cyc.com/2006/07/27/cyc/Accelr8TechnologyCorporation> a <http://sw.cyc.com/2006/07/27/cyc/Individual> , <http://sw.cyc.com/2006/07/27/cyc/PubliclyHeldCorporation> ;
	<http://sw.cyc.com/2006/07/27/cyc/prettyString-Canonical> "Accelr 8 Technology Corporation" .

<http://sw.cyc.com/2006/07/27/cyc/AccentFurniture> a <http://sw.cyc.com/2006/07/27/cyc/ExistingObjectType> , <http://sw.cyc.com/2006/07/27/cyc/SpatiallyDisjointObjectType> , <http://sw.cyc.com/2006/07/27/cyc/ArtifactTypeByGenericCategory> ;
	<http://sw.cyc.com/2006/07/27/cyc/prettyString-Canonical> "accent furniture" ;
	<http://www.w3.org/2000/01/rdf-schema#subClassOf> <http://sw.cyc.com/2006/07/27/cyc/FurniturePiece> .

<http://sw.cyc.com/2006/07/27/cyc/FurniturePiece> <http://www.w3.org/2000/01/rdf-schema#comment> """A specialization of #$DurableGoods, #$HumanOccupationConstructObject, 
and #$SolidTangibleProduct.  Each instance of #$FurniturePiece is a 
durable artifact of a type that is typically used in human dwellings 
(see #$HumanShelterConstruction) to make them more comfortable.  Many
useful specializations of this collection can be classified according 
to the main function their instances serve.  Such functions include: 
(i) providing support for people's bodies while they are seated or 
reclining (e.g. #$Bed-PieceOfFurniture and #$FootStool), (ii) providing 
work or activity surfaces (e.g. #$Desk-PieceOfFurniture and 
#$DiningRoomTable), (iii) providing organized or protective storage 
for one's belongings (e.g. #$Dresser-PieceOfFurniture and 
#$Bookcase-PieceOfFurniture), and (iv) providing illumination (e.g. 
#$ElectricLamp).  Most pieces of furniture are #$NonPoweredDevices 
(q.v.) in that they don't need any energy input in order to serve their 
function; but of course there are plenty of exceptions to this, such 
as electric lamps, console TVs, and hospital beds.  Note that 
#$FurniturePiece only includes _whole_ pieces of furniture; e.g. a 
sofa is an instance, but an arm of a sofa is not.""" ;
	a <http://sw.cyc.com/2006/07/27/cyc/ExistingObjectType> , <http://sw.cyc.com/2006/07/27/cyc/SpatiallyDisjointObjectType> , <http://sw.cyc.com/2006/07/27/cyc/ArtifactTypeByGenericCategory> .

<http://sw.cyc.com/2006/07/27/cyc/acceptableTreatmentForMaleficiaryType> a <http://sw.cyc.com/2006/07/27/cyc/TernaryPredicate> , <http://sw.cyc.com/2006/07/27/cyc/FirstOrderCollectionPredicate> ;
	<http://sw.cyc.com/2006/07/27/cyc/prettyString-Canonical> "Acceptable Treatment For Maleficiary Type" ;
	<http://www.w3.org/2000/01/rdf-schema#domain> <http://sw.cyc.com/2006/07/27/cyc/FirstOrderCollection> ;
	<http://sw.cyc.com/2006/07/27/cyc/arg3Isa> <http://sw.cyc.com/2006/07/27/cyc/ExistingObjectType> ;
	<http://sw.cyc.com/2006/07/27/cyc/arity> "3"^^<http://www.w3.org/2001/XMLSchema#long> ;
	<http://www.w3.org/2000/01/rdf-schema#range> <http://sw.cyc.com/2006/07/27/cyc/PhysiologicalConditionType> ;
	<http://sw.cyc.com/2006/07/27/cyc/arg1Genl> <http://sw.cyc.com/2006/07/27/cyc/MedicalTreatmentEvent> ;
	<http://sw.cyc.com/2006/07/27/cyc/arg2Genl> <http://sw.cyc.com/2006/07/27/cyc/PhysiologicalCondition> ;
	<http://sw.cyc.com/2006/07/27/cyc/arg3Genl> <http://sw.cyc.com/2006/07/27/cyc/Organism-Whole> .

<http://sw.cyc.com/2006/07/27/cyc/PhysiologicalCondition> <http://www.w3.org/2000/01/rdf-schema#comment> """A specialization of #$SystemCondition.  Each instance of #$PhysiologicalCondition involves an #$Organism-Whole being in some physiological state that is not  typical for that organism's species, modulo considerations about the organism's sex or (in some cases) subspecies.  Thus #$Menstruating, though not typical among all persons, is part of being a healthy adult female, and so is not a specialization of #$PhysiologicalCondition (though it is a type of #$PhysiologicalProcess); #$Pregnancy, on the other hand, is a specialization of #$PhysiologicalCondition.  Note that some but not all
#$PhysiologicalConditions are events; but they are all #$Situations.
Thus each physiological condition has a temporal start and end, though in some cases (e.g. dwarfism) these will be the same as the start and end of the life of the organism.""" ;
	a <http://sw.cyc.com/2006/07/27/cyc/TemporalStuffType> , <http://sw.cyc.com/2006/07/27/cyc/QAClarifyingCollectionType> , <http://sw.cyc.com/2006/07/27/cyc/Ailments-Topic> , <http://sw.cyc.com/2006/07/27/cyc/GeneralMedicine-Topic> , <http://sw.cyc.com/2006/07/27/cyc/AnimalPhysiology-Physiology-Topic> ;
	<http://sw.cyc.com/2006/07/27/cyc/prettyString-Canonical> "physiological condition" ;
	<http://sw.cyc.com/2006/07/27/cyc/prettyString> "problem" , "problems" , "condition" , "conditions" , "physiological conditions" ;
	<http://www.w3.org/2000/01/rdf-schema#subClassOf> <http://sw.cyc.com/2006/07/27/cyc/AbnormalSystemCondition> , <http://sw.cyc.com/2006/07/27/cyc/PhysicalSituation> ;
	<http://sw.cyc.com/2006/07/27/cyc/quotedIsa> <http://sw.cyc.com/2006/07/27/cyc/ExtractedByNounLearnerFromMotleyFoolUKCorpus> ;
	<http://www.w3.org/2002/07/owl#disjointWith> <http://sw.cyc.com/2006/07/27/cyc/GridCondition> ;
	<http://sw.cyc.com/2006/07/27/cyc/requiredArg1Pred> <http://sw.cyc.com/2006/07/27/cyc/physiologicalConditionAffects> .

<http://sw.cyc.com/2006/07/27/cyc/PhysiologicalConditionType> <http://www.w3.org/2000/01/rdf-schema#comment> "A collection of collections.  Each instance of #$PhysiologicalConditionType is a specialization of  #$PhysiologicalCondition (q.v.), and thus a type of physiological state into which some organisms can enter.  Instances of #$PhysiologicalConditionType include  #$Cancer, #$PsychologicalAilment, #$Infection, and #$Malnutrition." ;
	a <http://sw.cyc.com/2006/07/27/cyc/AtemporalNecessarilyEssentialCollectionType> , <http://sw.cyc.com/2006/07/27/cyc/KEClarifyingCollectionType> , <http://sw.cyc.com/2006/07/27/cyc/FacetingCollectionType> , <http://sw.cyc.com/2006/07/27/cyc/SecondOrderCollection> , <http://sw.cyc.com/2006/07/27/cyc/AnimalPhysiology-Physiology-Topic> , <http://sw.cyc.com/2006/07/27/cyc/BBNEntityType> ;
	<http://sw.cyc.com/2006/07/27/cyc/prettyString-Canonical> "type of ailment" ;
	<http://sw.cyc.com/2006/07/27/cyc/prettyString> "health condition" , "health conditions" , "kind of ailment" , "kinds of ailment" , "type of health condition" , "types of health condition" , "types of ailment" ;
	<http://www.w3.org/2000/01/rdf-schema#subClassOf> <http://sw.cyc.com/2006/07/27/cyc/ObjectType> , <http://sw.cyc.com/2006/07/27/cyc/TemporalStuffType> , <http://sw.cyc.com/2006/07/27/cyc/KEClarifyingCollectionType> ;
	<http://sw.cyc.com/2006/07/27/cyc/typeGenls> <http://sw.cyc.com/2006/07/27/cyc/PhysiologicalCondition> .

<http://sw.cyc.com/2006/07/27/cyc/arg3Genl> <http://www.w3.org/2000/01/rdf-schema#comment> "A binary #$ArgGenlPredicate (q.v.).  <code>(#$arg3Genl RELN COL)</code>  means that semantic well-formedness requires that anything given as the third argument to <code>RELN</code> must be a subcollection of <code>COL</code>.  That is, <code>(RELN ARG1 ARG2 ARG3 ...)</code> is semantically well-formed only if <code>(#$genls ARG3 COL)</code> holds.  For an  explanation of semantic well-formedness, see #$CycLExpression-Assertible and its specializations.  See #$argGenl for a similar but more flexible ternary  predicate." ;
	a <http://sw.cyc.com/2006/07/27/cyc/DefaultMonotonicPredicate> , <http://sw.cyc.com/2006/07/27/cyc/IntangibleObjectRelatingPredicate> , <http://sw.cyc.com/2006/07/27/cyc/NonAbduciblePredicate> , <http://sw.cyc.com/2006/07/27/cyc/ArgumentGenl-Fundamental-Topic> , <http://sw.cyc.com/2006/07/27/cyc/ArgGenlBinaryPredicate> ;
	<http://sw.cyc.com/2006/07/27/cyc/prettyString-Canonical> "Arg 3 Genl" ;
	<http://sw.cyc.com/2006/07/27/cyc/quotedIsa> <http://sw.cyc.com/2006/07/27/cyc/OpenCycDefinitionalPredicate> ;
	<http://www.w3.org/2000/01/rdf-schema#domain> <http://sw.cyc.com/2006/07/27/cyc/Relation> ;
	<http://sw.cyc.com/2006/07/27/cyc/arity> "2"^^<http://www.w3.org/2001/XMLSchema#long> ;
	<http://sw.cyc.com/2006/07/27/cyc/sharedNotes> <http://sw.cyc.com/2006/07/27/cyc/ArgumentTypeChecking-FORTSvsNonReifiedNATS> ;
	<http://www.w3.org/2000/01/rdf-schema#range> <http://www.w3.org/2002/07/owl#Class> ;
	<http://www.w3.org/2000/01/rdf-schema#subPropertyOf> <http://sw.cyc.com/2006/07/27/cyc/relationExplicitlyInvokesTypeDerivatively-ArgGenl> ;
	<http://sw.cyc.com/2006/07/27/cyc/arg2Genl> <http://www.w3.org/2002/07/owl#Thing> ;
	<http://sw.cyc.com/2006/07/27/cyc/arg1Format> <http://sw.cyc.com/2006/07/27/cyc/SetTheFormat> ;
	<http://sw.cyc.com/2006/07/27/cyc/arg2Format> <http://sw.cyc.com/2006/07/27/cyc/SetTheFormat> ;
	<http://sw.cyc.com/2006/07/27/cyc/negationPreds> <http://sw.cyc.com/2006/07/27/cyc/arg3NotGenl> ;
	<http://sw.cyc.com/2006/07/27/cyc/oldConstantName> "argumentThreeGenls" ;
	<http://sw.cyc.com/2006/07/27/cyc/constrainsArg> "3"^^<http://www.w3.org/2001/XMLSchema#long> .

<http://sw.cyc.com/2006/07/27/cyc/Organism-Whole> <http://www.w3.org/2000/01/rdf-schema#comment> "A specialization of #$BiologicalLivingObject.  Each instance of #$Organism-Whole is a biological living object (BLO) that is a whole, and not part of some other BLO.  Most instances of #$Organism-Whole are capable of existing and reproducing while physically separate from other organisms (with allowances for eating and mating).  Abnormal BLOs which are nonetheless considered to be instances of #$Organism-Whole include instances of #$Virus, as well as sterile hybrids and colony organisms, like those in slime molds or the instances of #$PortugueseManOfWar." ;
	a <http://sw.cyc.com/2006/07/27/cyc/ExistingObjectType> , <http://sw.cyc.com/2006/07/27/cyc/SpatiallyDisjointObjectType> , <http://sw.cyc.com/2006/07/27/cyc/TestOWLExportConcept> , <http://sw.cyc.com/2006/07/27/cyc/OrganismParts-Biology-Topic> , <http://sw.cyc.com/2006/07/27/cyc/Biology-Topic> ;
	<http://sw.cyc.com/2006/07/27/cyc/prettyString-Canonical> "organism" ;
	<http://sw.cyc.com/2006/07/27/cyc/prettyString> "organisms" ;
	<http://www.w3.org/2000/01/rdf-schema#subClassOf> <http://sw.cyc.com/2006/07/27/cyc/BiologicalLivingObject> , <http://sw.cyc.com/2006/07/27/cyc/Alive> , <http://sw.cyc.com/2006/07/27/cyc/SpatiallyContinuousThing> ;
	<http://www.w3.org/2002/07/owl#disjointWith> <http://sw.cyc.com/2006/07/27/cyc/Neurotransmitter> , <http://sw.cyc.com/2006/07/27/cyc/OrganismPart> , <http://sw.cyc.com/2006/07/27/cyc/Covering-Object> , <http://sw.cyc.com/2006/07/27/cyc/Secretion-Bodily> , <http://sw.cyc.com/2006/07/27/cyc/PhysiologicalFeatureOfSurface> .

<http://sw.cyc.com/2006/07/27/cyc/AcceptingAnApology> <http://www.w3.org/2000/01/rdf-schema#subClassOf> <http://sw.cyc.com/2006/07/27/cyc/ApprovingARequest> .

<http://sw.cyc.com/2006/07/27/cyc/Forgiving> <http://www.w3.org/2000/01/rdf-schema#comment> "The collection of acts in which a human agent pardons some past perceived wrong on the part of another human agent." ;
	a <http://sw.cyc.com/2006/07/27/cyc/TemporalObjectType> ;
	<http://sw.cyc.com/2006/07/27/cyc/prettyString-Canonical> "forgiving" ;
	<http://sw.cyc.com/2006/07/27/cyc/prettyString> "forgiveness" , "forgivenesses" , "forgive" , "forgave" , "forgiven" , "forgives" , "have forgiven" , "has forgiven" , "will forgive" , "had forgiven" , "will have forgiven" ;
	<http://www.w3.org/2000/01/rdf-schema#subClassOf> <http://sw.cyc.com/2006/07/27/cyc/Action> , <http://sw.cyc.com/2006/07/27/cyc/SocialOccurrence> .

<http://sw.cyc.com/2006/07/27/cyc/ApprovingARequest> <http://www.w3.org/2000/01/rdf-schema#comment> "The collection of communication actions in which an agent approves a request." ;
	a <http://sw.cyc.com/2006/07/27/cyc/TemporalObjectType> , <http://sw.cyc.com/2006/07/27/cyc/TypicalHumanActivityType-AtLeastOnce> ;
	<http://sw.cyc.com/2006/07/27/cyc/prettyString-Canonical> "approving a request" ;
	<http://sw.cyc.com/2006/07/27/cyc/prettyString> "approve a request" , "approved a request" , "approves a request" , "have approved a request" , "has approved a request" , "will approve a request" , "had approved a request" , "will have approved a request" ;
	<http://www.w3.org/2000/01/rdf-schema#subClassOf> <http://sw.cyc.com/2006/07/27/cyc/Approval-CommunicationAct> .

<http://sw.cyc.com/2006/07/27/cyc/AcceptingAnInvitation> <http://www.w3.org/2000/01/rdf-schema#comment> "The collection of acknowledgements in which an invitation is accepted." ;
	a <http://sw.cyc.com/2006/07/27/cyc/TemporalObjectType> , <http://sw.cyc.com/2006/07/27/cyc/TypicalHumanActivityType-AtLeastOnce> ;
	<http://sw.cyc.com/2006/07/27/cyc/prettyString-Canonical> "accepting an invitation" ;
	<http://sw.cyc.com/2006/07/27/cyc/prettyString> "accept an invitation" , "accepted an invitation" , "accepts an invitation" , "have accepted an invitation" , "has accepted an invitation" , "will accept an invitation" , "had accepted an invitation" , "will have accepted an invitation" ;
	<http://www.w3.org/2000/01/rdf-schema#subClassOf> <http://sw.cyc.com/2006/07/27/cyc/ApprovingARequest> .

<http://sw.cyc.com/2006/07/27/cyc/TypicalHumanActivityType-AtLeastOnce> <http://www.w3.org/2000/01/rdf-schema#comment> "The collection of specializations of #$HumanActivity such that persons typically are involved in (#$actors) at least one instance of the activity type in their lifetime." ;
	a <http://www.w3.org/2002/07/owl#Class> , <http://sw.cyc.com/2006/07/27/cyc/CollectionType> ;
	<http://sw.cyc.com/2006/07/27/cyc/prettyString-Canonical> "typical human activity type at least once" ;
	<http://www.w3.org/2000/01/rdf-schema#subClassOf> <http://www.w3.org/2002/07/owl#Class> .

<http://sw.cyc.com/2006/07/27/cyc/AcceptingCommissive-CommunicationAct> <http://www.w3.org/2000/01/rdf-schema#comment> "A collection of speech acts each of which involves the acceptance of some promise, offer or other commissive act by some other agent. " ;
	a <http://sw.cyc.com/2006/07/27/cyc/TemporalObjectType> ;
	<http://sw.cyc.com/2006/07/27/cyc/prettyString-Canonical> "accepting commissive communication act" .

<http://sw.cyc.com/2006/07/27/cyc/AcceptingProgramUserCommunication> <http://www.w3.org/2002/07/owl#disjointWith> <http://sw.cyc.com/2006/07/27/cyc/PoweringADevice> .

<http://sw.cyc.com/2006/07/27/cyc/PoweringADevice> <http://www.w3.org/2000/01/rdf-schema#comment> "A collection of events; a subset of #$HandlingADevice.  An instance of #$PoweringADevice is an event in which a human or non-human animal #$Agent (or set of them) uses a device which is designed to transform some repetitive muscular motion into useful work, namely into providing the power for some device to function.  E.g., a #$Rowing event is such an event, and causes (provides the power for) the device (the rowboat) to move.  The same for #$PedalingABicycle .  The same for pulling a covered wagon (in which case a team of horses may be providing the power.)" ;
	a <http://sw.cyc.com/2006/07/27/cyc/TemporalStuffType> , <http://sw.cyc.com/2006/07/27/cyc/TypicalHumanActivityType-AtLeastOnce> , <http://sw.cyc.com/2006/07/27/cyc/Action-Device-Topic> ;
	<http://sw.cyc.com/2006/07/27/cyc/prettyString-Canonical> "powering" ;
	<http://sw.cyc.com/2006/07/27/cyc/prettyString> "Powers" , "power" , "powered" , "have powered" , "has powered" , "will power" , "had powered" , "will have powered" ;
	<http://www.w3.org/2000/01/rdf-schema#subClassOf> <http://sw.cyc.com/2006/07/27/cyc/HandlingADevice> ;
	<http://sw.cyc.com/2006/07/27/cyc/requiredActorSlots> <http://sw.cyc.com/2006/07/27/cyc/devicePowered> .

<http://sw.cyc.com/2006/07/27/cyc/AccessingAnIBT> <http://www.w3.org/2000/01/rdf-schema#comment> "A specialization of both #$InformationTransferEvent and #$PurposefulAction.  Each instance of #$AccessingAnIBT is an action by which an agent accesses the content of some instance(s) of #$InformationBearingThing.  Examples include (getting information from) reading a newspaper, watching a film, listening to a musical performance, decoding an encrypted message, seeing a traffic police officer wave one on, or hearing one's roommate ask one to take out the trash." ;
	a <http://sw.cyc.com/2006/07/27/cyc/TemporalStuffType> , <http://sw.cyc.com/2006/07/27/cyc/InformationAndCWs-Topic> ;
	<http://sw.cyc.com/2006/07/27/cyc/prettyString-Canonical> "information-accessing event" ;
	<http://sw.cyc.com/2006/07/27/cyc/prettyString> "accessed" , "accesses" , "accessing" , "have accessed" , "has accessed" , "will access" , "had accessed" , "will have accessed" , "information accessing event" , "information accessing events" , "information-accessing events" , "access" ;
	<http://www.w3.org/2000/01/rdf-schema#subClassOf> <http://sw.cyc.com/2006/07/27/cyc/TransferIn> , <http://sw.cyc.com/2006/07/27/cyc/InformationTransferEvent> , <http://sw.cyc.com/2006/07/27/cyc/Action> ;
	<http://www.w3.org/2002/07/owl#disjointWith> <http://sw.cyc.com/2006/07/27/cyc/PhysiologicalProcess> , <http://sw.cyc.com/2006/07/27/cyc/LocomotionEvent> , <http://sw.cyc.com/2006/07/27/cyc/AthleticActivity> , <http://sw.cyc.com/2006/07/27/cyc/MakingSomething> , <http://sw.cyc.com/2006/07/27/cyc/IntrinsicStateChangeEvent> , <http://sw.cyc.com/2006/07/27/cyc/ChangeInUserRights> , <http://sw.cyc.com/2006/07/27/cyc/Conveying-Generic> , <http://sw.cyc.com/2006/07/27/cyc/MedicalCareEvent> .

<http://sw.cyc.com/2006/07/27/cyc/ComputerUserInteraction> <http://www.w3.org/2000/01/rdf-schema#comment> "Communication between human user and computer." ;
	a <http://sw.cyc.com/2006/07/27/cyc/TemporalStuffType> ;
	<http://sw.cyc.com/2006/07/27/cyc/prettyString-Canonical> "computer user interaction" ;
	<http://sw.cyc.com/2006/07/27/cyc/prettyString> "computer user interactions" ;
	<http://www.w3.org/2000/01/rdf-schema#subClassOf> <http://sw.cyc.com/2006/07/27/cyc/ComputerActivity> ;
	<http://sw.cyc.com/2006/07/27/cyc/requiredActorSlots> <http://sw.cyc.com/2006/07/27/cyc/computerInteractionUser> .

<http://sw.cyc.com/2006/07/27/cyc/ComputerActivityType> <http://www.w3.org/2000/01/rdf-schema#comment> "An instance of #$SiblingDisjointCollectionType. Each instance of this (second-order) collection is a subcollection of #$ComputerActivity all of whose instances are a particular and distinct type of activity. Examples include #$EMailSending, #$BootingAComputer, #$ComputerCrashing and #$OnlineChat. #$AttackByComputerOperation is not an instance as it is not distinct enough. #$EnteringAComputerPassword is an instance, but #$EnteringADomainAdministratorPassword is not as it is too specific. This collection is an instance of #$SiblingDisjointCollectionType because it is assumed that computer-related activities are analysed fine-grainedly enough that if a putative instance of #$ComputerActivity would fall under two sibling #$ComputerActivityTypes, it should be analysed as two events." ;
	a <http://sw.cyc.com/2006/07/27/cyc/SiblingDisjointCollectionType> , <http://sw.cyc.com/2006/07/27/cyc/FacetingCollectionType> , <http://sw.cyc.com/2006/07/27/cyc/SecondOrderCollection> ;
	<http://sw.cyc.com/2006/07/27/cyc/prettyString-Canonical> "computer activity type" ;
	<http://sw.cyc.com/2006/07/27/cyc/prettyString> "computer activity types" ;
	<http://www.w3.org/2000/01/rdf-schema#subClassOf> <http://sw.cyc.com/2006/07/27/cyc/DurativeEventType> ;
	<http://www.w3.org/2002/07/owl#disjointWith> <http://sw.cyc.com/2006/07/27/cyc/SportsCategoryType> , <http://sw.cyc.com/2006/07/27/cyc/CultureClassificationType> , <http://sw.cyc.com/2006/07/27/cyc/CourseOfStudyType> , <http://sw.cyc.com/2006/07/27/cyc/DayOfMonthType> , <http://sw.cyc.com/2006/07/27/cyc/DayOfWeekType> , <http://sw.cyc.com/2006/07/27/cyc/ScientificTechnique> ;
	<http://sw.cyc.com/2006/07/27/cyc/typeGenls> <http://sw.cyc.com/2006/07/27/cyc/ComputerActivity> .

<http://sw.cyc.com/2006/07/27/cyc/Acknowledging-SoftwareAgentCom> <http://www.w3.org/2000/01/rdf-schema#comment> "This collection of communication acts includes only those instances of #$Acknowledging-CommunicationAct that are performed by software agents." ;
	a <http://sw.cyc.com/2006/07/27/cyc/TemporalObjectType> ;
	<http://sw.cyc.com/2006/07/27/cyc/prettyString-Canonical> "acknowledging software agent com" ;
	<http://www.w3.org/2000/01/rdf-schema#subClassOf> <http://sw.cyc.com/2006/07/27/cyc/Acknowledging-CommunicationAct> , <http://sw.cyc.com/2006/07/27/cyc/SoftwareAgentCommunicationAct-Single> .

<http://sw.cyc.com/2006/07/27/cyc/AcceptingTheUserCommunication> a <http://sw.cyc.com/2006/07/27/cyc/FirstOrderCollection> ;
	<http://sw.cyc.com/2006/07/27/cyc/prettyString-Canonical> "accepting the user communication" .

<http://sw.cyc.com/2006/07/27/cyc/accessFilenameOfAIS> <http://sw.cyc.com/2006/07/27/cyc/arg1Format> <http://sw.cyc.com/2006/07/27/cyc/SetTheFormat> ;
	<http://sw.cyc.com/2006/07/27/cyc/arg2Format> <http://sw.cyc.com/2006/07/27/cyc/SetTheFormat> .

<http://sw.cyc.com/2006/07/27/cyc/ComputerFile-AIS> <http://www.w3.org/2000/01/rdf-schema#comment> "A specialization of #$DataStream (q.v.).  Each instance of #$ComputerFile-AIS is an abstract series of bits encoding some information and conforming to some file system protocol.  The instantiation (see #$fileCopies) of this abstract series of bits (e.g. on magnetic media) is a #$ComputerFileCopy (q.v.)." ;
	a <http://sw.cyc.com/2006/07/27/cyc/ObjectType> ;
	<http://sw.cyc.com/2006/07/27/cyc/prettyString-Canonical> "computer file" ;
	<http://sw.cyc.com/2006/07/27/cyc/prettyString> "computer files" ;
	<http://www.w3.org/2000/01/rdf-schema#subClassOf> <http://sw.cyc.com/2006/07/27/cyc/DataStream> ;
	<http://sw.cyc.com/2006/07/27/cyc/facets-Strict> <http://sw.cyc.com/2006/07/27/cyc/ComputerFileTypeByFormat> .

<http://sw.cyc.com/2006/07/27/cyc/FileManagement-Topic> a <http://sw.cyc.com/2006/07/27/cyc/KBDependentCollection> , <http://sw.cyc.com/2006/07/27/cyc/CycVocabularyTopic> ;
	<http://sw.cyc.com/2006/07/27/cyc/prettyString-Canonical> "file management topic" ;
	<http://www.w3.org/2000/01/rdf-schema#subClassOf> <http://sw.cyc.com/2006/07/27/cyc/Computers-Topic> .

<http://sw.cyc.com/2006/07/27/cyc/accessibleDiscourseReferentInUDS> <http://www.w3.org/2000/01/rdf-schema#comment> """(#$accessibleDiscourseReferentInUDS UDS1 PEG) is true iff there
exists another discourse structure UDS2 such that PEG is an
#$availableCoreferentInUDS in UDS2 and
 (#$subordinateTo-DiscourseStructure UDS1 UDS2). In other words, the
discourse entities that are candidate coreference targets in a given 
unit discourse structure are accessible from any of its subordinate 
structures (except itself).""" ;
	a <http://sw.cyc.com/2006/07/27/cyc/IntangibleObjectRelatingPredicate> , <http://sw.cyc.com/2006/07/27/cyc/DiscourseStructureBinaryRole> ;
	<http://sw.cyc.com/2006/07/27/cyc/prettyString-Canonical> "Accessible Discourse Referent In UDS" ;
	<http://www.w3.org/2000/01/rdf-schema#domain> <http://sw.cyc.com/2006/07/27/cyc/UnitDiscourseStructure> ;
	<http://sw.cyc.com/2006/07/27/cyc/arity> "2"^^<http://www.w3.org/2001/XMLSchema#long> ;
	<http://www.w3.org/2000/01/rdf-schema#range> <http://sw.cyc.com/2006/07/27/cyc/LinguisticExpressionPeg> ;
	<http://www.w3.org/2000/01/rdf-schema#subPropertyOf> <http://sw.cyc.com/2006/07/27/cyc/availableCoreferentInUDS> ;
	<http://sw.cyc.com/2006/07/27/cyc/quotedArgument> "2"^^<http://www.w3.org/2001/XMLSchema#long> ;
	<http://sw.cyc.com/2006/07/27/cyc/openEntryFormatInArgs> "2"^^<http://www.w3.org/2001/XMLSchema#long> ;
	<http://sw.cyc.com/2006/07/27/cyc/arg2Format> <http://sw.cyc.com/2006/07/27/cyc/openEntryFormatInArgs> .

<http://sw.cyc.com/2006/07/27/cyc/UnitDiscourseStructure> <http://www.w3.org/2000/01/rdf-schema#comment> """An instance of this collection is a local discourse context, that
is, the smallest unit of context in a discourse. Each new utterance
introduces an additional #$UnitDiscourseStructure in a discourse; some
parts of utterances have their own UDSs. The main properties of a UDS are represented by the predicates in #$DiscourseStructureBinaryRole (q.v.). Any number of
reference-resolving conditions (cf #$coReferring) may also be asserted in a
UDS.""" ;
	a <http://sw.cyc.com/2006/07/27/cyc/KBDependentCollection> , <http://sw.cyc.com/2006/07/27/cyc/MicrotheoryType> , <http://sw.cyc.com/2006/07/27/cyc/FormalSemanticStructureType> ;
	<http://sw.cyc.com/2006/07/27/cyc/prettyString-Canonical> "unit discourse structure" ;
	<http://sw.cyc.com/2006/07/27/cyc/prettyString> "unit discourse structures" ;
	<http://www.w3.org/2000/01/rdf-schema#subClassOf> <http://sw.cyc.com/2006/07/27/cyc/Microtheory> , <http://sw.cyc.com/2006/07/27/cyc/AbstractStructure> .

<http://sw.cyc.com/2006/07/27/cyc/LinguisticExpressionPeg> <http://www.w3.org/2000/01/rdf-schema#comment> """A collection of \"pegs\" used to keep track of the linguistic
objects which are important for representing a discourse.""" ;
	a <http://www.w3.org/2002/07/owl#Class> , <http://sw.cyc.com/2006/07/27/cyc/NonAbducibleCollection> , <http://sw.cyc.com/2006/07/27/cyc/KBDependentCollection> , <http://sw.cyc.com/2006/07/27/cyc/LinguisticObjectType> , <http://sw.cyc.com/2006/07/27/cyc/FormalSemanticStructureType> ;
	<http://sw.cyc.com/2006/07/27/cyc/prettyString-Canonical> "discourse referent marker" ;
	<http://sw.cyc.com/2006/07/27/cyc/prettyString> "PEG" , "pegs" , "discourse referent markers" ;
	<http://www.w3.org/2000/01/rdf-schema#subClassOf> <http://sw.cyc.com/2006/07/27/cyc/LinguisticObject> , <http://sw.cyc.com/2006/07/27/cyc/ContextualizedInformationStructure> , <http://sw.cyc.com/2006/07/27/cyc/DiscourseTrackingPeg> ;
	<http://sw.cyc.com/2006/07/27/cyc/facets-Covering> <http://sw.cyc.com/2006/07/27/cyc/LinguisticExpressionType> ;
	<http://sw.cyc.com/2006/07/27/cyc/facets-Generic> <http://sw.cyc.com/2006/07/27/cyc/LinguisticExpressionType> , <http://sw.cyc.com/2006/07/27/cyc/ExpressionTypeByNumber> ;
	<http://sw.cyc.com/2006/07/27/cyc/requiredArg1Pred> <http://sw.cyc.com/2006/07/27/cyc/expressionPegCategory> .

<http://sw.cyc.com/2006/07/27/cyc/availableCoreferentInUDS> <http://www.w3.org/2000/01/rdf-schema#comment> "(#$availableCoreferentInUDS UDS PEG) is true if PEG is a discourse entity that is a candidate co-reference target for anaphors in UDS. In particular, this means that PEG is either new (in the sense of #$newDiscourseReferentInUDS) or accessible from another discourse structure (cf. #$accessibleDiscourseReferentInUDS) that is super-ordinate to, i.e., \"visible\" to, UDS." ;
	a <http://sw.cyc.com/2006/07/27/cyc/IntangibleObjectRelatingPredicate> , <http://sw.cyc.com/2006/07/27/cyc/DiscourseStructureBinaryRole> ;
	<http://sw.cyc.com/2006/07/27/cyc/prettyString-Canonical> "Available Coreferent In UDS" ;
	<http://www.w3.org/2000/01/rdf-schema#domain> <http://sw.cyc.com/2006/07/27/cyc/UnitDiscourseStructure> ;
	<http://sw.cyc.com/2006/07/27/cyc/arity> "2"^^<http://www.w3.org/2001/XMLSchema#long> ;
	<http://www.w3.org/2000/01/rdf-schema#range> <http://sw.cyc.com/2006/07/27/cyc/LinguisticExpressionPeg> .

<http://sw.cyc.com/2006/07/27/cyc/AccessingAComputerAccount> <http://sw.cyc.com/2006/07/27/cyc/prettyString> "will access a computer account" , "had accessed a computer account" , "will have accessed a computer account" ;
	<http://www.w3.org/2000/01/rdf-schema#subClassOf> <http://sw.cyc.com/2006/07/27/cyc/IntelligentAgentActivity> , <http://sw.cyc.com/2006/07/27/cyc/AccessingAnIBT> .

<http://sw.cyc.com/2006/07/27/cyc/EmployeeComputerActivityType> <http://www.w3.org/2000/01/rdf-schema#comment> "A specialization of #$ComputerActivityType. Each instance of this (second-order) collection is a subcollection of #$ComputerActivity all of whose instances are a particular and distinct type of computer-involving activity which is typically performed by employees as part of their work duties. Examples include #$EMailCommunication and #$PreparingPresentationSlides. Examples of #$ComputerActivityType which are not instances of #$EmployeeComputerActivityType include #$InterfacingBetweenComputerDeviceAndOS and #$HomecamBroadcasting. Activities such as #$ModifyingAFile, though often performed by employees, are assumed to be too fine-grained and not distinct enough to warrant inclusion in this collection." ;
	a <http://sw.cyc.com/2006/07/27/cyc/FacetingCollectionType> , <http://sw.cyc.com/2006/07/27/cyc/SecondOrderCollection> ;
	<http://sw.cyc.com/2006/07/27/cyc/prettyString-Canonical> "employee computer activity type" ;
	<http://sw.cyc.com/2006/07/27/cyc/prettyString> "employee computer activity types" ;
	<http://www.w3.org/2000/01/rdf-schema#subClassOf> <http://sw.cyc.com/2006/07/27/cyc/ComputerActivityType> ;
	<http://sw.cyc.com/2006/07/27/cyc/typeGenls> <http://sw.cyc.com/2006/07/27/cyc/ComputerActivity> .

<http://sw.cyc.com/2006/07/27/cyc/LearnedActivityType> <http://www.w3.org/2000/01/rdf-schema#comment> "This is the collection of activities which must first be learned before they can be performed--i.e., before any role which is a specPred of #$doneBy can be played." ;
	a <http://sw.cyc.com/2006/07/27/cyc/AtemporalNecessarilyEssentialCollectionType> , <http://sw.cyc.com/2006/07/27/cyc/FacetingCollectionType> , <http://sw.cyc.com/2006/07/27/cyc/SecondOrderCollection> ;
	<http://sw.cyc.com/2006/07/27/cyc/prettyString-Canonical> "learned activity" ;
	<http://sw.cyc.com/2006/07/27/cyc/prettyString> "learned activities" ;
	<http://www.w3.org/2000/01/rdf-schema#subClassOf> <http://sw.cyc.com/2006/07/27/cyc/KEClarifyingCollectionType> , <http://sw.cyc.com/2006/07/27/cyc/DurativeEventType> ;
	<http://sw.cyc.com/2006/07/27/cyc/typeGenls> <http://sw.cyc.com/2006/07/27/cyc/IntelligentAgentActivity> , <http://sw.cyc.com/2006/07/27/cyc/AtLeastPartiallyMentalEvent> .

<http://sw.cyc.com/2006/07/27/cyc/AccessingACWFn> <http://www.w3.org/2000/01/rdf-schema#comment> "This function, given a #$ConceptualWork, returns the collection of #$AccessingAnIBT events involving #$InformationBearingThings that are instantiations of this type.  For instance, (#$AccessingAnIBTTypeFn #$PeloponnesianWarHistoryByThucydides) would return all the events of reading (portions of instances of) a copy (#$instantiationOfWork) of Thucydides' history of the Peloponnesian Wars.  If I ask, 'Have you ever seen the movie 2001?', I am asking if you have played the role of #$recipientOfInfo in an instance of (#$AccessingACWFn #$2001-ASpaceOdyssey-TheMovie)." ;
	a <http://sw.cyc.com/2006/07/27/cyc/CollectionDenotingFunction> , <http://sw.cyc.com/2006/07/27/cyc/UnaryFunction> , <http://sw.cyc.com/2006/07/27/cyc/ReifiableFunction> ;
	<http://sw.cyc.com/2006/07/27/cyc/prettyString-Canonical> "accessing acw fn" ;
	<http://www.w3.org/2000/01/rdf-schema#domain> <http://sw.cyc.com/2006/07/27/cyc/ConceptualWork> ;
	<http://sw.cyc.com/2006/07/27/cyc/arity> "1"^^<http://www.w3.org/2001/XMLSchema#long> ;
	<http://sw.cyc.com/2006/07/27/cyc/resultGenl> <http://sw.cyc.com/2006/07/27/cyc/AccessingAnIBT> ;
	<http://sw.cyc.com/2006/07/27/cyc/resultIsa> <http://sw.cyc.com/2006/07/27/cyc/FirstOrderCollection> .

<http://sw.cyc.com/2006/07/27/cyc/ConceptualWork> <http://www.w3.org/2000/01/rdf-schema#comment> "A specialization of #$DevisedPracticeOrWork (q.v.).   Each instance of #$ConceptualWork is a partially abstract work (in the sense that each instance has a beginning in time, but lacks a location in space) which either has an associated #$AbstractInformationStructure (q.v.) or has a version with an associated #$AbstractInformationStructure.  Conceptual works or versions of conceptual works can be instantiated in instances of #$InformationBearingThing (q.v.); every such instantiation of a conceptual work will also be an instantiation of an instance of #$AbstractInformationStructure.  Notable specializations of #$ConceptualWork include #$ComputerProgram-CW, #$VisualWork, and #$Book-CW." ;
	a <http://sw.cyc.com/2006/07/27/cyc/FirstOrderCollection> ;
	<http://sw.cyc.com/2006/07/27/cyc/prettyString-Canonical> "conceptual work" ;
	<http://sw.cyc.com/2006/07/27/cyc/prettyString> "piece" , "pieces" , "conceptual works" , "work" , "works" ;
	<http://www.w3.org/2000/01/rdf-schema#subClassOf> <http://sw.cyc.com/2006/07/27/cyc/DevisedPracticeOrWork> ;
	<http://sw.cyc.com/2006/07/27/cyc/facets-Generic> <http://sw.cyc.com/2006/07/27/cyc/ConceptualWorkTypeByGenre> , <http://sw.cyc.com/2006/07/27/cyc/ConceptualWorkTypeByCreator> .

<http://sw.cyc.com/2006/07/27/cyc/AccessingAFile> <http://www.w3.org/2000/01/rdf-schema#comment> "The collection of actions done by computers in which a computer reads information from a file." ;
	a <http://sw.cyc.com/2006/07/27/cyc/ComputerActivityType> ;
	<http://sw.cyc.com/2006/07/27/cyc/prettyString-Canonical> "accessing a file" ;
	<http://www.w3.org/2000/01/rdf-schema#subClassOf> <http://sw.cyc.com/2006/07/27/cyc/AccessingAnIBT> , <http://sw.cyc.com/2006/07/27/cyc/FileOperation> , <http://sw.cyc.com/2006/07/27/cyc/InformationTransferPhysicalEvent> ;
	<http://sw.cyc.com/2006/07/27/cyc/sharedNotes> <http://sw.cyc.com/2006/07/27/cyc/NoteOnProgramActions> .

<http://sw.cyc.com/2006/07/27/cyc/AccessingData-DVD> <http://www.w3.org/2000/01/rdf-schema#subClassOf> <http://sw.cyc.com/2006/07/27/cyc/CWInstantiating> , <http://sw.cyc.com/2006/07/27/cyc/ComputerActivity> , <http://sw.cyc.com/2006/07/27/cyc/DataSending> .

<http://sw.cyc.com/2006/07/27/cyc/AccessingData-MP3> <http://www.w3.org/2000/01/rdf-schema#comment> "A specialization of #$DataSending. Each instance of this collection is an #$Event in which data is accessed from a #$MP3FileCopy and sent to some output device." ;
	a <http://sw.cyc.com/2006/07/27/cyc/TemporalObjectType> , <http://sw.cyc.com/2006/07/27/cyc/EmployeeComputerActivityType> ;
	<http://sw.cyc.com/2006/07/27/cyc/prettyString-Canonical> "accessing data on MP3" ;
	<http://www.w3.org/2000/01/rdf-schema#subClassOf> <http://sw.cyc.com/2006/07/27/cyc/AccessingAnIBT> , <http://sw.cyc.com/2006/07/27/cyc/CWInstantiating> , <http://sw.cyc.com/2006/07/27/cyc/ComputerActivity> , <http://sw.cyc.com/2006/07/27/cyc/DataSending> .

<http://sw.cyc.com/2006/07/27/cyc/AccessingPersonalInformation> <http://www.w3.org/2000/01/rdf-schema#comment> "The collection of all events in which a person accesses personal information, such as an address book, calendar, memos, or etc." ;
	a <http://sw.cyc.com/2006/07/27/cyc/TemporalObjectType> ;
	<http://sw.cyc.com/2006/07/27/cyc/prettyString-Canonical> "accessing personal information" ;
	<http://www.w3.org/2000/01/rdf-schema#subClassOf> <http://sw.cyc.com/2006/07/27/cyc/AccessingAnIBT> .

<http://sw.cyc.com/2006/07/27/cyc/AccessingReferenceResources> <http://www.w3.org/2000/01/rdf-schema#comment> "The collection of all events in which a person accesses reference resources, such as a dictionary, thesaurus, atlas, encyclopedia, or etc." ;
	a <http://sw.cyc.com/2006/07/27/cyc/TemporalObjectType> ;
	<http://sw.cyc.com/2006/07/27/cyc/prettyString-Canonical> "accessing reference resources" ;
	<http://www.w3.org/2000/01/rdf-schema#subClassOf> <http://sw.cyc.com/2006/07/27/cyc/AccessingAnIBT> .

<http://sw.cyc.com/2006/07/27/cyc/AccessingScriptType> <http://www.w3.org/2000/01/rdf-schema#comment> "A collection of collections.  Each instance of #$AccessingScriptType is a type (i.e., a collection) of actions by which an agent may come to possess, or gain user rights to, some tangible thing.  Instances of #$AccessingScriptType include the collections #$Buying, #$Renting, and #$BorrowingSomething." ;
	a <http://sw.cyc.com/2006/07/27/cyc/SiblingDisjointCollectionType> , <http://sw.cyc.com/2006/07/27/cyc/FacetingCollectionType> , <http://sw.cyc.com/2006/07/27/cyc/SecondOrderCollection> , <http://sw.cyc.com/2006/07/27/cyc/TakingSomethingAway-PossTransfer-Topic> ;
	<http://sw.cyc.com/2006/07/27/cyc/prettyString-Canonical> "type of action that involves accessing something" ;
	<http://sw.cyc.com/2006/07/27/cyc/prettyString> "types of action that involves accessing something" ;
	<http://www.w3.org/2000/01/rdf-schema#subClassOf> <http://sw.cyc.com/2006/07/27/cyc/FirstOrderCollection> ;
	<http://www.w3.org/2002/07/owl#disjointWith> <http://sw.cyc.com/2006/07/27/cyc/MicrotheoryType> ;
	<http://sw.cyc.com/2006/07/27/cyc/typeGenls> <http://sw.cyc.com/2006/07/27/cyc/GeneralizedTransfer> .

<http://sw.cyc.com/2006/07/27/cyc/TakingSomethingAway-PossTransfer-Topic> a <http://sw.cyc.com/2006/07/27/cyc/KBDependentCollection> , <http://sw.cyc.com/2006/07/27/cyc/CycVocabularyTopic> ;
	<http://sw.cyc.com/2006/07/27/cyc/prettyString-Canonical> "taking something away poss transfer topic" ;
	<http://www.w3.org/2000/01/rdf-schema#subClassOf> <http://sw.cyc.com/2006/07/27/cyc/PossTransfer-Topic> .

<http://sw.cyc.com/2006/07/27/cyc/GeneralizedTransfer> <http://www.w3.org/2000/01/rdf-schema#comment> "A specialization of #$Event.  Each instance of #$GeneralizedTransfer is an event in which something (tangible or intangible) is transferred from one 'place' to another.  #$GeneralizedTransfer includes changes in physical location, in ownership or possession, transfer of information, and propagation of wave phenomena through space.  See also the related predicate #$transferredThing, and the specializations of this collection." ;
	a <http://sw.cyc.com/2006/07/27/cyc/QAClarifyingCollectionType> , <http://sw.cyc.com/2006/07/27/cyc/ProcessType> , <http://sw.cyc.com/2006/07/27/cyc/EventOrRoleConcept> , <http://sw.cyc.com/2006/07/27/cyc/Top-Topic> , <http://sw.cyc.com/2006/07/27/cyc/CDETagTranslationConstant> , <http://sw.cyc.com/2006/07/27/cyc/SaffronSituationTypeConstant> , <http://sw.cyc.com/2006/07/27/cyc/CumulativeEventType> ;
	<http://sw.cyc.com/2006/07/27/cyc/prettyString-Canonical> "transfer" ;
	<http://sw.cyc.com/2006/07/27/cyc/prettyString> "moving" , "move" , "moved" , "moves" , "have moved" , "has moved" , "will move" , "had moved" , "will have moved" , "transited" , "transiting" , "have transited" , "has transited" , "will transit" , "had transited" , "will have transited" , "transferred" , "transfers" , "transferring" .

<http://sw.cyc.com/2006/07/27/cyc/AccessorFn> <http://sw.cyc.com/2006/07/27/cyc/prettyString-Canonical> "Accessor Fn" ;
	<http://www.w3.org/2000/01/rdf-schema#domain> <http://sw.cyc.com/2006/07/27/cyc/Individual> ;
	<http://sw.cyc.com/2006/07/27/cyc/arity> "1"^^<http://www.w3.org/2001/XMLSchema#long> .

<http://sw.cyc.com/2006/07/27/cyc/AccessoryFn-Activity> <http://www.w3.org/2000/01/rdf-schema#comment> """The expression `(#$AccessoryFn-Activity ACTIVITY)' denotes the collection of
accessories for the #$ScriptType ACTIVITY.""" ;
	a <http://sw.cyc.com/2006/07/27/cyc/CollectionDenotingFunction> , <http://sw.cyc.com/2006/07/27/cyc/UnaryFunction> , <http://sw.cyc.com/2006/07/27/cyc/ReifiableFunction> ;
	<http://sw.cyc.com/2006/07/27/cyc/prettyString-Canonical> "Accessory Fn Activity" ;
	<http://www.w3.org/2000/01/rdf-schema#domain> <http://www.w3.org/2002/07/owl#Class> ;
	<http://sw.cyc.com/2006/07/27/cyc/arity> "1"^^<http://www.w3.org/2001/XMLSchema#long> ;
	<http://sw.cyc.com/2006/07/27/cyc/resultIsa> <http://sw.cyc.com/2006/07/27/cyc/ArtifactTypeByGenericCategory> , <http://sw.cyc.com/2006/07/27/cyc/FirstOrderCollection> ;
	<http://sw.cyc.com/2006/07/27/cyc/arg1Genl> <http://sw.cyc.com/2006/07/27/cyc/Event> .

<http://sw.cyc.com/2006/07/27/cyc/AccessoryFn-Artifact> <http://www.w3.org/2000/01/rdf-schema#comment> "The expression `(#$AccessoryFn-Artifact PRODTYPE)' denotes the collection of accessories for the product type PRODTYPE. To clarify, the resulting collection is such that every member of it is an accessory for some spec of PRODTYPE. For example, the collection of computer printers would be in the collection (#$AccessoryFn-Artifact #$PersonalComputer) because every computer printer is an accessory for some type of personal computer. However, no computer printer is an accessory for every personal computer." ;
	a <http://sw.cyc.com/2006/07/27/cyc/CollectionDenotingFunction> , <http://sw.cyc.com/2006/07/27/cyc/UnaryFunction> , <http://sw.cyc.com/2006/07/27/cyc/ReifiableFunction> ;
	<http://sw.cyc.com/2006/07/27/cyc/prettyString-Canonical> "Accessory Fn Artifact" ;
	<http://www.w3.org/2000/01/rdf-schema#domain> <http://sw.cyc.com/2006/07/27/cyc/ExistingObjectType> ;
	<http://sw.cyc.com/2006/07/27/cyc/arity> "1"^^<http://www.w3.org/2001/XMLSchema#long> ;
	<http://sw.cyc.com/2006/07/27/cyc/resultGenl> <http://sw.cyc.com/2006/07/27/cyc/PartiallyTangible> , <http://sw.cyc.com/2006/07/27/cyc/Artifact> , <http://sw.cyc.com/2006/07/27/cyc/Artifact-NonAgentive> ;
	<http://sw.cyc.com/2006/07/27/cyc/resultIsa> <http://sw.cyc.com/2006/07/27/cyc/ExistingObjectType> ;
	<http://sw.cyc.com/2006/07/27/cyc/arg1Genl> <http://sw.cyc.com/2006/07/27/cyc/PartiallyTangible> , <http://sw.cyc.com/2006/07/27/cyc/Artifact> .

<http://sw.cyc.com/2006/07/27/cyc/Artifact-NonAgentive> <http://www.w3.org/2000/01/rdf-schema#comment> "An instance of #$ObjectType, and a specialization of #$Artifact-Generic.  #$Artifact-NonAgentive is the collection of all artifacts that are _not_ agents (i.e., that are _not_ instances of #$Agent-Generic).  Specializations of #$Artifact-NonAgentive include #$Bicycle, #$Pants, #$Canal, and #$FoodUtensil." ;
	a <http://sw.cyc.com/2006/07/27/cyc/ObjectType> ;
	<http://sw.cyc.com/2006/07/27/cyc/prettyString-Canonical> "non-agentive artifact" ;
	<http://sw.cyc.com/2006/07/27/cyc/prettyString> "non-agentive artifacts" ;
	<http://www.w3.org/2000/01/rdf-schema#subClassOf> <http://sw.cyc.com/2006/07/27/cyc/Artifact-Generic> ;
	<http://www.w3.org/2002/07/owl#disjointWith> <http://sw.cyc.com/2006/07/27/cyc/Agent-Generic> .

<http://sw.cyc.com/2006/07/27/cyc/accessoryFor-Activity> <http://www.w3.org/2000/01/rdf-schema#comment> """This predicate is analogous to
#$accessoryFor, except that it relates products to activities for
which they are considered accessories rather than to other products.
Note that the intended interpretation is weak (compare to #$accessoryFor-Strict).
Saying that (#$accessoryFor-Activity PRODTYPE ACTTYPE) means that for
every spec of PRODTYPE there is some spec of ACTTYPE such that all instances
of the former may be used in performing any instance of the latter.""" ;
	a <http://www.w3.org/2002/07/owl#TransitiveProperty> , <http://sw.cyc.com/2006/07/27/cyc/AsymmetricBinaryPredicate> , <http://sw.cyc.com/2006/07/27/cyc/FirstOrderCollectionPredicate> ;
	<http://sw.cyc.com/2006/07/27/cyc/prettyString-Canonical> "accessory for activity" ;
	<http://www.w3.org/2000/01/rdf-schema#domain> <http://sw.cyc.com/2006/07/27/cyc/ExistingObjectType> ;
	<http://sw.cyc.com/2006/07/27/cyc/arity> "2"^^<http://www.w3.org/2001/XMLSchema#long> ;
	<http://www.w3.org/2000/01/rdf-schema#range> <http://www.w3.org/2002/07/owl#Class> ;
	<http://sw.cyc.com/2006/07/27/cyc/arg1Genl> <http://sw.cyc.com/2006/07/27/cyc/PartiallyTangible> ;
	<http://sw.cyc.com/2006/07/27/cyc/arg2Genl> <http://sw.cyc.com/2006/07/27/cyc/Event> ;
	<http://sw.cyc.com/2006/07/27/cyc/negationInverse> <http://sw.cyc.com/2006/07/27/cyc/accessoryFor-Activity> .

<http://sw.cyc.com/2006/07/27/cyc/accessoryFor> <http://www.w3.org/2000/01/rdf-schema#comment> "(#$accessoryFor ACCESSORY_TYPE DEVICE_TYPE) means that instances of ACCESSORY_TYPE are designed to be used either as parts of instances of DEVICE_TYPE or as devices to be used with or to help care for instances of DEVICE_TYPE." ;
	a <http://www.w3.org/2002/07/owl#TransitiveProperty> , <http://sw.cyc.com/2006/07/27/cyc/AsymmetricBinaryPredicate> , <http://sw.cyc.com/2006/07/27/cyc/FirstOrderCollectionPredicate> ;
	<http://sw.cyc.com/2006/07/27/cyc/prettyString-Canonical> "Accessory For" ;
	<http://www.w3.org/2000/01/rdf-schema#domain> <http://sw.cyc.com/2006/07/27/cyc/ExistingObjectType> ;
	<http://sw.cyc.com/2006/07/27/cyc/arity> "2"^^<http://www.w3.org/2001/XMLSchema#long> ;
	<http://www.w3.org/2000/01/rdf-schema#range> <http://sw.cyc.com/2006/07/27/cyc/ExistingObjectType> ;
	<http://sw.cyc.com/2006/07/27/cyc/arg1Genl> <http://sw.cyc.com/2006/07/27/cyc/PartiallyTangible> ;
	<http://sw.cyc.com/2006/07/27/cyc/arg2Genl> <http://sw.cyc.com/2006/07/27/cyc/PartiallyTangible> ;
	<http://sw.cyc.com/2006/07/27/cyc/arg2Format> <http://sw.cyc.com/2006/07/27/cyc/SetTheFormat> ;
	<http://sw.cyc.com/2006/07/27/cyc/negationInverse> <http://sw.cyc.com/2006/07/27/cyc/accessoryFor> .

<http://sw.cyc.com/2006/07/27/cyc/accessoryFor-Strict> a <http://sw.cyc.com/2006/07/27/cyc/IrreflexiveBinaryPredicate> , <http://sw.cyc.com/2006/07/27/cyc/FirstOrderCollectionPredicate> ;
	<http://sw.cyc.com/2006/07/27/cyc/prettyString-Canonical> "accessory for strict" ;
	<http://www.w3.org/2000/01/rdf-schema#domain> <http://sw.cyc.com/2006/07/27/cyc/ExistingObjectType> ;
	<http://sw.cyc.com/2006/07/27/cyc/arity> "2"^^<http://www.w3.org/2001/XMLSchema#long> ;
	<http://www.w3.org/2000/01/rdf-schema#range> <http://sw.cyc.com/2006/07/27/cyc/ExistingObjectType> ;
	<http://www.w3.org/2000/01/rdf-schema#subPropertyOf> <http://sw.cyc.com/2006/07/27/cyc/accessoryFor> ;
	<http://sw.cyc.com/2006/07/27/cyc/arg1Genl> <http://sw.cyc.com/2006/07/27/cyc/PartiallyTangible> ;
	<http://sw.cyc.com/2006/07/27/cyc/arg2Genl> <http://sw.cyc.com/2006/07/27/cyc/PartiallyTangible> .

<http://sw.cyc.com/2006/07/27/cyc/AccessoryHemiAzygosVein> a <http://sw.cyc.com/2006/07/27/cyc/AnimalBodyPartType> , <http://sw.cyc.com/2006/07/27/cyc/UniqueAnatomicalPartType> , <http://sw.cyc.com/2006/07/27/cyc/InternalAnimalBodyRegionType> ;
	<http://sw.cyc.com/2006/07/27/cyc/prettyString-Canonical> "accessory hemiazygous vein" ;
	<http://sw.cyc.com/2006/07/27/cyc/prettyString> "accessory hemiazygous veins" , "accessory hemiazygos vein" , "accessory hemiazygos veins" ;
	<http://www.w3.org/2000/01/rdf-schema#subClassOf> <http://sw.cyc.com/2006/07/27/cyc/SystemicVein> .

<http://sw.cyc.com/2006/07/27/cyc/SystemicVein> <http://www.w3.org/2000/01/rdf-schema#comment> "The collection of all #$Veins which drain #$DeoxygenatedBlood towards the #$Heart (the right #$VentricleOfHeart).  This includes all #$Veins except pulmonary veins (#$PulmonaryVein-Generic) which carry #$OxygenatedBlood and those in the #$HepaticPortalVein system which drain towards the #$Liver." ;
	a <http://sw.cyc.com/2006/07/27/cyc/AnimalBodyPartType> , <http://sw.cyc.com/2006/07/27/cyc/InternalAnimalBodyRegionType> ;
	<http://sw.cyc.com/2006/07/27/cyc/prettyString-Canonical> "systemic vein" ;
	<http://sw.cyc.com/2006/07/27/cyc/prettyString> "systemic veins" ;
	<http://www.w3.org/2000/01/rdf-schema#subClassOf> <http://sw.cyc.com/2006/07/27/cyc/Vein> .

<http://sw.cyc.com/2006/07/27/cyc/AccessoryNerve> <http://www.w3.org/2000/01/rdf-schema#comment> "The collection of all accessory #$Nerves.  The #$AccessoryNerve is the eleventh #$CranialNerve.  The #$AccessoryNerve #$innervates the #$Larynx, #$Pharynx and the large neck #$Muscles (#$Trapezius and #$SternoCleidoMastoid)." ;
	a <http://sw.cyc.com/2006/07/27/cyc/InternalAnimalBodyRegionType> , <http://sw.cyc.com/2006/07/27/cyc/SymmetricAnatomicalPartType> ;
	<http://sw.cyc.com/2006/07/27/cyc/prettyString-Canonical> "accessory nerve" ;
	<http://sw.cyc.com/2006/07/27/cyc/prettyString> "accessory nerves" , "spinal accessory" , "spinal accessories" , "spinal accessory nerve" , "spinal accessory nerves" , "eleventh cranial nerve" , "eleventh cranial nerves" ;
	<http://www.w3.org/2000/01/rdf-schema#subClassOf> <http://sw.cyc.com/2006/07/27/cyc/CranialNerve> , <http://sw.cyc.com/2006/07/27/cyc/MotorNerve> ;
	<http://sw.cyc.com/2006/07/27/cyc/sharedNotes> <http://sw.cyc.com/2006/07/27/cyc/BeforeMajorChangesToAnatomicalParts> .

<http://sw.cyc.com/2006/07/27/cyc/AccessPageFn-IBT> <http://www.w3.org/2000/01/rdf-schema#comment> "#$AccessPageFn-IBT takes as argument any instance or specialization of #$ElectroMagneticInformationBearingThing and returns the collection of all #$WorldWideWebPage-AIS via which one may access this IBT or type of IBT.  For example, (#$AccessPageFn-IBT Yahoo) would return the collection of all web pages via which the Yahoo search engine can be accessed.(#$Kean 10/8/99)" ;
	a <http://sw.cyc.com/2006/07/27/cyc/CollectionDenotingFunction> , <http://sw.cyc.com/2006/07/27/cyc/SubTopicFunction> ;
	<http://sw.cyc.com/2006/07/27/cyc/prettyString-Canonical> "Access Page Fn IBT" ;
	<http://www.w3.org/2000/01/rdf-schema#domain> <http://sw.cyc.com/2006/07/27/cyc/InformationStore> ;
	<http://sw.cyc.com/2006/07/27/cyc/arity> "1"^^<http://www.w3.org/2001/XMLSchema#long> ;
	<http://sw.cyc.com/2006/07/27/cyc/resultGenl> <http://sw.cyc.com/2006/07/27/cyc/WorldWideWebPage-AIS> ;
	<http://sw.cyc.com/2006/07/27/cyc/resultIsa> <http://sw.cyc.com/2006/07/27/cyc/IBTContentType> .

<http://sw.cyc.com/2006/07/27/cyc/InformationStore> <http://www.w3.org/2000/01/rdf-schema#comment> "A specialization of #$PartiallyIntangibleIndividual.  Each instance of #$InformationStore is a tangible or intangible, concrete or abstract repository of information.  The information stored in an information store is stored there as a consequence of the actions of one or more agents.  Wholly intangible instances of #$InformationStore include instances of #$AspatialInformationStore and #$PropositionalInformationThing.  Some instances of #$InformationStore -- namely, instances of #$InformationBearingObject, such as copies of a newspaper at a newsstand -- are only partially intangible." ;
	a <http://sw.cyc.com/2006/07/27/cyc/TemporalStuffType> ;
	<http://sw.cyc.com/2006/07/27/cyc/prettyString-Canonical> "store of information" ;
	<http://sw.cyc.com/2006/07/27/cyc/prettyString> "stores of information" ;
	<http://www.w3.org/2000/01/rdf-schema#subClassOf> <http://sw.cyc.com/2006/07/27/cyc/Expression-Underspecified> , <http://sw.cyc.com/2006/07/27/cyc/PartiallyIntangibleIndividual> .

<http://sw.cyc.com/2006/07/27/cyc/SubTopicFunction> <http://www.w3.org/2000/01/rdf-schema#comment> "A collection of functions.  Instances of #$SubTopicFunction are functions which take as argument some topic and return a collection which is a subtopic of the argument given. Examples of instances of #$SubTopicFunction include #$DesignForObjectTypeFn and #$CareAndFeedingFn." ;
	a <http://sw.cyc.com/2006/07/27/cyc/NonAbducibleCollection> , <http://sw.cyc.com/2006/07/27/cyc/AtemporalNecessarilyEssentialCollectionType> , <http://sw.cyc.com/2006/07/27/cyc/FunctionType> ;
	<http://sw.cyc.com/2006/07/27/cyc/prettyString-Canonical> "sub topic function" ;
	<http://www.w3.org/2000/01/rdf-schema#subClassOf> <http://sw.cyc.com/2006/07/27/cyc/CollectionDenotingFunction> , <http://sw.cyc.com/2006/07/27/cyc/UnaryFunction> , <http://sw.cyc.com/2006/07/27/cyc/ReifiableFunction> ;
	<http://sw.cyc.com/2006/07/27/cyc/quotedIsa> <http://sw.cyc.com/2006/07/27/cyc/QueryAugmentationConstant> .

<http://sw.cyc.com/2006/07/27/cyc/WorldWideWebPage-AIS> <http://www.w3.org/2000/01/rdf-schema#comment> "#$WorldWideWebPage-AIS is the collection of instances of #$WebPage-AIS that are #$subInformation of the #$WorldWideWeb-DynamicIndexedInfoSource." ;
	a <http://sw.cyc.com/2006/07/27/cyc/ObjectType> ;
	<http://sw.cyc.com/2006/07/27/cyc/prettyString-Canonical> "web page" ;
	<http://sw.cyc.com/2006/07/27/cyc/prettyString> "Page" , "pages" , "web pages" , "www page" , "www pages" , "world wide web page" , "world wide web pages" , "webpage" , "webpages" ;
	<http://www.w3.org/2000/01/rdf-schema#subClassOf> <http://sw.cyc.com/2006/07/27/cyc/WebPage-AIS> .

<http://sw.cyc.com/2006/07/27/cyc/IBTContentType> <http://www.w3.org/2000/01/rdf-schema#comment> "A collection of collections.  Instances of #$IBTContentType are specs of #$InformationBearingThing.  Each such instance (that is, each IBTContentType) is specified primarily by the type or organization of information contained by its instances.  For example, #$JazzMusic, #$ComputerProgramCopy, and #$Spreadsheet are all IBTContentTypes, since each is primarily distinguished from other kinds of IBTs by the nature or organization of the information contained.  Non-examples include #$CompactDisc-Generic, since compact discs are distinguished by their physical format, rather than their information content. (see #$IBTFormatType). IBTContentTypes whose instances contain not just similar but identical information (such as a single magazine issue, or #$CitizenKane-TheMovie), should be made specs of the more specific #$SpecifiedInformationBearingThingType.  IBTContentTypes whose instances are members of a series (for example, #$StarTrek-Classic) should be made instances of #$IBTSeriesType." ;
	a <http://sw.cyc.com/2006/07/27/cyc/AtemporalNecessarilyEssentialCollectionType> , <http://sw.cyc.com/2006/07/27/cyc/FacetingCollectionType> , <http://sw.cyc.com/2006/07/27/cyc/SecondOrderCollection> ;
	<http://sw.cyc.com/2006/07/27/cyc/prettyString-Canonical> "type of information bearing thing classified by content" ;
	<http://sw.cyc.com/2006/07/27/cyc/prettyString> "types of information bearing thing classified by content" ;
	<http://www.w3.org/2000/01/rdf-schema#subClassOf> <http://sw.cyc.com/2006/07/27/cyc/TemporalStuffType> ;
	<http://sw.cyc.com/2006/07/27/cyc/typeGenls> <http://sw.cyc.com/2006/07/27/cyc/InformationStore> .

<http://sw.cyc.com/2006/07/27/cyc/AccessPath-TheProgram> a <http://sw.cyc.com/2006/07/27/cyc/Individual> , <http://sw.cyc.com/2006/07/27/cyc/UnversionedProgram> , <http://sw.cyc.com/2006/07/27/cyc/ServerProgram> ;
	<http://sw.cyc.com/2006/07/27/cyc/prettyString-Canonical> "Cisco AccessPath" .

<http://sw.cyc.com/2006/07/27/cyc/AccessServer-TheProgram> a <http://sw.cyc.com/2006/07/27/cyc/Individual> , <http://sw.cyc.com/2006/07/27/cyc/UnversionedProgram> , <http://sw.cyc.com/2006/07/27/cyc/ServerProgram> ;
	<http://sw.cyc.com/2006/07/27/cyc/prettyString-Canonical> "Cisco Access Server" .

<http://sw.cyc.com/2006/07/27/cyc/accessSlotForType> a <http://www.w3.org/2000/01/rdf-schema#Property> ;
	<http://sw.cyc.com/2006/07/27/cyc/prettyString-Canonical> "Access Slot For Type" ;
	<http://sw.cyc.com/2006/07/27/cyc/arity> "2"^^<http://www.w3.org/2001/XMLSchema#long> ;
	<http://sw.cyc.com/2006/07/27/cyc/arg2QuotedIsa> <http://sw.cyc.com/2006/07/27/cyc/SubLList> ;
	<http://sw.cyc.com/2006/07/27/cyc/quotedArgument> "2"^^<http://www.w3.org/2001/XMLSchema#long> .

<http://sw.cyc.com/2006/07/27/cyc/SubLList> <http://www.w3.org/2000/01/rdf-schema#comment> "A collection of list-denoting expressions that are not represented in CycL (i.e. they are not #$CycLConstants or #$CycLNonAtomicTerms) but are represented in SubL, the underlying implementation language of the Cyc system.  Each instance of #$SubLList is a sequence of #$SubLListOrAtoms (q.v.) enclosed in parentheses.  SubL lists are those things that pass the #$defnIff LISTP. Note that this collection is \"quoted\" (see #$quotedCollection)." ;
	a <http://www.w3.org/2002/07/owl#Class> , <http://sw.cyc.com/2006/07/27/cyc/KBDependentCollection> , <http://sw.cyc.com/2006/07/27/cyc/AtemporalNecessarilyEssentialCollectionType> , <http://sw.cyc.com/2006/07/27/cyc/PragmaticallyDecontextualizedCollection> , <http://sw.cyc.com/2006/07/27/cyc/SubLExpressionType> , <http://sw.cyc.com/2006/07/27/cyc/ConnectionsToTheComputationalSubstrate-Fundamental-Topic> ;
	<http://sw.cyc.com/2006/07/27/cyc/prettyString-Canonical> "SubL list" ;
	<http://sw.cyc.com/2006/07/27/cyc/prettyString> "SubL lists" ;
	<http://www.w3.org/2000/01/rdf-schema#subClassOf> <http://sw.cyc.com/2006/07/27/cyc/KSID> , <http://sw.cyc.com/2006/07/27/cyc/SubLListOrAtom> ;
	<http://sw.cyc.com/2006/07/27/cyc/oldConstantName> "CycSystemList" ;
	<http://sw.cyc.com/2006/07/27/cyc/collectionConventionMt> <http://sw.cyc.com/2006/07/27/cyc/UniversalVocabularyMt> .

<http://sw.cyc.com/2006/07/27/cyc/AccessSoftwareInc> a <http://sw.cyc.com/2006/07/27/cyc/Individual> , <http://sw.cyc.com/2006/07/27/cyc/SoftwareVendor> ;
	<http://sw.cyc.com/2006/07/27/cyc/prettyString-Canonical> "Access Software" ;
	<http://sw.cyc.com/2006/07/27/cyc/prettyString> "Access Software, Inc." .

<http://sw.cyc.com/2006/07/27/cyc/Access-TheProgram> a <http://sw.cyc.com/2006/07/27/cyc/Individual> , <http://sw.cyc.com/2006/07/27/cyc/UnversionedProgram> , <http://sw.cyc.com/2006/07/27/cyc/UtilityProgram> ;
	<http://sw.cyc.com/2006/07/27/cyc/prettyString-Canonical> "access" .

<http://sw.cyc.com/2006/07/27/cyc/accessToExpected> <http://www.w3.org/2000/01/rdf-schema#comment> "(#$accessToExpected AGT IND) means that it is expected that the individual AGT would have access (see #$hasAccess) to the individual IND." ;
	a <http://www.w3.org/2000/01/rdf-schema#Property> ;
	<http://sw.cyc.com/2006/07/27/cyc/prettyString-Canonical> "Access To Expected" ;
	<http://www.w3.org/2000/01/rdf-schema#domain> <http://sw.cyc.com/2006/07/27/cyc/Agent-Generic> ;
	<http://sw.cyc.com/2006/07/27/cyc/arity> "2"^^<http://www.w3.org/2001/XMLSchema#long> ;
	<http://www.w3.org/2000/01/rdf-schema#range> <http://sw.cyc.com/2006/07/27/cyc/Individual> ;
	<http://sw.cyc.com/2006/07/27/cyc/arg1Format> <http://sw.cyc.com/2006/07/27/cyc/openEntryFormatInArgs> ;
	<http://sw.cyc.com/2006/07/27/cyc/arg2Format> <http://sw.cyc.com/2006/07/27/cyc/openEntryFormatInArgs> .

<http://sw.cyc.com/2006/07/27/cyc/accessToNotAmenable> <http://www.w3.org/2000/01/rdf-schema#comment> "(#$accessToNotAmenable AGT IND) means that it is expected that the individual AGT would not have access (see #$hasAccess) to the individual IND." ;
	a <http://www.w3.org/2000/01/rdf-schema#Property> ;
	<http://sw.cyc.com/2006/07/27/cyc/prettyString-Canonical> "Access To Not Amenable" ;
	<http://www.w3.org/2000/01/rdf-schema#domain> <http://sw.cyc.com/2006/07/27/cyc/Agent-Generic> ;
	<http://sw.cyc.com/2006/07/27/cyc/arity> "2"^^<http://www.w3.org/2001/XMLSchema#long> ;
	<http://www.w3.org/2000/01/rdf-schema#range> <http://sw.cyc.com/2006/07/27/cyc/Individual> ;
	<http://sw.cyc.com/2006/07/27/cyc/arg1Format> <http://sw.cyc.com/2006/07/27/cyc/openEntryFormatInArgs> ;
	<http://sw.cyc.com/2006/07/27/cyc/arg2Format> <http://sw.cyc.com/2006/07/27/cyc/openEntryFormatInArgs> .

<http://sw.cyc.com/2006/07/27/cyc/accessToTypeExpected> <http://www.w3.org/2000/01/rdf-schema#comment> "(#$accessToTypeExpected AGT TYPE) means that it is expected that the individual AGT would have access (see #$hasAccess) to any individuals that are instances of the collection TYPE." ;
	a <http://www.w3.org/2000/01/rdf-schema#Property> , <http://sw.cyc.com/2006/07/27/cyc/FirstOrderCollectionPredicate> ;
	<http://sw.cyc.com/2006/07/27/cyc/prettyString-Canonical> "Access To Type Expected" ;
	<http://www.w3.org/2000/01/rdf-schema#domain> <http://sw.cyc.com/2006/07/27/cyc/Agent-Generic> ;
	<http://sw.cyc.com/2006/07/27/cyc/arity> "2"^^<http://www.w3.org/2001/XMLSchema#long> ;
	<http://www.w3.org/2000/01/rdf-schema#range> <http://sw.cyc.com/2006/07/27/cyc/FirstOrderCollection> ;
	<http://sw.cyc.com/2006/07/27/cyc/arg2Genl> <http://sw.cyc.com/2006/07/27/cyc/Individual> ;
	<http://sw.cyc.com/2006/07/27/cyc/arg1Format> <http://sw.cyc.com/2006/07/27/cyc/openEntryFormatInArgs> ;
	<http://sw.cyc.com/2006/07/27/cyc/arg2Format> <http://sw.cyc.com/2006/07/27/cyc/openEntryFormatInArgs> ;
	<http://sw.cyc.com/2006/07/27/cyc/negationPreds> <http://sw.cyc.com/2006/07/27/cyc/accessToTypeNotAmenable> , <http://sw.cyc.com/2006/07/27/cyc/readableByNotAmenable-Type> .

<http://sw.cyc.com/2006/07/27/cyc/accessToTypeNotAmenable> <http://www.w3.org/2000/01/rdf-schema#comment> "(#$accessToTypeNotAmenable AGT TYPE) means that it is expected that the individual AGT would not have access (see #$hasAccess) to any individuals that are instances of the collection TYPE." ;
	a <http://www.w3.org/2000/01/rdf-schema#Property> , <http://sw.cyc.com/2006/07/27/cyc/FirstOrderCollectionPredicate> ;
	<http://sw.cyc.com/2006/07/27/cyc/prettyString-Canonical> "Access To Type Not Amenable" ;
	<http://www.w3.org/2000/01/rdf-schema#domain> <http://sw.cyc.com/2006/07/27/cyc/Agent-Generic> ;
	<http://sw.cyc.com/2006/07/27/cyc/arity> "2"^^<http://www.w3.org/2001/XMLSchema#long> ;
	<http://www.w3.org/2000/01/rdf-schema#range> <http://sw.cyc.com/2006/07/27/cyc/FirstOrderCollection> ;
	<http://sw.cyc.com/2006/07/27/cyc/arg2Genl> <http://sw.cyc.com/2006/07/27/cyc/Individual> ;
	<http://sw.cyc.com/2006/07/27/cyc/arg1Format> <http://sw.cyc.com/2006/07/27/cyc/openEntryFormatInArgs> ;
	<http://sw.cyc.com/2006/07/27/cyc/arg2Format> <http://sw.cyc.com/2006/07/27/cyc/openEntryFormatInArgs> .

<http://sw.cyc.com/2006/07/27/cyc/readableByNotAmenable-Type> <http://www.w3.org/2000/01/rdf-schema#comment> "(#$readableByNotAmenable-Type FILE-TYPE ACCOUNT) means that it is expected that the account ACCOUNT would not be able to read (see #$readableBy) files of the type FILE-TYPE." ;
	a <http://www.w3.org/2000/01/rdf-schema#Property> , <http://sw.cyc.com/2006/07/27/cyc/FirstOrderCollectionPredicate> ;
	<http://sw.cyc.com/2006/07/27/cyc/prettyString-Canonical> "Readable By Not Amenable Type" ;
	<http://www.w3.org/2000/01/rdf-schema#domain> <http://sw.cyc.com/2006/07/27/cyc/FirstOrderCollection> ;
	<http://sw.cyc.com/2006/07/27/cyc/arity> "2"^^<http://www.w3.org/2001/XMLSchema#long> ;
	<http://www.w3.org/2000/01/rdf-schema#range> <http://sw.cyc.com/2006/07/27/cyc/ComputerAccount> ;
	<http://sw.cyc.com/2006/07/27/cyc/arg1Genl> <http://sw.cyc.com/2006/07/27/cyc/ComputerFile-Abstract> ;
	<http://sw.cyc.com/2006/07/27/cyc/arg1Format> <http://sw.cyc.com/2006/07/27/cyc/openEntryFormatInArgs> ;
	<http://sw.cyc.com/2006/07/27/cyc/arg2Format> <http://sw.cyc.com/2006/07/27/cyc/openEntryFormatInArgs> ;
	<http://sw.cyc.com/2006/07/27/cyc/negationPreds> <http://sw.cyc.com/2006/07/27/cyc/readableByExpected-Type> .

<http://sw.cyc.com/2006/07/27/cyc/readableByExpected-Type> <http://www.w3.org/2000/01/rdf-schema#comment> "(#$readableByExpected-Type FILE-TYPE ACCOUNT) means that it is expected that the account ACCOUNT would be able to read (see #$readableBy) some files of the type FILE-TYPE.  See also #$readableByNotAmenable-Type." ;
	a <http://www.w3.org/2000/01/rdf-schema#Property> , <http://sw.cyc.com/2006/07/27/cyc/FirstOrderCollectionPredicate> ;
	<http://sw.cyc.com/2006/07/27/cyc/prettyString-Canonical> "Readable By Expected Type" ;
	<http://www.w3.org/2000/01/rdf-schema#domain> <http://sw.cyc.com/2006/07/27/cyc/FirstOrderCollection> ;
	<http://sw.cyc.com/2006/07/27/cyc/arity> "2"^^<http://www.w3.org/2001/XMLSchema#long> ;
	<http://www.w3.org/2000/01/rdf-schema#range> <http://sw.cyc.com/2006/07/27/cyc/ComputerAccount> ;
	<http://sw.cyc.com/2006/07/27/cyc/arg1Genl> <http://sw.cyc.com/2006/07/27/cyc/ComputerFile-Abstract> ;
	<http://sw.cyc.com/2006/07/27/cyc/arg1Format> <http://sw.cyc.com/2006/07/27/cyc/openEntryFormatInArgs> ;
	<http://sw.cyc.com/2006/07/27/cyc/arg2Format> <http://sw.cyc.com/2006/07/27/cyc/openEntryFormatInArgs> .

<http://sw.cyc.com/2006/07/27/cyc/AccessValidationFault> <http://www.w3.org/2000/01/rdf-schema#comment> "#$AccessValidationFault is an attribute of computer programs.  A program has an #$AccessValidationFault if its corresponding computer process can invoke an operation or read or write to a file outside the access domain of the user, accepts input from an unauthorized user, or fails to authenticate a user.  Note that #$AccessValidationFault is distinct from #$AuthenticationSoftwareBypassFault, which is an attribute of programs that actually do authenticate, albeit poorly." ;
	a <http://sw.cyc.com/2006/07/27/cyc/SoftwareObjectTypeByFault> ;
	<http://sw.cyc.com/2006/07/27/cyc/prettyString-Canonical> "access validation fault" ;
	<http://sw.cyc.com/2006/07/27/cyc/prettyString> "access validation faults" ;
	<http://www.w3.org/2000/01/rdf-schema#subClassOf> <http://sw.cyc.com/2006/07/27/cyc/ProgramFault> .

<http://sw.cyc.com/2006/07/27/cyc/ProgramFault> <http://www.w3.org/2000/01/rdf-schema#comment> "#$ProgramFault denotes the most general fault of computer software that leads to vulnerabilities in computers running that software.  Only extremely rarely would one assert simply that a program has this attribute, because such an assertion would amount to saying merely that a program has some unspecified flaw that could cause computers to be vulnerable to some unspecified threat.  In general it is better to assert that a program has a much more specific fault." ;
	a <http://sw.cyc.com/2006/07/27/cyc/SoftwareObjectTypeByFault> ;
	<http://sw.cyc.com/2006/07/27/cyc/prettyString-Canonical> "program fault" ;
	<http://sw.cyc.com/2006/07/27/cyc/prettyString> "program faults" ;
	<http://www.w3.org/2000/01/rdf-schema#subClassOf> <http://sw.cyc.com/2006/07/27/cyc/ComputerProgram-CW> , <http://sw.cyc.com/2006/07/27/cyc/FaultyThing> .

<http://sw.cyc.com/2006/07/27/cyc/SoftwareObjectTypeByFault> <http://www.w3.org/2000/01/rdf-schema#comment> "A collection of collections.  Each instance of #$SoftwareObjectTypeByFault is a collection of software objects that have a certain fault." ;
	a <http://sw.cyc.com/2006/07/27/cyc/FacetingCollectionType> , <http://sw.cyc.com/2006/07/27/cyc/SecondOrderCollection> ;
	<http://sw.cyc.com/2006/07/27/cyc/prettyString-Canonical> "software object type by fault" ;
	<http://www.w3.org/2000/01/rdf-schema#subClassOf> <http://sw.cyc.com/2006/07/27/cyc/ObjectType> , <http://sw.cyc.com/2006/07/27/cyc/TemporalStuffType> , <http://sw.cyc.com/2006/07/27/cyc/FacetInstanceCollection> ;
	<http://sw.cyc.com/2006/07/27/cyc/sharedNotes> <http://sw.cyc.com/2006/07/27/cyc/SharedNoteOnGenlsRelationsBetweenFacetingCollectionTypes> ;
	<http://sw.cyc.com/2006/07/27/cyc/typeGenls> <http://sw.cyc.com/2006/07/27/cyc/SoftwareObject> .

<http://sw.cyc.com/2006/07/27/cyc/AccessWorldwideCommunicationsInc> a <http://sw.cyc.com/2006/07/27/cyc/Individual> , <http://sw.cyc.com/2006/07/27/cyc/PubliclyHeldCorporation> ;
	<http://sw.cyc.com/2006/07/27/cyc/prettyString-Canonical> "Access Worldwide Communications, Inc." ;
	<http://sw.cyc.com/2006/07/27/cyc/prettyString> "Access Worldwide Communications" .

<http://sw.cyc.com/2006/07/27/cyc/AccidentallyLeavingSomethingSomewhere> <http://www.w3.org/2000/01/rdf-schema#comment> "A #$FirstOrderCollection and specialization of #$Accident and #$Forgetting-Generic.  Each instance of #$AccidentallyLeavingSomethingSomewhere is an #$Event in which an #$Agent accidentally leaves something somewhere, e.g. Bob's accidentally leaving his hat at a restaurant." , "A collection of events; a subcollection of #$Accident. In each #$AccidentallyLeavingSomethingSomewhere, someone leaves something behind unintentionally." ;
	a <http://sw.cyc.com/2006/07/27/cyc/FirstOrderCollection> ;
	<http://sw.cyc.com/2006/07/27/cyc/prettyString-Canonical> "forgeting" ;
	<http://sw.cyc.com/2006/07/27/cyc/prettyString> "leave" , "left" , "leaves" , "leaving" , "have left" , "has left" , "will leave" , "had left" .

<http://sw.cyc.com/2006/07/27/cyc/AccipitrineFamily> <http://www.w3.org/2000/01/rdf-schema#subClassOf> <http://sw.cyc.com/2006/07/27/cyc/FalconiformOrder> ;
	<http://sw.cyc.com/2006/07/27/cyc/superTaxons> <http://sw.cyc.com/2006/07/27/cyc/FalconiformOrder> .

<http://sw.cyc.com/2006/07/27/cyc/FalconiformOrder> <http://www.w3.org/2000/01/rdf-schema#comment> "The order Falconiformes, comprising the vultures, hawks, eagles, ospreys, falcons, caracaras, etc. They are swift and graceful, and known for their raptorial, or predatory, skills. The have hooked beaks, and highly developed senses of sight and hearing." ;
	a <http://sw.cyc.com/2006/07/27/cyc/BiologicalOrder> ;
	<http://sw.cyc.com/2006/07/27/cyc/prettyString-Canonical> "falconiform" ;
	<http://sw.cyc.com/2006/07/27/cyc/prettyString> "falconiforms" , "Falconiformes" ;
	<http://www.w3.org/2000/01/rdf-schema#subClassOf> <http://sw.cyc.com/2006/07/27/cyc/BirdOfPrey> .

<http://sw.cyc.com/2006/07/27/cyc/BiologicalFamily> <http://www.w3.org/2000/01/rdf-schema#comment> "The collection of biological taxonomic subdivisions below #$BiologicalOrder (or #$BiologicalSuborder) and above #$BiologicalGenus.  Especially important in Botanical classification." ;
	a <http://sw.cyc.com/2006/07/27/cyc/FacetingCollectionType> , <http://sw.cyc.com/2006/07/27/cyc/Biology-Topic> , <http://sw.cyc.com/2006/07/27/cyc/BiologicalTaxonType> ;
	<http://sw.cyc.com/2006/07/27/cyc/prettyString-Canonical> "biological family" ;
	<http://sw.cyc.com/2006/07/27/cyc/prettyString> "family" , "families" , "taxonomic family" , "taxonomic families" , "biological families" ;
	<http://www.w3.org/2000/01/rdf-schema#subClassOf> <http://sw.cyc.com/2006/07/27/cyc/FacetInstanceCollection> , <http://sw.cyc.com/2006/07/27/cyc/BiologicalTaxon> ;
	<http://sw.cyc.com/2006/07/27/cyc/sharedNotes> <http://sw.cyc.com/2006/07/27/cyc/SharedNoteOnGenlsRelationsBetweenFacetingCollectionTypes> ;
	<http://sw.cyc.com/2006/07/27/cyc/typeGenls> <http://sw.cyc.com/2006/07/27/cyc/Organism-Whole> .

<http://sw.cyc.com/2006/07/27/cyc/AcclaimEntertainmentInc> a <http://sw.cyc.com/2006/07/27/cyc/Individual> , <http://sw.cyc.com/2006/07/27/cyc/SoftwareVendor> , <http://sw.cyc.com/2006/07/27/cyc/PubliclyHeldCorporation> ;
	<http://sw.cyc.com/2006/07/27/cyc/prettyString-Canonical> "Acclaim Entertainment" ;
	<http://sw.cyc.com/2006/07/27/cyc/prettyString> "Acclaim Entertainment, Inc." .

<http://sw.cyc.com/2006/07/27/cyc/AccoladeInc> a <http://sw.cyc.com/2006/07/27/cyc/Individual> , <http://sw.cyc.com/2006/07/27/cyc/SoftwareVendor> ;
	<http://sw.cyc.com/2006/07/27/cyc/prettyString-Canonical> "accolade" ;
	<http://sw.cyc.com/2006/07/27/cyc/prettyString> "Accolade, Inc." .

<http://sw.cyc.com/2006/07/27/cyc/Accommodating-HelpingAnAgent> <http://www.w3.org/2000/01/rdf-schema#comment> "A sub-collection of #$HelpingAnAgent. Each instance is the act of providing something (lodging or seat or food) to meet a need of someone." ;
	a <http://sw.cyc.com/2006/07/27/cyc/FirstOrderCollection> , <http://sw.cyc.com/2006/07/27/cyc/TypicalHumanActivityType-AtLeastOnce> ;
	<http://sw.cyc.com/2006/07/27/cyc/prettyString-Canonical> "accommodation" ;
	<http://www.w3.org/2000/01/rdf-schema#subClassOf> <http://sw.cyc.com/2006/07/27/cyc/HelpingAnAgent> ;
	<http://sw.cyc.com/2006/07/27/cyc/quotedIsa> <http://sw.cyc.com/2006/07/27/cyc/WordNetWorkflowConstant-NotFullyReviewed> .

<http://sw.cyc.com/2006/07/27/cyc/HelpingAnAgent> <http://www.w3.org/2000/01/rdf-schema#comment> "A specialization of both #$PurposefulPhysicalAction and #$SocialOccurrence.  Each instance of #$HelpingAnAgent is an event in which some agent (see the collection #$Agent) helps another agent, either by doing something that directly benefits that agent, or by preventing something that would harm that agent.  Notable specializations of #$HelpingAnAgent include #$RescuingSomeone, #$ReliefOperation, and #$ServiceEvent." ;
	a <http://sw.cyc.com/2006/07/27/cyc/TemporalStuffType> , <http://sw.cyc.com/2006/07/27/cyc/KEClarifyingCollectionType> , <http://sw.cyc.com/2006/07/27/cyc/TypicalHumanActivityType-AtLeastOnce> ;
	<http://sw.cyc.com/2006/07/27/cyc/prettyString-Canonical> "helping" ;
	<http://sw.cyc.com/2006/07/27/cyc/prettyString> "AIDS" , "aid" , "minister" , "Help" , "ministers" , "aided" , "aiding" , "have aided" .

<http://sw.cyc.com/2006/07/27/cyc/Accompaniment> <http://sw.cyc.com/2006/07/27/cyc/prettyString> "co occurs" , "co occurring" , "co have occurred" , "co has occurred" , "co will occur" , "co had occurred" , "co will have occurred" , "co occurrences" ;
	<http://www.w3.org/2000/01/rdf-schema#subClassOf> <http://sw.cyc.com/2006/07/27/cyc/CoexistingWithSomethingElse> ;
	<http://sw.cyc.com/2006/07/27/cyc/quotedIsa> <http://sw.cyc.com/2006/07/27/cyc/WordNetWorkflowConstant-NotFullyReviewed> .

<http://sw.cyc.com/2006/07/27/cyc/CoexistingWithSomethingElse> <http://www.w3.org/2000/01/rdf-schema#comment> "A collection of situations; a subcollection of #$SomethingExisting. In each #$CoexistingWithSomethingElse, something exists together with something else." ;
	a <http://sw.cyc.com/2006/07/27/cyc/FirstOrderCollection> ;
	<http://sw.cyc.com/2006/07/27/cyc/prettyString-Canonical> "coexisting" ;
	<http://sw.cyc.com/2006/07/27/cyc/prettyString> "coexist" , "coexisted" , "coexists" , "have coexisted" , "has coexisted" , "will coexist" , "had coexisted" , "will have coexisted" ;
	<http://www.w3.org/2000/01/rdf-schema#subClassOf> <http://sw.cyc.com/2006/07/27/cyc/SomethingExisting> ;
	<http://sw.cyc.com/2006/07/27/cyc/quotedIsa> <http://sw.cyc.com/2006/07/27/cyc/WordNetWorkflowConstant-NotFullyReviewed> .

<http://sw.cyc.com/2006/07/27/cyc/accomplices> <http://www.w3.org/2000/01/rdf-schema#comment> "(#$accomplices AGT-1 AGT-2) holds just in case there is some event in which AGT-1 and AGT-2 are cooperating (to some degree) in.  This predicate is temporally quantifiable and it holds during the time period when AGT-1 and AGT-2 were actively cooperating.  Most often this predicate is used to characterize the cooperating performers of illegal acts.  But, two agents could also be accomplices in the performance of legal acts such as a planning a surprise birthday party." ;
	a <http://www.w3.org/2002/07/owl#TransitiveProperty> , <http://sw.cyc.com/2006/07/27/cyc/CoexistingObjectsPredicate> , <http://www.w3.org/2002/07/owl#SymmetricProperty> , <http://sw.cyc.com/2006/07/27/cyc/IrreflexiveBinaryPredicate> , <http://sw.cyc.com/2006/07/27/cyc/RelationalNounSlot> , <http://sw.cyc.com/2006/07/27/cyc/PersonalAssociationPredReplacement> , <http://sw.cyc.com/2006/07/27/cyc/PersonalAssociationPredicate> ;
	<http://sw.cyc.com/2006/07/27/cyc/prettyString-Canonical> "accomplice" ;
	<http://sw.cyc.com/2006/07/27/cyc/prettyString> "accomplices" ;
	<http://sw.cyc.com/2006/07/27/cyc/quotedIsa> <http://sw.cyc.com/2006/07/27/cyc/TerrorismOntologyConstant> ;
	<http://www.w3.org/2000/01/rdf-schema#domain> <http://sw.cyc.com/2006/07/27/cyc/IndividualAgent> ;
	<http://sw.cyc.com/2006/07/27/cyc/arity> "2"^^<http://www.w3.org/2001/XMLSchema#long> ;
	<http://www.w3.org/2000/01/rdf-schema#range> <http://sw.cyc.com/2006/07/27/cyc/IndividualAgent> ;
	<http://www.w3.org/2000/01/rdf-schema#subPropertyOf> <http://sw.cyc.com/2006/07/27/cyc/mutualAcquaintances> , <http://sw.cyc.com/2006/07/27/cyc/positiveVestedInterest> , <http://sw.cyc.com/2006/07/27/cyc/affiliatedWith> ;
	<http://sw.cyc.com/2006/07/27/cyc/genlInverse> <http://sw.cyc.com/2006/07/27/cyc/accomplices> .

<http://sw.cyc.com/2006/07/27/cyc/genlInverse> <http://www.w3.org/2000/01/rdf-schema#comment> "A #$MetaPredicate for stating that one binary  predicate is a generalization of the <i>inverse</i> of another binary predicate.   <code>(#$genlInverse PRED GENL-INV-PRED)</code> means that <code>GENL-INV-PRED</code> is a  \"generalized inverse\" of <code>PRED</code>.  That is, <code>(PRED ARG1 ARG2)</code> implies  <code>(GENL-INV-PRED ARG2 ARG1)</code>.  For example, <code>(#$genlInverse #$grandchildren #$ancestors)</code> means that grandparents are  ancestors of their grandchildren.  See also #$genlPreds and #$negationInverse." ;
	a <http://www.w3.org/2002/07/owl#TransitiveProperty> , <http://www.w3.org/2002/07/owl#SymmetricProperty> , <http://sw.cyc.com/2006/07/27/cyc/AntiSymmetricBinaryPredicate> , <http://sw.cyc.com/2006/07/27/cyc/AsymmetricBinaryPredicate> , <http://sw.cyc.com/2006/07/27/cyc/ReflexiveBinaryPredicate> , <http://sw.cyc.com/2006/07/27/cyc/IrreflexiveBinaryPredicate> , <http://sw.cyc.com/2006/07/27/cyc/DefaultMonotonicPredicate> .

<http://sw.cyc.com/2006/07/27/cyc/AccomplishmentType> <http://sw.cyc.com/2006/07/27/cyc/prettyString> "accomplishment type" , "accomplishment types" , "types of accomplishment" ;
	<http://www.w3.org/2000/01/rdf-schema#subClassOf> <http://sw.cyc.com/2006/07/27/cyc/TemporalObjectType> , <http://sw.cyc.com/2006/07/27/cyc/SituationalObjectType> ;
	<http://sw.cyc.com/2006/07/27/cyc/sharedNotes> <http://sw.cyc.com/2006/07/27/cyc/NoteOnTheClassificationOfAktionsarten> , <http://sw.cyc.com/2006/07/27/cyc/SharedNoteOnProcessesVsAccomplishments> ;
	<http://www.w3.org/2002/07/owl#disjointWith> <http://sw.cyc.com/2006/07/27/cyc/ProcessType> ;
	<http://sw.cyc.com/2006/07/27/cyc/typeGenls> <http://sw.cyc.com/2006/07/27/cyc/Event> .

<http://sw.cyc.com/2006/07/27/cyc/singleEntryFormatInArgs> <http://www.w3.org/2000/01/rdf-schema#comment> "An instance of #$SpecificEntryFormatPredicate (q.v.).  (#$singleEntryFormatInArgs PRED N) means that, for any particular way of fixing the other arguments to PRED besides the Nth, there is at most one thing such that, if taken as the Nth argument, PRED holds of those arguments.  That is, if the sequences <... ARGN ...> and <... ARGN-PRIME ...> differ at most in their Nth items and both (PRED ... ARGN ...) and (PRED ... ARGN-PRIME ...) hold, then ARGN = ARGN-PRIME (see #$equals).  For example, #$singleEntryFormatInArgs holds of #$biologicalMother with respect to its second argument-place, since an animal can only have one biological mother.  A predicate with a single-entry format argument-place is thus a #$StrictlyFunctionalPredicate (q.v.) that is \"functional\" with respect to that argument-place (see #$strictlyFunctionalInArgs).  Contrast with #$openEntryFormatInArgs." ;
	a <http://sw.cyc.com/2006/07/27/cyc/IntangibleObjectRelatingPredicate> , <http://sw.cyc.com/2006/07/27/cyc/MetaPredicate> , <http://sw.cyc.com/2006/07/27/cyc/SpecificEntryFormatPredicate> ;
	<http://sw.cyc.com/2006/07/27/cyc/prettyString-Canonical> "Single Entry Format In Args" ;
	<http://sw.cyc.com/2006/07/27/cyc/quotedIsa> <http://sw.cyc.com/2006/07/27/cyc/OpenCycDefinitionalPredicate> ;
	<http://www.w3.org/2000/01/rdf-schema#domain> <http://sw.cyc.com/2006/07/27/cyc/StrictlyFunctionalPredicate> ;
	<http://sw.cyc.com/2006/07/27/cyc/arity> "2"^^<http://www.w3.org/2001/XMLSchema#long> ;
	<http://www.w3.org/2000/01/rdf-schema#range> <http://sw.cyc.com/2006/07/27/cyc/PositiveInteger> ;
	<http://www.w3.org/2000/01/rdf-schema#subPropertyOf> <http://sw.cyc.com/2006/07/27/cyc/strictlyFunctionalInArgs> .

<http://sw.cyc.com/2006/07/27/cyc/ProcessType> <http://www.w3.org/2000/01/rdf-schema#comment> "A #$SecondOrderCollection.  #$ProcessType is the collection intersection of #$TemporalStuffType and #$DurativeEventType; that is, a thing is an instance of #$ProcessType if and only if it is an instance of both #$TemporalStuffType and #$DurativeEventType.  Instances of #$ProcessType can be constructed from instances of #$AccomplishmentType using #$ProcessFn (q.v.)." ;
	a <http://www.w3.org/2002/07/owl#Class> , <http://sw.cyc.com/2006/07/27/cyc/AtemporalNecessarilyEssentialCollectionType> , <http://sw.cyc.com/2006/07/27/cyc/SecondOrderCollection> ;
	<http://sw.cyc.com/2006/07/27/cyc/prettyString-Canonical> "process type" ;
	<http://sw.cyc.com/2006/07/27/cyc/prettyString> "type of temporally stuff-like thing that has been also a type of durative event" ;
	<http://www.w3.org/2000/01/rdf-schema#subClassOf> <http://sw.cyc.com/2006/07/27/cyc/FirstOrderCollection> , <http://sw.cyc.com/2006/07/27/cyc/TemporalStuffType> , <http://sw.cyc.com/2006/07/27/cyc/DurativeEventType> ;
	<http://sw.cyc.com/2006/07/27/cyc/sharedNotes> <http://sw.cyc.com/2006/07/27/cyc/NoteOnTheClassificationOfAktionsarten> , <http://sw.cyc.com/2006/07/27/cyc/SharedNoteOnProcessesVsAccomplishments> ;
	<http://sw.cyc.com/2006/07/27/cyc/typeGenls> <http://sw.cyc.com/2006/07/27/cyc/Event> .

<http://sw.cyc.com/2006/07/27/cyc/SituationalObjectType> <http://www.w3.org/2000/01/rdf-schema#comment> """A specialization of #$ObjectType (q.v.) whose instances are all and only those collections that are situationally object-like. A collection <code>COL</code> is situationally object-like just in case it generally holds that any proper sub-situation (see #$properSubSituations) of an instance of <code>COL</code> is not itself an instance of <code>COL</code>.  More precisely, a collection <code>COL</code> is an instance of #$SituationalObjectType just in case it satisfies the following: For any distinct <code>OBJ1</code> and <code>OBJ2</code>, if <code>(#$isa OBJ1 COL)</code> and <code>(#$subSituations OBJ1 OBJ2)</code>, then <i>not</i> <code>(#$isa OBJ2 COL)</code>.
<p>
For example, none of the proper sub-situations of a #$Suicide is itself a suicide.  Likewise for #$CrossingAGap.  So #$Suicide and #$CrossingAGap are both instances of #$SituationalObjectType. Conversely, a proper sub-situation of a given #$SportsCompetition might itself be a #$SportsCompetition (e.g. the biathalon during some Olympic games); so #$SportsCompetition is <i>not</i> a situational-object-type.
<p>
See #$SituationalStuffType for the disjoint notion of being situationally stuff-like.""" ;
	a <http://www.w3.org/2002/07/owl#Class> , <http://sw.cyc.com/2006/07/27/cyc/AtemporalNecessarilyEssentialCollectionType> , <http://sw.cyc.com/2006/07/27/cyc/FacetingCollectionType> , <http://sw.cyc.com/2006/07/27/cyc/SecondOrderCollection> ;
	<http://sw.cyc.com/2006/07/27/cyc/prettyString-Canonical> "situational object type" ;
	<http://www.w3.org/2000/01/rdf-schema#subClassOf> <http://sw.cyc.com/2006/07/27/cyc/ObjectType> , <http://sw.cyc.com/2006/07/27/cyc/FirstOrderCollection> .

<http://sw.cyc.com/2006/07/27/cyc/TestOWLExportConcept> <http://www.w3.org/2000/01/rdf-schema#comment> "A #$ConceptTypeByDomain (q.v.).  Instances of #$TestOWLExportConcept are concepts each of which tests some aspect of the new export schema." ;
	a <http://sw.cyc.com/2006/07/27/cyc/NonAbducibleCollection> , <http://sw.cyc.com/2006/07/27/cyc/ConceptTypeByDomain> ;
	<http://sw.cyc.com/2006/07/27/cyc/prettyString-Canonical> "test OWL export concept" ;
	<http://www.w3.org/2000/01/rdf-schema#subClassOf> <http://www.w3.org/2002/07/owl#Thing> .

<http://sw.cyc.com/2006/07/27/cyc/NoteOnTheClassificationOfAktionsarten> <http://www.w3.org/2000/01/rdf-schema#comment> "This refers to the classification of verb phrases according to their denotation in accomplishments, achievements, activities and states, a classification that is standardly used in many NL semantics treatments -- i.e., according to the `type of action' they denote (not sure when the German term came into use, but it seems that it's now in common use). The standard contemporary reference for the classification is work by the philosopher Zeno Vendler, although its origins are traced to #$Aristotle's writings. (1) *Accomplishments* have an intrinsic completion or `culmination' point: an event of this type may occur without reaching this culmination. Example: you may write a letter for 2 hours, though it's not necessarily the case that the letter is written when you stop. (2) *Achievements* are logically `point-like': in an event of this type, whatever occurs previously is generally irrelevant to whether it's felicitous to assert that the event has taken place. Example: `reaching New York City' (after a long trip, say) is an achievement event: it occurs *when* you get there. Suppose you drive for 36 hours toward NYC, but stop in NJ just before crossing the Hudson: then you have *not* reached NYC, even though of course you *have driven to* NYC for quite a long time. This also shows the distinction between achievements (`reaching NYC') and accomplishments (`driving to NYC', which may or may not be completed by getting there). (3) *Activities*: these are occurrences that take place somewhat `uniformly' over time, without a definite completion point. Example: just *writing* is something you can do for a while -- whereas *writing a letter* is an accomplishment, in that it has a definite culmination. (4) *States*: these aren't events at all, in that they denote the holding true of a condition, not the occurrence of a change. In Cyc, this classification is partially reflected by specs of #$Situation and a cluster of collections of event types: #$AccomplishmentType corresponds to (1). #$ProcessType corresponds more or less to (3). States (4) aren't clearly represented in and of themselves: #$StaticSituation comes closest, although most of the verbs Vendler-Aristotle would classify as *stative* are actually represented as relations. (2) is partially captured by another distinction that cuts across the traditional classification of (1), (2) and (3): that between #$DurativeEventType and #$PunctualEventType (for which check out also the #$NoteOnDurativeVsPunctualEvents). The classification of Aktionsarten is essential to characterizing the temporal interpretation of aspect and tense." ;
	a <http://sw.cyc.com/2006/07/27/cyc/Individual> ;
	<http://sw.cyc.com/2006/07/27/cyc/prettyString-Canonical> "Note On The Classification Of Aktionsarten" ;
	<http://sw.cyc.com/2006/07/27/cyc/quotedIsa> <http://sw.cyc.com/2006/07/27/cyc/SharedNote> .

<http://sw.cyc.com/2006/07/27/cyc/SharedNoteOnProcessesVsAccomplishments> <http://www.w3.org/2000/01/rdf-schema#comment> """Intuitively, a process (qua process) is an event that \"goes on\" for a while without necessarily coming to a completion point.  Such events are typically represented in English by using the progressive aspect of a verb (i.e. the result of preceding the verb with 'be' and following it with '-ing'; cf. #$aspectProgressive), as in 
<p>
(1) Alice is (was, will be) writing a proposal.
<p>
The process implicitly referred to in this sentence may or may not result in a completed proposal; the important thing is that Alice is the performer of an event whose end goal, or telos, was the completion of a proposal.  (1) implies, in some (perhaps defeasible) sense, that Alice is capable of completing a proposal, and that there is a good possibility that she will eventually do so, provided nothing out of the ordinary happens.
<p>
An accomplishment (qua accomplishment), on the other hand, is an event that necessarily comes to a completion point.  #$WritingAProposal is an #$AccomplishmentType; accordingly we have:
<p>
(#$relationAllExists #$outputsCreated #$WritingAProposal #$Proposal).
<p>
Thus if we want to say that Alice <i>completed</i> the process of writing a proposal, we can assert:
<pre>
(2) (#$thereExists ?WRITING
      (#$and
        (#$isa ?WRITING #$WritingAProposal)
        (#$performedBy ?WRITING Alice)))
</pre>
On the other hand, we might merely want to assert that Alice was in the process of writing a proposal (say, for a few hours), and didn't necessarily complete the proposal.  In that case, we would assert:
<pre>
(3) (#$thereExists ?WRITING
      (#$and
        (#$isa ?WRITING (#$ProcessFn #$WritingAProposal))
        (#$performedBy ?WRITING Alice)))
</pre>
Every instance of an #$AccomplishmentType is an instance of the corresponding #$ProcessType, but not vice versa.  Thus (2) entails (3), but not vice versa.
<p>
In general, when an event type is potentially ambiguous between an \"accomplishment\" and a \"process\" interpretation, it should be given the accomplishment interpretation.  The process version of the collection can be denoted functionally using #$ProcessFn.""" ;
	a <http://sw.cyc.com/2006/07/27/cyc/Individual> ;
	<http://sw.cyc.com/2006/07/27/cyc/prettyString-Canonical> "Shared Note On Processes Vs Accomplishments" ;
	<http://sw.cyc.com/2006/07/27/cyc/quotedIsa> <http://sw.cyc.com/2006/07/27/cyc/SharedNote> .

<http://sw.cyc.com/2006/07/27/cyc/Accordion> a <http://sw.cyc.com/2006/07/27/cyc/ExistingObjectType> , <http://sw.cyc.com/2006/07/27/cyc/SpatiallyDisjointObjectType> ;
	<http://sw.cyc.com/2006/07/27/cyc/prettyString-Canonical> "accordion" ;
	<http://sw.cyc.com/2006/07/27/cyc/prettyString> "accordions" ;
	<http://www.w3.org/2000/01/rdf-schema#subClassOf> <http://sw.cyc.com/2006/07/27/cyc/MusicalInstrument> , <http://sw.cyc.com/2006/07/27/cyc/PortableObject> , <http://sw.cyc.com/2006/07/27/cyc/Artifact-HumanCreated> ;
	<http://sw.cyc.com/2006/07/27/cyc/quotedIsa> <http://sw.cyc.com/2006/07/27/cyc/StubTerm> .

<http://sw.cyc.com/2006/07/27/cyc/MusicalInstrument> <http://www.w3.org/2000/01/rdf-schema#comment> """A collection of physical devices.  An instance of #$MusicalInstrument is a device that  (in the standard case) is designed to be manipulated by a person to generate music -- that is, s/he successively plays the notes of the music  by manipulating the instrument during the playing.  Possibly the player also supplies by muscle power the force that produces the sound, but possibly it uses another power source (e.g., electricity, or steam).   The music may or may not be of his or her own composition, but the player's actions determine that the notes are produced by the instrument (in the standard sense).  
Note:  If the directive role of the human player is subsumed by the device -- as it is, e.g., by some electronic instruments which are programmable and/or pre-programmed to produce music or musical sounds -- the device loses some of its instrument-like quality, and some automated uses may be abnormal cases of `playing' an instrument.  An older but analogous example is: player pianos.  If the device is pre-programmed so that humans can't direct the music at all, then the device is not a musical instrument (but a musical device) -- for example, music boxes.  Also excluded from #$MusicalInstrument are devices which produce music `at random' (such as wind chimes).  Devices such as radios, tape decks, CD players, which are used to play wholly pre-recorded or otherwise other-controlled music, are also not included in this collection.""" ;
	a <http://sw.cyc.com/2006/07/27/cyc/ExistingObjectType> , <http://sw.cyc.com/2006/07/27/cyc/SpatiallyDisjointObjectType> , <http://sw.cyc.com/2006/07/27/cyc/ArtifactTypeByGenericCategory> , <http://sw.cyc.com/2006/07/27/cyc/QAClarifyingCollectionType> , <http://sw.cyc.com/2006/07/27/cyc/SpecializationsOfPhysicalDevice-Device-Topic> , <http://sw.cyc.com/2006/07/27/cyc/CandidateKBCompletenessNode> ;
	<http://sw.cyc.com/2006/07/27/cyc/prettyString-Canonical> "musical instrument" ;
	<http://sw.cyc.com/2006/07/27/cyc/prettyString> "instruments" , "instrument" , "musical instruments" ;
	<http://www.w3.org/2000/01/rdf-schema#subClassOf> <http://sw.cyc.com/2006/07/27/cyc/Collectible> , <http://sw.cyc.com/2006/07/27/cyc/Device-UserControlled> , <http://sw.cyc.com/2006/07/27/cyc/MusicEquipment> ;
	<http://www.w3.org/2002/07/owl#disjointWith> <http://sw.cyc.com/2006/07/27/cyc/Weapon> , <http://sw.cyc.com/2006/07/27/cyc/ContainerArtifact> , <http://sw.cyc.com/2006/07/27/cyc/ConsumableProduct> , <http://sw.cyc.com/2006/07/27/cyc/HumanlyOccupiedSpatialObject> , <http://sw.cyc.com/2006/07/27/cyc/GameBoard> , <http://sw.cyc.com/2006/07/27/cyc/PlumbingFixture> , <http://sw.cyc.com/2006/07/27/cyc/ControlDevice> , <http://sw.cyc.com/2006/07/27/cyc/MeasuringDevice> .

<http://sw.cyc.com/2006/07/27/cyc/PortableObject> <http://www.w3.org/2000/01/rdf-schema#comment> """A specialization of #$HumanScaleObject (q.v.).  Each instance of #$PortableObject is a tangible object that is not \"fastened down\" and is light enough for an average human (or, more to the point, for its average intended user) to move easily.  
<p>
For many instances of #$PortableObject, portability is important for the fulfillment of their primary functions;  for example, an article of clothing (an instance of #$SomethingToWear),  a hand-guided tool (an instance of #$HandTool), a coin or dollar bill (an instance of #$Currency), or a flashlight (an instance of #$Flashlight) would be pretty useless if they weren't portable.  In other cases, making a device portable, or making a portable version of a device, simply provides a convenience, as with the subcollections #$PortableTelevision and #$PortableStereoSystem.  
<p>
Note that #$Tool is not a subcollection of #$PortableObject, since many tools are heavy and/or stationary.  A borderline example of a #$PortableObject would be a heart/lung machine; although the beneficiary of its primary function is in no position to move it around, the physicians and nurses who also are \"using\" it can and do exactly that.  The same goes for a playpen; the kids in it had better <i>not</i> be able to move it around, but the adults who set it up and put them there can and do move it.   A borderline non-example would be a car; even though its user can make it move around, that is more a controlling action than a transporting action -- i.e., the car is doing the transporting in that case, not the driver.  A borderline example is a cat; even though it moves under its own power, it is light enough for its owner to pick it up and move it around.  A borderline example is a bed or a dresser; though too heavy to lift, its owners can generally move it around (by sliding, disassembling and reassembling, and so on).""" ;
	a <http://sw.cyc.com/2006/07/27/cyc/ExistingObjectType> , <http://sw.cyc.com/2006/07/27/cyc/SpatiallyDisjointObjectType> , <http://sw.cyc.com/2006/07/27/cyc/SpecializationsOfPhysicalDevice-Device-Topic> ;
	<http://sw.cyc.com/2006/07/27/cyc/prettyString-Canonical> "portable object" ;
	<http://sw.cyc.com/2006/07/27/cyc/prettyString> "portability" , "more portability" .

<http://sw.cyc.com/2006/07/27/cyc/Accountant> <http://sw.cyc.com/2006/07/27/cyc/prettyString-Canonical> "accountant" ;
	<http://sw.cyc.com/2006/07/27/cyc/prettyString> "controller" , "controllers" , "Accountants" ;
	<http://www.w3.org/2000/01/rdf-schema#subClassOf> <http://sw.cyc.com/2006/07/27/cyc/Professional> , <http://sw.cyc.com/2006/07/27/cyc/DeskWorker> .

<http://sw.cyc.com/2006/07/27/cyc/Professional> <http://www.w3.org/2000/01/rdf-schema#comment> "The collection of all people who work at a job for which a skill that most adults do not have.  This skill is normally achieved through training, however people who use a \"native\" skill such as an artistic skill, in their work are also considered Professionals.  A person with a #$HighSchoolDiploma, but no additional training, is not expected to be able to be hired to a professional position and perform the job requirements.  The training need not be academic in nature.  One can be a professional child actress, chess player, boxer, or shaman, as well as a professional lawyer, architect, secretary, or politician.  Although factory workers, farm workers, construction workers, etc. develop a level of skill that makes them able to do their jobs far better than a person off the street (professional or not) these positions are not considered professional positions because the skill is developed experientially on the job." ;
	a <http://sw.cyc.com/2006/07/27/cyc/PersonTypeByOccupation> ;
	<http://sw.cyc.com/2006/07/27/cyc/prettyString-Canonical> "Professional" ;
	<http://sw.cyc.com/2006/07/27/cyc/prettyString> "Pro" , "pros" , "professionals" ;
	<http://www.w3.org/2000/01/rdf-schema#subClassOf> <http://sw.cyc.com/2006/07/27/cyc/SkilledWorker> .

<http://sw.cyc.com/2006/07/27/cyc/DeskWorker> <http://www.w3.org/2000/01/rdf-schema#comment> "A subcollection of #$PersonWithOccupation.  #$DeskWorker is a very broad category, consisting of those people who do a significant amount of their work sitting at desks (as opposed, e.g., to those who do physically demanding or outdoor work).  While the sorts of work performed at desks make up too heterogeneous a class for #$DeskWorker itself to be considered an #$PersonTypeByOccupation (q.v.), some of its subcollections do correspond to types of occupations, e.g. #$Administrator, #$ComputerOperator, and #$Secretary." ;
	a <http://sw.cyc.com/2006/07/27/cyc/PersonTypeByOccupation> , <http://sw.cyc.com/2006/07/27/cyc/OccupationsByTypeOfActivity-Professional-Topic> ;
	<http://sw.cyc.com/2006/07/27/cyc/prettyString-Canonical> "office worker" ;
	<http://sw.cyc.com/2006/07/27/cyc/prettyString> "office clerk" , "office clerks" , "desk worker" , "desk workers" , "office workers" ;
	<http://www.w3.org/2000/01/rdf-schema#subClassOf> <http://sw.cyc.com/2006/07/27/cyc/AdultAnimal> , <http://sw.cyc.com/2006/07/27/cyc/PersonWithOccupation> .

<http://sw.cyc.com/2006/07/27/cyc/PersonTypeByActivity> <http://www.w3.org/2000/01/rdf-schema#comment> "A collection of collections.  Each instance of #$PersonTypeByActivity is a collection of #$Persons that classifies people by some kind of activity that they do on a regular basis.  Examples include #$Student, #$Tourist, and #$HornPlayer.  If the differentiating activity is one that is normally done as a career or job, it is preferable to make the collection an instance of the more specific #$PersonTypeByOccupation (q.v.)." ;
	a <http://sw.cyc.com/2006/07/27/cyc/AtemporalNecessarilyEssentialCollectionType> , <http://sw.cyc.com/2006/07/27/cyc/FacetingCollectionType> , <http://sw.cyc.com/2006/07/27/cyc/SecondOrderCollection> , <http://sw.cyc.com/2006/07/27/cyc/GeneralProfessionConstants-Professional-Topic> ;
	<http://sw.cyc.com/2006/07/27/cyc/prettyString-Canonical> "type of person classified by activity" ;
	<http://sw.cyc.com/2006/07/27/cyc/prettyString> "type of person by activity" , "types of person by activity" , "types of person classified by activity" ;
	<http://www.w3.org/2000/01/rdf-schema#subClassOf> <http://sw.cyc.com/2006/07/27/cyc/ExistingObjectType> , <http://sw.cyc.com/2006/07/27/cyc/KEClarifyingCollectionType> , <http://sw.cyc.com/2006/07/27/cyc/FacetInstanceCollection> , <http://sw.cyc.com/2006/07/27/cyc/ExistenceDependentNonInitialIntermittentCollection> ;
	<http://sw.cyc.com/2006/07/27/cyc/sharedNotes> <http://sw.cyc.com/2006/07/27/cyc/SharedNoteOnGenlsRelationsBetweenFacetingCollectionTypes> ;
	<http://www.w3.org/2002/07/owl#disjointWith> <http://sw.cyc.com/2006/07/27/cyc/OrganizationTypeByActivityType> , <http://sw.cyc.com/2006/07/27/cyc/PersonTypeByRegionalAffiliation> , <http://sw.cyc.com/2006/07/27/cyc/PharmacyProductType> , <http://sw.cyc.com/2006/07/27/cyc/OrganismPartType> , <http://sw.cyc.com/2006/07/27/cyc/RoadVehicleType> , <http://sw.cyc.com/2006/07/27/cyc/GeopoliticalEntityTypeByBasicCategory> , <http://sw.cyc.com/2006/07/27/cyc/HumanTypeByClothingSize> , <http://sw.cyc.com/2006/07/27/cyc/MoleculeTypeByChemicalCompoundType> ;
	<http://sw.cyc.com/2006/07/27/cyc/typeGenls> <http://sw.cyc.com/2006/07/27/cyc/Person> ;
	<http://sw.cyc.com/2006/07/27/cyc/requiredArg2Pred> <http://sw.cyc.com/2006/07/27/cyc/prototypicalActivityTypeOfPersonType> .

<http://sw.cyc.com/2006/07/27/cyc/accountants> <http://www.w3.org/2000/01/rdf-schema#comment> "The people who perform the accounting functions for this organization" ;
	a <http://www.w3.org/2002/07/owl#TransitiveProperty> , <http://sw.cyc.com/2006/07/27/cyc/CoexistingObjectsPredicate> , <http://www.w3.org/2002/07/owl#SymmetricProperty> , <http://sw.cyc.com/2006/07/27/cyc/AntiSymmetricBinaryPredicate> , <http://sw.cyc.com/2006/07/27/cyc/AsymmetricBinaryPredicate> , <http://sw.cyc.com/2006/07/27/cyc/ReflexiveBinaryPredicate> , <http://sw.cyc.com/2006/07/27/cyc/IrreflexiveBinaryPredicate> , <http://sw.cyc.com/2006/07/27/cyc/RelationalNounSlot> , <http://sw.cyc.com/2006/07/27/cyc/CotemporalPredicate> ;
	<http://sw.cyc.com/2006/07/27/cyc/prettyString-Canonical> "Accountants" ;
	<http://www.w3.org/2000/01/rdf-schema#domain> <http://sw.cyc.com/2006/07/27/cyc/Agent-Generic> ;
	<http://sw.cyc.com/2006/07/27/cyc/arity> "2"^^<http://www.w3.org/2001/XMLSchema#long> ;
	<http://www.w3.org/2000/01/rdf-schema#range> <http://sw.cyc.com/2006/07/27/cyc/Accountant> ;
	<http://www.w3.org/2000/01/rdf-schema#subPropertyOf> <http://sw.cyc.com/2006/07/27/cyc/receivesServicesFrom> ;
	<http://sw.cyc.com/2006/07/27/cyc/arg2Format> <http://sw.cyc.com/2006/07/27/cyc/SetTheFormat> .

<http://sw.cyc.com/2006/07/27/cyc/receivesServicesFrom> <http://www.w3.org/2000/01/rdf-schema#comment> "This predicate relates potential service recipients to service providers that are bound to provide services of some type to that agent.  The first argument place should be the potential recipient of service and the second argument place should contain the potential service provider.  The relationship holds while the agreement to provide the service is in place, not just while the service is being provided.  This agreement need not be a formal agreement but it should involve the service provider in a task for which he, she, it or the service provider's controller is paid, although not necessarily by the service recipient.  Hence, #$mother is not a specpred (#$specs) of this predicate but the relationship between a client and social worker or between parishioner and priest might be even if the client or parishioner does not pay for the service.  If a company, Company001, puts a lawyer, Lawyer001, on retainer, then it is true that (#$receivesServicesFrom Company001 Lawyer001) even before the lawyer has provided any services.  Usually it is preferable to use one of the specializations of this predicate. See, for instance, #$accountants, #$attorneys or #$hasWorkers. #$receivesServicesFrom is more general than #$hasWorkers as it can describe the relationship between a person and her dentist or priest and the relationship between an organization that may occassionally receive a service from an agent, e.g. a subcontractor.  If a business, Business001 has a certain accountancy firm, AccountantsRUs001, perform occasional bookkeeping work, it is not true throughout the year that (#$hasWorkers BusinessOO1 AccountsRUs001) but it may be true throughout the year that (#$receivesServicesFrom Business001 AccountantsRUs001)." ;
	a <http://sw.cyc.com/2006/07/27/cyc/CoexistingObjectsPredicate> ;
	<http://sw.cyc.com/2006/07/27/cyc/prettyString-Canonical> "recipient of services" ;
	<http://sw.cyc.com/2006/07/27/cyc/prettyString> "recipients of services" ;
	<http://www.w3.org/2000/01/rdf-schema#domain> <http://sw.cyc.com/2006/07/27/cyc/Agent-Generic> ;
	<http://sw.cyc.com/2006/07/27/cyc/arity> "2"^^<http://www.w3.org/2001/XMLSchema#long> ;
	<http://www.w3.org/2000/01/rdf-schema#range> <http://sw.cyc.com/2006/07/27/cyc/Agent-Generic> ;
	<http://www.w3.org/2000/01/rdf-schema#subPropertyOf> <http://sw.cyc.com/2006/07/27/cyc/temporallyCoexist> ;
	<http://sw.cyc.com/2006/07/27/cyc/arg1Format> <http://sw.cyc.com/2006/07/27/cyc/SetTheFormat> ;
	<http://sw.cyc.com/2006/07/27/cyc/arg2Format> <http://sw.cyc.com/2006/07/27/cyc/SetTheFormat> ;
	<http://sw.cyc.com/2006/07/27/cyc/negationInverse> <http://sw.cyc.com/2006/07/27/cyc/inactiveWRT> .

<http://sw.cyc.com/2006/07/27/cyc/CotemporalPredicate> <http://www.w3.org/2000/01/rdf-schema#comment> """A specialization of #$TemporalExistencePredicate (q.v.).  This is the collection of predicates that are used to make statements that imply the current temporal existence of any of their arguments that happen to be temporal things.  
<p>
More precisely, a predicate <code>PRED</code> is an instance of #$CotemporalPredicate if and only if the following two conditions hold.  (i) If a sentence of the form <code>(PRED ARG<sub>1</sub> ... ARG<sub>N</sub>)</code> is true at a given time <code>T</code>, then any <code>ARG<sub>i</sub></code> (<code>1<=i<=N</code>) that is a #$TemporalThing temporally-subsumes <code>T</code> (see #$temporallySubsumes).  (ii) <code>PRED</code> holds of at least one sequence of arguments that includes at least one instance of #$TemporalThing.
<p>
(Condition (ii) above prevents predicates that never hold of temporal things from trivially qualifying as #$CotemporalPredicates. Its practical import is that at least one of <code>PRED</code>'s argument-places must not be type-constrained (see #$argIsa) to any collection that is #$disjointWith #$TemporalThing.)
<p>
For example, #$owns is a #$CotemporalPredicate.  So the sentence <code>(#$owns Nick Spot)</code> with time-index (see #$mtTimeIndex) <code>(#$YearFn 1992)</code> implies (given that Nick and Spot are temporal things) that Nick and Spot were alive throughout 1992.  In contrast, the predicate #$awareOf is <i>not</i> a #$CotemporalPredicate.  The sentence <code>(#$awareOf Fred #$GeorgeWashington)</code>, with the same time-index as above, does <i>not</i> imply <code>(#$temporallySubsumes #$GeorgeWashington (#$YearFn 1992))</code>.
<p>
See also the specialization #$CoexistingObjectsPredicate, the collection of cotemporal predicates <i>all</i> of whose argument-places are constrained (at least) to #$TemporalThing.  And see the predicate #$contemporaryInArg.""" ;
	a <http://sw.cyc.com/2006/07/27/cyc/KEClarifyingCollectionType> , <http://sw.cyc.com/2006/07/27/cyc/PredicateType> , <http://sw.cyc.com/2006/07/27/cyc/Time-RelatedPredicateTypes-Time-Topic> ;
	<http://sw.cyc.com/2006/07/27/cyc/prettyString-Canonical> "cotemporal predicate" ;
	<http://sw.cyc.com/2006/07/27/cyc/prettyString> "cotemporal predicates" ;
	<http://www.w3.org/2000/01/rdf-schema#subClassOf> <http://sw.cyc.com/2006/07/27/cyc/TemporalExistencePredicate> , <http://sw.cyc.com/2006/07/27/cyc/ObjectPredicate> , <http://sw.cyc.com/2006/07/27/cyc/CoexistenceRelation> , <http://sw.cyc.com/2006/07/27/cyc/SituationPredicate> .

<http://sw.cyc.com/2006/07/27/cyc/accountBalance> <http://www.w3.org/2000/01/rdf-schema#comment> "The predicate #$accountBalance is used to indicate the balance of a particular account.  (#$accountBalance ACCT BAL) means that the #$FinancialAccount ACCT has the balance BAL; BAL is the amount of #$MonetaryValue either owed by, or available to, the #$accountHolder (depending upon the type of account)." ;
	a <http://sw.cyc.com/2006/07/27/cyc/TemporalExistencePredicate> , <http://sw.cyc.com/2006/07/27/cyc/MeasurableQuantitySlot> , <http://sw.cyc.com/2006/07/27/cyc/RelationalNounSlot> , <http://sw.cyc.com/2006/07/27/cyc/CommercialOrganizationsAndAccounts-Financial-Topic> ;
	<http://sw.cyc.com/2006/07/27/cyc/prettyString-Canonical> "account balance" .

<http://sw.cyc.com/2006/07/27/cyc/accountForProgram> <http://sw.cyc.com/2006/07/27/cyc/prettyString-Canonical> "Account For Program" ;
	<http://www.w3.org/2000/01/rdf-schema#domain> <http://sw.cyc.com/2006/07/27/cyc/ApplicationAccount> ;
	<http://sw.cyc.com/2006/07/27/cyc/arity> "2"^^<http://www.w3.org/2001/XMLSchema#long> ;
	<http://www.w3.org/2000/01/rdf-schema#range> <http://sw.cyc.com/2006/07/27/cyc/ComputerProgram-CW> .

<http://sw.cyc.com/2006/07/27/cyc/ApplicationAccount> <http://www.w3.org/2000/01/rdf-schema#comment> "A person with an instance of #$ApplicationAccount is able to access a set of files associated with a computer application program.  The most notable subcollection of #$ApplicationAccount is #$FTPAccount, but there are many others." ;
	a <http://sw.cyc.com/2006/07/27/cyc/ObjectType> ;
	<http://sw.cyc.com/2006/07/27/cyc/prettyString-Canonical> "application account" ;
	<http://www.w3.org/2000/01/rdf-schema#subClassOf> <http://sw.cyc.com/2006/07/27/cyc/Artifact-Intangible> .

<http://sw.cyc.com/2006/07/27/cyc/accountForProgramCopy> <http://www.w3.org/2000/01/rdf-schema#comment> "(#$accountForProgramCopy ACCOUNT COPY) means that ACCOUNT is an account for COPY; that is, it is possible to log in to a running process of COPY as ACCOUNT." ;
	a <http://www.w3.org/2000/01/rdf-schema#Property> ;
	<http://sw.cyc.com/2006/07/27/cyc/prettyString-Canonical> "Account For Program Copy" ;
	<http://www.w3.org/2000/01/rdf-schema#domain> <http://sw.cyc.com/2006/07/27/cyc/ApplicationAccount> ;
	<http://sw.cyc.com/2006/07/27/cyc/arity> "2"^^<http://www.w3.org/2001/XMLSchema#long> ;
	<http://www.w3.org/2000/01/rdf-schema#range> <http://sw.cyc.com/2006/07/27/cyc/ComputerProgramCopy> .

<http://sw.cyc.com/2006/07/27/cyc/ComputerProgramCopy> <http://www.w3.org/2000/01/rdf-schema#comment> "A collection of #$InformationBearingThings which are #$programCopies of a #$ComputerProgram-CW. Examples: A bank of memory registers, a set of hard disk sectors, a stack of punch cards, a printout of #$ComputerCode, a satellite transmission. A #$ComputerProgramCopy might not have the exact same #$ComputerCode as  other #$programCopies of the same #$ComputerProgram-CW, and it might not even have the exact same algorithms, but the functionality must be about the same." ;
	a <http://sw.cyc.com/2006/07/27/cyc/SpatiallyDisjointObjectType> , <http://sw.cyc.com/2006/07/27/cyc/TemporalStuffType> ;
	<http://sw.cyc.com/2006/07/27/cyc/prettyString-Canonical> "copy of a computer program" ;
	<http://sw.cyc.com/2006/07/27/cyc/prettyString> "copies of a computer program" ;
	<http://www.w3.org/2000/01/rdf-schema#subClassOf> <http://sw.cyc.com/2006/07/27/cyc/Artifact-Generic> , <http://sw.cyc.com/2006/07/27/cyc/ComputerCodeCopy> ;
	<http://sw.cyc.com/2006/07/27/cyc/facets-Generic> <http://sw.cyc.com/2006/07/27/cyc/SoftwareTypeByFlaw> .

<http://sw.cyc.com/2006/07/27/cyc/accountForSystem> <http://www.w3.org/2000/01/rdf-schema#comment> "A predicate relating instances of #$ComputerAccount with instances of #$AccountSystem.  (#$accountForSystem ACCOUNT SYSTEM) means that ACCOUNT is an account in the account system SYSTEM (which may  allow logging in to one individual computer or to many)." ;
	a <http://www.w3.org/2000/01/rdf-schema#Property> ;
	<http://sw.cyc.com/2006/07/27/cyc/prettyString-Canonical> "Account For System" ;
	<http://www.w3.org/2000/01/rdf-schema#domain> <http://sw.cyc.com/2006/07/27/cyc/ComputerAccount> ;
	<http://sw.cyc.com/2006/07/27/cyc/arity> "2"^^<http://www.w3.org/2001/XMLSchema#long> ;
	<http://www.w3.org/2000/01/rdf-schema#range> <http://sw.cyc.com/2006/07/27/cyc/AccountSystem> .

<http://sw.cyc.com/2006/07/27/cyc/AccountSystem> <http://www.w3.org/2000/01/rdf-schema#comment> "#$AccountSystem is a specialization of #$ComputerNetwork.  Each instance of #$AccountSystem is a computational system which is such that users must log on to it to make use of it.  Instances  of #$AccountSystem can consist of one or many nodes (i.e. computers).  Each node in an #$AccountSystem shares a given set of accounts with any other nodes in that #$AccountSystem (such that someone with an account can log in at any node).  See also #$nodeInAccountSystem, #$accountForSystem, and #$ComputerAccount." ;
	a <http://sw.cyc.com/2006/07/27/cyc/ExistingObjectType> , <http://sw.cyc.com/2006/07/27/cyc/SpatiallyDisjointObjectType> ;
	<http://sw.cyc.com/2006/07/27/cyc/prettyString-Canonical> "account system" ;
	<http://sw.cyc.com/2006/07/27/cyc/prettyString> "account systems" ;
	<http://www.w3.org/2000/01/rdf-schema#subClassOf> <http://sw.cyc.com/2006/07/27/cyc/ComputerNetwork> .

<http://sw.cyc.com/2006/07/27/cyc/accountFullName> <http://www.w3.org/2000/01/rdf-schema#comment> "A predicate that relates computer accounts to the full names listed for them in the 'etc/passwd' file. (#$accountFullName ACCOUNT FULL-NAME) means that the #$ComputerAccount ACCOUNT's full name is FULL-NAME. For the account's 'username', see #$accountName." ;
	a <http://www.w3.org/2000/01/rdf-schema#Property> ;
	<http://sw.cyc.com/2006/07/27/cyc/prettyString-Canonical> "Account Full Name" ;
	<http://www.w3.org/2000/01/rdf-schema#domain> <http://sw.cyc.com/2006/07/27/cyc/ComputerAccount> ;
	<http://sw.cyc.com/2006/07/27/cyc/arity> "2"^^<http://www.w3.org/2001/XMLSchema#long> ;
	<http://www.w3.org/2000/01/rdf-schema#range> <http://sw.cyc.com/2006/07/27/cyc/CharacterString> ;
	<http://www.w3.org/2000/01/rdf-schema#subPropertyOf> <http://sw.cyc.com/2006/07/27/cyc/identificationStrings> ;
	<http://sw.cyc.com/2006/07/27/cyc/arg2Format> <http://sw.cyc.com/2006/07/27/cyc/singleEntryFormatInArgs> .

<http://sw.cyc.com/2006/07/27/cyc/identificationStrings> <http://www.w3.org/2000/01/rdf-schema#comment> "A #$BinaryPredicate that relates instances of #$Thing to instances of #$IDString.  <code>(#$identificationStrings THING STRING)</code> means that <code>STRING</code> is used somehow to identify <code>THING</code>. Its many notable specializations include #$constantID, #$taxIDNumber and #$computerIP. <code>STRING</code> may be a unique identifier for <code>THING</code> or it may be possible that more than one thing is identified by <code>STRING</code>." ;
	a <http://www.w3.org/2000/01/rdf-schema#Property> , <http://sw.cyc.com/2006/07/27/cyc/FunctionalPredicate> , <http://sw.cyc.com/2006/07/27/cyc/ObjectPredicate> ;
	<http://sw.cyc.com/2006/07/27/cyc/prettyString-Canonical> "Identification Strings" ;
	<http://www.w3.org/2000/01/rdf-schema#domain> <http://www.w3.org/2002/07/owl#Thing> ;
	<http://sw.cyc.com/2006/07/27/cyc/arity> "2"^^<http://www.w3.org/2001/XMLSchema#long> ;
	<http://www.w3.org/2000/01/rdf-schema#range> <http://sw.cyc.com/2006/07/27/cyc/IDString> ;
	<http://sw.cyc.com/2006/07/27/cyc/arg2Format> <http://sw.cyc.com/2006/07/27/cyc/SetTheFormat> ;
	<http://sw.cyc.com/2006/07/27/cyc/genlInverse> <http://sw.cyc.com/2006/07/27/cyc/signifies> .

<http://sw.cyc.com/2006/07/27/cyc/LegalAgreement> <http://www.w3.org/2000/01/rdf-schema#comment> "An instance of #$ObjectType, and a specialization of #$Agreement.  Each instance of #$LegalAgreement is an agreement which has a legal status; that is, it is recognized as a valid agreement by some government.  Notable specializations of #$LegalAgreement include #$SalesContract, #$Visa-Permit, and #$Account." ;
	a <http://sw.cyc.com/2006/07/27/cyc/ObjectType> , <http://sw.cyc.com/2006/07/27/cyc/TemporalStuffType> , <http://sw.cyc.com/2006/07/27/cyc/SomeSampleKindsOfAgreements-Agreement-Topic> ;
	<http://sw.cyc.com/2006/07/27/cyc/prettyString-Canonical> "legal agreement" ;
	<http://sw.cyc.com/2006/07/27/cyc/prettyString> "legal agreements" ;
	<http://www.w3.org/2000/01/rdf-schema#subClassOf> <http://sw.cyc.com/2006/07/27/cyc/Obligation> , <http://sw.cyc.com/2006/07/27/cyc/Agreement> , <http://sw.cyc.com/2006/07/27/cyc/BusinessRelatedDocumentOrAgreement> .

<http://sw.cyc.com/2006/07/27/cyc/AuthorizedAgreement> <http://www.w3.org/2000/01/rdf-schema#comment> "A specialization of #$Agreement.  Each instance of #$Agreement is a generic agreement that is authorized by one of the agreeing parties (typically by the issuer of the document embodying the agreement).  #$AuthorizedAgreements are generic in the sense that their authorizing agents are party to many similar agreements; for that reason, an #$AuthorizedAgreement is typically given a unique identification number.  Notable positive examples include bank accounts, driver's licenses, and stock certificates." ;
	a <http://sw.cyc.com/2006/07/27/cyc/ObjectType> , <http://sw.cyc.com/2006/07/27/cyc/CommercialActivities-Financial-Topic> ;
	<http://sw.cyc.com/2006/07/27/cyc/prettyString-Canonical> "authorized agreement" ;
	<http://sw.cyc.com/2006/07/27/cyc/prettyString> "authorized agreements" ;
	<http://www.w3.org/2000/01/rdf-schema#subClassOf> <http://sw.cyc.com/2006/07/27/cyc/Agreement> .

<http://sw.cyc.com/2006/07/27/cyc/AccountGroupFn> <http://www.w3.org/2000/01/rdf-schema#comment> "(#$AccountGroupFn ACCOUNT_SYSTEM ID) denotes the #$UserAccountGroup on ACCOUNT_SYSTEM (#$groupForAccountSystem, q.v.) which is uniquely identified by the number ID.  For example, (#$AccountGroupFn #$CycorpLANAccountSystem-Unix \"3\") denotes group no. 3 on the Cycorp UNIX LAN." .

<http://sw.cyc.com/2006/07/27/cyc/FinanceDepartment> <http://www.w3.org/2000/01/rdf-schema#comment> "A specialization of #$Department. Each instance of this collection is a sub-organization of a business, government, or academic organization which deals somehow with the organization's finances or cash-flow. Notable specializations of this collection include #$BudgetDepartment,  #$PayrollDepartment and #$AccountingDepartment." ;
	a <http://sw.cyc.com/2006/07/27/cyc/DepartmentTypeByFunction> ;
	<http://sw.cyc.com/2006/07/27/cyc/prettyString-Canonical> "finance department" ;
	<http://sw.cyc.com/2006/07/27/cyc/prettyString> "finance departments" ;
	<http://www.w3.org/2000/01/rdf-schema#subClassOf> <http://sw.cyc.com/2006/07/27/cyc/Department> ;
	<http://sw.cyc.com/2006/07/27/cyc/quotedIsa> <http://sw.cyc.com/2006/07/27/cyc/TerrorismOntologyConstant> ;
	<http://sw.cyc.com/2006/07/27/cyc/siblingDisjointExceptions> <http://sw.cyc.com/2006/07/27/cyc/HumanResourcesDepartment> .

<http://sw.cyc.com/2006/07/27/cyc/AccountingFirm> <http://www.w3.org/2000/01/rdf-schema#comment> "Commercial organizations which perform financial accounting services for their clients/customers." ;
	a <http://sw.cyc.com/2006/07/27/cyc/ExistingObjectType> ;
	<http://sw.cyc.com/2006/07/27/cyc/prettyString-Canonical> "accounting firm" ;
	<http://sw.cyc.com/2006/07/27/cyc/prettyString> "accounting firms" ;
	<http://www.w3.org/2000/01/rdf-schema#subClassOf> <http://sw.cyc.com/2006/07/27/cyc/FinancialOrganization> , <http://sw.cyc.com/2006/07/27/cyc/CommercialServiceOrganization> , <http://sw.cyc.com/2006/07/27/cyc/ProfessionalServiceOrganization> , <http://sw.cyc.com/2006/07/27/cyc/PrivateSectorOrganization> .

<http://sw.cyc.com/2006/07/27/cyc/FinancialOrganization> <http://www.w3.org/2000/01/rdf-schema#comment> "#$FinancialOrganization is a specialization of #$Organization.  Each instance of #$FinancialOrganization is primarily or significantly engaged in the #$FinancialIndustry or whose activities focus on that industry.  Instances of both #$CommercialServiceOrganizations (e.g., banks and brokerage houses) and #$NonProfitOrganizations (e.g., #$InternationalMonetaryFund) may be instances of #$FinancialOrganization.  Specializations of #$FinancialOrganization include #$BankOrganization, #$FinancialExchange, and #$InvestmentOrganization." ;
	a <http://sw.cyc.com/2006/07/27/cyc/OrganizationTypeByActivityType> , <http://sw.cyc.com/2006/07/27/cyc/CommercialOrganizationsAndAccounts-Financial-Topic> , <http://sw.cyc.com/2006/07/27/cyc/Financial-Topic> , <http://sw.cyc.com/2006/07/27/cyc/OrganizationsByFunction-Organization-Topic> , <http://sw.cyc.com/2006/07/27/cyc/OrganizationTypeByIndustry> ;
	<http://sw.cyc.com/2006/07/27/cyc/prettyString-Canonical> "financial organization" ;
	<http://sw.cyc.com/2006/07/27/cyc/prettyString> "financial organisation" , "financial organisations" , "financial organizations" ;
	<http://www.w3.org/2000/01/rdf-schema#subClassOf> <http://sw.cyc.com/2006/07/27/cyc/Organization> , <http://sw.cyc.com/2006/07/27/cyc/Agent-NonGeographical> ;
	<http://sw.cyc.com/2006/07/27/cyc/quotedIsa> <http://sw.cyc.com/2006/07/27/cyc/TerrorismOntologyConstant> ;
	<http://www.w3.org/2002/07/owl#disjointWith> <http://sw.cyc.com/2006/07/27/cyc/TransportationOrganization> , <http://sw.cyc.com/2006/07/27/cyc/TravelOrganization> , <http://sw.cyc.com/2006/07/27/cyc/Beauty-CosmeticsOrganization> , <http://sw.cyc.com/2006/07/27/cyc/Secretariat> , <http://sw.cyc.com/2006/07/27/cyc/JudicialOrganization> , <http://sw.cyc.com/2006/07/27/cyc/AnimalOrganization> , <http://sw.cyc.com/2006/07/27/cyc/ConstructionRepairOrMaintenanceOrganization> , <http://sw.cyc.com/2006/07/27/cyc/WorkersOrganization> , <http://sw.cyc.com/2006/07/27/cyc/StateOrProvinceWideOrganization> .

<http://sw.cyc.com/2006/07/27/cyc/CommercialServiceOrganization> <http://www.w3.org/2000/01/rdf-schema#comment> "A specialization of #$CommercialOrganization.  Each instance of #$CommercialServiceOrganization is a commercial organization which sells some service(s), rather than tangible goods, as its main product.  Some tangible goods may accompany or supplement the main service sold, but only as side products; for example, some instances of #$HairSalon sell hair care products." ;
	a <http://sw.cyc.com/2006/07/27/cyc/OrganizationTypeByActivityType> , <http://sw.cyc.com/2006/07/27/cyc/CommercialOrganizationsAndAccounts-Financial-Topic> , <http://sw.cyc.com/2006/07/27/cyc/OrganizationsByFunction-Organization-Topic> ;
	<http://sw.cyc.com/2006/07/27/cyc/prettyString-Canonical> "service company" ;
	<http://sw.cyc.com/2006/07/27/cyc/prettyString> "commercial service" , "commercial services" , "service companies" ;
	<http://www.w3.org/2000/01/rdf-schema#subClassOf> <http://sw.cyc.com/2006/07/27/cyc/CommercialOrganization> , <http://sw.cyc.com/2006/07/27/cyc/ServiceOrganization> , <http://sw.cyc.com/2006/07/27/cyc/SalesOrServiceRelatedCompany> ;
	<http://sw.cyc.com/2006/07/27/cyc/quotedIsa> <http://sw.cyc.com/2006/07/27/cyc/TerrorismOntologyConstant> .

<http://sw.cyc.com/2006/07/27/cyc/accountLoggedInOn> <http://www.w3.org/2000/01/rdf-schema#range> <http://sw.cyc.com/2006/07/27/cyc/AccountSystem> .

<http://sw.cyc.com/2006/07/27/cyc/AccountManager> a <http://sw.cyc.com/2006/07/27/cyc/PersonTypeByPositionInOrg> ;
	<http://sw.cyc.com/2006/07/27/cyc/prettyString-Canonical> "account manager" ;
	<http://sw.cyc.com/2006/07/27/cyc/prettyString> "account managers" ;
	<http://www.w3.org/2000/01/rdf-schema#subClassOf> <http://sw.cyc.com/2006/07/27/cyc/Administrator> , <http://sw.cyc.com/2006/07/27/cyc/Manager> , <http://sw.cyc.com/2006/07/27/cyc/BusinessPerson> .

<http://sw.cyc.com/2006/07/27/cyc/Administrator> <http://www.w3.org/2000/01/rdf-schema#comment> "A specialization of #$AdministrativeStaffPerson.  Each instance of #$Administrator is an employee of an organization who is responsible for managing its organizational affairs.  Instances of #$Administrator may or may not also be required to manage people.  If so, then they are also #$Managers (q.v.)." ;
	a <http://sw.cyc.com/2006/07/27/cyc/ExistingObjectType> , <http://www.w3.org/2002/07/owl#Class> , <http://sw.cyc.com/2006/07/27/cyc/FirstOrderCollection> , <http://sw.cyc.com/2006/07/27/cyc/OccupationsByTypeOfActivity-Professional-Topic> , <http://sw.cyc.com/2006/07/27/cyc/SetOrCollection> , <http://sw.cyc.com/2006/07/27/cyc/PersonTypeByPositionInOrg> ;
	<http://sw.cyc.com/2006/07/27/cyc/prettyString-Canonical> "administrator" ;
	<http://sw.cyc.com/2006/07/27/cyc/prettyString> "layman that has been Has Administrators of an institutes" , "laymen that has been Has Administrators of an institutes" , "persons that has been Has Administrators of an institutes" , "mortals that has been Has Administrators of an institutes" , "humaner that has been Has Administrators of an institutes" , "humanest that has been Has Administrators of an institutes" , "human thing that has been Has Administrators of an institutes" , "person that is Has Administrators of an institutes" , "human that is Has Administrators of an institutes" , "people that is Has Administrators of an institutes" , "mortal that is Has Administrators of an institutes" , "layman that is Has Administrators of an institutes" , "laymen that is Has Administrators of an institutes" , "persons that is Has Administrators of an institutes" , "mortals that is Has Administrators of an institutes" , "humaner that is Has Administrators of an institutes" , "humanest that is Has Administrators of an institutes" , "human thing that is Has Administrators of an institutes" , "person that has been Has Administrators of an institution" , "human that has been Has Administrators of an institution" , "people that has been Has Administrators of an institution" , "mortal that has been Has Administrators of an institution" , "layman that has been Has Administrators of an institution" , "laymen that has been Has Administrators of an institution" , "persons that has been Has Administrators of an institution" , "mortals that has been Has Administrators of an institution" , "humaner that has been Has Administrators of an institution" , "humanest that has been Has Administrators of an institution" , "human thing that has been Has Administrators of an institution" , "person that is Has Administrators of an institution" , "human that is Has Administrators of an institution" , "people that is Has Administrators of an institution" , "mortal that is Has Administrators of an institution" , "layman that is Has Administrators of an institution" , "laymen that is Has Administrators of an institution" .

<http://sw.cyc.com/2006/07/27/cyc/AccountPending> <http://sw.cyc.com/2006/07/27/cyc/prettyString> "account pendingest" ;
	<http://www.w3.org/2000/01/rdf-schema#subClassOf> <http://sw.cyc.com/2006/07/27/cyc/Account> .

<http://sw.cyc.com/2006/07/27/cyc/accountRepresentatives> <http://www.w3.org/2000/01/rdf-schema#comment> "Entries will the person who is the account representative for the organization" ;
	a <http://sw.cyc.com/2006/07/27/cyc/CoexistingObjectsPredicate> ;
	<http://sw.cyc.com/2006/07/27/cyc/prettyString-Canonical> "Account Representatives" ;
	<http://www.w3.org/2000/01/rdf-schema#domain> <http://sw.cyc.com/2006/07/27/cyc/Organization> ;
	<http://sw.cyc.com/2006/07/27/cyc/arity> "2"^^<http://www.w3.org/2001/XMLSchema#long> ;
	<http://www.w3.org/2000/01/rdf-schema#range> <http://sw.cyc.com/2006/07/27/cyc/Person> ;
	<http://www.w3.org/2000/01/rdf-schema#subPropertyOf> <http://sw.cyc.com/2006/07/27/cyc/temporallyCoexist> , <http://sw.cyc.com/2006/07/27/cyc/personRepresentingAgent> ;
	<http://sw.cyc.com/2006/07/27/cyc/arg2Format> <http://sw.cyc.com/2006/07/27/cyc/SetTheFormat> .

<http://sw.cyc.com/2006/07/27/cyc/personRepresentingAgent> a <http://www.w3.org/2002/07/owl#TransitiveProperty> , <http://sw.cyc.com/2006/07/27/cyc/CoexistingObjectsPredicate> , <http://www.w3.org/2002/07/owl#SymmetricProperty> , <http://sw.cyc.com/2006/07/27/cyc/AntiSymmetricBinaryPredicate> , <http://sw.cyc.com/2006/07/27/cyc/AsymmetricBinaryPredicate> , <http://sw.cyc.com/2006/07/27/cyc/ReflexiveBinaryPredicate> , <http://sw.cyc.com/2006/07/27/cyc/IrreflexiveBinaryPredicate> ;
	<http://sw.cyc.com/2006/07/27/cyc/prettyString-Canonical> "Person Representing Agent" ;
	<http://www.w3.org/2000/01/rdf-schema#domain> <http://sw.cyc.com/2006/07/27/cyc/IntelligentAgent> ;
	<http://sw.cyc.com/2006/07/27/cyc/arity> "2"^^<http://www.w3.org/2001/XMLSchema#long> ;
	<http://www.w3.org/2000/01/rdf-schema#range> <http://sw.cyc.com/2006/07/27/cyc/Person> ;
	<http://www.w3.org/2000/01/rdf-schema#subPropertyOf> <http://sw.cyc.com/2006/07/27/cyc/receivesServicesFrom> ;
	<http://sw.cyc.com/2006/07/27/cyc/arg2Format> <http://sw.cyc.com/2006/07/27/cyc/SetTheFormat> .

<http://sw.cyc.com/2006/07/27/cyc/requiredArg1Pred> <http://www.w3.org/2000/01/rdf-schema#comment> """A #$MetaPredicate for stating that every instance of a given collection is related to some thing or things by a given predicate.  <code>(#$requiredArg1Pred COL PRED)</code> means that for every  instance <code>INST</code> of <code>COL</code>, there exists some sequence <code>ARGS</code> such that <code>(PRED INST . ARGS)</code> holds.  For example, (#$requiredArg1Pred #$Organization #$hasMembers) means that every organization has at least one member.  
<p>
See also #$requiredArg2Pred and #$requiredArg3Pred.""" ;
	a <http://www.w3.org/2000/01/rdf-schema#Property> , <http://sw.cyc.com/2006/07/27/cyc/RuleMacroPredicate> , <http://sw.cyc.com/2006/07/27/cyc/NonAbduciblePredicate> , <http://sw.cyc.com/2006/07/27/cyc/MetaPredicate> , <http://sw.cyc.com/2006/07/27/cyc/RuleMacro-Topic> ;
	<http://sw.cyc.com/2006/07/27/cyc/prettyString-Canonical> "Required Arg 1 Pred" ;
	<http://sw.cyc.com/2006/07/27/cyc/quotedIsa> <http://sw.cyc.com/2006/07/27/cyc/OpenCycDefinitionalPredicate> ;
	<http://www.w3.org/2000/01/rdf-schema#domain> <http://www.w3.org/2002/07/owl#Class> ;
	<http://sw.cyc.com/2006/07/27/cyc/arity> "2"^^<http://www.w3.org/2001/XMLSchema#long> ;
	<http://www.w3.org/2000/01/rdf-schema#range> <http://sw.cyc.com/2006/07/27/cyc/Predicate> ;
	<http://www.w3.org/2000/01/rdf-schema#subPropertyOf> <http://sw.cyc.com/2006/07/27/cyc/requires-Underspecified> ;
	<http://sw.cyc.com/2006/07/27/cyc/arg1Genl> <http://www.w3.org/2002/07/owl#Thing> ;
	<http://sw.cyc.com/2006/07/27/cyc/arg1Format> <http://sw.cyc.com/2006/07/27/cyc/SetTheFormat> ;
	<http://sw.cyc.com/2006/07/27/cyc/arg2Format> <http://sw.cyc.com/2006/07/27/cyc/SetTheFormat> .

<http://sw.cyc.com/2006/07/27/cyc/accountStatus> <http://www.w3.org/2000/01/rdf-schema#comment> "The predicate #$accountStatus indicates whether a particular account is paid up, overdue, delinquent, etc.  (#$accountStatus ACCT STATUS) means that the #$Account ACCT has the attribute STATUS (see also #$AccountStatusAttribute)." ;
	a <http://www.w3.org/2000/01/rdf-schema#Property> , <http://sw.cyc.com/2006/07/27/cyc/CommercialOrganizationsAndAccounts-Financial-Topic> ;
	<http://sw.cyc.com/2006/07/27/cyc/prettyString-Canonical> "account status" ;
	<http://www.w3.org/2000/01/rdf-schema#domain> <http://sw.cyc.com/2006/07/27/cyc/Account> ;
	<http://sw.cyc.com/2006/07/27/cyc/arity> "2"^^<http://www.w3.org/2001/XMLSchema#long> ;
	<http://www.w3.org/2000/01/rdf-schema#range> <http://sw.cyc.com/2006/07/27/cyc/AccountTypeByStatus> ;
	<http://www.w3.org/2000/01/rdf-schema#subPropertyOf> <http://www.w3.org/1999/02/22-rdf-syntax-ns#type> ;
	<http://sw.cyc.com/2006/07/27/cyc/typedGenlPreds> <http://www.w3.org/1999/02/22-rdf-syntax-ns#type> .

<http://sw.cyc.com/2006/07/27/cyc/accountsPayable> <http://www.w3.org/2000/01/rdf-schema#comment> "This predicate is used to state the total amount the #$IntelligentAgent is due to pay.  To specify the #$TimeInterval in which this is true use #$holdsIn.  So (accountsPayable AGENT MONEY) means that the AGENT has due bills of total amount MONEY.  Borrowed moneys are not part of #$accountsPayable unless they are currently due." ;
	a <http://sw.cyc.com/2006/07/27/cyc/TemporalExistencePredicate> , <http://sw.cyc.com/2006/07/27/cyc/MeasurableQuantitySlot> ;
	<http://sw.cyc.com/2006/07/27/cyc/prettyString-Canonical> "Accounts Payable" ;
	<http://www.w3.org/2000/01/rdf-schema#domain> <http://sw.cyc.com/2006/07/27/cyc/IntelligentAgent> ;
	<http://sw.cyc.com/2006/07/27/cyc/arity> "2"^^<http://www.w3.org/2001/XMLSchema#long> ;
	<http://www.w3.org/2000/01/rdf-schema#range> <http://sw.cyc.com/2006/07/27/cyc/MonetaryValue> ;
	<http://sw.cyc.com/2006/07/27/cyc/arg2Format> <http://sw.cyc.com/2006/07/27/cyc/IntervalEntry> , <http://sw.cyc.com/2006/07/27/cyc/intervalEntryFormatInArgs> ;
	<http://sw.cyc.com/2006/07/27/cyc/functionalInArgs> "2"^^<http://www.w3.org/2001/XMLSchema#long> ;
	<http://sw.cyc.com/2006/07/27/cyc/intervalEntryFormatInArgs> "2"^^<http://www.w3.org/2001/XMLSchema#long> .

<http://sw.cyc.com/2006/07/27/cyc/AccountsPayableDepartment> <http://www.w3.org/2000/01/rdf-schema#comment> "A subset of #$AccountingDepartment; those departments responsible for making payments." ;
	a <http://sw.cyc.com/2006/07/27/cyc/ExistingObjectType> ;
	<http://sw.cyc.com/2006/07/27/cyc/prettyString-Canonical> "accounts payable department" ;
	<http://sw.cyc.com/2006/07/27/cyc/prettyString> "accounts payable departments" ;
	<http://www.w3.org/2000/01/rdf-schema#subClassOf> <http://sw.cyc.com/2006/07/27/cyc/AccountingDepartment> .

<http://sw.cyc.com/2006/07/27/cyc/AccountsPayableWorker> <http://www.w3.org/2000/01/rdf-schema#comment> "accounting dept employees who handle co's bills to others" ;
	a <http://sw.cyc.com/2006/07/27/cyc/PersonTypeByOccupation> ;
	<http://sw.cyc.com/2006/07/27/cyc/prettyString-Canonical> "accounts payable clerk" ;
	<http://sw.cyc.com/2006/07/27/cyc/prettyString> "accounts payable clerks" ;
	<http://www.w3.org/2000/01/rdf-schema#subClassOf> <http://sw.cyc.com/2006/07/27/cyc/DeskWorker> .

<http://sw.cyc.com/2006/07/27/cyc/accountsReceivable> <http://www.w3.org/2000/01/rdf-schema#comment> "This predicate is used to state the amount of money the named #$IntelligentAgent is owed.  Assertions should be made using #$holdsIn to specify during which #$TimeInterval they are true.  So, (accountsReceivable AGENT MONEY) means that AGENT is owed MONEY.  Usually AGENT is owed MONEY due to sales." ;
	a <http://sw.cyc.com/2006/07/27/cyc/TemporalExistencePredicate> , <http://sw.cyc.com/2006/07/27/cyc/MeasurableQuantitySlot> ;
	<http://sw.cyc.com/2006/07/27/cyc/prettyString-Canonical> "accounts receivable" ;
	<http://www.w3.org/2000/01/rdf-schema#domain> <http://sw.cyc.com/2006/07/27/cyc/IntelligentAgent> ;
	<http://sw.cyc.com/2006/07/27/cyc/arity> "2"^^<http://www.w3.org/2001/XMLSchema#long> ;
	<http://www.w3.org/2000/01/rdf-schema#range> <http://sw.cyc.com/2006/07/27/cyc/MonetaryValue> ;
	<http://sw.cyc.com/2006/07/27/cyc/arg2Format> <http://sw.cyc.com/2006/07/27/cyc/IntervalEntry> ;
	<http://sw.cyc.com/2006/07/27/cyc/functionalInArgs> "2"^^<http://www.w3.org/2001/XMLSchema#long> ;
	<http://sw.cyc.com/2006/07/27/cyc/intervalEntryFormatInArgs> "2"^^<http://www.w3.org/2001/XMLSchema#long> .

<http://sw.cyc.com/2006/07/27/cyc/AccountsReceivableDepartment> <http://www.w3.org/2000/01/rdf-schema#comment> "A subset of #$AccountingDepartment; those departments responsible for              invoicing and receiving payments." ;
	a <http://sw.cyc.com/2006/07/27/cyc/ExistingObjectType> ;
	<http://sw.cyc.com/2006/07/27/cyc/prettyString-Canonical> "accounts receivable department" ;
	<http://sw.cyc.com/2006/07/27/cyc/prettyString> "accounts receivable departments" ;
	<http://www.w3.org/2000/01/rdf-schema#subClassOf> <http://sw.cyc.com/2006/07/27/cyc/AccountingDepartment> .

<http://sw.cyc.com/2006/07/27/cyc/accountSystemAccessed> <http://www.w3.org/2000/01/rdf-schema#comment> "(#$accountSystemAccessed ASSESS SYSTEM) means that in the #$AccessingAComputerAccount event ACCESS, the #$AccountSystem on which an account is accessed is SYSTEM." ;
	a <http://sw.cyc.com/2006/07/27/cyc/BinaryRolePredicate> ;
	<http://sw.cyc.com/2006/07/27/cyc/prettyString-Canonical> "Account System Accessed" ;
	<http://sw.cyc.com/2006/07/27/cyc/quotedIsa> <http://sw.cyc.com/2006/07/27/cyc/HasBeenReviewedInRolePredicateSweep> ;
	<http://www.w3.org/2000/01/rdf-schema#domain> <http://sw.cyc.com/2006/07/27/cyc/AccessingAComputerAccount> ;
	<http://sw.cyc.com/2006/07/27/cyc/arity> "2"^^<http://www.w3.org/2001/XMLSchema#long> ;
	<http://www.w3.org/2000/01/rdf-schema#range> <http://sw.cyc.com/2006/07/27/cyc/AccountSystem> .

<http://sw.cyc.com/2006/07/27/cyc/AccountSystemFn> <http://www.w3.org/2000/01/rdf-schema#comment> "(#$AccountSystemFn SYSTEM-TYPE STRING) denotes an #$AccountSystem of type SYSTEM-TYPE which is hosted on a domain uniquely identified by STRING. For example, (#$AccountSystemFn #$NISDomain \"hello.world.net\") denotes the #$NetworkInformationSystem account system on hello.world.net." ;
	a <http://sw.cyc.com/2006/07/27/cyc/ReifiableFunction> , <http://sw.cyc.com/2006/07/27/cyc/BinaryFunction> , <http://sw.cyc.com/2006/07/27/cyc/IndividualDenotingFunction> ;
	<http://sw.cyc.com/2006/07/27/cyc/prettyString-Canonical> "Account System Fn" ;
	<http://www.w3.org/2000/01/rdf-schema#domain> <http://sw.cyc.com/2006/07/27/cyc/AccountSystemTypeByImplementationMeans> ;
	<http://sw.cyc.com/2006/07/27/cyc/arity> "2"^^<http://www.w3.org/2001/XMLSchema#long> ;
	<http://www.w3.org/2000/01/rdf-schema#range> <http://sw.cyc.com/2006/07/27/cyc/CharacterString> ;
	<http://sw.cyc.com/2006/07/27/cyc/resultIsa> <http://sw.cyc.com/2006/07/27/cyc/AccountSystem> .

<http://sw.cyc.com/2006/07/27/cyc/AccountSystemTypeByImplementationMeans> <http://www.w3.org/2000/01/rdf-schema#comment> "A collection of types of #$AccountSystem, divided by their means of implementation. The two most notable instances are #$NISDomain and #$NTDomain." ;
	a <http://sw.cyc.com/2006/07/27/cyc/AtemporalNecessarilyEssentialCollectionType> , <http://sw.cyc.com/2006/07/27/cyc/SiblingDisjointCollectionType> , <http://sw.cyc.com/2006/07/27/cyc/SecondOrderCollection> ;
	<http://sw.cyc.com/2006/07/27/cyc/prettyString-Canonical> "type of account system" ;
	<http://sw.cyc.com/2006/07/27/cyc/prettyString> "types of account system" ;
	<http://www.w3.org/2000/01/rdf-schema#subClassOf> <http://sw.cyc.com/2006/07/27/cyc/ExistingObjectType> ;
	<http://sw.cyc.com/2006/07/27/cyc/typeGenls> <http://sw.cyc.com/2006/07/27/cyc/AccountSystem> .

<http://sw.cyc.com/2006/07/27/cyc/ComputerNetwork> <http://www.w3.org/2000/01/rdf-schema#comment> "A specialization of #$ConnectedPathSystem and #$ComputationalSystem. Each instance of this collection is a network used to link computational systems together to allow them to transfer information between each other. This is typically done using \"packets\" of information (see #$Packet-Network) exchanged according to certain well-defined protocols (see #$NetworkProtocol). A particularly large and notable instance of this collection is #$Internet. Networks may be structured according to certain specific topologies, the most notable of which are #$BusNetwork, #$StarNetwork and #$RingNetwork." ;
	a <http://sw.cyc.com/2006/07/27/cyc/ExistingObjectType> , <http://sw.cyc.com/2006/07/27/cyc/SpatiallyDisjointObjectType> , <http://sw.cyc.com/2006/07/27/cyc/QAClarifyingCollectionType> ;
	<http://sw.cyc.com/2006/07/27/cyc/prettyString-Canonical> "computer network" ;
	<http://sw.cyc.com/2006/07/27/cyc/prettyString> "network" , "networks" , "net" , "nets" , "computer networks" ;
	<http://www.w3.org/2000/01/rdf-schema#subClassOf> <http://sw.cyc.com/2006/07/27/cyc/DurableGood> , <http://sw.cyc.com/2006/07/27/cyc/PathArtifactSystem> , <http://sw.cyc.com/2006/07/27/cyc/ComputationalSystem> , <http://sw.cyc.com/2006/07/27/cyc/CustomarySystemOfLinks-Comm> ;
	<http://sw.cyc.com/2006/07/27/cyc/facets-Generic> <http://sw.cyc.com/2006/07/27/cyc/ComputerNetworkTypeByVulnerability> ;
	<http://sw.cyc.com/2006/07/27/cyc/facets-Strict> <http://sw.cyc.com/2006/07/27/cyc/ComputerNetworkTypeByTopology> .

<http://sw.cyc.com/2006/07/27/cyc/accountSystemOnNetwork> <http://www.w3.org/2000/01/rdf-schema#comment> "A binary predicate that relates instances of #$AccountSystem to instances of #$ComputerNetwork.  (#$accountSystemOnNetwork SYSTEM NETWORK) means that SYSTEM is an instance of #$AccountSystem such that either (#$nodeInSystem SYSTEM NETWORK) holds or (#$subNetwork NETWORK SYSTEM) holds." ;
	a <http://sw.cyc.com/2006/07/27/cyc/CoexistingObjectsPredicate> .

<http://sw.cyc.com/2006/07/27/cyc/AccPropA> <http://sw.cyc.com/2006/07/27/cyc/prettyString-Canonical> "Acc Prop A" .

<http://sw.cyc.com/2006/07/27/cyc/Accreditation> <http://www.w3.org/2000/01/rdf-schema#comment> "A collection of abstract (intangible) objects consisting of information; a subset of #$Credential.  Each element of #$Accreditation is a credential, issued to an organization by the appropriate authority, that declares the issuer's approval of the quality of the recipient's activities.  For example, accreditation of an educational organization to offer a kind of degree or training; or accreditation of a hospital to offer medical services." ;
	a <http://sw.cyc.com/2006/07/27/cyc/ObjectType> , <http://sw.cyc.com/2006/07/27/cyc/QAClarifyingCollectionType> , <http://sw.cyc.com/2006/07/27/cyc/InformationAndCWs-Topic> ;
	<http://sw.cyc.com/2006/07/27/cyc/prettyString-Canonical> "accreditation" ;
	<http://www.w3.org/2000/01/rdf-schema#subClassOf> <http://sw.cyc.com/2006/07/27/cyc/Credential> .

<http://sw.cyc.com/2006/07/27/cyc/AccreditationEvent> a <http://sw.cyc.com/2006/07/27/cyc/FirstOrderCollection> ;
	<http://sw.cyc.com/2006/07/27/cyc/prettyString-Canonical> "accreditation" ;
	<http://sw.cyc.com/2006/07/27/cyc/prettyString> "accredit" , "accredited" , "accredits" , "accrediting" , "have accredited" , "has accredited" , "will accredit" , "had accredited" , "will have accredited" , "accreditations" ;
	<http://www.w3.org/2000/01/rdf-schema#subClassOf> <http://sw.cyc.com/2006/07/27/cyc/ChangeOfStatusEvent> ;
	<http://sw.cyc.com/2006/07/27/cyc/quotedIsa> <http://sw.cyc.com/2006/07/27/cyc/StubTerm> .

<http://sw.cyc.com/2006/07/27/cyc/ChangeOfStatusEvent> <http://www.w3.org/2000/01/rdf-schema#comment> "Elements of #$ChangeOfStatusEvent are events in which the status of a person, group, or organization changes." ;
	a <http://sw.cyc.com/2006/07/27/cyc/TemporalObjectType> ;
	<http://sw.cyc.com/2006/07/27/cyc/prettyString-Canonical> "change in status" ;
	<http://sw.cyc.com/2006/07/27/cyc/prettyString> "change of status" , "changes of status" , "changes in status" ;
	<http://www.w3.org/2000/01/rdf-schema#subClassOf> <http://sw.cyc.com/2006/07/27/cyc/GeneralizedTransfer> , <http://sw.cyc.com/2006/07/27/cyc/SocialOccurrence> ;
	<http://www.w3.org/2002/07/owl#disjointWith> <http://sw.cyc.com/2006/07/27/cyc/Collapsing-Generic> ;
	<http://sw.cyc.com/2006/07/27/cyc/requiredActorSlots> <http://sw.cyc.com/2006/07/27/cyc/objectOfStatusChange> .

<http://sw.cyc.com/2006/07/27/cyc/Credential> <http://www.w3.org/2000/01/rdf-schema#comment> "A specialization of #$PropositionalInformationThing.  Each instance of #$Credential is specific information about one #$SocialBeing (q.v.), provided by another #$SocialBeing.  The information content of a credential consists of favorable, enabling, or empowering propositional declarations.  Although each instance of #$Credential is wholly intangible, instances of #$Credential usually have some associated #$TextualMaterial (e.g. a diploma associated with a college degree, a driver's license).  A credential may certify that the holder (i.e. the subject of the credential) has a particular skill (e.g. legal bar certification or the ability to drive); has completed certain training (e.g. GED schooling or satisfying PhD requirements); is allowed to do a certain thing (e.g. a travel visa or permission slip); and so on.  See also the predicate #$issuesCredential." ;
	a <http://sw.cyc.com/2006/07/27/cyc/ObjectType> , <http://sw.cyc.com/2006/07/27/cyc/QAClarifyingCollectionType> , <http://sw.cyc.com/2006/07/27/cyc/InformationAndCWs-Topic> ;
	<http://sw.cyc.com/2006/07/27/cyc/prettyString-Canonical> "credential" ;
	<http://sw.cyc.com/2006/07/27/cyc/prettyString> "credentials" ;
	<http://www.w3.org/2000/01/rdf-schema#subClassOf> <http://sw.cyc.com/2006/07/27/cyc/PropositionalConceptualWork> ;
	<http://www.w3.org/2002/07/owl#disjointWith> <http://sw.cyc.com/2006/07/27/cyc/TradeableSecurity> ;
	<http://sw.cyc.com/2006/07/27/cyc/facets-Strict> <http://sw.cyc.com/2006/07/27/cyc/CredentialTypeBySkill> .

<http://sw.cyc.com/2006/07/27/cyc/AccredoHealthIncorporated> a <http://sw.cyc.com/2006/07/27/cyc/Individual> , <http://sw.cyc.com/2006/07/27/cyc/PubliclyHeldCorporation> ;
	<http://sw.cyc.com/2006/07/27/cyc/prettyString-Canonical> "Accredo Health Incorporated" .

<http://sw.cyc.com/2006/07/27/cyc/AccruingInterest> <http://www.w3.org/2000/01/rdf-schema#comment> "A specialization of #$IncreasingTheBalanceOnAnAccount.  Each instance of #$AccruingInterest is an event in which the balance (see #$accountBalance) on an account is increased due to the crediting/charging of interest towards the balance." ;
	a <http://sw.cyc.com/2006/07/27/cyc/TemporalObjectType> ;
	<http://sw.cyc.com/2006/07/27/cyc/prettyString-Canonical> "accruing interest" ;
	<http://sw.cyc.com/2006/07/27/cyc/prettyString> "accrue interest" , "accrued interest" , "accrues interest" .

<http://sw.cyc.com/2006/07/27/cyc/AccruingInterestOnACD> <http://sw.cyc.com/2006/07/27/cyc/prettyString> "will accrue interest on a CD" , "had accrued interest on a CD" , "will have accrued interest on a CD" , "accrue interest on a Certificate of Deposit" , "accrued interest on a Certificate of Deposit" , "accrues interest on a Certificate of Deposit" , "accruing interest on a Certificate of Deposit" , "have accrued interest on a Certificate of Deposit" , "has accrued interest on a Certificate of Deposit" , "will accrue interest on a Certificate of Deposit" , "had accrued interest on a Certificate of Deposit" , "will have accrued interest on a Certificate of Deposit" , "accrue interest on a Certificate of Deposit account" , "accrued interest on a Certificate of Deposit account" , "accrues interest on a Certificate of Deposit account" , "accruing interest on a Certificate of Deposit account" , "have accrued interest on a Certificate of Deposit account" , "has accrued interest on a Certificate of Deposit account" , "will accrue interest on a Certificate of Deposit account" , "had accrued interest on a Certificate of Deposit account" , "will have accrued interest on a Certificate of Deposit account" , "accrue interest on a CD account" , "accrued interest on a CD account" , "accrues interest on a CD account" , "have accrued interest on a CD account" , "has accrued interest on a CD account" , "will accrue interest on a CD account" , "had accrued interest on a CD account" , "will have accrued interest on a CD account" ;
	<http://www.w3.org/2000/01/rdf-schema#subClassOf> <http://sw.cyc.com/2006/07/27/cyc/AccruingInterest> , <http://sw.cyc.com/2006/07/27/cyc/AccruingInterestOnABankAccount> .

<http://sw.cyc.com/2006/07/27/cyc/AccruingInterestOnALoan> <http://www.w3.org/2000/01/rdf-schema#comment> "A specialization of #$IncreasingTheBalanceOnAnAccount.  Each instance of #$AccruingInterestOnALoan is an event in which an agent accumulates interest on an outstanding loan balance." ;
	a <http://sw.cyc.com/2006/07/27/cyc/InterestAccrualTypeByAccountType> ;
	<http://sw.cyc.com/2006/07/27/cyc/prettyString-Canonical> "accruing interest on a loan" ;
	<http://sw.cyc.com/2006/07/27/cyc/prettyString> "accrue interest on a loan" , "accrued interest on a loan" , "accrues interest on a loan" , "have accrued interest on a loan" , "has accrued interest on a loan" , "will accrue interest on a loan" , "had accrued interest on a loan" , "will have accrued interest on a loan" ;
	<http://www.w3.org/2000/01/rdf-schema#subClassOf> <http://sw.cyc.com/2006/07/27/cyc/AccruingInterest> .

<http://sw.cyc.com/2006/07/27/cyc/AccruingInterestOnASavingsAccount> <http://www.w3.org/2000/01/rdf-schema#comment> "The collection of all instances of #$AccruingInterest in which the account that interest is credited to is an instance of #$SavingsAccount." ;
	a <http://sw.cyc.com/2006/07/27/cyc/InterestAccrualTypeByAccountType> ;
	<http://sw.cyc.com/2006/07/27/cyc/prettyString-Canonical> "accruing interest on a savings account" ;
	<http://sw.cyc.com/2006/07/27/cyc/prettyString> "accrue interest on a savings account" , "accrued interest on a savings account" , "accrues interest on a savings account" , "has accrued interest on a savings account" , "will accrue interest on a savings account" , "had accrued interest on a savings account" , "will have accrued interest on a savings account" ;
	<http://www.w3.org/2000/01/rdf-schema#subClassOf> <http://sw.cyc.com/2006/07/27/cyc/AccruingInterestOnABankAccount> .

<http://sw.cyc.com/2006/07/27/cyc/Accstat-TheProgram> <http://www.w3.org/2000/01/rdf-schema#comment> "The accessibility status indicator for #$MSWindows." ;
	a <http://sw.cyc.com/2006/07/27/cyc/Individual> , <http://sw.cyc.com/2006/07/27/cyc/UnversionedProgram> , <http://sw.cyc.com/2006/07/27/cyc/LocalProgram> , <http://sw.cyc.com/2006/07/27/cyc/UserProgram> , <http://sw.cyc.com/2006/07/27/cyc/MSWindowsApplication> , <http://sw.cyc.com/2006/07/27/cyc/MicrosoftComputerProgram> ;
	<http://sw.cyc.com/2006/07/27/cyc/prettyString-Canonical> "Windows Accessibility Status Indicator" ;
	<http://sw.cyc.com/2006/07/27/cyc/prettyString> "Accstat" .

<http://sw.cyc.com/2006/07/27/cyc/MSWindowsApplication> <http://www.w3.org/2000/01/rdf-schema#comment> "Programs that are made to run under #$MSWindows and #$MSWindowsNT" ;
	a <http://www.w3.org/2002/07/owl#Class> , <http://sw.cyc.com/2006/07/27/cyc/ObjectType> , <http://sw.cyc.com/2006/07/27/cyc/AtemporalNecessarilyEssentialCollectionType> , <http://sw.cyc.com/2006/07/27/cyc/QAClarifyingCollectionType> ;
	<http://sw.cyc.com/2006/07/27/cyc/prettyString-Canonical> "Windows application" ;
	<http://sw.cyc.com/2006/07/27/cyc/prettyString> "Windows applications" ;
	<http://www.w3.org/2000/01/rdf-schema#subClassOf> <http://sw.cyc.com/2006/07/27/cyc/ApplicationProgram> .

<http://sw.cyc.com/2006/07/27/cyc/MicrosoftComputerProgram> <http://www.w3.org/2000/01/rdf-schema#comment> "Software products made by #$MicrosoftInc." ;
	a <http://sw.cyc.com/2006/07/27/cyc/AtemporalNecessarilyEssentialCollectionType> , <http://sw.cyc.com/2006/07/27/cyc/ComputerProgramTypeByCreator> ;
	<http://sw.cyc.com/2006/07/27/cyc/prettyString-Canonical> "Microsoft computer program" ;
	<http://sw.cyc.com/2006/07/27/cyc/prettyString> "Microsoft software" , "Microsoft programme" , "Microsoft program" , "Microsoft programs" , "Microsoft programz" , "Microsoft computer programme" , "Microsoft computer programs" , "Microsoft computer programz" ;
	<http://www.w3.org/2000/01/rdf-schema#subClassOf> <http://sw.cyc.com/2006/07/27/cyc/ComputerProgram-CW> .

<http://sw.cyc.com/2006/07/27/cyc/AccumulatingSteadily> <http://www.w3.org/2000/01/rdf-schema#comment> "A collection of events; a subcollection of #$IntrinsicStateChangeEvent. In each #$AccumulatingSteadily, something forms or accumulates steadily." ;
	a <http://sw.cyc.com/2006/07/27/cyc/FirstOrderCollection> ;
	<http://sw.cyc.com/2006/07/27/cyc/prettyString-Canonical> "building up" ;
	<http://sw.cyc.com/2006/07/27/cyc/prettyString> "BUILDING" , "build" , "built" , "builds" , "have built" , "has built" , "will build" , "had built" , "will have built" , "build up" , "built up" , "builds up" , "have built up" , "has built up" , "will build up" , "had built up" , "will have built up" , "work up" , "worked up" , "works up" , "working up" , "have worked up" , "has worked up" , "will work up" , "had worked up" , "will have worked up" , "progress" , "progressed" , "progresses" , "progressing" , "have progressed" , "has progressed" , "had progressed" , "will have progressed" ;
	<http://www.w3.org/2000/01/rdf-schema#subClassOf> <http://sw.cyc.com/2006/07/27/cyc/IntrinsicStateChangeEvent> ;
	<http://sw.cyc.com/2006/07/27/cyc/quotedIsa> <http://sw.cyc.com/2006/07/27/cyc/WordNetWorkflowConstant-NotFullyReviewed> .

<http://sw.cyc.com/2006/07/27/cyc/Accumulation-Profits> <http://www.w3.org/2000/01/rdf-schema#comment> "A sub-collection of #$Profits. Each instance is profits that are not paid out as dividends but are added to the capital base of the corporation." ;
	a <http://sw.cyc.com/2006/07/27/cyc/FirstOrderCollection> ;
	<http://sw.cyc.com/2006/07/27/cyc/prettyString-Canonical> "accumulation" ;
	<http://www.w3.org/2000/01/rdf-schema#subClassOf> <http://sw.cyc.com/2006/07/27/cyc/Profits> ;
	<http://sw.cyc.com/2006/07/27/cyc/quotedIsa> <http://sw.cyc.com/2006/07/27/cyc/WordNetWorkflowConstant-NotFullyReviewed> .

<http://sw.cyc.com/2006/07/27/cyc/Profits> <http://www.w3.org/2000/01/rdf-schema#comment> "A sub-collection of #$MonetaryRate. Each instance is the excess of revenues over outlays in a given period of time (including depreciation and other non-cash expenses)." ;
	a <http://www.w3.org/2002/07/owl#Class> , <http://sw.cyc.com/2006/07/27/cyc/FirstOrderCollection> ;
	<http://sw.cyc.com/2006/07/27/cyc/prettyString-Canonical> "net income" ;
	<http://sw.cyc.com/2006/07/27/cyc/prettyString> "profits" , "profit" , "Net Profit" , "net" , "monetary flow rate that has been a profit of a companies" , "rate of monetary flow that is a profit of a companies" , "monetary flow rate that is a profit of a companies" , "rate of monetary flow that has been a profit of a businesses" , "monetary flow rate that has been a profit of a businesses" , "rate of monetary flow that is a profit of a businesses" , "monetary flow rate that is a profit of a businesses" , "rate of monetary flow that has been a profit of a enterprise" , "monetary flow rate that has been a profit of a enterprise" , "rate of monetary flow that is a profit of a enterprise" , "monetary flow rate that is a profit of a enterprise" , "rate of monetary flow that has been a profit of a business firm" , "monetary flow rate that has been a profit of a business firm" , "rate of monetary flow that is a profit of a business firm" , "monetary flow rate that is a profit of a business firm" , "rate of monetary flow that has been a profit of a business concern" , "monetary flow rate that has been a profit of a business concern" , "rate of monetary flow that is a profit of a business concern" , "monetary flow rate that is a profit of a business concern" , "rate of monetary flow that has been a profit of a business organization" , "monetary flow rate that has been a profit of a business organization" , "rate of monetary flow that is a profit of a business organization" , "monetary flow rate that is a profit of a business organization" , "positive monetary income received by a business" , "lucre" , "rate of monetary flow that has been a profit of a business" , "monetary flow rate that has been a profit of a business" , "rate of monetary flow that is a profit of a business" , "monetary flow rate that is a profit of a business" , "rate of monetary flow that has been a profit of a firm" , "monetary flow rate that has been a profit of a firm" , "rate of monetary flow that is a profit of a firm" , "monetary flow rate that is a profit of a firm" .

<http://sw.cyc.com/2006/07/27/cyc/Accusing> <http://sw.cyc.com/2006/07/27/cyc/prettyString> "have accused" , "has accused" , "will accuse" , "had accused" , "will have accused" ;
	<http://www.w3.org/2000/01/rdf-schema#subClassOf> <http://sw.cyc.com/2006/07/27/cyc/HostileSocialAction> , <http://sw.cyc.com/2006/07/27/cyc/AttributingResponsibility> ;
	<http://sw.cyc.com/2006/07/27/cyc/requiredArg1Pred> <http://sw.cyc.com/2006/07/27/cyc/accusedOfRoleInEvent> , <http://sw.cyc.com/2006/07/27/cyc/accusedOfRoleInType> .

<http://sw.cyc.com/2006/07/27/cyc/intendedMaleficiary> <http://www.w3.org/2000/01/rdf-schema#comment> "<code>(#$intendedMaleficiary ACTION AGENT)</code> means that either (i) some agent who directs (see #$directingAgent) <code>ACTION</code> intends that <code>AGENT</code> be harmed in (see #$maleficiary) <code>ACTION</code> or (ii) there is no directing agent, but some agent who performs (see #$performedBy) <code>ACTION</code> intends that <code>AGENT</code> be a maleficiary of <code>ACTION</code>." ;
	a <http://sw.cyc.com/2006/07/27/cyc/BinaryRolePredicate> , <http://sw.cyc.com/2006/07/27/cyc/RelationalNounSlot> , <http://sw.cyc.com/2006/07/27/cyc/Terrorism-Topic> ;
	<http://sw.cyc.com/2006/07/27/cyc/prettyString-Canonical> "intended maleficiary" ;
	<http://sw.cyc.com/2006/07/27/cyc/prettyString> "intended maleficiaries" ;
	<http://www.w3.org/2000/01/rdf-schema#domain> <http://sw.cyc.com/2006/07/27/cyc/PurposefulAction> ;
	<http://sw.cyc.com/2006/07/27/cyc/arity> "2"^^<http://www.w3.org/2001/XMLSchema#long> ;
	<http://www.w3.org/2000/01/rdf-schema#range> <http://sw.cyc.com/2006/07/27/cyc/Agent-Generic> ;
	<http://www.w3.org/2000/01/rdf-schema#subPropertyOf> <http://sw.cyc.com/2006/07/27/cyc/against-Underspecified> , <http://sw.cyc.com/2006/07/27/cyc/focalSubject> , <http://sw.cyc.com/2006/07/27/cyc/highlyRelevantInEvent> ;
	<http://sw.cyc.com/2006/07/27/cyc/genlInverse> <http://sw.cyc.com/2006/07/27/cyc/negativeVestedInterest> .

<http://sw.cyc.com/2006/07/27/cyc/containsInformationAbout-Focally> <http://www.w3.org/2000/01/rdf-schema#comment> "This predicate relates sources of information to their main topics.  (#$containsInformationAbout-Focally IS THING) means that IS is generally \"about\" THING -- which may be any instance of #$Thing at all. This predicate represents a very general notion of aboutness, which does not require that THING be explicitly named in IS, but that it be one of the main topics of IS. Note that IS can have more than one main topic -- e.g., a textbook can have both logic and set theory as main topics.  Use the more general predicate #$containsInformationAbout to specify that IS contains some information about THING, but that THING is not a main topic of IS." ;
	a <http://www.w3.org/2000/01/rdf-schema#Property> , <http://www.w3.org/2002/07/owl#TransitiveProperty> , <http://www.w3.org/2002/07/owl#SymmetricProperty> , <http://sw.cyc.com/2006/07/27/cyc/AntiSymmetricBinaryPredicate> , <http://sw.cyc.com/2006/07/27/cyc/ReflexiveBinaryPredicate> , <http://sw.cyc.com/2006/07/27/cyc/IrreflexiveBinaryPredicate> ;
	<http://sw.cyc.com/2006/07/27/cyc/prettyString-Canonical> "Contains Information About Focally" ;
	<http://www.w3.org/2000/01/rdf-schema#domain> <http://sw.cyc.com/2006/07/27/cyc/InformationStore> ;
	<http://sw.cyc.com/2006/07/27/cyc/arity> "2"^^<http://www.w3.org/2001/XMLSchema#long> ;
	<http://www.w3.org/2000/01/rdf-schema#range> <http://www.w3.org/2002/07/owl#Thing> ;
	<http://www.w3.org/2000/01/rdf-schema#subPropertyOf> <http://www.w3.org/2000/01/rdf-schema#isDefinedBy> ;
	<http://sw.cyc.com/2006/07/27/cyc/arg1Format> <http://sw.cyc.com/2006/07/27/cyc/openEntryFormatInArgs> ;
	<http://sw.cyc.com/2006/07/27/cyc/arg2Format> <http://sw.cyc.com/2006/07/27/cyc/openEntryFormatInArgs> .

<http://sw.cyc.com/2006/07/27/cyc/claimsResponsible> <http://www.w3.org/2000/01/rdf-schema#comment> "'(#$claimsResponsible CLAIM AGENT)' means that in the #$AttributingResponsibility action CLAIM, responsibility is attributed to AGENT." ;
	a <http://sw.cyc.com/2006/07/27/cyc/BinaryRolePredicate> ;
	<http://sw.cyc.com/2006/07/27/cyc/prettyString-Canonical> "Claims Responsible" ;
	<http://www.w3.org/2000/01/rdf-schema#domain> <http://sw.cyc.com/2006/07/27/cyc/AttributingResponsibility> ;
	<http://sw.cyc.com/2006/07/27/cyc/arity> "2"^^<http://www.w3.org/2001/XMLSchema#long> ;
	<http://www.w3.org/2000/01/rdf-schema#range> <http://sw.cyc.com/2006/07/27/cyc/Agent-Generic> ;
	<http://www.w3.org/2000/01/rdf-schema#subPropertyOf> <http://sw.cyc.com/2006/07/27/cyc/containsInformationAbout-Focally> .

<http://sw.cyc.com/2006/07/27/cyc/accusedOf> <http://www.w3.org/2000/01/rdf-schema#comment> "A #$BinaryPredicate that relates an #$Accusing to an #$Action.  <code>(#$accusedOf ACCUSING ACTION)</code> means that the agent playing the role of #$accused in <code>ACCUSING</code> is accused of performing <code>ACTION</code>.  See also #$accusedOfRoleInEvent, #$accusedOfRoleInType, and #$accusedOfPerformingActionType." ;
	a <http://sw.cyc.com/2006/07/27/cyc/AsymmetricBinaryPredicate> ;
	<http://sw.cyc.com/2006/07/27/cyc/prettyString-Canonical> "Accused Of" ;
	<http://www.w3.org/2000/01/rdf-schema#domain> <http://sw.cyc.com/2006/07/27/cyc/Accusing> ;
	<http://sw.cyc.com/2006/07/27/cyc/arity> "2"^^<http://www.w3.org/2001/XMLSchema#long> ;
	<http://www.w3.org/2000/01/rdf-schema#range> <http://sw.cyc.com/2006/07/27/cyc/Action> ;
	<http://www.w3.org/2000/01/rdf-schema#subPropertyOf> <http://sw.cyc.com/2006/07/27/cyc/actAttributed> ;
	<http://sw.cyc.com/2006/07/27/cyc/negationInverse> <http://sw.cyc.com/2006/07/27/cyc/accusedOf> .

<http://sw.cyc.com/2006/07/27/cyc/actAttributed> <http://www.w3.org/2000/01/rdf-schema#comment> "'(#$actAttributed ATTRIBUTING ACT)' means that ACT is the action for which responsibility is attributed in the #$AttributingResponsibility ATTRIBUTING." ;
	a <http://sw.cyc.com/2006/07/27/cyc/BinaryRolePredicate> ;
	<http://sw.cyc.com/2006/07/27/cyc/prettyString-Canonical> "Act Attributed" ;
	<http://sw.cyc.com/2006/07/27/cyc/quotedIsa> <http://sw.cyc.com/2006/07/27/cyc/HasBeenReviewedInRolePredicateSweep> ;
	<http://www.w3.org/2000/01/rdf-schema#domain> <http://sw.cyc.com/2006/07/27/cyc/AttributingResponsibility> ;
	<http://sw.cyc.com/2006/07/27/cyc/arity> "2"^^<http://www.w3.org/2001/XMLSchema#long> .

<http://sw.cyc.com/2006/07/27/cyc/Accwiz-TheProgram> a <http://sw.cyc.com/2006/07/27/cyc/UserProgram> , <http://sw.cyc.com/2006/07/27/cyc/UtilityProgram> , <http://sw.cyc.com/2006/07/27/cyc/MSWindowsApplication> , <http://sw.cyc.com/2006/07/27/cyc/MicrosoftComputerProgram> ;
	<http://sw.cyc.com/2006/07/27/cyc/prettyString-Canonical> "Windows Accessibility Wizard" ;
	<http://sw.cyc.com/2006/07/27/cyc/prettyString> "Microsoft Accessibility Wizard" .

<http://sw.cyc.com/2006/07/27/cyc/AC-DC-MusicGroup> a <http://sw.cyc.com/2006/07/27/cyc/Individual> , <http://sw.cyc.com/2006/07/27/cyc/RockMusicPerformer> ;
	<http://sw.cyc.com/2006/07/27/cyc/prettyString-Canonical> "AC/DC" ;
	<http://sw.cyc.com/2006/07/27/cyc/prettyString> "AC DC" , "ACDC" .

<http://sw.cyc.com/2006/07/27/cyc/ACDSee> <http://www.w3.org/2000/01/rdf-schema#comment> "ACDSee is an image browser/viewer/editing software program developed by ACD Systems." ;
	a <http://sw.cyc.com/2006/07/27/cyc/Individual> , <http://sw.cyc.com/2006/07/27/cyc/UnversionedProgram> , <http://sw.cyc.com/2006/07/27/cyc/GraphicsEditingProgram> ;
	<http://sw.cyc.com/2006/07/27/cyc/prettyString-Canonical> "ACDSee" .

<http://sw.cyc.com/2006/07/27/cyc/GraphicsEditingProgram> <http://www.w3.org/2000/01/rdf-schema#comment> """This is a #$ComputerProgramTypeByFunction where the function in question is
the creation and manipulation of computer images.""" ;
	a <http://sw.cyc.com/2006/07/27/cyc/KEClarifyingCollectionType> , <http://sw.cyc.com/2006/07/27/cyc/ComputerProgramTypeByFunction> ;
	<http://sw.cyc.com/2006/07/27/cyc/prettyString-Canonical> "graphics editing program" ;
	<http://sw.cyc.com/2006/07/27/cyc/prettyString> "graphics software" , "graphics editor" , "graphics editors" , "graphics editing programme" , "graphics editing programs" , "graphics editing programz" ;
	<http://www.w3.org/2000/01/rdf-schema#subClassOf> <http://sw.cyc.com/2006/07/27/cyc/FileWritingProgram> , <http://sw.cyc.com/2006/07/27/cyc/ImageFileViewingProgram> .

<http://sw.cyc.com/2006/07/27/cyc/Acebutolol> <http://www.w3.org/2000/01/rdf-schema#comment> "The chemical compound which is a beta blocker.  This drug is intended to be used for therapeutic treatment of hypertension." ;
	a <http://sw.cyc.com/2006/07/27/cyc/PharmaceuticalType> ;
	<http://sw.cyc.com/2006/07/27/cyc/prettyString-Canonical> "acebutolol" ;
	<http://www.w3.org/2000/01/rdf-schema#subClassOf> <http://sw.cyc.com/2006/07/27/cyc/BetaBlocker> .

<http://sw.cyc.com/2006/07/27/cyc/BetaBlocker> <http://www.w3.org/2000/01/rdf-schema#comment> "A drug substance that interfers with the transmission of sympathetic nervous inhibiting stimuli at the adrenergic beta receptors .  Each #$BetaBlocker is a #$CardiovascularAgent." ;
	a <http://sw.cyc.com/2006/07/27/cyc/TherapeuticClassType> ;
	<http://sw.cyc.com/2006/07/27/cyc/prettyString-Canonical> "beta blocker" ;
	<http://sw.cyc.com/2006/07/27/cyc/prettyString> "beta blockers" ;
	<http://www.w3.org/2000/01/rdf-schema#subClassOf> <http://sw.cyc.com/2006/07/27/cyc/ManufacturedGoods> , <http://sw.cyc.com/2006/07/27/cyc/CardiovascularAgent> .

<http://sw.cyc.com/2006/07/27/cyc/AceCashExpressInc> a <http://sw.cyc.com/2006/07/27/cyc/Individual> , <http://sw.cyc.com/2006/07/27/cyc/PubliclyHeldCorporation> ;
	<http://sw.cyc.com/2006/07/27/cyc/prettyString-Canonical> "Ace Cash Express Inc" .

<http://sw.cyc.com/2006/07/27/cyc/ACECOMMCorporation> a <http://sw.cyc.com/2006/07/27/cyc/Individual> , <http://sw.cyc.com/2006/07/27/cyc/PubliclyHeldCorporation> ;
	<http://sw.cyc.com/2006/07/27/cyc/prettyString-Canonical> "ACECOMM Corporation" .

<http://sw.cyc.com/2006/07/27/cyc/AcehnesePerson> <http://www.w3.org/2000/01/rdf-schema#comment> "Indigenous inhabitants of #$Aceh-RegionIndonesia." ;
	a <http://sw.cyc.com/2006/07/27/cyc/PersonTypeByRegionalAffiliation> ;
	<http://sw.cyc.com/2006/07/27/cyc/prettyString-Canonical> "acehnese" ;
	<http://www.w3.org/2000/01/rdf-schema#subClassOf> <http://sw.cyc.com/2006/07/27/cyc/Person> , <http://sw.cyc.com/2006/07/27/cyc/EasternHemispherePerson> , <http://sw.cyc.com/2006/07/27/cyc/AsianCitizenOrSubject> .

<http://sw.cyc.com/2006/07/27/cyc/EasternHemispherePerson> <http://www.w3.org/2000/01/rdf-schema#comment> "The collection of instances of #$Person who identify themselves (or who are identified by others as) 'easterners.' This is a very broadly defined collection, subsuming both nationalities and ethnic group types." ;
	a <http://sw.cyc.com/2006/07/27/cyc/PersonTypeByRegionalAffiliation> ;
	<http://sw.cyc.com/2006/07/27/cyc/prettyString-Canonical> "Eastern Hemisphere person" ;
	<http://sw.cyc.com/2006/07/27/cyc/prettyString> "Eastern Hemisphere people" , "Eastern Hemisphere persons" ;
	<http://www.w3.org/2000/01/rdf-schema#subClassOf> <http://sw.cyc.com/2006/07/27/cyc/Person> .

<http://sw.cyc.com/2006/07/27/cyc/AsianCitizenOrSubject> <http://www.w3.org/2000/01/rdf-schema#comment> "The collection of people who are citizens of, or otherwise by status under the jurisdiction of, a country or other #$GeopoliticalEntity whose territory is located in the #$ContinentOfAsia.  A person native to an area of Asia not under the jurisdiction of any #$GeopoliticalEntity would also be an instance of #$AsianCitizenOrSubject." ;
	a <http://sw.cyc.com/2006/07/27/cyc/PersonTypeByContinentAffiliation> , <http://sw.cyc.com/2006/07/27/cyc/PersonTypeByGeographicResidence> .

<http://sw.cyc.com/2006/07/27/cyc/ACELimited> a <http://sw.cyc.com/2006/07/27/cyc/PubliclyHeldCorporation> ;
	<http://sw.cyc.com/2006/07/27/cyc/prettyString-Canonical> "ACE Limited" .

<http://sw.cyc.com/2006/07/27/cyc/AceOfBase-MusicGroup> a <http://sw.cyc.com/2006/07/27/cyc/Individual> , <http://sw.cyc.com/2006/07/27/cyc/RockMusicPerformer> , <http://sw.cyc.com/2006/07/27/cyc/PopRockMusicPerformer> ;
	<http://sw.cyc.com/2006/07/27/cyc/prettyString-Canonical> "Ace Of Base" .

<http://sw.cyc.com/2006/07/27/cyc/AceOfPenguins-TheGame> a <http://sw.cyc.com/2006/07/27/cyc/Individual> , <http://sw.cyc.com/2006/07/27/cyc/UnversionedProgram> , <http://sw.cyc.com/2006/07/27/cyc/ComputerGameProgram> , <http://sw.cyc.com/2006/07/27/cyc/Freeware> , <http://sw.cyc.com/2006/07/27/cyc/OpenSourceComputerProgram> ;
	<http://sw.cyc.com/2006/07/27/cyc/prettyString-Canonical> "Ace of Penguins" .

<http://sw.cyc.com/2006/07/27/cyc/AcerAcernoteComputer> a <http://sw.cyc.com/2006/07/27/cyc/SpatiallyDisjointObjectType> , <http://sw.cyc.com/2006/07/27/cyc/ComputerHardwareTypeByBrandVersion> , <http://sw.cyc.com/2006/07/27/cyc/ComputerTypeByBrand> ;
	<http://sw.cyc.com/2006/07/27/cyc/prettyString-Canonical> "Acernote" ;
	<http://www.w3.org/2000/01/rdf-schema#subClassOf> <http://sw.cyc.com/2006/07/27/cyc/ManufacturedGoods> , <http://sw.cyc.com/2006/07/27/cyc/LaptopComputer> , <http://sw.cyc.com/2006/07/27/cyc/AcerComputer> .

<http://sw.cyc.com/2006/07/27/cyc/LaptopComputer> a <http://sw.cyc.com/2006/07/27/cyc/ExistingObjectType> , <http://sw.cyc.com/2006/07/27/cyc/SpatiallyDisjointObjectType> , <http://sw.cyc.com/2006/07/27/cyc/ArtifactTypeByGenericCategory> , <http://sw.cyc.com/2006/07/27/cyc/ComputerHardwareDeviceType> ;
	<http://sw.cyc.com/2006/07/27/cyc/prettyString-Canonical> "laptop computer" ;
	<http://sw.cyc.com/2006/07/27/cyc/prettyString> "laptop" , "laptops" , "laptop computers" ;
	<http://www.w3.org/2000/01/rdf-schema#subClassOf> <http://sw.cyc.com/2006/07/27/cyc/PortableObject> , <http://sw.cyc.com/2006/07/27/cyc/PersonalComputer> ;
	<http://sw.cyc.com/2006/07/27/cyc/siblingDisjointExceptions> <http://sw.cyc.com/2006/07/27/cyc/ComputerWorkstation> .

<http://sw.cyc.com/2006/07/27/cyc/AcerComputer> a <http://sw.cyc.com/2006/07/27/cyc/ExistingObjectType> , <http://sw.cyc.com/2006/07/27/cyc/SpatiallyDisjointObjectType> , <http://sw.cyc.com/2006/07/27/cyc/ComputerTypeByBrand> , <http://sw.cyc.com/2006/07/27/cyc/Computers-Topic> ;
	<http://sw.cyc.com/2006/07/27/cyc/prettyString-Canonical> "Acer computer" ;
	<http://sw.cyc.com/2006/07/27/cyc/prettyString> "Acer computers" ;
	<http://www.w3.org/2000/01/rdf-schema#subClassOf> <http://sw.cyc.com/2006/07/27/cyc/ManufacturedGoods> , <http://sw.cyc.com/2006/07/27/cyc/PersonalComputer> .

<http://sw.cyc.com/2006/07/27/cyc/ComputerHardwareTypeByBrandVersion> <http://www.w3.org/2000/01/rdf-schema#comment> """A specialization of #$ComputerHardwareTypeByBrand and #$ProductTypeByBrandVersion. Each instance of this (second-order) collection is
a spec of #$ComputerHardwareItem which is a version of a type of brand-name computer (for example, #$AppleiMacComputer) or a version of a type of brand-name computer hardware item (for
example, #$Motorola68C000Processor).""" ;
	a <http://sw.cyc.com/2006/07/27/cyc/SecondOrderCollection> ;
	<http://sw.cyc.com/2006/07/27/cyc/prettyString-Canonical> "computer hardware type by brand version" ;
	<http://www.w3.org/2000/01/rdf-schema#subClassOf> <http://sw.cyc.com/2006/07/27/cyc/ProductTypeByBrandVersion> , <http://sw.cyc.com/2006/07/27/cyc/ComputerHardwareTypeByBrand> ;
	<http://sw.cyc.com/2006/07/27/cyc/typeGenls> <http://sw.cyc.com/2006/07/27/cyc/ManufacturedGoods> , <http://sw.cyc.com/2006/07/27/cyc/ComputerHardwareItem> .

<http://sw.cyc.com/2006/07/27/cyc/ComputerTypeByBrand> <http://www.w3.org/2000/01/rdf-schema#comment> "A collection of collections.  Each instance of #$ComputerTypeByBrand is a collection of computers, where that collection is a #$ProductTypeByBrand." ;
	a <http://sw.cyc.com/2006/07/27/cyc/AtemporalNecessarilyEssentialCollectionType> , <http://sw.cyc.com/2006/07/27/cyc/SiblingDisjointCollectionType> , <http://sw.cyc.com/2006/07/27/cyc/FacetingCollectionType> .

<http://sw.cyc.com/2006/07/27/cyc/AcerInc> <http://sw.cyc.com/2006/07/27/cyc/prettyString-Canonical> "Acer" ;
	<http://sw.cyc.com/2006/07/27/cyc/prettyString> "Acer, Inc." .

<http://sw.cyc.com/2006/07/27/cyc/ComputerManufacturer> a <http://sw.cyc.com/2006/07/27/cyc/Computers-Topic> , <http://sw.cyc.com/2006/07/27/cyc/ManufacturerTypeByFocalProductType> ;
	<http://sw.cyc.com/2006/07/27/cyc/prettyString-Canonical> "computer manufacturer" ;
	<http://sw.cyc.com/2006/07/27/cyc/prettyString> "computer manufacturer" , "computers manufacturer" , "computer makers" , "hardware company" , "hardware companies" , "computer manufacturers" ;
	<http://www.w3.org/2000/01/rdf-schema#subClassOf> <http://sw.cyc.com/2006/07/27/cyc/HighTechManufacturingEnterprise> ;
	<http://sw.cyc.com/2006/07/27/cyc/quotedIsa> <http://sw.cyc.com/2006/07/27/cyc/WordNetWorkflowConstant-NotFullyReviewed> .

<http://sw.cyc.com/2006/07/27/cyc/ACertainRatio-MusicGroup> a <http://sw.cyc.com/2006/07/27/cyc/Individual> ;
	<http://sw.cyc.com/2006/07/27/cyc/prettyString-Canonical> "A Certain Ratio" .

<http://sw.cyc.com/2006/07/27/cyc/ACEServer-TheProgram> <http://www.w3.org/2000/01/rdf-schema#comment> "ACE/Server is an authentication solution that uses SecureID tokens offered by RSA Data Security for Microsoft's Windows 2000 and Solaris." ;
	a <http://sw.cyc.com/2006/07/27/cyc/Individual> , <http://sw.cyc.com/2006/07/27/cyc/UnversionedProgram> , <http://sw.cyc.com/2006/07/27/cyc/AuthenticationProgram-Remote> ;
	<http://sw.cyc.com/2006/07/27/cyc/prettyString-Canonical> "ACE/Server" .

<http://sw.cyc.com/2006/07/27/cyc/AuthenticationProgram-Remote> <http://www.w3.org/2000/01/rdf-schema#comment> """The collection of 
authentication applications for users and services on a network.""" ;
	a <http://sw.cyc.com/2006/07/27/cyc/KEClarifyingCollectionType> , <http://sw.cyc.com/2006/07/27/cyc/ComputerProgramTypeByFunction> ;
	<http://sw.cyc.com/2006/07/27/cyc/prettyString-Canonical> "remote authentication program" ;
	<http://sw.cyc.com/2006/07/27/cyc/prettyString> "remote authentication programme" , "remote authentication programs" , "remote authentication programz" ;
	<http://www.w3.org/2000/01/rdf-schema#subClassOf> <http://sw.cyc.com/2006/07/27/cyc/SecurityProgram> .

<http://sw.cyc.com/2006/07/27/cyc/AcesTheCompleteCollectorsEdition-TheGame> a <http://sw.cyc.com/2006/07/27/cyc/Individual> , <http://sw.cyc.com/2006/07/27/cyc/UnversionedProgram> , <http://sw.cyc.com/2006/07/27/cyc/SimulationGameProgram> ;
	<http://sw.cyc.com/2006/07/27/cyc/prettyString-Canonical> "Aces The Complete Collector's Edition" ;
	<http://sw.cyc.com/2006/07/27/cyc/prettyString> "Aces: The Complete Collector's Edition" .

<http://sw.cyc.com/2006/07/27/cyc/Acetabulum> a <http://sw.cyc.com/2006/07/27/cyc/SpatiallyDisjointObjectType> , <http://sw.cyc.com/2006/07/27/cyc/UniqueAnatomicalPartType> , <http://sw.cyc.com/2006/07/27/cyc/InternalAnimalBodyRegionType> , <http://sw.cyc.com/2006/07/27/cyc/SymmetricAnatomicalPartType> ;
	<http://sw.cyc.com/2006/07/27/cyc/prettyString-Canonical> "acetabulum" ;
	<http://sw.cyc.com/2006/07/27/cyc/prettyString> "acetabula" ;
	<http://www.w3.org/2000/01/rdf-schema#subClassOf> <http://sw.cyc.com/2006/07/27/cyc/CavityWithWalls> , <http://sw.cyc.com/2006/07/27/cyc/BoneSubPart> ;
	<http://sw.cyc.com/2006/07/27/cyc/sharedNotes> <http://sw.cyc.com/2006/07/27/cyc/BeforeMajorChangesToAnatomicalParts> .

<http://sw.cyc.com/2006/07/27/cyc/BoneSubPart> <http://www.w3.org/2000/01/rdf-schema#comment> "A #$BoneSubPart is a distinuishable part (or all) of a #$Bone-BodyPart." ;
	a <http://sw.cyc.com/2006/07/27/cyc/SpatiallyDisjointObjectType> , <http://sw.cyc.com/2006/07/27/cyc/AnimalBodyPartType> , <http://sw.cyc.com/2006/07/27/cyc/InternalAnimalBodyRegionType> ;
	<http://sw.cyc.com/2006/07/27/cyc/prettyString-Canonical> "bone part" ;
	<http://sw.cyc.com/2006/07/27/cyc/prettyString> "part of bone" , "parts of bone" .

<http://sw.cyc.com/2006/07/27/cyc/AceticAcid> <http://sw.cyc.com/2006/07/27/cyc/prettyString-Canonical> "acetic acid" ;
	<http://www.w3.org/2000/01/rdf-schema#subClassOf> <http://sw.cyc.com/2006/07/27/cyc/ChemicallyAcidicSubstance> , <http://sw.cyc.com/2006/07/27/cyc/WeakElectrolyte> .

<http://sw.cyc.com/2006/07/27/cyc/ChemicallyAcidicSubstance> <http://www.w3.org/2000/01/rdf-schema#comment> "The collection of all samples of stuff that can be classified as acidic." ;
	a <http://sw.cyc.com/2006/07/27/cyc/ExistingStuffType> ;
	<http://sw.cyc.com/2006/07/27/cyc/prettyString-Canonical> "chemically acidic substance" ;
	<http://sw.cyc.com/2006/07/27/cyc/prettyString> "acid" , "acidic substance" , "acidic substances" , "acidic stuff" , "chemically acidic stuff" , "chemically acidic substances" ;
	<http://www.w3.org/2000/01/rdf-schema#subClassOf> <http://sw.cyc.com/2006/07/27/cyc/RustCausingStuff> ;
	<http://www.w3.org/2002/07/owl#disjointWith> <http://sw.cyc.com/2006/07/27/cyc/MilitaryHardware> , <http://sw.cyc.com/2006/07/27/cyc/ChemicallyBasicSubstance> , <http://sw.cyc.com/2006/07/27/cyc/ChemicallyNeutralSubstance> .

<http://sw.cyc.com/2006/07/27/cyc/WeakElectrolyte> <http://www.w3.org/2000/01/rdf-schema#comment> "The collection of all polyatomic chemical stuffs that partially decompose into ions when disolved in water.  An instance of #$WeakElectrolyte may be a mixture of chemical compounds.  It need not be an instance of an instance of #$ChemicalCompoundTypeByChemicalSpecies." ;
	a <http://sw.cyc.com/2006/07/27/cyc/TangibleStuffCompositionType> ;
	<http://sw.cyc.com/2006/07/27/cyc/prettyString-Canonical> "weak electrolyte" ;
	<http://sw.cyc.com/2006/07/27/cyc/prettyString> "weak electrolytes" ;
	<http://www.w3.org/2000/01/rdf-schema#subClassOf> <http://sw.cyc.com/2006/07/27/cyc/Electrolyte> .

<http://sw.cyc.com/2006/07/27/cyc/AcidType-Monoprotic> <http://www.w3.org/2000/01/rdf-schema#comment> "The collection of monoprotic acids and a specialization of #$AcidType-Lewis.  The instances of this collection are all types of acids whose instances contain a single hydrogen atom per molecule that is susceptible to dissociation in aqueous solution." ;
	a <http://sw.cyc.com/2006/07/27/cyc/SecondOrderCollection> ;
	<http://sw.cyc.com/2006/07/27/cyc/prettyString-Canonical> "monoprotic acid" ;
	<http://sw.cyc.com/2006/07/27/cyc/prettyString> "monoprotic acids" ;
	<http://www.w3.org/2002/07/owl#disjointWith> <http://sw.cyc.com/2006/07/27/cyc/AcidType-Polyprotic> .

<http://sw.cyc.com/2006/07/27/cyc/AcidType-Weak> <http://www.w3.org/2000/01/rdf-schema#comment> """The collection of weak acid types and a specialization of #$ChemicalSubstanceType.
The instances of the instances of this collection only partly dissociate in water.""" ;
	a <http://sw.cyc.com/2006/07/27/cyc/SecondOrderCollection> ;
	<http://sw.cyc.com/2006/07/27/cyc/prettyString-Canonical> "weak acid" ;
	<http://sw.cyc.com/2006/07/27/cyc/prettyString> "weak acids" ;
	<http://www.w3.org/2000/01/rdf-schema#subClassOf> <http://sw.cyc.com/2006/07/27/cyc/AcidType-Lewis> ;
	<http://www.w3.org/2002/07/owl#disjointWith> <http://sw.cyc.com/2006/07/27/cyc/AcidType-Negligible> , <http://sw.cyc.com/2006/07/27/cyc/IonicCompoundType> ;
	<http://sw.cyc.com/2006/07/27/cyc/typeGenls> <http://sw.cyc.com/2006/07/27/cyc/WeakElectrolyte> .

<http://sw.cyc.com/2006/07/27/cyc/AcidType-Arrhenius> <http://www.w3.org/2000/01/rdf-schema#comment> """An instance of #$SecondOrderCollection and a specialization of
#$ChemicalSubstanceType.  Each instance of #$AcidType-Arrhenius is a type of
substance instances of which, when dissolved in water, increase the
concentration of #$HydroniumIons in those samples.""" ;
	a <http://sw.cyc.com/2006/07/27/cyc/SecondOrderCollection> ;
	<http://sw.cyc.com/2006/07/27/cyc/prettyString-Canonical> "Arrhenius acid" ;
	<http://sw.cyc.com/2006/07/27/cyc/prettyString> "Arrhenius acids" ;
	<http://www.w3.org/2000/01/rdf-schema#subClassOf> <http://sw.cyc.com/2006/07/27/cyc/AcidType-Bronsted-Lowry> ;
	<http://www.w3.org/2002/07/owl#disjointWith> <http://sw.cyc.com/2006/07/27/cyc/BaseType-Arrhenius> .

<http://sw.cyc.com/2006/07/27/cyc/IonicDecomposableCompoundType> <http://www.w3.org/2000/01/rdf-schema#comment> "A specialization of ChemicalCompoundTypeByChemicalSpecies.  Each instance of #$IonicDecomposableCompoundType is a type of compound whose instances decomposes under certain conditions in positively and negatively charged ions.  #$IonicDecomposableCompoundType is a generalization of #$IonicCompoundType (those compounds of ions that form in three-dimensional blocks) and of compounds formed from a hydrogen ion [#$HydrogenPlusIon] and an anion, including #$AcidType-Strong. Note that strong acids can exist in molecular form (e.g., as gases) even though they dissolve into ions in aqueous solution." ;
	a <http://sw.cyc.com/2006/07/27/cyc/SecondOrderCollection> ;
	<http://sw.cyc.com/2006/07/27/cyc/prettyString-Canonical> "compound decomposable into ions" ;
	<http://sw.cyc.com/2006/07/27/cyc/prettyString> "compounds decomposable into ions" ;
	<http://www.w3.org/2000/01/rdf-schema#subClassOf> <http://sw.cyc.com/2006/07/27/cyc/ChemicalCompoundTypeByChemicalSpecies> ;
	<http://sw.cyc.com/2006/07/27/cyc/typeGenls> <http://sw.cyc.com/2006/07/27/cyc/Electrolyte> ;
	<http://sw.cyc.com/2006/07/27/cyc/requiredArg1Pred> <http://sw.cyc.com/2006/07/27/cyc/anionTypeOfIonicCompoundType> , <http://sw.cyc.com/2006/07/27/cyc/cationTypeOfIonicCompoundType> , <http://sw.cyc.com/2006/07/27/cyc/ionicDecomposition> .

<http://sw.cyc.com/2006/07/27/cyc/AceticAnhydride> <http://www.w3.org/2000/01/rdf-schema#comment> "#$AceticAnhydride is an instance of #$ChemicalCompoundTypeByChemicalSpecies.   It is a clear, colorless liquid with a very pungent, penetrating, vinegar-like odor that combines with water to form acetic acid (see #$AceticAcid). Acetic anhydride is used in the manufacture of cellulose acetate having the application as a base for magnetic tape and in the manufacture of textile fibers. Also, it is heated with salicylic acid to produce acetylsalicylic acid (aspirin). It is also used in the manufacture of pigments, dyes, cellulose and pesticides etc." ;
	a <http://sw.cyc.com/2006/07/27/cyc/ChemicalCompoundTypeByChemicalSpecies> ;
	<http://sw.cyc.com/2006/07/27/cyc/prettyString-Canonical> "acetic anhydride" ;
	<http://sw.cyc.com/2006/07/27/cyc/prettyString> "acetic oxide" , "acetyl acetate" , "acetyl ether" , "acetic acid anhydride" , "ethanoic anhydride" , "acetyl oxide" ;
	<http://www.w3.org/2000/01/rdf-schema#subClassOf> <http://sw.cyc.com/2006/07/27/cyc/PartiallyTangible> .

<http://sw.cyc.com/2006/07/27/cyc/AcetoCorporation> a <http://sw.cyc.com/2006/07/27/cyc/Individual> , <http://sw.cyc.com/2006/07/27/cyc/PubliclyHeldCorporation> ;
	<http://sw.cyc.com/2006/07/27/cyc/prettyString-Canonical> "Aceto Corp" .

<http://sw.cyc.com/2006/07/27/cyc/Acetone> <http://www.w3.org/2000/01/rdf-schema#comment> "C3H6O. #$Acetone is a ketone.  It is also known as 'propanone' and it is a common household solvent." .

<http://sw.cyc.com/2006/07/27/cyc/AcetylcholinePoisoning> <http://sw.cyc.com/2006/07/27/cyc/prettyString-Canonical> "acetylcholine poisoning" ;
	<http://www.w3.org/2000/01/rdf-schema#subClassOf> <http://sw.cyc.com/2006/07/27/cyc/Poisoning> .

<http://sw.cyc.com/2006/07/27/cyc/Poisoning> <http://www.w3.org/2000/01/rdf-schema#comment> "A specialization of #$AilmentCondition (q.v.).  This is the collection of _conditions_ resulting from the intake of a substance by an organism (where the kind and quantity of the substance is toxic to the organism in question).  Note that none of the instances of this collection include the actual intake of the substance.  For a collection with instances that do include these, see #$Poisoning-Script." ;
	a <http://sw.cyc.com/2006/07/27/cyc/KEClarifyingCollectionType> , <http://sw.cyc.com/2006/07/27/cyc/PhysiologicalConditionType> ;
	<http://sw.cyc.com/2006/07/27/cyc/prettyString-Canonical> "poisoning" ;
	<http://sw.cyc.com/2006/07/27/cyc/prettyString> "poisons" , "poisoned" , "have poisoned" , "has poisoned" , "will poison" , "had poisoned" , "will have poisoned" , "Poison" ;
	<http://www.w3.org/2000/01/rdf-schema#subClassOf> <http://sw.cyc.com/2006/07/27/cyc/AilmentCondition> , <http://sw.cyc.com/2006/07/27/cyc/LifeThreateningCondition> ;
	<http://sw.cyc.com/2006/07/27/cyc/facets-Covering> <http://sw.cyc.com/2006/07/27/cyc/PoisoningTypeByAgentType> ;
	<http://sw.cyc.com/2006/07/27/cyc/facets-Generic> <http://sw.cyc.com/2006/07/27/cyc/PoisoningTypeByAgentType> ;
	<http://sw.cyc.com/2006/07/27/cyc/requiredArg1Pred> <http://sw.cyc.com/2006/07/27/cyc/poisonedWithSubstanceType> ;
	<http://sw.cyc.com/2006/07/27/cyc/covering> <http://sw.cyc.com/2006/07/27/cyc/PoisoningTypeByAgentType> .

<http://sw.cyc.com/2006/07/27/cyc/PoisoningTypeByAgentType> <http://www.w3.org/2000/01/rdf-schema#comment> "A #$CollectionType (collection of collections) and a covering on #$Poisoning.  Each instance is a collection of poisonings whose instances have the common feature of a particular type of substance being involved, e.g. poisoning by cyanide." ;
	a <http://sw.cyc.com/2006/07/27/cyc/FacetingCollectionType> , <http://sw.cyc.com/2006/07/27/cyc/SecondOrderCollection> ;
	<http://sw.cyc.com/2006/07/27/cyc/prettyString-Canonical> "type of poisoning" ;
	<http://sw.cyc.com/2006/07/27/cyc/prettyString> "types of poisoning" ;
	<http://www.w3.org/2000/01/rdf-schema#subClassOf> <http://sw.cyc.com/2006/07/27/cyc/FacetInstanceCollection> , <http://sw.cyc.com/2006/07/27/cyc/PhysiologicalConditionType> ;
	<http://sw.cyc.com/2006/07/27/cyc/sharedNotes> <http://sw.cyc.com/2006/07/27/cyc/SharedNoteOnGenlsRelationsBetweenFacetingCollectionTypes> ;
	<http://sw.cyc.com/2006/07/27/cyc/typeGenls> <http://sw.cyc.com/2006/07/27/cyc/Poisoning> .

<http://sw.cyc.com/2006/07/27/cyc/Acetylcholinesterase> <http://www.w3.org/2000/01/rdf-schema#comment> "A kind of #$ChemicalSubstanceType, which serves to break down #$Acetylcholine, thereby preventing continuous, uncontrolled stimulation of muscarinic and nicotinic receptors." ;
	a <http://sw.cyc.com/2006/07/27/cyc/ChemicalCompoundTypeByChemicalSpecies> ;
	<http://sw.cyc.com/2006/07/27/cyc/prettyString-Canonical> "acetylcholinesterase" ;
	<http://sw.cyc.com/2006/07/27/cyc/prettyString> "cholinesterase" ;
	<http://www.w3.org/2000/01/rdf-schema#subClassOf> <http://sw.cyc.com/2006/07/27/cyc/PartiallyTangible> .

<http://sw.cyc.com/2006/07/27/cyc/Acetylene> <http://www.w3.org/2000/01/rdf-schema#comment> "The chemical with formula C2H2. It is a precursor for #$Lewisite." ;
	a <http://sw.cyc.com/2006/07/27/cyc/ChemicalCompoundTypeByChemicalSpecies> ;
	<http://sw.cyc.com/2006/07/27/cyc/prettyString-Canonical> "acetylene" ;
	<http://sw.cyc.com/2006/07/27/cyc/prettyString> "ethenylene" ;
	<http://www.w3.org/2000/01/rdf-schema#subClassOf> <http://sw.cyc.com/2006/07/27/cyc/PartiallyTangible> .

<http://sw.cyc.com/2006/07/27/cyc/AcetylsalicylicAcid> a <http://sw.cyc.com/2006/07/27/cyc/ChemicalCompoundTypeByChemicalSpecies> , <http://sw.cyc.com/2006/07/27/cyc/PharmaceuticalType> ;
	<http://sw.cyc.com/2006/07/27/cyc/prettyString-Canonical> "aspirin" ;
	<http://sw.cyc.com/2006/07/27/cyc/prettyString> "acetylsalicylic acid" ;
	<http://www.w3.org/2000/01/rdf-schema#subClassOf> <http://sw.cyc.com/2006/07/27/cyc/ChemicallyAcidicSubstance> , <http://sw.cyc.com/2006/07/27/cyc/Analgesic> .

<http://sw.cyc.com/2006/07/27/cyc/Analgesic> <http://www.w3.org/2000/01/rdf-schema#comment> "Drugs which are used to reduce or relieve pain." ;
	a <http://sw.cyc.com/2006/07/27/cyc/TherapeuticClassType> ;
	<http://sw.cyc.com/2006/07/27/cyc/prettyString-Canonical> "pain pill" ;
	<http://sw.cyc.com/2006/07/27/cyc/prettyString> "analgesic" , "analgesics" , "painkiller" , "painkillers" , "pain killer" , "pain killers" , "pain pills" ;
	<http://www.w3.org/2000/01/rdf-schema#subClassOf> <http://sw.cyc.com/2006/07/27/cyc/ManufacturedGoods> , <http://sw.cyc.com/2006/07/27/cyc/DrugProduct> .

<http://sw.cyc.com/2006/07/27/cyc/AceVenturaPetDetective-TheMovie> a <http://sw.cyc.com/2006/07/27/cyc/Individual> , <http://sw.cyc.com/2006/07/27/cyc/ComedyMovie> ;
	<http://sw.cyc.com/2006/07/27/cyc/prettyString-Canonical> "Ace Ventura Pet Detective" .

<http://sw.cyc.com/2006/07/27/cyc/AceVentura-TheGame> a <http://sw.cyc.com/2006/07/27/cyc/Individual> , <http://sw.cyc.com/2006/07/27/cyc/UnversionedProgram> , <http://sw.cyc.com/2006/07/27/cyc/ActionGameProgram> ;
	<http://sw.cyc.com/2006/07/27/cyc/prettyString-Canonical> "Ace Ventura" .

<http://sw.cyc.com/2006/07/27/cyc/AceVenturaWhenNatureCalls-TheMovie> a <http://sw.cyc.com/2006/07/27/cyc/Individual> , <http://sw.cyc.com/2006/07/27/cyc/ComedyMovie> ;
	<http://sw.cyc.com/2006/07/27/cyc/prettyString-Canonical> "Ace Ventura When Nature Calls" ;
	<http://sw.cyc.com/2006/07/27/cyc/prettyString> "Ace Ventura: When Nature Calls" .

<http://sw.cyc.com/2006/07/27/cyc/A_Change-ThePrefix> <http://www.w3.org/2000/01/rdf-schema#comment> "The prefix \"a\" means something like *in the act of*. It combines (generally) with #$Verbs and results (generally) in #$PredicativeOnlyAdjectives. Example: (#$derivedUsingPrefix #$Aglow-TheWord #$A_Change-ThePrefix)." ;
	a <http://sw.cyc.com/2006/07/27/cyc/Individual> , <http://sw.cyc.com/2006/07/27/cyc/AdjectiveProducingAffix> , <http://sw.cyc.com/2006/07/27/cyc/UnproductiveLexicalAffix> , <http://sw.cyc.com/2006/07/27/cyc/CategoryChangingPrefix> , <http://sw.cyc.com/2006/07/27/cyc/EnglishDerivationalPrefix> , <http://sw.cyc.com/2006/07/27/cyc/DeverbalAffix> , <http://sw.cyc.com/2006/07/27/cyc/LexicalPrefix> ;
	<http://sw.cyc.com/2006/07/27/cyc/prettyString-Canonical> "a prefix" ;
	<http://sw.cyc.com/2006/07/27/cyc/prettyString> "a prefixes" ;
	<http://sw.cyc.com/2006/07/27/cyc/quotedIsa> <http://sw.cyc.com/2006/07/27/cyc/NLMorphologyTerm> .

<http://sw.cyc.com/2006/07/27/cyc/AdjectiveProducingAffix> <http://www.w3.org/2000/01/rdf-schema#comment> "The collection of affixes which serve to convert words into #$Adjectives. Example: #$Delight-TheWord + #$Ful_AdjectiveProducing-TheSuffix = #$Delightful-TheWord." ;
	a <http://sw.cyc.com/2006/07/27/cyc/NLMorphologyCollection> .

<http://sw.cyc.com/2006/07/27/cyc/absolute-PreconditionFor-PropSit> <http://www.w3.org/2000/01/rdf-schema#comment> "A specialization of the predicate #$preconditionFor-PropSit needed for the external problem solver." .

<http://sw.cyc.com/2006/07/27/cyc/AbsoluteValueFn> <http://sw.cyc.com/2006/07/27/cyc/oldConstantName> "AbsoluteValue" .

<http://sw.cyc.com/2006/07/27/cyc/NonNegativeScalarInterval> <http://sw.cyc.com/2006/07/27/cyc/prettyString> "quantities or number greater than or equal to zero" .

<http://sw.cyc.com/2006/07/27/cyc/DispositionalQuantity> a <http://sw.cyc.com/2006/07/27/cyc/UnitOfMeasureConcept> .

<http://sw.cyc.com/2006/07/27/cyc/AbsorptionEvent> <http://www.w3.org/2000/01/rdf-schema#comment> "The event in which objects are taken into some structure across some membrane." .

<http://sw.cyc.com/2006/07/27/cyc/FluidFlow-Translation> a <http://sw.cyc.com/2006/07/27/cyc/KeyMovementCollectionsFromTheSecondaryLevel-Movement-Topic> .

<http://sw.cyc.com/2006/07/27/cyc/TransferIn> <http://sw.cyc.com/2006/07/27/cyc/prettyString> "get intos" .

<http://sw.cyc.com/2006/07/27/cyc/ABSResin> <http://www.w3.org/2000/01/rdf-schema#comment> "A specialization of #$Thermoplastic.  Each instance of #$ABSResin is piece of material made of some ratio of #$Acrylonitrile, #$Butadiene and #$Styrene.  This compound is typically used for plastic parts of consumer goods: telephones, bottles, luggage, shower stalls, etc." .

<http://sw.cyc.com/2006/07/27/cyc/Voting> a <http://sw.cyc.com/2006/07/27/cyc/TypicalHumanActivityType-AtLeastOnce> .

<http://sw.cyc.com/2006/07/27/cyc/Abstinence> <http://www.w3.org/2000/01/rdf-schema#subClassOf> <http://sw.cyc.com/2006/07/27/cyc/Inaction> .

<http://sw.cyc.com/2006/07/27/cyc/AbstractStructure> <http://sw.cyc.com/2006/07/27/cyc/prettyString-Canonical> "abstract structure" .

<http://sw.cyc.com/2006/07/27/cyc/NLMorphologyCollection> a <http://sw.cyc.com/2006/07/27/cyc/CollectionType> .

<http://sw.cyc.com/2006/07/27/cyc/containsStructure-CW> <http://sw.cyc.com/2006/07/27/cyc/arity> "2"^^<http://www.w3.org/2001/XMLSchema#long> .

